<?xml version="1.0"?>
<rdf:RDF xmlns="http://nlpkg.sebis.cit.tum.de/nlp-fos-hierarchy.owl#"
     xml:base="http://nlpkg.sebis.cit.tum.de/nlp-fos-hierarchy.owl"
     xmlns:owl="http://www.w3.org/2002/07/owl#"
     xmlns:rdf="http://www.w3.org/1999/02/22-rdf-syntax-ns#"
     xmlns:xml="http://www.w3.org/XML/1998/namespace"
     xmlns:xsd="http://www.w3.org/2001/XMLSchema#"
     xmlns:rdfs="http://www.w3.org/2000/01/rdf-schema#"
     xmlns:dcterms="http://purl.org/dc/terms/"
     xmlns:oboInOwl="http://www.geneontology.org/formats/oboInOwl#"
     xmlns:nlp-taxonomy="http://nlpkg.sebis.cit.tum.de/nlp-taxonomy.owl#"
     xmlns:nlp-fos-hierarchy="http://nlpkg.sebis.cit.tum.de/nlp-fos-hierarchy.owl#">
    <owl:Ontology rdf:about="http://nlpkg.sebis.cit.tum.de/nlp-fos-hierarchy.owl">
        <owl:versionIRI rdf:resource="http://nlpkg.sebis.cit.tum.de/nlp-fos-hierarchy.owl/1.0.0"/>
        <dcterms:creator rdf:datatype="http://www.w3.org/2001/XMLSchema#string">Tim Schopf</dcterms:creator>
        <dcterms:description rdf:datatype="http://www.w3.org/2001/XMLSchema#string">A hierarchy of fields of study in Natural Language Processing (NLP).

This is the machine readable version of the NLP fields of study hierarchy developed in the paper &quot;NLP-KG: A System for Exploratory Search of Scientific Literature in Natural Language Processing (Schopf &amp; Matthes, ACL 2024)&quot;, which is available at https://aclanthology.org/2024.acl-demos.13. 

It is an extension of the NLP Taxonomy deveoped in the paper &quot;Exploring the Landscape of Natural Language Processing Research (Schopf et al., RANLP 2023)&quot;, which is available at https://aclanthology.org/2023.ranlp-1.111.</dcterms:description>
        <dcterms:title rdf:datatype="http://www.w3.org/2001/XMLSchema#string">NLP Fields of Study Hierarchy</dcterms:title>
    </owl:Ontology>
    


    <!-- 
    ///////////////////////////////////////////////////////////////////////////////////////
    //
    // Annotation properties
    //
    ///////////////////////////////////////////////////////////////////////////////////////
     -->

    


    <!-- http://purl.org/dc/terms/creator -->

    <owl:AnnotationProperty rdf:about="http://purl.org/dc/terms/creator"/>
    


    <!-- http://purl.org/dc/terms/description -->

    <owl:AnnotationProperty rdf:about="http://purl.org/dc/terms/description"/>
    


    <!-- http://purl.org/dc/terms/title -->

    <owl:AnnotationProperty rdf:about="http://purl.org/dc/terms/title"/>
    


    <!-- http://www.geneontology.org/formats/oboInOwl#hasSynonym -->

    <owl:AnnotationProperty rdf:about="http://www.geneontology.org/formats/oboInOwl#hasSynonym"/>
    


    <!-- 
    ///////////////////////////////////////////////////////////////////////////////////////
    //
    // Object Properties
    //
    ///////////////////////////////////////////////////////////////////////////////////////
     -->

    


    <!-- http://nlpkg.sebis.cit.tum.de/nlp-fos-hierarchy.owl#evaluatedBy -->

    <owl:ObjectProperty rdf:about="http://nlpkg.sebis.cit.tum.de/nlp-fos-hierarchy.owl#evaluatedBy">
        <owl:inverseOf rdf:resource="http://nlpkg.sebis.cit.tum.de/nlp-fos-hierarchy.owl#evaluates"/>
        <rdfs:domain rdf:resource="http://nlpkg.sebis.cit.tum.de/nlp-taxonomy.owl#FieldOfStudy"/>
        <rdfs:range rdf:resource="http://nlpkg.sebis.cit.tum.de/nlp-taxonomy.owl#FieldOfStudy"/>
        <rdfs:comment xml:lang="en">A specific task or method can be evaluated by a metric or dataset.</rdfs:comment>
    </owl:ObjectProperty>
    


    <!-- http://nlpkg.sebis.cit.tum.de/nlp-fos-hierarchy.owl#evaluates -->

    <owl:ObjectProperty rdf:about="http://nlpkg.sebis.cit.tum.de/nlp-fos-hierarchy.owl#evaluates">
        <rdfs:domain rdf:resource="http://nlpkg.sebis.cit.tum.de/nlp-taxonomy.owl#FieldOfStudy"/>
        <rdfs:range rdf:resource="http://nlpkg.sebis.cit.tum.de/nlp-taxonomy.owl#FieldOfStudy"/>
        <rdfs:comment xml:lang="en">A metric or dataset that can be used to evaluate a specific task or method.</rdfs:comment>
    </owl:ObjectProperty>
    


    <!-- http://nlpkg.sebis.cit.tum.de/nlp-fos-hierarchy.owl#has_author -->

    <owl:ObjectProperty rdf:about="http://nlpkg.sebis.cit.tum.de/nlp-fos-hierarchy.owl#has_author">
        <owl:inverseOf rdf:resource="http://nlpkg.sebis.cit.tum.de/nlp-fos-hierarchy.owl#is_author_of"/>
        <rdfs:domain rdf:resource="http://nlpkg.sebis.cit.tum.de/nlp-fos-hierarchy.owl#Publication"/>
        <rdfs:range rdf:resource="http://nlpkg.sebis.cit.tum.de/nlp-fos-hierarchy.owl#Researcher"/>
    </owl:ObjectProperty>
    


    <!-- http://nlpkg.sebis.cit.tum.de/nlp-fos-hierarchy.owl#has_field_of_study -->

    <owl:ObjectProperty rdf:about="http://nlpkg.sebis.cit.tum.de/nlp-fos-hierarchy.owl#has_field_of_study">
        <owl:inverseOf rdf:resource="http://nlpkg.sebis.cit.tum.de/nlp-fos-hierarchy.owl#is_studied_in"/>
        <rdfs:domain rdf:resource="http://nlpkg.sebis.cit.tum.de/nlp-fos-hierarchy.owl#Publication"/>
        <rdfs:range rdf:resource="http://nlpkg.sebis.cit.tum.de/nlp-taxonomy.owl#FieldOfStudy"/>
    </owl:ObjectProperty>
    


    <!-- http://nlpkg.sebis.cit.tum.de/nlp-fos-hierarchy.owl#is_author_of -->

    <owl:ObjectProperty rdf:about="http://nlpkg.sebis.cit.tum.de/nlp-fos-hierarchy.owl#is_author_of">
        <rdfs:domain rdf:resource="http://nlpkg.sebis.cit.tum.de/nlp-fos-hierarchy.owl#Researcher"/>
        <rdfs:range rdf:resource="http://nlpkg.sebis.cit.tum.de/nlp-fos-hierarchy.owl#Publication"/>
    </owl:ObjectProperty>
    


    <!-- http://nlpkg.sebis.cit.tum.de/nlp-fos-hierarchy.owl#is_referenced_by -->

    <owl:ObjectProperty rdf:about="http://nlpkg.sebis.cit.tum.de/nlp-fos-hierarchy.owl#is_referenced_by">
        <owl:inverseOf rdf:resource="http://nlpkg.sebis.cit.tum.de/nlp-fos-hierarchy.owl#references"/>
        <rdfs:domain rdf:resource="http://nlpkg.sebis.cit.tum.de/nlp-fos-hierarchy.owl#Publication"/>
        <rdfs:range rdf:resource="http://nlpkg.sebis.cit.tum.de/nlp-fos-hierarchy.owl#Publication"/>
        <rdfs:comment xml:lang="en">Relates a publication to another publication that references the
first publication.</rdfs:comment>
        <rdfs:label xml:lang="en">is_referenced_by</rdfs:label>
    </owl:ObjectProperty>
    


    <!-- http://nlpkg.sebis.cit.tum.de/nlp-fos-hierarchy.owl#is_studied_by -->

    <owl:ObjectProperty rdf:about="http://nlpkg.sebis.cit.tum.de/nlp-fos-hierarchy.owl#is_studied_by">
        <owl:inverseOf rdf:resource="http://nlpkg.sebis.cit.tum.de/nlp-fos-hierarchy.owl#studies"/>
        <rdfs:domain rdf:resource="http://nlpkg.sebis.cit.tum.de/nlp-taxonomy.owl#FieldOfStudy"/>
        <rdfs:range rdf:resource="http://nlpkg.sebis.cit.tum.de/nlp-fos-hierarchy.owl#Researcher"/>
    </owl:ObjectProperty>
    


    <!-- http://nlpkg.sebis.cit.tum.de/nlp-fos-hierarchy.owl#is_studied_in -->

    <owl:ObjectProperty rdf:about="http://nlpkg.sebis.cit.tum.de/nlp-fos-hierarchy.owl#is_studied_in">
        <rdfs:domain rdf:resource="http://nlpkg.sebis.cit.tum.de/nlp-taxonomy.owl#FieldOfStudy"/>
        <rdfs:range rdf:resource="http://nlpkg.sebis.cit.tum.de/nlp-fos-hierarchy.owl#Publication"/>
    </owl:ObjectProperty>
    


    <!-- http://nlpkg.sebis.cit.tum.de/nlp-fos-hierarchy.owl#preferentialEquivalent -->

    <owl:ObjectProperty rdf:about="http://nlpkg.sebis.cit.tum.de/nlp-fos-hierarchy.owl#preferentialEquivalent">
        <rdf:type rdf:resource="http://www.w3.org/2002/07/owl#FunctionalProperty"/>
        <rdfs:domain rdf:resource="http://nlpkg.sebis.cit.tum.de/nlp-taxonomy.owl#FieldOfStudy"/>
        <rdfs:range rdf:resource="http://nlpkg.sebis.cit.tum.de/nlp-taxonomy.owl#FieldOfStudy"/>
    </owl:ObjectProperty>
    


    <!-- http://nlpkg.sebis.cit.tum.de/nlp-fos-hierarchy.owl#references -->

    <owl:ObjectProperty rdf:about="http://nlpkg.sebis.cit.tum.de/nlp-fos-hierarchy.owl#references">
        <rdfs:domain rdf:resource="http://nlpkg.sebis.cit.tum.de/nlp-fos-hierarchy.owl#Publication"/>
        <rdfs:range rdf:resource="http://nlpkg.sebis.cit.tum.de/nlp-fos-hierarchy.owl#Publication"/>
        <rdfs:comment xml:lang="en">Relates a publication to another publication that references the
first publication.</rdfs:comment>
        <rdfs:label xml:lang="de">references</rdfs:label>
    </owl:ObjectProperty>
    


    <!-- http://nlpkg.sebis.cit.tum.de/nlp-fos-hierarchy.owl#similar_to -->

    <owl:ObjectProperty rdf:about="http://nlpkg.sebis.cit.tum.de/nlp-fos-hierarchy.owl#similar_to">
        <owl:inverseOf rdf:resource="http://nlpkg.sebis.cit.tum.de/nlp-fos-hierarchy.owl#similar_to"/>
        <rdfs:domain rdf:resource="http://nlpkg.sebis.cit.tum.de/nlp-fos-hierarchy.owl#Publication"/>
        <rdfs:domain rdf:resource="http://nlpkg.sebis.cit.tum.de/nlp-taxonomy.owl#FieldOfStudy"/>
        <rdfs:range rdf:resource="http://nlpkg.sebis.cit.tum.de/nlp-fos-hierarchy.owl#Publication"/>
        <rdfs:range rdf:resource="http://nlpkg.sebis.cit.tum.de/nlp-taxonomy.owl#FieldOfStudy"/>
        <rdfs:comment xml:lang="en">The semantic similarity of different FoS and publications to each other.</rdfs:comment>
    </owl:ObjectProperty>
    


    <!-- http://nlpkg.sebis.cit.tum.de/nlp-fos-hierarchy.owl#studies -->

    <owl:ObjectProperty rdf:about="http://nlpkg.sebis.cit.tum.de/nlp-fos-hierarchy.owl#studies">
        <rdfs:domain rdf:resource="http://nlpkg.sebis.cit.tum.de/nlp-fos-hierarchy.owl#Researcher"/>
        <rdfs:range rdf:resource="http://nlpkg.sebis.cit.tum.de/nlp-taxonomy.owl#FieldOfStudy"/>
        <owl:propertyChainAxiom rdf:parseType="Collection">
            <rdf:Description rdf:about="http://nlpkg.sebis.cit.tum.de/nlp-fos-hierarchy.owl#is_author_of"/>
            <rdf:Description rdf:about="http://nlpkg.sebis.cit.tum.de/nlp-fos-hierarchy.owl#has_field_of_study"/>
        </owl:propertyChainAxiom>
    </owl:ObjectProperty>
    


    <!-- http://nlpkg.sebis.cit.tum.de/nlp-fos-hierarchy.owl#usedFor -->

    <owl:ObjectProperty rdf:about="http://nlpkg.sebis.cit.tum.de/nlp-fos-hierarchy.owl#usedFor">
        <owl:inverseOf rdf:resource="http://nlpkg.sebis.cit.tum.de/nlp-fos-hierarchy.owl#uses"/>
        <rdfs:domain rdf:resource="http://nlpkg.sebis.cit.tum.de/nlp-taxonomy.owl#FieldOfStudy"/>
        <rdfs:range rdf:resource="http://nlpkg.sebis.cit.tum.de/nlp-taxonomy.owl#FieldOfStudy"/>
    </owl:ObjectProperty>
    


    <!-- http://nlpkg.sebis.cit.tum.de/nlp-fos-hierarchy.owl#uses -->

    <owl:ObjectProperty rdf:about="http://nlpkg.sebis.cit.tum.de/nlp-fos-hierarchy.owl#uses">
        <rdfs:domain rdf:resource="http://nlpkg.sebis.cit.tum.de/nlp-taxonomy.owl#FieldOfStudy"/>
        <rdfs:range rdf:resource="http://nlpkg.sebis.cit.tum.de/nlp-taxonomy.owl#FieldOfStudy"/>
    </owl:ObjectProperty>
    


    <!-- http://nlpkg.sebis.cit.tum.de/nlp-taxonomy.owl#subFieldOf -->

    <owl:ObjectProperty rdf:about="http://nlpkg.sebis.cit.tum.de/nlp-taxonomy.owl#subFieldOf">
        <owl:inverseOf rdf:resource="http://nlpkg.sebis.cit.tum.de/nlp-taxonomy.owl#superFieldOf"/>
        <rdfs:domain rdf:resource="http://nlpkg.sebis.cit.tum.de/nlp-taxonomy.owl#FieldOfStudy"/>
        <rdfs:range rdf:resource="http://nlpkg.sebis.cit.tum.de/nlp-taxonomy.owl#FieldOfStudy"/>
        <rdfs:comment xml:lang="en">The direct descendant of a Field of Study concept.</rdfs:comment>
    </owl:ObjectProperty>
    


    <!-- http://nlpkg.sebis.cit.tum.de/nlp-taxonomy.owl#superFieldOf -->

    <owl:ObjectProperty rdf:about="http://nlpkg.sebis.cit.tum.de/nlp-taxonomy.owl#superFieldOf">
        <rdfs:domain rdf:resource="http://nlpkg.sebis.cit.tum.de/nlp-taxonomy.owl#FieldOfStudy"/>
        <rdfs:range rdf:resource="http://nlpkg.sebis.cit.tum.de/nlp-taxonomy.owl#FieldOfStudy"/>
        <rdfs:comment xml:lang="en">The direct ancestor of a Field of Study concept.</rdfs:comment>
    </owl:ObjectProperty>
    


    <!-- 
    ///////////////////////////////////////////////////////////////////////////////////////
    //
    // Data properties
    //
    ///////////////////////////////////////////////////////////////////////////////////////
     -->

    


    <!-- http://nlpkg.sebis.cit.tum.de/nlp-fos-hierarchy.owl#aclBibkey -->

    <owl:DatatypeProperty rdf:about="http://nlpkg.sebis.cit.tum.de/nlp-fos-hierarchy.owl#aclBibkey">
        <rdfs:domain rdf:resource="http://nlpkg.sebis.cit.tum.de/nlp-fos-hierarchy.owl#Publication"/>
        <rdfs:range rdf:resource="http://www.w3.org/2001/XMLSchema#string"/>
        <rdfs:comment xml:lang="en">The bibtex key of a publication in the ACL Anthology.</rdfs:comment>
    </owl:DatatypeProperty>
    


    <!-- http://nlpkg.sebis.cit.tum.de/nlp-fos-hierarchy.owl#aclId -->

    <owl:DatatypeProperty rdf:about="http://nlpkg.sebis.cit.tum.de/nlp-fos-hierarchy.owl#aclId">
        <rdfs:domain rdf:resource="http://nlpkg.sebis.cit.tum.de/nlp-fos-hierarchy.owl#Publication"/>
        <rdfs:domain rdf:resource="http://nlpkg.sebis.cit.tum.de/nlp-fos-hierarchy.owl#Researcher"/>
        <rdfs:range rdf:resource="http://www.w3.org/2001/XMLSchema#string"/>
        <rdfs:comment xml:lang="en">The ID of a publication in the ACL Anthology.</rdfs:comment>
    </owl:DatatypeProperty>
    


    <!-- http://nlpkg.sebis.cit.tum.de/nlp-fos-hierarchy.owl#aclUrl -->

    <owl:DatatypeProperty rdf:about="http://nlpkg.sebis.cit.tum.de/nlp-fos-hierarchy.owl#aclUrl">
        <rdfs:domain rdf:resource="http://nlpkg.sebis.cit.tum.de/nlp-fos-hierarchy.owl#Publication"/>
        <rdfs:range rdf:resource="http://www.w3.org/2001/XMLSchema#string"/>
        <rdfs:comment xml:lang="en">The ACL Anthology URL of a publication.</rdfs:comment>
    </owl:DatatypeProperty>
    


    <!-- http://nlpkg.sebis.cit.tum.de/nlp-fos-hierarchy.owl#affiliations -->

    <owl:DatatypeProperty rdf:about="http://nlpkg.sebis.cit.tum.de/nlp-fos-hierarchy.owl#affiliations">
        <rdfs:domain rdf:resource="http://nlpkg.sebis.cit.tum.de/nlp-fos-hierarchy.owl#Researcher"/>
        <rdfs:range rdf:resource="http://www.w3.org/2001/XMLSchema#string"/>
        <rdfs:comment xml:lang="en">Author&apos;s affiliations - sourced from claimed authors who have set affiliation on their S2 author page.</rdfs:comment>
    </owl:DatatypeProperty>
    


    <!-- http://nlpkg.sebis.cit.tum.de/nlp-fos-hierarchy.owl#arxivId -->

    <owl:DatatypeProperty rdf:about="http://nlpkg.sebis.cit.tum.de/nlp-fos-hierarchy.owl#arxivId">
        <rdfs:domain rdf:resource="http://nlpkg.sebis.cit.tum.de/nlp-fos-hierarchy.owl#Publication"/>
        <rdfs:domain rdf:resource="http://nlpkg.sebis.cit.tum.de/nlp-fos-hierarchy.owl#Researcher"/>
        <rdfs:range rdf:resource="http://www.w3.org/2001/XMLSchema#string"/>
        <rdfs:comment xml:lang="en">The ID of a publication in arXiv.</rdfs:comment>
    </owl:DatatypeProperty>
    


    <!-- http://nlpkg.sebis.cit.tum.de/nlp-fos-hierarchy.owl#arxivUrl -->

    <owl:DatatypeProperty rdf:about="http://nlpkg.sebis.cit.tum.de/nlp-fos-hierarchy.owl#arxivUrl">
        <rdfs:domain rdf:resource="http://nlpkg.sebis.cit.tum.de/nlp-fos-hierarchy.owl#Publication"/>
        <rdfs:range rdf:resource="http://www.w3.org/2001/XMLSchema#string"/>
        <rdfs:comment xml:lang="en">The arXiv URL of a publication.</rdfs:comment>
    </owl:DatatypeProperty>
    


    <!-- http://nlpkg.sebis.cit.tum.de/nlp-fos-hierarchy.owl#author -->

    <owl:DatatypeProperty rdf:about="http://nlpkg.sebis.cit.tum.de/nlp-fos-hierarchy.owl#author">
        <rdfs:domain rdf:resource="http://nlpkg.sebis.cit.tum.de/nlp-fos-hierarchy.owl#Publication"/>
        <rdfs:range rdf:resource="http://www.w3.org/2001/XMLSchema#string"/>
        <rdfs:comment xml:lang="en">The author of a publication. This data property can be used to store additional authors that do not exist as individuals.</rdfs:comment>
    </owl:DatatypeProperty>
    


    <!-- http://nlpkg.sebis.cit.tum.de/nlp-fos-hierarchy.owl#authorList -->

    <owl:DatatypeProperty rdf:about="http://nlpkg.sebis.cit.tum.de/nlp-fos-hierarchy.owl#authorList">
        <rdfs:domain rdf:resource="http://nlpkg.sebis.cit.tum.de/nlp-fos-hierarchy.owl#Publication"/>
        <rdfs:range rdf:resource="http://www.w3.org/2001/XMLSchema#string"/>
        <rdfs:comment xml:lang="en">Ordered list of authors of a publication. Data type is a string and elements are separated by the &quot;;&quot; delimeter. This data property can be used to store the order of authors as well as additional authors that do not exist as individuals.</rdfs:comment>
    </owl:DatatypeProperty>
    


    <!-- http://nlpkg.sebis.cit.tum.de/nlp-fos-hierarchy.owl#code -->

    <owl:DatatypeProperty rdf:about="http://nlpkg.sebis.cit.tum.de/nlp-fos-hierarchy.owl#code">
        <rdfs:domain rdf:resource="http://nlpkg.sebis.cit.tum.de/nlp-taxonomy.owl#FieldOfStudy"/>
        <rdfs:range rdf:resource="http://www.w3.org/2001/XMLSchema#string"/>
        <rdfs:comment xml:lang="en">A link to relevant code implementation for a Field of Study.</rdfs:comment>
    </owl:DatatypeProperty>
    


    <!-- http://nlpkg.sebis.cit.tum.de/nlp-fos-hierarchy.owl#displayName -->

    <owl:DatatypeProperty rdf:about="http://nlpkg.sebis.cit.tum.de/nlp-fos-hierarchy.owl#displayName">
        <rdfs:domain rdf:resource="http://nlpkg.sebis.cit.tum.de/nlp-taxonomy.owl#FieldOfStudy"/>
        <rdfs:range rdf:resource="http://www.w3.org/2001/XMLSchema#string"/>
        <rdfs:comment xml:lang="en">The English-language label of the concept.</rdfs:comment>
    </owl:DatatypeProperty>
    


    <!-- http://nlpkg.sebis.cit.tum.de/nlp-fos-hierarchy.owl#doi -->

    <owl:DatatypeProperty rdf:about="http://nlpkg.sebis.cit.tum.de/nlp-fos-hierarchy.owl#doi">
        <rdf:type rdf:resource="http://www.w3.org/2002/07/owl#FunctionalProperty"/>
        <rdfs:domain rdf:resource="http://nlpkg.sebis.cit.tum.de/nlp-fos-hierarchy.owl#Publication"/>
        <rdfs:range rdf:resource="http://www.w3.org/2001/XMLSchema#string"/>
        <rdfs:comment xml:lang="en">Digital Object Identifier (DOI) of a publication.</rdfs:comment>
        <rdfs:label xml:lang="en">doi</rdfs:label>
    </owl:DatatypeProperty>
    


    <!-- http://nlpkg.sebis.cit.tum.de/nlp-fos-hierarchy.owl#email -->

    <owl:DatatypeProperty rdf:about="http://nlpkg.sebis.cit.tum.de/nlp-fos-hierarchy.owl#email">
        <rdfs:range rdf:resource="http://www.w3.org/2001/XMLSchema#string"/>
    </owl:DatatypeProperty>
    


    <!-- http://nlpkg.sebis.cit.tum.de/nlp-fos-hierarchy.owl#embedding -->

    <owl:DatatypeProperty rdf:about="http://nlpkg.sebis.cit.tum.de/nlp-fos-hierarchy.owl#embedding">
        <rdfs:domain rdf:resource="http://nlpkg.sebis.cit.tum.de/nlp-fos-hierarchy.owl#Publication"/>
        <rdfs:domain rdf:resource="http://nlpkg.sebis.cit.tum.de/nlp-taxonomy.owl#FieldOfStudy"/>
        <rdfs:range rdf:resource="http://www.w3.org/2001/XMLSchema#string"/>
        <rdfs:comment xml:lang="en">The semantic embedding of an entity in the knowledge graph.</rdfs:comment>
    </owl:DatatypeProperty>
    


    <!-- http://nlpkg.sebis.cit.tum.de/nlp-fos-hierarchy.owl#endPage -->

    <owl:DatatypeProperty rdf:about="http://nlpkg.sebis.cit.tum.de/nlp-fos-hierarchy.owl#endPage">
        <rdfs:domain rdf:resource="http://nlpkg.sebis.cit.tum.de/nlp-fos-hierarchy.owl#Publication"/>
        <rdfs:range rdf:resource="http://www.w3.org/2001/XMLSchema#int"/>
    </owl:DatatypeProperty>
    


    <!-- http://nlpkg.sebis.cit.tum.de/nlp-fos-hierarchy.owl#firstName -->

    <owl:DatatypeProperty rdf:about="http://nlpkg.sebis.cit.tum.de/nlp-fos-hierarchy.owl#firstName">
        <rdf:type rdf:resource="http://www.w3.org/2002/07/owl#FunctionalProperty"/>
        <rdfs:domain rdf:resource="http://nlpkg.sebis.cit.tum.de/nlp-fos-hierarchy.owl#Researcher"/>
        <rdfs:range rdf:resource="http://www.w3.org/2001/XMLSchema#string"/>
    </owl:DatatypeProperty>
    


    <!-- http://nlpkg.sebis.cit.tum.de/nlp-fos-hierarchy.owl#homepage -->

    <owl:DatatypeProperty rdf:about="http://nlpkg.sebis.cit.tum.de/nlp-fos-hierarchy.owl#homepage">
        <rdfs:domain rdf:resource="http://nlpkg.sebis.cit.tum.de/nlp-fos-hierarchy.owl#Researcher"/>
        <rdfs:range rdf:resource="http://www.w3.org/2001/XMLSchema#string"/>
    </owl:DatatypeProperty>
    


    <!-- http://nlpkg.sebis.cit.tum.de/nlp-fos-hierarchy.owl#isbn -->

    <owl:DatatypeProperty rdf:about="http://nlpkg.sebis.cit.tum.de/nlp-fos-hierarchy.owl#isbn">
        <rdfs:domain rdf:resource="http://nlpkg.sebis.cit.tum.de/nlp-fos-hierarchy.owl#Publication"/>
        <rdfs:range rdf:resource="http://www.w3.org/2001/XMLSchema#string"/>
    </owl:DatatypeProperty>
    


    <!-- http://nlpkg.sebis.cit.tum.de/nlp-fos-hierarchy.owl#issn -->

    <owl:DatatypeProperty rdf:about="http://nlpkg.sebis.cit.tum.de/nlp-fos-hierarchy.owl#issn">
        <rdfs:domain rdf:resource="http://nlpkg.sebis.cit.tum.de/nlp-fos-hierarchy.owl#Publication"/>
        <rdfs:range rdf:resource="http://www.w3.org/2001/XMLSchema#string"/>
    </owl:DatatypeProperty>
    


    <!-- http://nlpkg.sebis.cit.tum.de/nlp-fos-hierarchy.owl#lastName -->

    <owl:DatatypeProperty rdf:about="http://nlpkg.sebis.cit.tum.de/nlp-fos-hierarchy.owl#lastName">
        <rdf:type rdf:resource="http://www.w3.org/2002/07/owl#FunctionalProperty"/>
        <rdfs:domain rdf:resource="http://nlpkg.sebis.cit.tum.de/nlp-fos-hierarchy.owl#Researcher"/>
        <rdfs:range rdf:resource="http://www.w3.org/2001/XMLSchema#string"/>
    </owl:DatatypeProperty>
    


    <!-- http://nlpkg.sebis.cit.tum.de/nlp-fos-hierarchy.owl#middleName -->

    <owl:DatatypeProperty rdf:about="http://nlpkg.sebis.cit.tum.de/nlp-fos-hierarchy.owl#middleName">
        <rdfs:domain rdf:resource="http://nlpkg.sebis.cit.tum.de/nlp-fos-hierarchy.owl#Researcher"/>
        <rdfs:range rdf:resource="http://www.w3.org/2001/XMLSchema#string"/>
    </owl:DatatypeProperty>
    


    <!-- http://nlpkg.sebis.cit.tum.de/nlp-fos-hierarchy.owl#numberOfCitations -->

    <owl:DatatypeProperty rdf:about="http://nlpkg.sebis.cit.tum.de/nlp-fos-hierarchy.owl#numberOfCitations">
        <rdfs:range rdf:resource="http://www.w3.org/2001/XMLSchema#int"/>
    </owl:DatatypeProperty>
    


    <!-- http://nlpkg.sebis.cit.tum.de/nlp-fos-hierarchy.owl#numberOfPages -->

    <owl:DatatypeProperty rdf:about="http://nlpkg.sebis.cit.tum.de/nlp-fos-hierarchy.owl#numberOfPages">
        <rdfs:domain rdf:resource="http://nlpkg.sebis.cit.tum.de/nlp-fos-hierarchy.owl#Publication"/>
        <rdfs:range rdf:resource="http://www.w3.org/2001/XMLSchema#int"/>
    </owl:DatatypeProperty>
    


    <!-- http://nlpkg.sebis.cit.tum.de/nlp-fos-hierarchy.owl#origin -->

    <owl:DatatypeProperty rdf:about="http://nlpkg.sebis.cit.tum.de/nlp-fos-hierarchy.owl#origin">
        <rdfs:domain rdf:resource="http://nlpkg.sebis.cit.tum.de/nlp-taxonomy.owl#FieldOfStudy"/>
        <rdfs:range rdf:resource="http://www.w3.org/2001/XMLSchema#string"/>
        <rdfs:comment xml:lang="en">The link to the origin of a Field of Study concept.</rdfs:comment>
    </owl:DatatypeProperty>
    


    <!-- http://nlpkg.sebis.cit.tum.de/nlp-fos-hierarchy.owl#phoneNumber -->

    <owl:DatatypeProperty rdf:about="http://nlpkg.sebis.cit.tum.de/nlp-fos-hierarchy.owl#phoneNumber">
        <rdfs:range rdf:resource="http://www.w3.org/2001/XMLSchema#int"/>
        <rdfs:range rdf:resource="http://www.w3.org/2001/XMLSchema#string"/>
    </owl:DatatypeProperty>
    


    <!-- http://nlpkg.sebis.cit.tum.de/nlp-fos-hierarchy.owl#postalAddress -->

    <owl:DatatypeProperty rdf:about="http://nlpkg.sebis.cit.tum.de/nlp-fos-hierarchy.owl#postalAddress">
        <rdfs:range rdf:resource="http://www.w3.org/2001/XMLSchema#string"/>
    </owl:DatatypeProperty>
    


    <!-- http://nlpkg.sebis.cit.tum.de/nlp-fos-hierarchy.owl#publicationAbstract -->

    <owl:DatatypeProperty rdf:about="http://nlpkg.sebis.cit.tum.de/nlp-fos-hierarchy.owl#publicationAbstract">
        <rdfs:domain rdf:resource="http://nlpkg.sebis.cit.tum.de/nlp-fos-hierarchy.owl#Publication"/>
        <rdfs:range rdf:resource="http://www.w3.org/2001/XMLSchema#string"/>
        <rdfs:comment xml:lang="en">A summary of the publication.</rdfs:comment>
        <rdfs:label xml:lang="en">publicationAbstract</rdfs:label>
    </owl:DatatypeProperty>
    


    <!-- http://nlpkg.sebis.cit.tum.de/nlp-fos-hierarchy.owl#publicationDate -->

    <owl:DatatypeProperty rdf:about="http://nlpkg.sebis.cit.tum.de/nlp-fos-hierarchy.owl#publicationDate">
        <rdfs:domain rdf:resource="http://nlpkg.sebis.cit.tum.de/nlp-fos-hierarchy.owl#Publication"/>
    </owl:DatatypeProperty>
    


    <!-- http://nlpkg.sebis.cit.tum.de/nlp-fos-hierarchy.owl#publicationDay -->

    <owl:DatatypeProperty rdf:about="http://nlpkg.sebis.cit.tum.de/nlp-fos-hierarchy.owl#publicationDay">
        <rdfs:subPropertyOf rdf:resource="http://nlpkg.sebis.cit.tum.de/nlp-fos-hierarchy.owl#publicationDate"/>
        <rdfs:domain rdf:resource="http://nlpkg.sebis.cit.tum.de/nlp-fos-hierarchy.owl#Publication"/>
        <rdfs:range rdf:resource="http://www.w3.org/2001/XMLSchema#int"/>
    </owl:DatatypeProperty>
    


    <!-- http://nlpkg.sebis.cit.tum.de/nlp-fos-hierarchy.owl#publicationMonth -->

    <owl:DatatypeProperty rdf:about="http://nlpkg.sebis.cit.tum.de/nlp-fos-hierarchy.owl#publicationMonth">
        <rdfs:subPropertyOf rdf:resource="http://nlpkg.sebis.cit.tum.de/nlp-fos-hierarchy.owl#publicationDate"/>
        <rdfs:domain rdf:resource="http://nlpkg.sebis.cit.tum.de/nlp-fos-hierarchy.owl#Publication"/>
        <rdfs:range rdf:resource="http://www.w3.org/2001/XMLSchema#int"/>
    </owl:DatatypeProperty>
    


    <!-- http://nlpkg.sebis.cit.tum.de/nlp-fos-hierarchy.owl#publicationPlace -->

    <owl:DatatypeProperty rdf:about="http://nlpkg.sebis.cit.tum.de/nlp-fos-hierarchy.owl#publicationPlace">
        <rdfs:domain rdf:resource="http://nlpkg.sebis.cit.tum.de/nlp-fos-hierarchy.owl#Publication"/>
        <rdfs:range rdf:resource="http://www.w3.org/2001/XMLSchema#string"/>
    </owl:DatatypeProperty>
    


    <!-- http://nlpkg.sebis.cit.tum.de/nlp-fos-hierarchy.owl#publicationTitle -->

    <owl:DatatypeProperty rdf:about="http://nlpkg.sebis.cit.tum.de/nlp-fos-hierarchy.owl#publicationTitle">
        <rdfs:domain rdf:resource="http://nlpkg.sebis.cit.tum.de/nlp-fos-hierarchy.owl#Publication"/>
        <rdfs:range rdf:resource="http://www.w3.org/2001/XMLSchema#string"/>
    </owl:DatatypeProperty>
    


    <!-- http://nlpkg.sebis.cit.tum.de/nlp-fos-hierarchy.owl#publishedIn -->

    <owl:DatatypeProperty rdf:about="http://nlpkg.sebis.cit.tum.de/nlp-fos-hierarchy.owl#publishedIn">
        <rdfs:domain rdf:resource="http://nlpkg.sebis.cit.tum.de/nlp-fos-hierarchy.owl#Publication"/>
        <rdfs:range rdf:resource="http://www.w3.org/2001/XMLSchema#string"/>
        <rdfs:comment xml:lang="en">Where the publication was published.</rdfs:comment>
    </owl:DatatypeProperty>
    


    <!-- http://nlpkg.sebis.cit.tum.de/nlp-fos-hierarchy.owl#relevantInformation -->

    <owl:DatatypeProperty rdf:about="http://nlpkg.sebis.cit.tum.de/nlp-fos-hierarchy.owl#relevantInformation">
        <rdfs:domain rdf:resource="http://nlpkg.sebis.cit.tum.de/nlp-taxonomy.owl#FieldOfStudy"/>
        <rdfs:range rdf:resource="http://www.w3.org/2001/XMLSchema#string"/>
        <rdfs:comment xml:lang="en">A link to further relevant information and material for a Field of Study.</rdfs:comment>
    </owl:DatatypeProperty>
    


    <!-- http://nlpkg.sebis.cit.tum.de/nlp-fos-hierarchy.owl#s2Id -->

    <owl:DatatypeProperty rdf:about="http://nlpkg.sebis.cit.tum.de/nlp-fos-hierarchy.owl#s2Id">
        <rdfs:domain rdf:resource="http://nlpkg.sebis.cit.tum.de/nlp-fos-hierarchy.owl#Publication"/>
        <rdfs:domain rdf:resource="http://nlpkg.sebis.cit.tum.de/nlp-fos-hierarchy.owl#Researcher"/>
        <rdfs:range rdf:resource="http://www.w3.org/2001/XMLSchema#string"/>
        <rdfs:comment xml:lang="en">The ID of a publication in Semantic Scholar.</rdfs:comment>
    </owl:DatatypeProperty>
    


    <!-- http://nlpkg.sebis.cit.tum.de/nlp-fos-hierarchy.owl#startPage -->

    <owl:DatatypeProperty rdf:about="http://nlpkg.sebis.cit.tum.de/nlp-fos-hierarchy.owl#startPage">
        <rdfs:domain rdf:resource="http://nlpkg.sebis.cit.tum.de/nlp-fos-hierarchy.owl#Publication"/>
        <rdfs:range rdf:resource="http://www.w3.org/2001/XMLSchema#int"/>
    </owl:DatatypeProperty>
    


    <!-- http://nlpkg.sebis.cit.tum.de/nlp-fos-hierarchy.owl#survey -->

    <owl:DatatypeProperty rdf:about="http://nlpkg.sebis.cit.tum.de/nlp-fos-hierarchy.owl#survey">
        <rdfs:domain rdf:resource="http://nlpkg.sebis.cit.tum.de/nlp-taxonomy.owl#FieldOfStudy"/>
        <rdfs:range rdf:resource="http://www.w3.org/2001/XMLSchema#string"/>
        <rdfs:comment xml:lang="en">A link to a survey about a Field of Study concept.</rdfs:comment>
    </owl:DatatypeProperty>
    


    <!-- http://nlpkg.sebis.cit.tum.de/nlp-fos-hierarchy.owl#tldr -->

    <owl:DatatypeProperty rdf:about="http://nlpkg.sebis.cit.tum.de/nlp-fos-hierarchy.owl#tldr">
        <rdfs:domain rdf:resource="http://nlpkg.sebis.cit.tum.de/nlp-fos-hierarchy.owl#Publication"/>
        <rdfs:range rdf:resource="http://www.w3.org/2001/XMLSchema#string"/>
        <rdfs:comment xml:lang="en">TL;DR, or &quot;Too long; didn’t read&quot; is the short summary of the abstract of a publication.</rdfs:comment>
    </owl:DatatypeProperty>
    


    <!-- http://nlpkg.sebis.cit.tum.de/nlp-fos-hierarchy.owl#venue -->

    <owl:DatatypeProperty rdf:about="http://nlpkg.sebis.cit.tum.de/nlp-fos-hierarchy.owl#venue">
        <rdfs:domain rdf:resource="http://nlpkg.sebis.cit.tum.de/nlp-fos-hierarchy.owl#Publication"/>
        <rdfs:range rdf:resource="http://www.w3.org/2001/XMLSchema#string"/>
        <rdfs:comment xml:lang="en">The publication venue</rdfs:comment>
    </owl:DatatypeProperty>
    


    <!-- http://nlpkg.sebis.cit.tum.de/nlp-taxonomy.owl#level -->

    <owl:DatatypeProperty rdf:about="http://nlpkg.sebis.cit.tum.de/nlp-taxonomy.owl#level">
        <rdfs:domain rdf:resource="http://nlpkg.sebis.cit.tum.de/nlp-taxonomy.owl#FieldOfStudy"/>
        <rdfs:range rdf:resource="http://www.w3.org/2001/XMLSchema#int"/>
        <rdfs:comment xml:lang="en">The hierarchy level of the Field of Study concept.</rdfs:comment>
    </owl:DatatypeProperty>
    


    <!-- ttp://nlpkg.sebis.cit.tum.de/nlp-fos-hierarchy.owl#hIndex -->

    <owl:DatatypeProperty rdf:about="ttp://nlpkg.sebis.cit.tum.de/nlp-fos-hierarchy.owl#hIndex">
        <rdfs:domain rdf:resource="http://nlpkg.sebis.cit.tum.de/nlp-fos-hierarchy.owl#Researcher"/>
        <rdfs:range rdf:resource="http://www.w3.org/2001/XMLSchema#int"/>
        <rdfs:comment xml:lang="en">The h-index is an author-level metric that measures both the productivity and citation impact of the publications, initially used for an individual scientist or scholar. The h-index is defined as the maximum value of h such that the given author/journal has published at least h papers that have each been cited at least h times.</rdfs:comment>
        <rdfs:label xml:lang="en">h-index</rdfs:label>
    </owl:DatatypeProperty>
    


    <!-- ttp://nlpkg.sebis.cit.tum.de/nlp-fos-hierarchy.owl#publicationYear -->

    <owl:DatatypeProperty rdf:about="ttp://nlpkg.sebis.cit.tum.de/nlp-fos-hierarchy.owl#publicationYear">
        <rdfs:subPropertyOf rdf:resource="http://nlpkg.sebis.cit.tum.de/nlp-fos-hierarchy.owl#publicationDate"/>
        <rdfs:domain rdf:resource="http://nlpkg.sebis.cit.tum.de/nlp-fos-hierarchy.owl#Publication"/>
        <rdfs:range rdf:resource="http://www.w3.org/2001/XMLSchema#int"/>
    </owl:DatatypeProperty>
    


    <!-- 
    ///////////////////////////////////////////////////////////////////////////////////////
    //
    // Classes
    //
    ///////////////////////////////////////////////////////////////////////////////////////
     -->

    


    <!-- http://nlpkg.sebis.cit.tum.de/nlp-fos-hierarchy.owl#Article -->

    <owl:Class rdf:about="http://nlpkg.sebis.cit.tum.de/nlp-fos-hierarchy.owl#Article">
        <rdfs:subClassOf rdf:resource="http://nlpkg.sebis.cit.tum.de/nlp-fos-hierarchy.owl#Publication"/>
        <rdfs:label xml:lang="en">Article</rdfs:label>
    </owl:Class>
    


    <!-- http://nlpkg.sebis.cit.tum.de/nlp-fos-hierarchy.owl#BachelorsThesis -->

    <owl:Class rdf:about="http://nlpkg.sebis.cit.tum.de/nlp-fos-hierarchy.owl#BachelorsThesis">
        <rdfs:subClassOf rdf:resource="http://nlpkg.sebis.cit.tum.de/nlp-fos-hierarchy.owl#Thesis"/>
        <rdfs:label xml:lang="en">Bachelor&apos;s Thesis</rdfs:label>
    </owl:Class>
    


    <!-- http://nlpkg.sebis.cit.tum.de/nlp-fos-hierarchy.owl#Book -->

    <owl:Class rdf:about="http://nlpkg.sebis.cit.tum.de/nlp-fos-hierarchy.owl#Book">
        <rdfs:subClassOf rdf:resource="http://nlpkg.sebis.cit.tum.de/nlp-fos-hierarchy.owl#Publication"/>
        <rdfs:label xml:lang="en">Book</rdfs:label>
    </owl:Class>
    


    <!-- http://nlpkg.sebis.cit.tum.de/nlp-fos-hierarchy.owl#BookArticle -->

    <owl:Class rdf:about="http://nlpkg.sebis.cit.tum.de/nlp-fos-hierarchy.owl#BookArticle">
        <rdfs:subClassOf rdf:resource="http://nlpkg.sebis.cit.tum.de/nlp-fos-hierarchy.owl#Article"/>
        <rdfs:label xml:lang="en">Book Article</rdfs:label>
    </owl:Class>
    


    <!-- http://nlpkg.sebis.cit.tum.de/nlp-fos-hierarchy.owl#ConferencePaper -->

    <owl:Class rdf:about="http://nlpkg.sebis.cit.tum.de/nlp-fos-hierarchy.owl#ConferencePaper">
        <rdfs:subClassOf rdf:resource="http://nlpkg.sebis.cit.tum.de/nlp-fos-hierarchy.owl#Article"/>
        <rdfs:label xml:lang="en">Conference Paper</rdfs:label>
    </owl:Class>
    


    <!-- http://nlpkg.sebis.cit.tum.de/nlp-fos-hierarchy.owl#DataStructure -->

    <owl:Class rdf:about="http://nlpkg.sebis.cit.tum.de/nlp-fos-hierarchy.owl#DataStructure">
        <rdfs:subClassOf rdf:resource="http://nlpkg.sebis.cit.tum.de/nlp-taxonomy.owl#FieldOfStudy"/>
        <dcterms:description xml:lang="en">A specialized format for organizing, processing, retrieving, and storing data.</dcterms:description>
        <rdfs:label xml:lang="en">Data Structure</rdfs:label>
    </owl:Class>
    


    <!-- http://nlpkg.sebis.cit.tum.de/nlp-fos-hierarchy.owl#DoctoralThesis -->

    <owl:Class rdf:about="http://nlpkg.sebis.cit.tum.de/nlp-fos-hierarchy.owl#DoctoralThesis">
        <rdfs:subClassOf rdf:resource="http://nlpkg.sebis.cit.tum.de/nlp-fos-hierarchy.owl#Thesis"/>
        <rdfs:label xml:lang="en">Doctoral Thesis</rdfs:label>
    </owl:Class>
    


    <!-- http://nlpkg.sebis.cit.tum.de/nlp-fos-hierarchy.owl#Journal -->

    <owl:Class rdf:about="http://nlpkg.sebis.cit.tum.de/nlp-fos-hierarchy.owl#Journal">
        <rdfs:subClassOf rdf:resource="http://nlpkg.sebis.cit.tum.de/nlp-fos-hierarchy.owl#Periodical"/>
        <rdfs:label xml:lang="en">Journal</rdfs:label>
    </owl:Class>
    


    <!-- http://nlpkg.sebis.cit.tum.de/nlp-fos-hierarchy.owl#JournalArticle -->

    <owl:Class rdf:about="http://nlpkg.sebis.cit.tum.de/nlp-fos-hierarchy.owl#JournalArticle">
        <rdfs:subClassOf rdf:resource="http://nlpkg.sebis.cit.tum.de/nlp-fos-hierarchy.owl#Article"/>
        <rdfs:label xml:lang="en">Journal Article</rdfs:label>
    </owl:Class>
    


    <!-- http://nlpkg.sebis.cit.tum.de/nlp-fos-hierarchy.owl#Magazine -->

    <owl:Class rdf:about="http://nlpkg.sebis.cit.tum.de/nlp-fos-hierarchy.owl#Magazine">
        <rdfs:subClassOf rdf:resource="http://nlpkg.sebis.cit.tum.de/nlp-fos-hierarchy.owl#Periodical"/>
        <rdfs:label xml:lang="en">Magazine</rdfs:label>
    </owl:Class>
    


    <!-- http://nlpkg.sebis.cit.tum.de/nlp-fos-hierarchy.owl#MastersThesis -->

    <owl:Class rdf:about="http://nlpkg.sebis.cit.tum.de/nlp-fos-hierarchy.owl#MastersThesis">
        <rdfs:subClassOf rdf:resource="http://nlpkg.sebis.cit.tum.de/nlp-fos-hierarchy.owl#Thesis"/>
        <rdfs:label xml:lang="en">Master&apos;s Thesis</rdfs:label>
    </owl:Class>
    


    <!-- http://nlpkg.sebis.cit.tum.de/nlp-fos-hierarchy.owl#Method -->

    <owl:Class rdf:about="http://nlpkg.sebis.cit.tum.de/nlp-fos-hierarchy.owl#Method">
        <rdfs:subClassOf rdf:resource="http://nlpkg.sebis.cit.tum.de/nlp-taxonomy.owl#FieldOfStudy"/>
        <dcterms:description xml:lang="en">An approach how to solve a specific problem, often in the form of an algorithm or mathematical model.</dcterms:description>
        <rdfs:label xml:lang="en">Method</rdfs:label>
    </owl:Class>
    


    <!-- http://nlpkg.sebis.cit.tum.de/nlp-fos-hierarchy.owl#OtherPublication -->

    <owl:Class rdf:about="http://nlpkg.sebis.cit.tum.de/nlp-fos-hierarchy.owl#OtherPublication">
        <rdfs:subClassOf rdf:resource="http://nlpkg.sebis.cit.tum.de/nlp-fos-hierarchy.owl#Publication"/>
        <rdfs:label xml:lang="en">Other Publication</rdfs:label>
    </owl:Class>
    


    <!-- http://nlpkg.sebis.cit.tum.de/nlp-fos-hierarchy.owl#OtherScientificField -->

    <owl:Class rdf:about="http://nlpkg.sebis.cit.tum.de/nlp-fos-hierarchy.owl#OtherScientificField">
        <rdfs:subClassOf rdf:resource="http://nlpkg.sebis.cit.tum.de/nlp-taxonomy.owl#FieldOfStudy"/>
        <dcterms:description xml:lang="en">Any Field of Study that doesn&apos;t belong to the other categoreis.</dcterms:description>
        <rdfs:label xml:lang="en">Other Scientific Field</rdfs:label>
    </owl:Class>
    


    <!-- http://nlpkg.sebis.cit.tum.de/nlp-fos-hierarchy.owl#Periodical -->

    <owl:Class rdf:about="http://nlpkg.sebis.cit.tum.de/nlp-fos-hierarchy.owl#Periodical">
        <rdfs:subClassOf rdf:resource="http://nlpkg.sebis.cit.tum.de/nlp-fos-hierarchy.owl#Publication"/>
        <rdfs:label xml:lang="en">Periodical</rdfs:label>
    </owl:Class>
    


    <!-- http://nlpkg.sebis.cit.tum.de/nlp-fos-hierarchy.owl#Proceedings -->

    <owl:Class rdf:about="http://nlpkg.sebis.cit.tum.de/nlp-fos-hierarchy.owl#Proceedings">
        <rdfs:subClassOf rdf:resource="http://nlpkg.sebis.cit.tum.de/nlp-fos-hierarchy.owl#Publication"/>
        <rdfs:label xml:lang="en">Proceedings</rdfs:label>
    </owl:Class>
    


    <!-- http://nlpkg.sebis.cit.tum.de/nlp-fos-hierarchy.owl#Publication -->

    <owl:Class rdf:about="http://nlpkg.sebis.cit.tum.de/nlp-fos-hierarchy.owl#Publication">
        <rdfs:subClassOf rdf:resource="http://www.w3.org/2002/07/owl#Thing"/>
        <rdfs:subClassOf>
            <owl:Restriction>
                <owl:onProperty rdf:resource="http://nlpkg.sebis.cit.tum.de/nlp-fos-hierarchy.owl#is_referenced_by"/>
                <owl:someValuesFrom rdf:resource="http://nlpkg.sebis.cit.tum.de/nlp-fos-hierarchy.owl#Publication"/>
            </owl:Restriction>
        </rdfs:subClassOf>
        <rdfs:subClassOf>
            <owl:Restriction>
                <owl:onProperty rdf:resource="http://nlpkg.sebis.cit.tum.de/nlp-fos-hierarchy.owl#references"/>
                <owl:someValuesFrom rdf:resource="http://nlpkg.sebis.cit.tum.de/nlp-fos-hierarchy.owl#Publication"/>
            </owl:Restriction>
        </rdfs:subClassOf>
        <rdfs:subClassOf>
            <owl:Restriction>
                <owl:onProperty rdf:resource="http://nlpkg.sebis.cit.tum.de/nlp-fos-hierarchy.owl#studies"/>
                <owl:someValuesFrom rdf:resource="http://nlpkg.sebis.cit.tum.de/nlp-taxonomy.owl#FieldOfStudy"/>
            </owl:Restriction>
        </rdfs:subClassOf>
        <rdfs:subClassOf>
            <owl:Restriction>
                <owl:onProperty rdf:resource="http://nlpkg.sebis.cit.tum.de/nlp-fos-hierarchy.owl#has_author"/>
                <owl:minQualifiedCardinality rdf:datatype="http://www.w3.org/2001/XMLSchema#nonNegativeInteger">1</owl:minQualifiedCardinality>
                <owl:onClass rdf:resource="http://nlpkg.sebis.cit.tum.de/nlp-fos-hierarchy.owl#Researcher"/>
            </owl:Restriction>
        </rdfs:subClassOf>
        <rdfs:subClassOf>
            <owl:Restriction>
                <owl:onProperty rdf:resource="http://nlpkg.sebis.cit.tum.de/nlp-fos-hierarchy.owl#displayName"/>
                <owl:qualifiedCardinality rdf:datatype="http://www.w3.org/2001/XMLSchema#nonNegativeInteger">1</owl:qualifiedCardinality>
                <owl:onDataRange rdf:resource="http://www.w3.org/2001/XMLSchema#string"/>
            </owl:Restriction>
        </rdfs:subClassOf>
        <rdfs:subClassOf>
            <owl:Restriction>
                <owl:onProperty rdf:resource="http://nlpkg.sebis.cit.tum.de/nlp-fos-hierarchy.owl#numberOfCitations"/>
                <owl:qualifiedCardinality rdf:datatype="http://www.w3.org/2001/XMLSchema#nonNegativeInteger">1</owl:qualifiedCardinality>
                <owl:onDataRange rdf:resource="http://www.w3.org/2001/XMLSchema#integer"/>
            </owl:Restriction>
        </rdfs:subClassOf>
        <rdfs:subClassOf>
            <owl:Restriction>
                <owl:onProperty rdf:resource="http://nlpkg.sebis.cit.tum.de/nlp-fos-hierarchy.owl#aclId"/>
                <owl:maxQualifiedCardinality rdf:datatype="http://www.w3.org/2001/XMLSchema#nonNegativeInteger">1</owl:maxQualifiedCardinality>
                <owl:onDataRange rdf:resource="http://www.w3.org/2001/XMLSchema#string"/>
            </owl:Restriction>
        </rdfs:subClassOf>
        <rdfs:subClassOf>
            <owl:Restriction>
                <owl:onProperty rdf:resource="http://nlpkg.sebis.cit.tum.de/nlp-fos-hierarchy.owl#arxivId"/>
                <owl:maxQualifiedCardinality rdf:datatype="http://www.w3.org/2001/XMLSchema#nonNegativeInteger">1</owl:maxQualifiedCardinality>
                <owl:onDataRange rdf:resource="http://www.w3.org/2001/XMLSchema#string"/>
            </owl:Restriction>
        </rdfs:subClassOf>
        <rdfs:subClassOf>
            <owl:Restriction>
                <owl:onProperty rdf:resource="http://nlpkg.sebis.cit.tum.de/nlp-fos-hierarchy.owl#doi"/>
                <owl:maxQualifiedCardinality rdf:datatype="http://www.w3.org/2001/XMLSchema#nonNegativeInteger">1</owl:maxQualifiedCardinality>
                <owl:onDataRange rdf:resource="http://www.w3.org/2001/XMLSchema#string"/>
            </owl:Restriction>
        </rdfs:subClassOf>
        <rdfs:subClassOf>
            <owl:Restriction>
                <owl:onProperty rdf:resource="http://nlpkg.sebis.cit.tum.de/nlp-fos-hierarchy.owl#endPage"/>
                <owl:maxQualifiedCardinality rdf:datatype="http://www.w3.org/2001/XMLSchema#nonNegativeInteger">1</owl:maxQualifiedCardinality>
                <owl:onDataRange rdf:resource="http://www.w3.org/2001/XMLSchema#int"/>
            </owl:Restriction>
        </rdfs:subClassOf>
        <rdfs:subClassOf>
            <owl:Restriction>
                <owl:onProperty rdf:resource="http://nlpkg.sebis.cit.tum.de/nlp-fos-hierarchy.owl#isbn"/>
                <owl:maxQualifiedCardinality rdf:datatype="http://www.w3.org/2001/XMLSchema#nonNegativeInteger">1</owl:maxQualifiedCardinality>
                <owl:onDataRange rdf:resource="http://www.w3.org/2001/XMLSchema#string"/>
            </owl:Restriction>
        </rdfs:subClassOf>
        <rdfs:subClassOf>
            <owl:Restriction>
                <owl:onProperty rdf:resource="http://nlpkg.sebis.cit.tum.de/nlp-fos-hierarchy.owl#issn"/>
                <owl:maxQualifiedCardinality rdf:datatype="http://www.w3.org/2001/XMLSchema#nonNegativeInteger">1</owl:maxQualifiedCardinality>
                <owl:onDataRange rdf:resource="http://www.w3.org/2001/XMLSchema#string"/>
            </owl:Restriction>
        </rdfs:subClassOf>
        <rdfs:subClassOf>
            <owl:Restriction>
                <owl:onProperty rdf:resource="http://nlpkg.sebis.cit.tum.de/nlp-fos-hierarchy.owl#publicationAbstract"/>
                <owl:maxQualifiedCardinality rdf:datatype="http://www.w3.org/2001/XMLSchema#nonNegativeInteger">1</owl:maxQualifiedCardinality>
                <owl:onDataRange rdf:resource="http://www.w3.org/2001/XMLSchema#string"/>
            </owl:Restriction>
        </rdfs:subClassOf>
        <rdfs:subClassOf>
            <owl:Restriction>
                <owl:onProperty rdf:resource="http://nlpkg.sebis.cit.tum.de/nlp-fos-hierarchy.owl#publicationDate"/>
                <owl:maxQualifiedCardinality rdf:datatype="http://www.w3.org/2001/XMLSchema#nonNegativeInteger">1</owl:maxQualifiedCardinality>
                <owl:onDataRange rdf:resource="http://www.w3.org/2001/XMLSchema#string"/>
            </owl:Restriction>
        </rdfs:subClassOf>
        <rdfs:subClassOf>
            <owl:Restriction>
                <owl:onProperty rdf:resource="http://nlpkg.sebis.cit.tum.de/nlp-fos-hierarchy.owl#publicationDay"/>
                <owl:maxQualifiedCardinality rdf:datatype="http://www.w3.org/2001/XMLSchema#nonNegativeInteger">1</owl:maxQualifiedCardinality>
                <owl:onDataRange rdf:resource="http://www.w3.org/2001/XMLSchema#string"/>
            </owl:Restriction>
        </rdfs:subClassOf>
        <rdfs:subClassOf>
            <owl:Restriction>
                <owl:onProperty rdf:resource="http://nlpkg.sebis.cit.tum.de/nlp-fos-hierarchy.owl#publicationMonth"/>
                <owl:maxQualifiedCardinality rdf:datatype="http://www.w3.org/2001/XMLSchema#nonNegativeInteger">1</owl:maxQualifiedCardinality>
                <owl:onDataRange rdf:resource="http://www.w3.org/2001/XMLSchema#string"/>
            </owl:Restriction>
        </rdfs:subClassOf>
        <rdfs:subClassOf>
            <owl:Restriction>
                <owl:onProperty rdf:resource="http://nlpkg.sebis.cit.tum.de/nlp-fos-hierarchy.owl#publicationTitle"/>
                <owl:maxQualifiedCardinality rdf:datatype="http://www.w3.org/2001/XMLSchema#nonNegativeInteger">1</owl:maxQualifiedCardinality>
                <owl:onDataRange rdf:resource="http://www.w3.org/2001/XMLSchema#string"/>
            </owl:Restriction>
        </rdfs:subClassOf>
        <rdfs:subClassOf>
            <owl:Restriction>
                <owl:onProperty rdf:resource="http://nlpkg.sebis.cit.tum.de/nlp-fos-hierarchy.owl#s2Id"/>
                <owl:maxQualifiedCardinality rdf:datatype="http://www.w3.org/2001/XMLSchema#nonNegativeInteger">1</owl:maxQualifiedCardinality>
                <owl:onDataRange rdf:resource="http://www.w3.org/2001/XMLSchema#string"/>
            </owl:Restriction>
        </rdfs:subClassOf>
        <rdfs:subClassOf>
            <owl:Restriction>
                <owl:onProperty rdf:resource="http://nlpkg.sebis.cit.tum.de/nlp-fos-hierarchy.owl#startPage"/>
                <owl:maxQualifiedCardinality rdf:datatype="http://www.w3.org/2001/XMLSchema#nonNegativeInteger">1</owl:maxQualifiedCardinality>
                <owl:onDataRange rdf:resource="http://www.w3.org/2001/XMLSchema#int"/>
            </owl:Restriction>
        </rdfs:subClassOf>
        <rdfs:subClassOf>
            <owl:Restriction>
                <owl:onProperty rdf:resource="ttp://nlpkg.sebis.cit.tum.de/nlp-fos-hierarchy.owl#publicationYear"/>
                <owl:maxQualifiedCardinality rdf:datatype="http://www.w3.org/2001/XMLSchema#nonNegativeInteger">1</owl:maxQualifiedCardinality>
                <owl:onDataRange rdf:resource="http://www.w3.org/2001/XMLSchema#string"/>
            </owl:Restriction>
        </rdfs:subClassOf>
        <rdfs:label xml:lang="en">Publication</rdfs:label>
    </owl:Class>
    


    <!-- http://nlpkg.sebis.cit.tum.de/nlp-fos-hierarchy.owl#Report -->

    <owl:Class rdf:about="http://nlpkg.sebis.cit.tum.de/nlp-fos-hierarchy.owl#Report">
        <rdfs:subClassOf rdf:resource="http://nlpkg.sebis.cit.tum.de/nlp-fos-hierarchy.owl#Publication"/>
        <rdfs:label xml:lang="en">Report</rdfs:label>
    </owl:Class>
    


    <!-- http://nlpkg.sebis.cit.tum.de/nlp-fos-hierarchy.owl#Researcher -->

    <owl:Class rdf:about="http://nlpkg.sebis.cit.tum.de/nlp-fos-hierarchy.owl#Researcher">
        <rdfs:subClassOf rdf:resource="http://www.w3.org/2002/07/owl#Thing"/>
        <rdfs:subClassOf>
            <owl:Restriction>
                <owl:onProperty rdf:resource="http://nlpkg.sebis.cit.tum.de/nlp-fos-hierarchy.owl#is_author_of"/>
                <owl:someValuesFrom rdf:resource="http://nlpkg.sebis.cit.tum.de/nlp-fos-hierarchy.owl#Publication"/>
            </owl:Restriction>
        </rdfs:subClassOf>
        <rdfs:subClassOf>
            <owl:Restriction>
                <owl:onProperty rdf:resource="http://nlpkg.sebis.cit.tum.de/nlp-fos-hierarchy.owl#affiliations"/>
                <owl:someValuesFrom rdf:resource="http://www.w3.org/2001/XMLSchema#string"/>
            </owl:Restriction>
        </rdfs:subClassOf>
        <rdfs:subClassOf>
            <owl:Restriction>
                <owl:onProperty rdf:resource="http://nlpkg.sebis.cit.tum.de/nlp-fos-hierarchy.owl#email"/>
                <owl:someValuesFrom rdf:resource="http://www.w3.org/2001/XMLSchema#string"/>
            </owl:Restriction>
        </rdfs:subClassOf>
        <rdfs:subClassOf>
            <owl:Restriction>
                <owl:onProperty rdf:resource="http://nlpkg.sebis.cit.tum.de/nlp-fos-hierarchy.owl#middleName"/>
                <owl:someValuesFrom rdf:resource="http://www.w3.org/2002/07/owl#rational"/>
            </owl:Restriction>
        </rdfs:subClassOf>
        <rdfs:subClassOf>
            <owl:Restriction>
                <owl:onProperty rdf:resource="ttp://nlpkg.sebis.cit.tum.de/nlp-fos-hierarchy.owl#hIndex"/>
                <owl:someValuesFrom rdf:resource="http://www.w3.org/2001/XMLSchema#string"/>
            </owl:Restriction>
        </rdfs:subClassOf>
        <rdfs:subClassOf>
            <owl:Restriction>
                <owl:onProperty rdf:resource="http://nlpkg.sebis.cit.tum.de/nlp-fos-hierarchy.owl#firstName"/>
                <owl:qualifiedCardinality rdf:datatype="http://www.w3.org/2001/XMLSchema#nonNegativeInteger">1</owl:qualifiedCardinality>
                <owl:onDataRange rdf:resource="http://www.w3.org/2001/XMLSchema#string"/>
            </owl:Restriction>
        </rdfs:subClassOf>
        <rdfs:subClassOf>
            <owl:Restriction>
                <owl:onProperty rdf:resource="http://nlpkg.sebis.cit.tum.de/nlp-fos-hierarchy.owl#lastName"/>
                <owl:qualifiedCardinality rdf:datatype="http://www.w3.org/2001/XMLSchema#nonNegativeInteger">1</owl:qualifiedCardinality>
                <owl:onDataRange rdf:resource="http://www.w3.org/2001/XMLSchema#string"/>
            </owl:Restriction>
        </rdfs:subClassOf>
        <rdfs:subClassOf>
            <owl:Restriction>
                <owl:onProperty rdf:resource="http://nlpkg.sebis.cit.tum.de/nlp-fos-hierarchy.owl#aclId"/>
                <owl:maxQualifiedCardinality rdf:datatype="http://www.w3.org/2001/XMLSchema#nonNegativeInteger">1</owl:maxQualifiedCardinality>
                <owl:onDataRange rdf:resource="http://www.w3.org/2001/XMLSchema#string"/>
            </owl:Restriction>
        </rdfs:subClassOf>
        <rdfs:subClassOf>
            <owl:Restriction>
                <owl:onProperty rdf:resource="http://nlpkg.sebis.cit.tum.de/nlp-fos-hierarchy.owl#arxivId"/>
                <owl:maxQualifiedCardinality rdf:datatype="http://www.w3.org/2001/XMLSchema#nonNegativeInteger">1</owl:maxQualifiedCardinality>
                <owl:onDataRange rdf:resource="http://www.w3.org/2001/XMLSchema#string"/>
            </owl:Restriction>
        </rdfs:subClassOf>
        <rdfs:label xml:lang="en">Researcher</rdfs:label>
    </owl:Class>
    


    <!-- http://nlpkg.sebis.cit.tum.de/nlp-fos-hierarchy.owl#Task -->

    <owl:Class rdf:about="http://nlpkg.sebis.cit.tum.de/nlp-fos-hierarchy.owl#Task">
        <rdfs:subClassOf rdf:resource="http://nlpkg.sebis.cit.tum.de/nlp-taxonomy.owl#FieldOfStudy"/>
        <dcterms:description xml:lang="en">Applications, problems to solve, systems to construct.</dcterms:description>
        <rdfs:label xml:lang="en">Task</rdfs:label>
    </owl:Class>
    


    <!-- http://nlpkg.sebis.cit.tum.de/nlp-fos-hierarchy.owl#Thesis -->

    <owl:Class rdf:about="http://nlpkg.sebis.cit.tum.de/nlp-fos-hierarchy.owl#Thesis">
        <rdfs:subClassOf rdf:resource="http://nlpkg.sebis.cit.tum.de/nlp-fos-hierarchy.owl#Publication"/>
        <rdfs:label xml:lang="en">Thesis</rdfs:label>
    </owl:Class>
    


    <!-- http://nlpkg.sebis.cit.tum.de/nlp-fos-hierarchy.owl#WorkshopPaper -->

    <owl:Class rdf:about="http://nlpkg.sebis.cit.tum.de/nlp-fos-hierarchy.owl#WorkshopPaper">
        <rdfs:subClassOf rdf:resource="http://nlpkg.sebis.cit.tum.de/nlp-fos-hierarchy.owl#Article"/>
        <rdfs:label xml:lang="en">Workshop Paper</rdfs:label>
    </owl:Class>
    


    <!-- http://nlpkg.sebis.cit.tum.de/nlp-taxonomy.owl#FieldOfStudy -->

    <owl:Class rdf:about="http://nlpkg.sebis.cit.tum.de/nlp-taxonomy.owl#FieldOfStudy">
        <rdfs:subClassOf rdf:resource="http://www.w3.org/2002/07/owl#Thing"/>
        <rdfs:subClassOf>
            <owl:Restriction>
                <owl:onProperty rdf:resource="http://nlpkg.sebis.cit.tum.de/nlp-taxonomy.owl#subFieldOf"/>
                <owl:someValuesFrom rdf:resource="http://nlpkg.sebis.cit.tum.de/nlp-taxonomy.owl#FieldOfStudy"/>
            </owl:Restriction>
        </rdfs:subClassOf>
        <rdfs:subClassOf>
            <owl:Restriction>
                <owl:onProperty rdf:resource="http://nlpkg.sebis.cit.tum.de/nlp-taxonomy.owl#superFieldOf"/>
                <owl:someValuesFrom rdf:resource="http://nlpkg.sebis.cit.tum.de/nlp-taxonomy.owl#FieldOfStudy"/>
            </owl:Restriction>
        </rdfs:subClassOf>
        <rdfs:label xml:lang="en">Field of Study</rdfs:label>
    </owl:Class>
    


    <!-- 
    ///////////////////////////////////////////////////////////////////////////////////////
    //
    // Individuals
    //
    ///////////////////////////////////////////////////////////////////////////////////////
     -->

    


    <!-- http://nlpkg.sebis.cit.tum.de/nlp-fos-hierarchy.owl#AMR-to-Text -->

    <owl:NamedIndividual rdf:about="http://nlpkg.sebis.cit.tum.de/nlp-fos-hierarchy.owl#AMR-to-Text">
        <rdf:type rdf:resource="http://nlpkg.sebis.cit.tum.de/nlp-fos-hierarchy.owl#Task"/>
        <rdf:type rdf:resource="http://nlpkg.sebis.cit.tum.de/nlp-taxonomy.owl#FieldOfStudy"/>
        <nlp-taxonomy:subFieldOf rdf:resource="http://nlpkg.sebis.cit.tum.de/nlp-fos-hierarchy.owl#Abstract_Meaning_Representation"/>
        <nlp-taxonomy:subFieldOf rdf:resource="http://nlpkg.sebis.cit.tum.de/nlp-fos-hierarchy.owl#Graph-to-Text"/>
        <survey>https://arxiv.org/abs/2206.07328</survey>
        <nlp-taxonomy:level rdf:datatype="http://www.w3.org/2001/XMLSchema#integer">4</nlp-taxonomy:level>
        <nlp-taxonomy:level rdf:datatype="http://www.w3.org/2001/XMLSchema#integer">5</nlp-taxonomy:level>
        <nlp-taxonomy:level rdf:datatype="http://www.w3.org/2001/XMLSchema#integer">6</nlp-taxonomy:level>
        <dcterms:description xml:lang="en">AMR-to-Text is a task that aims at generating fluent texts from Abstract Meaning Representation (AMR) graphs.</dcterms:description>
        <oboInOwl:hasSynonym xml:lang="en">Abstract Meaning Representation to Text</oboInOwl:hasSynonym>
        <rdfs:label xml:lang="en">AMR-to-Text</rdfs:label>
    </owl:NamedIndividual>
    


    <!-- http://nlpkg.sebis.cit.tum.de/nlp-fos-hierarchy.owl#Abstract_Meaning_Representation -->

    <owl:NamedIndividual rdf:about="http://nlpkg.sebis.cit.tum.de/nlp-fos-hierarchy.owl#Abstract_Meaning_Representation">
        <rdf:type rdf:resource="http://nlpkg.sebis.cit.tum.de/nlp-fos-hierarchy.owl#DataStructure"/>
        <rdf:type rdf:resource="http://nlpkg.sebis.cit.tum.de/nlp-taxonomy.owl#FieldOfStudy"/>
        <nlp-taxonomy:subFieldOf rdf:resource="http://nlpkg.sebis.cit.tum.de/nlp-fos-hierarchy.owl#Graphs"/>
        <nlp-taxonomy:subFieldOf rdf:resource="http://nlpkg.sebis.cit.tum.de/nlp-fos-hierarchy.owl#Text_Representations"/>
        <nlp-taxonomy:superFieldOf rdf:resource="http://nlpkg.sebis.cit.tum.de/nlp-fos-hierarchy.owl#AMR-to-Text"/>
        <relevantInformation>https://web.stanford.edu/~jurafsky/slp3/19.pdf</relevantInformation>
        <survey>https://arxiv.org/abs/2206.07328</survey>
        <nlp-taxonomy:level rdf:datatype="http://www.w3.org/2001/XMLSchema#integer">4</nlp-taxonomy:level>
        <nlp-taxonomy:level rdf:datatype="http://www.w3.org/2001/XMLSchema#integer">5</nlp-taxonomy:level>
        <dcterms:description xml:lang="en">Abstract Meaning Representation (AMR) is a semantic representation language that encodes meanings of sentences in a structured and interpretable form. It represents sentences as rooted, directed, acyclic graphs that capture core semantic information, such as who is doing what to whom, along with additional details like modality, tense, and polarity.</dcterms:description>
        <oboInOwl:hasSynonym xml:lang="en">AMR</oboInOwl:hasSynonym>
        <oboInOwl:hasSynonym xml:lang="en">Meaning Representation</oboInOwl:hasSynonym>
        <rdfs:label xml:lang="en">Abstract Meaning Representation</rdfs:label>
    </owl:NamedIndividual>
    


    <!-- http://nlpkg.sebis.cit.tum.de/nlp-fos-hierarchy.owl#Abstractive_Summarization -->

    <owl:NamedIndividual rdf:about="http://nlpkg.sebis.cit.tum.de/nlp-fos-hierarchy.owl#Abstractive_Summarization">
        <rdf:type rdf:resource="http://nlpkg.sebis.cit.tum.de/nlp-fos-hierarchy.owl#Task"/>
        <rdf:type rdf:resource="http://nlpkg.sebis.cit.tum.de/nlp-taxonomy.owl#FieldOfStudy"/>
        <nlp-taxonomy:subFieldOf rdf:resource="http://nlpkg.sebis.cit.tum.de/nlp-taxonomy.owl#Summarization"/>
        <survey>https://arxiv.org/abs/1812.02303</survey>
        <survey>https://arxiv.org/abs/2104.14839</survey>
        <survey>https://arxiv.org/abs/2208.04163</survey>
        <survey>https://arxiv.org/abs/2303.17650</survey>
        <nlp-taxonomy:level rdf:datatype="http://www.w3.org/2001/XMLSchema#integer">3</nlp-taxonomy:level>
        <dcterms:description xml:lang="en">Abstractive Summarization involves generating a concise and coherent summary of a longer text by interpreting and rephrasing the content in a more abstract or human-like manner. Abstractive Summarization aims to produce concise, coherent, and informative summaries by generating new sentences or phrases that capture the essence of the source material. This approach allows for flexibility in summarizing content but can be challenging to ensure the generated summaries are both accurate and coherent.</dcterms:description>
        <oboInOwl:hasSynonym xml:lang="en">Abstractive Summarisation</oboInOwl:hasSynonym>
        <oboInOwl:hasSynonym xml:lang="en">Generative Summarisation</oboInOwl:hasSynonym>
        <oboInOwl:hasSynonym xml:lang="en">Generative Summarization</oboInOwl:hasSynonym>
        <rdfs:label xml:lang="en">Abstractive Summarization</rdfs:label>
    </owl:NamedIndividual>
    


    <!-- http://nlpkg.sebis.cit.tum.de/nlp-fos-hierarchy.owl#Acoustic_Modeling -->

    <owl:NamedIndividual rdf:about="http://nlpkg.sebis.cit.tum.de/nlp-fos-hierarchy.owl#Acoustic_Modeling">
        <rdf:type rdf:resource="http://nlpkg.sebis.cit.tum.de/nlp-fos-hierarchy.owl#Task"/>
        <rdf:type rdf:resource="http://nlpkg.sebis.cit.tum.de/nlp-taxonomy.owl#FieldOfStudy"/>
        <nlp-taxonomy:subFieldOf rdf:resource="http://nlpkg.sebis.cit.tum.de/nlp-taxonomy.owl#Speech_Recognition"/>
        <nlp-taxonomy:level rdf:datatype="http://www.w3.org/2001/XMLSchema#integer">4</nlp-taxonomy:level>
        <dcterms:description xml:lang="en">Acoustic Modeling involves the process of modeling and analyzing the acoustic properties of spoken language, specifically the relationship between the acoustic signal (i.e., the audio waveform) and the phonemes or other linguistic content of speech.</dcterms:description>
        <rdfs:label xml:lang="en">Acoustic Modeling</rdfs:label>
    </owl:NamedIndividual>
    


    <!-- http://nlpkg.sebis.cit.tum.de/nlp-fos-hierarchy.owl#Acoustic_Signal_Processing -->

    <owl:NamedIndividual rdf:about="http://nlpkg.sebis.cit.tum.de/nlp-fos-hierarchy.owl#Acoustic_Signal_Processing">
        <rdf:type rdf:resource="http://nlpkg.sebis.cit.tum.de/nlp-fos-hierarchy.owl#Task"/>
        <rdf:type rdf:resource="http://nlpkg.sebis.cit.tum.de/nlp-taxonomy.owl#FieldOfStudy"/>
        <nlp-taxonomy:subFieldOf rdf:resource="http://nlpkg.sebis.cit.tum.de/nlp-taxonomy.owl#Speech_Recognition"/>
        <nlp-taxonomy:level rdf:datatype="http://www.w3.org/2001/XMLSchema#integer">4</nlp-taxonomy:level>
        <dcterms:description xml:lang="en">Acoustic Signal Processing focuses on the analysis, manipulation, and enhancement of sound signals, particularly in the context of audio and speech applications. It involves various techniques and algorithms for processing audio and speech signals to extract meaningful information, improve their quality, or achieve specific objectives.</dcterms:description>
        <rdfs:label xml:lang="en">Acoustic Signal Processing</rdfs:label>
    </owl:NamedIndividual>
    


    <!-- http://nlpkg.sebis.cit.tum.de/nlp-fos-hierarchy.owl#Active_Learning -->

    <owl:NamedIndividual rdf:about="http://nlpkg.sebis.cit.tum.de/nlp-fos-hierarchy.owl#Active_Learning">
        <rdf:type rdf:resource="http://nlpkg.sebis.cit.tum.de/nlp-fos-hierarchy.owl#Task"/>
        <rdf:type rdf:resource="http://nlpkg.sebis.cit.tum.de/nlp-taxonomy.owl#FieldOfStudy"/>
        <nlp-taxonomy:subFieldOf rdf:resource="http://nlpkg.sebis.cit.tum.de/nlp-taxonomy.owl#Low-Resource_NLP"/>
        <nlp-taxonomy:subFieldOf rdf:resource="http://nlpkg.sebis.cit.tum.de/nlp-taxonomy.owl#Green_&amp;_Sustainable_NLP"/>
        <nlp-taxonomy:superFieldOf rdf:resource="http://nlpkg.sebis.cit.tum.de/nlp-fos-hierarchy.owl#Proactive_Learning"/>
        <survey>https://aclanthology.org/2022.emnlp-main.414</survey>
        <survey>https://arxiv.org/abs/2008.07267</survey>
        <nlp-taxonomy:level rdf:datatype="http://www.w3.org/2001/XMLSchema#integer">3</nlp-taxonomy:level>
        <dcterms:description xml:lang="en">Active Learning is a machine learning approach where the model selects the data from which it learns. The model queries a user (an oracle who can provide the correct output) to label new data based on what it thinks will improve its learning the most. This approach is particularly useful when there is a lot of unlabeled data and labeling it all would be too time-consuming or expensive.</dcterms:description>
        <rdfs:label xml:lang="en">Active Learning</rdfs:label>
    </owl:NamedIndividual>
    


    <!-- http://nlpkg.sebis.cit.tum.de/nlp-fos-hierarchy.owl#Adversarial_Attacks -->

    <owl:NamedIndividual rdf:about="http://nlpkg.sebis.cit.tum.de/nlp-fos-hierarchy.owl#Adversarial_Attacks">
        <rdf:type rdf:resource="http://nlpkg.sebis.cit.tum.de/nlp-fos-hierarchy.owl#Task"/>
        <rdf:type rdf:resource="http://nlpkg.sebis.cit.tum.de/nlp-taxonomy.owl#FieldOfStudy"/>
        <nlp-taxonomy:subFieldOf rdf:resource="http://nlpkg.sebis.cit.tum.de/nlp-fos-hierarchy.owl#Privacy,_Security_&amp;_Safety_in_NLP"/>
        <nlp-taxonomy:superFieldOf rdf:resource="http://nlpkg.sebis.cit.tum.de/nlp-fos-hierarchy.owl#Adversarial_Defenses"/>
        <code>https://github.com/QData/TextAttack</code>
        <survey>https://arxiv.org/abs/1901.06796</survey>
        <survey>https://arxiv.org/abs/2005.14108</survey>
        <survey>https://arxiv.org/abs/2103.00676</survey>
        <survey>https://arxiv.org/abs/2310.10844</survey>
        <nlp-taxonomy:level rdf:datatype="http://www.w3.org/2001/XMLSchema#integer">4</nlp-taxonomy:level>
        <dcterms:description xml:lang="en">Adversarial attacks refer to the manipulation of input data with malicious intent to deceive NLP systems. This is typically done by introducing small, often imperceptible alterations to the original data, which can lead to significant changes in the system&apos;s output. The goal of these attacks is to exploit the vulnerabilities of the NLP models and cause them to make errors or produce incorrect results.</dcterms:description>
        <rdfs:label xml:lang="en">Adversarial Attacks</rdfs:label>
    </owl:NamedIndividual>
    


    <!-- http://nlpkg.sebis.cit.tum.de/nlp-fos-hierarchy.owl#Adversarial_Defenses -->

    <owl:NamedIndividual rdf:about="http://nlpkg.sebis.cit.tum.de/nlp-fos-hierarchy.owl#Adversarial_Defenses">
        <rdf:type rdf:resource="http://nlpkg.sebis.cit.tum.de/nlp-fos-hierarchy.owl#Task"/>
        <rdf:type rdf:resource="http://nlpkg.sebis.cit.tum.de/nlp-taxonomy.owl#FieldOfStudy"/>
        <uses rdf:resource="http://nlpkg.sebis.cit.tum.de/nlp-fos-hierarchy.owl#Adversarial_Training"/>
        <nlp-taxonomy:subFieldOf rdf:resource="http://nlpkg.sebis.cit.tum.de/nlp-fos-hierarchy.owl#Adversarial_Attacks"/>
        <survey>https://arxiv.org/abs/2005.14108</survey>
        <survey>https://arxiv.org/abs/2203.06414</survey>
        <nlp-taxonomy:level rdf:datatype="http://www.w3.org/2001/XMLSchema#integer">5</nlp-taxonomy:level>
        <dcterms:description xml:lang="en">Adversarial Defenses refer to strategies or techniques used to protect NLP systems from adversarial attacks. These attacks typically involve inputting deceptive data designed to trick or manipulate the system&apos;s output. Adversarial defenses aim to make the system robust against such attacks, ensuring the integrity and reliability of the system&apos;s performance.</dcterms:description>
        <rdfs:label xml:lang="en">Adversarial Defenses</rdfs:label>
    </owl:NamedIndividual>
    


    <!-- http://nlpkg.sebis.cit.tum.de/nlp-fos-hierarchy.owl#Adversarial_Prompting -->

    <owl:NamedIndividual rdf:about="http://nlpkg.sebis.cit.tum.de/nlp-fos-hierarchy.owl#Adversarial_Prompting">
        <rdf:type rdf:resource="http://nlpkg.sebis.cit.tum.de/nlp-fos-hierarchy.owl#Method"/>
        <rdf:type rdf:resource="http://nlpkg.sebis.cit.tum.de/nlp-taxonomy.owl#FieldOfStudy"/>
        <nlp-taxonomy:subFieldOf rdf:resource="http://nlpkg.sebis.cit.tum.de/nlp-fos-hierarchy.owl#Prompt_Injection"/>
        <code>https://github.com/hwchase17/adversarial-prompts</code>
        <origin>https://arxiv.org/abs/2302.04237</origin>
        <nlp-taxonomy:level rdf:datatype="http://www.w3.org/2001/XMLSchema#integer">5</nlp-taxonomy:level>
        <nlp-taxonomy:level rdf:datatype="http://www.w3.org/2001/XMLSchema#integer">6</nlp-taxonomy:level>
        <dcterms:description xml:lang="en">Adversarial Prompting refers to injecting prompts that can be standalone or prepended to begining prompts and induce specific behaviors into the generative process, such as generating images of a particular object or generating high perplexity text.</dcterms:description>
        <oboInOwl:hasSynonym xml:lang="en">Adversarial Prompt</oboInOwl:hasSynonym>
        <rdfs:label xml:lang="en">Adversarial Prompting</rdfs:label>
    </owl:NamedIndividual>
    


    <!-- http://nlpkg.sebis.cit.tum.de/nlp-fos-hierarchy.owl#Adversarial_Training -->

    <owl:NamedIndividual rdf:about="http://nlpkg.sebis.cit.tum.de/nlp-fos-hierarchy.owl#Adversarial_Training">
        <rdf:type rdf:resource="http://nlpkg.sebis.cit.tum.de/nlp-fos-hierarchy.owl#Task"/>
        <rdf:type rdf:resource="http://nlpkg.sebis.cit.tum.de/nlp-taxonomy.owl#FieldOfStudy"/>
        <usedFor rdf:resource="http://nlpkg.sebis.cit.tum.de/nlp-fos-hierarchy.owl#Adversarial_Defenses"/>
        <nlp-taxonomy:subFieldOf rdf:resource="http://nlpkg.sebis.cit.tum.de/nlp-taxonomy.owl#Robustness_In_NLP"/>
        <nlp-taxonomy:level rdf:datatype="http://www.w3.org/2001/XMLSchema#integer">3</nlp-taxonomy:level>
        <dcterms:description xml:lang="en">Adversarial Training is a technique used to improve the robustness and generalization of models. It involves training a model with malicious inputs (adversarial examples) created to mislead the model&apos;s learning process. These adversarial examples are typically generated by applying small but intentionally worst-case perturbations to instances from the training dataset, which makes the model more resilient and capable of handling unexpected or misleading input data.</dcterms:description>
        <rdfs:label xml:lang="en">Adversarial Training</rdfs:label>
    </owl:NamedIndividual>
    


    <!-- http://nlpkg.sebis.cit.tum.de/nlp-fos-hierarchy.owl#Age_Bias -->

    <owl:NamedIndividual rdf:about="http://nlpkg.sebis.cit.tum.de/nlp-fos-hierarchy.owl#Age_Bias">
        <rdf:type rdf:resource="http://nlpkg.sebis.cit.tum.de/nlp-fos-hierarchy.owl#OtherScientificField"/>
        <rdf:type rdf:resource="http://nlpkg.sebis.cit.tum.de/nlp-taxonomy.owl#FieldOfStudy"/>
        <nlp-taxonomy:subFieldOf rdf:resource="http://nlpkg.sebis.cit.tum.de/nlp-fos-hierarchy.owl#Social_Bias"/>
        <nlp-taxonomy:level rdf:datatype="http://www.w3.org/2001/XMLSchema#integer">5</nlp-taxonomy:level>
        <dcterms:description xml:lang="en">Age Bias refers to the discrimination or prejudice based on a person&apos;s age. It can occur at any stage of life, but it is most commonly experienced by older adults.</dcterms:description>
        <rdfs:label xml:lang="en">Age Bias</rdfs:label>
    </owl:NamedIndividual>
    


    <!-- http://nlpkg.sebis.cit.tum.de/nlp-fos-hierarchy.owl#All-words_Word_Sense_Disambiguation -->

    <owl:NamedIndividual rdf:about="http://nlpkg.sebis.cit.tum.de/nlp-fos-hierarchy.owl#All-words_Word_Sense_Disambiguation">
        <rdf:type rdf:resource="http://nlpkg.sebis.cit.tum.de/nlp-fos-hierarchy.owl#Task"/>
        <rdf:type rdf:resource="http://nlpkg.sebis.cit.tum.de/nlp-taxonomy.owl#FieldOfStudy"/>
        <nlp-taxonomy:subFieldOf rdf:resource="http://nlpkg.sebis.cit.tum.de/nlp-taxonomy.owl#Word_Sense_Disambiguation"/>
        <nlp-taxonomy:level rdf:datatype="http://www.w3.org/2001/XMLSchema#integer">3</nlp-taxonomy:level>
        <dcterms:description xml:lang="en">All-words Word Sense Disambiguation (WSD) is a task that involves identifying the correct meaning or sense of every word in a given text, based on the context. This is crucial because many words in a language can have multiple meanings, and understanding the correct sense is important for accurate language understanding and processing.</dcterms:description>
        <oboInOwl:hasSynonym xml:lang="en">All-words WSD</oboInOwl:hasSynonym>
        <rdfs:label xml:lang="en">All-words Word Sense Disambiguation</rdfs:label>
    </owl:NamedIndividual>
    


    <!-- http://nlpkg.sebis.cit.tum.de/nlp-fos-hierarchy.owl#Alternative_Lexicalization_Discourse_Relation_Recognition -->

    <owl:NamedIndividual rdf:about="http://nlpkg.sebis.cit.tum.de/nlp-fos-hierarchy.owl#Alternative_Lexicalization_Discourse_Relation_Recognition">
        <rdf:type rdf:resource="http://nlpkg.sebis.cit.tum.de/nlp-fos-hierarchy.owl#Task"/>
        <rdf:type rdf:resource="http://nlpkg.sebis.cit.tum.de/nlp-taxonomy.owl#FieldOfStudy"/>
        <nlp-taxonomy:subFieldOf rdf:resource="http://nlpkg.sebis.cit.tum.de/nlp-fos-hierarchy.owl#Discourse_Relation_Recognition"/>
        <nlp-taxonomy:level rdf:datatype="http://www.w3.org/2001/XMLSchema#integer">4</nlp-taxonomy:level>
        <nlp-taxonomy:level rdf:datatype="http://www.w3.org/2001/XMLSchema#integer">5</nlp-taxonomy:level>
        <nlp-taxonomy:level rdf:datatype="http://www.w3.org/2001/XMLSchema#integer">9</nlp-taxonomy:level>
        <dcterms:description xml:lang="en">Alternative Lexicalization Discourse Relation Recognition refers to the process of identifying and understanding the relationship between different parts of a text, even when they are expressed in different words or phrases. This involves recognizing synonyms, paraphrases, and other forms of alternative lexicalization, which can greatly affect the meaning and interpretation of a text.</dcterms:description>
        <oboInOwl:hasSynonym xml:lang="en">Alternative Lexicalization Discourse Relation Extraction</oboInOwl:hasSynonym>
        <rdfs:label xml:lang="en">Alternative Lexicalization Discourse Relation Recognition</rdfs:label>
    </owl:NamedIndividual>
    


    <!-- http://nlpkg.sebis.cit.tum.de/nlp-fos-hierarchy.owl#Analogical_Reasoning -->

    <owl:NamedIndividual rdf:about="http://nlpkg.sebis.cit.tum.de/nlp-fos-hierarchy.owl#Analogical_Reasoning">
        <rdf:type rdf:resource="http://nlpkg.sebis.cit.tum.de/nlp-fos-hierarchy.owl#Task"/>
        <rdf:type rdf:resource="http://nlpkg.sebis.cit.tum.de/nlp-taxonomy.owl#FieldOfStudy"/>
        <nlp-taxonomy:subFieldOf rdf:resource="http://nlpkg.sebis.cit.tum.de/nlp-taxonomy.owl#Reasoning"/>
        <nlp-taxonomy:superFieldOf rdf:resource="http://nlpkg.sebis.cit.tum.de/nlp-fos-hierarchy.owl#Analogy_Detection"/>
        <survey>https://arxiv.org/abs/2212.09196</survey>
        <survey>https://doi.org/10.1007/978-3-540-45091-7_2</survey>
        <nlp-taxonomy:level rdf:datatype="http://www.w3.org/2001/XMLSchema#integer">2</nlp-taxonomy:level>
        <dcterms:description xml:lang="en">Analogical Reasoning refers to the ability of a model to understand and apply logical analogies. It involves identifying patterns and drawing parallels between certain concepts or entities. For example, in the analogy &quot;man is to king as woman is to queen&quot;, the model should be able to understand the relationship between man and king, and apply the same relationship to woman and queen.</dcterms:description>
        <oboInOwl:hasSynonym xml:lang="en">Argument from Analogy</oboInOwl:hasSynonym>
        <oboInOwl:hasSynonym xml:lang="en">False Analogy</oboInOwl:hasSynonym>
        <rdfs:label xml:lang="en">Analogical Reasoning</rdfs:label>
    </owl:NamedIndividual>
    


    <!-- http://nlpkg.sebis.cit.tum.de/nlp-fos-hierarchy.owl#Analogy_Detection -->

    <owl:NamedIndividual rdf:about="http://nlpkg.sebis.cit.tum.de/nlp-fos-hierarchy.owl#Analogy_Detection">
        <rdf:type rdf:resource="http://nlpkg.sebis.cit.tum.de/nlp-fos-hierarchy.owl#Task"/>
        <rdf:type rdf:resource="http://nlpkg.sebis.cit.tum.de/nlp-taxonomy.owl#FieldOfStudy"/>
        <nlp-taxonomy:subFieldOf rdf:resource="http://nlpkg.sebis.cit.tum.de/nlp-fos-hierarchy.owl#Analogical_Reasoning"/>
        <nlp-taxonomy:subFieldOf rdf:resource="http://nlpkg.sebis.cit.tum.de/nlp-taxonomy.owl#Text_Classification"/>
        <nlp-taxonomy:level rdf:datatype="http://www.w3.org/2001/XMLSchema#integer">3</nlp-taxonomy:level>
        <dcterms:description xml:lang="en">Analogy Detection refers to the task of identifying analogies in texts.</dcterms:description>
        <oboInOwl:hasSynonym xml:lang="en">Analogy Identification</oboInOwl:hasSynonym>
        <rdfs:label xml:lang="en">Analogy Detection</rdfs:label>
    </owl:NamedIndividual>
    


    <!-- http://nlpkg.sebis.cit.tum.de/nlp-fos-hierarchy.owl#Anaphora_Resolution -->

    <owl:NamedIndividual rdf:about="http://nlpkg.sebis.cit.tum.de/nlp-fos-hierarchy.owl#Anaphora_Resolution">
        <rdf:type rdf:resource="http://nlpkg.sebis.cit.tum.de/nlp-fos-hierarchy.owl#Task"/>
        <rdf:type rdf:resource="http://nlpkg.sebis.cit.tum.de/nlp-taxonomy.owl#FieldOfStudy"/>
        <usedFor rdf:resource="http://nlpkg.sebis.cit.tum.de/nlp-fos-hierarchy.owl#Entity-Level_Sentiment_Analysis"/>
        <nlp-taxonomy:subFieldOf rdf:resource="http://nlpkg.sebis.cit.tum.de/nlp-taxonomy.owl#Coreference_Resolution"/>
        <nlp-taxonomy:superFieldOf rdf:resource="http://nlpkg.sebis.cit.tum.de/nlp-fos-hierarchy.owl#Discourse_Deixis_Resolution"/>
        <nlp-taxonomy:superFieldOf rdf:resource="http://nlpkg.sebis.cit.tum.de/nlp-fos-hierarchy.owl#Pronominal_Anaphora_Resolution"/>
        <nlp-taxonomy:superFieldOf rdf:resource="http://nlpkg.sebis.cit.tum.de/nlp-fos-hierarchy.owl#Zero_Anaphora_Resolution"/>
        <relevantInformation>https://aclanthology.org/venues/crac/</relevantInformation>
        <survey>https://arxiv.org/abs/1805.11824</survey>
        <nlp-taxonomy:level rdf:datatype="http://www.w3.org/2001/XMLSchema#integer">3</nlp-taxonomy:level>
        <dcterms:description xml:lang="en">Anaphora Resolution refers to the task of determining what a pronoun, or a noun phrase refers to in a given context. It&apos;s about resolving references in the text, especially when pronouns like &apos;he&apos;, &apos;she&apos;, &apos;it&apos; are used, the system should be able to identify to whom or what these pronouns are referring to. This is crucial for understanding the semantics and the complete meaning of a text.</dcterms:description>
        <rdfs:label xml:lang="en">Anaphora Resolution</rdfs:label>
    </owl:NamedIndividual>
    


    <!-- http://nlpkg.sebis.cit.tum.de/nlp-fos-hierarchy.owl#Anonymization -->

    <owl:NamedIndividual rdf:about="http://nlpkg.sebis.cit.tum.de/nlp-fos-hierarchy.owl#Anonymization">
        <rdf:type rdf:resource="http://nlpkg.sebis.cit.tum.de/nlp-fos-hierarchy.owl#Task"/>
        <rdf:type rdf:resource="http://nlpkg.sebis.cit.tum.de/nlp-taxonomy.owl#FieldOfStudy"/>
        <uses rdf:resource="http://nlpkg.sebis.cit.tum.de/nlp-fos-hierarchy.owl#Obfuscation"/>
        <uses rdf:resource="http://nlpkg.sebis.cit.tum.de/nlp-fos-hierarchy.owl#Sanitization"/>
        <nlp-taxonomy:subFieldOf rdf:resource="http://nlpkg.sebis.cit.tum.de/nlp-fos-hierarchy.owl#De-Identification"/>
        <nlp-taxonomy:level rdf:datatype="http://www.w3.org/2001/XMLSchema#integer">5</nlp-taxonomy:level>
        <dcterms:description xml:lang="en">Anonymization refers to the process of removing or replacing personally identifiable information (PII) from a dataset to protect the privacy of individuals. This can include names, addresses, phone numbers, email addresses, etc. The goal is to ensure that the data can be used for analysis or machine learning without compromising privacy.</dcterms:description>
        <oboInOwl:hasSynonym xml:lang="en">Anonymisation</oboInOwl:hasSynonym>
        <rdfs:label xml:lang="en">Anonymization</rdfs:label>
    </owl:NamedIndividual>
    


    <!-- http://nlpkg.sebis.cit.tum.de/nlp-fos-hierarchy.owl#Argument_Extraction -->

    <owl:NamedIndividual rdf:about="http://nlpkg.sebis.cit.tum.de/nlp-fos-hierarchy.owl#Argument_Extraction">
        <rdf:type rdf:resource="http://nlpkg.sebis.cit.tum.de/nlp-fos-hierarchy.owl#Task"/>
        <rdf:type rdf:resource="http://nlpkg.sebis.cit.tum.de/nlp-taxonomy.owl#FieldOfStudy"/>
        <nlp-taxonomy:subFieldOf rdf:resource="http://nlpkg.sebis.cit.tum.de/nlp-taxonomy.owl#Argument_Mining"/>
        <nlp-taxonomy:superFieldOf rdf:resource="http://nlpkg.sebis.cit.tum.de/nlp-fos-hierarchy.owl#Event_Argument_Extraction"/>
        <nlp-taxonomy:level rdf:datatype="http://www.w3.org/2001/XMLSchema#integer">3</nlp-taxonomy:level>
        <dcterms:description xml:lang="en">Argument Extraction refers to the process of identifying and classifying the arguments or components of a sentence. This includes determining the subject, object, and other entities in a sentence, as well as their relationships or roles.</dcterms:description>
        <rdfs:label xml:lang="en">Argument Extraction</rdfs:label>
    </owl:NamedIndividual>
    


    <!-- http://nlpkg.sebis.cit.tum.de/nlp-fos-hierarchy.owl#Argument_Generation -->

    <owl:NamedIndividual rdf:about="http://nlpkg.sebis.cit.tum.de/nlp-fos-hierarchy.owl#Argument_Generation">
        <rdf:type rdf:resource="http://nlpkg.sebis.cit.tum.de/nlp-fos-hierarchy.owl#Task"/>
        <rdf:type rdf:resource="http://nlpkg.sebis.cit.tum.de/nlp-taxonomy.owl#FieldOfStudy"/>
        <nlp-taxonomy:subFieldOf rdf:resource="http://nlpkg.sebis.cit.tum.de/nlp-taxonomy.owl#Argument_Mining"/>
        <nlp-taxonomy:subFieldOf rdf:resource="http://nlpkg.sebis.cit.tum.de/nlp-taxonomy.owl#Text_Generation"/>
        <nlp-taxonomy:level rdf:datatype="http://www.w3.org/2001/XMLSchema#integer">2</nlp-taxonomy:level>
        <nlp-taxonomy:level rdf:datatype="http://www.w3.org/2001/XMLSchema#integer">3</nlp-taxonomy:level>
        <dcterms:description xml:lang="en">Argument Generation refers to the process of creating or generating arguments on a specific topic using AI algorithms. It involves the use of machine learning and language models to produce relevant, coherent, and persuasive arguments.</dcterms:description>
        <rdfs:label xml:lang="en">Argument Generation</rdfs:label>
    </owl:NamedIndividual>
    


    <!-- http://nlpkg.sebis.cit.tum.de/nlp-fos-hierarchy.owl#Argument_Pair_Identification -->

    <owl:NamedIndividual rdf:about="http://nlpkg.sebis.cit.tum.de/nlp-fos-hierarchy.owl#Argument_Pair_Identification">
        <rdf:type rdf:resource="http://nlpkg.sebis.cit.tum.de/nlp-fos-hierarchy.owl#Task"/>
        <rdf:type rdf:resource="http://nlpkg.sebis.cit.tum.de/nlp-taxonomy.owl#FieldOfStudy"/>
        <nlp-taxonomy:subFieldOf rdf:resource="http://nlpkg.sebis.cit.tum.de/nlp-taxonomy.owl#Argument_Mining"/>
        <nlp-taxonomy:subFieldOf rdf:resource="http://nlpkg.sebis.cit.tum.de/nlp-taxonomy.owl#Text_Classification"/>
        <nlp-taxonomy:level rdf:datatype="http://www.w3.org/2001/XMLSchema#integer">3</nlp-taxonomy:level>
        <dcterms:description xml:lang="en">Argument Pair Identification is aiming to identify whether two arguments are interactively related.</dcterms:description>
        <oboInOwl:hasSynonym xml:lang="en">Argument Pair Classification</oboInOwl:hasSynonym>
        <oboInOwl:hasSynonym xml:lang="en">Argument Pair Detection</oboInOwl:hasSynonym>
        <rdfs:label xml:lang="en">Argument Pair Identification</rdfs:label>
    </owl:NamedIndividual>
    


    <!-- http://nlpkg.sebis.cit.tum.de/nlp-fos-hierarchy.owl#Aspect-specific_Sentence_Embeddings -->

    <owl:NamedIndividual rdf:about="http://nlpkg.sebis.cit.tum.de/nlp-fos-hierarchy.owl#Aspect-specific_Sentence_Embeddings">
        <rdf:type rdf:resource="http://nlpkg.sebis.cit.tum.de/nlp-fos-hierarchy.owl#DataStructure"/>
        <rdf:type rdf:resource="http://nlpkg.sebis.cit.tum.de/nlp-taxonomy.owl#FieldOfStudy"/>
        <uses rdf:resource="http://nlpkg.sebis.cit.tum.de/nlp-fos-hierarchy.owl#Sentence-Transformers"/>
        <nlp-taxonomy:subFieldOf rdf:resource="http://nlpkg.sebis.cit.tum.de/nlp-fos-hierarchy.owl#Sentence_Embeddings"/>
        <origin>https://arxiv.org/abs/2203.14541</origin>
        <nlp-taxonomy:level rdf:datatype="http://www.w3.org/2001/XMLSchema#integer">6</nlp-taxonomy:level>
        <dcterms:description xml:lang="en">Aspect-specific Sentence Embeddings refer to the representation of sentences in a vector space that provide similarities between texts based on certain predefined aspects. The aspects are inherent properties of texts that must be considered when predicting their semantic similarity. Based on the different aspects focused on in texts, their similarities can be perceived very differently. Aspect-based Sentence Embeddings may represent a text not as a single generic embedding but as multiple specialized embeddings.</dcterms:description>
        <rdfs:label xml:lang="en">Aspect-specific Sentence Embeddings</rdfs:label>
    </owl:NamedIndividual>
    


    <!-- http://nlpkg.sebis.cit.tum.de/nlp-fos-hierarchy.owl#Aspect_Sentiment_Quad_Prediction -->

    <owl:NamedIndividual rdf:about="http://nlpkg.sebis.cit.tum.de/nlp-fos-hierarchy.owl#Aspect_Sentiment_Quad_Prediction">
        <rdf:type rdf:resource="http://nlpkg.sebis.cit.tum.de/nlp-fos-hierarchy.owl#Task"/>
        <rdf:type rdf:resource="http://nlpkg.sebis.cit.tum.de/nlp-taxonomy.owl#FieldOfStudy"/>
        <nlp-taxonomy:subFieldOf rdf:resource="http://nlpkg.sebis.cit.tum.de/nlp-taxonomy#Aspect-based_Sentiment_Analysis"/>
        <nlp-taxonomy:level rdf:datatype="http://www.w3.org/2001/XMLSchema#integer">3</nlp-taxonomy:level>
        <dcterms:description xml:lang="en">Aspect Sentiment Quad Prediction (ASQP) analyzes the aspect terms, opinion terms, sentiment polarity, and aspect categories in a text.</dcterms:description>
        <oboInOwl:hasSynonym xml:lang="en">ASQP</oboInOwl:hasSynonym>
        <rdfs:label xml:lang="en">Aspect Sentiment Quad Prediction</rdfs:label>
    </owl:NamedIndividual>
    


    <!-- http://nlpkg.sebis.cit.tum.de/nlp-fos-hierarchy.owl#Aspect_Sentiment_Triplet_Extraction -->

    <owl:NamedIndividual rdf:about="http://nlpkg.sebis.cit.tum.de/nlp-fos-hierarchy.owl#Aspect_Sentiment_Triplet_Extraction">
        <rdf:type rdf:resource="http://nlpkg.sebis.cit.tum.de/nlp-fos-hierarchy.owl#Task"/>
        <rdf:type rdf:resource="http://nlpkg.sebis.cit.tum.de/nlp-taxonomy.owl#FieldOfStudy"/>
        <nlp-taxonomy:subFieldOf rdf:resource="http://nlpkg.sebis.cit.tum.de/nlp-taxonomy#Aspect-based_Sentiment_Analysis"/>
        <nlp-taxonomy:level rdf:datatype="http://www.w3.org/2001/XMLSchema#integer">3</nlp-taxonomy:level>
        <dcterms:description xml:lang="en">Aspect Sentiment Triplet Extraction (ASTE) is a task that aims to extract fine-grained opinion information from a given text. This information is typically in the form of triplets: aspect term, opinion term, and sentiment polarity. The aspect term refers to the subject or entity being discussed, the opinion term refers to the specific attribute of the aspect that is being commented on, and the sentiment polarity indicates whether the sentiment is positive, negative, or neutral.</dcterms:description>
        <oboInOwl:hasSynonym xml:lang="en">ASTE</oboInOwl:hasSynonym>
        <rdfs:label xml:lang="en">Aspect Sentiment Triplet Extraction</rdfs:label>
    </owl:NamedIndividual>
    


    <!-- http://nlpkg.sebis.cit.tum.de/nlp-fos-hierarchy.owl#Aspect_Term_Extraction -->

    <owl:NamedIndividual rdf:about="http://nlpkg.sebis.cit.tum.de/nlp-fos-hierarchy.owl#Aspect_Term_Extraction">
        <rdf:type rdf:resource="http://nlpkg.sebis.cit.tum.de/nlp-fos-hierarchy.owl#Task"/>
        <rdf:type rdf:resource="http://nlpkg.sebis.cit.tum.de/nlp-taxonomy.owl#FieldOfStudy"/>
        <nlp-taxonomy:subFieldOf rdf:resource="http://nlpkg.sebis.cit.tum.de/nlp-taxonomy#Aspect-based_Sentiment_Analysis"/>
        <nlp-taxonomy:subFieldOf rdf:resource="http://nlpkg.sebis.cit.tum.de/nlp-taxonomy.owl#Term_Extraction"/>
        <nlp-taxonomy:level rdf:datatype="http://www.w3.org/2001/XMLSchema#integer">3</nlp-taxonomy:level>
        <dcterms:description xml:lang="en">Aspect Term Extraction (ATE) refers to the task of identifying specific aspects or attributes mentioned in text data. These aspects could be features of a product, service, or any other entity. For example, in a review about a smartphone, aspects could be &quot;battery life&quot;, &quot;screen size&quot;, &quot;camera quality&quot;, etc. ATE is a crucial part of aspect-based sentiment analysis, where the goal is to understand sentiments expressed towards specific aspects.</dcterms:description>
        <oboInOwl:hasSynonym xml:lang="en">ATE</oboInOwl:hasSynonym>
        <rdfs:label xml:lang="en">Aspect Term Extraction</rdfs:label>
    </owl:NamedIndividual>
    


    <!-- http://nlpkg.sebis.cit.tum.de/nlp-fos-hierarchy.owl#Attention -->

    <owl:NamedIndividual rdf:about="http://nlpkg.sebis.cit.tum.de/nlp-fos-hierarchy.owl#Attention">
        <rdf:type rdf:resource="http://nlpkg.sebis.cit.tum.de/nlp-fos-hierarchy.owl#Method"/>
        <rdf:type rdf:resource="http://nlpkg.sebis.cit.tum.de/nlp-taxonomy.owl#FieldOfStudy"/>
        <usedFor rdf:resource="http://nlpkg.sebis.cit.tum.de/nlp-fos-hierarchy.owl#Transformers_&amp;_Large_Language_Models"/>
        <nlp-taxonomy:subFieldOf rdf:resource="http://nlpkg.sebis.cit.tum.de/nlp-fos-hierarchy.owl#Language_Model_Mechanisms"/>
        <origin>https://arxiv.org/abs/1409.0473</origin>
        <relevantInformation>https://jalammar.github.io/visualizing-neural-machine-translation-mechanics-of-seq2seq-models-with-attention/</relevantInformation>
        <survey>https://arxiv.org/abs/1811.05544</survey>
        <survey>https://arxiv.org/abs/1902.02181</survey>
        <nlp-taxonomy:level rdf:datatype="http://www.w3.org/2001/XMLSchema#integer">4</nlp-taxonomy:level>
        <dcterms:description xml:lang="en">Attention is a mechanism that allows models to focus on specific parts of the input when generating the output. It helps the model to pay &apos;attention&apos; to relevant words or phrases, and ignore the less relevant ones.</dcterms:description>
        <rdfs:label xml:lang="en">Attention</rdfs:label>
    </owl:NamedIndividual>
    


    <!-- http://nlpkg.sebis.cit.tum.de/nlp-fos-hierarchy.owl#Attribute_Inference_Attack -->

    <owl:NamedIndividual rdf:about="http://nlpkg.sebis.cit.tum.de/nlp-fos-hierarchy.owl#Attribute_Inference_Attack">
        <rdf:type rdf:resource="http://nlpkg.sebis.cit.tum.de/nlp-fos-hierarchy.owl#Task"/>
        <rdf:type rdf:resource="http://nlpkg.sebis.cit.tum.de/nlp-taxonomy.owl#FieldOfStudy"/>
        <nlp-taxonomy:subFieldOf rdf:resource="http://nlpkg.sebis.cit.tum.de/nlp-fos-hierarchy.owl#Inference_Attacks"/>
        <survey>https://arxiv.org/abs/2209.01292</survey>
        <nlp-taxonomy:level rdf:datatype="http://www.w3.org/2001/XMLSchema#integer">4</nlp-taxonomy:level>
        <dcterms:description xml:lang="en">In an Attribute Inference Attack, an adversary has partial knowledge of some training records and access to a model trained on those records, and infers the unknown values of a sensitive feature of those records.</dcterms:description>
        <rdfs:label xml:lang="en">Attribute Inference Attack</rdfs:label>
    </owl:NamedIndividual>
    


    <!-- http://nlpkg.sebis.cit.tum.de/nlp-fos-hierarchy.owl#Authorship_Attribution -->

    <owl:NamedIndividual rdf:about="http://nlpkg.sebis.cit.tum.de/nlp-fos-hierarchy.owl#Authorship_Attribution">
        <rdf:type rdf:resource="http://nlpkg.sebis.cit.tum.de/nlp-fos-hierarchy.owl#Task"/>
        <rdf:type rdf:resource="http://nlpkg.sebis.cit.tum.de/nlp-taxonomy.owl#FieldOfStudy"/>
        <nlp-taxonomy:subFieldOf rdf:resource="http://nlpkg.sebis.cit.tum.de/nlp-taxonomy.owl#Text_Classification"/>
        <nlp-taxonomy:superFieldOf rdf:resource="http://nlpkg.sebis.cit.tum.de/nlp-fos-hierarchy.owl#Authorship_Verification"/>
        <survey>https://aclanthology.org/C18-1029</survey>
        <survey>https://arxiv.org/abs/2009.14445</survey>
        <nlp-taxonomy:level rdf:datatype="http://www.w3.org/2001/XMLSchema#integer">3</nlp-taxonomy:level>
        <dcterms:description xml:lang="en">Authorship Attribution refers to the task of identifying the author of a given text. It involves analyzing the linguistic style, word usage, syntax, and other textual features to determine the most likely author. This concept is widely used in fields like forensics, literature, and cybersecurity.</dcterms:description>
        <oboInOwl:hasSynonym xml:lang="en">Authorship Identification</oboInOwl:hasSynonym>
        <rdfs:label xml:lang="en">Authorship Attribution</rdfs:label>
    </owl:NamedIndividual>
    


    <!-- http://nlpkg.sebis.cit.tum.de/nlp-fos-hierarchy.owl#Authorship_Obfuscation -->

    <owl:NamedIndividual rdf:about="http://nlpkg.sebis.cit.tum.de/nlp-fos-hierarchy.owl#Authorship_Obfuscation">
        <rdf:type rdf:resource="http://nlpkg.sebis.cit.tum.de/nlp-fos-hierarchy.owl#Task"/>
        <rdf:type rdf:resource="http://nlpkg.sebis.cit.tum.de/nlp-taxonomy.owl#FieldOfStudy"/>
        <nlp-taxonomy:subFieldOf rdf:resource="http://nlpkg.sebis.cit.tum.de/nlp-fos-hierarchy.owl#Obfuscation"/>
        <nlp-taxonomy:level rdf:datatype="http://www.w3.org/2001/XMLSchema#integer">5</nlp-taxonomy:level>
        <dcterms:description xml:lang="en">Authorship Obfuscation refers to the process of concealing or altering the writing style of a text to hide the identity of the original author. This is typically done using various techniques such as changing the vocabulary, syntax, or structure of the text. The goal is to protect the author&apos;s privacy or to prevent authorship attribution techniques from accurately identifying the author.</dcterms:description>
        <rdfs:label xml:lang="en">Authorship Obfuscation</rdfs:label>
    </owl:NamedIndividual>
    


    <!-- http://nlpkg.sebis.cit.tum.de/nlp-fos-hierarchy.owl#Authorship_Verification -->

    <owl:NamedIndividual rdf:about="http://nlpkg.sebis.cit.tum.de/nlp-fos-hierarchy.owl#Authorship_Verification">
        <rdf:type rdf:resource="http://nlpkg.sebis.cit.tum.de/nlp-fos-hierarchy.owl#Task"/>
        <rdf:type rdf:resource="http://nlpkg.sebis.cit.tum.de/nlp-taxonomy.owl#FieldOfStudy"/>
        <nlp-taxonomy:subFieldOf rdf:resource="http://nlpkg.sebis.cit.tum.de/nlp-fos-hierarchy.owl#Authorship_Attribution"/>
        <nlp-taxonomy:level rdf:datatype="http://www.w3.org/2001/XMLSchema#integer">4</nlp-taxonomy:level>
        <dcterms:description xml:lang="en">In Authorship Verification, texts of known authorship by one author are presented to a system, which is then tasked to verify whether another text has also been written by that same author</dcterms:description>
        <rdfs:label xml:lang="en">Authorship Verification</rdfs:label>
    </owl:NamedIndividual>
    


    <!-- http://nlpkg.sebis.cit.tum.de/nlp-fos-hierarchy.owl#Autoencoder -->

    <owl:NamedIndividual rdf:about="http://nlpkg.sebis.cit.tum.de/nlp-fos-hierarchy.owl#Autoencoder">
        <rdf:type rdf:resource="http://nlpkg.sebis.cit.tum.de/nlp-fos-hierarchy.owl#Method"/>
        <rdf:type rdf:resource="http://nlpkg.sebis.cit.tum.de/nlp-taxonomy.owl#FieldOfStudy"/>
        <nlp-taxonomy:subFieldOf rdf:resource="http://nlpkg.sebis.cit.tum.de/nlp-taxonomy.owl#Language_Models"/>
        <nlp-taxonomy:level rdf:datatype="http://www.w3.org/2001/XMLSchema#integer">3</nlp-taxonomy:level>
        <dcterms:description xml:lang="en">Autoencoder is a type of artificial neural network used for learning efficient codings of input data. It&apos;s designed to reconstruct its inputs, which forces the model to learn representations of the data in a compressed form.</dcterms:description>
        <rdfs:label xml:lang="en">Autoencoder</rdfs:label>
    </owl:NamedIndividual>
    


    <!-- http://nlpkg.sebis.cit.tum.de/nlp-fos-hierarchy.owl#Automatic_Essay_Scoring -->

    <owl:NamedIndividual rdf:about="http://nlpkg.sebis.cit.tum.de/nlp-fos-hierarchy.owl#Automatic_Essay_Scoring">
        <rdf:type rdf:resource="http://nlpkg.sebis.cit.tum.de/nlp-fos-hierarchy.owl#Task"/>
        <rdf:type rdf:resource="http://nlpkg.sebis.cit.tum.de/nlp-taxonomy.owl#FieldOfStudy"/>
        <nlp-taxonomy:subFieldOf rdf:resource="http://nlpkg.sebis.cit.tum.de/nlp-fos-hierarchy.owl#Text_Regression"/>
        <nlp-taxonomy:subFieldOf rdf:resource="http://nlpkg.sebis.cit.tum.de/nlp-taxonomy.owl#Text_Classification"/>
        <survey>https://arxiv.org/abs/2307.05553</survey>
        <survey>https://doi.org/10.1007/s10462-021-10068-2</survey>
        <nlp-taxonomy:level rdf:datatype="http://www.w3.org/2001/XMLSchema#integer">3</nlp-taxonomy:level>
        <dcterms:description xml:lang="en">Automatic Essay Scoring (AES) is the use of specialized computer programs to assign grades to essays written in an educational setting. It is a method of educational assessment and an application of natural language processing. Its objective is to classify a large set of textual entities into a small number of discrete categories, corresponding to the possible grades.</dcterms:description>
        <oboInOwl:hasSynonym xml:lang="en">AES</oboInOwl:hasSynonym>
        <oboInOwl:hasSynonym>Automated Essay Grading</oboInOwl:hasSynonym>
        <oboInOwl:hasSynonym>Automated Essay Scoring</oboInOwl:hasSynonym>
        <oboInOwl:hasSynonym xml:lang="en">Automatic Essay Grading</oboInOwl:hasSynonym>
        <rdfs:label xml:lang="en">Automatic Essay Scoring</rdfs:label>
    </owl:NamedIndividual>
    


    <!-- http://nlpkg.sebis.cit.tum.de/nlp-fos-hierarchy.owl#Automatic_Post-Editing -->

    <owl:NamedIndividual rdf:about="http://nlpkg.sebis.cit.tum.de/nlp-fos-hierarchy.owl#Automatic_Post-Editing">
        <rdf:type rdf:resource="http://nlpkg.sebis.cit.tum.de/nlp-fos-hierarchy.owl#Task"/>
        <rdf:type rdf:resource="http://nlpkg.sebis.cit.tum.de/nlp-taxonomy.owl#FieldOfStudy"/>
        <nlp-taxonomy:subFieldOf rdf:resource="http://nlpkg.sebis.cit.tum.de/nlp-taxonomy.owl#Machine_Translation"/>
        <survey>https://aclanthology.org/I17-1013</survey>
        <survey>https://doi.org/10.1007/s10590-020-09252-y</survey>
        <nlp-taxonomy:level rdf:datatype="http://www.w3.org/2001/XMLSchema#integer">3</nlp-taxonomy:level>
        <dcterms:description xml:lang="en">Automatic Post-Editing (APE) refers to the process of automatically correcting errors in machine-translated text by learning from human corrections.</dcterms:description>
        <oboInOwl:hasSynonym xml:lang="en">APE</oboInOwl:hasSynonym>
        <rdfs:label xml:lang="en">Automatic Post-Editing</rdfs:label>
    </owl:NamedIndividual>
    


    <!-- http://nlpkg.sebis.cit.tum.de/nlp-fos-hierarchy.owl#Back_Translation -->

    <owl:NamedIndividual rdf:about="http://nlpkg.sebis.cit.tum.de/nlp-fos-hierarchy.owl#Back_Translation">
        <rdf:type rdf:resource="http://nlpkg.sebis.cit.tum.de/nlp-fos-hierarchy.owl#Task"/>
        <rdf:type rdf:resource="http://nlpkg.sebis.cit.tum.de/nlp-taxonomy.owl#FieldOfStudy"/>
        <nlp-taxonomy:subFieldOf rdf:resource="http://nlpkg.sebis.cit.tum.de/nlp-fos-hierarchy.owl#Data_Augmentation"/>
        <survey>https://arxiv.org/abs/2102.09708</survey>
        <nlp-taxonomy:level rdf:datatype="http://www.w3.org/2001/XMLSchema#integer">4</nlp-taxonomy:level>
        <dcterms:description xml:lang="en">Back Translation involves translating a sentence from the source language to the target language, and then translating it back to the source language.</dcterms:description>
        <oboInOwl:hasSynonym xml:lang="en">Back-Translation</oboInOwl:hasSynonym>
        <oboInOwl:hasSynonym xml:lang="en">Backtranslation</oboInOwl:hasSynonym>
        <rdfs:label xml:lang="en">Back Translation</rdfs:label>
    </owl:NamedIndividual>
    


    <!-- http://nlpkg.sebis.cit.tum.de/nlp-fos-hierarchy.owl#Backdoor_Attacks -->

    <owl:NamedIndividual rdf:about="http://nlpkg.sebis.cit.tum.de/nlp-fos-hierarchy.owl#Backdoor_Attacks">
        <rdf:type rdf:resource="http://nlpkg.sebis.cit.tum.de/nlp-fos-hierarchy.owl#Task"/>
        <rdf:type rdf:resource="http://nlpkg.sebis.cit.tum.de/nlp-taxonomy.owl#FieldOfStudy"/>
        <nlp-taxonomy:subFieldOf rdf:resource="http://nlpkg.sebis.cit.tum.de/nlp-fos-hierarchy.owl#Privacy,_Security_&amp;_Safety_in_NLP"/>
        <nlp-taxonomy:superFieldOf rdf:resource="http://nlpkg.sebis.cit.tum.de/nlp-fos-hierarchy.owl#Backdoor_Defenses"/>
        <origin>https://arxiv.org/abs/1708.06733</origin>
        <survey>https://aclanthology.org/2021.acl-long.431</survey>
        <survey>https://arxiv.org/abs/2211.11958</survey>
        <nlp-taxonomy:level rdf:datatype="http://www.w3.org/2001/XMLSchema#integer">4</nlp-taxonomy:level>
        <dcterms:description xml:lang="en">Backdoor Attacks inject triggers into the specified models that make the backdoored model learn to predict badly on samples with triggers.</dcterms:description>
        <rdfs:label xml:lang="en">Backdoor Attacks</rdfs:label>
    </owl:NamedIndividual>
    


    <!-- http://nlpkg.sebis.cit.tum.de/nlp-fos-hierarchy.owl#Backdoor_Defenses -->

    <owl:NamedIndividual rdf:about="http://nlpkg.sebis.cit.tum.de/nlp-fos-hierarchy.owl#Backdoor_Defenses">
        <rdf:type rdf:resource="http://nlpkg.sebis.cit.tum.de/nlp-fos-hierarchy.owl#Task"/>
        <rdf:type rdf:resource="http://nlpkg.sebis.cit.tum.de/nlp-taxonomy.owl#FieldOfStudy"/>
        <nlp-taxonomy:subFieldOf rdf:resource="http://nlpkg.sebis.cit.tum.de/nlp-fos-hierarchy.owl#Backdoor_Attacks"/>
        <survey>https://arxiv.org/abs/2211.11958</survey>
        <nlp-taxonomy:level rdf:datatype="http://www.w3.org/2001/XMLSchema#integer">5</nlp-taxonomy:level>
        <dcterms:description xml:lang="en">Backdoor Defenses are effective against Backdoor Attacks that inject triggers into the specified models that make the backdoored model learn to predict badly on samples with triggers.</dcterms:description>
        <rdfs:label xml:lang="en">Backdoor Defenses</rdfs:label>
    </owl:NamedIndividual>
    


    <!-- http://nlpkg.sebis.cit.tum.de/nlp-fos-hierarchy.owl#Bag-of-Words -->

    <owl:NamedIndividual rdf:about="http://nlpkg.sebis.cit.tum.de/nlp-fos-hierarchy.owl#Bag-of-Words">
        <rdf:type rdf:resource="http://nlpkg.sebis.cit.tum.de/nlp-fos-hierarchy.owl#Method"/>
        <rdf:type rdf:resource="http://nlpkg.sebis.cit.tum.de/nlp-taxonomy.owl#FieldOfStudy"/>
        <nlp-taxonomy:subFieldOf rdf:resource="http://nlpkg.sebis.cit.tum.de/nlp-fos-hierarchy.owl#Sentence_Embeddings"/>
        <nlp-taxonomy:subFieldOf rdf:resource="http://nlpkg.sebis.cit.tum.de/nlp-fos-hierarchy.owl#Sparse_Embeddings"/>
        <nlp-taxonomy:subFieldOf rdf:resource="http://nlpkg.sebis.cit.tum.de/nlp-fos-hierarchy.owl#Static_Embeddings"/>
        <relevantInformation>https://en.wikipedia.org/wiki/Bag-of-words_model</relevantInformation>
        <nlp-taxonomy:level rdf:datatype="http://www.w3.org/2001/XMLSchema#integer">6</nlp-taxonomy:level>
        <dcterms:description xml:lang="en">Bag-of-Words (BoW) is a model where a text (such as a sentence or a document) is represented as the bag (multiset) of its words, disregarding grammar and even word order but keeping multiplicity.</dcterms:description>
        <oboInOwl:hasSynonym xml:lang="en">Bag of Words</oboInOwl:hasSynonym>
        <oboInOwl:hasSynonym xml:lang="en">BoW</oboInOwl:hasSynonym>
        <rdfs:label xml:lang="en">Bag-of-Words</rdfs:label>
    </owl:NamedIndividual>
    


    <!-- http://nlpkg.sebis.cit.tum.de/nlp-fos-hierarchy.owl#Bilingual_Lexicon_Induction -->

    <owl:NamedIndividual rdf:about="http://nlpkg.sebis.cit.tum.de/nlp-fos-hierarchy.owl#Bilingual_Lexicon_Induction">
        <rdf:type rdf:resource="http://nlpkg.sebis.cit.tum.de/nlp-fos-hierarchy.owl#Task"/>
        <rdf:type rdf:resource="http://nlpkg.sebis.cit.tum.de/nlp-taxonomy.owl#FieldOfStudy"/>
        <usedFor rdf:resource="http://nlpkg.sebis.cit.tum.de/nlp-fos-hierarchy.owl#Translation_Memory"/>
        <uses rdf:resource="http://nlpkg.sebis.cit.tum.de/nlp-fos-hierarchy.owl#Text_Embeddings"/>
        <nlp-taxonomy:subFieldOf rdf:resource="http://nlpkg.sebis.cit.tum.de/nlp-taxonomy.owl#Machine_Translation"/>
        <survey>https://aclanthology.org/J17-2001</survey>
        <nlp-taxonomy:level rdf:datatype="http://www.w3.org/2001/XMLSchema#integer">3</nlp-taxonomy:level>
        <dcterms:description xml:lang="en">Bilingual Lexicon Induction (BLI) refers to the process of automatically generating a bilingual dictionary or lexicon. This involves mapping words in one language to their equivalents in another language, typically using machine learning algorithms.</dcterms:description>
        <oboInOwl:hasSynonym xml:lang="en">BLI</oboInOwl:hasSynonym>
        <rdfs:label xml:lang="en">Bilingual Lexicon Induction</rdfs:label>
    </owl:NamedIndividual>
    


    <!-- http://nlpkg.sebis.cit.tum.de/nlp-fos-hierarchy.owl#Binary_Classification -->

    <owl:NamedIndividual rdf:about="http://nlpkg.sebis.cit.tum.de/nlp-fos-hierarchy.owl#Binary_Classification">
        <rdf:type rdf:resource="http://nlpkg.sebis.cit.tum.de/nlp-fos-hierarchy.owl#Task"/>
        <rdf:type rdf:resource="http://nlpkg.sebis.cit.tum.de/nlp-taxonomy.owl#FieldOfStudy"/>
        <nlp-taxonomy:subFieldOf rdf:resource="http://nlpkg.sebis.cit.tum.de/nlp-taxonomy.owl#Text_Classification"/>
        <nlp-taxonomy:level rdf:datatype="http://www.w3.org/2001/XMLSchema#integer">3</nlp-taxonomy:level>
        <dcterms:description xml:lang="en">Binary Classification is a type of classification that deals with only two classes or categories. It is used to predict which of two possible classes an instance of data belongs to. It&apos;s essentially a yes/no decision.</dcterms:description>
        <rdfs:label xml:lang="en">Binary Classification</rdfs:label>
    </owl:NamedIndividual>
    


    <!-- http://nlpkg.sebis.cit.tum.de/nlp-fos-hierarchy.owl#Chatbots -->

    <owl:NamedIndividual rdf:about="http://nlpkg.sebis.cit.tum.de/nlp-fos-hierarchy.owl#Chatbots">
        <rdf:type rdf:resource="http://nlpkg.sebis.cit.tum.de/nlp-fos-hierarchy.owl#OtherScientificField"/>
        <rdf:type rdf:resource="http://nlpkg.sebis.cit.tum.de/nlp-taxonomy.owl#FieldOfStudy"/>
        <uses rdf:resource="http://nlpkg.sebis.cit.tum.de/nlp-fos-hierarchy.owl#Controllable_Text_Generation"/>
        <uses rdf:resource="http://nlpkg.sebis.cit.tum.de/nlp-fos-hierarchy.owl#Instruction_Learning"/>
        <uses rdf:resource="http://nlpkg.sebis.cit.tum.de/nlp-fos-hierarchy.owl#Language_Model_Alignment"/>
        <nlp-taxonomy:subFieldOf rdf:resource="http://nlpkg.sebis.cit.tum.de/nlp-taxonomy.owl#Dialogue_Systems_&amp;_Conversational_Agents"/>
        <survey>https://arxiv.org/abs/1906.09774</survey>
        <survey>https://arxiv.org/abs/2105.11197</survey>
        <survey>https://arxiv.org/abs/2201.06657</survey>
        <nlp-taxonomy:level rdf:datatype="http://www.w3.org/2001/XMLSchema#integer">3</nlp-taxonomy:level>
        <dcterms:description xml:lang="en">Chatbots are designed to simulate human conversation, typically through text or voice interactions. They aim to understand and respond to user queries, providing automated assistance, information, or services in a conversational manner.</dcterms:description>
        <rdfs:label xml:lang="en">Chatbots</rdfs:label>
    </owl:NamedIndividual>
    


    <!-- http://nlpkg.sebis.cit.tum.de/nlp-fos-hierarchy.owl#Claim_Detection -->

    <owl:NamedIndividual rdf:about="http://nlpkg.sebis.cit.tum.de/nlp-fos-hierarchy.owl#Claim_Detection">
        <rdf:type rdf:resource="http://nlpkg.sebis.cit.tum.de/nlp-fos-hierarchy.owl#Task"/>
        <rdf:type rdf:resource="http://nlpkg.sebis.cit.tum.de/nlp-taxonomy.owl#FieldOfStudy"/>
        <nlp-taxonomy:subFieldOf rdf:resource="http://nlpkg.sebis.cit.tum.de/nlp-taxonomy.owl#Text_Classification"/>
        <nlp-taxonomy:subFieldOf rdf:resource="http://nlpkg.sebis.cit.tum.de/nlp-taxonomy.owl#Fact_&amp;_Claim_Verification"/>
        <nlp-taxonomy:superFieldOf rdf:resource="http://nlpkg.sebis.cit.tum.de/nlp-fos-hierarchy.owl#Rumor_Detection"/>
        <survey>https://aclanthology.org/2023.nodalida-1.1</survey>
        <nlp-taxonomy:level rdf:datatype="http://www.w3.org/2001/XMLSchema#integer">3</nlp-taxonomy:level>
        <dcterms:description xml:lang="en">Claim Detection refers to the process of identifying claims or assertions from a given text that should be selected for verification.</dcterms:description>
        <oboInOwl:hasSynonym xml:lang="en">Automated Claim Detection</oboInOwl:hasSynonym>
        <oboInOwl:hasSynonym xml:lang="en">Claim Classification</oboInOwl:hasSynonym>
        <oboInOwl:hasSynonym xml:lang="en">Claim Identification</oboInOwl:hasSynonym>
        <rdfs:label xml:lang="en">Claim Detection</rdfs:label>
    </owl:NamedIndividual>
    


    <!-- http://nlpkg.sebis.cit.tum.de/nlp-fos-hierarchy.owl#Claim_Verification -->

    <owl:NamedIndividual rdf:about="http://nlpkg.sebis.cit.tum.de/nlp-fos-hierarchy.owl#Claim_Verification">
        <rdf:type rdf:resource="http://nlpkg.sebis.cit.tum.de/nlp-fos-hierarchy.owl#Task"/>
        <rdf:type rdf:resource="http://nlpkg.sebis.cit.tum.de/nlp-taxonomy.owl#FieldOfStudy"/>
        <nlp-taxonomy:subFieldOf rdf:resource="http://nlpkg.sebis.cit.tum.de/nlp-fos-hierarchy.owl#Factual_Verification"/>
        <nlp-taxonomy:superFieldOf rdf:resource="http://nlpkg.sebis.cit.tum.de/nlp-fos-hierarchy.owl#Justification_Production"/>
        <nlp-taxonomy:superFieldOf rdf:resource="http://nlpkg.sebis.cit.tum.de/nlp-fos-hierarchy.owl#Verdict_Prediction"/>
        <nlp-taxonomy:level rdf:datatype="http://www.w3.org/2001/XMLSchema#integer">4</nlp-taxonomy:level>
        <dcterms:description xml:lang="en">Claim Verification is the task of to assessing the veracity of a claim based on available evidence.</dcterms:description>
        <rdfs:label xml:lang="en">Claim Verification</rdfs:label>
    </owl:NamedIndividual>
    


    <!-- http://nlpkg.sebis.cit.tum.de/nlp-fos-hierarchy.owl#Closed_Book_Question_Answering -->

    <owl:NamedIndividual rdf:about="http://nlpkg.sebis.cit.tum.de/nlp-fos-hierarchy.owl#Closed_Book_Question_Answering">
        <rdf:type rdf:resource="http://nlpkg.sebis.cit.tum.de/nlp-fos-hierarchy.owl#Task"/>
        <rdf:type rdf:resource="http://nlpkg.sebis.cit.tum.de/nlp-taxonomy.owl#FieldOfStudy"/>
        <nlp-taxonomy:subFieldOf rdf:resource="http://nlpkg.sebis.cit.tum.de/nlp-taxonomy.owl#Question_Answering"/>
        <nlp-taxonomy:level rdf:datatype="http://www.w3.org/2001/XMLSchema#integer">3</nlp-taxonomy:level>
        <dcterms:description xml:lang="en">Closed Book Question Answering is a task where a model answers questions based on the knowledge it has been trained on, without the ability to access or retrieve information from external sources or databases. The model relies solely on its internal knowledge learned during training.</dcterms:description>
        <oboInOwl:hasSynonym xml:lang="en">Closed Book QA</oboInOwl:hasSynonym>
        <oboInOwl:hasSynonym xml:lang="en">Closed-book QA</oboInOwl:hasSynonym>
        <oboInOwl:hasSynonym xml:lang="en">Closed-book Question Answering</oboInOwl:hasSynonym>
        <rdfs:label xml:lang="en">Closed Book Question Answering</rdfs:label>
    </owl:NamedIndividual>
    


    <!-- http://nlpkg.sebis.cit.tum.de/nlp-fos-hierarchy.owl#Closed_Domain_Question_Answering -->

    <owl:NamedIndividual rdf:about="http://nlpkg.sebis.cit.tum.de/nlp-fos-hierarchy.owl#Closed_Domain_Question_Answering">
        <rdf:type rdf:resource="http://nlpkg.sebis.cit.tum.de/nlp-fos-hierarchy.owl#Task"/>
        <rdf:type rdf:resource="http://nlpkg.sebis.cit.tum.de/nlp-taxonomy.owl#FieldOfStudy"/>
        <nlp-taxonomy:subFieldOf rdf:resource="http://nlpkg.sebis.cit.tum.de/nlp-taxonomy.owl#Question_Answering"/>
        <nlp-taxonomy:level rdf:datatype="http://www.w3.org/2001/XMLSchema#integer">3</nlp-taxonomy:level>
        <dcterms:description xml:lang="en">Closed Domain Question Answering refers to a type of question answering system where the system is expected to answer questions from a specific field or domain, such as medicine, law, or sports. The system is designed with a limited and fixed set of data, and it can only provide answers that are within this predefined data set.</dcterms:description>
        <oboInOwl:hasSynonym xml:lang="en">Closed Domain QA</oboInOwl:hasSynonym>
        <oboInOwl:hasSynonym xml:lang="en">Closed-domain QA</oboInOwl:hasSynonym>
        <oboInOwl:hasSynonym xml:lang="en">Closed-domain Question Answering</oboInOwl:hasSynonym>
        <rdfs:label xml:lang="en">Closed Domain Question Answering</rdfs:label>
    </owl:NamedIndividual>
    


    <!-- http://nlpkg.sebis.cit.tum.de/nlp-fos-hierarchy.owl#Code-specific_Language_Models -->

    <owl:NamedIndividual rdf:about="http://nlpkg.sebis.cit.tum.de/nlp-fos-hierarchy.owl#Code-specific_Language_Models">
        <rdf:type rdf:resource="http://nlpkg.sebis.cit.tum.de/nlp-fos-hierarchy.owl#OtherScientificField"/>
        <rdf:type rdf:resource="http://nlpkg.sebis.cit.tum.de/nlp-taxonomy.owl#FieldOfStudy"/>
        <nlp-taxonomy:subFieldOf rdf:resource="http://nlpkg.sebis.cit.tum.de/nlp-fos-hierarchy.owl#Multimodal_Language_Models"/>
        <nlp-taxonomy:subFieldOf rdf:resource="http://nlpkg.sebis.cit.tum.de/nlp-taxonomy.owl#Programming_Languages_In_NLP"/>
        <survey>https://arxiv.org/abs/2205.11739</survey>
        <survey>https://arxiv.org/abs/2212.10079</survey>
        <survey>https://arxiv.org/abs/2302.04026</survey>
        <survey>https://arxiv.org/abs/2305.19915</survey>
        <survey>https://arxiv.org/abs/2307.02503</survey>
        <survey>https://arxiv.org/abs/2308.10620</survey>
        <survey>https://arxiv.org/abs/2308.11396</survey>
        <survey>https://arxiv.org/abs/2310.17903</survey>
        <survey>https://arxiv.org/abs/2311.07989</survey>
        <survey>https://arxiv.org/abs/2401.00812</survey>
        <nlp-taxonomy:level rdf:datatype="http://www.w3.org/2001/XMLSchema#integer">3</nlp-taxonomy:level>
        <nlp-taxonomy:level rdf:datatype="http://www.w3.org/2001/XMLSchema#integer">4</nlp-taxonomy:level>
        <dcterms:description xml:lang="en">&quot;Code-specific Language Models&quot; refers to language models that are designed and fine-tuned specifically for tasks related to computer programming and software development. These models would aim to understand and generate code in various programming languages, assist with debugging, answer programming-related questions, and provide guidance on software development best practices.</dcterms:description>
        <oboInOwl:hasSynonym xml:lang="en">Code Language Models</oboInOwl:hasSynonym>
        <rdfs:label xml:lang="en">Code-specific Language Models</rdfs:label>
    </owl:NamedIndividual>
    


    <!-- http://nlpkg.sebis.cit.tum.de/nlp-fos-hierarchy.owl#Code_Search -->

    <owl:NamedIndividual rdf:about="http://nlpkg.sebis.cit.tum.de/nlp-fos-hierarchy.owl#Code_Search">
        <rdf:type rdf:resource="http://nlpkg.sebis.cit.tum.de/nlp-fos-hierarchy.owl#Task"/>
        <rdf:type rdf:resource="http://nlpkg.sebis.cit.tum.de/nlp-taxonomy.owl#FieldOfStudy"/>
        <nlp-taxonomy:subFieldOf rdf:resource="http://nlpkg.sebis.cit.tum.de/nlp-taxonomy.owl#Programming_Languages_In_NLP"/>
        <nlp-taxonomy:subFieldOf rdf:resource="http://nlpkg.sebis.cit.tum.de/nlp-taxonomy.owl#Semantic_Search"/>
        <nlp-taxonomy:level rdf:datatype="http://www.w3.org/2001/XMLSchema#integer">3</nlp-taxonomy:level>
        <dcterms:description xml:lang="en">The goal of Code Search is to retrieve code fragments from a large programming code corpus that most closely match a developer’s intent, which is expressed in natural language.</dcterms:description>
        <rdfs:label xml:lang="en">Code Search</rdfs:label>
    </owl:NamedIndividual>
    


    <!-- http://nlpkg.sebis.cit.tum.de/nlp-fos-hierarchy.owl#Code_Summarization -->

    <owl:NamedIndividual rdf:about="http://nlpkg.sebis.cit.tum.de/nlp-fos-hierarchy.owl#Code_Summarization">
        <rdf:type rdf:resource="http://nlpkg.sebis.cit.tum.de/nlp-fos-hierarchy.owl#Task"/>
        <rdf:type rdf:resource="http://nlpkg.sebis.cit.tum.de/nlp-taxonomy.owl#FieldOfStudy"/>
        <nlp-taxonomy:subFieldOf rdf:resource="http://nlpkg.sebis.cit.tum.de/nlp-taxonomy.owl#Programming_Languages_In_NLP"/>
        <nlp-taxonomy:subFieldOf rdf:resource="http://nlpkg.sebis.cit.tum.de/nlp-taxonomy.owl#Summarization"/>
        <nlp-taxonomy:level rdf:datatype="http://www.w3.org/2001/XMLSchema#integer">3</nlp-taxonomy:level>
        <dcterms:description xml:lang="en">Code Summarization is a task that tries to comprehend code and automatically generate descriptions directly from the source code.</dcterms:description>
        <oboInOwl:hasSynonym xml:lang="en">Code Summarisation</oboInOwl:hasSynonym>
        <oboInOwl:hasSynonym xml:lang="en">Code-to-Text</oboInOwl:hasSynonym>
        <oboInOwl:hasSynonym xml:lang="en">Code-to-Text Generation</oboInOwl:hasSynonym>
        <oboInOwl:hasSynonym xml:lang="en">Source Code Summarisation</oboInOwl:hasSynonym>
        <oboInOwl:hasSynonym xml:lang="en">Source Code Summarization</oboInOwl:hasSynonym>
        <rdfs:label xml:lang="en">Code Summarization</rdfs:label>
    </owl:NamedIndividual>
    


    <!-- http://nlpkg.sebis.cit.tum.de/nlp-fos-hierarchy.owl#Commonsense_Question_Answering -->

    <owl:NamedIndividual rdf:about="http://nlpkg.sebis.cit.tum.de/nlp-fos-hierarchy.owl#Commonsense_Question_Answering">
        <rdf:type rdf:resource="http://nlpkg.sebis.cit.tum.de/nlp-fos-hierarchy.owl#Task"/>
        <rdf:type rdf:resource="http://nlpkg.sebis.cit.tum.de/nlp-taxonomy.owl#FieldOfStudy"/>
        <usedFor rdf:resource="http://nlpkg.sebis.cit.tum.de/nlp-fos-hierarchy.owl#Open_Book_Question_Answering"/>
        <nlp-taxonomy:subFieldOf rdf:resource="http://nlpkg.sebis.cit.tum.de/nlp-taxonomy.owl#Commonsense_Reasoning"/>
        <nlp-taxonomy:subFieldOf rdf:resource="http://nlpkg.sebis.cit.tum.de/nlp-taxonomy.owl#Question_Answering"/>
        <nlp-taxonomy:level rdf:datatype="http://www.w3.org/2001/XMLSchema#integer">3</nlp-taxonomy:level>
        <dcterms:description xml:lang="en">Commonsense Question Answering refers to the ability of an AI system to answer questions that require understanding of everyday facts and general knowledge that are usually known to humans. It involves the application of commonsense reasoning, which is a key aspect of human intelligence, allowing the system to infer and predict answers even when not all information is explicitly stated in the text.</dcterms:description>
        <rdfs:label xml:lang="en">Commonsense Question Answering</rdfs:label>
    </owl:NamedIndividual>
    


    <!-- http://nlpkg.sebis.cit.tum.de/nlp-fos-hierarchy.owl#Compositional_Semantic_Parsing -->

    <owl:NamedIndividual rdf:about="http://nlpkg.sebis.cit.tum.de/nlp-fos-hierarchy.owl#Compositional_Semantic_Parsing">
        <rdf:type rdf:resource="http://nlpkg.sebis.cit.tum.de/nlp-fos-hierarchy.owl#Task"/>
        <rdf:type rdf:resource="http://nlpkg.sebis.cit.tum.de/nlp-taxonomy.owl#FieldOfStudy"/>
        <nlp-taxonomy:subFieldOf rdf:resource="http://nlpkg.sebis.cit.tum.de/nlp-taxonomy.owl#Semantic_Parsing"/>
        <nlp-taxonomy:level rdf:datatype="http://www.w3.org/2001/XMLSchema#integer">3</nlp-taxonomy:level>
        <dcterms:description xml:lang="en">Compositional Semantic Parsing refers to the process of converting natural language into a structured, machine-understandable representation. It involves understanding the meaning of individual words, the grammatical structure of the sentence, and how these elements combine to produce the overall meaning. The &quot;compositional&quot; aspect refers to the idea that the meaning of a sentence is built up from the meanings of its parts and the way they are syntactically combined.</dcterms:description>
        <oboInOwl:hasSynonym xml:lang="en">Deep Semantic Parsing</oboInOwl:hasSynonym>
        <rdfs:label xml:lang="en">Compositional Semantic Parsing</rdfs:label>
    </owl:NamedIndividual>
    


    <!-- http://nlpkg.sebis.cit.tum.de/nlp-fos-hierarchy.owl#Conditional_Random_Field -->

    <owl:NamedIndividual rdf:about="http://nlpkg.sebis.cit.tum.de/nlp-fos-hierarchy.owl#Conditional_Random_Field">
        <rdf:type rdf:resource="http://nlpkg.sebis.cit.tum.de/nlp-fos-hierarchy.owl#Method"/>
        <rdf:type rdf:resource="http://nlpkg.sebis.cit.tum.de/nlp-taxonomy.owl#FieldOfStudy"/>
        <usedFor rdf:resource="http://nlpkg.sebis.cit.tum.de/nlp-fos-hierarchy.owl#Sequence_Labeling"/>
        <nlp-taxonomy:subFieldOf rdf:resource="http://nlpkg.sebis.cit.tum.de/nlp-taxonomy.owl#Language_Models"/>
        <relevantInformation>https://towardsdatascience.com/conditional-random-fields-explained-e5b8256da776</relevantInformation>
        <nlp-taxonomy:level rdf:datatype="http://www.w3.org/2001/XMLSchema#integer">3</nlp-taxonomy:level>
        <dcterms:description xml:lang="en">Conditional Random Field (CRF) is a statistical modeling method often used for structured prediction. It&apos;s a type of discriminative undirected probabilistic graphical model that predicts a sequence of labels for a sequence of input samples. It&apos;s particularly used in tasks like named entity recognition, part of speech tagging, and text chunking where context is crucial to predict the output. Unlike other methods, CRF takes into account the context within the input sequence to make a prediction, which often results in improved accuracy.</dcterms:description>
        <oboInOwl:hasSynonym xml:lang="en">CRF</oboInOwl:hasSynonym>
        <rdfs:label xml:lang="en">Conditional Random Field</rdfs:label>
    </owl:NamedIndividual>
    


    <!-- http://nlpkg.sebis.cit.tum.de/nlp-fos-hierarchy.owl#Confounding_Bias -->

    <owl:NamedIndividual rdf:about="http://nlpkg.sebis.cit.tum.de/nlp-fos-hierarchy.owl#Confounding_Bias">
        <rdf:type rdf:resource="http://nlpkg.sebis.cit.tum.de/nlp-fos-hierarchy.owl#OtherScientificField"/>
        <rdf:type rdf:resource="http://nlpkg.sebis.cit.tum.de/nlp-taxonomy.owl#FieldOfStudy"/>
        <nlp-taxonomy:subFieldOf rdf:resource="http://nlpkg.sebis.cit.tum.de/nlp-fos-hierarchy.owl#Biases_&amp;_Fairness_in_NLP"/>
        <nlp-taxonomy:level rdf:datatype="http://www.w3.org/2001/XMLSchema#integer">4</nlp-taxonomy:level>
        <dcterms:description xml:lang="en">Confounding Bias refers to the distortion that occurs when the effect of multiple variables on a response is mixed up. This bias can lead to incorrect conclusions about the relationships between variables. For example, a model might incorrectly attribute an effect to one variable when it is actually caused by another variable that wasn&apos;t accounted for. This can be particularly problematic in NLP when trying to understand the influence of specific words or phrases on the outcome of a language model.</dcterms:description>
        <rdfs:label xml:lang="en">Confounding Bias</rdfs:label>
    </owl:NamedIndividual>
    


    <!-- http://nlpkg.sebis.cit.tum.de/nlp-fos-hierarchy.owl#Constituency_Parse_Tree -->

    <owl:NamedIndividual rdf:about="http://nlpkg.sebis.cit.tum.de/nlp-fos-hierarchy.owl#Constituency_Parse_Tree">
        <rdf:type rdf:resource="http://nlpkg.sebis.cit.tum.de/nlp-fos-hierarchy.owl#DataStructure"/>
        <rdf:type rdf:resource="http://nlpkg.sebis.cit.tum.de/nlp-taxonomy.owl#FieldOfStudy"/>
        <nlp-taxonomy:subFieldOf rdf:resource="http://nlpkg.sebis.cit.tum.de/nlp-fos-hierarchy.owl#Constituency_Parsing"/>
        <nlp-taxonomy:subFieldOf rdf:resource="http://nlpkg.sebis.cit.tum.de/nlp-fos-hierarchy.owl#Constituency_Tree"/>
        <nlp-taxonomy:subFieldOf rdf:resource="http://nlpkg.sebis.cit.tum.de/nlp-fos-hierarchy.owl#Parse_Tree"/>
        <nlp-taxonomy:level rdf:datatype="http://www.w3.org/2001/XMLSchema#integer">4</nlp-taxonomy:level>
        <nlp-taxonomy:level rdf:datatype="http://www.w3.org/2001/XMLSchema#integer">6</nlp-taxonomy:level>
        <dcterms:description xml:lang="en">Constituency Parse Tree is a tree representation of the syntactic structure of a sentence according to constituency grammar rules. Each node of the tree represents a constituent (word or group of words) and the edges represent the grammatical relationship between them. The root of the tree represents the entire sentence.</dcterms:description>
        <rdfs:label xml:lang="en">Constituency Parse Tree</rdfs:label>
    </owl:NamedIndividual>
    


    <!-- http://nlpkg.sebis.cit.tum.de/nlp-fos-hierarchy.owl#Constituency_Parsing -->

    <owl:NamedIndividual rdf:about="http://nlpkg.sebis.cit.tum.de/nlp-fos-hierarchy.owl#Constituency_Parsing">
        <rdf:type rdf:resource="http://nlpkg.sebis.cit.tum.de/nlp-fos-hierarchy.owl#Task"/>
        <rdf:type rdf:resource="http://nlpkg.sebis.cit.tum.de/nlp-taxonomy.owl#FieldOfStudy"/>
        <nlp-taxonomy:subFieldOf rdf:resource="http://nlpkg.sebis.cit.tum.de/nlp-taxonomy.owl#Syntactic_Parsing"/>
        <nlp-taxonomy:superFieldOf rdf:resource="http://nlpkg.sebis.cit.tum.de/nlp-fos-hierarchy.owl#Constituency_Parse_Tree"/>
        <relevantInformation>https://web.stanford.edu/~jurafsky/slp3/17.pdf</relevantInformation>
        <relevantInformation>https://web.stanford.edu/~jurafsky/slp3/C.pdf</relevantInformation>
        <survey>https://arxiv.org/abs/2006.11056</survey>
        <nlp-taxonomy:level rdf:datatype="http://www.w3.org/2001/XMLSchema#integer">3</nlp-taxonomy:level>
        <dcterms:description xml:lang="en">Constituency Parsing is the task of analyzing the grammatical structure of a sentence by dividing it into hierarchical, nested phrases or constituents. It aims to identify the syntactic relationships between words and group them into parts of speech, such as noun phrases and verb phrases, to create a parse tree that represents the sentence&apos;s grammatical structure.</dcterms:description>
        <rdfs:label xml:lang="en">Constituency Parsing</rdfs:label>
    </owl:NamedIndividual>
    


    <!-- http://nlpkg.sebis.cit.tum.de/nlp-fos-hierarchy.owl#Constituency_Tree -->

    <owl:NamedIndividual rdf:about="http://nlpkg.sebis.cit.tum.de/nlp-fos-hierarchy.owl#Constituency_Tree">
        <rdf:type rdf:resource="http://nlpkg.sebis.cit.tum.de/nlp-fos-hierarchy.owl#DataStructure"/>
        <rdf:type rdf:resource="http://nlpkg.sebis.cit.tum.de/nlp-taxonomy.owl#FieldOfStudy"/>
        <nlp-taxonomy:subFieldOf rdf:resource="http://nlpkg.sebis.cit.tum.de/nlp-fos-hierarchy.owl#Tree"/>
        <nlp-taxonomy:superFieldOf rdf:resource="http://nlpkg.sebis.cit.tum.de/nlp-fos-hierarchy.owl#Constituency_Parse_Tree"/>
        <nlp-taxonomy:level rdf:datatype="http://www.w3.org/2001/XMLSchema#integer">5</nlp-taxonomy:level>
        <dcterms:description xml:lang="en">Constituency Trees are graphical representations that depict the organization and hierarchical structure of sentences. They are based on the syntax of the language and show how a sentence is divided into its constituent parts (like phrases or individual words), and how these parts are related to each other.</dcterms:description>
        <rdfs:label xml:lang="en">Constituency Tree</rdfs:label>
    </owl:NamedIndividual>
    


    <!-- http://nlpkg.sebis.cit.tum.de/nlp-fos-hierarchy.owl#Construction_Grammar -->

    <owl:NamedIndividual rdf:about="http://nlpkg.sebis.cit.tum.de/nlp-fos-hierarchy.owl#Construction_Grammar">
        <rdf:type rdf:resource="http://nlpkg.sebis.cit.tum.de/nlp-fos-hierarchy.owl#OtherScientificField"/>
        <rdf:type rdf:resource="http://nlpkg.sebis.cit.tum.de/nlp-taxonomy.owl#FieldOfStudy"/>
        <nlp-taxonomy:subFieldOf rdf:resource="http://nlpkg.sebis.cit.tum.de/nlp-taxonomy.owl#Linguistic_Theories"/>
        <survey>https://aclanthology.org/2023.cxgsnlp-1.1</survey>
        <nlp-taxonomy:level rdf:datatype="http://www.w3.org/2001/XMLSchema#integer">3</nlp-taxonomy:level>
        <dcterms:description xml:lang="en">Construction Grammar (CxG) is a usage-based approach to language which views grammatical structure as a set of form-meaning mappings called a constructicon. From this usage-based perspective, a construction could belong in the grammar either (i) because it is sufficiently entrenched (i.e., frequent) that it is stored and processed as a unique item or (ii) because it is sufficiently irregular (i.e., idiomatic) that it requires a unique grammatical description (Goldberg, 2006). The advantage of CxG from this perspective is that it focuses on explaining the creativity, the flexibility, and the idiosyncrasy of actual language use in real-world settings</dcterms:description>
        <oboInOwl:hasSynonym xml:lang="en">CxG</oboInOwl:hasSynonym>
        <rdfs:label xml:lang="en">Construction Grammar</rdfs:label>
    </owl:NamedIndividual>
    


    <!-- http://nlpkg.sebis.cit.tum.de/nlp-fos-hierarchy.owl#Contextualized_Embeddings -->

    <owl:NamedIndividual rdf:about="http://nlpkg.sebis.cit.tum.de/nlp-fos-hierarchy.owl#Contextualized_Embeddings">
        <rdf:type rdf:resource="http://nlpkg.sebis.cit.tum.de/nlp-fos-hierarchy.owl#DataStructure"/>
        <rdf:type rdf:resource="http://nlpkg.sebis.cit.tum.de/nlp-taxonomy.owl#FieldOfStudy"/>
        <nlp-taxonomy:subFieldOf rdf:resource="http://nlpkg.sebis.cit.tum.de/nlp-fos-hierarchy.owl#Text_Embeddings"/>
        <nlp-taxonomy:superFieldOf rdf:resource="http://nlpkg.sebis.cit.tum.de/nlp-fos-hierarchy.owl#Sentence-Transformers"/>
        <survey>https://aclanthology.org/W19-3805</survey>
        <survey>https://arxiv.org/abs/2003.07278</survey>
        <nlp-taxonomy:level rdf:datatype="http://www.w3.org/2001/XMLSchema#integer">5</nlp-taxonomy:level>
        <dcterms:description xml:lang="en">Contextualized Embeddings refer to the representation of words that capture their meanings based on the surrounding context. Unlike traditional embeddings that assign a fixed vector to each word regardless of its context, contextualized embeddings assign different vectors to the same word depending on its usage in a sentence. This allows the model to better understand nuances in language.</dcterms:description>
        <oboInOwl:hasSynonym xml:lang="en">Contextual Embeddings</oboInOwl:hasSynonym>
        <rdfs:label xml:lang="en">Contextualized Embeddings</rdfs:label>
    </owl:NamedIndividual>
    


    <!-- http://nlpkg.sebis.cit.tum.de/nlp-fos-hierarchy.owl#Controllable_Text_Generation -->

    <owl:NamedIndividual rdf:about="http://nlpkg.sebis.cit.tum.de/nlp-fos-hierarchy.owl#Controllable_Text_Generation">
        <rdf:type rdf:resource="http://nlpkg.sebis.cit.tum.de/nlp-fos-hierarchy.owl#Task"/>
        <rdf:type rdf:resource="http://nlpkg.sebis.cit.tum.de/nlp-taxonomy.owl#FieldOfStudy"/>
        <usedFor rdf:resource="http://nlpkg.sebis.cit.tum.de/nlp-fos-hierarchy.owl#Chatbots"/>
        <usedFor rdf:resource="http://nlpkg.sebis.cit.tum.de/nlp-fos-hierarchy.owl#Instruction_Learning"/>
        <usedFor rdf:resource="http://nlpkg.sebis.cit.tum.de/nlp-fos-hierarchy.owl#Language_Model_Alignment"/>
        <usedFor rdf:resource="http://nlpkg.sebis.cit.tum.de/nlp-taxonomy.owl#Paraphrasing"/>
        <nlp-taxonomy:subFieldOf rdf:resource="http://nlpkg.sebis.cit.tum.de/nlp-taxonomy.owl#Text_Generation"/>
        <nlp-taxonomy:superFieldOf rdf:resource="http://nlpkg.sebis.cit.tum.de/nlp-fos-hierarchy.owl#Story_Generation"/>
        <survey>https://aclanthology.org/2020.coling-main.1</survey>
        <survey>https://aclanthology.org/2020.findings-emnlp.301</survey>
        <survey>https://arxiv.org/abs/2201.05337</survey>
        <survey>https://arxiv.org/abs/2310.14542</survey>
        <survey>https://arxiv.org/abs/2310.16343</survey>
        <nlp-taxonomy:level rdf:datatype="http://www.w3.org/2001/XMLSchema#integer">2</nlp-taxonomy:level>
        <dcterms:description xml:lang="en">Controllable Text Generation (CTG) is the task of generating natural sentences whose attributes can be controlled. The attributes to control can range from being stylistic such politeness, sentiment, formality, etc.; demographic attributes of the person writing the text such as gender, age, etc.; content such as information, keywords, entities, etc.; ordering of information, events, like plot summaries etc. It is regarded as crucial for the development of advanced text generation technologies that better meet the specific constraints in practical applications.</dcterms:description>
        <oboInOwl:hasSynonym xml:lang="en">CTG</oboInOwl:hasSynonym>
        <oboInOwl:hasSynonym>Constrained Text Generation</oboInOwl:hasSynonym>
        <oboInOwl:hasSynonym>Controlled Generation</oboInOwl:hasSynonym>
        <rdfs:label xml:lang="en">Controllable Text Generation</rdfs:label>
    </owl:NamedIndividual>
    


    <!-- http://nlpkg.sebis.cit.tum.de/nlp-fos-hierarchy.owl#Conversational_Machine_Comprehension -->

    <owl:NamedIndividual rdf:about="http://nlpkg.sebis.cit.tum.de/nlp-fos-hierarchy.owl#Conversational_Machine_Comprehension">
        <rdf:type rdf:resource="http://nlpkg.sebis.cit.tum.de/nlp-fos-hierarchy.owl#Task"/>
        <rdf:type rdf:resource="http://nlpkg.sebis.cit.tum.de/nlp-taxonomy.owl#FieldOfStudy"/>
        <nlp-taxonomy:subFieldOf rdf:resource="http://nlpkg.sebis.cit.tum.de/nlp-fos-hierarchy.owl#Conversational_Question_Answering"/>
        <nlp-taxonomy:subFieldOf rdf:resource="http://nlpkg.sebis.cit.tum.de/nlp-taxonomy.owl#Machine_Reading_Comprehension"/>
        <survey>https://aclanthology.org/2020.coling-main.247</survey>
        <nlp-taxonomy:level rdf:datatype="http://www.w3.org/2001/XMLSchema#integer">3</nlp-taxonomy:level>
        <nlp-taxonomy:level rdf:datatype="http://www.w3.org/2001/XMLSchema#integer">4</nlp-taxonomy:level>
        <dcterms:description xml:lang="en">Conversational Machine Comprehension (CMC) expects the machine to understand an open-domain natural language text and thereafter engage in a multi-turn conversation to answer questions related to the text.</dcterms:description>
        <oboInOwl:hasSynonym xml:lang="en">CMC</oboInOwl:hasSynonym>
        <rdfs:label xml:lang="en">Conversational Machine Comprehension</rdfs:label>
    </owl:NamedIndividual>
    


    <!-- http://nlpkg.sebis.cit.tum.de/nlp-fos-hierarchy.owl#Conversational_Question_Answering -->

    <owl:NamedIndividual rdf:about="http://nlpkg.sebis.cit.tum.de/nlp-fos-hierarchy.owl#Conversational_Question_Answering">
        <rdf:type rdf:resource="http://nlpkg.sebis.cit.tum.de/nlp-fos-hierarchy.owl#Task"/>
        <rdf:type rdf:resource="http://nlpkg.sebis.cit.tum.de/nlp-taxonomy.owl#FieldOfStudy"/>
        <nlp-taxonomy:subFieldOf rdf:resource="http://nlpkg.sebis.cit.tum.de/nlp-taxonomy.owl#Question_Answering"/>
        <nlp-taxonomy:subFieldOf rdf:resource="http://nlpkg.sebis.cit.tum.de/nlp-taxonomy.owl#Dialogue_Systems_&amp;_Conversational_Agents"/>
        <nlp-taxonomy:superFieldOf rdf:resource="http://nlpkg.sebis.cit.tum.de/nlp-fos-hierarchy.owl#Conversational_Machine_Comprehension"/>
        <survey>https://aclanthology.org/W17-5522</survey>
        <survey>https://arxiv.org/abs/2106.00874</survey>
        <nlp-taxonomy:level rdf:datatype="http://www.w3.org/2001/XMLSchema#integer">3</nlp-taxonomy:level>
        <dcterms:description xml:lang="en">Conversational Question Answering (CQA) is a natural language processing task that involves answering a series of questions within the context of an ongoing conversation or dialogue. It goes beyond traditional question-answering systems by considering the conversational history and previous responses to provide more contextually relevant and coherent answers. CQA systems aim to understand the nuances of a conversation and provide accurate responses that take into account the conversation&apos;s evolving context.</dcterms:description>
        <oboInOwl:hasSynonym xml:lang="en">CQA</oboInOwl:hasSynonym>
        <rdfs:label xml:lang="en">Conversational Question Answering</rdfs:label>
    </owl:NamedIndividual>
    


    <!-- http://nlpkg.sebis.cit.tum.de/nlp-fos-hierarchy.owl#Curriculum_Learning -->

    <owl:NamedIndividual rdf:about="http://nlpkg.sebis.cit.tum.de/nlp-fos-hierarchy.owl#Curriculum_Learning">
        <rdf:type rdf:resource="http://nlpkg.sebis.cit.tum.de/nlp-fos-hierarchy.owl#Task"/>
        <rdf:type rdf:resource="http://nlpkg.sebis.cit.tum.de/nlp-taxonomy.owl#FieldOfStudy"/>
        <nlp-taxonomy:subFieldOf rdf:resource="http://nlpkg.sebis.cit.tum.de/nlp-taxonomy.owl#Language_Models"/>
        <nlp-taxonomy:subFieldOf rdf:resource="http://nlpkg.sebis.cit.tum.de/nlp-taxonomy.owl#Green_&amp;_Sustainable_NLP"/>
        <survey>https://arxiv.org/abs/2010.13166</survey>
        <survey>https://arxiv.org/abs/2101.10382</survey>
        <nlp-taxonomy:level rdf:datatype="http://www.w3.org/2001/XMLSchema#integer">3</nlp-taxonomy:level>
        <dcterms:description xml:lang="en">Curriculum Learning (CL) is a training strategy where the model learns from easy examples first and gradually from more complex ones, similar to how humans learn. This approach is based on the idea that a model can perform better if it first learns to predict simpler patterns before attempting to understand more complex structures. It&apos;s like a learning schedule or syllabus for the model.</dcterms:description>
        <oboInOwl:hasSynonym xml:lang="en">CL</oboInOwl:hasSynonym>
        <rdfs:label xml:lang="en">Curriculum Learning</rdfs:label>
    </owl:NamedIndividual>
    


    <!-- http://nlpkg.sebis.cit.tum.de/nlp-fos-hierarchy.owl#Data_Augmentation -->

    <owl:NamedIndividual rdf:about="http://nlpkg.sebis.cit.tum.de/nlp-fos-hierarchy.owl#Data_Augmentation">
        <rdf:type rdf:resource="http://nlpkg.sebis.cit.tum.de/nlp-fos-hierarchy.owl#Task"/>
        <rdf:type rdf:resource="http://nlpkg.sebis.cit.tum.de/nlp-taxonomy.owl#FieldOfStudy"/>
        <nlp-taxonomy:subFieldOf rdf:resource="http://nlpkg.sebis.cit.tum.de/nlp-taxonomy.owl#Low-Resource_NLP"/>
        <nlp-taxonomy:superFieldOf rdf:resource="http://nlpkg.sebis.cit.tum.de/nlp-fos-hierarchy.owl#Back_Translation"/>
        <nlp-taxonomy:superFieldOf rdf:resource="http://nlpkg.sebis.cit.tum.de/nlp-fos-hierarchy.owl#Lexical_Substitution"/>
        <code>https://github.com/QData/TextAttack</code>
        <code>https://github.com/makcedward/nlpaug</code>
        <relevantInformation>https://amitness.com/2020/05/data-augmentation-for-nlp/</relevantInformation>
        <survey>https://aclanthology.org/2021.findings-acl.84</survey>
        <survey>https://aclanthology.org/2023.tacl-1.12</survey>
        <survey>https://arxiv.org/abs/2107.03158</survey>
        <survey>https://arxiv.org/abs/2110.01852</survey>
        <survey>https://arxiv.org/abs/2212.10888</survey>
        <survey>https://arxiv.org/abs/2305.19915</survey>
        <nlp-taxonomy:level rdf:datatype="http://www.w3.org/2001/XMLSchema#integer">3</nlp-taxonomy:level>
        <dcterms:description xml:lang="en">Data Augmentation is a strategy used to increase the amount and diversity of data. It involves creating new synthetic data by slightly altering the existing data, such as changing the word order, replacing words with their synonyms, or translating sentences to another language and then back to the original language. This technique helps improve the performance and robustness of NLP models by providing more varied training data.</dcterms:description>
        <rdfs:label xml:lang="en">Data Augmentation</rdfs:label>
    </owl:NamedIndividual>
    


    <!-- http://nlpkg.sebis.cit.tum.de/nlp-fos-hierarchy.owl#De-Identification -->

    <owl:NamedIndividual rdf:about="http://nlpkg.sebis.cit.tum.de/nlp-fos-hierarchy.owl#De-Identification">
        <rdf:type rdf:resource="http://nlpkg.sebis.cit.tum.de/nlp-fos-hierarchy.owl#Task"/>
        <rdf:type rdf:resource="http://nlpkg.sebis.cit.tum.de/nlp-taxonomy.owl#FieldOfStudy"/>
        <nlp-taxonomy:subFieldOf rdf:resource="http://nlpkg.sebis.cit.tum.de/nlp-fos-hierarchy.owl#Privacy,_Security_&amp;_Safety_in_NLP"/>
        <nlp-taxonomy:superFieldOf rdf:resource="http://nlpkg.sebis.cit.tum.de/nlp-fos-hierarchy.owl#Anonymization"/>
        <nlp-taxonomy:superFieldOf rdf:resource="http://nlpkg.sebis.cit.tum.de/nlp-fos-hierarchy.owl#Pseudonymization"/>
        <survey>https://aclanthology.org/2023.nodalida-1.2</survey>
        <nlp-taxonomy:level rdf:datatype="http://www.w3.org/2001/XMLSchema#integer">4</nlp-taxonomy:level>
        <dcterms:description xml:lang="en">De-Identification is the task of hiding personally identifiable information (PII) in a dataset to protect the privacy of individuals.</dcterms:description>
        <rdfs:label xml:lang="en">De-Identification</rdfs:label>
    </owl:NamedIndividual>
    


    <!-- http://nlpkg.sebis.cit.tum.de/nlp-fos-hierarchy.owl#Debiasing -->

    <owl:NamedIndividual rdf:about="http://nlpkg.sebis.cit.tum.de/nlp-fos-hierarchy.owl#Debiasing">
        <rdf:type rdf:resource="http://nlpkg.sebis.cit.tum.de/nlp-fos-hierarchy.owl#Task"/>
        <rdf:type rdf:resource="http://nlpkg.sebis.cit.tum.de/nlp-taxonomy.owl#FieldOfStudy"/>
        <nlp-taxonomy:subFieldOf rdf:resource="http://nlpkg.sebis.cit.tum.de/nlp-fos-hierarchy.owl#Biases_&amp;_Fairness_in_NLP"/>
        <survey>https://aclanthology.org/2021.emnlp-main.193</survey>
        <survey>https://aclanthology.org/2022.acl-long.132</survey>
        <survey>https://arxiv.org/abs/2211.05617</survey>
        <nlp-taxonomy:level rdf:datatype="http://www.w3.org/2001/XMLSchema#integer">4</nlp-taxonomy:level>
        <dcterms:description xml:lang="en">Debiasing refers to the process of reducing or eliminating biases that may exist in the data used for machine learning or AI models. Debiasing techniques aim to ensure that the AI models treat all inputs fairly and do not perpetuate harmful stereotypes or prejudices.</dcterms:description>
        <rdfs:label xml:lang="en">Debiasing</rdfs:label>
    </owl:NamedIndividual>
    


    <!-- http://nlpkg.sebis.cit.tum.de/nlp-fos-hierarchy.owl#Decision_Tree -->

    <owl:NamedIndividual rdf:about="http://nlpkg.sebis.cit.tum.de/nlp-fos-hierarchy.owl#Decision_Tree">
        <rdf:type rdf:resource="http://nlpkg.sebis.cit.tum.de/nlp-fos-hierarchy.owl#Method"/>
        <rdf:type rdf:resource="http://nlpkg.sebis.cit.tum.de/nlp-taxonomy.owl#FieldOfStudy"/>
        <nlp-taxonomy:subFieldOf rdf:resource="http://nlpkg.sebis.cit.tum.de/nlp-taxonomy.owl#Text_Classification"/>
        <code>https://scikit-learn.org/stable/modules/tree.html#tree</code>
        <nlp-taxonomy:level rdf:datatype="http://www.w3.org/2001/XMLSchema#integer">3</nlp-taxonomy:level>
        <nlp-taxonomy:level rdf:datatype="http://www.w3.org/2001/XMLSchema#integer">4</nlp-taxonomy:level>
        <dcterms:description xml:lang="en">Decision Trees are machine learning models used for making predictions based on certain decision rules. They use a tree-like model of decisions where each internal node represents a &quot;test&quot; on an attribute, each branch represents the outcome of the test, and each leaf node represents a class label (decision taken after computing all attributes).</dcterms:description>
        <oboInOwl:hasSynonym xml:lang="en">DTLA</oboInOwl:hasSynonym>
        <oboInOwl:hasSynonym xml:lang="en">Decision Tree Learning Algorithmus</oboInOwl:hasSynonym>
        <rdfs:label xml:lang="en">Decision Tree</rdfs:label>
    </owl:NamedIndividual>
    


    <!-- http://nlpkg.sebis.cit.tum.de/nlp-fos-hierarchy.owl#Decoding -->

    <owl:NamedIndividual rdf:about="http://nlpkg.sebis.cit.tum.de/nlp-fos-hierarchy.owl#Decoding">
        <rdf:type rdf:resource="http://nlpkg.sebis.cit.tum.de/nlp-fos-hierarchy.owl#Task"/>
        <rdf:type rdf:resource="http://nlpkg.sebis.cit.tum.de/nlp-taxonomy.owl#FieldOfStudy"/>
        <nlp-taxonomy:subFieldOf rdf:resource="http://nlpkg.sebis.cit.tum.de/nlp-fos-hierarchy.owl#Language_Model_Mechanisms"/>
        <relevantInformation>https://medium.com/towards-data-science/decoding-strategies-in-large-language-models-9733a8f70539</relevantInformation>
        <nlp-taxonomy:level rdf:datatype="http://www.w3.org/2001/XMLSchema#integer">4</nlp-taxonomy:level>
        <dcterms:description xml:lang="en">Decoding refers to the methods used to translate the output of a language model (usually in the form of encoded tokens or probabilities) into a human-readable text. These strategies determine how the model selects the next word in a sequence, balancing between diversity and accuracy.</dcterms:description>
        <rdfs:label xml:lang="en">Decoding</rdfs:label>
    </owl:NamedIndividual>
    


    <!-- http://nlpkg.sebis.cit.tum.de/nlp-fos-hierarchy.owl#Dense_Document_Retrieval -->

    <owl:NamedIndividual rdf:about="http://nlpkg.sebis.cit.tum.de/nlp-fos-hierarchy.owl#Dense_Document_Retrieval">
        <rdf:type rdf:resource="http://nlpkg.sebis.cit.tum.de/nlp-fos-hierarchy.owl#Task"/>
        <rdf:type rdf:resource="http://nlpkg.sebis.cit.tum.de/nlp-taxonomy.owl#FieldOfStudy"/>
        <uses rdf:resource="http://nlpkg.sebis.cit.tum.de/nlp-fos-hierarchy.owl#Dense_Embeddings"/>
        <nlp-taxonomy:subFieldOf rdf:resource="http://nlpkg.sebis.cit.tum.de/nlp-taxonomy.owl#Document_Retrieval"/>
        <survey>https://arxiv.org/abs/2211.14876</survey>
        <nlp-taxonomy:level rdf:datatype="http://www.w3.org/2001/XMLSchema#integer">3</nlp-taxonomy:level>
        <dcterms:description xml:lang="en">Dense Document Retrieval refers to the process of retrieving relevant documents from a large corpus based on semantic similarity rather than keyword matching. It uses dense vector representations (embeddings) of documents and queries to calculate their similarity. This approach allows for a more nuanced understanding of the content, as it can capture semantic relationships between words and phrases, and can retrieve relevant documents even if they do not share exact keywords with the query.</dcterms:description>
        <oboInOwl:hasSynonym xml:lang="en">Dense Retrieval</oboInOwl:hasSynonym>
        <rdfs:label xml:lang="en">Dense Document Retrieval</rdfs:label>
    </owl:NamedIndividual>
    


    <!-- http://nlpkg.sebis.cit.tum.de/nlp-fos-hierarchy.owl#Dense_Embeddings -->

    <owl:NamedIndividual rdf:about="http://nlpkg.sebis.cit.tum.de/nlp-fos-hierarchy.owl#Dense_Embeddings">
        <rdf:type rdf:resource="http://nlpkg.sebis.cit.tum.de/nlp-fos-hierarchy.owl#DataStructure"/>
        <rdf:type rdf:resource="http://nlpkg.sebis.cit.tum.de/nlp-taxonomy.owl#FieldOfStudy"/>
        <usedFor rdf:resource="http://nlpkg.sebis.cit.tum.de/nlp-fos-hierarchy.owl#Dense_Document_Retrieval"/>
        <usedFor rdf:resource="http://nlpkg.sebis.cit.tum.de/nlp-fos-hierarchy.owl#Dense_Passage_Retrieval"/>
        <nlp-taxonomy:subFieldOf rdf:resource="http://nlpkg.sebis.cit.tum.de/nlp-fos-hierarchy.owl#Text_Embeddings"/>
        <nlp-taxonomy:superFieldOf rdf:resource="http://nlpkg.sebis.cit.tum.de/nlp-fos-hierarchy.owl#Sentence-Transformers"/>
        <survey>https://arxiv.org/abs/1805.04032</survey>
        <nlp-taxonomy:level rdf:datatype="http://www.w3.org/2001/XMLSchema#integer">5</nlp-taxonomy:level>
        <dcterms:description xml:lang="en">Dense Embeddings refer to the representation of words or phrases in a continuous vector space. Each word or phrase is mapped to a vector of real numbers, which capture the semantic meaning and context of the word. These vectors are called &quot;dense&quot; because they are usually high-dimensional and contain non-zero values, as opposed to sparse vectors which contain many zeros. Dense embeddings are used to reduce the dimensionality of text data and are a key part of many NLP tasks.</dcterms:description>
        <oboInOwl:hasSynonym xml:lang="en">Distributed Representations</oboInOwl:hasSynonym>
        <rdfs:label xml:lang="en">Dense Embeddings</rdfs:label>
    </owl:NamedIndividual>
    


    <!-- http://nlpkg.sebis.cit.tum.de/nlp-fos-hierarchy.owl#Dense_Passage_Retrieval -->

    <owl:NamedIndividual rdf:about="http://nlpkg.sebis.cit.tum.de/nlp-fos-hierarchy.owl#Dense_Passage_Retrieval">
        <rdf:type rdf:resource="http://nlpkg.sebis.cit.tum.de/nlp-fos-hierarchy.owl#Task"/>
        <rdf:type rdf:resource="http://nlpkg.sebis.cit.tum.de/nlp-taxonomy.owl#FieldOfStudy"/>
        <uses rdf:resource="http://nlpkg.sebis.cit.tum.de/nlp-fos-hierarchy.owl#Dense_Embeddings"/>
        <nlp-taxonomy:subFieldOf rdf:resource="http://nlpkg.sebis.cit.tum.de/nlp-taxonomy.owl#Passage_Retrieval"/>
        <origin>https://aclanthology.org/2020.emnlp-main.550</origin>
        <relevantInformation>https://huggingface.co/docs/transformers/model_doc/dpr</relevantInformation>
        <survey>https://arxiv.org/abs/2211.14876</survey>
        <nlp-taxonomy:level rdf:datatype="http://www.w3.org/2001/XMLSchema#integer">3</nlp-taxonomy:level>
        <dcterms:description xml:lang="en">Dense Passage Retrieval (DPR) is a method for retrieving relevant information from a large text corpus. Unlike traditional methods that rely on sparse lexical matches, DPR uses dense vector representations of text passages and queries to find relevant information. This approach allows for more nuanced understanding of the text, as it can capture semantic similarities beyond exact word matches.</dcterms:description>
        <oboInOwl:hasSynonym xml:lang="en">DPR</oboInOwl:hasSynonym>
        <oboInOwl:hasSynonym xml:lang="en">Dense Retrieval</oboInOwl:hasSynonym>
        <rdfs:label xml:lang="en">Dense Passage Retrieval</rdfs:label>
    </owl:NamedIndividual>
    


    <!-- http://nlpkg.sebis.cit.tum.de/nlp-fos-hierarchy.owl#Dependency_Graphs -->

    <owl:NamedIndividual rdf:about="http://nlpkg.sebis.cit.tum.de/nlp-fos-hierarchy.owl#Dependency_Graphs">
        <rdf:type rdf:resource="http://nlpkg.sebis.cit.tum.de/nlp-fos-hierarchy.owl#DataStructure"/>
        <rdf:type rdf:resource="http://nlpkg.sebis.cit.tum.de/nlp-taxonomy.owl#FieldOfStudy"/>
        <nlp-taxonomy:subFieldOf rdf:resource="http://nlpkg.sebis.cit.tum.de/nlp-fos-hierarchy.owl#Dependency_Parsing"/>
        <nlp-taxonomy:subFieldOf rdf:resource="http://nlpkg.sebis.cit.tum.de/nlp-fos-hierarchy.owl#Graphs"/>
        <nlp-taxonomy:subFieldOf rdf:resource="http://nlpkg.sebis.cit.tum.de/nlp-fos-hierarchy.owl#Parse_Tree"/>
        <nlp-taxonomy:level rdf:datatype="http://www.w3.org/2001/XMLSchema#integer">4</nlp-taxonomy:level>
        <nlp-taxonomy:level rdf:datatype="http://www.w3.org/2001/XMLSchema#integer">5</nlp-taxonomy:level>
        <nlp-taxonomy:level rdf:datatype="http://www.w3.org/2001/XMLSchema#integer">6</nlp-taxonomy:level>
        <dcterms:description xml:lang="en">Dependency Graphs represent the grammatical structure of a sentence based on dependency grammar. Each word in the sentence is a node in the graph and the edges between nodes represent the grammatical relationships between the words. These relationships help in understanding the context and meaning of the sentence.</dcterms:description>
        <oboInOwl:hasSynonym xml:lang="en">Dependency Parse Tree</oboInOwl:hasSynonym>
        <oboInOwl:hasSynonym xml:lang="en">Dependency Trees</oboInOwl:hasSynonym>
        <rdfs:label xml:lang="en">Dependency Graphs</rdfs:label>
    </owl:NamedIndividual>
    


    <!-- http://nlpkg.sebis.cit.tum.de/nlp-fos-hierarchy.owl#Dependency_Parsing -->

    <owl:NamedIndividual rdf:about="http://nlpkg.sebis.cit.tum.de/nlp-fos-hierarchy.owl#Dependency_Parsing">
        <rdf:type rdf:resource="http://nlpkg.sebis.cit.tum.de/nlp-fos-hierarchy.owl#Task"/>
        <rdf:type rdf:resource="http://nlpkg.sebis.cit.tum.de/nlp-taxonomy.owl#FieldOfStudy"/>
        <nlp-taxonomy:subFieldOf rdf:resource="http://nlpkg.sebis.cit.tum.de/nlp-taxonomy.owl#Syntactic_Parsing"/>
        <nlp-taxonomy:superFieldOf rdf:resource="http://nlpkg.sebis.cit.tum.de/nlp-fos-hierarchy.owl#Dependency_Graphs"/>
        <relevantInformation>https://web.stanford.edu/~jurafsky/slp3/18.pdf</relevantInformation>
        <survey>https://aclanthology.org/2020.coling-main.227</survey>
        <survey>https://arxiv.org/abs/2006.11056</survey>
        <nlp-taxonomy:level rdf:datatype="http://www.w3.org/2001/XMLSchema#integer">3</nlp-taxonomy:level>
        <dcterms:description xml:lang="en">Dependency Parsing is a technique used to determine the grammatical structure of a sentence based on the dependencies between the words. It helps to understand the relationship between words, where one word is the dependent of another.</dcterms:description>
        <rdfs:label xml:lang="en">Dependency Parsing</rdfs:label>
    </owl:NamedIndividual>
    


    <!-- http://nlpkg.sebis.cit.tum.de/nlp-fos-hierarchy.owl#Dialogue_Discourse_Parsing -->

    <owl:NamedIndividual rdf:about="http://nlpkg.sebis.cit.tum.de/nlp-fos-hierarchy.owl#Dialogue_Discourse_Parsing">
        <rdf:type rdf:resource="http://nlpkg.sebis.cit.tum.de/nlp-fos-hierarchy.owl#Task"/>
        <rdf:type rdf:resource="http://nlpkg.sebis.cit.tum.de/nlp-taxonomy.owl#FieldOfStudy"/>
        <usedFor rdf:resource="http://nlpkg.sebis.cit.tum.de/nlp-fos-hierarchy.owl#Dialogue_Understanding"/>
        <nlp-taxonomy:subFieldOf rdf:resource="http://nlpkg.sebis.cit.tum.de/nlp-fos-hierarchy.owl#Discourse_Parsing"/>
        <nlp-taxonomy:level rdf:datatype="http://www.w3.org/2001/XMLSchema#integer">4</nlp-taxonomy:level>
        <dcterms:description xml:lang="en">Dialogue Discourse Parsing refers to the process of analyzing and structuring the conversational flow and structure within a dialogue or conversation. It involves identifying the the discourse links and corresponding relations between individual utterances or sentences in a multi-participant conversation to understand how they contribute to the overall meaning and coherence of the conversation.</dcterms:description>
        <oboInOwl:hasSynonym xml:lang="en">Dialog DP</oboInOwl:hasSynonym>
        <oboInOwl:hasSynonym xml:lang="en">Dialog Discourse Parsing</oboInOwl:hasSynonym>
        <oboInOwl:hasSynonym xml:lang="en">Dialogue DP</oboInOwl:hasSynonym>
        <rdfs:label xml:lang="en">Dialogue Discourse Parsing</rdfs:label>
    </owl:NamedIndividual>
    


    <!-- http://nlpkg.sebis.cit.tum.de/nlp-fos-hierarchy.owl#Dialogue_Management -->

    <owl:NamedIndividual rdf:about="http://nlpkg.sebis.cit.tum.de/nlp-fos-hierarchy.owl#Dialogue_Management">
        <rdf:type rdf:resource="http://nlpkg.sebis.cit.tum.de/nlp-fos-hierarchy.owl#Task"/>
        <rdf:type rdf:resource="http://nlpkg.sebis.cit.tum.de/nlp-taxonomy.owl#FieldOfStudy"/>
        <nlp-taxonomy:subFieldOf rdf:resource="http://nlpkg.sebis.cit.tum.de/nlp-taxonomy.owl#Dialogue_Systems_&amp;_Conversational_Agents"/>
        <nlp-taxonomy:superFieldOf rdf:resource="http://nlpkg.sebis.cit.tum.de/nlp-fos-hierarchy.owl#Dialogue_Policy"/>
        <nlp-taxonomy:superFieldOf rdf:resource="http://nlpkg.sebis.cit.tum.de/nlp-fos-hierarchy.owl#Dialogue_State_Tracking"/>
        <survey>https://arxiv.org/abs/2005.02233</survey>
        <survey>https://arxiv.org/abs/2307.09021</survey>
        <nlp-taxonomy:level rdf:datatype="http://www.w3.org/2001/XMLSchema#integer">3</nlp-taxonomy:level>
        <dcterms:description xml:lang="en">Dialogue Management refers to the process of controlling and orchestrating a conversation between a computer system or chatbot and a user. It involves managing the flow of conversation, understanding user inputs, generating appropriate responses, and maintaining context throughout the interaction to ensure a coherent and effective dialogue. Dialogue management is a crucial component of building conversational AI systems and plays a key role in providing meaningful and responsive interactions.</dcterms:description>
        <oboInOwl:hasSynonym xml:lang="en">Dialog Management</oboInOwl:hasSynonym>
        <rdfs:label xml:lang="en">Dialogue Management</rdfs:label>
    </owl:NamedIndividual>
    


    <!-- http://nlpkg.sebis.cit.tum.de/nlp-fos-hierarchy.owl#Dialogue_Policy -->

    <owl:NamedIndividual rdf:about="http://nlpkg.sebis.cit.tum.de/nlp-fos-hierarchy.owl#Dialogue_Policy">
        <rdf:type rdf:resource="http://nlpkg.sebis.cit.tum.de/nlp-fos-hierarchy.owl#OtherScientificField"/>
        <rdf:type rdf:resource="http://nlpkg.sebis.cit.tum.de/nlp-taxonomy.owl#FieldOfStudy"/>
        <nlp-taxonomy:subFieldOf rdf:resource="http://nlpkg.sebis.cit.tum.de/nlp-fos-hierarchy.owl#Dialogue_Management"/>
        <nlp-taxonomy:superFieldOf rdf:resource="http://nlpkg.sebis.cit.tum.de/nlp-fos-hierarchy.owl#Dialogue_Policy_Learning"/>
        <nlp-taxonomy:level rdf:datatype="http://www.w3.org/2001/XMLSchema#integer">4</nlp-taxonomy:level>
        <dcterms:description xml:lang="en">A Dialogue Policy refers to a set of rules, algorithms, or models that govern how a conversational agent or chatbot should respond to user inputs in a dialogue or conversation. It defines the agent&apos;s behavior, including when to ask questions, provide information, or take specific actions based on the context of the conversation. Dialogue policies are crucial for designing effective and responsive conversational systems.</dcterms:description>
        <oboInOwl:hasSynonym xml:lang="en">Dialog Policy</oboInOwl:hasSynonym>
        <rdfs:label xml:lang="en">Dialogue Policy</rdfs:label>
    </owl:NamedIndividual>
    


    <!-- http://nlpkg.sebis.cit.tum.de/nlp-fos-hierarchy.owl#Dialogue_Policy_Learning -->

    <owl:NamedIndividual rdf:about="http://nlpkg.sebis.cit.tum.de/nlp-fos-hierarchy.owl#Dialogue_Policy_Learning">
        <rdf:type rdf:resource="http://nlpkg.sebis.cit.tum.de/nlp-fos-hierarchy.owl#Task"/>
        <rdf:type rdf:resource="http://nlpkg.sebis.cit.tum.de/nlp-taxonomy.owl#FieldOfStudy"/>
        <nlp-taxonomy:subFieldOf rdf:resource="http://nlpkg.sebis.cit.tum.de/nlp-fos-hierarchy.owl#Dialogue_Policy"/>
        <survey>https://arxiv.org/abs/2202.13675</survey>
        <nlp-taxonomy:level rdf:datatype="http://www.w3.org/2001/XMLSchema#integer">5</nlp-taxonomy:level>
        <dcterms:description xml:lang="en">Dialogue Policy Learning (DPL) refers to the process of training a machine learning model, often using reinforcement learning techniques, to determine the optimal actions or responses in a conversational dialogue. It involves teaching a system how to make decisions at each turn of a conversation to achieve specific goals or objectives, such as providing helpful responses or taking appropriate actions based on user input. Dialogue Policy Learning is a crucial component in building chatbots, virtual assistants, and other conversational AI systems.</dcterms:description>
        <oboInOwl:hasSynonym xml:lang="en">DPL</oboInOwl:hasSynonym>
        <oboInOwl:hasSynonym xml:lang="en">Dialog Policy Learning</oboInOwl:hasSynonym>
        <rdfs:label xml:lang="en">Dialogue Policy Learning</rdfs:label>
    </owl:NamedIndividual>
    


    <!-- http://nlpkg.sebis.cit.tum.de/nlp-fos-hierarchy.owl#Dialogue_State_Tracking -->

    <owl:NamedIndividual rdf:about="http://nlpkg.sebis.cit.tum.de/nlp-fos-hierarchy.owl#Dialogue_State_Tracking">
        <rdf:type rdf:resource="http://nlpkg.sebis.cit.tum.de/nlp-fos-hierarchy.owl#Task"/>
        <rdf:type rdf:resource="http://nlpkg.sebis.cit.tum.de/nlp-taxonomy.owl#FieldOfStudy"/>
        <uses rdf:resource="http://nlpkg.sebis.cit.tum.de/nlp-fos-hierarchy.owl#Slot_Filling"/>
        <nlp-taxonomy:subFieldOf rdf:resource="http://nlpkg.sebis.cit.tum.de/nlp-fos-hierarchy.owl#Dialogue_Management"/>
        <survey>https://aclanthology.org/2022.sigdial-1.33</survey>
        <nlp-taxonomy:level rdf:datatype="http://www.w3.org/2001/XMLSchema#integer">4</nlp-taxonomy:level>
        <dcterms:description xml:lang="en">Dialogue State Tracking (DST) refers to the process of monitoring and maintaining an understanding of the current state of a conversational dialogue. It involves tracking relevant information such as user intents, entity mentions, and context within a conversation. DST is crucial in building effective dialogue systems, chatbots, or virtual assistants as it helps in interpreting and responding to user queries accurately by keeping track of the evolving conversation context.</dcterms:description>
        <oboInOwl:hasSynonym xml:lang="en">DST</oboInOwl:hasSynonym>
        <oboInOwl:hasSynonym xml:lang="en">Dialog State Tracking</oboInOwl:hasSynonym>
        <rdfs:label xml:lang="en">Dialogue State Tracking</rdfs:label>
    </owl:NamedIndividual>
    


    <!-- http://nlpkg.sebis.cit.tum.de/nlp-fos-hierarchy.owl#Dialogue_Understanding -->

    <owl:NamedIndividual rdf:about="http://nlpkg.sebis.cit.tum.de/nlp-fos-hierarchy.owl#Dialogue_Understanding">
        <rdf:type rdf:resource="http://nlpkg.sebis.cit.tum.de/nlp-fos-hierarchy.owl#Task"/>
        <rdf:type rdf:resource="http://nlpkg.sebis.cit.tum.de/nlp-taxonomy.owl#FieldOfStudy"/>
        <uses rdf:resource="http://nlpkg.sebis.cit.tum.de/nlp-fos-hierarchy.owl#Dialogue_Discourse_Parsing"/>
        <uses rdf:resource="http://nlpkg.sebis.cit.tum.de/nlp-taxonomy.owl#Intent_Recognition"/>
        <uses rdf:resource="http://nlpkg.sebis.cit.tum.de/nlp-taxonomy.owl#Named_Entity_Recognition"/>
        <nlp-taxonomy:subFieldOf rdf:resource="http://nlpkg.sebis.cit.tum.de/nlp-taxonomy.owl#Dialogue_Systems_&amp;_Conversational_Agents"/>
        <survey>https://aclanthology.org/2022.sigdial-1.54</survey>
        <survey>https://arxiv.org/abs/1505.03084</survey>
        <survey>https://arxiv.org/abs/2009.13902</survey>
        <survey>https://arxiv.org/abs/2103.03125</survey>
        <nlp-taxonomy:level rdf:datatype="http://www.w3.org/2001/XMLSchema#integer">3</nlp-taxonomy:level>
        <dcterms:description xml:lang="en">Dialogue Understanding involves the ability of systems to comprehend and interpret natural language conversations between humans or between humans and machines. It involves extracting meaning, context, intent, and relevant information from spoken or written dialogues to enable effective communication and decision-making.</dcterms:description>
        <oboInOwl:hasSynonym xml:lang="en">Dialog Comprehension</oboInOwl:hasSynonym>
        <oboInOwl:hasSynonym xml:lang="en">Dialog Understanding</oboInOwl:hasSynonym>
        <oboInOwl:hasSynonym xml:lang="en">Dialogue Comprehension</oboInOwl:hasSynonym>
        <rdfs:label xml:lang="en">Dialogue Understanding</rdfs:label>
    </owl:NamedIndividual>
    


    <!-- http://nlpkg.sebis.cit.tum.de/nlp-fos-hierarchy.owl#Dictionary -->

    <owl:NamedIndividual rdf:about="http://nlpkg.sebis.cit.tum.de/nlp-fos-hierarchy.owl#Dictionary">
        <rdf:type rdf:resource="http://nlpkg.sebis.cit.tum.de/nlp-fos-hierarchy.owl#DataStructure"/>
        <rdf:type rdf:resource="http://nlpkg.sebis.cit.tum.de/nlp-taxonomy.owl#FieldOfStudy"/>
        <nlp-taxonomy:subFieldOf rdf:resource="http://nlpkg.sebis.cit.tum.de/nlp-fos-hierarchy.owl#Knowledge_Bases"/>
        <nlp-taxonomy:superFieldOf rdf:resource="http://nlpkg.sebis.cit.tum.de/nlp-fos-hierarchy.owl#Translation_Memory"/>
        <nlp-taxonomy:level rdf:datatype="http://www.w3.org/2001/XMLSchema#integer">4</nlp-taxonomy:level>
        <dcterms:description xml:lang="en">Dictionary is a data structure that holds a set of words or phrases and their associated information. This information can include definitions, synonyms, antonyms, translations, and other linguistic attributes.</dcterms:description>
        <oboInOwl:hasSynonym xml:lang="en">Lexicon</oboInOwl:hasSynonym>
        <rdfs:label xml:lang="en">Dictionary</rdfs:label>
    </owl:NamedIndividual>
    


    <!-- http://nlpkg.sebis.cit.tum.de/nlp-fos-hierarchy.owl#Differential_Privacy -->

    <owl:NamedIndividual rdf:about="http://nlpkg.sebis.cit.tum.de/nlp-fos-hierarchy.owl#Differential_Privacy">
        <rdf:type rdf:resource="http://nlpkg.sebis.cit.tum.de/nlp-fos-hierarchy.owl#OtherScientificField"/>
        <rdf:type rdf:resource="http://nlpkg.sebis.cit.tum.de/nlp-taxonomy.owl#FieldOfStudy"/>
        <nlp-taxonomy:subFieldOf rdf:resource="http://nlpkg.sebis.cit.tum.de/nlp-fos-hierarchy.owl#Privacy,_Security_&amp;_Safety_in_NLP"/>
        <survey>https://aclanthology.org/2021.findings-emnlp.102</survey>
        <survey>https://aclanthology.org/2022.privatenlp-1.1</survey>
        <nlp-taxonomy:level rdf:datatype="http://www.w3.org/2001/XMLSchema#integer">4</nlp-taxonomy:level>
        <dcterms:description xml:lang="en">Differential Privacy is a concept that aims to provide a certain level of data privacy and security when processing and analyzing text data. It ensures that the results of any analysis (like machine learning algorithms) are essentially the same, irrespective of whether an individual&apos;s data is included in the dataset or not. This way, it prevents the disclosure of sensitive information about individuals in the dataset, providing a balance between data utility and privacy.</dcterms:description>
        <rdfs:label xml:lang="en">Differential Privacy</rdfs:label>
    </owl:NamedIndividual>
    


    <!-- http://nlpkg.sebis.cit.tum.de/nlp-fos-hierarchy.owl#Discourse_Analysis -->

    <owl:NamedIndividual rdf:about="http://nlpkg.sebis.cit.tum.de/nlp-fos-hierarchy.owl#Discourse_Analysis">
        <rdf:type rdf:resource="http://nlpkg.sebis.cit.tum.de/nlp-fos-hierarchy.owl#Task"/>
        <rdf:type rdf:resource="http://nlpkg.sebis.cit.tum.de/nlp-taxonomy.owl#FieldOfStudy"/>
        <uses rdf:resource="http://nlpkg.sebis.cit.tum.de/nlp-fos-hierarchy.owl#Discourse_Parsing"/>
        <uses rdf:resource="http://nlpkg.sebis.cit.tum.de/nlp-fos-hierarchy.owl#Discourse_Segmentation"/>
        <nlp-taxonomy:subFieldOf rdf:resource="http://nlpkg.sebis.cit.tum.de/nlp-taxonomy.owl#Discourse_&amp;_Pragmatics"/>
        <nlp-taxonomy:level rdf:datatype="http://www.w3.org/2001/XMLSchema#integer">3</nlp-taxonomy:level>
        <dcterms:description xml:lang="en">Discourse Analysis refers to the study and interpretation of written, spoken, or sign language use. It involves understanding, interpreting, and analyzing the broader context of communication, including the social, political, and cultural structures that influence text or speech. It goes beyond the understanding of individual words or sentences to comprehend how different parts of the text interact to produce meaning.</dcterms:description>
        <oboInOwl:hasSynonym xml:lang="en">Automatic Discourse Processing</oboInOwl:hasSynonym>
        <oboInOwl:hasSynonym xml:lang="en">Discourse Processing</oboInOwl:hasSynonym>
        <rdfs:label xml:lang="en">Discourse Analysis</rdfs:label>
    </owl:NamedIndividual>
    


    <!-- http://nlpkg.sebis.cit.tum.de/nlp-fos-hierarchy.owl#Discourse_Deixis_Resolution -->

    <owl:NamedIndividual rdf:about="http://nlpkg.sebis.cit.tum.de/nlp-fos-hierarchy.owl#Discourse_Deixis_Resolution">
        <rdf:type rdf:resource="http://nlpkg.sebis.cit.tum.de/nlp-fos-hierarchy.owl#Task"/>
        <rdf:type rdf:resource="http://nlpkg.sebis.cit.tum.de/nlp-taxonomy.owl#FieldOfStudy"/>
        <nlp-taxonomy:subFieldOf rdf:resource="http://nlpkg.sebis.cit.tum.de/nlp-fos-hierarchy.owl#Anaphora_Resolution"/>
        <nlp-taxonomy:subFieldOf rdf:resource="http://nlpkg.sebis.cit.tum.de/nlp-taxonomy.owl#Discourse_&amp;_Pragmatics"/>
        <nlp-taxonomy:superFieldOf rdf:resource="http://nlpkg.sebis.cit.tum.de/nlp-fos-hierarchy.owl#Event_Discourse_Deixis_Resolution"/>
        <nlp-taxonomy:superFieldOf rdf:resource="http://nlpkg.sebis.cit.tum.de/nlp-fos-hierarchy.owl#Fact_Discourse_Deixis_Resolution"/>
        <survey>https://aclanthology.org/J18-3007</survey>
        <nlp-taxonomy:level rdf:datatype="http://www.w3.org/2001/XMLSchema#integer">3</nlp-taxonomy:level>
        <nlp-taxonomy:level rdf:datatype="http://www.w3.org/2001/XMLSchema#integer">4</nlp-taxonomy:level>
        <dcterms:description xml:lang="en">Discourse Deixis Resolution (or Abstract Anaphora Resolution) refers to the process of determining the referents of certain types of expressions, such as pronouns or definite noun phrases, within a given discourse or conversation. These expressions often refer back to previously mentioned concepts or forward to upcoming concepts in the discourse. The resolution process involves understanding the context of the conversation and the relationships between different entities or concepts within it.</dcterms:description>
        <oboInOwl:hasSynonym xml:lang="en">Abstract Anaphora Resolution</oboInOwl:hasSynonym>
        <oboInOwl:hasSynonym xml:lang="en">DD Resolution</oboInOwl:hasSynonym>
        <rdfs:label xml:lang="en">Discourse Deixis Resolution</rdfs:label>
    </owl:NamedIndividual>
    


    <!-- http://nlpkg.sebis.cit.tum.de/nlp-fos-hierarchy.owl#Discourse_Parsing -->

    <owl:NamedIndividual rdf:about="http://nlpkg.sebis.cit.tum.de/nlp-fos-hierarchy.owl#Discourse_Parsing">
        <rdf:type rdf:resource="http://nlpkg.sebis.cit.tum.de/nlp-fos-hierarchy.owl#Task"/>
        <rdf:type rdf:resource="http://nlpkg.sebis.cit.tum.de/nlp-taxonomy.owl#FieldOfStudy"/>
        <usedFor rdf:resource="http://nlpkg.sebis.cit.tum.de/nlp-fos-hierarchy.owl#Discourse_Analysis"/>
        <uses rdf:resource="http://nlpkg.sebis.cit.tum.de/nlp-fos-hierarchy.owl#Elementary_Discourse_Unit_Segmentation"/>
        <uses rdf:resource="http://nlpkg.sebis.cit.tum.de/nlp-fos-hierarchy.owl#Relation_Directionality_Classification"/>
        <uses rdf:resource="http://nlpkg.sebis.cit.tum.de/nlp-taxonomy.owl#Relation_Extraction"/>
        <nlp-taxonomy:subFieldOf rdf:resource="http://nlpkg.sebis.cit.tum.de/nlp-taxonomy.owl#Semantic_Parsing"/>
        <nlp-taxonomy:subFieldOf rdf:resource="http://nlpkg.sebis.cit.tum.de/nlp-taxonomy.owl#Discourse_&amp;_Pragmatics"/>
        <nlp-taxonomy:superFieldOf rdf:resource="http://nlpkg.sebis.cit.tum.de/nlp-fos-hierarchy.owl#Dialogue_Discourse_Parsing"/>
        <nlp-taxonomy:superFieldOf rdf:resource="http://nlpkg.sebis.cit.tum.de/nlp-fos-hierarchy.owl#Discourse_Relation_Recognition"/>
        <nlp-taxonomy:superFieldOf rdf:resource="http://nlpkg.sebis.cit.tum.de/nlp-fos-hierarchy.owl#Penn_Discourse_Treebank_Discourse_Parsing"/>
        <nlp-taxonomy:superFieldOf rdf:resource="http://nlpkg.sebis.cit.tum.de/nlp-fos-hierarchy.owl#Rhetorical_Structure_Theory_Discourse_Parsing"/>
        <nlp-taxonomy:superFieldOf rdf:resource="http://nlpkg.sebis.cit.tum.de/nlp-fos-hierarchy.owl#Segmented_Discourse_Representation_Theory_Discopurse_Parsing"/>
        <nlp-taxonomy:level rdf:datatype="http://www.w3.org/2001/XMLSchema#integer">3</nlp-taxonomy:level>
        <dcterms:description xml:lang="en">Discourse Parsing (DP) is the process of analyzing and understanding the structure and relationships within a piece of text or conversation beyond individual sentences. It aims to identify how sentences and utterances are connected, such as through discourse markers, coreference resolution, and rhetorical structure, to extract a coherent representation of the overall discourse or conversation. This helps in understanding the flow of ideas, arguments, and information in a text or conversation.</dcterms:description>
        <oboInOwl:hasSynonym xml:lang="en">DP</oboInOwl:hasSynonym>
        <rdfs:label xml:lang="en">Discourse Parsing</rdfs:label>
    </owl:NamedIndividual>
    


    <!-- http://nlpkg.sebis.cit.tum.de/nlp-fos-hierarchy.owl#Discourse_Relation_Recognition -->

    <owl:NamedIndividual rdf:about="http://nlpkg.sebis.cit.tum.de/nlp-fos-hierarchy.owl#Discourse_Relation_Recognition">
        <rdf:type rdf:resource="http://nlpkg.sebis.cit.tum.de/nlp-fos-hierarchy.owl#Task"/>
        <rdf:type rdf:resource="http://nlpkg.sebis.cit.tum.de/nlp-taxonomy.owl#FieldOfStudy"/>
        <nlp-taxonomy:subFieldOf rdf:resource="http://nlpkg.sebis.cit.tum.de/nlp-fos-hierarchy.owl#Discourse_Parsing"/>
        <nlp-taxonomy:subFieldOf rdf:resource="http://nlpkg.sebis.cit.tum.de/nlp-taxonomy.owl#Relation_Extraction"/>
        <nlp-taxonomy:superFieldOf rdf:resource="http://nlpkg.sebis.cit.tum.de/nlp-fos-hierarchy.owl#Alternative_Lexicalization_Discourse_Relation_Recognition"/>
        <nlp-taxonomy:superFieldOf rdf:resource="http://nlpkg.sebis.cit.tum.de/nlp-fos-hierarchy.owl#Entity-based_Coherence_Discourse_Relation_Recognition"/>
        <nlp-taxonomy:superFieldOf rdf:resource="http://nlpkg.sebis.cit.tum.de/nlp-fos-hierarchy.owl#Explicit_Discourse_Relation_Recognition"/>
        <nlp-taxonomy:superFieldOf rdf:resource="http://nlpkg.sebis.cit.tum.de/nlp-fos-hierarchy.owl#Implicit_Discourse_Relation_Recognition"/>
        <nlp-taxonomy:level rdf:datatype="http://www.w3.org/2001/XMLSchema#integer">3</nlp-taxonomy:level>
        <nlp-taxonomy:level rdf:datatype="http://www.w3.org/2001/XMLSchema#integer">4</nlp-taxonomy:level>
        <nlp-taxonomy:level rdf:datatype="http://www.w3.org/2001/XMLSchema#integer">8</nlp-taxonomy:level>
        <dcterms:description xml:lang="en">Discourse Relation Recognition refers to the task of identifying and categorizing the relationship between different sentences or clauses in a text. These relations can be causal, contrastive, temporal, etc.</dcterms:description>
        <oboInOwl:hasSynonym xml:lang="en">DRE</oboInOwl:hasSynonym>
        <oboInOwl:hasSynonym xml:lang="en">DRR</oboInOwl:hasSynonym>
        <oboInOwl:hasSynonym xml:lang="en">Discourse Relation Extraction</oboInOwl:hasSynonym>
        <rdfs:label xml:lang="en">Discourse Relation Recognition</rdfs:label>
    </owl:NamedIndividual>
    


    <!-- http://nlpkg.sebis.cit.tum.de/nlp-fos-hierarchy.owl#Discourse_Segmentation -->

    <owl:NamedIndividual rdf:about="http://nlpkg.sebis.cit.tum.de/nlp-fos-hierarchy.owl#Discourse_Segmentation">
        <rdf:type rdf:resource="http://nlpkg.sebis.cit.tum.de/nlp-fos-hierarchy.owl#Task"/>
        <rdf:type rdf:resource="http://nlpkg.sebis.cit.tum.de/nlp-taxonomy.owl#FieldOfStudy"/>
        <usedFor rdf:resource="http://nlpkg.sebis.cit.tum.de/nlp-fos-hierarchy.owl#Discourse_Analysis"/>
        <nlp-taxonomy:subFieldOf rdf:resource="http://nlpkg.sebis.cit.tum.de/nlp-taxonomy.owl#Discourse_&amp;_Pragmatics"/>
        <nlp-taxonomy:superFieldOf rdf:resource="http://nlpkg.sebis.cit.tum.de/nlp-fos-hierarchy.owl#Elementary_Discourse_Unit_Segmentation"/>
        <survey>https://arxiv.org/abs/2005.00468</survey>
        <nlp-taxonomy:level rdf:datatype="http://www.w3.org/2001/XMLSchema#integer">3</nlp-taxonomy:level>
        <dcterms:description xml:lang="en">Discourse segmentation refers to the task of dividing a continuous text or conversation into coherent and meaningful segments or units. These segments often represent distinct topics, ideas, or conversational turns within the text.</dcterms:description>
        <rdfs:label xml:lang="en">Discourse Segmentation</rdfs:label>
    </owl:NamedIndividual>
    


    <!-- http://nlpkg.sebis.cit.tum.de/nlp-fos-hierarchy.owl#Discrimination_Analysis -->

    <owl:NamedIndividual rdf:about="http://nlpkg.sebis.cit.tum.de/nlp-fos-hierarchy.owl#Discrimination_Analysis">
        <rdf:type rdf:resource="http://nlpkg.sebis.cit.tum.de/nlp-fos-hierarchy.owl#Task"/>
        <rdf:type rdf:resource="http://nlpkg.sebis.cit.tum.de/nlp-taxonomy.owl#FieldOfStudy"/>
        <nlp-taxonomy:subFieldOf rdf:resource="http://nlpkg.sebis.cit.tum.de/nlp-taxonomy.owl#Ethical_NLP"/>
        <nlp-taxonomy:superFieldOf rdf:resource="http://nlpkg.sebis.cit.tum.de/nlp-fos-hierarchy.owl#Hate_Speech_Detection"/>
        <nlp-taxonomy:superFieldOf rdf:resource="http://nlpkg.sebis.cit.tum.de/nlp-fos-hierarchy.owl#Offensive_Language_Detection"/>
        <survey>https://aclanthology.org/2020.findings-emnlp.301</survey>
        <survey>https://arxiv.org/abs/2308.15745</survey>
        <nlp-taxonomy:level rdf:datatype="http://www.w3.org/2001/XMLSchema#integer">3</nlp-taxonomy:level>
        <dcterms:description xml:lang="en">Discrimination Analysis refers to the study and evaluation of biases and discrimination that may be present texts or in language models. It involves identifying and addressing issues such as gender, racial, or cultural biases that can be inadvertently learned and propagated by AI systems. The goal is to ensure fairness, transparency, and accountability in NLP systems, and to prevent the perpetuation of harmful stereotypes or discriminatory practices.</dcterms:description>
        <rdfs:label xml:lang="en">Discrimination Analysis</rdfs:label>
    </owl:NamedIndividual>
    


    <!-- http://nlpkg.sebis.cit.tum.de/nlp-fos-hierarchy.owl#Distant_Supervision -->

    <owl:NamedIndividual rdf:about="http://nlpkg.sebis.cit.tum.de/nlp-fos-hierarchy.owl#Distant_Supervision">
        <rdf:type rdf:resource="http://nlpkg.sebis.cit.tum.de/nlp-fos-hierarchy.owl#OtherScientificField"/>
        <rdf:type rdf:resource="http://nlpkg.sebis.cit.tum.de/nlp-taxonomy.owl#FieldOfStudy"/>
        <usedFor rdf:resource="http://nlpkg.sebis.cit.tum.de/nlp-taxonomy.owl#Relation_Extraction"/>
        <nlp-taxonomy:subFieldOf rdf:resource="http://nlpkg.sebis.cit.tum.de/nlp-fos-hierarchy.owl#Weak_Supervision"/>
        <survey>https://aclanthology.org/2021.findings-acl.112</survey>
        <survey>https://arxiv.org/abs/1705.03751</survey>
        <nlp-taxonomy:level rdf:datatype="http://www.w3.org/2001/XMLSchema#integer">4</nlp-taxonomy:level>
        <dcterms:description xml:lang="en">Distant Supervision is a method used to create weakly labeled training data automatically. It involves using an existing knowledge base to generate labels for text data under the assumption that if two entities participate in a relationship in the knowledge base, then any sentence that contains those two entities might express that relationship. This approach is particularly useful when manual labeling of data is not feasible due to the large volume of data.</dcterms:description>
        <rdfs:label xml:lang="en">Distant Supervision</rdfs:label>
    </owl:NamedIndividual>
    


    <!-- http://nlpkg.sebis.cit.tum.de/nlp-fos-hierarchy.owl#Distributional_Semantics -->

    <owl:NamedIndividual rdf:about="http://nlpkg.sebis.cit.tum.de/nlp-fos-hierarchy.owl#Distributional_Semantics">
        <rdf:type rdf:resource="http://nlpkg.sebis.cit.tum.de/nlp-fos-hierarchy.owl#OtherScientificField"/>
        <rdf:type rdf:resource="http://nlpkg.sebis.cit.tum.de/nlp-taxonomy.owl#FieldOfStudy"/>
        <usedFor rdf:resource="http://nlpkg.sebis.cit.tum.de/nlp-fos-hierarchy.owl#Word_Embeddings"/>
        <nlp-taxonomy:subFieldOf rdf:resource="http://nlpkg.sebis.cit.tum.de/nlp-taxonomy.owl#Linguistic_Theories"/>
        <survey>https://arxiv.org/abs/1905.01896</survey>
        <nlp-taxonomy:level rdf:datatype="http://www.w3.org/2001/XMLSchema#integer">3</nlp-taxonomy:level>
        <dcterms:description xml:lang="en">Distributional Semantics is a research area that develops and studies theories and methods for quantifying and categorizing semantic similarities between linguistic items based on their distributional properties in large samples of language data. The basic hypothesis is that words that occur in the same contexts tend to have similar meanings.</dcterms:description>
        <rdfs:label xml:lang="en">Distributional Semantics</rdfs:label>
    </owl:NamedIndividual>
    


    <!-- http://nlpkg.sebis.cit.tum.de/nlp-fos-hierarchy.owl#Document_Expansion -->

    <owl:NamedIndividual rdf:about="http://nlpkg.sebis.cit.tum.de/nlp-fos-hierarchy.owl#Document_Expansion">
        <rdf:type rdf:resource="http://nlpkg.sebis.cit.tum.de/nlp-fos-hierarchy.owl#Task"/>
        <rdf:type rdf:resource="http://nlpkg.sebis.cit.tum.de/nlp-taxonomy.owl#FieldOfStudy"/>
        <nlp-taxonomy:subFieldOf rdf:resource="http://nlpkg.sebis.cit.tum.de/nlp-taxonomy.owl#Semantic_Search"/>
        <survey>https://arxiv.org/abs/2309.08541</survey>
        <nlp-taxonomy:level rdf:datatype="http://www.w3.org/2001/XMLSchema#integer">3</nlp-taxonomy:level>
        <dcterms:description xml:lang="en">Document Expansion is the task of expanding documents with terms that are related or representative of the documents&apos; content to improve the retrieval effectiveness of a search engine.</dcterms:description>
        <rdfs:label xml:lang="en">Document Expansion</rdfs:label>
    </owl:NamedIndividual>
    


    <!-- http://nlpkg.sebis.cit.tum.de/nlp-fos-hierarchy.owl#Domain_Adaptation -->

    <owl:NamedIndividual rdf:about="http://nlpkg.sebis.cit.tum.de/nlp-fos-hierarchy.owl#Domain_Adaptation">
        <rdf:type rdf:resource="http://nlpkg.sebis.cit.tum.de/nlp-fos-hierarchy.owl#Task"/>
        <rdf:type rdf:resource="http://nlpkg.sebis.cit.tum.de/nlp-taxonomy.owl#FieldOfStudy"/>
        <uses rdf:resource="http://nlpkg.sebis.cit.tum.de/nlp-fos-hierarchy.owl#Meta-Learning"/>
        <nlp-taxonomy:subFieldOf rdf:resource="http://nlpkg.sebis.cit.tum.de/nlp-taxonomy.owl#Language_Models"/>
        <nlp-taxonomy:subFieldOf rdf:resource="http://nlpkg.sebis.cit.tum.de/nlp-taxonomy.owl#Low-Resource_NLP"/>
        <survey>https://aclanthology.org/2020.coling-main.603</survey>
        <survey>https://aclanthology.org/2021.naacl-main.147</survey>
        <survey>https://aclanthology.org/C18-1111</survey>
        <survey>https://arxiv.org/abs/2104.06951</survey>
        <survey>https://arxiv.org/abs/2211.03154</survey>
        <nlp-taxonomy:level rdf:datatype="http://www.w3.org/2001/XMLSchema#integer">3</nlp-taxonomy:level>
        <dcterms:description xml:lang="en">Domain Adaptation refers to the process of modifying a model trained on one domain (source domain) to perform better on a different, but related domain (target domain). This is often necessary because the language use, terms, and context can vary greatly between different domains, causing a model trained on one domain to perform poorly on another. Domain adaptation techniques aim to overcome this issue and improve the model&apos;s performance on the target domain.</dcterms:description>
        <rdfs:label xml:lang="en">Domain Adaptation</rdfs:label>
    </owl:NamedIndividual>
    


    <!-- http://nlpkg.sebis.cit.tum.de/nlp-fos-hierarchy.owl#Efficient_Transformers -->

    <owl:NamedIndividual rdf:about="http://nlpkg.sebis.cit.tum.de/nlp-fos-hierarchy.owl#Efficient_Transformers">
        <rdf:type rdf:resource="http://nlpkg.sebis.cit.tum.de/nlp-fos-hierarchy.owl#OtherScientificField"/>
        <rdf:type rdf:resource="http://nlpkg.sebis.cit.tum.de/nlp-taxonomy.owl#FieldOfStudy"/>
        <nlp-taxonomy:subFieldOf rdf:resource="http://nlpkg.sebis.cit.tum.de/nlp-fos-hierarchy.owl#Transformers_&amp;_Large_Language_Models"/>
        <nlp-taxonomy:subFieldOf rdf:resource="http://nlpkg.sebis.cit.tum.de/nlp-taxonomy.owl#Green_&amp;_Sustainable_NLP"/>
        <nlp-taxonomy:superFieldOf rdf:resource="http://nlpkg.sebis.cit.tum.de/nlp-fos-hierarchy.owl#Knowledge_Distillation"/>
        <nlp-taxonomy:superFieldOf rdf:resource="http://nlpkg.sebis.cit.tum.de/nlp-fos-hierarchy.owl#Long-Range_Transformers"/>
        <survey>https://arxiv.org/abs/2008.05221</survey>
        <survey>https://arxiv.org/abs/2009.06732</survey>
        <survey>https://arxiv.org/abs/2202.07105</survey>
        <survey>https://arxiv.org/abs/2302.01107</survey>
        <survey>https://arxiv.org/abs/2304.03589</survey>
        <survey>https://arxiv.org/abs/2306.01768</survey>
        <nlp-taxonomy:level rdf:datatype="http://www.w3.org/2001/XMLSchema#integer">4</nlp-taxonomy:level>
        <dcterms:description xml:lang="en">Efficient Transformers to a group of transformer models that are designed to reduce the computational resources required by traditional transformer models. They aim to maintain or improve the performance of NLP tasks while reducing the memory and time complexity.</dcterms:description>
        <dcterms:description xml:lang="en">Transformer Inference Optimization</dcterms:description>
        <oboInOwl:hasSynonym xml:lang="en">Language Model Compression</oboInOwl:hasSynonym>
        <oboInOwl:hasSynonym xml:lang="en">Model Compression</oboInOwl:hasSynonym>
        <rdfs:label xml:lang="en">Efficient Transformers</rdfs:label>
    </owl:NamedIndividual>
    


    <!-- http://nlpkg.sebis.cit.tum.de/nlp-fos-hierarchy.owl#Elementary_Discourse_Unit -->

    <owl:NamedIndividual rdf:about="http://nlpkg.sebis.cit.tum.de/nlp-fos-hierarchy.owl#Elementary_Discourse_Unit">
        <rdf:type rdf:resource="http://nlpkg.sebis.cit.tum.de/nlp-fos-hierarchy.owl#OtherScientificField"/>
        <rdf:type rdf:resource="http://nlpkg.sebis.cit.tum.de/nlp-taxonomy.owl#FieldOfStudy"/>
        <usedFor rdf:resource="http://nlpkg.sebis.cit.tum.de/nlp-fos-hierarchy.owl#Elementary_Discourse_Unit_Segmentation"/>
        <usedFor rdf:resource="http://nlpkg.sebis.cit.tum.de/nlp-fos-hierarchy.owl#Rhetorical_Structure_Theory_Discourse_Tree"/>
        <nlp-taxonomy:subFieldOf rdf:resource="http://nlpkg.sebis.cit.tum.de/nlp-fos-hierarchy.owl#Rhetorical_Structure_Theory_Discourse_Parsing"/>
        <nlp-taxonomy:level rdf:datatype="http://www.w3.org/2001/XMLSchema#integer">5</nlp-taxonomy:level>
        <dcterms:description xml:lang="en">An Elementary Discourse Unit (EDU) refers to the smallest meaningful or syntactic unit in a discourse or text, often used for analyzing and structuring textual information. EDUs are typically used in discourse analysis to understand the hierarchical relationships and organization of sentences or phrases within a larger text, helping to break down and analyze complex language structures for various NLP tasks.</dcterms:description>
        <oboInOwl:hasSynonym xml:lang="en">EDU</oboInOwl:hasSynonym>
        <rdfs:label xml:lang="en">Elementary Discourse Unit</rdfs:label>
    </owl:NamedIndividual>
    


    <!-- http://nlpkg.sebis.cit.tum.de/nlp-fos-hierarchy.owl#Elementary_Discourse_Unit_Segmentation -->

    <owl:NamedIndividual rdf:about="http://nlpkg.sebis.cit.tum.de/nlp-fos-hierarchy.owl#Elementary_Discourse_Unit_Segmentation">
        <rdf:type rdf:resource="http://nlpkg.sebis.cit.tum.de/nlp-fos-hierarchy.owl#Task"/>
        <rdf:type rdf:resource="http://nlpkg.sebis.cit.tum.de/nlp-taxonomy.owl#FieldOfStudy"/>
        <usedFor rdf:resource="http://nlpkg.sebis.cit.tum.de/nlp-fos-hierarchy.owl#Discourse_Parsing"/>
        <uses rdf:resource="http://nlpkg.sebis.cit.tum.de/nlp-fos-hierarchy.owl#Elementary_Discourse_Unit"/>
        <nlp-taxonomy:subFieldOf rdf:resource="http://nlpkg.sebis.cit.tum.de/nlp-fos-hierarchy.owl#Discourse_Segmentation"/>
        <nlp-taxonomy:level rdf:datatype="http://www.w3.org/2001/XMLSchema#integer">4</nlp-taxonomy:level>
        <dcterms:description xml:lang="en">Elementary Discourse Unit (EDU) Segmentation is the process of dividing a continuous text or spoken discourse into its constituent units of meaning, often referred to as elementary discourse units (EDUs). These EDUs are typically short, coherent segments of text that represent individual ideas or thoughts within a larger discourse.</dcterms:description>
        <oboInOwl:hasSynonym xml:lang="en">EDU Segmentation</oboInOwl:hasSynonym>
        <rdfs:label xml:lang="en">Elementary Discourse Unit Segmentation</rdfs:label>
    </owl:NamedIndividual>
    


    <!-- http://nlpkg.sebis.cit.tum.de/nlp-fos-hierarchy.owl#Emotion-Cause_Pair_Extraction -->

    <owl:NamedIndividual rdf:about="http://nlpkg.sebis.cit.tum.de/nlp-fos-hierarchy.owl#Emotion-Cause_Pair_Extraction">
        <rdf:type rdf:resource="http://nlpkg.sebis.cit.tum.de/nlp-fos-hierarchy.owl#Task"/>
        <rdf:type rdf:resource="http://nlpkg.sebis.cit.tum.de/nlp-taxonomy.owl#FieldOfStudy"/>
        <nlp-taxonomy:subFieldOf rdf:resource="http://nlpkg.sebis.cit.tum.de/nlp-fos-hierarchy.owl#Emotion_Cause_Analysis"/>
        <code>https://github.com/NUSTM/ECPE</code>
        <origin>https://aclanthology.org/P19-1096</origin>
        <nlp-taxonomy:level rdf:datatype="http://www.w3.org/2001/XMLSchema#integer">4</nlp-taxonomy:level>
        <nlp-taxonomy:level rdf:datatype="http://www.w3.org/2001/XMLSchema#integer">5</nlp-taxonomy:level>
        <dcterms:description xml:lang="en">Emotion-Cause Pair Extraction (ECPE) aims to extract the potential pairs of emotions and corresponding causes in a document. Typically it involves a 2-step approach to address the ECPE task, which first performs individual emotion extraction and cause extraction via multi-task learning, and then conduct emotion-cause pairing and filtering.</dcterms:description>
        <oboInOwl:hasSynonym xml:lang="en">ECPE</oboInOwl:hasSynonym>
        <rdfs:label xml:lang="en">Emotion-Cause Pair Extraction</rdfs:label>
    </owl:NamedIndividual>
    


    <!-- http://nlpkg.sebis.cit.tum.de/nlp-fos-hierarchy.owl#Emotion_Cause_Analysis -->

    <owl:NamedIndividual rdf:about="http://nlpkg.sebis.cit.tum.de/nlp-fos-hierarchy.owl#Emotion_Cause_Analysis">
        <rdf:type rdf:resource="http://nlpkg.sebis.cit.tum.de/nlp-fos-hierarchy.owl#Task"/>
        <rdf:type rdf:resource="http://nlpkg.sebis.cit.tum.de/nlp-taxonomy.owl#FieldOfStudy"/>
        <nlp-taxonomy:subFieldOf rdf:resource="http://nlpkg.sebis.cit.tum.de/nlp-taxonomy.owl#Emotion_Analysis"/>
        <nlp-taxonomy:superFieldOf rdf:resource="http://nlpkg.sebis.cit.tum.de/nlp-fos-hierarchy.owl#Emotion-Cause_Pair_Extraction"/>
        <nlp-taxonomy:level rdf:datatype="http://www.w3.org/2001/XMLSchema#integer">3</nlp-taxonomy:level>
        <nlp-taxonomy:level rdf:datatype="http://www.w3.org/2001/XMLSchema#integer">4</nlp-taxonomy:level>
        <dcterms:description xml:lang="en">Emotion Cause Analysis refers to the process of identifying and understanding the causes or reasons behind certain emotional expressions in a given text. It involves determining what events, entities, or situations have triggered specific emotions.</dcterms:description>
        <oboInOwl:hasSynonym xml:lang="en">ECE</oboInOwl:hasSynonym>
        <oboInOwl:hasSynonym xml:lang="en">Emotion Cause Extraction</oboInOwl:hasSynonym>
        <rdfs:label xml:lang="en">Emotion Cause Analysis</rdfs:label>
    </owl:NamedIndividual>
    


    <!-- http://nlpkg.sebis.cit.tum.de/nlp-fos-hierarchy.owl#Ensemble_Models -->

    <owl:NamedIndividual rdf:about="http://nlpkg.sebis.cit.tum.de/nlp-fos-hierarchy.owl#Ensemble_Models">
        <rdf:type rdf:resource="http://nlpkg.sebis.cit.tum.de/nlp-fos-hierarchy.owl#Method"/>
        <rdf:type rdf:resource="http://nlpkg.sebis.cit.tum.de/nlp-taxonomy.owl#FieldOfStudy"/>
        <nlp-taxonomy:subFieldOf rdf:resource="http://nlpkg.sebis.cit.tum.de/nlp-fos-hierarchy.owl#Multi-Agent_Systems_&amp;_Multi-Model_Language_Models"/>
        <nlp-taxonomy:level rdf:datatype="http://www.w3.org/2001/XMLSchema#integer">4</nlp-taxonomy:level>
        <dcterms:description xml:lang="en">Ensemble Models refer to the method of combining multiple machine learning models to improve the overall performance and accuracy in solving complex problems. This approach helps in reducing overfitting, improving the robustness of the model, and increasing the generalizability of the predictions.</dcterms:description>
        <oboInOwl:hasSynonym xml:lang="en">Ensembles</oboInOwl:hasSynonym>
        <rdfs:label xml:lang="en">Ensemble Models</rdfs:label>
    </owl:NamedIndividual>
    


    <!-- http://nlpkg.sebis.cit.tum.de/nlp-fos-hierarchy.owl#Entity-Level_Sentiment_Analysis -->

    <owl:NamedIndividual rdf:about="http://nlpkg.sebis.cit.tum.de/nlp-fos-hierarchy.owl#Entity-Level_Sentiment_Analysis">
        <rdf:type rdf:resource="http://nlpkg.sebis.cit.tum.de/nlp-fos-hierarchy.owl#Task"/>
        <rdf:type rdf:resource="http://nlpkg.sebis.cit.tum.de/nlp-taxonomy.owl#FieldOfStudy"/>
        <uses rdf:resource="http://nlpkg.sebis.cit.tum.de/nlp-fos-hierarchy.owl#Anaphora_Resolution"/>
        <uses rdf:resource="http://nlpkg.sebis.cit.tum.de/nlp-fos-hierarchy.owl#Entity_Resolution"/>
        <uses rdf:resource="http://nlpkg.sebis.cit.tum.de/nlp-taxonomy.owl#Coreference_Resolution"/>
        <uses rdf:resource="http://nlpkg.sebis.cit.tum.de/nlp-taxonomy.owl#Named_Entity_Recognition"/>
        <nlp-taxonomy:subFieldOf rdf:resource="http://nlpkg.sebis.cit.tum.de/nlp-taxonomy.owl#Sentiment_Analysis"/>
        <survey>https://aclanthology.org/2022.coling-1.589</survey>
        <nlp-taxonomy:level rdf:datatype="http://www.w3.org/2001/XMLSchema#integer">2</nlp-taxonomy:level>
        <dcterms:description xml:lang="en">Entity-Level Sentiment Analysis (ELSA) refers to the task of identifying the overall sentiment expressed towards volitional entities (persons and organizations) in a document.</dcterms:description>
        <oboInOwl:hasSynonym xml:lang="en">ELSA</oboInOwl:hasSynonym>
        <oboInOwl:hasSynonym xml:lang="en">Entity Sentiment Analysis</oboInOwl:hasSynonym>
        <rdfs:label xml:lang="en">Entity-Level Sentiment Analysis</rdfs:label>
    </owl:NamedIndividual>
    


    <!-- http://nlpkg.sebis.cit.tum.de/nlp-fos-hierarchy.owl#Entity-based_Coherence_Discourse_Relation_Recognition -->

    <owl:NamedIndividual rdf:about="http://nlpkg.sebis.cit.tum.de/nlp-fos-hierarchy.owl#Entity-based_Coherence_Discourse_Relation_Recognition">
        <rdf:type rdf:resource="http://nlpkg.sebis.cit.tum.de/nlp-fos-hierarchy.owl#Task"/>
        <rdf:type rdf:resource="http://nlpkg.sebis.cit.tum.de/nlp-taxonomy.owl#FieldOfStudy"/>
        <nlp-taxonomy:subFieldOf rdf:resource="http://nlpkg.sebis.cit.tum.de/nlp-fos-hierarchy.owl#Discourse_Relation_Recognition"/>
        <nlp-taxonomy:level rdf:datatype="http://www.w3.org/2001/XMLSchema#integer">4</nlp-taxonomy:level>
        <nlp-taxonomy:level rdf:datatype="http://www.w3.org/2001/XMLSchema#integer">5</nlp-taxonomy:level>
        <nlp-taxonomy:level rdf:datatype="http://www.w3.org/2001/XMLSchema#integer">9</nlp-taxonomy:level>
        <dcterms:description xml:lang="en">Entity-based Coherence Discourse Relation Recognition refers to the process of identifying and understanding the relationships between different entities (like people, places, things) in a text. This involves analyzing the coherence or logical consistency of the discourse, which is the way these entities and their relationships are presented and developed throughout the text.</dcterms:description>
        <oboInOwl:hasSynonym xml:lang="en">Entity-based Coherence Discourse Relation Extraction</oboInOwl:hasSynonym>
        <rdfs:label xml:lang="en">Entity-based Coherence Discourse Relation Recognition</rdfs:label>
    </owl:NamedIndividual>
    


    <!-- http://nlpkg.sebis.cit.tum.de/nlp-fos-hierarchy.owl#Entity_Alignment -->

    <owl:NamedIndividual rdf:about="http://nlpkg.sebis.cit.tum.de/nlp-fos-hierarchy.owl#Entity_Alignment">
        <rdf:type rdf:resource="http://nlpkg.sebis.cit.tum.de/nlp-fos-hierarchy.owl#Task"/>
        <rdf:type rdf:resource="http://nlpkg.sebis.cit.tum.de/nlp-taxonomy.owl#FieldOfStudy"/>
        <nlp-taxonomy:subFieldOf rdf:resource="http://nlpkg.sebis.cit.tum.de/nlp-fos-hierarchy.owl#Knowledge_Graph_Construction_&amp;_Completion"/>
        <nlp-taxonomy:level rdf:datatype="http://www.w3.org/2001/XMLSchema#integer">7</nlp-taxonomy:level>
        <dcterms:description xml:lang="en">Entity Alignment refers to the process of identifying and linking entities in different knowledge bases that refer to the same real-world object. This is crucial in integrating information from various sources and enhancing the comprehensiveness and accuracy of knowledge graphs. It involves matching entities based on their attributes, relations, and contextual information.</dcterms:description>
        <rdfs:label xml:lang="en">Entity Alignment</rdfs:label>
    </owl:NamedIndividual>
    


    <!-- http://nlpkg.sebis.cit.tum.de/nlp-fos-hierarchy.owl#Entity_Linking -->

    <owl:NamedIndividual rdf:about="http://nlpkg.sebis.cit.tum.de/nlp-fos-hierarchy.owl#Entity_Linking">
        <rdf:type rdf:resource="http://nlpkg.sebis.cit.tum.de/nlp-fos-hierarchy.owl#Task"/>
        <rdf:type rdf:resource="http://nlpkg.sebis.cit.tum.de/nlp-taxonomy.owl#FieldOfStudy"/>
        <nlp-taxonomy:subFieldOf rdf:resource="http://nlpkg.sebis.cit.tum.de/nlp-fos-hierarchy.owl#Knowledge_Graph_Construction_&amp;_Completion"/>
        <survey>https://arxiv.org/abs/2006.00575</survey>
        <survey>https://arxiv.org/abs/2010.11075</survey>
        <survey>https://arxiv.org/abs/2112.01989</survey>
        <nlp-taxonomy:level rdf:datatype="http://www.w3.org/2001/XMLSchema#integer">7</nlp-taxonomy:level>
        <dcterms:description xml:lang="en">Entity Linking (or Named Entity Disambiguation) is a process that identifies specific entities in a text and links them to their corresponding entries in a knowledge base. This process helps in resolving ambiguities in text, as a single term can refer to multiple entities. For example, the term &quot;Apple&quot; could refer to the technology company or the fruit. Entity Linking helps in determining the correct entity based on the context of the text.</dcterms:description>
        <oboInOwl:hasSynonym xml:lang="en">Entity Matching</oboInOwl:hasSynonym>
        <oboInOwl:hasSynonym xml:lang="en">NED</oboInOwl:hasSynonym>
        <oboInOwl:hasSynonym xml:lang="en">NEL</oboInOwl:hasSynonym>
        <oboInOwl:hasSynonym xml:lang="en">NEN</oboInOwl:hasSynonym>
        <oboInOwl:hasSynonym xml:lang="en">NERD</oboInOwl:hasSynonym>
        <oboInOwl:hasSynonym xml:lang="en">Named Entity Disambiguation</oboInOwl:hasSynonym>
        <oboInOwl:hasSynonym xml:lang="en">Named Entity Linking</oboInOwl:hasSynonym>
        <oboInOwl:hasSynonym xml:lang="en">Named Entity Normalization</oboInOwl:hasSynonym>
        <oboInOwl:hasSynonym xml:lang="en">Named Entity Recognition and Disambiguation</oboInOwl:hasSynonym>
        <rdfs:label xml:lang="en">Entity Linking</rdfs:label>
    </owl:NamedIndividual>
    


    <!-- http://nlpkg.sebis.cit.tum.de/nlp-fos-hierarchy.owl#Entity_Resolution -->

    <owl:NamedIndividual rdf:about="http://nlpkg.sebis.cit.tum.de/nlp-fos-hierarchy.owl#Entity_Resolution">
        <rdf:type rdf:resource="http://nlpkg.sebis.cit.tum.de/nlp-fos-hierarchy.owl#Task"/>
        <rdf:type rdf:resource="http://nlpkg.sebis.cit.tum.de/nlp-taxonomy.owl#FieldOfStudy"/>
        <usedFor rdf:resource="http://nlpkg.sebis.cit.tum.de/nlp-fos-hierarchy.owl#Entity-Level_Sentiment_Analysis"/>
        <nlp-taxonomy:subFieldOf rdf:resource="http://nlpkg.sebis.cit.tum.de/nlp-fos-hierarchy.owl#Knowledge_Graph_Construction_&amp;_Completion"/>
        <nlp-taxonomy:level rdf:datatype="http://www.w3.org/2001/XMLSchema#integer">7</nlp-taxonomy:level>
        <dcterms:description xml:lang="en">Entity Resolution is the process of identifying and linking mentions of the same entity in texts or knowledge bases. It involves determining when two entities mentioned in texts or knowledge bases actually refer to the same thing, even if they are referred to in different ways. For example, &quot;Barack Obama&quot;, &quot;Obama&quot;, and &quot;the former president&quot; in texts and knowledge bases could all refer to the same person. Identifying and linking different representations of the same real-world entity (like a person, place, or thing) across various data sources helps in reducing data redundancy and improving the accuracy and reliability of a knowledge base.</dcterms:description>
        <rdfs:label xml:lang="en">Entity Resolution</rdfs:label>
    </owl:NamedIndividual>
    


    <!-- http://nlpkg.sebis.cit.tum.de/nlp-fos-hierarchy.owl#Euphemism_Detection -->

    <owl:NamedIndividual rdf:about="http://nlpkg.sebis.cit.tum.de/nlp-fos-hierarchy.owl#Euphemism_Detection">
        <rdf:type rdf:resource="http://nlpkg.sebis.cit.tum.de/nlp-fos-hierarchy.owl#Task"/>
        <rdf:type rdf:resource="http://nlpkg.sebis.cit.tum.de/nlp-taxonomy.owl#FieldOfStudy"/>
        <nlp-taxonomy:subFieldOf rdf:resource="http://nlpkg.sebis.cit.tum.de/nlp-fos-hierarchy.owl#Figurative_Language"/>
        <nlp-taxonomy:subFieldOf rdf:resource="http://nlpkg.sebis.cit.tum.de/nlp-taxonomy.owl#Text_Classification"/>
        <survey>https://aclanthology.org/2022.flp-1.18</survey>
        <nlp-taxonomy:level rdf:datatype="http://www.w3.org/2001/XMLSchema#integer">3</nlp-taxonomy:level>
        <nlp-taxonomy:level rdf:datatype="http://www.w3.org/2001/XMLSchema#integer">4</nlp-taxonomy:level>
        <dcterms:description xml:lang="en">Euphemism Detection is a task to detect words or phrases that are used to softens an uncomfortable topic. Euphemism is a ubiquitous figurative language tool, wherein the speaker refers to taboo topics in indirect, metaphorical terms to convey politeness or formality. Identifying euphemism can reveal tacit facts about the speaker’s intention and the context of the utterance.</dcterms:description>
        <oboInOwl:hasSynonym xml:lang="en">Euphemism Classification</oboInOwl:hasSynonym>
        <oboInOwl:hasSynonym xml:lang="en">Euphemism Identification</oboInOwl:hasSynonym>
        <rdfs:label xml:lang="en">Euphemism Detection</rdfs:label>
    </owl:NamedIndividual>
    


    <!-- http://nlpkg.sebis.cit.tum.de/nlp-fos-hierarchy.owl#Evaluation -->

    <owl:NamedIndividual rdf:about="http://nlpkg.sebis.cit.tum.de/nlp-fos-hierarchy.owl#Evaluation">
        <rdf:type rdf:resource="http://nlpkg.sebis.cit.tum.de/nlp-fos-hierarchy.owl#Task"/>
        <rdf:type rdf:resource="http://nlpkg.sebis.cit.tum.de/nlp-taxonomy.owl#FieldOfStudy"/>
        <nlp-taxonomy:subFieldOf rdf:resource="http://nlpkg.sebis.cit.tum.de/nlp-taxonomy.owl#Natural_Language_Processing"/>
        <relevantInformation>https://aclanthology.org/venues/eval4nlp/</relevantInformation>
        <relevantInformation>https://aclanthology.org/venues/gem/</relevantInformation>
        <survey>https://aclanthology.org/2020.acl-main.491</survey>
        <survey>https://aclanthology.org/2020.emnlp-main.751</survey>
        <survey>https://aclanthology.org/2020.eval4nlp-1.10</survey>
        <survey>https://aclanthology.org/2020.inlg-1.19</survey>
        <survey>https://aclanthology.org/2021.acl-long.148</survey>
        <survey>https://aclanthology.org/2021.acl-long.565</survey>
        <survey>https://aclanthology.org/2021.eacl-main.160</survey>
        <survey>https://aclanthology.org/2021.gem-1.6</survey>
        <survey>https://aclanthology.org/2021.gem-1.9/</survey>
        <survey>https://aclanthology.org/2021.humeval-1.8</survey>
        <survey>https://aclanthology.org/2021.motra-1.3</survey>
        <survey>https://aclanthology.org/2021.tacl-1.24</survey>
        <survey>https://aclanthology.org/2022.insights-1.25</survey>
        <survey>https://aclanthology.org/2022.lrec-1.804</survey>
        <survey>https://aclanthology.org/2022.nlppower-1.1</survey>
        <survey>https://aclanthology.org/2023.acl-long.307</survey>
        <survey>https://aclanthology.org/2023.findings-acl.139</survey>
        <survey>https://aclanthology.org/D18-1269</survey>
        <survey>https://aclanthology.org/E06-1032</survey>
        <survey>https://aclanthology.org/P19-1164</survey>
        <survey>https://aclanthology.org/Q18-1008</survey>
        <survey>https://aclanthology.org/W13-0102</survey>
        <survey>https://aclanthology.org/W17-5522</survey>
        <survey>https://aclanthology.org/W19-0418</survey>
        <survey>https://arxiv.org/abs/1605.04515</survey>
        <survey>https://arxiv.org/abs/1709.04409</survey>
        <survey>https://arxiv.org/abs/1801.09536</survey>
        <survey>https://arxiv.org/abs/1905.04071</survey>
        <survey>https://arxiv.org/abs/2005.00816</survey>
        <survey>https://arxiv.org/abs/2006.14799</survey>
        <survey>https://arxiv.org/abs/2008.12009</survey>
        <survey>https://arxiv.org/abs/2010.03061</survey>
        <survey>https://arxiv.org/abs/2105.11197</survey>
        <survey>https://arxiv.org/abs/2106.04747</survey>
        <survey>https://arxiv.org/abs/2108.01369</survey>
        <survey>https://arxiv.org/abs/2202.06935</survey>
        <survey>https://arxiv.org/abs/2206.15030</survey>
        <survey>https://arxiv.org/abs/2210.07566</survey>
        <survey>https://arxiv.org/abs/2306.15261</survey>
        <survey>https://arxiv.org/abs/2307.03109</survey>
        <survey>https://arxiv.org/abs/2308.07902</survey>
        <survey>https://arxiv.org/abs/2308.11696</survey>
        <survey>https://arxiv.org/abs/2310.13650</survey>
        <survey>https://arxiv.org/abs/2310.14424</survey>
        <survey>https://arxiv.org/abs/2310.17514</survey>
        <survey>https://arxiv.org/abs/2310.18018</survey>
        <survey>https://arxiv.org/abs/2310.19736</survey>
        <survey>https://arxiv.org/abs/2311.00681</survey>
        <survey>https://arxiv.org/abs/2311.00686</survey>
        <survey>https://arxiv.org/abs/2311.01964</survey>
        <survey>https://arxiv.org/abs/2311.02049</survey>
        <survey>https://arxiv.org/abs/2401.07103</survey>
        <nlp-taxonomy:level rdf:datatype="http://www.w3.org/2001/XMLSchema#integer">1</nlp-taxonomy:level>
        <dcterms:description xml:lang="en">Evaluation refers to the process of determining the performance or accuracy of a model or algorithm. It involves comparing the model&apos;s predictions or outputs against a set of pre-defined correct results (ground truth or gold labels). The choice of evaluation method usually depends on the specific task or problem at hand.</dcterms:description>
        <rdfs:label xml:lang="en">Evaluation</rdfs:label>
    </owl:NamedIndividual>
    


    <!-- http://nlpkg.sebis.cit.tum.de/nlp-fos-hierarchy.owl#Event_Argument_Extraction -->

    <owl:NamedIndividual rdf:about="http://nlpkg.sebis.cit.tum.de/nlp-fos-hierarchy.owl#Event_Argument_Extraction">
        <rdf:type rdf:resource="http://nlpkg.sebis.cit.tum.de/nlp-fos-hierarchy.owl#Task"/>
        <rdf:type rdf:resource="http://nlpkg.sebis.cit.tum.de/nlp-taxonomy.owl#FieldOfStudy"/>
        <nlp-taxonomy:subFieldOf rdf:resource="http://nlpkg.sebis.cit.tum.de/nlp-fos-hierarchy.owl#Argument_Extraction"/>
        <nlp-taxonomy:subFieldOf rdf:resource="http://nlpkg.sebis.cit.tum.de/nlp-taxonomy.owl#Event_Extraction"/>
        <nlp-taxonomy:level rdf:datatype="http://www.w3.org/2001/XMLSchema#integer">3</nlp-taxonomy:level>
        <nlp-taxonomy:level rdf:datatype="http://www.w3.org/2001/XMLSchema#integer">4</nlp-taxonomy:level>
        <dcterms:description xml:lang="en">Event Argument Extraction is a task that involves identifying and classifying the roles of entities in events described in text.</dcterms:description>
        <rdfs:label xml:lang="en">Event Argument Extraction</rdfs:label>
    </owl:NamedIndividual>
    


    <!-- http://nlpkg.sebis.cit.tum.de/nlp-fos-hierarchy.owl#Event_Coreference_Resolution -->

    <owl:NamedIndividual rdf:about="http://nlpkg.sebis.cit.tum.de/nlp-fos-hierarchy.owl#Event_Coreference_Resolution">
        <rdf:type rdf:resource="http://nlpkg.sebis.cit.tum.de/nlp-fos-hierarchy.owl#Task"/>
        <rdf:type rdf:resource="http://nlpkg.sebis.cit.tum.de/nlp-taxonomy.owl#FieldOfStudy"/>
        <nlp-taxonomy:subFieldOf rdf:resource="http://nlpkg.sebis.cit.tum.de/nlp-taxonomy.owl#Coreference_Resolution"/>
        <nlp-taxonomy:subFieldOf rdf:resource="http://nlpkg.sebis.cit.tum.de/nlp-taxonomy.owl#Event_Extraction"/>
        <nlp-taxonomy:level rdf:datatype="http://www.w3.org/2001/XMLSchema#integer">3</nlp-taxonomy:level>
        <dcterms:description xml:lang="en">Event Coreference Resolution refers to the task of determining when two expressions in a text refer to the same event. This is crucial for understanding the context and semantics of a text, as it helps in linking different parts of a text that are talking about the same event.</dcterms:description>
        <oboInOwl:hasSynonym xml:lang="en">ECR</oboInOwl:hasSynonym>
        <rdfs:label xml:lang="en">Event Coreference Resolution</rdfs:label>
    </owl:NamedIndividual>
    


    <!-- http://nlpkg.sebis.cit.tum.de/nlp-fos-hierarchy.owl#Event_Detection -->

    <owl:NamedIndividual rdf:about="http://nlpkg.sebis.cit.tum.de/nlp-fos-hierarchy.owl#Event_Detection">
        <rdf:type rdf:resource="http://nlpkg.sebis.cit.tum.de/nlp-fos-hierarchy.owl#Task"/>
        <rdf:type rdf:resource="http://nlpkg.sebis.cit.tum.de/nlp-taxonomy.owl#FieldOfStudy"/>
        <nlp-taxonomy:subFieldOf rdf:resource="http://nlpkg.sebis.cit.tum.de/nlp-taxonomy.owl#Event_Extraction"/>
        <nlp-taxonomy:subFieldOf rdf:resource="http://nlpkg.sebis.cit.tum.de/nlp-taxonomy.owl#Text_Classification"/>
        <nlp-taxonomy:level rdf:datatype="http://www.w3.org/2001/XMLSchema#integer">3</nlp-taxonomy:level>
        <dcterms:description xml:lang="en">Event Detection refers to the process of identifying and categorizing specific events or occurrences within a text. These instances can be anything from a simple action, such as a transaction, to a complex incident, like a natural disaster.</dcterms:description>
        <oboInOwl:hasSynonym xml:lang="en">Event Classification</oboInOwl:hasSynonym>
        <oboInOwl:hasSynonym xml:lang="en">Event Identification</oboInOwl:hasSynonym>
        <rdfs:label xml:lang="en">Event Detection</rdfs:label>
    </owl:NamedIndividual>
    


    <!-- http://nlpkg.sebis.cit.tum.de/nlp-fos-hierarchy.owl#Event_Discourse_Deixis_Resolution -->

    <owl:NamedIndividual rdf:about="http://nlpkg.sebis.cit.tum.de/nlp-fos-hierarchy.owl#Event_Discourse_Deixis_Resolution">
        <rdf:type rdf:resource="http://nlpkg.sebis.cit.tum.de/nlp-fos-hierarchy.owl#Task"/>
        <rdf:type rdf:resource="http://nlpkg.sebis.cit.tum.de/nlp-taxonomy.owl#FieldOfStudy"/>
        <nlp-taxonomy:subFieldOf rdf:resource="http://nlpkg.sebis.cit.tum.de/nlp-fos-hierarchy.owl#Discourse_Deixis_Resolution"/>
        <nlp-taxonomy:level rdf:datatype="http://www.w3.org/2001/XMLSchema#integer">4</nlp-taxonomy:level>
        <nlp-taxonomy:level rdf:datatype="http://www.w3.org/2001/XMLSchema#integer">5</nlp-taxonomy:level>
        <dcterms:description xml:lang="en">Event Discourse Deixis Resolution (EDDR) refers to the process of identifying and interpreting the meaning of event-related expressions within a given conversation or discourse. These expressions, also known as deictic expressions, are context-dependent and their understanding requires knowledge about the situation, time, or location in which they are used. EDDR involves resolving these expressions to provide accurate understanding and representation of the text.</dcterms:description>
        <oboInOwl:hasSynonym xml:lang="en">EDDR</oboInOwl:hasSynonym>
        <rdfs:label xml:lang="en">Event Discourse Deixis Resolution</rdfs:label>
    </owl:NamedIndividual>
    


    <!-- http://nlpkg.sebis.cit.tum.de/nlp-fos-hierarchy.owl#Event_Sequencing -->

    <owl:NamedIndividual rdf:about="http://nlpkg.sebis.cit.tum.de/nlp-fos-hierarchy.owl#Event_Sequencing">
        <rdf:type rdf:resource="http://nlpkg.sebis.cit.tum.de/nlp-fos-hierarchy.owl#Task"/>
        <rdf:type rdf:resource="http://nlpkg.sebis.cit.tum.de/nlp-taxonomy.owl#FieldOfStudy"/>
        <nlp-taxonomy:subFieldOf rdf:resource="http://nlpkg.sebis.cit.tum.de/nlp-taxonomy.owl#Event_Extraction"/>
        <survey>https://arxiv.org/abs/2202.07941</survey>
        <nlp-taxonomy:level rdf:datatype="http://www.w3.org/2001/XMLSchema#integer">3</nlp-taxonomy:level>
        <dcterms:description xml:lang="en">Event Sequencing refers to the process of identifying and understanding the order of events as they occur in a text. This involves determining the temporal relationships between different events. Event sequencing helps in understanding the storyline or narrative structure of a text.</dcterms:description>
        <oboInOwl:hasSynonym xml:lang="en">Event Sequence Analysis</oboInOwl:hasSynonym>
        <rdfs:label xml:lang="en">Event Sequencing</rdfs:label>
    </owl:NamedIndividual>
    


    <!-- http://nlpkg.sebis.cit.tum.de/nlp-fos-hierarchy.owl#Evidence_Mining -->

    <owl:NamedIndividual rdf:about="http://nlpkg.sebis.cit.tum.de/nlp-fos-hierarchy.owl#Evidence_Mining">
        <rdf:type rdf:resource="http://nlpkg.sebis.cit.tum.de/nlp-fos-hierarchy.owl#Task"/>
        <rdf:type rdf:resource="http://nlpkg.sebis.cit.tum.de/nlp-taxonomy.owl#FieldOfStudy"/>
        <uses rdf:resource="http://nlpkg.sebis.cit.tum.de/nlp-fos-hierarchy.owl#Stance_Detection"/>
        <nlp-taxonomy:subFieldOf rdf:resource="http://nlpkg.sebis.cit.tum.de/nlp-fos-hierarchy.owl#Factual_Verification"/>
        <nlp-taxonomy:subFieldOf rdf:resource="http://nlpkg.sebis.cit.tum.de/nlp-taxonomy.owl#Text_Classification"/>
        <nlp-taxonomy:level rdf:datatype="http://www.w3.org/2001/XMLSchema#integer">3</nlp-taxonomy:level>
        <nlp-taxonomy:level rdf:datatype="http://www.w3.org/2001/XMLSchema#integer">4</nlp-taxonomy:level>
        <dcterms:description xml:lang="en">Evidence Mining is the process of retrieving and extracting useful and relevant information or &apos;evidence&apos; from unstructured text data. This can involve identifying patterns, relationships, facts, sentiments, and other insights from text documents, social media posts, reviews, etc. Commonly, the task is being modeled that given a hypothesis as a query triplet, find the textual evidence sentences in a corpus that support the input query.</dcterms:description>
        <oboInOwl:hasSynonym xml:lang="en">Evidence Classification</oboInOwl:hasSynonym>
        <oboInOwl:hasSynonym xml:lang="en">Evidence Detection</oboInOwl:hasSynonym>
        <oboInOwl:hasSynonym xml:lang="en">Evidence Identification</oboInOwl:hasSynonym>
        <oboInOwl:hasSynonym xml:lang="en">Evidence Retrieval</oboInOwl:hasSynonym>
        <oboInOwl:hasSynonym xml:lang="en">Textual Evidence Mining</oboInOwl:hasSynonym>
        <rdfs:label xml:lang="en">Evidence Mining</rdfs:label>
    </owl:NamedIndividual>
    


    <!-- http://nlpkg.sebis.cit.tum.de/nlp-fos-hierarchy.owl#Explicit_Discourse_Relation_Recognition -->

    <owl:NamedIndividual rdf:about="http://nlpkg.sebis.cit.tum.de/nlp-fos-hierarchy.owl#Explicit_Discourse_Relation_Recognition">
        <rdf:type rdf:resource="http://nlpkg.sebis.cit.tum.de/nlp-fos-hierarchy.owl#Task"/>
        <rdf:type rdf:resource="http://nlpkg.sebis.cit.tum.de/nlp-taxonomy.owl#FieldOfStudy"/>
        <nlp-taxonomy:subFieldOf rdf:resource="http://nlpkg.sebis.cit.tum.de/nlp-fos-hierarchy.owl#Discourse_Relation_Recognition"/>
        <nlp-taxonomy:level rdf:datatype="http://www.w3.org/2001/XMLSchema#integer">4</nlp-taxonomy:level>
        <nlp-taxonomy:level rdf:datatype="http://www.w3.org/2001/XMLSchema#integer">5</nlp-taxonomy:level>
        <nlp-taxonomy:level rdf:datatype="http://www.w3.org/2001/XMLSchema#integer">9</nlp-taxonomy:level>
        <dcterms:description xml:lang="en">Explicit Discourse Relation Recognition refers to the task of identifying and classifying the relationship between two or more sentences or clauses in a text based on explicit discourse connectives. These connectives are words or phrases like &quot;because&quot;, &quot;however&quot;, &quot;in addition&quot;, which explicitly signal the type of discourse relation such as cause-effect, contrast, or addition. This recognition is crucial for understanding the overall coherence and meaning of a text.</dcterms:description>
        <oboInOwl:hasSynonym xml:lang="en">EDRR</oboInOwl:hasSynonym>
        <oboInOwl:hasSynonym xml:lang="en">Explicit Discourse Relation Extraction</oboInOwl:hasSynonym>
        <rdfs:label xml:lang="en">Explicit Discourse Relation Recognition</rdfs:label>
    </owl:NamedIndividual>
    


    <!-- http://nlpkg.sebis.cit.tum.de/nlp-fos-hierarchy.owl#Explicit_Semantic_Role_Labeling -->

    <owl:NamedIndividual rdf:about="http://nlpkg.sebis.cit.tum.de/nlp-fos-hierarchy.owl#Explicit_Semantic_Role_Labeling">
        <rdf:type rdf:resource="http://nlpkg.sebis.cit.tum.de/nlp-fos-hierarchy.owl#Task"/>
        <rdf:type rdf:resource="http://nlpkg.sebis.cit.tum.de/nlp-taxonomy.owl#FieldOfStudy"/>
        <nlp-taxonomy:subFieldOf rdf:resource="http://nlpkg.sebis.cit.tum.de/nlp-fos-hierarchy.owl#Slot_Filling"/>
        <nlp-taxonomy:level rdf:datatype="http://www.w3.org/2001/XMLSchema#integer">4</nlp-taxonomy:level>
        <dcterms:description xml:lang="en">Explicit Semantic Role Labeling (ESRL) is the task of assigning labels to words or phrases in a sentence that indicate their semantic role in the sentence. These roles can include the agent (doer of the action), the patient (receiver of the action), the instrument (means by which the action is performed), etc. The goal is to achieve a deeper understanding of the sentence by identifying how different components relate to each other.</dcterms:description>
        <oboInOwl:hasSynonym xml:lang="en">ESRL</oboInOwl:hasSynonym>
        <rdfs:label xml:lang="en">Explicit Semantic Role Labeling</rdfs:label>
    </owl:NamedIndividual>
    


    <!-- http://nlpkg.sebis.cit.tum.de/nlp-fos-hierarchy.owl#Exposure_Bias -->

    <owl:NamedIndividual rdf:about="http://nlpkg.sebis.cit.tum.de/nlp-fos-hierarchy.owl#Exposure_Bias">
        <rdf:type rdf:resource="http://nlpkg.sebis.cit.tum.de/nlp-fos-hierarchy.owl#OtherScientificField"/>
        <rdf:type rdf:resource="http://nlpkg.sebis.cit.tum.de/nlp-taxonomy.owl#FieldOfStudy"/>
        <nlp-taxonomy:subFieldOf rdf:resource="http://nlpkg.sebis.cit.tum.de/nlp-fos-hierarchy.owl#Biases_&amp;_Fairness_in_NLP"/>
        <survey>https://aclanthology.org/2022.findings-acl.58</survey>
        <nlp-taxonomy:level rdf:datatype="http://www.w3.org/2001/XMLSchema#integer">4</nlp-taxonomy:level>
        <dcterms:description xml:lang="en">Exposure Bias refers to the discrepancy between the training and testing phases of a language model. During training, the model is exposed to the ground truth data at each step, but during testing, the model only sees its own predictions. This can lead to the accumulation of errors during testing, as the model has not been trained to correct its own mistakes. This discrepancy and its potential impact on the model&apos;s performance is known as Exposure Bias.</dcterms:description>
        <rdfs:label xml:lang="en">Exposure Bias</rdfs:label>
    </owl:NamedIndividual>
    


    <!-- http://nlpkg.sebis.cit.tum.de/nlp-fos-hierarchy.owl#Extractive_Question_Answering -->

    <owl:NamedIndividual rdf:about="http://nlpkg.sebis.cit.tum.de/nlp-fos-hierarchy.owl#Extractive_Question_Answering">
        <rdf:type rdf:resource="http://nlpkg.sebis.cit.tum.de/nlp-fos-hierarchy.owl#Task"/>
        <rdf:type rdf:resource="http://nlpkg.sebis.cit.tum.de/nlp-taxonomy.owl#FieldOfStudy"/>
        <nlp-taxonomy:subFieldOf rdf:resource="http://nlpkg.sebis.cit.tum.de/nlp-taxonomy.owl#Question_Answering"/>
        <nlp-taxonomy:level rdf:datatype="http://www.w3.org/2001/XMLSchema#integer">3</nlp-taxonomy:level>
        <dcterms:description xml:lang="en">Extractive Question Answering is task where a model extracts a specific span of text or passage from a given document to answer a question. The model selects and outputs a segment of text directly from the source document that contains the answer to the question. Extractive QA systems are designed to identify and extract the most relevant information from a text corpus to provide accurate answers to user queries.</dcterms:description>
        <oboInOwl:hasSynonym xml:lang="en">Extractive QA</oboInOwl:hasSynonym>
        <rdfs:label xml:lang="en">Extractive Question Answering</rdfs:label>
    </owl:NamedIndividual>
    


    <!-- http://nlpkg.sebis.cit.tum.de/nlp-fos-hierarchy.owl#Extractive_Summarization -->

    <owl:NamedIndividual rdf:about="http://nlpkg.sebis.cit.tum.de/nlp-fos-hierarchy.owl#Extractive_Summarization">
        <rdf:type rdf:resource="http://nlpkg.sebis.cit.tum.de/nlp-fos-hierarchy.owl#Task"/>
        <rdf:type rdf:resource="http://nlpkg.sebis.cit.tum.de/nlp-taxonomy.owl#FieldOfStudy"/>
        <nlp-taxonomy:subFieldOf rdf:resource="http://nlpkg.sebis.cit.tum.de/nlp-taxonomy.owl#Summarization"/>
        <nlp-taxonomy:level rdf:datatype="http://www.w3.org/2001/XMLSchema#integer">3</nlp-taxonomy:level>
        <dcterms:description xml:lang="en">Extractive Summarization involves automatically selecting and extracting key sentences or phrases from a text document to create a concise summary. Extractive Summarization identifies and reuses the most informative and relevant content from the original text to produce a summary that captures the main ideas and important details.</dcterms:description>
        <oboInOwl:hasSynonym xml:lang="en">Extractive Summarisation</oboInOwl:hasSynonym>
        <rdfs:label xml:lang="en">Extractive Summarization</rdfs:label>
    </owl:NamedIndividual>
    


    <!-- http://nlpkg.sebis.cit.tum.de/nlp-fos-hierarchy.owl#Fact_Discourse_Deixis_Resolution -->

    <owl:NamedIndividual rdf:about="http://nlpkg.sebis.cit.tum.de/nlp-fos-hierarchy.owl#Fact_Discourse_Deixis_Resolution">
        <rdf:type rdf:resource="http://nlpkg.sebis.cit.tum.de/nlp-fos-hierarchy.owl#Task"/>
        <rdf:type rdf:resource="http://nlpkg.sebis.cit.tum.de/nlp-taxonomy.owl#FieldOfStudy"/>
        <nlp-taxonomy:subFieldOf rdf:resource="http://nlpkg.sebis.cit.tum.de/nlp-fos-hierarchy.owl#Discourse_Deixis_Resolution"/>
        <nlp-taxonomy:level rdf:datatype="http://www.w3.org/2001/XMLSchema#integer">4</nlp-taxonomy:level>
        <nlp-taxonomy:level rdf:datatype="http://www.w3.org/2001/XMLSchema#integer">5</nlp-taxonomy:level>
        <dcterms:description xml:lang="en">Fact Discourse Deixis Resolution (FDDR) refers to the process of identifying and interpreting factual information that is context-dependent within a discourse or conversation. Deixis are words or phrases that cannot be fully understood without additional contextual information. In the case of FDDR, the focus is on resolving the meaning of such expressions when they refer to factual information, which can be crucial for understanding the overall context and meaning of a text.</dcterms:description>
        <oboInOwl:hasSynonym xml:lang="en">FDDR</oboInOwl:hasSynonym>
        <rdfs:label xml:lang="en">Fact Discourse Deixis Resolution</rdfs:label>
    </owl:NamedIndividual>
    


    <!-- http://nlpkg.sebis.cit.tum.de/nlp-fos-hierarchy.owl#Factual_Verification -->

    <owl:NamedIndividual rdf:about="http://nlpkg.sebis.cit.tum.de/nlp-fos-hierarchy.owl#Factual_Verification">
        <rdf:type rdf:resource="http://nlpkg.sebis.cit.tum.de/nlp-fos-hierarchy.owl#Task"/>
        <rdf:type rdf:resource="http://nlpkg.sebis.cit.tum.de/nlp-taxonomy.owl#FieldOfStudy"/>
        <nlp-taxonomy:subFieldOf rdf:resource="http://nlpkg.sebis.cit.tum.de/nlp-taxonomy.owl#Fact_&amp;_Claim_Verification"/>
        <nlp-taxonomy:superFieldOf rdf:resource="http://nlpkg.sebis.cit.tum.de/nlp-fos-hierarchy.owl#Claim_Verification"/>
        <nlp-taxonomy:superFieldOf rdf:resource="http://nlpkg.sebis.cit.tum.de/nlp-fos-hierarchy.owl#Evidence_Mining"/>
        <survey>https://arxiv.org/abs/2010.03001</survey>
        <survey>https://arxiv.org/abs/2111.03299</survey>
        <survey>https://arxiv.org/abs/2309.09444</survey>
        <survey>https://arxiv.org/abs/2310.14564</survey>
        <nlp-taxonomy:level rdf:datatype="http://www.w3.org/2001/XMLSchema#integer">3</nlp-taxonomy:level>
        <dcterms:description xml:lang="en">Factual Verification (FV) refers to the task of finding reliable documents to verify a given claim and generate a verdict about the veracity of the claim.</dcterms:description>
        <oboInOwl:hasSynonym xml:lang="en">FV</oboInOwl:hasSynonym>
        <oboInOwl:hasSynonym xml:lang="en">Fact Extraction</oboInOwl:hasSynonym>
        <oboInOwl:hasSynonym xml:lang="en">Fact Verification</oboInOwl:hasSynonym>
        <rdfs:label xml:lang="en">Factual Verification</rdfs:label>
    </owl:NamedIndividual>
    


    <!-- http://nlpkg.sebis.cit.tum.de/nlp-fos-hierarchy.owl#Fake_News_Detection -->

    <owl:NamedIndividual rdf:about="http://nlpkg.sebis.cit.tum.de/nlp-fos-hierarchy.owl#Fake_News_Detection">
        <rdf:type rdf:resource="http://nlpkg.sebis.cit.tum.de/nlp-fos-hierarchy.owl#Task"/>
        <rdf:type rdf:resource="http://nlpkg.sebis.cit.tum.de/nlp-taxonomy.owl#FieldOfStudy"/>
        <uses rdf:resource="http://nlpkg.sebis.cit.tum.de/nlp-fos-hierarchy.owl#Stance_Detection"/>
        <nlp-taxonomy:subFieldOf rdf:resource="http://nlpkg.sebis.cit.tum.de/nlp-fos-hierarchy.owl#Misinformation_Detection"/>
        <survey>https://aclanthology.org/2020.lrec-1.747</survey>
        <survey>https://arxiv.org/abs/1812.00315</survey>
        <survey>https://arxiv.org/abs/1907.00181</survey>
        <survey>https://arxiv.org/abs/2110.11240</survey>
        <survey>https://arxiv.org/abs/2111.03299</survey>
        <survey>https://arxiv.org/abs/2112.11185</survey>
        <survey>https://arxiv.org/abs/2307.12639</survey>
        <nlp-taxonomy:level rdf:datatype="http://www.w3.org/2001/XMLSchema#integer">4</nlp-taxonomy:level>
        <dcterms:description xml:lang="en">Fake News Detection refers to the application of NLP techniques to identify and filter out false information or &quot;fake news&quot;. This involves analyzing the text data, and understanding the context, sentiment, and other linguistic features to determine the authenticity of the information.</dcterms:description>
        <oboInOwl:hasSynonym xml:lang="en">Fake News Classification</oboInOwl:hasSynonym>
        <oboInOwl:hasSynonym xml:lang="en">Fake News Identification</oboInOwl:hasSynonym>
        <rdfs:label xml:lang="en">Fake News Detection</rdfs:label>
    </owl:NamedIndividual>
    


    <!-- http://nlpkg.sebis.cit.tum.de/nlp-fos-hierarchy.owl#Federated_Learning -->

    <owl:NamedIndividual rdf:about="http://nlpkg.sebis.cit.tum.de/nlp-fos-hierarchy.owl#Federated_Learning">
        <rdf:type rdf:resource="http://nlpkg.sebis.cit.tum.de/nlp-fos-hierarchy.owl#Task"/>
        <rdf:type rdf:resource="http://nlpkg.sebis.cit.tum.de/nlp-taxonomy.owl#FieldOfStudy"/>
        <nlp-taxonomy:subFieldOf rdf:resource="http://nlpkg.sebis.cit.tum.de/nlp-fos-hierarchy.owl#Privacy,_Security_&amp;_Safety_in_NLP"/>
        <survey>https://aclanthology.org/2022.findings-naacl.13</survey>
        <survey>https://arxiv.org/abs/2107.12603</survey>
        <nlp-taxonomy:level rdf:datatype="http://www.w3.org/2001/XMLSchema#integer">4</nlp-taxonomy:level>
        <dcterms:description xml:lang="en">Federated Learning is a machine learning approach where a model is trained across multiple decentralized devices or servers holding local data samples, without exchanging them. This approach addresses privacy concerns and reduces the amount of data that needs to be sent over the network. The model learns from data located at the source, updates itself and shares only the model updates, keeping the raw data localized.</dcterms:description>
        <rdfs:label xml:lang="en">Federated Learning</rdfs:label>
    </owl:NamedIndividual>
    


    <!-- http://nlpkg.sebis.cit.tum.de/nlp-fos-hierarchy.owl#Few-shot_Learning -->

    <owl:NamedIndividual rdf:about="http://nlpkg.sebis.cit.tum.de/nlp-fos-hierarchy.owl#Few-shot_Learning">
        <rdf:type rdf:resource="http://nlpkg.sebis.cit.tum.de/nlp-fos-hierarchy.owl#Task"/>
        <rdf:type rdf:resource="http://nlpkg.sebis.cit.tum.de/nlp-taxonomy.owl#FieldOfStudy"/>
        <uses rdf:resource="http://nlpkg.sebis.cit.tum.de/nlp-fos-hierarchy.owl#Meta-Learning"/>
        <nlp-taxonomy:subFieldOf rdf:resource="http://nlpkg.sebis.cit.tum.de/nlp-taxonomy.owl#Language_Models"/>
        <nlp-taxonomy:subFieldOf rdf:resource="http://nlpkg.sebis.cit.tum.de/nlp-taxonomy.owl#Low-Resource_NLP"/>
        <nlp-taxonomy:subFieldOf rdf:resource="http://nlpkg.sebis.cit.tum.de/nlp-taxonomy.owl#Green_&amp;_Sustainable_NLP"/>
        <nlp-taxonomy:superFieldOf rdf:resource="http://nlpkg.sebis.cit.tum.de/nlp-fos-hierarchy.owl#In-Context_Learning"/>
        <survey>https://aclanthology.org/2023.findings-acl.779</survey>
        <survey>https://arxiv.org/abs/2007.09604</survey>
        <survey>https://arxiv.org/abs/2310.19055</survey>
        <nlp-taxonomy:level rdf:datatype="http://www.w3.org/2001/XMLSchema#integer">3</nlp-taxonomy:level>
        <dcterms:description xml:lang="en">Few-shot Learning (FSL) refers to the ability of a machine learning model to understand and start performing a task with a very small amount of training data, typically just a few examples. This concept is inspired by the human ability to acquire new knowledge with a small number of examples. In NLP, this could mean learning to understand and generate text in a new language or understanding the sentiment of a sentence with just a few training examples.</dcterms:description>
        <oboInOwl:hasSynonym xml:lang="en">FSL</oboInOwl:hasSynonym>
        <oboInOwl:hasSynonym xml:lang="en">Few shot</oboInOwl:hasSynonym>
        <oboInOwl:hasSynonym xml:lang="en">Few-shot</oboInOwl:hasSynonym>
        <rdfs:label xml:lang="en">Few-shot Learning</rdfs:label>
    </owl:NamedIndividual>
    


    <!-- http://nlpkg.sebis.cit.tum.de/nlp-fos-hierarchy.owl#Figurative_Language -->

    <owl:NamedIndividual rdf:about="http://nlpkg.sebis.cit.tum.de/nlp-fos-hierarchy.owl#Figurative_Language">
        <rdf:type rdf:resource="http://nlpkg.sebis.cit.tum.de/nlp-fos-hierarchy.owl#OtherScientificField"/>
        <rdf:type rdf:resource="http://nlpkg.sebis.cit.tum.de/nlp-taxonomy.owl#FieldOfStudy"/>
        <nlp-taxonomy:subFieldOf rdf:resource="http://nlpkg.sebis.cit.tum.de/nlp-taxonomy.owl#Stylistic_Analysis"/>
        <nlp-taxonomy:superFieldOf rdf:resource="http://nlpkg.sebis.cit.tum.de/nlp-fos-hierarchy.owl#Euphemism_Detection"/>
        <nlp-taxonomy:superFieldOf rdf:resource="http://nlpkg.sebis.cit.tum.de/nlp-fos-hierarchy.owl#Idiom_Identification"/>
        <survey>https://aclanthology.org/2022.tacl-1.34</survey>
        <nlp-taxonomy:level rdf:datatype="http://www.w3.org/2001/XMLSchema#integer">3</nlp-taxonomy:level>
        <dcterms:description xml:lang="en">Figurative Language refers to the use of words or expressions that deviate from their literal interpretation in order to achieve a particular effect or emphasis. This includes similes, personification, hyperbole, idioms, etc. Understanding and processing figurative language is a complex task in NLP as it requires contextual understanding and often cultural knowledge.</dcterms:description>
        <rdfs:label xml:lang="en">Figurative Language</rdfs:label>
    </owl:NamedIndividual>
    


    <!-- http://nlpkg.sebis.cit.tum.de/nlp-fos-hierarchy.owl#Gazetteers -->

    <owl:NamedIndividual rdf:about="http://nlpkg.sebis.cit.tum.de/nlp-fos-hierarchy.owl#Gazetteers">
        <rdf:type rdf:resource="http://nlpkg.sebis.cit.tum.de/nlp-fos-hierarchy.owl#DataStructure"/>
        <rdf:type rdf:resource="http://nlpkg.sebis.cit.tum.de/nlp-taxonomy.owl#FieldOfStudy"/>
        <usedFor rdf:resource="http://nlpkg.sebis.cit.tum.de/nlp-taxonomy.owl#Named_Entity_Recognition"/>
        <nlp-taxonomy:subFieldOf rdf:resource="http://nlpkg.sebis.cit.tum.de/nlp-fos-hierarchy.owl#Knowledge_Bases"/>
        <nlp-taxonomy:level rdf:datatype="http://www.w3.org/2001/XMLSchema#integer">4</nlp-taxonomy:level>
        <dcterms:description xml:lang="en">Gazetteers refer to lists of names or entities such as names of people, places, organizations, or even specific industry terms. They are used in information extraction and entity recognition tasks to identify and categorize words or phrases in a text. For example, a gazetteer could be used to identify all city or country names in a document.</dcterms:description>
        <rdfs:label xml:lang="en">Gazetteers</rdfs:label>
    </owl:NamedIndividual>
    


    <!-- http://nlpkg.sebis.cit.tum.de/nlp-fos-hierarchy.owl#Gender_Bias -->

    <owl:NamedIndividual rdf:about="http://nlpkg.sebis.cit.tum.de/nlp-fos-hierarchy.owl#Gender_Bias">
        <rdf:type rdf:resource="http://nlpkg.sebis.cit.tum.de/nlp-fos-hierarchy.owl#OtherScientificField"/>
        <rdf:type rdf:resource="http://nlpkg.sebis.cit.tum.de/nlp-taxonomy.owl#FieldOfStudy"/>
        <nlp-taxonomy:subFieldOf rdf:resource="http://nlpkg.sebis.cit.tum.de/nlp-fos-hierarchy.owl#Social_Bias"/>
        <survey>https://aclanthology.org/2020.acl-main.619</survey>
        <survey>https://aclanthology.org/2021.tacl-1.51</survey>
        <survey>https://aclanthology.org/P19-1159</survey>
        <survey>https://aclanthology.org/P19-1164</survey>
        <survey>https://aclanthology.org/W19-3805</survey>
        <survey>https://arxiv.org/abs/2112.14168</survey>
        <survey>https://arxiv.org/abs/2306.10530</survey>
        <survey>https://arxiv.org/abs/2310.17530</survey>
        <nlp-taxonomy:level rdf:datatype="http://www.w3.org/2001/XMLSchema#integer">5</nlp-taxonomy:level>
        <dcterms:description xml:lang="en">Gender Bias refers to the unequal treatment or perceptions of individuals based on their gender.</dcterms:description>
        <rdfs:label xml:lang="en">Gender Bias</rdfs:label>
    </owl:NamedIndividual>
    


    <!-- http://nlpkg.sebis.cit.tum.de/nlp-fos-hierarchy.owl#Generative_Dialogue_Response_Generation -->

    <owl:NamedIndividual rdf:about="http://nlpkg.sebis.cit.tum.de/nlp-fos-hierarchy.owl#Generative_Dialogue_Response_Generation">
        <rdf:type rdf:resource="http://nlpkg.sebis.cit.tum.de/nlp-fos-hierarchy.owl#Task"/>
        <rdf:type rdf:resource="http://nlpkg.sebis.cit.tum.de/nlp-taxonomy.owl#FieldOfStudy"/>
        <nlp-taxonomy:subFieldOf rdf:resource="http://nlpkg.sebis.cit.tum.de/nlp-taxonomy.owl#Dialogue_Response_Generation"/>
        <nlp-taxonomy:level rdf:datatype="http://www.w3.org/2001/XMLSchema#integer">3</nlp-taxonomy:level>
        <nlp-taxonomy:level rdf:datatype="http://www.w3.org/2001/XMLSchema#integer">4</nlp-taxonomy:level>
        <dcterms:description xml:lang="en">Generative Dialogue Response Generation refers to the process of generating natural and contextually relevant responses in a conversational setting. It involves the generation of text-based responses that mimic human conversation, making it appear as if a machine is engaging in a meaningful and coherent dialogue with a user.</dcterms:description>
        <rdfs:label xml:lang="en">Generative Dialogue Response Generation</rdfs:label>
    </owl:NamedIndividual>
    


    <!-- http://nlpkg.sebis.cit.tum.de/nlp-fos-hierarchy.owl#Generative_Question_Answering -->

    <owl:NamedIndividual rdf:about="http://nlpkg.sebis.cit.tum.de/nlp-fos-hierarchy.owl#Generative_Question_Answering">
        <rdf:type rdf:resource="http://nlpkg.sebis.cit.tum.de/nlp-fos-hierarchy.owl#Task"/>
        <rdf:type rdf:resource="http://nlpkg.sebis.cit.tum.de/nlp-taxonomy.owl#FieldOfStudy"/>
        <nlp-taxonomy:subFieldOf rdf:resource="http://nlpkg.sebis.cit.tum.de/nlp-taxonomy.owl#Question_Answering"/>
        <nlp-taxonomy:superFieldOf rdf:resource="http://nlpkg.sebis.cit.tum.de/nlp-fos-hierarchy.owl#Retrieval_Augmented_Generation"/>
        <nlp-taxonomy:level rdf:datatype="http://www.w3.org/2001/XMLSchema#integer">3</nlp-taxonomy:level>
        <dcterms:description xml:lang="en">Generative Question Answering is a task where a model generates human-like responses in natural language to answer questions posed by users. Instead of selecting a pre-existing answer from a set of options (as in multiple-choice questions), generative question answering models generate responses from scratch based on their understanding of the input question and available knowledge, making them capable of providing more contextually relevant and open-ended answers.</dcterms:description>
        <oboInOwl:hasSynonym xml:lang="en">Generative QA</oboInOwl:hasSynonym>
        <rdfs:label xml:lang="en">Generative Question Answering</rdfs:label>
    </owl:NamedIndividual>
    


    <!-- http://nlpkg.sebis.cit.tum.de/nlp-fos-hierarchy.owl#Goal_Hijacking -->

    <owl:NamedIndividual rdf:about="http://nlpkg.sebis.cit.tum.de/nlp-fos-hierarchy.owl#Goal_Hijacking">
        <rdf:type rdf:resource="http://nlpkg.sebis.cit.tum.de/nlp-fos-hierarchy.owl#Task"/>
        <rdf:type rdf:resource="http://nlpkg.sebis.cit.tum.de/nlp-taxonomy.owl#FieldOfStudy"/>
        <nlp-taxonomy:subFieldOf rdf:resource="http://nlpkg.sebis.cit.tum.de/nlp-fos-hierarchy.owl#Prompt_Injection"/>
        <code>https://github.com/agencyenterprise/PromptInject</code>
        <origin>https://arxiv.org/abs/2211.09527</origin>
        <relevantInformation>https://learnprompting.org/docs/prompt_hacking/jailbreaking</relevantInformation>
        <nlp-taxonomy:level rdf:datatype="http://www.w3.org/2001/XMLSchema#integer">5</nlp-taxonomy:level>
        <nlp-taxonomy:level rdf:datatype="http://www.w3.org/2001/XMLSchema#integer">6</nlp-taxonomy:level>
        <dcterms:description xml:lang="en">In Goal Hijacking the new goal is to print a specific target string, which may contain malicious instructions. This process uses prompt injection to specifically bypass safety and moderation features placed on LLMs by their creators. Jailbreaking usually refers to Chatbots which have successfully been prompt injected and now are in a state where the user can ask any question they would like.</dcterms:description>
        <oboInOwl:hasSynonym xml:lang="en">Jailbreaking</oboInOwl:hasSynonym>
        <rdfs:label xml:lang="en">Goal Hijacking</rdfs:label>
    </owl:NamedIndividual>
    


    <!-- http://nlpkg.sebis.cit.tum.de/nlp-fos-hierarchy.owl#Grammar_Induction -->

    <owl:NamedIndividual rdf:about="http://nlpkg.sebis.cit.tum.de/nlp-fos-hierarchy.owl#Grammar_Induction">
        <rdf:type rdf:resource="http://nlpkg.sebis.cit.tum.de/nlp-fos-hierarchy.owl#Task"/>
        <rdf:type rdf:resource="http://nlpkg.sebis.cit.tum.de/nlp-taxonomy.owl#FieldOfStudy"/>
        <nlp-taxonomy:subFieldOf rdf:resource="http://nlpkg.sebis.cit.tum.de/nlp-taxonomy.owl#Text_Error_Correction"/>
        <nlp-taxonomy:level rdf:datatype="http://www.w3.org/2001/XMLSchema#integer">3</nlp-taxonomy:level>
        <dcterms:description xml:lang="en">Grammar Induction refers to the process of learning the grammar rules of a language from raw data. This involves identifying patterns and structures in sentences and using these to formulate rules that can be used to understand or generate new sentences.</dcterms:description>
        <rdfs:label xml:lang="en">Grammar Induction</rdfs:label>
    </owl:NamedIndividual>
    


    <!-- http://nlpkg.sebis.cit.tum.de/nlp-fos-hierarchy.owl#Grammatical_Error_Correction -->

    <owl:NamedIndividual rdf:about="http://nlpkg.sebis.cit.tum.de/nlp-fos-hierarchy.owl#Grammatical_Error_Correction">
        <rdf:type rdf:resource="http://nlpkg.sebis.cit.tum.de/nlp-fos-hierarchy.owl#Task"/>
        <rdf:type rdf:resource="http://nlpkg.sebis.cit.tum.de/nlp-taxonomy.owl#FieldOfStudy"/>
        <nlp-taxonomy:subFieldOf rdf:resource="http://nlpkg.sebis.cit.tum.de/nlp-taxonomy.owl#Text_Error_Correction"/>
        <survey>https://aclanthology.org/2022.findings-acl.324</survey>
        <survey>https://arxiv.org/abs/1804.00540</survey>
        <survey>https://arxiv.org/abs/2005.06600</survey>
        <survey>https://arxiv.org/abs/2211.05166</survey>
        <nlp-taxonomy:level rdf:datatype="http://www.w3.org/2001/XMLSchema#integer">3</nlp-taxonomy:level>
        <dcterms:description xml:lang="en">Grammatical Error Correction (GEC) refers to the task of identifying and correcting grammatical mistakes in text.</dcterms:description>
        <oboInOwl:hasSynonym xml:lang="en">GEC</oboInOwl:hasSynonym>
        <oboInOwl:hasSynonym xml:lang="en">GED</oboInOwl:hasSynonym>
        <oboInOwl:hasSynonym xml:lang="en">Grammar Checking</oboInOwl:hasSynonym>
        <oboInOwl:hasSynonym xml:lang="en">Grammar Error Correction</oboInOwl:hasSynonym>
        <oboInOwl:hasSynonym xml:lang="en">Grammatical Error Diagnosis</oboInOwl:hasSynonym>
        <rdfs:label xml:lang="en">Grammatical Error Correction</rdfs:label>
    </owl:NamedIndividual>
    


    <!-- http://nlpkg.sebis.cit.tum.de/nlp-fos-hierarchy.owl#Graph-to-Text -->

    <owl:NamedIndividual rdf:about="http://nlpkg.sebis.cit.tum.de/nlp-fos-hierarchy.owl#Graph-to-Text">
        <rdf:type rdf:resource="http://nlpkg.sebis.cit.tum.de/nlp-fos-hierarchy.owl#Task"/>
        <rdf:type rdf:resource="http://nlpkg.sebis.cit.tum.de/nlp-taxonomy.owl#FieldOfStudy"/>
        <nlp-taxonomy:subFieldOf rdf:resource="http://nlpkg.sebis.cit.tum.de/nlp-fos-hierarchy.owl#Graphs"/>
        <nlp-taxonomy:subFieldOf rdf:resource="http://nlpkg.sebis.cit.tum.de/nlp-taxonomy.owl#Data-to-Text_Generation"/>
        <nlp-taxonomy:superFieldOf rdf:resource="http://nlpkg.sebis.cit.tum.de/nlp-fos-hierarchy.owl#AMR-to-Text"/>
        <survey>https://aclanthology.org/2021.nlp4convai-1.20</survey>
        <survey>https://arxiv.org/abs/2307.14712</survey>
        <nlp-taxonomy:level rdf:datatype="http://www.w3.org/2001/XMLSchema#integer">3</nlp-taxonomy:level>
        <nlp-taxonomy:level rdf:datatype="http://www.w3.org/2001/XMLSchema#integer">4</nlp-taxonomy:level>
        <nlp-taxonomy:level rdf:datatype="http://www.w3.org/2001/XMLSchema#integer">5</nlp-taxonomy:level>
        <dcterms:description xml:lang="en">Graph-to-Text Generation aims to generate fluent texts from graph-based data.</dcterms:description>
        <oboInOwl:hasSynonym xml:lang="en">Graph-to-Text Generation</oboInOwl:hasSynonym>
        <oboInOwl:hasSynonym xml:lang="en">KG-to-Text</oboInOwl:hasSynonym>
        <oboInOwl:hasSynonym xml:lang="en">Knowledge Graph-to-Text Generation</oboInOwl:hasSynonym>
        <rdfs:label xml:lang="en">Graph-to-Text</rdfs:label>
    </owl:NamedIndividual>
    


    <!-- http://nlpkg.sebis.cit.tum.de/nlp-fos-hierarchy.owl#Graph_Neural_Networks -->

    <owl:NamedIndividual rdf:about="http://nlpkg.sebis.cit.tum.de/nlp-fos-hierarchy.owl#Graph_Neural_Networks">
        <rdf:type rdf:resource="http://nlpkg.sebis.cit.tum.de/nlp-fos-hierarchy.owl#OtherScientificField"/>
        <rdf:type rdf:resource="http://nlpkg.sebis.cit.tum.de/nlp-taxonomy.owl#FieldOfStudy"/>
        <nlp-taxonomy:subFieldOf rdf:resource="http://nlpkg.sebis.cit.tum.de/nlp-fos-hierarchy.owl#Graphs"/>
        <code>https://github.com/graph4ai/graph4nlp</code>
        <survey>https://arxiv.org/abs/2106.06090</survey>
        <survey>https://graph-neural-networks.github.io/gnnbook_Chapter21.html</survey>
        <nlp-taxonomy:level rdf:datatype="http://www.w3.org/2001/XMLSchema#integer">5</nlp-taxonomy:level>
        <dcterms:description xml:lang="en">Graph Neural Networks (GNNs) are a type of neural network designed to perform inference on data structured as graphs. They are particularly useful for tasks where data is represented as nodes and edges. GNNs work by passing messages between nodes in the graph, updating each node&apos;s state based on its own state, the states of its neighbors, and the features of the edges connecting them. This allows GNNs to capture complex patterns in the graph structure.</dcterms:description>
        <oboInOwl:hasSynonym xml:lang="en">GNN</oboInOwl:hasSynonym>
        <rdfs:label xml:lang="en">Graph Neural Networks</rdfs:label>
    </owl:NamedIndividual>
    


    <!-- http://nlpkg.sebis.cit.tum.de/nlp-fos-hierarchy.owl#Graphs -->

    <owl:NamedIndividual rdf:about="http://nlpkg.sebis.cit.tum.de/nlp-fos-hierarchy.owl#Graphs">
        <rdf:type rdf:resource="http://nlpkg.sebis.cit.tum.de/nlp-fos-hierarchy.owl#DataStructure"/>
        <rdf:type rdf:resource="http://nlpkg.sebis.cit.tum.de/nlp-taxonomy.owl#FieldOfStudy"/>
        <nlp-taxonomy:subFieldOf rdf:resource="http://nlpkg.sebis.cit.tum.de/nlp-fos-hierarchy.owl#Knowledge_Bases"/>
        <nlp-taxonomy:superFieldOf rdf:resource="http://nlpkg.sebis.cit.tum.de/nlp-fos-hierarchy.owl#Abstract_Meaning_Representation"/>
        <nlp-taxonomy:superFieldOf rdf:resource="http://nlpkg.sebis.cit.tum.de/nlp-fos-hierarchy.owl#Dependency_Graphs"/>
        <nlp-taxonomy:superFieldOf rdf:resource="http://nlpkg.sebis.cit.tum.de/nlp-fos-hierarchy.owl#Graph-to-Text"/>
        <nlp-taxonomy:superFieldOf rdf:resource="http://nlpkg.sebis.cit.tum.de/nlp-fos-hierarchy.owl#Graph_Neural_Networks"/>
        <nlp-taxonomy:superFieldOf rdf:resource="http://nlpkg.sebis.cit.tum.de/nlp-fos-hierarchy.owl#Knowledge_Graphs"/>
        <nlp-taxonomy:superFieldOf rdf:resource="http://nlpkg.sebis.cit.tum.de/nlp-fos-hierarchy.owl#Ontologies"/>
        <survey>https://arxiv.org/abs/2312.02783</survey>
        <nlp-taxonomy:level rdf:datatype="http://www.w3.org/2001/XMLSchema#integer">4</nlp-taxonomy:level>
        <dcterms:description xml:lang="en">Graphs are used to represent and analyze linguistic and semantic data. They are mathematical structures that model the relationships between different entities. The nodes of the graph represent these entities, while the edges represent the relationships between them.</dcterms:description>
        <rdfs:label xml:lang="en">Graphs</rdfs:label>
    </owl:NamedIndividual>
    


    <!-- http://nlpkg.sebis.cit.tum.de/nlp-fos-hierarchy.owl#Hallucination_Detection -->

    <owl:NamedIndividual rdf:about="http://nlpkg.sebis.cit.tum.de/nlp-fos-hierarchy.owl#Hallucination_Detection">
        <rdf:type rdf:resource="http://nlpkg.sebis.cit.tum.de/nlp-fos-hierarchy.owl#Task"/>
        <rdf:type rdf:resource="http://nlpkg.sebis.cit.tum.de/nlp-taxonomy.owl#FieldOfStudy"/>
        <uses rdf:resource="http://nlpkg.sebis.cit.tum.de/nlp-taxonomy.owl#Fact_&amp;_Claim_Verification"/>
        <nlp-taxonomy:subFieldOf rdf:resource="http://nlpkg.sebis.cit.tum.de/nlp-fos-hierarchy.owl#Language_Model_Hallucination"/>
        <nlp-taxonomy:subFieldOf rdf:resource="http://nlpkg.sebis.cit.tum.de/nlp-taxonomy.owl#Text_Classification"/>
        <nlp-taxonomy:level rdf:datatype="http://www.w3.org/2001/XMLSchema#integer">3</nlp-taxonomy:level>
        <nlp-taxonomy:level rdf:datatype="http://www.w3.org/2001/XMLSchema#integer">4</nlp-taxonomy:level>
        <dcterms:description xml:lang="en">Hallucination Detection refers to the identification of instances where a language model generates text or information that is fluent and grammatically correct but factually incorrect or unrelated to the input. This phenomenon, known as &quot;hallucination&quot;, can lead to the production of inaccurate or misleading outputs. The goal of hallucination detection is to ensure the reliability and accuracy of the generated text by identifying these hallucinations.</dcterms:description>
        <oboInOwl:hasSynonym xml:lang="en">Hallucination Classification</oboInOwl:hasSynonym>
        <oboInOwl:hasSynonym xml:lang="en">Hallucination Identification</oboInOwl:hasSynonym>
        <rdfs:label xml:lang="en">Hallucination Detection</rdfs:label>
    </owl:NamedIndividual>
    


    <!-- http://nlpkg.sebis.cit.tum.de/nlp-fos-hierarchy.owl#Hallucination_Prevention -->

    <owl:NamedIndividual rdf:about="http://nlpkg.sebis.cit.tum.de/nlp-fos-hierarchy.owl#Hallucination_Prevention">
        <rdf:type rdf:resource="http://nlpkg.sebis.cit.tum.de/nlp-fos-hierarchy.owl#Task"/>
        <rdf:type rdf:resource="http://nlpkg.sebis.cit.tum.de/nlp-taxonomy.owl#FieldOfStudy"/>
        <nlp-taxonomy:subFieldOf rdf:resource="http://nlpkg.sebis.cit.tum.de/nlp-fos-hierarchy.owl#Language_Model_Hallucination"/>
        <survey>https://arxiv.org/abs/2309.16459</survey>
        <survey>https://arxiv.org/abs/2401.01313</survey>
        <nlp-taxonomy:level rdf:datatype="http://www.w3.org/2001/XMLSchema#integer">4</nlp-taxonomy:level>
        <dcterms:description xml:lang="en">Hallucination Prevention refers to the process of preventing or reducing the generation of incorrect or nonsensical outputs by language models. &quot;Hallucination&quot; in this context refers to instances where the model generates text that is fluent and grammatically correct but factually incorrect or unrelated to the input.</dcterms:description>
        <oboInOwl:hasSynonym xml:lang="en">Hallucination Mitigation</oboInOwl:hasSynonym>
        <rdfs:label xml:lang="en">Hallucination Prevention</rdfs:label>
    </owl:NamedIndividual>
    


    <!-- http://nlpkg.sebis.cit.tum.de/nlp-fos-hierarchy.owl#Hard_Prompts -->

    <owl:NamedIndividual rdf:about="http://nlpkg.sebis.cit.tum.de/nlp-fos-hierarchy.owl#Hard_Prompts">
        <rdf:type rdf:resource="http://nlpkg.sebis.cit.tum.de/nlp-fos-hierarchy.owl#OtherScientificField"/>
        <rdf:type rdf:resource="http://nlpkg.sebis.cit.tum.de/nlp-taxonomy.owl#FieldOfStudy"/>
        <nlp-taxonomy:subFieldOf rdf:resource="http://nlpkg.sebis.cit.tum.de/nlp-fos-hierarchy.owl#Prompt_Optimization"/>
        <nlp-taxonomy:level rdf:datatype="http://www.w3.org/2001/XMLSchema#integer">5</nlp-taxonomy:level>
        <dcterms:description xml:lang="en">Hard Prompts or Discrete Prompts are text prompts with discrete inputs and made from interpretable words and tokens, usually hand-crafted by humans.</dcterms:description>
        <oboInOwl:hasSynonym xml:lang="en">Discrete Prompts</oboInOwl:hasSynonym>
        <rdfs:label xml:lang="en">Hard Prompts</rdfs:label>
    </owl:NamedIndividual>
    


    <!-- http://nlpkg.sebis.cit.tum.de/nlp-fos-hierarchy.owl#Hate_Speech_Detection -->

    <owl:NamedIndividual rdf:about="http://nlpkg.sebis.cit.tum.de/nlp-fos-hierarchy.owl#Hate_Speech_Detection">
        <rdf:type rdf:resource="http://nlpkg.sebis.cit.tum.de/nlp-fos-hierarchy.owl#Task"/>
        <rdf:type rdf:resource="http://nlpkg.sebis.cit.tum.de/nlp-taxonomy.owl#FieldOfStudy"/>
        <nlp-taxonomy:subFieldOf rdf:resource="http://nlpkg.sebis.cit.tum.de/nlp-fos-hierarchy.owl#Discrimination_Analysis"/>
        <nlp-taxonomy:subFieldOf rdf:resource="http://nlpkg.sebis.cit.tum.de/nlp-taxonomy.owl#Text_Classification"/>
        <survey>https://aclanthology.org/W17-1101</survey>
        <survey>https://arxiv.org/abs/2102.08886</survey>
        <survey>https://arxiv.org/abs/2106.00742</survey>
        <survey>https://arxiv.org/abs/2203.03584</survey>
        <survey>https://arxiv.org/abs/2209.05294</survey>
        <nlp-taxonomy:level rdf:datatype="http://www.w3.org/2001/XMLSchema#integer">3</nlp-taxonomy:level>
        <nlp-taxonomy:level rdf:datatype="http://www.w3.org/2001/XMLSchema#integer">4</nlp-taxonomy:level>
        <dcterms:description xml:lang="en">Hate Speech Detection refers to the application of machine learning and AI techniques to identify and filter out harmful content that promotes violence or discrimination against individuals or groups based on attributes such as race, religion, sexual orientation, or other characteristics.</dcterms:description>
        <rdfs:label xml:lang="en">Hate Speech Detection</rdfs:label>
    </owl:NamedIndividual>
    


    <!-- http://nlpkg.sebis.cit.tum.de/nlp-fos-hierarchy.owl#Head-driven_Phrase_Structure_Grammar -->

    <owl:NamedIndividual rdf:about="http://nlpkg.sebis.cit.tum.de/nlp-fos-hierarchy.owl#Head-driven_Phrase_Structure_Grammar">
        <rdf:type rdf:resource="http://nlpkg.sebis.cit.tum.de/nlp-fos-hierarchy.owl#OtherScientificField"/>
        <rdf:type rdf:resource="http://nlpkg.sebis.cit.tum.de/nlp-taxonomy.owl#FieldOfStudy"/>
        <nlp-taxonomy:subFieldOf rdf:resource="http://nlpkg.sebis.cit.tum.de/nlp-taxonomy.owl#Linguistic_Theories"/>
        <nlp-taxonomy:level rdf:datatype="http://www.w3.org/2001/XMLSchema#integer">3</nlp-taxonomy:level>
        <dcterms:description xml:lang="en">Head-driven Phrase Structure Grammar (HPSG) is a framework in computational linguistics that uses type feature structures to represent syntactic, semantic, and morphological information about linguistic expressions. It is called &quot;head-driven&quot; because the head word of a phrase determines many of its syntactic properties. HPSG provides a formalism for creating detailed, machine-readable descriptions of natural language syntax.</dcterms:description>
        <oboInOwl:hasSynonym xml:lang="en">HPSG</oboInOwl:hasSynonym>
        <rdfs:label xml:lang="en">Head-driven Phrase Structure Grammar</rdfs:label>
    </owl:NamedIndividual>
    


    <!-- http://nlpkg.sebis.cit.tum.de/nlp-fos-hierarchy.owl#Hierarchical_Clustering -->

    <owl:NamedIndividual rdf:about="http://nlpkg.sebis.cit.tum.de/nlp-fos-hierarchy.owl#Hierarchical_Clustering">
        <rdf:type rdf:resource="http://nlpkg.sebis.cit.tum.de/nlp-fos-hierarchy.owl#Task"/>
        <rdf:type rdf:resource="http://nlpkg.sebis.cit.tum.de/nlp-taxonomy.owl#FieldOfStudy"/>
        <nlp-taxonomy:subFieldOf rdf:resource="http://nlpkg.sebis.cit.tum.de/nlp-taxonomy.owl#Text_Clustering"/>
        <nlp-taxonomy:level rdf:datatype="http://www.w3.org/2001/XMLSchema#integer">3</nlp-taxonomy:level>
        <nlp-taxonomy:level rdf:datatype="http://www.w3.org/2001/XMLSchema#integer">5</nlp-taxonomy:level>
        <dcterms:description xml:lang="en">Hierarchical Clustering is a method which seeks to build a hierarchy of clusters.</dcterms:description>
        <rdfs:label xml:lang="en">Hierarchical Clustering</rdfs:label>
    </owl:NamedIndividual>
    


    <!-- http://nlpkg.sebis.cit.tum.de/nlp-fos-hierarchy.owl#Hierarchical_Phrase-based_Machine_Translation -->

    <owl:NamedIndividual rdf:about="http://nlpkg.sebis.cit.tum.de/nlp-fos-hierarchy.owl#Hierarchical_Phrase-based_Machine_Translation">
        <rdf:type rdf:resource="http://nlpkg.sebis.cit.tum.de/nlp-fos-hierarchy.owl#Task"/>
        <rdf:type rdf:resource="http://nlpkg.sebis.cit.tum.de/nlp-taxonomy.owl#FieldOfStudy"/>
        <nlp-taxonomy:subFieldOf rdf:resource="http://nlpkg.sebis.cit.tum.de/nlp-fos-hierarchy.owl#Phrase-based_Machine_Translation"/>
        <nlp-taxonomy:subFieldOf rdf:resource="http://nlpkg.sebis.cit.tum.de/nlp-fos-hierarchy.owl#Syntax-based_Machine_Translation"/>
        <origin>https://aclanthology.org/P05-1033</origin>
        <nlp-taxonomy:level rdf:datatype="http://www.w3.org/2001/XMLSchema#integer">5</nlp-taxonomy:level>
        <dcterms:description xml:lang="en">Hierarchical Phrase-based Machine Translation (HPBMT) combines the phrase-based and syntax-based approaches to translation. This approach that translates sentences by dividing them into a hierarchy of phrases, rather than translating word by word. This approach allows for more accurate translations by considering the context and grammatical structure of the sentence, rather than just the individual words. It uses a statistical model to determine the most likely translation of a given phrase within its specific context.</dcterms:description>
        <oboInOwl:hasSynonym xml:lang="en">HPBMT</oboInOwl:hasSynonym>
        <rdfs:label xml:lang="en">Hierarchical Phrase-based Machine Translation</rdfs:label>
    </owl:NamedIndividual>
    


    <!-- http://nlpkg.sebis.cit.tum.de/nlp-fos-hierarchy.owl#Hybrid_Machine_Translation -->

    <owl:NamedIndividual rdf:about="http://nlpkg.sebis.cit.tum.de/nlp-fos-hierarchy.owl#Hybrid_Machine_Translation">
        <rdf:type rdf:resource="http://nlpkg.sebis.cit.tum.de/nlp-fos-hierarchy.owl#Task"/>
        <rdf:type rdf:resource="http://nlpkg.sebis.cit.tum.de/nlp-taxonomy.owl#FieldOfStudy"/>
        <nlp-taxonomy:subFieldOf rdf:resource="http://nlpkg.sebis.cit.tum.de/nlp-taxonomy.owl#Machine_Translation"/>
        <nlp-taxonomy:level rdf:datatype="http://www.w3.org/2001/XMLSchema#integer">3</nlp-taxonomy:level>
        <dcterms:description xml:lang="en">Hybrid Machine Translation (HMT) is a method of machine translation that is characterized by the use of multiple machine translation approaches within a single machine translation system. The motivation for developing hybrid machine translation systems stems from the failure of any single technique to achieve a satisfactory level of accuracy.</dcterms:description>
        <oboInOwl:hasSynonym xml:lang="en">HMT</oboInOwl:hasSynonym>
        <rdfs:label xml:lang="en">Hybrid Machine Translation</rdfs:label>
    </owl:NamedIndividual>
    


    <!-- http://nlpkg.sebis.cit.tum.de/nlp-fos-hierarchy.owl#Idiom_Identification -->

    <owl:NamedIndividual rdf:about="http://nlpkg.sebis.cit.tum.de/nlp-fos-hierarchy.owl#Idiom_Identification">
        <rdf:type rdf:resource="http://nlpkg.sebis.cit.tum.de/nlp-fos-hierarchy.owl#Task"/>
        <rdf:type rdf:resource="http://nlpkg.sebis.cit.tum.de/nlp-taxonomy.owl#FieldOfStudy"/>
        <nlp-taxonomy:subFieldOf rdf:resource="http://nlpkg.sebis.cit.tum.de/nlp-fos-hierarchy.owl#Figurative_Language"/>
        <nlp-taxonomy:subFieldOf rdf:resource="http://nlpkg.sebis.cit.tum.de/nlp-taxonomy.owl#Text_Classification"/>
        <survey>https://aclanthology.org/2021.tacl-1.92</survey>
        <nlp-taxonomy:level rdf:datatype="http://www.w3.org/2001/XMLSchema#integer">3</nlp-taxonomy:level>
        <nlp-taxonomy:level rdf:datatype="http://www.w3.org/2001/XMLSchema#integer">4</nlp-taxonomy:level>
        <dcterms:description xml:lang="en">Idiom Detection</dcterms:description>
        <dcterms:description xml:lang="en">Idiom Identification refers to the process of detecting and understanding idiomatic expressions within a text. Idioms are phrases that have a figurative meaning different from the literal interpretation of the individual words. This task is challenging in NLP due to the complexity and variability of idiomatic expressions in different languages.</dcterms:description>
        <oboInOwl:hasSynonym xml:lang="en">Idiom Classification</oboInOwl:hasSynonym>
        <oboInOwl:hasSynonym xml:lang="en">Idiom Expression Classification</oboInOwl:hasSynonym>
        <oboInOwl:hasSynonym xml:lang="en">Idiomatic Expression Detection</oboInOwl:hasSynonym>
        <oboInOwl:hasSynonym xml:lang="en">Idiomatic Expression Identification</oboInOwl:hasSynonym>
        <rdfs:label xml:lang="en">Idiom Identification</rdfs:label>
    </owl:NamedIndividual>
    


    <!-- http://nlpkg.sebis.cit.tum.de/nlp-fos-hierarchy.owl#Image-to-Text_Retrieval -->

    <owl:NamedIndividual rdf:about="http://nlpkg.sebis.cit.tum.de/nlp-fos-hierarchy.owl#Image-to-Text_Retrieval">
        <rdf:type rdf:resource="http://nlpkg.sebis.cit.tum.de/nlp-fos-hierarchy.owl#Task"/>
        <rdf:type rdf:resource="http://nlpkg.sebis.cit.tum.de/nlp-taxonomy.owl#FieldOfStudy"/>
        <nlp-taxonomy:subFieldOf rdf:resource="http://nlpkg.sebis.cit.tum.de/nlp-taxonomy.owl#Information_Retrieval"/>
        <nlp-taxonomy:subFieldOf rdf:resource="http://nlpkg.sebis.cit.tum.de/nlp-taxonomy.owl#Visual_Data_In_NLP"/>
        <survey>https://arxiv.org/abs/2203.14713</survey>
        <nlp-taxonomy:level rdf:datatype="http://www.w3.org/2001/XMLSchema#integer">2</nlp-taxonomy:level>
        <nlp-taxonomy:level rdf:datatype="http://www.w3.org/2001/XMLSchema#integer">3</nlp-taxonomy:level>
        <dcterms:description xml:lang="en">Image-to-Text Retrieval refers to the process of finding and retrieving relevant texts based on a given imagery. It involves using techniques to understand semantic content of images and then searching for texts that best match or represent the content of the image.</dcterms:description>
        <oboInOwl:hasSynonym xml:lang="en">I2T Retrieval</oboInOwl:hasSynonym>
        <oboInOwl:hasSynonym xml:lang="en">ITR</oboInOwl:hasSynonym>
        <oboInOwl:hasSynonym xml:lang="en">Image-Text Retrieval</oboInOwl:hasSynonym>
        <rdfs:label xml:lang="en">Image-to-Text Retrieval</rdfs:label>
    </owl:NamedIndividual>
    


    <!-- http://nlpkg.sebis.cit.tum.de/nlp-fos-hierarchy.owl#Image_Captioning -->

    <owl:NamedIndividual rdf:about="http://nlpkg.sebis.cit.tum.de/nlp-fos-hierarchy.owl#Image_Captioning">
        <rdf:type rdf:resource="http://nlpkg.sebis.cit.tum.de/nlp-fos-hierarchy.owl#Task"/>
        <rdf:type rdf:resource="http://nlpkg.sebis.cit.tum.de/nlp-taxonomy.owl#FieldOfStudy"/>
        <nlp-taxonomy:subFieldOf rdf:resource="http://nlpkg.sebis.cit.tum.de/nlp-taxonomy.owl#Captioning"/>
        <nlp-taxonomy:subFieldOf rdf:resource="http://nlpkg.sebis.cit.tum.de/nlp-taxonomy.owl#Visual_Data_In_NLP"/>
        <nlp-taxonomy:superFieldOf rdf:resource="http://nlpkg.sebis.cit.tum.de/nlp-fos-hierarchy.owl#Sign_Language_Recognition"/>
        <survey>https://arxiv.org/abs/1601.03896</survey>
        <survey>https://arxiv.org/abs/1905.08110</survey>
        <survey>https://arxiv.org/abs/2107.06912</survey>
        <survey>https://arxiv.org/abs/2107.13114</survey>
        <nlp-taxonomy:level rdf:datatype="http://www.w3.org/2001/XMLSchema#integer">3</nlp-taxonomy:level>
        <dcterms:description xml:lang="en">Image captioning involves generating descriptive textual descriptions or captions for images. The goal of image captioning is to create a meaningful and coherent sentence or phrase that describes the content and context of an image, allowing humans to understand the image&apos;s content without actually viewing it.</dcterms:description>
        <oboInOwl:hasSynonym xml:lang="en">I2T</oboInOwl:hasSynonym>
        <oboInOwl:hasSynonym xml:lang="en">Image-to-Text</oboInOwl:hasSynonym>
        <rdfs:label xml:lang="en">Image Captioning</rdfs:label>
    </owl:NamedIndividual>
    


    <!-- http://nlpkg.sebis.cit.tum.de/nlp-fos-hierarchy.owl#Image_Question_Answering -->

    <owl:NamedIndividual rdf:about="http://nlpkg.sebis.cit.tum.de/nlp-fos-hierarchy.owl#Image_Question_Answering">
        <rdf:type rdf:resource="http://nlpkg.sebis.cit.tum.de/nlp-fos-hierarchy.owl#Task"/>
        <rdf:type rdf:resource="http://nlpkg.sebis.cit.tum.de/nlp-taxonomy.owl#FieldOfStudy"/>
        <nlp-taxonomy:subFieldOf rdf:resource="http://nlpkg.sebis.cit.tum.de/nlp-fos-hierarchy.owl#Visual_Question_Answering"/>
        <nlp-taxonomy:level rdf:datatype="http://www.w3.org/2001/XMLSchema#integer">4</nlp-taxonomy:level>
        <dcterms:description xml:lang="en">Image Question Answering (ImageQA) involves answering questions about the content of an image using natural language responses. This task requires a system to understand both the visual information contained within an image and the textual information in a question, and then generate a relevant textual answer.</dcterms:description>
        <oboInOwl:hasSynonym xml:lang="en">ImageQA</oboInOwl:hasSynonym>
        <rdfs:label xml:lang="en">Image Question Answering</rdfs:label>
    </owl:NamedIndividual>
    


    <!-- http://nlpkg.sebis.cit.tum.de/nlp-fos-hierarchy.owl#Implicit_Discourse_Relation_Recognition -->

    <owl:NamedIndividual rdf:about="http://nlpkg.sebis.cit.tum.de/nlp-fos-hierarchy.owl#Implicit_Discourse_Relation_Recognition">
        <rdf:type rdf:resource="http://nlpkg.sebis.cit.tum.de/nlp-fos-hierarchy.owl#Task"/>
        <rdf:type rdf:resource="http://nlpkg.sebis.cit.tum.de/nlp-taxonomy.owl#FieldOfStudy"/>
        <nlp-taxonomy:subFieldOf rdf:resource="http://nlpkg.sebis.cit.tum.de/nlp-fos-hierarchy.owl#Discourse_Relation_Recognition"/>
        <survey>https://arxiv.org/abs/2203.02982</survey>
        <nlp-taxonomy:level rdf:datatype="http://www.w3.org/2001/XMLSchema#integer">4</nlp-taxonomy:level>
        <nlp-taxonomy:level rdf:datatype="http://www.w3.org/2001/XMLSchema#integer">5</nlp-taxonomy:level>
        <nlp-taxonomy:level rdf:datatype="http://www.w3.org/2001/XMLSchema#integer">9</nlp-taxonomy:level>
        <dcterms:description xml:lang="en">Implicit Discourse Relation Recognition (IDRR) refers to the task of identifying and classifying the hidden/latent or unstated relationships between different parts of a text. These relations are not explicitly stated through conjunctions or other markers but are inferred from the context and content of the sentences.</dcterms:description>
        <oboInOwl:hasSynonym xml:lang="en">IDRR</oboInOwl:hasSynonym>
        <oboInOwl:hasSynonym xml:lang="en">Implicit Discourse Relation Extraction</oboInOwl:hasSynonym>
        <rdfs:label xml:lang="en">Implicit Discourse Relation Recognition</rdfs:label>
    </owl:NamedIndividual>
    


    <!-- http://nlpkg.sebis.cit.tum.de/nlp-fos-hierarchy.owl#Implicit_Semantic_Role_Labeling -->

    <owl:NamedIndividual rdf:about="http://nlpkg.sebis.cit.tum.de/nlp-fos-hierarchy.owl#Implicit_Semantic_Role_Labeling">
        <rdf:type rdf:resource="http://nlpkg.sebis.cit.tum.de/nlp-fos-hierarchy.owl#Task"/>
        <rdf:type rdf:resource="http://nlpkg.sebis.cit.tum.de/nlp-taxonomy.owl#FieldOfStudy"/>
        <nlp-taxonomy:subFieldOf rdf:resource="http://nlpkg.sebis.cit.tum.de/nlp-fos-hierarchy.owl#Slot_Filling"/>
        <survey>https://arxiv.org/abs/2107.08523</survey>
        <nlp-taxonomy:level rdf:datatype="http://www.w3.org/2001/XMLSchema#integer">4</nlp-taxonomy:level>
        <dcterms:description xml:lang="en">Implicit Semantic Role Labeling (ISRL) is the task of identifying and classifying the semantic roles of arguments in a sentence, even when they are not explicitly mentioned. It involves understanding the context and inferring the roles based on the given information.</dcterms:description>
        <oboInOwl:hasSynonym xml:lang="en">Argument Linking</oboInOwl:hasSynonym>
        <oboInOwl:hasSynonym xml:lang="en">ISRL</oboInOwl:hasSynonym>
        <rdfs:label xml:lang="en">Implicit Semantic Role Labeling</rdfs:label>
    </owl:NamedIndividual>
    


    <!-- http://nlpkg.sebis.cit.tum.de/nlp-fos-hierarchy.owl#In-Context_Learning -->

    <owl:NamedIndividual rdf:about="http://nlpkg.sebis.cit.tum.de/nlp-fos-hierarchy.owl#In-Context_Learning">
        <rdf:type rdf:resource="http://nlpkg.sebis.cit.tum.de/nlp-fos-hierarchy.owl#Task"/>
        <rdf:type rdf:resource="http://nlpkg.sebis.cit.tum.de/nlp-taxonomy.owl#FieldOfStudy"/>
        <nlp-taxonomy:subFieldOf rdf:resource="http://nlpkg.sebis.cit.tum.de/nlp-fos-hierarchy.owl#Few-shot_Learning"/>
        <nlp-taxonomy:subFieldOf rdf:resource="http://nlpkg.sebis.cit.tum.de/nlp-fos-hierarchy.owl#Prompting,_Prompt_Learning_&amp;_Prompt_Engineering"/>
        <survey>https://aclanthology.org/2023.findings-acl.779</survey>
        <survey>https://aclanthology.org/2023.ranlp-1.69</survey>
        <survey>https://arxiv.org/abs/2301.00234</survey>
        <survey>https://arxiv.org/abs/2309.01809</survey>
        <nlp-taxonomy:level rdf:datatype="http://www.w3.org/2001/XMLSchema#integer">4</nlp-taxonomy:level>
        <dcterms:description xml:lang="en">In-Context Learning (ICL) refers to the process where the model learns from the context provided in the prompt itself. It doesn&apos;t require explicit fine-tuning or training on a specific task. Instead, it uses the information given in the prompt to generate appropriate responses.</dcterms:description>
        <oboInOwl:hasSynonym xml:lang="en">Few-shot Prompting</oboInOwl:hasSynonym>
        <oboInOwl:hasSynonym xml:lang="en">ICL</oboInOwl:hasSynonym>
        <rdfs:label xml:lang="en">In-Context Learning</rdfs:label>
    </owl:NamedIndividual>
    


    <!-- http://nlpkg.sebis.cit.tum.de/nlp-fos-hierarchy.owl#Inductive_Bias -->

    <owl:NamedIndividual rdf:about="http://nlpkg.sebis.cit.tum.de/nlp-fos-hierarchy.owl#Inductive_Bias">
        <rdf:type rdf:resource="http://nlpkg.sebis.cit.tum.de/nlp-fos-hierarchy.owl#OtherScientificField"/>
        <rdf:type rdf:resource="http://nlpkg.sebis.cit.tum.de/nlp-taxonomy.owl#FieldOfStudy"/>
        <nlp-taxonomy:subFieldOf rdf:resource="http://nlpkg.sebis.cit.tum.de/nlp-fos-hierarchy.owl#Biases_&amp;_Fairness_in_NLP"/>
        <survey>https://aclanthology.org/2021.acl-long.38</survey>
        <nlp-taxonomy:level rdf:datatype="http://www.w3.org/2001/XMLSchema#integer">4</nlp-taxonomy:level>
        <dcterms:description xml:lang="en">Inductive Bias refers to the set of assumptions that a machine learning algorithm uses to predict outputs given inputs that it has not encountered before. It is the bias or set of preconceptions that a system has before learning begins, which guides the system towards a particular solution when faced with ambiguous or new situations.</dcterms:description>
        <oboInOwl:hasSynonym xml:lang="en">Learning Bias</oboInOwl:hasSynonym>
        <rdfs:label xml:lang="en">Inductive Bias</rdfs:label>
    </owl:NamedIndividual>
    


    <!-- http://nlpkg.sebis.cit.tum.de/nlp-fos-hierarchy.owl#Inference_Attacks -->

    <owl:NamedIndividual rdf:about="http://nlpkg.sebis.cit.tum.de/nlp-fos-hierarchy.owl#Inference_Attacks">
        <rdf:type rdf:resource="http://nlpkg.sebis.cit.tum.de/nlp-fos-hierarchy.owl#Task"/>
        <rdf:type rdf:resource="http://nlpkg.sebis.cit.tum.de/nlp-taxonomy.owl#FieldOfStudy"/>
        <nlp-taxonomy:subFieldOf rdf:resource="http://nlpkg.sebis.cit.tum.de/nlp-fos-hierarchy.owl#Privacy,_Security_&amp;_Safety_in_NLP"/>
        <nlp-taxonomy:superFieldOf rdf:resource="http://nlpkg.sebis.cit.tum.de/nlp-fos-hierarchy.owl#Attribute_Inference_Attack"/>
        <nlp-taxonomy:superFieldOf rdf:resource="http://nlpkg.sebis.cit.tum.de/nlp-fos-hierarchy.owl#Membership_Inference_Attack"/>
        <nlp-taxonomy:superFieldOf rdf:resource="http://nlpkg.sebis.cit.tum.de/nlp-fos-hierarchy.owl#Model_Inversion_Attack"/>
        <nlp-taxonomy:superFieldOf rdf:resource="http://nlpkg.sebis.cit.tum.de/nlp-fos-hierarchy.owl#Model_Stealing_Attack"/>
        <nlp-taxonomy:level rdf:datatype="http://www.w3.org/2001/XMLSchema#integer">4</nlp-taxonomy:level>
        <dcterms:description xml:lang="en">Inference Attacks refer to the methods used to uncover sensitive information from seemingly non-sensitive data. These attacks use machine learning algorithms to infer or predict confidential data based on the patterns and correlations in the available data. For instance, even if a dataset is anonymized, an inference attack might still be able to predict sensitive attributes like gender, age, or health status based on the patterns in the text.</dcterms:description>
        <rdfs:label xml:lang="en">Inference Attacks</rdfs:label>
    </owl:NamedIndividual>
    


    <!-- http://nlpkg.sebis.cit.tum.de/nlp-fos-hierarchy.owl#Instruction_Learning -->

    <owl:NamedIndividual rdf:about="http://nlpkg.sebis.cit.tum.de/nlp-fos-hierarchy.owl#Instruction_Learning">
        <rdf:type rdf:resource="http://nlpkg.sebis.cit.tum.de/nlp-fos-hierarchy.owl#Task"/>
        <rdf:type rdf:resource="http://nlpkg.sebis.cit.tum.de/nlp-taxonomy.owl#FieldOfStudy"/>
        <usedFor rdf:resource="http://nlpkg.sebis.cit.tum.de/nlp-fos-hierarchy.owl#Chatbots"/>
        <usedFor rdf:resource="http://nlpkg.sebis.cit.tum.de/nlp-fos-hierarchy.owl#Language_Model_Alignment"/>
        <usedFor rdf:resource="http://nlpkg.sebis.cit.tum.de/nlp-fos-hierarchy.owl#Multi-task_Learning"/>
        <uses rdf:resource="http://nlpkg.sebis.cit.tum.de/nlp-fos-hierarchy.owl#Controllable_Text_Generation"/>
        <nlp-taxonomy:subFieldOf rdf:resource="http://nlpkg.sebis.cit.tum.de/nlp-fos-hierarchy.owl#Prompting,_Prompt_Learning_&amp;_Prompt_Engineering"/>
        <nlp-taxonomy:superFieldOf rdf:resource="http://nlpkg.sebis.cit.tum.de/nlp-fos-hierarchy.owl#Instruction_Tuning"/>
        <relevantInformation>https://github.com/RenzeLou/awesome-instruction-learning</relevantInformation>
        <survey>https://arxiv.org/abs/2303.10475</survey>
        <nlp-taxonomy:level rdf:datatype="http://www.w3.org/2001/XMLSchema#integer">4</nlp-taxonomy:level>
        <dcterms:description xml:lang="en">Instruction Learning refers to the ability of a machine learning model to understand and follow natural language instructions given in the prompt. It involves training the model to understand and follow the instructions accurately to generate the desired output. This concept is crucial in developing intelligent systems that can interact with humans in a more intuitive and natural manner.</dcterms:description>
        <rdfs:label xml:lang="en">Instruction Learning</rdfs:label>
    </owl:NamedIndividual>
    


    <!-- http://nlpkg.sebis.cit.tum.de/nlp-fos-hierarchy.owl#Instruction_Tuning -->

    <owl:NamedIndividual rdf:about="http://nlpkg.sebis.cit.tum.de/nlp-fos-hierarchy.owl#Instruction_Tuning">
        <rdf:type rdf:resource="http://nlpkg.sebis.cit.tum.de/nlp-fos-hierarchy.owl#Task"/>
        <rdf:type rdf:resource="http://nlpkg.sebis.cit.tum.de/nlp-taxonomy.owl#FieldOfStudy"/>
        <nlp-taxonomy:subFieldOf rdf:resource="http://nlpkg.sebis.cit.tum.de/nlp-fos-hierarchy.owl#Instruction_Learning"/>
        <origin>https://arxiv.org/abs/2109.01652</origin>
        <relevantInformation>https://github.com/SinclairCoder/Instruction-Tuning-Papers</relevantInformation>
        <relevantInformation>https://yaofu.notion.site/June-2023-A-Stage-Review-of-Instruction-Tuning-f59dbfc36e2d4e12a33443bd6b2012c2</relevantInformation>
        <survey>https://arxiv.org/abs/2308.10792</survey>
        <survey>https://arxiv.org/abs/2310.14103</survey>
        <nlp-taxonomy:level rdf:datatype="http://www.w3.org/2001/XMLSchema#integer">5</nlp-taxonomy:level>
        <dcterms:description xml:lang="en">Instruction Tuning refers to the process of fine-tuning a pre-trained language model on a dataset of instructions. The goal is to make the model follow specific instructions in the input prompt. It&apos;s a way to control the behavior of the model without modifying the model architecture or retraining from scratch.</dcterms:description>
        <oboInOwl:hasSynonym xml:lang="en">IFT</oboInOwl:hasSynonym>
        <oboInOwl:hasSynonym xml:lang="en">Instruction Fine-Tuning</oboInOwl:hasSynonym>
        <rdfs:label xml:lang="en">Instruction Tuning</rdfs:label>
    </owl:NamedIndividual>
    


    <!-- http://nlpkg.sebis.cit.tum.de/nlp-fos-hierarchy.owl#Irony_Detection -->

    <owl:NamedIndividual rdf:about="http://nlpkg.sebis.cit.tum.de/nlp-fos-hierarchy.owl#Irony_Detection">
        <rdf:type rdf:resource="http://nlpkg.sebis.cit.tum.de/nlp-fos-hierarchy.owl#Task"/>
        <rdf:type rdf:resource="http://nlpkg.sebis.cit.tum.de/nlp-taxonomy.owl#FieldOfStudy"/>
        <nlp-taxonomy:subFieldOf rdf:resource="http://nlpkg.sebis.cit.tum.de/nlp-taxonomy.owl#Stylistic_Analysis"/>
        <nlp-taxonomy:subFieldOf rdf:resource="http://nlpkg.sebis.cit.tum.de/nlp-taxonomy.owl#Text_Classification"/>
        <survey>https://aclanthology.org/2022.coling-1.69</survey>
        <nlp-taxonomy:level rdf:datatype="http://www.w3.org/2001/XMLSchema#integer">3</nlp-taxonomy:level>
        <dcterms:description xml:lang="en">Irony Detection refers to the computational task of identifying ironic statements in text. This is a challenging task as it often requires understanding the context, the speaker&apos;s intent, and cultural nuances. It&apos;s a significant aspect of sentiment analysis, as misinterpreting irony can lead to an incorrect understanding of the sentiment expressed in the text.</dcterms:description>
        <oboInOwl:hasSynonym xml:lang="en">Irony Classification</oboInOwl:hasSynonym>
        <oboInOwl:hasSynonym xml:lang="en">Irony Identification</oboInOwl:hasSynonym>
        <oboInOwl:hasSynonym xml:lang="en">Irony Processing</oboInOwl:hasSynonym>
        <rdfs:label xml:lang="en">Irony Detection</rdfs:label>
    </owl:NamedIndividual>
    


    <!-- http://nlpkg.sebis.cit.tum.de/nlp-fos-hierarchy.owl#Justification_Production -->

    <owl:NamedIndividual rdf:about="http://nlpkg.sebis.cit.tum.de/nlp-fos-hierarchy.owl#Justification_Production">
        <rdf:type rdf:resource="http://nlpkg.sebis.cit.tum.de/nlp-fos-hierarchy.owl#Task"/>
        <rdf:type rdf:resource="http://nlpkg.sebis.cit.tum.de/nlp-taxonomy.owl#FieldOfStudy"/>
        <uses rdf:resource="http://nlpkg.sebis.cit.tum.de/nlp-taxonomy.owl#Summarization"/>
        <uses rdf:resource="http://nlpkg.sebis.cit.tum.de/nlp-taxonomy.owl#Explainability_&amp;_Interpretability_In_NLP"/>
        <nlp-taxonomy:subFieldOf rdf:resource="http://nlpkg.sebis.cit.tum.de/nlp-fos-hierarchy.owl#Claim_Verification"/>
        <nlp-taxonomy:level rdf:datatype="http://www.w3.org/2001/XMLSchema#integer">5</nlp-taxonomy:level>
        <dcterms:description xml:lang="en">Justification Production refers to the process of generating explanations or justifications for a particular machine-generated verdict on a claim.</dcterms:description>
        <rdfs:label xml:lang="en">Justification Production</rdfs:label>
    </owl:NamedIndividual>
    


    <!-- http://nlpkg.sebis.cit.tum.de/nlp-fos-hierarchy.owl#Knowledge_Augmented_Language_Models -->

    <owl:NamedIndividual rdf:about="http://nlpkg.sebis.cit.tum.de/nlp-fos-hierarchy.owl#Knowledge_Augmented_Language_Models">
        <rdf:type rdf:resource="http://nlpkg.sebis.cit.tum.de/nlp-fos-hierarchy.owl#OtherScientificField"/>
        <rdf:type rdf:resource="http://nlpkg.sebis.cit.tum.de/nlp-taxonomy.owl#FieldOfStudy"/>
        <uses rdf:resource="http://nlpkg.sebis.cit.tum.de/nlp-fos-hierarchy.owl#Knowledge_Bases"/>
        <nlp-taxonomy:subFieldOf rdf:resource="http://nlpkg.sebis.cit.tum.de/nlp-fos-hierarchy.owl#Transformers_&amp;_Large_Language_Models"/>
        <nlp-taxonomy:superFieldOf rdf:resource="http://nlpkg.sebis.cit.tum.de/nlp-fos-hierarchy.owl#Knowledge_Editing"/>
        <survey>https://arxiv.org/abs/2010.04389</survey>
        <survey>https://arxiv.org/abs/2101.12294</survey>
        <survey>https://arxiv.org/abs/2110.00269</survey>
        <survey>https://arxiv.org/abs/2110.08455</survey>
        <survey>https://arxiv.org/abs/2211.05994</survey>
        <survey>https://arxiv.org/abs/2212.13428</survey>
        <survey>https://arxiv.org/abs/2302.07842</survey>
        <survey>https://arxiv.org/abs/2306.08302</survey>
        <nlp-taxonomy:level rdf:datatype="http://www.w3.org/2001/XMLSchema#integer">4</nlp-taxonomy:level>
        <dcterms:description xml:lang="en">Knowledge Augmented Language Models refer to language models that are enhanced with external knowledge sources. These models are designed to improve the understanding and generation of text by incorporating information from databases, knowledge graphs, or other structured forms of knowledge. This augmentation helps the model to provide more accurate, detailed, and contextually relevant responses, overcoming the limitations of models trained solely on text data.</dcterms:description>
        <oboInOwl:hasSynonym xml:lang="en">KE-PLMs</oboInOwl:hasSynonym>
        <oboInOwl:hasSynonym xml:lang="en">Knowledge Enhanced Language Models</oboInOwl:hasSynonym>
        <oboInOwl:hasSynonym xml:lang="en">Knowledge Enhanced Pretrained Language Models</oboInOwl:hasSynonym>
        <rdfs:label xml:lang="en">Knowledge Augmented Language Models</rdfs:label>
    </owl:NamedIndividual>
    


    <!-- http://nlpkg.sebis.cit.tum.de/nlp-fos-hierarchy.owl#Knowledge_Base_Question_Answering -->

    <owl:NamedIndividual rdf:about="http://nlpkg.sebis.cit.tum.de/nlp-fos-hierarchy.owl#Knowledge_Base_Question_Answering">
        <rdf:type rdf:resource="http://nlpkg.sebis.cit.tum.de/nlp-fos-hierarchy.owl#Task"/>
        <rdf:type rdf:resource="http://nlpkg.sebis.cit.tum.de/nlp-taxonomy.owl#FieldOfStudy"/>
        <uses rdf:resource="http://nlpkg.sebis.cit.tum.de/nlp-fos-hierarchy.owl#Retrieval_Augmented_Generation"/>
        <nlp-taxonomy:subFieldOf rdf:resource="http://nlpkg.sebis.cit.tum.de/nlp-fos-hierarchy.owl#Knowledge_Bases"/>
        <nlp-taxonomy:subFieldOf rdf:resource="http://nlpkg.sebis.cit.tum.de/nlp-taxonomy.owl#Question_Answering"/>
        <nlp-taxonomy:superFieldOf rdf:resource="http://nlpkg.sebis.cit.tum.de/nlp-fos-hierarchy.owl#Knowledge_Graph_Question_Answering"/>
        <nlp-taxonomy:superFieldOf rdf:resource="http://nlpkg.sebis.cit.tum.de/nlp-fos-hierarchy.owl#Table_Question_Answering"/>
        <survey>https://arxiv.org/abs/2007.13069</survey>
        <survey>https://arxiv.org/abs/2105.11644</survey>
        <survey>https://arxiv.org/abs/2108.06688</survey>
        <survey>https://arxiv.org/abs/2211.08170</survey>
        <nlp-taxonomy:level rdf:datatype="http://www.w3.org/2001/XMLSchema#integer">3</nlp-taxonomy:level>
        <nlp-taxonomy:level rdf:datatype="http://www.w3.org/2001/XMLSchema#integer">4</nlp-taxonomy:level>
        <dcterms:description xml:lang="en">Knowledge Base Question Answering (KBQA) is a task that involves extracting information from structured knowledge bases or databases in response to natural language questions. It combines techniques from NLP and database querying to enable systems to understand and answer questions posed in human language by retrieving relevant information from a predefined knowledge base. KBQA systems aim to bridge the gap between unstructured text data and structured knowledge sources, making it easier for users to access specific information through natural language queries.</dcterms:description>
        <oboInOwl:hasSynonym xml:lang="en">KB Question Answering</oboInOwl:hasSynonym>
        <oboInOwl:hasSynonym xml:lang="en">KBQA</oboInOwl:hasSynonym>
        <rdfs:label xml:lang="en">Knowledge Base Question Answering</rdfs:label>
    </owl:NamedIndividual>
    


    <!-- http://nlpkg.sebis.cit.tum.de/nlp-fos-hierarchy.owl#Knowledge_Bases -->

    <owl:NamedIndividual rdf:about="http://nlpkg.sebis.cit.tum.de/nlp-fos-hierarchy.owl#Knowledge_Bases">
        <rdf:type rdf:resource="http://nlpkg.sebis.cit.tum.de/nlp-fos-hierarchy.owl#DataStructure"/>
        <rdf:type rdf:resource="http://nlpkg.sebis.cit.tum.de/nlp-taxonomy.owl#FieldOfStudy"/>
        <usedFor rdf:resource="http://nlpkg.sebis.cit.tum.de/nlp-fos-hierarchy.owl#Knowledge_Augmented_Language_Models"/>
        <nlp-taxonomy:subFieldOf rdf:resource="http://nlpkg.sebis.cit.tum.de/nlp-taxonomy.owl#Knowledge_Representation"/>
        <nlp-taxonomy:subFieldOf rdf:resource="http://nlpkg.sebis.cit.tum.de/nlp-taxonomy.owl#Structured_Data_In_NLP"/>
        <nlp-taxonomy:superFieldOf rdf:resource="http://nlpkg.sebis.cit.tum.de/nlp-fos-hierarchy.owl#Dictionary"/>
        <nlp-taxonomy:superFieldOf rdf:resource="http://nlpkg.sebis.cit.tum.de/nlp-fos-hierarchy.owl#Gazetteers"/>
        <nlp-taxonomy:superFieldOf rdf:resource="http://nlpkg.sebis.cit.tum.de/nlp-fos-hierarchy.owl#Graphs"/>
        <nlp-taxonomy:superFieldOf rdf:resource="http://nlpkg.sebis.cit.tum.de/nlp-fos-hierarchy.owl#Knowledge_Base_Question_Answering"/>
        <nlp-taxonomy:superFieldOf rdf:resource="http://nlpkg.sebis.cit.tum.de/nlp-fos-hierarchy.owl#Taxonomies"/>
        <nlp-taxonomy:superFieldOf rdf:resource="http://nlpkg.sebis.cit.tum.de/nlp-fos-hierarchy.owl#Thesaurus"/>
        <nlp-taxonomy:superFieldOf rdf:resource="http://nlpkg.sebis.cit.tum.de/nlp-fos-hierarchy.owl#Tree"/>
        <survey>https://aclanthology.org/2021.emnlp-main.81</survey>
        <survey>https://arxiv.org/abs/2204.06031</survey>
        <survey>https://arxiv.org/abs/2302.02093</survey>
        <survey>https://arxiv.org/abs/2303.07616</survey>
        <nlp-taxonomy:level rdf:datatype="http://www.w3.org/2001/XMLSchema#integer">3</nlp-taxonomy:level>
        <dcterms:description xml:lang="en">Knowledge Bases refer to structured collections of information or data that are organized and stored in a way that makes it accessible and usable for computational analysis and reasoning. Knowledge bases typically consist of facts, entities, relationships, and attributes. These knowledge bases can be manually curated or automatically generated from large text corpora and are essential for enhancing the understanding and reasoning abilities of NLP systems.</dcterms:description>
        <oboInOwl:hasSynonym xml:lang="en">KB</oboInOwl:hasSynonym>
        <oboInOwl:hasSynonym xml:lang="en">KBs</oboInOwl:hasSynonym>
        <rdfs:label xml:lang="en">Knowledge Bases</rdfs:label>
    </owl:NamedIndividual>
    


    <!-- http://nlpkg.sebis.cit.tum.de/nlp-fos-hierarchy.owl#Knowledge_Distillation -->

    <owl:NamedIndividual rdf:about="http://nlpkg.sebis.cit.tum.de/nlp-fos-hierarchy.owl#Knowledge_Distillation">
        <rdf:type rdf:resource="http://nlpkg.sebis.cit.tum.de/nlp-fos-hierarchy.owl#Task"/>
        <rdf:type rdf:resource="http://nlpkg.sebis.cit.tum.de/nlp-taxonomy.owl#FieldOfStudy"/>
        <uses rdf:resource="http://nlpkg.sebis.cit.tum.de/nlp-fos-hierarchy.owl#Learn_to_Knowledge_Distillation"/>
        <nlp-taxonomy:subFieldOf rdf:resource="http://nlpkg.sebis.cit.tum.de/nlp-fos-hierarchy.owl#Efficient_Transformers"/>
        <nlp-taxonomy:level rdf:datatype="http://www.w3.org/2001/XMLSchema#integer">5</nlp-taxonomy:level>
        <dcterms:description xml:lang="en">Knowledge Distillation (KD) is a technique where a smaller, simpler model (student) is trained to mimic the behavior of a larger, more complex model (teacher). The aim is to transfer the knowledge from the teacher model to the student model. This is particularly useful in NLP tasks where deploying large models is computationally expensive. The student model, being smaller, is more efficient to use but still maintains a high level of performance by learning from the teacher model.</dcterms:description>
        <oboInOwl:hasSynonym xml:lang="en">KD</oboInOwl:hasSynonym>
        <rdfs:label xml:lang="en">Knowledge Distillation</rdfs:label>
    </owl:NamedIndividual>
    


    <!-- http://nlpkg.sebis.cit.tum.de/nlp-fos-hierarchy.owl#Knowledge_Editing -->

    <owl:NamedIndividual rdf:about="http://nlpkg.sebis.cit.tum.de/nlp-fos-hierarchy.owl#Knowledge_Editing">
        <rdf:type rdf:resource="http://nlpkg.sebis.cit.tum.de/nlp-fos-hierarchy.owl#Task"/>
        <rdf:type rdf:resource="http://nlpkg.sebis.cit.tum.de/nlp-taxonomy.owl#FieldOfStudy"/>
        <nlp-taxonomy:subFieldOf rdf:resource="http://nlpkg.sebis.cit.tum.de/nlp-fos-hierarchy.owl#Knowledge_Augmented_Language_Models"/>
        <survey>https://arxiv.org/abs/2310.02129</survey>
        <survey>https://arxiv.org/abs/2310.16218</survey>
        <survey>https://arxiv.org/abs/2310.19704</survey>
        <survey>https://arxiv.org/abs/2401.01286</survey>
        <nlp-taxonomy:level rdf:datatype="http://www.w3.org/2001/XMLSchema#integer">5</nlp-taxonomy:level>
        <dcterms:description xml:lang="en">Knowledge Editing methods aim to precisely modify language models to incorporate specific knowledge, without negatively influencing other irrelevant knowledge. In knowledge editing, the update of a specific piece of knowledge in language models is typically formulated as an edit, such as rectifying the answer to “Who is the president of the USA?” from “Trump” to “Biden”. Regarding a specific edit, knowledge editing strategies typically modify the model output by either introducing an auxiliary network (or set of parameters) into the pre-trained model or updating the (partial) parameters to store the new knowledge.</dcterms:description>
        <oboInOwl:hasSynonym xml:lang="en">KME</oboInOwl:hasSynonym>
        <oboInOwl:hasSynonym xml:lang="en">Knowledge-based Model Editing</oboInOwl:hasSynonym>
        <rdfs:label xml:lang="en">Knowledge Editing</rdfs:label>
    </owl:NamedIndividual>
    


    <!-- http://nlpkg.sebis.cit.tum.de/nlp-fos-hierarchy.owl#Knowledge_Graph_Embeddings -->

    <owl:NamedIndividual rdf:about="http://nlpkg.sebis.cit.tum.de/nlp-fos-hierarchy.owl#Knowledge_Graph_Embeddings">
        <rdf:type rdf:resource="http://nlpkg.sebis.cit.tum.de/nlp-fos-hierarchy.owl#DataStructure"/>
        <rdf:type rdf:resource="http://nlpkg.sebis.cit.tum.de/nlp-taxonomy.owl#FieldOfStudy"/>
        <nlp-taxonomy:subFieldOf rdf:resource="http://nlpkg.sebis.cit.tum.de/nlp-taxonomy.owl#Knowledge_Graph_Reasoning"/>
        <nlp-taxonomy:subFieldOf rdf:resource="http://nlpkg.sebis.cit.tum.de/nlp-taxonomy.owl#Representation_Learning"/>
        <survey>https://arxiv.org/abs/1812.10901</survey>
        <survey>https://arxiv.org/abs/1910.12507</survey>
        <survey>https://arxiv.org/abs/2002.00819</survey>
        <survey>https://arxiv.org/abs/2010.13688</survey>
        <survey>https://arxiv.org/abs/2107.07842</survey>
        <survey>https://arxiv.org/abs/2211.03536</survey>
        <nlp-taxonomy:level rdf:datatype="http://www.w3.org/2001/XMLSchema#integer">3</nlp-taxonomy:level>
        <nlp-taxonomy:level rdf:datatype="http://www.w3.org/2001/XMLSchema#integer">7</nlp-taxonomy:level>
        <dcterms:description xml:lang="en">Knowledge Graph Embeddings (KGE) refer to the process of transforming the entities and relationships in a knowledge graph into numerical vectors or embeddings. These embeddings capture the semantic information and the complex relationships between entities in a multi-dimensional space.</dcterms:description>
        <oboInOwl:hasSynonym xml:lang="en">KG Embeddings</oboInOwl:hasSynonym>
        <oboInOwl:hasSynonym>KGE</oboInOwl:hasSynonym>
        <oboInOwl:hasSynonym xml:lang="en">Knowledge Representation Learning</oboInOwl:hasSynonym>
        <rdfs:label xml:lang="en">Knowledge Graph Embeddings</rdfs:label>
    </owl:NamedIndividual>
    


    <!-- http://nlpkg.sebis.cit.tum.de/nlp-fos-hierarchy.owl#Knowledge_Graph_Error_Detection -->

    <owl:NamedIndividual rdf:about="http://nlpkg.sebis.cit.tum.de/nlp-fos-hierarchy.owl#Knowledge_Graph_Error_Detection">
        <rdf:type rdf:resource="http://nlpkg.sebis.cit.tum.de/nlp-fos-hierarchy.owl#Task"/>
        <rdf:type rdf:resource="http://nlpkg.sebis.cit.tum.de/nlp-taxonomy.owl#FieldOfStudy"/>
        <nlp-taxonomy:subFieldOf rdf:resource="http://nlpkg.sebis.cit.tum.de/nlp-taxonomy.owl#Knowledge_Graph_Reasoning"/>
        <nlp-taxonomy:level rdf:datatype="http://www.w3.org/2001/XMLSchema#integer">3</nlp-taxonomy:level>
        <nlp-taxonomy:level rdf:datatype="http://www.w3.org/2001/XMLSchema#integer">7</nlp-taxonomy:level>
        <dcterms:description xml:lang="en">Knowledge Graph Error Detection refers to the process of identifying and correcting inaccuracies, inconsistencies, or discrepancies in the data represented in a knowledge graph. This could include incorrect or missing relationships, inaccurate entity attributes, or other forms of misinformation. The goal is to improve the quality and reliability of the information in the knowledge graph.</dcterms:description>
        <oboInOwl:hasSynonym xml:lang="en">KG Error Detection</oboInOwl:hasSynonym>
        <rdfs:label xml:lang="en">Knowledge Graph Error Detection</rdfs:label>
    </owl:NamedIndividual>
    


    <!-- http://nlpkg.sebis.cit.tum.de/nlp-fos-hierarchy.owl#Knowledge_Graph_Question_Answering -->

    <owl:NamedIndividual rdf:about="http://nlpkg.sebis.cit.tum.de/nlp-fos-hierarchy.owl#Knowledge_Graph_Question_Answering">
        <rdf:type rdf:resource="http://nlpkg.sebis.cit.tum.de/nlp-fos-hierarchy.owl#Task"/>
        <rdf:type rdf:resource="http://nlpkg.sebis.cit.tum.de/nlp-taxonomy.owl#FieldOfStudy"/>
        <nlp-taxonomy:subFieldOf rdf:resource="http://nlpkg.sebis.cit.tum.de/nlp-fos-hierarchy.owl#Knowledge_Base_Question_Answering"/>
        <nlp-taxonomy:subFieldOf rdf:resource="http://nlpkg.sebis.cit.tum.de/nlp-fos-hierarchy.owl#Knowledge_Graphs"/>
        <nlp-taxonomy:superFieldOf rdf:resource="http://nlpkg.sebis.cit.tum.de/nlp-fos-hierarchy.owl#Multi-Hop_Reasoning"/>
        <nlp-taxonomy:superFieldOf rdf:resource="http://nlpkg.sebis.cit.tum.de/nlp-fos-hierarchy.owl#One-Hop_Reasoning"/>
        <survey>https://arxiv.org/abs/1907.09361</survey>
        <nlp-taxonomy:level rdf:datatype="http://www.w3.org/2001/XMLSchema#integer">4</nlp-taxonomy:level>
        <nlp-taxonomy:level rdf:datatype="http://www.w3.org/2001/XMLSchema#integer">5</nlp-taxonomy:level>
        <nlp-taxonomy:level rdf:datatype="http://www.w3.org/2001/XMLSchema#integer">6</nlp-taxonomy:level>
        <dcterms:description xml:lang="en">Knowledge Graph Question Answering (KGQA) refers to the task of using a knowledge graph, which is a structured representation of information, to answer natural language questions. KGQA systems extract relevant information from the knowledge graph to provide accurate answers to user queries.</dcterms:description>
        <oboInOwl:hasSynonym xml:lang="en">KG Question Answering</oboInOwl:hasSynonym>
        <oboInOwl:hasSynonym xml:lang="en">KGQA</oboInOwl:hasSynonym>
        <oboInOwl:hasSynonym xml:lang="en">Question Answering over Knowledge Graphs</oboInOwl:hasSynonym>
        <rdfs:label xml:lang="en">Knowledge Graph Question Answering</rdfs:label>
    </owl:NamedIndividual>
    


    <!-- http://nlpkg.sebis.cit.tum.de/nlp-fos-hierarchy.owl#Knowledge_Graphs -->

    <owl:NamedIndividual rdf:about="http://nlpkg.sebis.cit.tum.de/nlp-fos-hierarchy.owl#Knowledge_Graphs">
        <rdf:type rdf:resource="http://nlpkg.sebis.cit.tum.de/nlp-fos-hierarchy.owl#DataStructure"/>
        <rdf:type rdf:resource="http://nlpkg.sebis.cit.tum.de/nlp-taxonomy.owl#FieldOfStudy"/>
        <nlp-taxonomy:subFieldOf rdf:resource="http://nlpkg.sebis.cit.tum.de/nlp-fos-hierarchy.owl#Graphs"/>
        <nlp-taxonomy:superFieldOf rdf:resource="http://nlpkg.sebis.cit.tum.de/nlp-fos-hierarchy.owl#Knowledge_Graph_Question_Answering"/>
        <nlp-taxonomy:superFieldOf rdf:resource="http://nlpkg.sebis.cit.tum.de/nlp-fos-hierarchy.owl#Knowledge_Graph_Construction_&amp;_Completion"/>
        <nlp-taxonomy:superFieldOf rdf:resource="http://nlpkg.sebis.cit.tum.de/nlp-taxonomy.owl#Knowledge_Graph_Reasoning"/>
        <survey>https://aclanthology.org/2022.aacl-main.46</survey>
        <survey>https://aclanthology.org/2022.aacl-main.49</survey>
        <survey>https://arxiv.org/abs/1503.00759</survey>
        <survey>https://arxiv.org/abs/2002.00388</survey>
        <survey>https://arxiv.org/abs/2003.02320</survey>
        <survey>https://arxiv.org/abs/2011.10180</survey>
        <survey>https://arxiv.org/abs/2112.15280</survey>
        <survey>https://arxiv.org/abs/2201.11794</survey>
        <survey>https://arxiv.org/abs/2303.02411</survey>
        <survey>https://arxiv.org/abs/2308.10168</survey>
        <survey>https://arxiv.org/abs/2308.13676</survey>
        <nlp-taxonomy:level rdf:datatype="http://www.w3.org/2001/XMLSchema#integer">5</nlp-taxonomy:level>
        <dcterms:description xml:lang="en">Knowledge Graphs are graphs of data intended to accumulate and convey knowledge of the real world, whose nodes represent entities of interest and whose edges represent relations between these entities</dcterms:description>
        <oboInOwl:hasSynonym xml:lang="en">KG</oboInOwl:hasSynonym>
        <oboInOwl:hasSynonym xml:lang="en">KGs</oboInOwl:hasSynonym>
        <rdfs:label xml:lang="en">Knowledge Graphs</rdfs:label>
    </owl:NamedIndividual>
    


    <!-- http://nlpkg.sebis.cit.tum.de/nlp-fos-hierarchy.owl#Language_Grounding -->

    <owl:NamedIndividual rdf:about="http://nlpkg.sebis.cit.tum.de/nlp-fos-hierarchy.owl#Language_Grounding">
        <rdf:type rdf:resource="http://nlpkg.sebis.cit.tum.de/nlp-fos-hierarchy.owl#Task"/>
        <rdf:type rdf:resource="http://nlpkg.sebis.cit.tum.de/nlp-taxonomy.owl#FieldOfStudy"/>
        <uses rdf:resource="http://nlpkg.sebis.cit.tum.de/nlp-taxonomy.owl#Programming_Languages_In_NLP"/>
        <uses rdf:resource="http://nlpkg.sebis.cit.tum.de/nlp-taxonomy.owl#Structured_Data_In_NLP"/>
        <uses rdf:resource="http://nlpkg.sebis.cit.tum.de/nlp-taxonomy.owl#Visual_Data_In_NLP"/>
        <uses rdf:resource="http://nlpkg.sebis.cit.tum.de/nlp-taxonomy.owl#Speech_&amp;_Audio_In_NLP"/>
        <nlp-taxonomy:subFieldOf rdf:resource="http://nlpkg.sebis.cit.tum.de/nlp-taxonomy.owl#Multimodality"/>
        <nlp-taxonomy:level rdf:datatype="http://www.w3.org/2001/XMLSchema#integer">2</nlp-taxonomy:level>
        <dcterms:description xml:lang="en">Language Grounding is the ability to tie verbal expressions to their referents in the non-linguistic world. The non-linguistic world can be physical or non-physical such as real-world objects,  visual content, actions, or concepts. It involves bridging the gap between linguistic symbols and the underlying meaning or context.</dcterms:description>
        <oboInOwl:hasSynonym xml:lang="en">Grounding</oboInOwl:hasSynonym>
        <rdfs:label xml:lang="en">Language Grounding</rdfs:label>
    </owl:NamedIndividual>
    


    <!-- http://nlpkg.sebis.cit.tum.de/nlp-fos-hierarchy.owl#Language_Identification -->

    <owl:NamedIndividual rdf:about="http://nlpkg.sebis.cit.tum.de/nlp-fos-hierarchy.owl#Language_Identification">
        <rdf:type rdf:resource="http://nlpkg.sebis.cit.tum.de/nlp-fos-hierarchy.owl#Task"/>
        <rdf:type rdf:resource="http://nlpkg.sebis.cit.tum.de/nlp-taxonomy.owl#FieldOfStudy"/>
        <nlp-taxonomy:subFieldOf rdf:resource="http://nlpkg.sebis.cit.tum.de/nlp-taxonomy.owl#Text_Classification"/>
        <code>https://github.com/bsolomon1124/pycld3</code>
        <survey>https://arxiv.org/abs/1804.08186</survey>
        <nlp-taxonomy:level rdf:datatype="http://www.w3.org/2001/XMLSchema#integer">3</nlp-taxonomy:level>
        <dcterms:description xml:lang="en">Language Identification refers to the task of automatically determining the natural language of a given content.</dcterms:description>
        <oboInOwl:hasSynonym xml:lang="en">Language Classification</oboInOwl:hasSynonym>
        <oboInOwl:hasSynonym xml:lang="en">Language Detection</oboInOwl:hasSynonym>
        <rdfs:label xml:lang="en">Language Identification</rdfs:label>
    </owl:NamedIndividual>
    


    <!-- http://nlpkg.sebis.cit.tum.de/nlp-fos-hierarchy.owl#Language_Model_Adapters -->

    <owl:NamedIndividual rdf:about="http://nlpkg.sebis.cit.tum.de/nlp-fos-hierarchy.owl#Language_Model_Adapters">
        <rdf:type rdf:resource="http://nlpkg.sebis.cit.tum.de/nlp-fos-hierarchy.owl#OtherScientificField"/>
        <rdf:type rdf:resource="http://nlpkg.sebis.cit.tum.de/nlp-taxonomy.owl#FieldOfStudy"/>
        <nlp-taxonomy:subFieldOf rdf:resource="http://nlpkg.sebis.cit.tum.de/nlp-fos-hierarchy.owl#Parameter-Efficient_Fine-Tuning"/>
        <code>https://github.com/Adapter-Hub/adapter-transformers</code>
        <origin>https://arxiv.org/abs/1902.00751</origin>
        <relevantInformation>https://adapterhub.ml</relevantInformation>
        <nlp-taxonomy:level rdf:datatype="http://www.w3.org/2001/XMLSchema#integer">4</nlp-taxonomy:level>
        <nlp-taxonomy:level rdf:datatype="http://www.w3.org/2001/XMLSchema#integer">5</nlp-taxonomy:level>
        <dcterms:description xml:lang="en">Language Model Adapters are a method of fine-tuning pre-trained language models. Instead of fine-tuning all parameters of the model, only a small set of parameters in added adapter modules are trained. This approach allows for a more efficient adaptation of the model to a specific task, while preserving the original model weights. It also enables multi-task learning and transfer learning, as different adapters can be plugged into the model for different tasks.</dcterms:description>
        <oboInOwl:hasSynonym xml:lang="en">Adapters</oboInOwl:hasSynonym>
        <rdfs:label xml:lang="en">Language Model Adapters</rdfs:label>
    </owl:NamedIndividual>
    


    <!-- http://nlpkg.sebis.cit.tum.de/nlp-fos-hierarchy.owl#Language_Model_Alignment -->

    <owl:NamedIndividual rdf:about="http://nlpkg.sebis.cit.tum.de/nlp-fos-hierarchy.owl#Language_Model_Alignment">
        <rdf:type rdf:resource="http://nlpkg.sebis.cit.tum.de/nlp-fos-hierarchy.owl#Task"/>
        <rdf:type rdf:resource="http://nlpkg.sebis.cit.tum.de/nlp-taxonomy.owl#FieldOfStudy"/>
        <usedFor rdf:resource="http://nlpkg.sebis.cit.tum.de/nlp-fos-hierarchy.owl#Chatbots"/>
        <usedFor rdf:resource="http://nlpkg.sebis.cit.tum.de/nlp-taxonomy.owl#Robustness_In_NLP"/>
        <uses rdf:resource="http://nlpkg.sebis.cit.tum.de/nlp-fos-hierarchy.owl#Controllable_Text_Generation"/>
        <uses rdf:resource="http://nlpkg.sebis.cit.tum.de/nlp-fos-hierarchy.owl#Instruction_Learning"/>
        <nlp-taxonomy:subFieldOf rdf:resource="http://nlpkg.sebis.cit.tum.de/nlp-taxonomy.owl#Ethical_NLP"/>
        <nlp-taxonomy:subFieldOf rdf:resource="http://nlpkg.sebis.cit.tum.de/nlp-taxonomy.owl#Language_Models"/>
        <origin>https://arxiv.org/abs/2203.02155</origin>
        <relevantInformation>https://github.com/GaryYufei/AlignLLMHumanSurvey</relevantInformation>
        <survey>https://aclanthology.org/2020.findings-emnlp.301</survey>
        <survey>https://arxiv.org/abs/2307.12966</survey>
        <survey>https://arxiv.org/abs/2308.05374</survey>
        <survey>https://arxiv.org/abs/2308.12014</survey>
        <survey>https://arxiv.org/abs/2309.15025</survey>
        <nlp-taxonomy:level rdf:datatype="http://www.w3.org/2001/XMLSchema#integer">3</nlp-taxonomy:level>
        <dcterms:description xml:lang="en">Language Model Alignment is the process of ensuring that a language model&apos;s outputs align with the preferences and intentions of a human user. It involves training the model to understand and respond accurately to the inputs it receives, minimizing misunderstanding or misinterpretation. This concept is crucial in developing AI systems that can effectively and safely interact with humans meaningfully.</dcterms:description>
        <oboInOwl:hasSynonym xml:lang="en">Alignment</oboInOwl:hasSynonym>
        <rdfs:label xml:lang="en">Language Model Alignment</rdfs:label>
    </owl:NamedIndividual>
    


    <!-- http://nlpkg.sebis.cit.tum.de/nlp-fos-hierarchy.owl#Language_Model_Hallucination -->

    <owl:NamedIndividual rdf:about="http://nlpkg.sebis.cit.tum.de/nlp-fos-hierarchy.owl#Language_Model_Hallucination">
        <rdf:type rdf:resource="http://nlpkg.sebis.cit.tum.de/nlp-fos-hierarchy.owl#OtherScientificField"/>
        <rdf:type rdf:resource="http://nlpkg.sebis.cit.tum.de/nlp-taxonomy.owl#FieldOfStudy"/>
        <nlp-taxonomy:subFieldOf rdf:resource="http://nlpkg.sebis.cit.tum.de/nlp-taxonomy.owl#Language_Models"/>
        <nlp-taxonomy:subFieldOf rdf:resource="http://nlpkg.sebis.cit.tum.de/nlp-taxonomy.owl#Robustness_In_NLP"/>
        <nlp-taxonomy:superFieldOf rdf:resource="http://nlpkg.sebis.cit.tum.de/nlp-fos-hierarchy.owl#Hallucination_Detection"/>
        <nlp-taxonomy:superFieldOf rdf:resource="http://nlpkg.sebis.cit.tum.de/nlp-fos-hierarchy.owl#Hallucination_Prevention"/>
        <survey>https://arxiv.org/abs/2202.03629</survey>
        <survey>https://arxiv.org/abs/2309.01219</survey>
        <survey>https://arxiv.org/abs/2309.05922</survey>
        <survey>https://arxiv.org/abs/2309.06794</survey>
        <survey>https://arxiv.org/abs/2310.14564</survey>
        <survey>https://arxiv.org/abs/2311.05232</survey>
        <nlp-taxonomy:level rdf:datatype="http://www.w3.org/2001/XMLSchema#integer">3</nlp-taxonomy:level>
        <dcterms:description xml:lang="en">Language Model Hallucination refers to the phenomenon where the model generates text or information that is fluent and grammatically correct but factually incorrect or unrelated to the input. It&apos;s a significant challenge in developing reliable and accurate language models.</dcterms:description>
        <oboInOwl:hasSynonym xml:lang="en">Hallucination</oboInOwl:hasSynonym>
        <rdfs:label xml:lang="en">Language Model Hallucination</rdfs:label>
    </owl:NamedIndividual>
    


    <!-- http://nlpkg.sebis.cit.tum.de/nlp-fos-hierarchy.owl#Language_Model_Mechanisms -->

    <owl:NamedIndividual rdf:about="http://nlpkg.sebis.cit.tum.de/nlp-fos-hierarchy.owl#Language_Model_Mechanisms">
        <rdf:type rdf:resource="http://nlpkg.sebis.cit.tum.de/nlp-fos-hierarchy.owl#OtherScientificField"/>
        <rdf:type rdf:resource="http://nlpkg.sebis.cit.tum.de/nlp-taxonomy.owl#FieldOfStudy"/>
        <nlp-taxonomy:subFieldOf rdf:resource="http://nlpkg.sebis.cit.tum.de/nlp-taxonomy.owl#Language_Models"/>
        <nlp-taxonomy:superFieldOf rdf:resource="http://nlpkg.sebis.cit.tum.de/nlp-fos-hierarchy.owl#Attention"/>
        <nlp-taxonomy:superFieldOf rdf:resource="http://nlpkg.sebis.cit.tum.de/nlp-fos-hierarchy.owl#Decoding"/>
        <nlp-taxonomy:superFieldOf rdf:resource="http://nlpkg.sebis.cit.tum.de/nlp-fos-hierarchy.owl#Positional_Encoding"/>
        <nlp-taxonomy:superFieldOf rdf:resource="http://nlpkg.sebis.cit.tum.de/nlp-fos-hierarchy.owl#Regularization"/>
        <nlp-taxonomy:level rdf:datatype="http://www.w3.org/2001/XMLSchema#integer">3</nlp-taxonomy:level>
        <dcterms:description xml:lang="en">Language Model Mechanisms refer to the design decisions and concepts used to build language models.</dcterms:description>
        <rdfs:label xml:lang="en">Language Model Mechanisms</rdfs:label>
    </owl:NamedIndividual>
    


    <!-- http://nlpkg.sebis.cit.tum.de/nlp-fos-hierarchy.owl#Language_Model_Quantization -->

    <owl:NamedIndividual rdf:about="http://nlpkg.sebis.cit.tum.de/nlp-fos-hierarchy.owl#Language_Model_Quantization">
        <rdf:type rdf:resource="http://nlpkg.sebis.cit.tum.de/nlp-fos-hierarchy.owl#Task"/>
        <rdf:type rdf:resource="http://nlpkg.sebis.cit.tum.de/nlp-taxonomy.owl#FieldOfStudy"/>
        <nlp-taxonomy:subFieldOf rdf:resource="http://nlpkg.sebis.cit.tum.de/nlp-taxonomy.owl#Language_Models"/>
        <nlp-taxonomy:subFieldOf rdf:resource="http://nlpkg.sebis.cit.tum.de/nlp-taxonomy.owl#Green_&amp;_Sustainable_NLP"/>
        <nlp-taxonomy:superFieldOf rdf:resource="http://nlpkg.sebis.cit.tum.de/nlp-fos-hierarchy.owl#Post-Training_Quantization"/>
        <nlp-taxonomy:superFieldOf rdf:resource="http://nlpkg.sebis.cit.tum.de/nlp-fos-hierarchy.owl#Quantization_Aware_Training"/>
        <relevantInformation>https://huggingface.co/docs/optimum/concept_guides/quantization</relevantInformation>
        <nlp-taxonomy:level rdf:datatype="http://www.w3.org/2001/XMLSchema#integer">3</nlp-taxonomy:level>
        <nlp-taxonomy:level rdf:datatype="http://www.w3.org/2001/XMLSchema#integer">4</nlp-taxonomy:level>
        <dcterms:description xml:lang="en">Language Model Quantization refers to the process of reducing the precision of the numerical values in a language model to make it smaller and faster. This involves converting the continuous values into discrete counterparts. The main goal of quantization is to reduce the computational and storage requirements of the model, which can be particularly beneficial for deploying NLP models on devices with limited resources. However, it&apos;s a challenge to perform quantization without significantly impacting the model&apos;s performance.</dcterms:description>
        <oboInOwl:hasSynonym xml:lang="en">Quantization</oboInOwl:hasSynonym>
        <rdfs:label xml:lang="en">Language Model Quantization</rdfs:label>
    </owl:NamedIndividual>
    


    <!-- http://nlpkg.sebis.cit.tum.de/nlp-fos-hierarchy.owl#Learn_to_Knowledge_Distillation -->

    <owl:NamedIndividual rdf:about="http://nlpkg.sebis.cit.tum.de/nlp-fos-hierarchy.owl#Learn_to_Knowledge_Distillation">
        <rdf:type rdf:resource="http://nlpkg.sebis.cit.tum.de/nlp-fos-hierarchy.owl#Task"/>
        <rdf:type rdf:resource="http://nlpkg.sebis.cit.tum.de/nlp-taxonomy.owl#FieldOfStudy"/>
        <usedFor rdf:resource="http://nlpkg.sebis.cit.tum.de/nlp-fos-hierarchy.owl#Knowledge_Distillation"/>
        <nlp-taxonomy:subFieldOf rdf:resource="http://nlpkg.sebis.cit.tum.de/nlp-fos-hierarchy.owl#Meta-Learning"/>
        <nlp-taxonomy:level rdf:datatype="http://www.w3.org/2001/XMLSchema#integer">4</nlp-taxonomy:level>
        <dcterms:description xml:lang="en">Learn to Knowledge Distillation is a concept that involves training a smaller model (student) to mimic the behavior of a larger, more complex model (teacher). The goal is to transfer the knowledge from the larger model to the smaller one, thereby improving the efficiency and performance of the smaller model. In the context of Meta-Learning, this involves to train a meta teacher model that works better than a single teacher model and to optimize the transferring process and force the teacher model to be aware of the student model.</dcterms:description>
        <rdfs:label xml:lang="en">Learn to Knowledge Distillation</rdfs:label>
    </owl:NamedIndividual>
    


    <!-- http://nlpkg.sebis.cit.tum.de/nlp-fos-hierarchy.owl#Learn_to_Lifelong_Learning -->

    <owl:NamedIndividual rdf:about="http://nlpkg.sebis.cit.tum.de/nlp-fos-hierarchy.owl#Learn_to_Lifelong_Learning">
        <rdf:type rdf:resource="http://nlpkg.sebis.cit.tum.de/nlp-fos-hierarchy.owl#Task"/>
        <rdf:type rdf:resource="http://nlpkg.sebis.cit.tum.de/nlp-taxonomy.owl#FieldOfStudy"/>
        <nlp-taxonomy:subFieldOf rdf:resource="http://nlpkg.sebis.cit.tum.de/nlp-fos-hierarchy.owl#Meta-Learning"/>
        <nlp-taxonomy:level rdf:datatype="http://www.w3.org/2001/XMLSchema#integer">4</nlp-taxonomy:level>
        <dcterms:description xml:lang="en">Learn to Lifelong Learning refers to the ability of a model to continuously learn and adapt from new data or experiences over time. This concept emphasizes the development of learning algorithms that can not only learn from a single task but also generalize their learning to new tasks. It involves the model&apos;s ability to remember previous knowledge, adapt to new tasks with few examples, and not forget the old tasks while learning new ones (avoiding catastrophic forgetting).</dcterms:description>
        <oboInOwl:hasSynonym xml:lang="en">Meta-Learning to Improve Lifelong Learning (LLL)</oboInOwl:hasSynonym>
        <rdfs:label xml:lang="en">Learn to Lifelong Learning</rdfs:label>
    </owl:NamedIndividual>
    


    <!-- http://nlpkg.sebis.cit.tum.de/nlp-fos-hierarchy.owl#Learning_to_Compare -->

    <owl:NamedIndividual rdf:about="http://nlpkg.sebis.cit.tum.de/nlp-fos-hierarchy.owl#Learning_to_Compare">
        <rdf:type rdf:resource="http://nlpkg.sebis.cit.tum.de/nlp-fos-hierarchy.owl#Task"/>
        <rdf:type rdf:resource="http://nlpkg.sebis.cit.tum.de/nlp-taxonomy.owl#FieldOfStudy"/>
        <nlp-taxonomy:subFieldOf rdf:resource="http://nlpkg.sebis.cit.tum.de/nlp-fos-hierarchy.owl#Meta-Learning"/>
        <nlp-taxonomy:level rdf:datatype="http://www.w3.org/2001/XMLSchema#integer">4</nlp-taxonomy:level>
        <dcterms:description xml:lang="en">Learning to Compare refers to a method where the model learns to compare new information with existing knowledge. This is done by training the model on a variety of tasks, and then using this learned knowledge to make comparisons and predictions on new, unseen tasks. In NLP, this could involve comparing the semantic similarity of sentences or documents, or comparing the relevance of a document to a query. The goal is to enable the model to generalize from its learned knowledge to new tasks, improving its performance and adaptability.</dcterms:description>
        <rdfs:label xml:lang="en">Learning to Compare</rdfs:label>
    </owl:NamedIndividual>
    


    <!-- http://nlpkg.sebis.cit.tum.de/nlp-fos-hierarchy.owl#Learning_to_Initialize -->

    <owl:NamedIndividual rdf:about="http://nlpkg.sebis.cit.tum.de/nlp-fos-hierarchy.owl#Learning_to_Initialize">
        <rdf:type rdf:resource="http://nlpkg.sebis.cit.tum.de/nlp-fos-hierarchy.owl#Task"/>
        <rdf:type rdf:resource="http://nlpkg.sebis.cit.tum.de/nlp-taxonomy.owl#FieldOfStudy"/>
        <nlp-taxonomy:subFieldOf rdf:resource="http://nlpkg.sebis.cit.tum.de/nlp-fos-hierarchy.owl#Meta-Learning"/>
        <nlp-taxonomy:superFieldOf rdf:resource="http://nlpkg.sebis.cit.tum.de/nlp-fos-hierarchy.owl#Model-Agnostic_Meta-Learning"/>
        <nlp-taxonomy:level rdf:datatype="http://www.w3.org/2001/XMLSchema#integer">4</nlp-taxonomy:level>
        <dcterms:description xml:lang="en">Learning to Initialize refers to the process where the model learns the optimal initialization of parameters. This is done so that a few steps of gradient descent during the fine-tuning phase can adapt the model to a specific task. This concept is particularly useful in meta-learning where the goal is to design models that can learn new skills or adapt to new environments rapidly with a few training examples. In the context of NLP, this could mean adapting to new languages or new language tasks.</dcterms:description>
        <rdfs:label xml:lang="en">Learning to Initialize</rdfs:label>
    </owl:NamedIndividual>
    


    <!-- http://nlpkg.sebis.cit.tum.de/nlp-fos-hierarchy.owl#Lemmatization -->

    <owl:NamedIndividual rdf:about="http://nlpkg.sebis.cit.tum.de/nlp-fos-hierarchy.owl#Lemmatization">
        <rdf:type rdf:resource="http://nlpkg.sebis.cit.tum.de/nlp-fos-hierarchy.owl#Task"/>
        <rdf:type rdf:resource="http://nlpkg.sebis.cit.tum.de/nlp-taxonomy.owl#FieldOfStudy"/>
        <usedFor rdf:resource="http://nlpkg.sebis.cit.tum.de/nlp-taxonomy.owl#Text_Normalization"/>
        <nlp-taxonomy:subFieldOf rdf:resource="http://nlpkg.sebis.cit.tum.de/nlp-taxonomy.owl#Morphology"/>
        <code>https://spacy.io/usage/linguistic-features#lemmatization</code>
        <nlp-taxonomy:level rdf:datatype="http://www.w3.org/2001/XMLSchema#integer">3</nlp-taxonomy:level>
        <dcterms:description xml:lang="en">Lemmatization is the process of reducing words to their base or root form, known as a lemma. Unlike stemming, which simply removes certain end characters from words, lemmatization considers the context and part of speech of a word in order to accurately convert it to its base form. For example, the word &quot;better&quot; would be lemmatized to &quot;good&quot;.</dcterms:description>
        <rdfs:label xml:lang="en">Lemmatization</rdfs:label>
    </owl:NamedIndividual>
    


    <!-- http://nlpkg.sebis.cit.tum.de/nlp-fos-hierarchy.owl#Lexical_Sample_Word_Sense_Disambiguation -->

    <owl:NamedIndividual rdf:about="http://nlpkg.sebis.cit.tum.de/nlp-fos-hierarchy.owl#Lexical_Sample_Word_Sense_Disambiguation">
        <rdf:type rdf:resource="http://nlpkg.sebis.cit.tum.de/nlp-fos-hierarchy.owl#Task"/>
        <rdf:type rdf:resource="http://nlpkg.sebis.cit.tum.de/nlp-taxonomy.owl#FieldOfStudy"/>
        <nlp-taxonomy:subFieldOf rdf:resource="http://nlpkg.sebis.cit.tum.de/nlp-taxonomy.owl#Word_Sense_Disambiguation"/>
        <nlp-taxonomy:level rdf:datatype="http://www.w3.org/2001/XMLSchema#integer">3</nlp-taxonomy:level>
        <dcterms:description xml:lang="en">Lexical Sample Word Sense Disambiguation (WSD) is a task where the system is given a particular word along with a context, and it has to correctly identify the sense or meaning of the word in that context. This task is performed on a small sample of specific words, hence the term &apos;lexical sample&apos;. The challenge lies in the fact that many words in a language have multiple meanings and the system has to accurately determine which meaning is applicable in the given context.</dcterms:description>
        <oboInOwl:hasSynonym xml:lang="en">Lexical Sample WSD</oboInOwl:hasSynonym>
        <rdfs:label xml:lang="en">Lexical Sample Word Sense Disambiguation</rdfs:label>
    </owl:NamedIndividual>
    


    <!-- http://nlpkg.sebis.cit.tum.de/nlp-fos-hierarchy.owl#Lexical_Simplification -->

    <owl:NamedIndividual rdf:about="http://nlpkg.sebis.cit.tum.de/nlp-fos-hierarchy.owl#Lexical_Simplification">
        <rdf:type rdf:resource="http://nlpkg.sebis.cit.tum.de/nlp-fos-hierarchy.owl#Task"/>
        <rdf:type rdf:resource="http://nlpkg.sebis.cit.tum.de/nlp-taxonomy.owl#FieldOfStudy"/>
        <nlp-taxonomy:subFieldOf rdf:resource="http://nlpkg.sebis.cit.tum.de/nlp-fos-hierarchy.owl#Text_Simplification"/>
        <survey>https://arxiv.org/abs/2305.12000</survey>
        <nlp-taxonomy:level rdf:datatype="http://www.w3.org/2001/XMLSchema#integer">4</nlp-taxonomy:level>
        <dcterms:description xml:lang="en">Lexical Simplification is a task that involves replacing complex words in a text with simpler, more commonly used words, without changing the overall meaning of the text. This technique is often used to make text more understandable for a wider audience, including children, non-native speakers, or individuals with reading difficulties.</dcterms:description>
        <rdfs:label xml:lang="en">Lexical Simplification</rdfs:label>
    </owl:NamedIndividual>
    


    <!-- http://nlpkg.sebis.cit.tum.de/nlp-fos-hierarchy.owl#Lexical_Substitution -->

    <owl:NamedIndividual rdf:about="http://nlpkg.sebis.cit.tum.de/nlp-fos-hierarchy.owl#Lexical_Substitution">
        <rdf:type rdf:resource="http://nlpkg.sebis.cit.tum.de/nlp-fos-hierarchy.owl#Task"/>
        <rdf:type rdf:resource="http://nlpkg.sebis.cit.tum.de/nlp-taxonomy.owl#FieldOfStudy"/>
        <nlp-taxonomy:subFieldOf rdf:resource="http://nlpkg.sebis.cit.tum.de/nlp-fos-hierarchy.owl#Data_Augmentation"/>
        <nlp-taxonomy:level rdf:datatype="http://www.w3.org/2001/XMLSchema#integer">4</nlp-taxonomy:level>
        <dcterms:description xml:lang="en">Lexical Substitution refers to the process of replacing a word in a sentence with another word that maintains the same overall meaning of the sentence.</dcterms:description>
        <oboInOwl:hasSynonym xml:lang="en">Synonym Substitution</oboInOwl:hasSynonym>
        <rdfs:label xml:lang="en">Lexical Substitution</rdfs:label>
    </owl:NamedIndividual>
    


    <!-- http://nlpkg.sebis.cit.tum.de/nlp-fos-hierarchy.owl#Link_Prediction -->

    <owl:NamedIndividual rdf:about="http://nlpkg.sebis.cit.tum.de/nlp-fos-hierarchy.owl#Link_Prediction">
        <rdf:type rdf:resource="http://nlpkg.sebis.cit.tum.de/nlp-fos-hierarchy.owl#Task"/>
        <rdf:type rdf:resource="http://nlpkg.sebis.cit.tum.de/nlp-taxonomy.owl#FieldOfStudy"/>
        <nlp-taxonomy:subFieldOf rdf:resource="http://nlpkg.sebis.cit.tum.de/nlp-taxonomy.owl#Knowledge_Graph_Reasoning"/>
        <survey>https://arxiv.org/abs/2002.00819</survey>
        <nlp-taxonomy:level rdf:datatype="http://www.w3.org/2001/XMLSchema#integer">3</nlp-taxonomy:level>
        <nlp-taxonomy:level rdf:datatype="http://www.w3.org/2001/XMLSchema#integer">7</nlp-taxonomy:level>
        <dcterms:description xml:lang="en">Link Prediction is the task of inferring missing links between entities in existing knowledge bases often performed via ranking entities as possible answers to queries.</dcterms:description>
        <rdfs:label xml:lang="en">Link Prediction</rdfs:label>
    </owl:NamedIndividual>
    


    <!-- http://nlpkg.sebis.cit.tum.de/nlp-fos-hierarchy.owl#Long-Range_Transformers -->

    <owl:NamedIndividual rdf:about="http://nlpkg.sebis.cit.tum.de/nlp-fos-hierarchy.owl#Long-Range_Transformers">
        <rdf:type rdf:resource="http://nlpkg.sebis.cit.tum.de/nlp-fos-hierarchy.owl#OtherScientificField"/>
        <rdf:type rdf:resource="http://nlpkg.sebis.cit.tum.de/nlp-taxonomy.owl#FieldOfStudy"/>
        <nlp-taxonomy:subFieldOf rdf:resource="http://nlpkg.sebis.cit.tum.de/nlp-fos-hierarchy.owl#Efficient_Transformers"/>
        <survey>https://aclanthology.org/2023.eacl-main.273</survey>
        <survey>https://arxiv.org/abs/2302.14502</survey>
        <nlp-taxonomy:level rdf:datatype="http://www.w3.org/2001/XMLSchema#integer">5</nlp-taxonomy:level>
        <dcterms:description xml:lang="en">Long-Range Transformers refer to a type of transformer model that is designed to handle long sequences of data more efficiently. Traditional transformer models struggle with long sequences due to their quadratic complexity with respect to the sequence length. Long-Range Transformers address this issue by using methods such as sparse attention mechanisms or other techniques to reduce the computational complexity, enabling the model to process longer sequences of text while maintaining high performance.</dcterms:description>
        <rdfs:label xml:lang="en">Long-Range Transformers</rdfs:label>
    </owl:NamedIndividual>
    


    <!-- http://nlpkg.sebis.cit.tum.de/nlp-fos-hierarchy.owl#MVP -->

    <owl:NamedIndividual rdf:about="http://nlpkg.sebis.cit.tum.de/nlp-fos-hierarchy.owl#MVP">
        <code>https://github.com/RUCAIBox/MVP</code>
        <code>https://huggingface.co/docs/transformers/model_doc/mvp</code>
        <origin>https://aclanthology.org/2023.findings-acl.558</origin>
        <nlp-taxonomy:level rdf:datatype="http://www.w3.org/2001/XMLSchema#integer">5</nlp-taxonomy:level>
        <dcterms:description xml:lang="en">MVP (Multi-task superVised Pre-training) is a language model that is specially designed for natural language generation and can be adapted to a wide range of generation tasks, including but not limited to summarization, data-to-text generation, open-ended dialogue system, story generation, question answering, question generation, task-oriented dialogue system, commonsense generation, paraphrase generation, text style transfer, and text simplification. The model can also be adapted to natural language understanding tasks such as sequence classification and (extractive) question answering.</dcterms:description>
        <oboInOwl:hasSynonym xml:lang="en">Multi-task superVised Pre-training</oboInOwl:hasSynonym>
        <rdfs:label xml:lang="en">MVP</rdfs:label>
    </owl:NamedIndividual>
    


    <!-- http://nlpkg.sebis.cit.tum.de/nlp-fos-hierarchy.owl#Machine_Generated_Text_Detection -->

    <owl:NamedIndividual rdf:about="http://nlpkg.sebis.cit.tum.de/nlp-fos-hierarchy.owl#Machine_Generated_Text_Detection">
        <rdf:type rdf:resource="http://nlpkg.sebis.cit.tum.de/nlp-fos-hierarchy.owl#Task"/>
        <rdf:type rdf:resource="http://nlpkg.sebis.cit.tum.de/nlp-taxonomy.owl#FieldOfStudy"/>
        <nlp-taxonomy:subFieldOf rdf:resource="http://nlpkg.sebis.cit.tum.de/nlp-taxonomy.owl#Text_Classification"/>
        <survey>https://aclanthology.org/2020.coling-main.208</survey>
        <survey>https://aclanthology.org/2023.ranlp-stud.1</survey>
        <survey>https://arxiv.org/abs/2210.06336</survey>
        <survey>https://arxiv.org/abs/2210.07321</survey>
        <survey>https://arxiv.org/abs/2303.07205</survey>
        <survey>https://arxiv.org/abs/2304.04736</survey>
        <survey>https://arxiv.org/abs/2310.05030</survey>
        <survey>https://arxiv.org/abs/2310.14724</survey>
        <nlp-taxonomy:level rdf:datatype="http://www.w3.org/2001/XMLSchema#integer">3</nlp-taxonomy:level>
        <dcterms:description xml:lang="en">Machine Generated Text Detection refers to the process of identifying and distinguishing text that has been generated by an artificial intelligence or machine learning model, as opposed to text that has been written by a human.</dcterms:description>
        <oboInOwl:hasSynonym xml:lang="en">AGTD</oboInOwl:hasSynonym>
        <oboInOwl:hasSynonym xml:lang="en">AI-Generated Text Classification</oboInOwl:hasSynonym>
        <oboInOwl:hasSynonym xml:lang="en">AI-Generated Text Detection</oboInOwl:hasSynonym>
        <oboInOwl:hasSynonym xml:lang="en">AI-Generated Text Identification</oboInOwl:hasSynonym>
        <oboInOwl:hasSynonym xml:lang="en">Machine Generated Text Classification</oboInOwl:hasSynonym>
        <oboInOwl:hasSynonym xml:lang="en">Machine Generated Text Identification</oboInOwl:hasSynonym>
        <oboInOwl:hasSynonym xml:lang="en">Synthetic Text Classification</oboInOwl:hasSynonym>
        <oboInOwl:hasSynonym xml:lang="en">Synthetic Text Detection</oboInOwl:hasSynonym>
        <oboInOwl:hasSynonym xml:lang="en">Synthetic Text Identification</oboInOwl:hasSynonym>
        <rdfs:label xml:lang="en">Machine Generated Text Detection</rdfs:label>
    </owl:NamedIndividual>
    


    <!-- http://nlpkg.sebis.cit.tum.de/nlp-fos-hierarchy.owl#Math_Word_Problem_Solving -->

    <owl:NamedIndividual rdf:about="http://nlpkg.sebis.cit.tum.de/nlp-fos-hierarchy.owl#Math_Word_Problem_Solving">
        <rdf:type rdf:resource="http://nlpkg.sebis.cit.tum.de/nlp-fos-hierarchy.owl#Task"/>
        <rdf:type rdf:resource="http://nlpkg.sebis.cit.tum.de/nlp-taxonomy.owl#FieldOfStudy"/>
        <nlp-taxonomy:subFieldOf rdf:resource="http://nlpkg.sebis.cit.tum.de/nlp-taxonomy.owl#Numerical_Reasoning"/>
        <survey>https://aclanthology.org/2021.naacl-main.168</survey>
        <survey>https://arxiv.org/abs/1808.07290</survey>
        <survey>https://arxiv.org/abs/2205.15683</survey>
        <nlp-taxonomy:level rdf:datatype="http://www.w3.org/2001/XMLSchema#integer">3</nlp-taxonomy:level>
        <dcterms:description xml:lang="en">Math Word Problem Solving refers to the ability of an AI system to understand and solve mathematical problems presented in natural language. This involves the system&apos;s ability to accurately interpret the problem, identify the mathematical operations required, and perform those operations to produce a correct answer. This is a complex task as it requires a deep understanding of language semantics, the ability to handle ambiguity, and proficiency in mathematical reasoning.</dcterms:description>
        <oboInOwl:hasSynonym xml:lang="en">Arithmetic Word Problem Solving</oboInOwl:hasSynonym>
        <oboInOwl:hasSynonym xml:lang="en">MWP Solving</oboInOwl:hasSynonym>
        <oboInOwl:hasSynonym xml:lang="en">Word Problem Solving</oboInOwl:hasSynonym>
        <rdfs:label xml:lang="en">Math Word Problem Solving</rdfs:label>
    </owl:NamedIndividual>
    


    <!-- http://nlpkg.sebis.cit.tum.de/nlp-fos-hierarchy.owl#Media_Bias -->

    <owl:NamedIndividual rdf:about="http://nlpkg.sebis.cit.tum.de/nlp-fos-hierarchy.owl#Media_Bias">
        <rdf:type rdf:resource="http://nlpkg.sebis.cit.tum.de/nlp-fos-hierarchy.owl#OtherScientificField"/>
        <rdf:type rdf:resource="http://nlpkg.sebis.cit.tum.de/nlp-taxonomy.owl#FieldOfStudy"/>
        <nlp-taxonomy:subFieldOf rdf:resource="http://nlpkg.sebis.cit.tum.de/nlp-fos-hierarchy.owl#Biases_&amp;_Fairness_in_NLP"/>
        <survey>https://arxiv.org/abs/2103.12506</survey>
        <survey>https://arxiv.org/abs/2309.08069</survey>
        <nlp-taxonomy:level rdf:datatype="http://www.w3.org/2001/XMLSchema#integer">4</nlp-taxonomy:level>
        <dcterms:description xml:lang="en">Media Bias refers to the perceived or actual bias of journalists and news producers within the mass media, in the selection of events and stories that are reported, and how they are covered. This bias can be in terms of political, economic, racial, cultural, or ideological perspectives. It can manifest in the framing of narratives, omission of certain facts or events, and disproportionate coverage of certain topics.</dcterms:description>
        <rdfs:label xml:lang="en">Media Bias</rdfs:label>
    </owl:NamedIndividual>
    


    <!-- http://nlpkg.sebis.cit.tum.de/nlp-fos-hierarchy.owl#Membership_Inference_Attack -->

    <owl:NamedIndividual rdf:about="http://nlpkg.sebis.cit.tum.de/nlp-fos-hierarchy.owl#Membership_Inference_Attack">
        <rdf:type rdf:resource="http://nlpkg.sebis.cit.tum.de/nlp-fos-hierarchy.owl#Task"/>
        <rdf:type rdf:resource="http://nlpkg.sebis.cit.tum.de/nlp-taxonomy.owl#FieldOfStudy"/>
        <nlp-taxonomy:subFieldOf rdf:resource="http://nlpkg.sebis.cit.tum.de/nlp-fos-hierarchy.owl#Inference_Attacks"/>
        <nlp-taxonomy:level rdf:datatype="http://www.w3.org/2001/XMLSchema#integer">4</nlp-taxonomy:level>
        <dcterms:description xml:lang="en">Membership Inference Attacks (MIAs) aim to predict whether a data sample was present in the training data of a machine learning model or not, and are widely used for assessing the privacy risks of language models.</dcterms:description>
        <oboInOwl:hasSynonym xml:lang="en">MIA</oboInOwl:hasSynonym>
        <rdfs:label xml:lang="en">Membership Inference Attack</rdfs:label>
    </owl:NamedIndividual>
    


    <!-- http://nlpkg.sebis.cit.tum.de/nlp-fos-hierarchy.owl#Meme_Classification -->

    <owl:NamedIndividual rdf:about="http://nlpkg.sebis.cit.tum.de/nlp-fos-hierarchy.owl#Meme_Classification">
        <rdf:type rdf:resource="http://nlpkg.sebis.cit.tum.de/nlp-fos-hierarchy.owl#Task"/>
        <rdf:type rdf:resource="http://nlpkg.sebis.cit.tum.de/nlp-taxonomy.owl#FieldOfStudy"/>
        <nlp-taxonomy:subFieldOf rdf:resource="http://nlpkg.sebis.cit.tum.de/nlp-taxonomy.owl#Visual_Data_In_NLP"/>
        <survey>https://arxiv.org/abs/2009.08395</survey>
        <nlp-taxonomy:level rdf:datatype="http://www.w3.org/2001/XMLSchema#integer">3</nlp-taxonomy:level>
        <dcterms:description xml:lang="en">Meme Classification refers to the task of classifying internet memes. Memes are graphics and text overlapped so that together they present concepts that become dubious if one of them is absent. It is spread mostly on social media platforms, in the form of jokes, sarcasm, motivating, etc.</dcterms:description>
        <rdfs:label xml:lang="en">Meme Classification</rdfs:label>
    </owl:NamedIndividual>
    


    <!-- http://nlpkg.sebis.cit.tum.de/nlp-fos-hierarchy.owl#Meta-Learning -->

    <owl:NamedIndividual rdf:about="http://nlpkg.sebis.cit.tum.de/nlp-fos-hierarchy.owl#Meta-Learning">
        <rdf:type rdf:resource="http://nlpkg.sebis.cit.tum.de/nlp-fos-hierarchy.owl#Task"/>
        <rdf:type rdf:resource="http://nlpkg.sebis.cit.tum.de/nlp-taxonomy.owl#FieldOfStudy"/>
        <usedFor rdf:resource="http://nlpkg.sebis.cit.tum.de/nlp-fos-hierarchy.owl#Domain_Adaptation"/>
        <usedFor rdf:resource="http://nlpkg.sebis.cit.tum.de/nlp-fos-hierarchy.owl#Few-shot_Learning"/>
        <usedFor rdf:resource="http://nlpkg.sebis.cit.tum.de/nlp-fos-hierarchy.owl#Multi-task_Learning"/>
        <usedFor rdf:resource="http://nlpkg.sebis.cit.tum.de/nlp-taxonomy.owl#Cross-Lingual_Transfer"/>
        <usedFor rdf:resource="http://nlpkg.sebis.cit.tum.de/nlp-taxonomy.owl#Robustness_In_NLP"/>
        <nlp-taxonomy:subFieldOf rdf:resource="http://nlpkg.sebis.cit.tum.de/nlp-taxonomy.owl#Language_Models"/>
        <nlp-taxonomy:superFieldOf rdf:resource="http://nlpkg.sebis.cit.tum.de/nlp-fos-hierarchy.owl#Learn_to_Knowledge_Distillation"/>
        <nlp-taxonomy:superFieldOf rdf:resource="http://nlpkg.sebis.cit.tum.de/nlp-fos-hierarchy.owl#Learn_to_Lifelong_Learning"/>
        <nlp-taxonomy:superFieldOf rdf:resource="http://nlpkg.sebis.cit.tum.de/nlp-fos-hierarchy.owl#Learning_to_Compare"/>
        <nlp-taxonomy:superFieldOf rdf:resource="http://nlpkg.sebis.cit.tum.de/nlp-fos-hierarchy.owl#Learning_to_Initialize"/>
        <nlp-taxonomy:superFieldOf rdf:resource="http://nlpkg.sebis.cit.tum.de/nlp-fos-hierarchy.owl#Meta-Learning_for_Data_Selection"/>
        <nlp-taxonomy:superFieldOf rdf:resource="http://nlpkg.sebis.cit.tum.de/nlp-fos-hierarchy.owl#Neural_Network_Architecture_Search"/>
        <survey>https://aclanthology.org/2022.naacl-main.49</survey>
        <survey>https://arxiv.org/abs/2007.09604</survey>
        <nlp-taxonomy:level rdf:datatype="http://www.w3.org/2001/XMLSchema#integer">3</nlp-taxonomy:level>
        <dcterms:description xml:lang="en">Meta-Learning in machine learning refers to the concept where the algorithm learns from the output of other machine learning algorithms. It typically refers to ensemble learning algorithms like stacking that learn how to combine the predictions from ensemble members. Meta-learning also refers to algorithms that learn how to learn across a suite of related prediction tasks, referred to as multi-task learning. It&apos;s essentially &quot;learning how to learn&quot;. Meta-learning allows faster fine-tuning, converges to better performance, yields more generalizable models, and it achieves great results in few-shot settings.</dcterms:description>
        <oboInOwl:hasSynonym xml:lang="en">Learning to Learn</oboInOwl:hasSynonym>
        <oboInOwl:hasSynonym xml:lang="en">Meta Learning</oboInOwl:hasSynonym>
        <rdfs:label xml:lang="en">Meta-Learning</rdfs:label>
    </owl:NamedIndividual>
    


    <!-- http://nlpkg.sebis.cit.tum.de/nlp-fos-hierarchy.owl#Meta-Learning_for_Data_Selection -->

    <owl:NamedIndividual rdf:about="http://nlpkg.sebis.cit.tum.de/nlp-fos-hierarchy.owl#Meta-Learning_for_Data_Selection">
        <rdf:type rdf:resource="http://nlpkg.sebis.cit.tum.de/nlp-fos-hierarchy.owl#Task"/>
        <rdf:type rdf:resource="http://nlpkg.sebis.cit.tum.de/nlp-taxonomy.owl#FieldOfStudy"/>
        <nlp-taxonomy:subFieldOf rdf:resource="http://nlpkg.sebis.cit.tum.de/nlp-fos-hierarchy.owl#Meta-Learning"/>
        <nlp-taxonomy:level rdf:datatype="http://www.w3.org/2001/XMLSchema#integer">4</nlp-taxonomy:level>
        <dcterms:description xml:lang="en">Meta-Learning for Data Selection can be used to determine which data samples are most useful for training a model. This can be particularly when the amount of available data can be vast and varied. The goal is to optimize the learning process by selecting the most relevant and useful data for the task at hand.</dcterms:description>
        <rdfs:label xml:lang="en">Meta-Learning for Data Selection</rdfs:label>
    </owl:NamedIndividual>
    


    <!-- http://nlpkg.sebis.cit.tum.de/nlp-fos-hierarchy.owl#Metaphor_Detection -->

    <owl:NamedIndividual rdf:about="http://nlpkg.sebis.cit.tum.de/nlp-fos-hierarchy.owl#Metaphor_Detection">
        <rdf:type rdf:resource="http://nlpkg.sebis.cit.tum.de/nlp-fos-hierarchy.owl#Task"/>
        <rdf:type rdf:resource="http://nlpkg.sebis.cit.tum.de/nlp-taxonomy.owl#FieldOfStudy"/>
        <nlp-taxonomy:subFieldOf rdf:resource="http://nlpkg.sebis.cit.tum.de/nlp-taxonomy.owl#Stylistic_Analysis"/>
        <nlp-taxonomy:subFieldOf rdf:resource="http://nlpkg.sebis.cit.tum.de/nlp-taxonomy.owl#Text_Classification"/>
        <survey>https://arxiv.org/abs/2308.04306</survey>
        <nlp-taxonomy:level rdf:datatype="http://www.w3.org/2001/XMLSchema#integer">3</nlp-taxonomy:level>
        <dcterms:description xml:lang="en">Metaphor Detection refers to the ability of a machine learning model or algorithm to identify and understand metaphors in a given text. Metaphors are figures of speech that describe an object or action in a way that isn&apos;t literally true, but helps explain an idea or make a comparison. Detecting and interpreting them correctly is a complex task as it requires a deep understanding of the context and the nuances of the language.</dcterms:description>
        <oboInOwl:hasSynonym xml:lang="en">Metaphor Classification</oboInOwl:hasSynonym>
        <oboInOwl:hasSynonym xml:lang="en">Metaphor Identification</oboInOwl:hasSynonym>
        <oboInOwl:hasSynonym xml:lang="en">Metaphor Recognition</oboInOwl:hasSynonym>
        <rdfs:label xml:lang="en">Metaphor Detection</rdfs:label>
    </owl:NamedIndividual>
    


    <!-- http://nlpkg.sebis.cit.tum.de/nlp-fos-hierarchy.owl#Misinformation_Detection -->

    <owl:NamedIndividual rdf:about="http://nlpkg.sebis.cit.tum.de/nlp-fos-hierarchy.owl#Misinformation_Detection">
        <rdf:type rdf:resource="http://nlpkg.sebis.cit.tum.de/nlp-fos-hierarchy.owl#Task"/>
        <rdf:type rdf:resource="http://nlpkg.sebis.cit.tum.de/nlp-taxonomy.owl#FieldOfStudy"/>
        <uses rdf:resource="http://nlpkg.sebis.cit.tum.de/nlp-taxonomy.owl#Fact_&amp;_Claim_Verification"/>
        <nlp-taxonomy:subFieldOf rdf:resource="http://nlpkg.sebis.cit.tum.de/nlp-taxonomy.owl#Ethical_NLP"/>
        <nlp-taxonomy:subFieldOf rdf:resource="http://nlpkg.sebis.cit.tum.de/nlp-taxonomy.owl#Text_Classification"/>
        <nlp-taxonomy:superFieldOf rdf:resource="http://nlpkg.sebis.cit.tum.de/nlp-fos-hierarchy.owl#Fake_News_Detection"/>
        <survey>https://aclanthology.org/2022.coling-1.576</survey>
        <survey>https://aclanthology.org/2022.findings-naacl.94</survey>
        <survey>https://arxiv.org/abs/1910.12073</survey>
        <nlp-taxonomy:level rdf:datatype="http://www.w3.org/2001/XMLSchema#integer">3</nlp-taxonomy:level>
        <dcterms:description xml:lang="en">Misinformation Detection refers to the application of NLP techniques to identify and filter out false or misleading information. This can involve analyzing text data to determine its truthfulness, reliability, and relevance. It&apos;s particularly important in areas like social media, news, and online content where misinformation can spread quickly.</dcterms:description>
        <oboInOwl:hasSynonym xml:lang="en">Disinformation Classification</oboInOwl:hasSynonym>
        <oboInOwl:hasSynonym xml:lang="en">Disinformation Detection</oboInOwl:hasSynonym>
        <oboInOwl:hasSynonym xml:lang="en">Disinformation Identification</oboInOwl:hasSynonym>
        <oboInOwl:hasSynonym xml:lang="en">Misinformation Classification</oboInOwl:hasSynonym>
        <oboInOwl:hasSynonym xml:lang="en">Misinformation Identification</oboInOwl:hasSynonym>
        <rdfs:label xml:lang="en">Misinformation Detection</rdfs:label>
    </owl:NamedIndividual>
    


    <!-- http://nlpkg.sebis.cit.tum.de/nlp-fos-hierarchy.owl#Mixture_of_Experts -->

    <owl:NamedIndividual rdf:about="http://nlpkg.sebis.cit.tum.de/nlp-fos-hierarchy.owl#Mixture_of_Experts">
        <rdf:type rdf:resource="http://nlpkg.sebis.cit.tum.de/nlp-fos-hierarchy.owl#Method"/>
        <rdf:type rdf:resource="http://nlpkg.sebis.cit.tum.de/nlp-taxonomy.owl#FieldOfStudy"/>
        <nlp-taxonomy:subFieldOf rdf:resource="http://nlpkg.sebis.cit.tum.de/nlp-fos-hierarchy.owl#Multi-Agent_Systems_&amp;_Multi-Model_Language_Models"/>
        <survey>https://arxiv.org/abs/2208.02813</survey>
        <nlp-taxonomy:level rdf:datatype="http://www.w3.org/2001/XMLSchema#integer">4</nlp-taxonomy:level>
        <dcterms:description xml:lang="en">Mixture of Experts (MoE) is a machine learning technique that involves training multiple models, each specializing in a different aspect of the data (the &quot;experts&quot;), and then combining their outputs. The idea is to leverage the strengths of each expert on the parts of the data where they perform best. This approach can improve overall performance and accuracy in complex NLP tasks.</dcterms:description>
        <oboInOwl:hasSynonym xml:lang="en">MoE</oboInOwl:hasSynonym>
        <rdfs:label xml:lang="en">Mixture of Experts</rdfs:label>
    </owl:NamedIndividual>
    


    <!-- http://nlpkg.sebis.cit.tum.de/nlp-fos-hierarchy.owl#Model-Agnostic_Meta-Learning -->

    <owl:NamedIndividual rdf:about="http://nlpkg.sebis.cit.tum.de/nlp-fos-hierarchy.owl#Model-Agnostic_Meta-Learning">
        <rdf:type rdf:resource="http://nlpkg.sebis.cit.tum.de/nlp-fos-hierarchy.owl#Task"/>
        <rdf:type rdf:resource="http://nlpkg.sebis.cit.tum.de/nlp-taxonomy.owl#FieldOfStudy"/>
        <nlp-taxonomy:subFieldOf rdf:resource="http://nlpkg.sebis.cit.tum.de/nlp-fos-hierarchy.owl#Learning_to_Initialize"/>
        <nlp-taxonomy:level rdf:datatype="http://www.w3.org/2001/XMLSchema#integer">5</nlp-taxonomy:level>
        <dcterms:description xml:lang="en">Model-Agnostic Meta-Learning (MAML) is a learning framework that aims to train a model on a variety of learning tasks, enabling it to quickly adapt to new tasks using a small number of training samples. MAML is &quot;model-agnostic&quot; in that it is compatible with any model trained with gradient descent and applicable to a variety of different learning tasks, including classification, regression, and reinforcement learning.</dcterms:description>
        <oboInOwl:hasSynonym xml:lang="en">MAML</oboInOwl:hasSynonym>
        <rdfs:label xml:lang="en">Model-Agnostic Meta-Learning</rdfs:label>
    </owl:NamedIndividual>
    


    <!-- http://nlpkg.sebis.cit.tum.de/nlp-fos-hierarchy.owl#Model_Inversion_Attack -->

    <owl:NamedIndividual rdf:about="http://nlpkg.sebis.cit.tum.de/nlp-fos-hierarchy.owl#Model_Inversion_Attack">
        <rdf:type rdf:resource="http://nlpkg.sebis.cit.tum.de/nlp-fos-hierarchy.owl#Task"/>
        <rdf:type rdf:resource="http://nlpkg.sebis.cit.tum.de/nlp-taxonomy.owl#FieldOfStudy"/>
        <nlp-taxonomy:subFieldOf rdf:resource="http://nlpkg.sebis.cit.tum.de/nlp-fos-hierarchy.owl#Inference_Attacks"/>
        <nlp-taxonomy:level rdf:datatype="http://www.w3.org/2001/XMLSchema#integer">4</nlp-taxonomy:level>
        <dcterms:description xml:lang="en">Model Inversion Attacks refer to a type of cyber attack where an attacker tries to extract sensitive information from a machine learning model. The attacker uses the outputs of the model and possibly some additional information to reconstruct the original input data or some properties of it. This can lead to privacy breaches, especially when the model has been trained on sensitive data like personal emails or confidential documents.</dcterms:description>
        <oboInOwl:hasSynonym xml:lang="en">Inversion Attack</oboInOwl:hasSynonym>
        <rdfs:label xml:lang="en">Model Inversion Attack</rdfs:label>
    </owl:NamedIndividual>
    


    <!-- http://nlpkg.sebis.cit.tum.de/nlp-fos-hierarchy.owl#Model_Stealing_Attack -->

    <owl:NamedIndividual rdf:about="http://nlpkg.sebis.cit.tum.de/nlp-fos-hierarchy.owl#Model_Stealing_Attack">
        <rdf:type rdf:resource="http://nlpkg.sebis.cit.tum.de/nlp-fos-hierarchy.owl#Task"/>
        <rdf:type rdf:resource="http://nlpkg.sebis.cit.tum.de/nlp-taxonomy.owl#FieldOfStudy"/>
        <nlp-taxonomy:subFieldOf rdf:resource="http://nlpkg.sebis.cit.tum.de/nlp-fos-hierarchy.owl#Inference_Attacks"/>
        <nlp-taxonomy:level rdf:datatype="http://www.w3.org/2001/XMLSchema#integer">4</nlp-taxonomy:level>
        <dcterms:description xml:lang="en">Model Stealing Attack refers to a type of cyber attack where an attacker aims to duplicate the functionality of a machine learning model without having access to the original model&apos;s parameters or training data. The attacker typically uses a series of queries to the model and uses the responses to train a replica. This can lead to intellectual property theft and potential misuse of the model.</dcterms:description>
        <oboInOwl:hasSynonym xml:lang="en">Stealing Attack</oboInOwl:hasSynonym>
        <rdfs:label xml:lang="en">Model Stealing Attack</rdfs:label>
    </owl:NamedIndividual>
    


    <!-- http://nlpkg.sebis.cit.tum.de/nlp-fos-hierarchy.owl#Morphemes -->

    <owl:NamedIndividual rdf:about="http://nlpkg.sebis.cit.tum.de/nlp-fos-hierarchy.owl#Morphemes">
        <rdf:type rdf:resource="http://nlpkg.sebis.cit.tum.de/nlp-fos-hierarchy.owl#OtherScientificField"/>
        <rdf:type rdf:resource="http://nlpkg.sebis.cit.tum.de/nlp-taxonomy.owl#FieldOfStudy"/>
        <nlp-taxonomy:subFieldOf rdf:resource="http://nlpkg.sebis.cit.tum.de/nlp-fos-hierarchy.owl#Morphological_Segmentation"/>
        <nlp-taxonomy:level rdf:datatype="http://www.w3.org/2001/XMLSchema#integer">4</nlp-taxonomy:level>
        <dcterms:description xml:lang="en">Morphemes refer to the smallest meaningful units of a language. They are the building blocks of words, which can&apos;t be further divided without losing or changing their meaning. For example, the word &quot;unhappiness&quot; contains three morphemes: &quot;un-&quot;, &quot;happy&quot;, and &quot;-ness&quot;.</dcterms:description>
        <rdfs:label xml:lang="en">Morphemes</rdfs:label>
    </owl:NamedIndividual>
    


    <!-- http://nlpkg.sebis.cit.tum.de/nlp-fos-hierarchy.owl#Morphological_Inflection -->

    <owl:NamedIndividual rdf:about="http://nlpkg.sebis.cit.tum.de/nlp-fos-hierarchy.owl#Morphological_Inflection">
        <rdf:type rdf:resource="http://nlpkg.sebis.cit.tum.de/nlp-fos-hierarchy.owl#Task"/>
        <rdf:type rdf:resource="http://nlpkg.sebis.cit.tum.de/nlp-taxonomy.owl#FieldOfStudy"/>
        <nlp-taxonomy:subFieldOf rdf:resource="http://nlpkg.sebis.cit.tum.de/nlp-taxonomy.owl#Morphology"/>
        <nlp-taxonomy:level rdf:datatype="http://www.w3.org/2001/XMLSchema#integer">3</nlp-taxonomy:level>
        <dcterms:description xml:lang="en">Morphological Inflection refers to the process of using rules and algorithms to generate different forms of a word. This concept is based on the linguistic phenomenon where the form of a word changes to express different grammatical categories such as tense, case, voice, aspect, person, number, gender, and mood. For example, the verb &apos;run&apos; can be inflected to &apos;runs&apos;, &apos;running&apos;, or &apos;ran&apos; to indicate different tenses.</dcterms:description>
        <rdfs:label xml:lang="en">Morphological Inflection</rdfs:label>
    </owl:NamedIndividual>
    


    <!-- http://nlpkg.sebis.cit.tum.de/nlp-fos-hierarchy.owl#Morphological_Segmentation -->

    <owl:NamedIndividual rdf:about="http://nlpkg.sebis.cit.tum.de/nlp-fos-hierarchy.owl#Morphological_Segmentation">
        <rdf:type rdf:resource="http://nlpkg.sebis.cit.tum.de/nlp-fos-hierarchy.owl#Task"/>
        <rdf:type rdf:resource="http://nlpkg.sebis.cit.tum.de/nlp-taxonomy.owl#FieldOfStudy"/>
        <nlp-taxonomy:subFieldOf rdf:resource="http://nlpkg.sebis.cit.tum.de/nlp-taxonomy.owl#Morphology"/>
        <nlp-taxonomy:subFieldOf rdf:resource="http://nlpkg.sebis.cit.tum.de/nlp-taxonomy.owl#Text_Segmentation"/>
        <nlp-taxonomy:superFieldOf rdf:resource="http://nlpkg.sebis.cit.tum.de/nlp-fos-hierarchy.owl#Morphemes"/>
        <nlp-taxonomy:level rdf:datatype="http://www.w3.org/2001/XMLSchema#integer">3</nlp-taxonomy:level>
        <dcterms:description xml:lang="en">Morphological Segmentation refers to the process of dividing words into individual units called morphemes. Morphemes are the smallest meaningful units in a language, which include root words, prefixes, and suffixes.</dcterms:description>
        <rdfs:label xml:lang="en">Morphological Segmentation</rdfs:label>
    </owl:NamedIndividual>
    


    <!-- http://nlpkg.sebis.cit.tum.de/nlp-fos-hierarchy.owl#Multi-Hop_Reasoning -->

    <owl:NamedIndividual rdf:about="http://nlpkg.sebis.cit.tum.de/nlp-fos-hierarchy.owl#Multi-Hop_Reasoning">
        <rdf:type rdf:resource="http://nlpkg.sebis.cit.tum.de/nlp-fos-hierarchy.owl#Task"/>
        <rdf:type rdf:resource="http://nlpkg.sebis.cit.tum.de/nlp-taxonomy.owl#FieldOfStudy"/>
        <nlp-taxonomy:subFieldOf rdf:resource="http://nlpkg.sebis.cit.tum.de/nlp-fos-hierarchy.owl#Knowledge_Graph_Question_Answering"/>
        <nlp-taxonomy:subFieldOf rdf:resource="http://nlpkg.sebis.cit.tum.de/nlp-taxonomy.owl#Reasoning"/>
        <survey>https://arxiv.org/abs/2204.09140</survey>
        <survey>https://arxiv.org/abs/2212.04070</survey>
        <survey>https://arxiv.org/abs/2212.04072</survey>
        <nlp-taxonomy:level rdf:datatype="http://www.w3.org/2001/XMLSchema#integer">2</nlp-taxonomy:level>
        <nlp-taxonomy:level rdf:datatype="http://www.w3.org/2001/XMLSchema#integer">5</nlp-taxonomy:level>
        <nlp-taxonomy:level rdf:datatype="http://www.w3.org/2001/XMLSchema#integer">6</nlp-taxonomy:level>
        <nlp-taxonomy:level rdf:datatype="http://www.w3.org/2001/XMLSchema#integer">7</nlp-taxonomy:level>
        <dcterms:description xml:lang="en">Multi-Hop Reasoning is a concept where the system uses a knowledge graph or multiple text passages to answer complex queries by making multiple inferential leaps (hops). It involves traversing through the graph or text passages and making connections between different evidences to derive new information or answer a query.</dcterms:description>
        <oboInOwl:hasSynonym xml:lang="en">Multi-Hop KG Reasoning</oboInOwl:hasSynonym>
        <oboInOwl:hasSynonym xml:lang="en">Multi-Hop Knowledge Graph Reasoning</oboInOwl:hasSynonym>
        <oboInOwl:hasSynonym xml:lang="en">Multi-Hop MRC</oboInOwl:hasSynonym>
        <oboInOwl:hasSynonym xml:lang="en">Multi-Hop Machine Reading Comprehension</oboInOwl:hasSynonym>
        <oboInOwl:hasSynonym xml:lang="en">Multi-Hop QA</oboInOwl:hasSynonym>
        <oboInOwl:hasSynonym xml:lang="en">Multi-Hop Question Answering</oboInOwl:hasSynonym>
        <rdfs:label xml:lang="en">Multi-Hop Reasoning</rdfs:label>
    </owl:NamedIndividual>
    


    <!-- http://nlpkg.sebis.cit.tum.de/nlp-fos-hierarchy.owl#Multi-class_Classification -->

    <owl:NamedIndividual rdf:about="http://nlpkg.sebis.cit.tum.de/nlp-fos-hierarchy.owl#Multi-class_Classification">
        <rdf:type rdf:resource="http://nlpkg.sebis.cit.tum.de/nlp-fos-hierarchy.owl#Task"/>
        <rdf:type rdf:resource="http://nlpkg.sebis.cit.tum.de/nlp-taxonomy.owl#FieldOfStudy"/>
        <nlp-taxonomy:subFieldOf rdf:resource="http://nlpkg.sebis.cit.tum.de/nlp-taxonomy.owl#Text_Classification"/>
        <nlp-taxonomy:level rdf:datatype="http://www.w3.org/2001/XMLSchema#integer">3</nlp-taxonomy:level>
        <dcterms:description xml:lang="en">Multi-class Classification is a type of machine learning algorithm that categorizes instances into one of three or more classes. It is an extension of binary classification, which only categorizes instances into one of two classes. The goal of multi-class classification is to assign an instance to one of several different classes.</dcterms:description>
        <rdfs:label xml:lang="en">Multi-class Classification</rdfs:label>
    </owl:NamedIndividual>
    


    <!-- http://nlpkg.sebis.cit.tum.de/nlp-fos-hierarchy.owl#Multi-label_Classification -->

    <owl:NamedIndividual rdf:about="http://nlpkg.sebis.cit.tum.de/nlp-fos-hierarchy.owl#Multi-label_Classification">
        <rdf:type rdf:resource="http://nlpkg.sebis.cit.tum.de/nlp-fos-hierarchy.owl#Task"/>
        <rdf:type rdf:resource="http://nlpkg.sebis.cit.tum.de/nlp-taxonomy.owl#FieldOfStudy"/>
        <nlp-taxonomy:subFieldOf rdf:resource="http://nlpkg.sebis.cit.tum.de/nlp-taxonomy.owl#Text_Classification"/>
        <nlp-taxonomy:level rdf:datatype="http://www.w3.org/2001/XMLSchema#integer">3</nlp-taxonomy:level>
        <dcterms:description xml:lang="en">Multi-label classification is a type of machine learning problem where an instance/sample can be classified into multiple classes or labels. In other words, it is not limited to assigning a single label to each instance, but allows for one or more labels to be assigned. This is different from multi-class classification, where each instance is assigned only one label from multiple classes.</dcterms:description>
        <rdfs:label xml:lang="en">Multi-label Classification</rdfs:label>
    </owl:NamedIndividual>
    


    <!-- http://nlpkg.sebis.cit.tum.de/nlp-fos-hierarchy.owl#Multi-task_Learning -->

    <owl:NamedIndividual rdf:about="http://nlpkg.sebis.cit.tum.de/nlp-fos-hierarchy.owl#Multi-task_Learning">
        <rdf:type rdf:resource="http://nlpkg.sebis.cit.tum.de/nlp-fos-hierarchy.owl#Task"/>
        <rdf:type rdf:resource="http://nlpkg.sebis.cit.tum.de/nlp-taxonomy.owl#FieldOfStudy"/>
        <uses rdf:resource="http://nlpkg.sebis.cit.tum.de/nlp-fos-hierarchy.owl#Instruction_Learning"/>
        <uses rdf:resource="http://nlpkg.sebis.cit.tum.de/nlp-fos-hierarchy.owl#Meta-Learning"/>
        <nlp-taxonomy:subFieldOf rdf:resource="http://nlpkg.sebis.cit.tum.de/nlp-taxonomy.owl#Language_Models"/>
        <nlp-taxonomy:subFieldOf rdf:resource="http://nlpkg.sebis.cit.tum.de/nlp-taxonomy.owl#Low-Resource_NLP"/>
        <nlp-taxonomy:subFieldOf rdf:resource="http://nlpkg.sebis.cit.tum.de/nlp-taxonomy.owl#Green_&amp;_Sustainable_NLP"/>
        <survey>https://aclanthology.org/2023.eacl-main.66</survey>
        <survey>https://arxiv.org/abs/2109.09138</survey>
        <survey>https://arxiv.org/abs/2308.08234</survey>
        <nlp-taxonomy:level rdf:datatype="http://www.w3.org/2001/XMLSchema#integer">3</nlp-taxonomy:level>
        <dcterms:description xml:lang="en">Multi-task Learning (MTL) is a learning paradigm where multiple learning tasks are solved at the same time, while exploiting commonalities and differences across tasks. This approach aims to improve the performance of individual tasks by leveraging the shared information among them. It&apos;s particularly useful in NLP where datasets can be scarce or imbalanced, as it allows models to learn representations across different tasks, enhancing generalization and robustness.</dcterms:description>
        <oboInOwl:hasSynonym xml:lang="en">MTL</oboInOwl:hasSynonym>
        <rdfs:label xml:lang="en">Multi-task Learning</rdfs:label>
    </owl:NamedIndividual>
    


    <!-- http://nlpkg.sebis.cit.tum.de/nlp-fos-hierarchy.owl#Multilingual_Language_Models -->

    <owl:NamedIndividual rdf:about="http://nlpkg.sebis.cit.tum.de/nlp-fos-hierarchy.owl#Multilingual_Language_Models">
        <rdf:type rdf:resource="http://nlpkg.sebis.cit.tum.de/nlp-fos-hierarchy.owl#OtherScientificField"/>
        <rdf:type rdf:resource="http://nlpkg.sebis.cit.tum.de/nlp-taxonomy.owl#FieldOfStudy"/>
        <usedFor rdf:resource="http://nlpkg.sebis.cit.tum.de/nlp-fos-hierarchy.owl#Neural_Machine_Translation"/>
        <usedFor rdf:resource="http://nlpkg.sebis.cit.tum.de/nlp-taxonomy.owl#Cross-Lingual_Transfer"/>
        <nlp-taxonomy:subFieldOf rdf:resource="http://nlpkg.sebis.cit.tum.de/nlp-taxonomy.owl#Language_Models"/>
        <nlp-taxonomy:subFieldOf rdf:resource="http://nlpkg.sebis.cit.tum.de/nlp-taxonomy.owl#Multilinguality"/>
        <survey>https://aclanthology.org/2023.acl-long.323</survey>
        <survey>https://aclanthology.org/2023.findings-acl.439</survey>
        <survey>https://arxiv.org/abs/2110.02052</survey>
        <nlp-taxonomy:level rdf:datatype="http://www.w3.org/2001/XMLSchema#integer">2</nlp-taxonomy:level>
        <nlp-taxonomy:level rdf:datatype="http://www.w3.org/2001/XMLSchema#integer">3</nlp-taxonomy:level>
        <dcterms:description xml:lang="en">Multilingual Language Models are models that are designed to understand, interpret, generate, or translate multiple languages. These models are trained on text data from several languages, enabling them to perform tasks across different languages.</dcterms:description>
        <rdfs:label xml:lang="en">Multilingual Language Models</rdfs:label>
    </owl:NamedIndividual>
    


    <!-- http://nlpkg.sebis.cit.tum.de/nlp-fos-hierarchy.owl#Multimodal_Language_Models -->

    <owl:NamedIndividual rdf:about="http://nlpkg.sebis.cit.tum.de/nlp-fos-hierarchy.owl#Multimodal_Language_Models">
        <rdf:type rdf:resource="http://nlpkg.sebis.cit.tum.de/nlp-fos-hierarchy.owl#OtherScientificField"/>
        <rdf:type rdf:resource="http://nlpkg.sebis.cit.tum.de/nlp-taxonomy.owl#FieldOfStudy"/>
        <nlp-taxonomy:subFieldOf rdf:resource="http://nlpkg.sebis.cit.tum.de/nlp-taxonomy.owl#Language_Models"/>
        <nlp-taxonomy:subFieldOf rdf:resource="http://nlpkg.sebis.cit.tum.de/nlp-taxonomy.owl#Multimodality"/>
        <nlp-taxonomy:superFieldOf rdf:resource="http://nlpkg.sebis.cit.tum.de/nlp-fos-hierarchy.owl#Code-specific_Language_Models"/>
        <nlp-taxonomy:superFieldOf rdf:resource="http://nlpkg.sebis.cit.tum.de/nlp-fos-hierarchy.owl#Vision-specific_Language_Models"/>
        <nlp-taxonomy:superFieldOf rdf:resource="http://nlpkg.sebis.cit.tum.de/nlp-fos-hierarchy.owl#Speech_&amp;_Audio-specific_Language_Models"/>
        <survey>https://arxiv.org/abs/2104.13225</survey>
        <survey>https://arxiv.org/abs/2206.06488</survey>
        <survey>https://arxiv.org/abs/2302.10035</survey>
        <survey>https://arxiv.org/abs/2306.13549</survey>
        <survey>https://arxiv.org/abs/2309.10020</survey>
        <nlp-taxonomy:level rdf:datatype="http://www.w3.org/2001/XMLSchema#integer">2</nlp-taxonomy:level>
        <nlp-taxonomy:level rdf:datatype="http://www.w3.org/2001/XMLSchema#integer">3</nlp-taxonomy:level>
        <dcterms:description xml:lang="en">Multimodal Language Models are advanced AI models that can understand and generate information from different types of data such as text, images, and sound simultaneously. These models are designed to capture the complex relationships between different data modes, enabling more comprehensive understanding and generation of content.</dcterms:description>
        <oboInOwl:hasSynonym xml:lang="en">Multi-Modal Language Models</oboInOwl:hasSynonym>
        <oboInOwl:hasSynonym xml:lang="en">Multi-Modal Pre-trained Models</oboInOwl:hasSynonym>
        <oboInOwl:hasSynonym>Multimodal Foundation Models</oboInOwl:hasSynonym>
        <rdfs:label xml:lang="en">Multimodal Language Models</rdfs:label>
    </owl:NamedIndividual>
    


    <!-- http://nlpkg.sebis.cit.tum.de/nlp-fos-hierarchy.owl#Multiword_Expression_Identification -->

    <owl:NamedIndividual rdf:about="http://nlpkg.sebis.cit.tum.de/nlp-fos-hierarchy.owl#Multiword_Expression_Identification">
        <rdf:type rdf:resource="http://nlpkg.sebis.cit.tum.de/nlp-fos-hierarchy.owl#Task"/>
        <rdf:type rdf:resource="http://nlpkg.sebis.cit.tum.de/nlp-taxonomy.owl#FieldOfStudy"/>
        <nlp-taxonomy:subFieldOf rdf:resource="http://nlpkg.sebis.cit.tum.de/nlp-fos-hierarchy.owl#Multiword_Expression_Processing"/>
        <survey>https://aclanthology.org/2023.mwe-1.15</survey>
        <nlp-taxonomy:level rdf:datatype="http://www.w3.org/2001/XMLSchema#integer">4</nlp-taxonomy:level>
        <dcterms:description xml:lang="en">Multiword Expression (MWE) Identification refers to the process of detecting and classifying sequences of words that have a different meaning collectively than the individual meanings of the words. These expressions include idioms, compound nouns, phrasal verbs, etc. MWE identification is crucial in NLP tasks as it helps in understanding the semantic meaning of texts more accurately.</dcterms:description>
        <oboInOwl:hasSynonym xml:lang="en">MWE Detection</oboInOwl:hasSynonym>
        <oboInOwl:hasSynonym xml:lang="en">MWE Identification</oboInOwl:hasSynonym>
        <oboInOwl:hasSynonym xml:lang="en">Multiword Expression Detection</oboInOwl:hasSynonym>
        <rdfs:label xml:lang="en">Multiword Expression Identification</rdfs:label>
    </owl:NamedIndividual>
    


    <!-- http://nlpkg.sebis.cit.tum.de/nlp-fos-hierarchy.owl#Multiword_Expression_Processing -->

    <owl:NamedIndividual rdf:about="http://nlpkg.sebis.cit.tum.de/nlp-fos-hierarchy.owl#Multiword_Expression_Processing">
        <rdf:type rdf:resource="http://nlpkg.sebis.cit.tum.de/nlp-fos-hierarchy.owl#Task"/>
        <rdf:type rdf:resource="http://nlpkg.sebis.cit.tum.de/nlp-taxonomy.owl#FieldOfStudy"/>
        <nlp-taxonomy:subFieldOf rdf:resource="http://nlpkg.sebis.cit.tum.de/nlp-taxonomy.owl#Stylistic_Analysis"/>
        <nlp-taxonomy:superFieldOf rdf:resource="http://nlpkg.sebis.cit.tum.de/nlp-fos-hierarchy.owl#Multiword_Expression_Identification"/>
        <survey>https://aclanthology.org/J17-4005/</survey>
        <nlp-taxonomy:level rdf:datatype="http://www.w3.org/2001/XMLSchema#integer">3</nlp-taxonomy:level>
        <dcterms:description xml:lang="en">Multiword Expression Processing focuses on the identification, interpretation, and utilization of multiword expressions (MWEs). MWEs are phrases or combinations of words that have a specific, unique meaning when used together, which cannot be deduced from the meanings of the individual words. Examples include idioms like &quot;kick the bucket&quot;, compound nouns like &quot;hot dog&quot;, or verb-particle constructions like &quot;look up&quot;.</dcterms:description>
        <oboInOwl:hasSynonym xml:lang="en">MWE Processing</oboInOwl:hasSynonym>
        <rdfs:label xml:lang="en">Multiword Expression Processing</rdfs:label>
    </owl:NamedIndividual>
    


    <!-- http://nlpkg.sebis.cit.tum.de/nlp-fos-hierarchy.owl#Music_in_NLP -->

    <owl:NamedIndividual rdf:about="http://nlpkg.sebis.cit.tum.de/nlp-fos-hierarchy.owl#Music_in_NLP">
        <rdf:type rdf:resource="http://nlpkg.sebis.cit.tum.de/nlp-fos-hierarchy.owl#OtherScientificField"/>
        <rdf:type rdf:resource="http://nlpkg.sebis.cit.tum.de/nlp-taxonomy.owl#FieldOfStudy"/>
        <nlp-taxonomy:subFieldOf rdf:resource="http://nlpkg.sebis.cit.tum.de/nlp-taxonomy.owl#Speech_&amp;_Audio_In_NLP"/>
        <nlp-taxonomy:level rdf:datatype="http://www.w3.org/2001/XMLSchema#integer">3</nlp-taxonomy:level>
        <dcterms:description xml:lang="en">Music in NLP refers to the textual or symbolic representation of musical information, such as lyrics, musical notes, scores, or metadata related to music.  NLP techniques can be applied to analyze, generate, and derive insights from this textual data related to music.</dcterms:description>
        <rdfs:label xml:lang="en">Music in NLP</rdfs:label>
    </owl:NamedIndividual>
    


    <!-- http://nlpkg.sebis.cit.tum.de/nlp-fos-hierarchy.owl#Neural_Machine_Translation -->

    <owl:NamedIndividual rdf:about="http://nlpkg.sebis.cit.tum.de/nlp-fos-hierarchy.owl#Neural_Machine_Translation">
        <rdf:type rdf:resource="http://nlpkg.sebis.cit.tum.de/nlp-fos-hierarchy.owl#Task"/>
        <rdf:type rdf:resource="http://nlpkg.sebis.cit.tum.de/nlp-taxonomy.owl#FieldOfStudy"/>
        <uses rdf:resource="http://nlpkg.sebis.cit.tum.de/nlp-fos-hierarchy.owl#Multilingual_Language_Models"/>
        <nlp-taxonomy:subFieldOf rdf:resource="http://nlpkg.sebis.cit.tum.de/nlp-taxonomy.owl#Machine_Translation"/>
        <survey>https://aclanthology.org/C18-1111</survey>
        <survey>https://aclanthology.org/D17-1151</survey>
        <survey>https://arxiv.org/abs/1703.01619</survey>
        <survey>https://arxiv.org/abs/1901.09115</survey>
        <survey>https://arxiv.org/abs/1905.05395</survey>
        <survey>https://arxiv.org/abs/1910.00373</survey>
        <survey>https://arxiv.org/abs/1912.02047</survey>
        <survey>https://arxiv.org/abs/1912.08494</survey>
        <survey>https://arxiv.org/abs/2001.01115</survey>
        <survey>https://arxiv.org/abs/2002.07526</survey>
        <survey>https://arxiv.org/abs/2004.05809</survey>
        <survey>https://arxiv.org/abs/2012.15515</survey>
        <survey>https://arxiv.org/abs/2104.06951</survey>
        <survey>https://arxiv.org/abs/2106.15115</survey>
        <survey>https://arxiv.org/abs/2107.04239</survey>
        <survey>https://arxiv.org/abs/2204.09269</survey>
        <survey>https://arxiv.org/abs/2204.10365</survey>
        <nlp-taxonomy:level rdf:datatype="http://www.w3.org/2001/XMLSchema#integer">3</nlp-taxonomy:level>
        <dcterms:description xml:lang="en">Neural Machine Translation (NMT) is a method of automatic language translation that uses artificial neural networks. Unlike traditional statistical machine translation, NMT translates whole sentences at a time, considering the context of each word for a more accurate translation. It uses deep learning models to predict the likelihood of a sequence of words, typically modeling entire sentences in a single integrated model.</dcterms:description>
        <oboInOwl:hasSynonym xml:lang="en">NMT</oboInOwl:hasSynonym>
        <rdfs:label xml:lang="en">Neural Machine Translation</rdfs:label>
    </owl:NamedIndividual>
    


    <!-- http://nlpkg.sebis.cit.tum.de/nlp-fos-hierarchy.owl#Neural_Network_Architecture_Search -->

    <owl:NamedIndividual rdf:about="http://nlpkg.sebis.cit.tum.de/nlp-fos-hierarchy.owl#Neural_Network_Architecture_Search">
        <rdf:type rdf:resource="http://nlpkg.sebis.cit.tum.de/nlp-fos-hierarchy.owl#Task"/>
        <rdf:type rdf:resource="http://nlpkg.sebis.cit.tum.de/nlp-taxonomy.owl#FieldOfStudy"/>
        <nlp-taxonomy:subFieldOf rdf:resource="http://nlpkg.sebis.cit.tum.de/nlp-fos-hierarchy.owl#Meta-Learning"/>
        <nlp-taxonomy:level rdf:datatype="http://www.w3.org/2001/XMLSchema#integer">4</nlp-taxonomy:level>
        <dcterms:description xml:lang="en">Neural Network Architecture Search (NAS) refers to the process of automatically finding the best neural network architecture for a specific task. In the context of Meta-Learning, it involves learning algorithms that can adapt quickly to new tasks. In NLP, it involves finding the optimal network structure for language processing tasks. The goal is to automate the design of machine learning models to reduce the need for manual tuning and to improve model performance.</dcterms:description>
        <oboInOwl:hasSynonym xml:lang="en">NAS</oboInOwl:hasSynonym>
        <rdfs:label xml:lang="en">Neural Network Architecture Search</rdfs:label>
    </owl:NamedIndividual>
    


    <!-- http://nlpkg.sebis.cit.tum.de/nlp-fos-hierarchy.owl#Obfuscation -->

    <owl:NamedIndividual rdf:about="http://nlpkg.sebis.cit.tum.de/nlp-fos-hierarchy.owl#Obfuscation">
        <rdf:type rdf:resource="http://nlpkg.sebis.cit.tum.de/nlp-fos-hierarchy.owl#Task"/>
        <rdf:type rdf:resource="http://nlpkg.sebis.cit.tum.de/nlp-taxonomy.owl#FieldOfStudy"/>
        <usedFor rdf:resource="http://nlpkg.sebis.cit.tum.de/nlp-fos-hierarchy.owl#Anonymization"/>
        <nlp-taxonomy:subFieldOf rdf:resource="http://nlpkg.sebis.cit.tum.de/nlp-fos-hierarchy.owl#Privacy,_Security_&amp;_Safety_in_NLP"/>
        <nlp-taxonomy:superFieldOf rdf:resource="http://nlpkg.sebis.cit.tum.de/nlp-fos-hierarchy.owl#Authorship_Obfuscation"/>
        <nlp-taxonomy:superFieldOf rdf:resource="http://nlpkg.sebis.cit.tum.de/nlp-fos-hierarchy.owl#Profanity_Obfuscation"/>
        <nlp-taxonomy:level rdf:datatype="http://www.w3.org/2001/XMLSchema#integer">4</nlp-taxonomy:level>
        <dcterms:description xml:lang="en">Obfuscation refers to the process of altering text data in a way that it becomes less easily understood or interpreted by humans or machines, while still retaining the original meaning or information. This is often done for privacy protection, data anonymization, or to prevent automated systems from understanding sensitive information.</dcterms:description>
        <rdfs:label xml:lang="en">Obfuscation</rdfs:label>
    </owl:NamedIndividual>
    


    <!-- http://nlpkg.sebis.cit.tum.de/nlp-fos-hierarchy.owl#Offensive_Language_Detection -->

    <owl:NamedIndividual rdf:about="http://nlpkg.sebis.cit.tum.de/nlp-fos-hierarchy.owl#Offensive_Language_Detection">
        <rdf:type rdf:resource="http://nlpkg.sebis.cit.tum.de/nlp-fos-hierarchy.owl#Task"/>
        <rdf:type rdf:resource="http://nlpkg.sebis.cit.tum.de/nlp-taxonomy.owl#FieldOfStudy"/>
        <nlp-taxonomy:subFieldOf rdf:resource="http://nlpkg.sebis.cit.tum.de/nlp-fos-hierarchy.owl#Discrimination_Analysis"/>
        <nlp-taxonomy:subFieldOf rdf:resource="http://nlpkg.sebis.cit.tum.de/nlp-taxonomy.owl#Text_Classification"/>
        <survey>https://arxiv.org/abs/1908.06024</survey>
        <survey>https://arxiv.org/abs/2012.12305</survey>
        <nlp-taxonomy:level rdf:datatype="http://www.w3.org/2001/XMLSchema#integer">3</nlp-taxonomy:level>
        <dcterms:description xml:lang="en">Offensive Language Detection refers to the application of machine learning and AI techniques to identify and filter out offensive, inappropriate, or harmful language in text.</dcterms:description>
        <oboInOwl:hasSynonym xml:lang="en">Abuse Classification</oboInOwl:hasSynonym>
        <oboInOwl:hasSynonym xml:lang="en">Abuse Detection</oboInOwl:hasSynonym>
        <oboInOwl:hasSynonym xml:lang="en">Abuse Identification</oboInOwl:hasSynonym>
        <oboInOwl:hasSynonym xml:lang="en">Abusive Language Classification</oboInOwl:hasSynonym>
        <oboInOwl:hasSynonym xml:lang="en">Abusive Language Detection</oboInOwl:hasSynonym>
        <oboInOwl:hasSynonym xml:lang="en">Abusive Language Identification</oboInOwl:hasSynonym>
        <oboInOwl:hasSynonym xml:lang="en">Offensive Language Classification</oboInOwl:hasSynonym>
        <oboInOwl:hasSynonym xml:lang="en">Offensive Language Identification</oboInOwl:hasSynonym>
        <oboInOwl:hasSynonym xml:lang="en">Toxic Language Classification</oboInOwl:hasSynonym>
        <oboInOwl:hasSynonym xml:lang="en">Toxic Language Detection</oboInOwl:hasSynonym>
        <oboInOwl:hasSynonym xml:lang="en">Toxic Language Identification</oboInOwl:hasSynonym>
        <rdfs:label xml:lang="en">Offensive Language Detection</rdfs:label>
    </owl:NamedIndividual>
    


    <!-- http://nlpkg.sebis.cit.tum.de/nlp-fos-hierarchy.owl#One-Hop_Reasoning -->

    <owl:NamedIndividual rdf:about="http://nlpkg.sebis.cit.tum.de/nlp-fos-hierarchy.owl#One-Hop_Reasoning">
        <rdf:type rdf:resource="http://nlpkg.sebis.cit.tum.de/nlp-fos-hierarchy.owl#Task"/>
        <rdf:type rdf:resource="http://nlpkg.sebis.cit.tum.de/nlp-taxonomy.owl#FieldOfStudy"/>
        <nlp-taxonomy:subFieldOf rdf:resource="http://nlpkg.sebis.cit.tum.de/nlp-fos-hierarchy.owl#Knowledge_Graph_Question_Answering"/>
        <nlp-taxonomy:subFieldOf rdf:resource="http://nlpkg.sebis.cit.tum.de/nlp-taxonomy.owl#Reasoning"/>
        <nlp-taxonomy:level rdf:datatype="http://www.w3.org/2001/XMLSchema#integer">2</nlp-taxonomy:level>
        <nlp-taxonomy:level rdf:datatype="http://www.w3.org/2001/XMLSchema#integer">5</nlp-taxonomy:level>
        <nlp-taxonomy:level rdf:datatype="http://www.w3.org/2001/XMLSchema#integer">6</nlp-taxonomy:level>
        <nlp-taxonomy:level rdf:datatype="http://www.w3.org/2001/XMLSchema#integer">7</nlp-taxonomy:level>
        <dcterms:description xml:lang="en">One-Hop Reasoning is a concept where the system uses a knowledge graph or text passage to answer simple queries by making a single &quot;hop&quot; or step from one entity to another. This involves identifying direct relationships or connections between entities in the graph or text passage. For example, if the query is about the capital of a country, the system would make one &quot;hop&quot; from the country to its capital in the knowledge graph or text passage.</dcterms:description>
        <oboInOwl:hasSynonym xml:lang="en">One-Hop KG Reasoning</oboInOwl:hasSynonym>
        <oboInOwl:hasSynonym xml:lang="en">One-Hop Knowledge Graph Reasoning</oboInOwl:hasSynonym>
        <oboInOwl:hasSynonym xml:lang="en">One-Hop MRC</oboInOwl:hasSynonym>
        <oboInOwl:hasSynonym xml:lang="en">One-Hop Machine Reading Comprehension</oboInOwl:hasSynonym>
        <oboInOwl:hasSynonym xml:lang="en">One-Hop QA</oboInOwl:hasSynonym>
        <oboInOwl:hasSynonym xml:lang="en">One-Hop Question Answering</oboInOwl:hasSynonym>
        <oboInOwl:hasSynonym xml:lang="en">SIngle-Hop Machine Reading Comprehension</oboInOwl:hasSynonym>
        <oboInOwl:hasSynonym xml:lang="en">Single-Hop KG Reasoning</oboInOwl:hasSynonym>
        <oboInOwl:hasSynonym xml:lang="en">Single-Hop MRC</oboInOwl:hasSynonym>
        <oboInOwl:hasSynonym xml:lang="en">Single-Hop QA</oboInOwl:hasSynonym>
        <oboInOwl:hasSynonym xml:lang="en">Single-Hop Question Answering</oboInOwl:hasSynonym>
        <oboInOwl:hasSynonym xml:lang="en">Single-Hop Reasoning</oboInOwl:hasSynonym>
        <rdfs:label xml:lang="en">One-Hop Reasoning</rdfs:label>
    </owl:NamedIndividual>
    


    <!-- http://nlpkg.sebis.cit.tum.de/nlp-fos-hierarchy.owl#Ontologies -->

    <owl:NamedIndividual rdf:about="http://nlpkg.sebis.cit.tum.de/nlp-fos-hierarchy.owl#Ontologies">
        <rdf:type rdf:resource="http://nlpkg.sebis.cit.tum.de/nlp-fos-hierarchy.owl#DataStructure"/>
        <rdf:type rdf:resource="http://nlpkg.sebis.cit.tum.de/nlp-taxonomy.owl#FieldOfStudy"/>
        <nlp-taxonomy:subFieldOf rdf:resource="http://nlpkg.sebis.cit.tum.de/nlp-fos-hierarchy.owl#Graphs"/>
        <nlp-taxonomy:superFieldOf rdf:resource="http://nlpkg.sebis.cit.tum.de/nlp-fos-hierarchy.owl#Ontology_Learning"/>
        <nlp-taxonomy:superFieldOf rdf:resource="http://nlpkg.sebis.cit.tum.de/nlp-fos-hierarchy.owl#Ontology_Reasoning"/>
        <nlp-taxonomy:level rdf:datatype="http://www.w3.org/2001/XMLSchema#integer">5</nlp-taxonomy:level>
        <dcterms:description xml:lang="en">Ontologies encompass a representation, formal naming, and definition of categories, properties, and relations between concepts, data, and entities.</dcterms:description>
        <rdfs:label xml:lang="en">Ontologies</rdfs:label>
    </owl:NamedIndividual>
    


    <!-- http://nlpkg.sebis.cit.tum.de/nlp-fos-hierarchy.owl#Ontology_Learning -->

    <owl:NamedIndividual rdf:about="http://nlpkg.sebis.cit.tum.de/nlp-fos-hierarchy.owl#Ontology_Learning">
        <rdf:type rdf:resource="http://nlpkg.sebis.cit.tum.de/nlp-fos-hierarchy.owl#Task"/>
        <rdf:type rdf:resource="http://nlpkg.sebis.cit.tum.de/nlp-taxonomy.owl#FieldOfStudy"/>
        <uses rdf:resource="http://nlpkg.sebis.cit.tum.de/nlp-taxonomy.owl#Coreference_Resolution"/>
        <uses rdf:resource="http://nlpkg.sebis.cit.tum.de/nlp-taxonomy.owl#Named_Entity_Recognition"/>
        <uses rdf:resource="http://nlpkg.sebis.cit.tum.de/nlp-taxonomy.owl#Relation_Extraction"/>
        <uses rdf:resource="http://nlpkg.sebis.cit.tum.de/nlp-taxonomy.owl#Term_Extraction"/>
        <nlp-taxonomy:subFieldOf rdf:resource="http://nlpkg.sebis.cit.tum.de/nlp-fos-hierarchy.owl#Ontologies"/>
        <survey>https://doi.org/10.1093/database/bay101</survey>
        <nlp-taxonomy:level rdf:datatype="http://www.w3.org/2001/XMLSchema#integer">6</nlp-taxonomy:level>
        <dcterms:description xml:lang="en">Ontology Learning focuses on the automatic or semi-automatic creation, evolution, and population of ontologies. It involves extracting information from various sources like text documents, databases, XML documents, etc., to create ontologies, which are structured sets of knowledge that include categories, properties, and relationships between entities.</dcterms:description>
        <oboInOwl:hasSynonym xml:lang="en">Ontology Acquisition</oboInOwl:hasSynonym>
        <oboInOwl:hasSynonym xml:lang="en">Ontology Extraction</oboInOwl:hasSynonym>
        <oboInOwl:hasSynonym xml:lang="en">Ontology Generation</oboInOwl:hasSynonym>
        <rdfs:label xml:lang="en">Ontology Learning</rdfs:label>
    </owl:NamedIndividual>
    


    <!-- http://nlpkg.sebis.cit.tum.de/nlp-fos-hierarchy.owl#Ontology_Reasoning -->

    <owl:NamedIndividual rdf:about="http://nlpkg.sebis.cit.tum.de/nlp-fos-hierarchy.owl#Ontology_Reasoning">
        <rdf:type rdf:resource="http://nlpkg.sebis.cit.tum.de/nlp-fos-hierarchy.owl#Task"/>
        <rdf:type rdf:resource="http://nlpkg.sebis.cit.tum.de/nlp-taxonomy.owl#FieldOfStudy"/>
        <nlp-taxonomy:subFieldOf rdf:resource="http://nlpkg.sebis.cit.tum.de/nlp-fos-hierarchy.owl#Ontologies"/>
        <nlp-taxonomy:level rdf:datatype="http://www.w3.org/2001/XMLSchema#integer">6</nlp-taxonomy:level>
        <dcterms:description xml:lang="en">Ontology Reasoning refers to the use of structured sets of knowledge (ontologies) to make inferences, draw conclusions, or make decisions. Ontologies, in this context, are a formal representation of knowledge within a domain, including the relationships between entities. This approach can help in understanding the context, semantics, and meaning of words in a text, thereby improving the accuracy of NLP tasks.</dcterms:description>
        <rdfs:label xml:lang="en">Ontology Reasoning</rdfs:label>
    </owl:NamedIndividual>
    


    <!-- http://nlpkg.sebis.cit.tum.de/nlp-fos-hierarchy.owl#Open_Book_Question_Answering -->

    <owl:NamedIndividual rdf:about="http://nlpkg.sebis.cit.tum.de/nlp-fos-hierarchy.owl#Open_Book_Question_Answering">
        <rdf:type rdf:resource="http://nlpkg.sebis.cit.tum.de/nlp-fos-hierarchy.owl#Task"/>
        <rdf:type rdf:resource="http://nlpkg.sebis.cit.tum.de/nlp-taxonomy.owl#FieldOfStudy"/>
        <uses rdf:resource="http://nlpkg.sebis.cit.tum.de/nlp-fos-hierarchy.owl#Commonsense_Question_Answering"/>
        <nlp-taxonomy:subFieldOf rdf:resource="http://nlpkg.sebis.cit.tum.de/nlp-taxonomy.owl#Question_Answering"/>
        <nlp-taxonomy:level rdf:datatype="http://www.w3.org/2001/XMLSchema#integer">3</nlp-taxonomy:level>
        <dcterms:description xml:lang="en">Open Book Question Answering is a type of natural language based QA (NLQA) where questions are expected to be answered with respect to a given set of open book facts, and common knowledge about a topic.</dcterms:description>
        <oboInOwl:hasSynonym xml:lang="en">Open Book QA</oboInOwl:hasSynonym>
        <oboInOwl:hasSynonym xml:lang="en">Open-book QA</oboInOwl:hasSynonym>
        <oboInOwl:hasSynonym xml:lang="en">Open-book Question Answering</oboInOwl:hasSynonym>
        <rdfs:label xml:lang="en">Open Book Question Answering</rdfs:label>
    </owl:NamedIndividual>
    


    <!-- http://nlpkg.sebis.cit.tum.de/nlp-fos-hierarchy.owl#Open_Domain_Question_Answering -->

    <owl:NamedIndividual rdf:about="http://nlpkg.sebis.cit.tum.de/nlp-fos-hierarchy.owl#Open_Domain_Question_Answering">
        <rdf:type rdf:resource="http://nlpkg.sebis.cit.tum.de/nlp-fos-hierarchy.owl#Task"/>
        <rdf:type rdf:resource="http://nlpkg.sebis.cit.tum.de/nlp-taxonomy.owl#FieldOfStudy"/>
        <nlp-taxonomy:subFieldOf rdf:resource="http://nlpkg.sebis.cit.tum.de/nlp-taxonomy.owl#Question_Answering"/>
        <survey>https://aclanthology.org/2021.tacl-1.61</survey>
        <survey>https://aclanthology.org/2023.acl-long.307</survey>
        <survey>https://aclanthology.org/2023.acl-long.808</survey>
        <survey>https://arxiv.org/abs/2101.00774</survey>
        <survey>https://arxiv.org/abs/2208.03197</survey>
        <nlp-taxonomy:level rdf:datatype="http://www.w3.org/2001/XMLSchema#integer">3</nlp-taxonomy:level>
        <dcterms:description xml:lang="en">Open Domain Question Answering (ODQA) is a task in natural language processing that involves responding to questions about any topic without a specific domain limitation.</dcterms:description>
        <oboInOwl:hasSynonym>ODQA</oboInOwl:hasSynonym>
        <oboInOwl:hasSynonym xml:lang="en">Open Domain QA</oboInOwl:hasSynonym>
        <oboInOwl:hasSynonym xml:lang="en">Open-Domain QA</oboInOwl:hasSynonym>
        <oboInOwl:hasSynonym xml:lang="en">Open-Domain Question Answering</oboInOwl:hasSynonym>
        <rdfs:label xml:lang="en">Open Domain Question Answering</rdfs:label>
    </owl:NamedIndividual>
    


    <!-- http://nlpkg.sebis.cit.tum.de/nlp-fos-hierarchy.owl#Optical_Character_Recognition -->

    <owl:NamedIndividual rdf:about="http://nlpkg.sebis.cit.tum.de/nlp-fos-hierarchy.owl#Optical_Character_Recognition">
        <rdf:type rdf:resource="http://nlpkg.sebis.cit.tum.de/nlp-fos-hierarchy.owl#Task"/>
        <rdf:type rdf:resource="http://nlpkg.sebis.cit.tum.de/nlp-taxonomy.owl#FieldOfStudy"/>
        <nlp-taxonomy:subFieldOf rdf:resource="http://nlpkg.sebis.cit.tum.de/nlp-taxonomy.owl#Visual_Data_In_NLP"/>
        <survey>https://arxiv.org/abs/2005.03492</survey>
        <survey>https://arxiv.org/abs/2006.04305</survey>
        <survey>https://arxiv.org/abs/2011.01314</survey>
        <survey>https://arxiv.org/abs/2011.13534</survey>
        <nlp-taxonomy:level rdf:datatype="http://www.w3.org/2001/XMLSchema#integer">3</nlp-taxonomy:level>
        <dcterms:description xml:lang="en">Optical Character Recognition (OCR) is a technology that enables the conversion of printed or handwritten text and characters into machine-readable digital text. It is a process of digitizing text from physical documents, such as scanned paper documents, photographs, or images, and making the content accessible and editable on a computer or other digital devices.</dcterms:description>
        <oboInOwl:hasSynonym xml:lang="en">ITT</oboInOwl:hasSynonym>
        <oboInOwl:hasSynonym xml:lang="en">Image-to-Text</oboInOwl:hasSynonym>
        <oboInOwl:hasSynonym xml:lang="en">OCR</oboInOwl:hasSynonym>
        <oboInOwl:hasSynonym xml:lang="en">Text Detection</oboInOwl:hasSynonym>
        <oboInOwl:hasSynonym xml:lang="en">Text Recognition</oboInOwl:hasSynonym>
        <rdfs:label xml:lang="en">Optical Character Recognition</rdfs:label>
    </owl:NamedIndividual>
    


    <!-- http://nlpkg.sebis.cit.tum.de/nlp-fos-hierarchy.owl#Parameter-Efficient_Fine-Tuning -->

    <owl:NamedIndividual rdf:about="http://nlpkg.sebis.cit.tum.de/nlp-fos-hierarchy.owl#Parameter-Efficient_Fine-Tuning">
        <rdf:type rdf:resource="http://nlpkg.sebis.cit.tum.de/nlp-fos-hierarchy.owl#Task"/>
        <rdf:type rdf:resource="http://nlpkg.sebis.cit.tum.de/nlp-taxonomy.owl#FieldOfStudy"/>
        <nlp-taxonomy:subFieldOf rdf:resource="http://nlpkg.sebis.cit.tum.de/nlp-taxonomy.owl#Language_Models"/>
        <nlp-taxonomy:subFieldOf rdf:resource="http://nlpkg.sebis.cit.tum.de/nlp-taxonomy.owl#Green_&amp;_Sustainable_NLP"/>
        <nlp-taxonomy:superFieldOf rdf:resource="http://nlpkg.sebis.cit.tum.de/nlp-fos-hierarchy.owl#Language_Model_Adapters"/>
        <nlp-taxonomy:superFieldOf rdf:resource="http://nlpkg.sebis.cit.tum.de/nlp-fos-hierarchy.owl#Soft_Prompts"/>
        <code>https://github.com/huggingface/peft</code>
        <relevantInformation>https://huggingface.co/blog/peft</relevantInformation>
        <nlp-taxonomy:level rdf:datatype="http://www.w3.org/2001/XMLSchema#integer">3</nlp-taxonomy:level>
        <nlp-taxonomy:level rdf:datatype="http://www.w3.org/2001/XMLSchema#integer">4</nlp-taxonomy:level>
        <dcterms:description xml:lang="en">Parameter-Efficient Fine-Tuning (PEFT) is a method that aims to reduce the number of parameters that need to be fine-tuned in large pre-trained language models. This is achieved by freezing the majority of the parameters and only fine-tuning a small subset, which makes the process more efficient in terms of computational resources and time. This approach also helps to mitigate overfitting, especially when the available fine-tuning data is limited.</dcterms:description>
        <oboInOwl:hasSynonym xml:lang="en">PEFT</oboInOwl:hasSynonym>
        <rdfs:label xml:lang="en">Parameter-Efficient Fine-Tuning</rdfs:label>
    </owl:NamedIndividual>
    


    <!-- http://nlpkg.sebis.cit.tum.de/nlp-fos-hierarchy.owl#Paraphrase_Detection -->

    <owl:NamedIndividual rdf:about="http://nlpkg.sebis.cit.tum.de/nlp-fos-hierarchy.owl#Paraphrase_Detection">
        <rdf:type rdf:resource="http://nlpkg.sebis.cit.tum.de/nlp-fos-hierarchy.owl#Task"/>
        <rdf:type rdf:resource="http://nlpkg.sebis.cit.tum.de/nlp-taxonomy.owl#FieldOfStudy"/>
        <nlp-taxonomy:subFieldOf rdf:resource="http://nlpkg.sebis.cit.tum.de/nlp-taxonomy.owl#Text_Classification"/>
        <survey>https://arxiv.org/abs/2106.00145</survey>
        <survey>https://arxiv.org/abs/2212.06933</survey>
        <survey>https://arxiv.org/abs/2303.13989</survey>
        <nlp-taxonomy:level rdf:datatype="http://www.w3.org/2001/XMLSchema#integer">3</nlp-taxonomy:level>
        <dcterms:description xml:lang="en">Paraphrase Detection is the task of determining whether two text strings are paraphrases of each other. In other words, it involves identifying if the two given sentences convey the same meaning using different words or sentence structures.</dcterms:description>
        <oboInOwl:hasSynonym xml:lang="en">Paraphrase Classification</oboInOwl:hasSynonym>
        <oboInOwl:hasSynonym xml:lang="en">Paraphrase Identification</oboInOwl:hasSynonym>
        <rdfs:label xml:lang="en">Paraphrase Detection</rdfs:label>
    </owl:NamedIndividual>
    


    <!-- http://nlpkg.sebis.cit.tum.de/nlp-fos-hierarchy.owl#Parse_Tree -->

    <owl:NamedIndividual rdf:about="http://nlpkg.sebis.cit.tum.de/nlp-fos-hierarchy.owl#Parse_Tree">
        <rdf:type rdf:resource="http://nlpkg.sebis.cit.tum.de/nlp-fos-hierarchy.owl#DataStructure"/>
        <rdf:type rdf:resource="http://nlpkg.sebis.cit.tum.de/nlp-taxonomy.owl#FieldOfStudy"/>
        <usedFor rdf:resource="http://nlpkg.sebis.cit.tum.de/nlp-fos-hierarchy.owl#Syntactic_Treebank"/>
        <nlp-taxonomy:subFieldOf rdf:resource="http://nlpkg.sebis.cit.tum.de/nlp-fos-hierarchy.owl#Tree"/>
        <nlp-taxonomy:superFieldOf rdf:resource="http://nlpkg.sebis.cit.tum.de/nlp-fos-hierarchy.owl#Constituency_Parse_Tree"/>
        <nlp-taxonomy:superFieldOf rdf:resource="http://nlpkg.sebis.cit.tum.de/nlp-fos-hierarchy.owl#Dependency_Graphs"/>
        <nlp-taxonomy:superFieldOf rdf:resource="http://nlpkg.sebis.cit.tum.de/nlp-fos-hierarchy.owl#Syntactic_Paths"/>
        <nlp-taxonomy:superFieldOf rdf:resource="http://nlpkg.sebis.cit.tum.de/nlp-fos-hierarchy.owl#Tree_Fragments"/>
        <nlp-taxonomy:level rdf:datatype="http://www.w3.org/2001/XMLSchema#integer">5</nlp-taxonomy:level>
        <dcterms:description xml:lang="en">A Parse Tree, or Syntax Tree, is a hierarchical representation of the syntactic structure of a sentence or text, showing how words and phrases are organized according to the grammar rules of a language. It visually illustrates how words are grouped into phrases and how those phrases relate to each other, helping to analyze the grammatical structure of the text.</dcterms:description>
        <oboInOwl:hasSynonym xml:lang="en">Syntactic Tree</oboInOwl:hasSynonym>
        <oboInOwl:hasSynonym xml:lang="en">Syntax Tree</oboInOwl:hasSynonym>
        <rdfs:label xml:lang="en">Parse Tree</rdfs:label>
    </owl:NamedIndividual>
    


    <!-- http://nlpkg.sebis.cit.tum.de/nlp-fos-hierarchy.owl#Part-of-Speech_Tagging -->

    <owl:NamedIndividual rdf:about="http://nlpkg.sebis.cit.tum.de/nlp-fos-hierarchy.owl#Part-of-Speech_Tagging">
        <rdf:type rdf:resource="http://nlpkg.sebis.cit.tum.de/nlp-fos-hierarchy.owl#Task"/>
        <rdf:type rdf:resource="http://nlpkg.sebis.cit.tum.de/nlp-taxonomy.owl#FieldOfStudy"/>
        <uses rdf:resource="http://nlpkg.sebis.cit.tum.de/nlp-fos-hierarchy.owl#Sequence_Labeling"/>
        <nlp-taxonomy:subFieldOf rdf:resource="http://nlpkg.sebis.cit.tum.de/nlp-taxonomy.owl#Tagging"/>
        <code>https://spacy.io/usage/linguistic-features#pos-tagging</code>
        <survey>https://arxiv.org/abs/2110.04977</survey>
        <nlp-taxonomy:level rdf:datatype="http://www.w3.org/2001/XMLSchema#integer">3</nlp-taxonomy:level>
        <dcterms:description xml:lang="en">Part-of-Speech (PoS) Tagging is a process where grammatical tags or categories are assigned to each word (or token) in a sentence. These tags indicate the role of the word in the sentence, such as whether it&apos;s a noun, verb, adjective, adverb, etc.</dcterms:description>
        <oboInOwl:hasSynonym xml:lang="en">POS Tagging</oboInOwl:hasSynonym>
        <oboInOwl:hasSynonym xml:lang="en">Part of Speech Tagging</oboInOwl:hasSynonym>
        <oboInOwl:hasSynonym xml:lang="en">Part-Of-Speech Tagging</oboInOwl:hasSynonym>
        <oboInOwl:hasSynonym xml:lang="en">Parts of Speech Tagging</oboInOwl:hasSynonym>
        <oboInOwl:hasSynonym xml:lang="en">Parts-of-Speech Tagging</oboInOwl:hasSynonym>
        <oboInOwl:hasSynonym xml:lang="en">PoS Tagging</oboInOwl:hasSynonym>
        <rdfs:label xml:lang="en">Part-of-Speech Tagging</rdfs:label>
    </owl:NamedIndividual>
    


    <!-- http://nlpkg.sebis.cit.tum.de/nlp-fos-hierarchy.owl#Penn_Discourse_Treebank_Discourse_Parsing -->

    <owl:NamedIndividual rdf:about="http://nlpkg.sebis.cit.tum.de/nlp-fos-hierarchy.owl#Penn_Discourse_Treebank_Discourse_Parsing">
        <rdf:type rdf:resource="http://nlpkg.sebis.cit.tum.de/nlp-fos-hierarchy.owl#Task"/>
        <rdf:type rdf:resource="http://nlpkg.sebis.cit.tum.de/nlp-taxonomy.owl#FieldOfStudy"/>
        <nlp-taxonomy:subFieldOf rdf:resource="http://nlpkg.sebis.cit.tum.de/nlp-fos-hierarchy.owl#Discourse_Parsing"/>
        <nlp-taxonomy:level rdf:datatype="http://www.w3.org/2001/XMLSchema#integer">4</nlp-taxonomy:level>
        <dcterms:description xml:lang="en">Penn Discourse Treebank Discourse Parsing, often referred to as PDTB Discourse Parsing, is a natural language processing (NLP) task focused on analyzing and structuring the relationships and coherence between different parts of a text. It involves creating a tree-like structure that represents how sentences, phrases, or clauses in a text are connected in terms of discourse relations such as contrast, elaboration, and cause-effect. This parsing is typically done using the Penn Discourse Treebank dataset.</dcterms:description>
        <oboInOwl:hasSynonym xml:lang="en">PDTB-DP</oboInOwl:hasSynonym>
        <oboInOwl:hasSynonym xml:lang="en">PDTB-style Discourse Parsing</oboInOwl:hasSynonym>
        <oboInOwl:hasSynonym xml:lang="en">Penn Discourse Tree-Bank Discourse Parsing</oboInOwl:hasSynonym>
        <rdfs:label xml:lang="en">Penn Discourse Treebank Discourse Parsing</rdfs:label>
    </owl:NamedIndividual>
    


    <!-- http://nlpkg.sebis.cit.tum.de/nlp-fos-hierarchy.owl#Phrase-based_Machine_Translation -->

    <owl:NamedIndividual rdf:about="http://nlpkg.sebis.cit.tum.de/nlp-fos-hierarchy.owl#Phrase-based_Machine_Translation">
        <rdf:type rdf:resource="http://nlpkg.sebis.cit.tum.de/nlp-fos-hierarchy.owl#Task"/>
        <rdf:type rdf:resource="http://nlpkg.sebis.cit.tum.de/nlp-taxonomy.owl#FieldOfStudy"/>
        <nlp-taxonomy:subFieldOf rdf:resource="http://nlpkg.sebis.cit.tum.de/nlp-fos-hierarchy.owl#Statistical_Machine_Translation"/>
        <nlp-taxonomy:superFieldOf rdf:resource="http://nlpkg.sebis.cit.tum.de/nlp-fos-hierarchy.owl#Hierarchical_Phrase-based_Machine_Translation"/>
        <nlp-taxonomy:level rdf:datatype="http://www.w3.org/2001/XMLSchema#integer">4</nlp-taxonomy:level>
        <dcterms:description xml:lang="en">Phrase-based Machine Translation (PBMT) is a method that translates whole phrases instead of individual words to capture more context and meaning. This approach allows the system to handle differences in word order between languages and to translate common idioms or phrases that don&apos;t make sense when translated word by word. It uses statistical models to determine the most likely translation.</dcterms:description>
        <oboInOwl:hasSynonym xml:lang="en">PBMT</oboInOwl:hasSynonym>
        <rdfs:label xml:lang="en">Phrase-based Machine Translation</rdfs:label>
    </owl:NamedIndividual>
    


    <!-- http://nlpkg.sebis.cit.tum.de/nlp-fos-hierarchy.owl#Political_Bias -->

    <owl:NamedIndividual rdf:about="http://nlpkg.sebis.cit.tum.de/nlp-fos-hierarchy.owl#Political_Bias">
        <rdf:type rdf:resource="http://nlpkg.sebis.cit.tum.de/nlp-fos-hierarchy.owl#OtherScientificField"/>
        <rdf:type rdf:resource="http://nlpkg.sebis.cit.tum.de/nlp-taxonomy.owl#FieldOfStudy"/>
        <nlp-taxonomy:subFieldOf rdf:resource="http://nlpkg.sebis.cit.tum.de/nlp-fos-hierarchy.owl#Social_Bias"/>
        <nlp-taxonomy:level rdf:datatype="http://www.w3.org/2001/XMLSchema#integer">5</nlp-taxonomy:level>
        <dcterms:description xml:lang="en">Political Bias is the tendency to favor a particular political party, ideology, or candidate, often resulting in presenting information in a way that unfairly supports one side over the other.</dcterms:description>
        <rdfs:label xml:lang="en">Political Bias</rdfs:label>
    </owl:NamedIndividual>
    


    <!-- http://nlpkg.sebis.cit.tum.de/nlp-fos-hierarchy.owl#Positional_Encoding -->

    <owl:NamedIndividual rdf:about="http://nlpkg.sebis.cit.tum.de/nlp-fos-hierarchy.owl#Positional_Encoding">
        <rdf:type rdf:resource="http://nlpkg.sebis.cit.tum.de/nlp-fos-hierarchy.owl#OtherScientificField"/>
        <rdf:type rdf:resource="http://nlpkg.sebis.cit.tum.de/nlp-taxonomy.owl#FieldOfStudy"/>
        <usedFor rdf:resource="http://nlpkg.sebis.cit.tum.de/nlp-fos-hierarchy.owl#Transformers_&amp;_Large_Language_Models"/>
        <nlp-taxonomy:subFieldOf rdf:resource="http://nlpkg.sebis.cit.tum.de/nlp-fos-hierarchy.owl#Language_Model_Mechanisms"/>
        <nlp-taxonomy:level rdf:datatype="http://www.w3.org/2001/XMLSchema#integer">4</nlp-taxonomy:level>
        <dcterms:description xml:lang="en">Positional Encoding is a technique used to give the model some information about the relative positions of the words in a sentence. It is used in transformer-based models where the order of words is not inherently considered. Positional encoding can be done in several ways, such as by adding a unique positional value to the word embeddings for each position in the sentence, or by using a sinusoidal function to generate positional encodings. This helps the model to understand the order of words and the grammar of the language.</dcterms:description>
        <oboInOwl:hasSynonym xml:lang="en">Positional Embedding</oboInOwl:hasSynonym>
        <rdfs:label xml:lang="en">Positional Encoding</rdfs:label>
    </owl:NamedIndividual>
    


    <!-- http://nlpkg.sebis.cit.tum.de/nlp-fos-hierarchy.owl#Post-Training_Quantization -->

    <owl:NamedIndividual rdf:about="http://nlpkg.sebis.cit.tum.de/nlp-fos-hierarchy.owl#Post-Training_Quantization">
        <rdf:type rdf:resource="http://nlpkg.sebis.cit.tum.de/nlp-fos-hierarchy.owl#Task"/>
        <rdf:type rdf:resource="http://nlpkg.sebis.cit.tum.de/nlp-taxonomy.owl#FieldOfStudy"/>
        <nlp-taxonomy:subFieldOf rdf:resource="http://nlpkg.sebis.cit.tum.de/nlp-fos-hierarchy.owl#Language_Model_Quantization"/>
        <nlp-taxonomy:level rdf:datatype="http://www.w3.org/2001/XMLSchema#integer">4</nlp-taxonomy:level>
        <nlp-taxonomy:level rdf:datatype="http://www.w3.org/2001/XMLSchema#integer">5</nlp-taxonomy:level>
        <dcterms:description xml:lang="en">Post-Training Quantization (PTQ) is a quantization technique where the model is quantized after it has been trained.</dcterms:description>
        <oboInOwl:hasSynonym xml:lang="en">PTQ</oboInOwl:hasSynonym>
        <rdfs:label xml:lang="en">Post-Training Quantization</rdfs:label>
    </owl:NamedIndividual>
    


    <!-- http://nlpkg.sebis.cit.tum.de/nlp-fos-hierarchy.owl#Pragmatic_Modeling -->

    <owl:NamedIndividual rdf:about="http://nlpkg.sebis.cit.tum.de/nlp-fos-hierarchy.owl#Pragmatic_Modeling">
        <rdf:type rdf:resource="http://nlpkg.sebis.cit.tum.de/nlp-fos-hierarchy.owl#Task"/>
        <rdf:type rdf:resource="http://nlpkg.sebis.cit.tum.de/nlp-taxonomy.owl#FieldOfStudy"/>
        <nlp-taxonomy:subFieldOf rdf:resource="http://nlpkg.sebis.cit.tum.de/nlp-taxonomy.owl#Discourse_&amp;_Pragmatics"/>
        <nlp-taxonomy:level rdf:datatype="http://www.w3.org/2001/XMLSchema#integer">3</nlp-taxonomy:level>
        <dcterms:description xml:lang="en">Pragmatics Modeling refers to the study and implementation of computational methods to understand and generate language that takes into account the context, speaker intentions, and the implied meaning beyond literal words and grammar. It focuses on how language is used in real-world situations and how context influences communication. Pragmatics modeling helps computers interpret and generate language that is contextually appropriate and conveys the intended meaning effectively.</dcterms:description>
        <rdfs:label xml:lang="en">Pragmatic Modeling</rdfs:label>
    </owl:NamedIndividual>
    


    <!-- http://nlpkg.sebis.cit.tum.de/nlp-fos-hierarchy.owl#Proactive_Learning -->

    <owl:NamedIndividual rdf:about="http://nlpkg.sebis.cit.tum.de/nlp-fos-hierarchy.owl#Proactive_Learning">
        <rdf:type rdf:resource="http://nlpkg.sebis.cit.tum.de/nlp-fos-hierarchy.owl#Task"/>
        <rdf:type rdf:resource="http://nlpkg.sebis.cit.tum.de/nlp-taxonomy.owl#FieldOfStudy"/>
        <nlp-taxonomy:subFieldOf rdf:resource="http://nlpkg.sebis.cit.tum.de/nlp-fos-hierarchy.owl#Active_Learning"/>
        <relevantInformation>https://academic-accelerator.com/encyclopedia/proactive-learning</relevantInformation>
        <survey>https://www.cs.cmu.edu/~jgc/Active-to-Proactive%20Learning.pdf</survey>
        <nlp-taxonomy:level rdf:datatype="http://www.w3.org/2001/XMLSchema#integer">4</nlp-taxonomy:level>
        <dcterms:description xml:lang="en">Proactive Learning is a generalization of active learning aimed at relaxing unrealistic assumptions and thereby reaching practical applications.</dcterms:description>
        <rdfs:label xml:lang="en">Proactive Learning</rdfs:label>
    </owl:NamedIndividual>
    


    <!-- http://nlpkg.sebis.cit.tum.de/nlp-fos-hierarchy.owl#Probing -->

    <owl:NamedIndividual rdf:about="http://nlpkg.sebis.cit.tum.de/nlp-fos-hierarchy.owl#Probing">
        <rdf:type rdf:resource="http://nlpkg.sebis.cit.tum.de/nlp-fos-hierarchy.owl#Task"/>
        <rdf:type rdf:resource="http://nlpkg.sebis.cit.tum.de/nlp-taxonomy.owl#FieldOfStudy"/>
        <usedFor rdf:resource="http://nlpkg.sebis.cit.tum.de/nlp-taxonomy.owl#Explainability_&amp;_Interpretability_In_NLP"/>
        <nlp-taxonomy:subFieldOf rdf:resource="http://nlpkg.sebis.cit.tum.de/nlp-taxonomy.owl#Language_Models"/>
        <survey>https://aclanthology.org/2022.cl-1.7</survey>
        <survey>https://arxiv.org/abs/2310.16570</survey>
        <nlp-taxonomy:level rdf:datatype="http://www.w3.org/2001/XMLSchema#integer">3</nlp-taxonomy:level>
        <dcterms:description xml:lang="en">Probing refers to the process of investigating and understanding what kind of information a trained language model has learned. It involves creating tasks or tests that can reveal the model&apos;s knowledge about specific linguistic phenomena or its ability to perform certain tasks. The goal is to gain insights into the model&apos;s internal representations and understand its capabilities and limitations.</dcterms:description>
        <oboInOwl:hasSynonym xml:lang="en">Knowledge Probing</oboInOwl:hasSynonym>
        <oboInOwl:hasSynonym xml:lang="en">Language Model Probing</oboInOwl:hasSynonym>
        <rdfs:label xml:lang="en">Probing</rdfs:label>
    </owl:NamedIndividual>
    


    <!-- http://nlpkg.sebis.cit.tum.de/nlp-fos-hierarchy.owl#Profanity_Obfuscation -->

    <owl:NamedIndividual rdf:about="http://nlpkg.sebis.cit.tum.de/nlp-fos-hierarchy.owl#Profanity_Obfuscation">
        <rdf:type rdf:resource="http://nlpkg.sebis.cit.tum.de/nlp-fos-hierarchy.owl#Task"/>
        <rdf:type rdf:resource="http://nlpkg.sebis.cit.tum.de/nlp-taxonomy.owl#FieldOfStudy"/>
        <nlp-taxonomy:subFieldOf rdf:resource="http://nlpkg.sebis.cit.tum.de/nlp-fos-hierarchy.owl#Obfuscation"/>
        <survey>https://aclanthology.org/2023.findings-acl.240</survey>
        <nlp-taxonomy:level rdf:datatype="http://www.w3.org/2001/XMLSchema#integer">5</nlp-taxonomy:level>
        <dcterms:description xml:lang="en">Profanity Obfuscation refers to the process of masking or altering offensive or inappropriate words in a text. This is often done to maintain the decency of content, prevent offensive language, and ensure that the content is suitable for all audiences. Techniques used may include replacing letters with symbols, removing the word entirely, or replacing it with a less offensive synonym.</dcterms:description>
        <rdfs:label xml:lang="en">Profanity Obfuscation</rdfs:label>
    </owl:NamedIndividual>
    


    <!-- http://nlpkg.sebis.cit.tum.de/nlp-fos-hierarchy.owl#Prompt_Hacking -->

    <owl:NamedIndividual rdf:about="http://nlpkg.sebis.cit.tum.de/nlp-fos-hierarchy.owl#Prompt_Hacking">
        <rdf:type rdf:resource="http://nlpkg.sebis.cit.tum.de/nlp-fos-hierarchy.owl#Task"/>
        <rdf:type rdf:resource="http://nlpkg.sebis.cit.tum.de/nlp-taxonomy.owl#FieldOfStudy"/>
        <nlp-taxonomy:subFieldOf rdf:resource="http://nlpkg.sebis.cit.tum.de/nlp-fos-hierarchy.owl#Privacy,_Security_&amp;_Safety_in_NLP"/>
        <nlp-taxonomy:subFieldOf rdf:resource="http://nlpkg.sebis.cit.tum.de/nlp-fos-hierarchy.owl#Prompting,_Prompt_Learning_&amp;_Prompt_Engineering"/>
        <nlp-taxonomy:superFieldOf rdf:resource="http://nlpkg.sebis.cit.tum.de/nlp-fos-hierarchy.owl#Prompt_Injection"/>
        <nlp-taxonomy:superFieldOf rdf:resource="http://nlpkg.sebis.cit.tum.de/nlp-fos-hierarchy.owl#Prompt_Injection_Defense"/>
        <relevantInformation>https://learnprompting.org/docs/prompt_hacking/intro</relevantInformation>
        <survey>https://arxiv.org/abs/2305.13860</survey>
        <survey>https://arxiv.org/abs/2305.14965</survey>
        <nlp-taxonomy:level rdf:datatype="http://www.w3.org/2001/XMLSchema#integer">4</nlp-taxonomy:level>
        <dcterms:description xml:lang="en">Prompt Hacking describes a type of attack that exploits the vulnerabilities of large language models, by manipulating their inputs or prompts. Unlike traditional hacking, which typically exploits software vulnerabilities, prompt hacking relies on carefully crafting prompts to deceive the large language models into performing unintended actions.</dcterms:description>
        <rdfs:label xml:lang="en">Prompt Hacking</rdfs:label>
    </owl:NamedIndividual>
    


    <!-- http://nlpkg.sebis.cit.tum.de/nlp-fos-hierarchy.owl#Prompt_Injection -->

    <owl:NamedIndividual rdf:about="http://nlpkg.sebis.cit.tum.de/nlp-fos-hierarchy.owl#Prompt_Injection">
        <rdf:type rdf:resource="http://nlpkg.sebis.cit.tum.de/nlp-fos-hierarchy.owl#Task"/>
        <rdf:type rdf:resource="http://nlpkg.sebis.cit.tum.de/nlp-taxonomy.owl#FieldOfStudy"/>
        <nlp-taxonomy:subFieldOf rdf:resource="http://nlpkg.sebis.cit.tum.de/nlp-fos-hierarchy.owl#Prompt_Hacking"/>
        <nlp-taxonomy:superFieldOf rdf:resource="http://nlpkg.sebis.cit.tum.de/nlp-fos-hierarchy.owl#Adversarial_Prompting"/>
        <nlp-taxonomy:superFieldOf rdf:resource="http://nlpkg.sebis.cit.tum.de/nlp-fos-hierarchy.owl#Goal_Hijacking"/>
        <relevantInformation>https://learnprompting.org/docs/prompt_hacking/injection</relevantInformation>
        <survey>https://arxiv.org/abs/2302.05733</survey>
        <survey>https://arxiv.org/abs/2302.12173</survey>
        <survey>https://arxiv.org/abs/2306.05499</survey>
        <nlp-taxonomy:level rdf:datatype="http://www.w3.org/2001/XMLSchema#integer">4</nlp-taxonomy:level>
        <nlp-taxonomy:level rdf:datatype="http://www.w3.org/2001/XMLSchema#integer">5</nlp-taxonomy:level>
        <dcterms:description xml:lang="en">Prompt Injection refers to manipulating the language model’s output via engineered malicious prompts. This enables hackers to override original instructions and employed controls.</dcterms:description>
        <oboInOwl:hasSynonym xml:lang="en">PI</oboInOwl:hasSynonym>
        <oboInOwl:hasSynonym xml:lang="en">Prompt Injection Attack</oboInOwl:hasSynonym>
        <rdfs:label xml:lang="en">Prompt Injection</rdfs:label>
    </owl:NamedIndividual>
    


    <!-- http://nlpkg.sebis.cit.tum.de/nlp-fos-hierarchy.owl#Prompt_Injection_Defense -->

    <owl:NamedIndividual rdf:about="http://nlpkg.sebis.cit.tum.de/nlp-fos-hierarchy.owl#Prompt_Injection_Defense">
        <rdf:type rdf:resource="http://nlpkg.sebis.cit.tum.de/nlp-fos-hierarchy.owl#Task"/>
        <rdf:type rdf:resource="http://nlpkg.sebis.cit.tum.de/nlp-taxonomy.owl#FieldOfStudy"/>
        <nlp-taxonomy:subFieldOf rdf:resource="http://nlpkg.sebis.cit.tum.de/nlp-fos-hierarchy.owl#Prompt_Hacking"/>
        <relevantInformation>https://learnprompting.org/docs/category/-defensive-measures</relevantInformation>
        <survey>https://arxiv.org/abs/2210.07321</survey>
        <nlp-taxonomy:level rdf:datatype="http://www.w3.org/2001/XMLSchema#integer">4</nlp-taxonomy:level>
        <nlp-taxonomy:level rdf:datatype="http://www.w3.org/2001/XMLSchema#integer">5</nlp-taxonomy:level>
        <dcterms:description xml:lang="en">Prompt Injection Defense is the process of preventing prompt injection attacks.</dcterms:description>
        <rdfs:label xml:lang="en">Prompt Injection Defense</rdfs:label>
    </owl:NamedIndividual>
    


    <!-- http://nlpkg.sebis.cit.tum.de/nlp-fos-hierarchy.owl#Prompt_Optimization -->

    <owl:NamedIndividual rdf:about="http://nlpkg.sebis.cit.tum.de/nlp-fos-hierarchy.owl#Prompt_Optimization">
        <rdf:type rdf:resource="http://nlpkg.sebis.cit.tum.de/nlp-fos-hierarchy.owl#Task"/>
        <rdf:type rdf:resource="http://nlpkg.sebis.cit.tum.de/nlp-taxonomy.owl#FieldOfStudy"/>
        <nlp-taxonomy:subFieldOf rdf:resource="http://nlpkg.sebis.cit.tum.de/nlp-fos-hierarchy.owl#Prompting,_Prompt_Learning_&amp;_Prompt_Engineering"/>
        <nlp-taxonomy:superFieldOf rdf:resource="http://nlpkg.sebis.cit.tum.de/nlp-fos-hierarchy.owl#Hard_Prompts"/>
        <nlp-taxonomy:superFieldOf rdf:resource="http://nlpkg.sebis.cit.tum.de/nlp-fos-hierarchy.owl#Soft_Prompts"/>
        <nlp-taxonomy:level rdf:datatype="http://www.w3.org/2001/XMLSchema#integer">4</nlp-taxonomy:level>
        <dcterms:description xml:lang="en">Prompt Optimization or Prompt Search refers to the process of fine-tuning the input or &quot;prompt&quot; given to a language model to improve its output. This can involve adjusting the phrasing, adding specific instructions, or using other techniques to guide the model towards generating more accurate, relevant, or creative responses. It&apos;s a way to control and enhance the performance of language models without modifying their internal parameters.</dcterms:description>
        <oboInOwl:hasSynonym xml:lang="en">Prompt Search</oboInOwl:hasSynonym>
        <rdfs:label xml:lang="en">Prompt Optimization</rdfs:label>
    </owl:NamedIndividual>
    


    <!-- http://nlpkg.sebis.cit.tum.de/nlp-fos-hierarchy.owl#Pronominal_Anaphora_Resolution -->

    <owl:NamedIndividual rdf:about="http://nlpkg.sebis.cit.tum.de/nlp-fos-hierarchy.owl#Pronominal_Anaphora_Resolution">
        <rdf:type rdf:resource="http://nlpkg.sebis.cit.tum.de/nlp-fos-hierarchy.owl#Task"/>
        <rdf:type rdf:resource="http://nlpkg.sebis.cit.tum.de/nlp-taxonomy.owl#FieldOfStudy"/>
        <nlp-taxonomy:subFieldOf rdf:resource="http://nlpkg.sebis.cit.tum.de/nlp-fos-hierarchy.owl#Anaphora_Resolution"/>
        <nlp-taxonomy:level rdf:datatype="http://www.w3.org/2001/XMLSchema#integer">4</nlp-taxonomy:level>
        <dcterms:description xml:lang="en">Pronominal Anaphora Resolution refers to the process of determining the correct antecedent of a pronoun in a given text. Anaphora is a linguistic term that refers to the use of pronouns or other words to refer back to previously mentioned entities in a text. The resolution part involves correctly linking these pronouns to their intended referents, which is crucial for understanding the meaning of the text.</dcterms:description>
        <rdfs:label xml:lang="en">Pronominal Anaphora Resolution</rdfs:label>
    </owl:NamedIndividual>
    


    <!-- http://nlpkg.sebis.cit.tum.de/nlp-fos-hierarchy.owl#Propaganda_Detection -->

    <owl:NamedIndividual rdf:about="http://nlpkg.sebis.cit.tum.de/nlp-fos-hierarchy.owl#Propaganda_Detection">
        <rdf:type rdf:resource="http://nlpkg.sebis.cit.tum.de/nlp-fos-hierarchy.owl#Task"/>
        <rdf:type rdf:resource="http://nlpkg.sebis.cit.tum.de/nlp-taxonomy.owl#FieldOfStudy"/>
        <nlp-taxonomy:subFieldOf rdf:resource="http://nlpkg.sebis.cit.tum.de/nlp-taxonomy.owl#Ethical_NLP"/>
        <nlp-taxonomy:subFieldOf rdf:resource="http://nlpkg.sebis.cit.tum.de/nlp-taxonomy.owl#Text_Classification"/>
        <survey>https://arxiv.org/abs/2007.08024</survey>
        <nlp-taxonomy:level rdf:datatype="http://www.w3.org/2001/XMLSchema#integer">3</nlp-taxonomy:level>
        <dcterms:description xml:lang="en">Propaganda Detection aims at identifying and analyzing the use of persuasive or manipulative techniques in text, with the goal of recognizing content that aims to spread biased or misleading information, often for political or ideological purposes.</dcterms:description>
        <oboInOwl:hasSynonym xml:lang="en">Propaganda Classification</oboInOwl:hasSynonym>
        <oboInOwl:hasSynonym xml:lang="en">Propaganda Identification</oboInOwl:hasSynonym>
        <rdfs:label xml:lang="en">Propaganda Detection</rdfs:label>
    </owl:NamedIndividual>
    


    <!-- http://nlpkg.sebis.cit.tum.de/nlp-fos-hierarchy.owl#Pseudonymization -->

    <owl:NamedIndividual rdf:about="http://nlpkg.sebis.cit.tum.de/nlp-fos-hierarchy.owl#Pseudonymization">
        <rdf:type rdf:resource="http://nlpkg.sebis.cit.tum.de/nlp-fos-hierarchy.owl#Task"/>
        <rdf:type rdf:resource="http://nlpkg.sebis.cit.tum.de/nlp-taxonomy.owl#FieldOfStudy"/>
        <nlp-taxonomy:subFieldOf rdf:resource="http://nlpkg.sebis.cit.tum.de/nlp-fos-hierarchy.owl#De-Identification"/>
        <nlp-taxonomy:level rdf:datatype="http://www.w3.org/2001/XMLSchema#integer">5</nlp-taxonomy:level>
        <dcterms:description xml:lang="en">Pseudonymization is the task of replacing personally identifiable information (PII) in such a way that it can be re-identified with the help of an identifier (additional information).</dcterms:description>
        <oboInOwl:hasSynonym xml:lang="en">Pseudonymisation</oboInOwl:hasSynonym>
        <rdfs:label xml:lang="en">Pseudonymization</rdfs:label>
    </owl:NamedIndividual>
    


    <!-- http://nlpkg.sebis.cit.tum.de/nlp-fos-hierarchy.owl#Quantization_Aware_Training -->

    <owl:NamedIndividual rdf:about="http://nlpkg.sebis.cit.tum.de/nlp-fos-hierarchy.owl#Quantization_Aware_Training">
        <rdf:type rdf:resource="http://nlpkg.sebis.cit.tum.de/nlp-fos-hierarchy.owl#Task"/>
        <rdf:type rdf:resource="http://nlpkg.sebis.cit.tum.de/nlp-taxonomy.owl#FieldOfStudy"/>
        <nlp-taxonomy:subFieldOf rdf:resource="http://nlpkg.sebis.cit.tum.de/nlp-fos-hierarchy.owl#Language_Model_Quantization"/>
        <nlp-taxonomy:level rdf:datatype="http://www.w3.org/2001/XMLSchema#integer">4</nlp-taxonomy:level>
        <nlp-taxonomy:level rdf:datatype="http://www.w3.org/2001/XMLSchema#integer">5</nlp-taxonomy:level>
        <dcterms:description xml:lang="en">Quantization Aware Training means training the model from the start using quantized weights and activations. Quantization is done in the model training process rather than after the fact, which can result in higher accuracy than post-training quantization.</dcterms:description>
        <oboInOwl:hasSynonym xml:lang="en">QAT</oboInOwl:hasSynonym>
        <oboInOwl:hasSynonym xml:lang="en">Quant-Aware Training</oboInOwl:hasSynonym>
        <rdfs:label xml:lang="en">Quantization Aware Training</rdfs:label>
    </owl:NamedIndividual>
    


    <!-- http://nlpkg.sebis.cit.tum.de/nlp-fos-hierarchy.owl#Query_Expansion -->

    <owl:NamedIndividual rdf:about="http://nlpkg.sebis.cit.tum.de/nlp-fos-hierarchy.owl#Query_Expansion">
        <rdf:type rdf:resource="http://nlpkg.sebis.cit.tum.de/nlp-fos-hierarchy.owl#Task"/>
        <rdf:type rdf:resource="http://nlpkg.sebis.cit.tum.de/nlp-taxonomy.owl#FieldOfStudy"/>
        <nlp-taxonomy:subFieldOf rdf:resource="http://nlpkg.sebis.cit.tum.de/nlp-taxonomy.owl#Semantic_Search"/>
        <relevantInformation>https://nlp.stanford.edu/IR-book/html/htmledition/query-expansion-1.html</relevantInformation>
        <survey>https://arxiv.org/abs/1708.00247</survey>
        <survey>https://arxiv.org/abs/2309.08541</survey>
        <nlp-taxonomy:level rdf:datatype="http://www.w3.org/2001/XMLSchema#integer">3</nlp-taxonomy:level>
        <dcterms:description xml:lang="en">Query Expansion is used to improve the accuracy of information retrieval systems. It involves expanding the initial search query by adding synonyms, misspellings, alternative spellings, and related words to the original query. This helps in retrieving more relevant documents, even if they don&apos;t contain the exact original search terms.</dcterms:description>
        <rdfs:label xml:lang="en">Query Expansion</rdfs:label>
    </owl:NamedIndividual>
    


    <!-- http://nlpkg.sebis.cit.tum.de/nlp-fos-hierarchy.owl#Query_Representation -->

    <owl:NamedIndividual rdf:about="http://nlpkg.sebis.cit.tum.de/nlp-fos-hierarchy.owl#Query_Representation">
        <rdf:type rdf:resource="http://nlpkg.sebis.cit.tum.de/nlp-fos-hierarchy.owl#OtherScientificField"/>
        <rdf:type rdf:resource="http://nlpkg.sebis.cit.tum.de/nlp-taxonomy.owl#FieldOfStudy"/>
        <nlp-taxonomy:subFieldOf rdf:resource="http://nlpkg.sebis.cit.tum.de/nlp-taxonomy.owl#Document_Retrieval"/>
        <nlp-taxonomy:subFieldOf rdf:resource="http://nlpkg.sebis.cit.tum.de/nlp-taxonomy.owl#Passage_Retrieval"/>
        <nlp-taxonomy:level rdf:datatype="http://www.w3.org/2001/XMLSchema#integer">3</nlp-taxonomy:level>
        <dcterms:description xml:lang="en">Query Representation refers to the process of transforming a user&apos;s information need into a suitable format or structure that can be processed by the retrieval system. The goal is to create a query that accurately represents the user&apos;s information need and can effectively retrieve relevant results from the database.</dcterms:description>
        <rdfs:label xml:lang="en">Query Representation</rdfs:label>
    </owl:NamedIndividual>
    


    <!-- http://nlpkg.sebis.cit.tum.de/nlp-fos-hierarchy.owl#Question_Classification -->

    <owl:NamedIndividual rdf:about="http://nlpkg.sebis.cit.tum.de/nlp-fos-hierarchy.owl#Question_Classification">
        <rdf:type rdf:resource="http://nlpkg.sebis.cit.tum.de/nlp-fos-hierarchy.owl#Task"/>
        <rdf:type rdf:resource="http://nlpkg.sebis.cit.tum.de/nlp-taxonomy.owl#FieldOfStudy"/>
        <nlp-taxonomy:subFieldOf rdf:resource="http://nlpkg.sebis.cit.tum.de/nlp-taxonomy.owl#Question_Answering"/>
        <nlp-taxonomy:subFieldOf rdf:resource="http://nlpkg.sebis.cit.tum.de/nlp-taxonomy.owl#Text_Classification"/>
        <survey>https://aclanthology.org/2020.lrec-1.665</survey>
        <nlp-taxonomy:level rdf:datatype="http://www.w3.org/2001/XMLSchema#integer">3</nlp-taxonomy:level>
        <dcterms:description xml:lang="en">Question Classification (QC) refers to the task of categorizing questions into predefined classes. It is a crucial step in question answering systems where understanding the type of question can help in determining the kind of answer required. For example, a &quot;who&quot; question requires a person as an answer, while a &quot;where&quot; question requires a location.</dcterms:description>
        <oboInOwl:hasSynonym xml:lang="en">QC</oboInOwl:hasSynonym>
        <rdfs:label xml:lang="en">Question Classification</rdfs:label>
    </owl:NamedIndividual>
    


    <!-- http://nlpkg.sebis.cit.tum.de/nlp-fos-hierarchy.owl#Race_Bias -->

    <owl:NamedIndividual rdf:about="http://nlpkg.sebis.cit.tum.de/nlp-fos-hierarchy.owl#Race_Bias">
        <rdf:type rdf:resource="http://nlpkg.sebis.cit.tum.de/nlp-fos-hierarchy.owl#OtherScientificField"/>
        <rdf:type rdf:resource="http://nlpkg.sebis.cit.tum.de/nlp-taxonomy.owl#FieldOfStudy"/>
        <nlp-taxonomy:subFieldOf rdf:resource="http://nlpkg.sebis.cit.tum.de/nlp-fos-hierarchy.owl#Social_Bias"/>
        <survey>https://aclanthology.org/2021.acl-long.149</survey>
        <nlp-taxonomy:level rdf:datatype="http://www.w3.org/2001/XMLSchema#integer">5</nlp-taxonomy:level>
        <dcterms:description xml:lang="en">Race Bias, also known as Racial Bias, refers to the prejudiced attitudes, beliefs, or actions that an individual or institution holds towards a particular race or racial group.</dcterms:description>
        <oboInOwl:hasSynonym xml:lang="en">Racial Bias</oboInOwl:hasSynonym>
        <rdfs:label xml:lang="en">Race Bias</rdfs:label>
    </owl:NamedIndividual>
    


    <!-- http://nlpkg.sebis.cit.tum.de/nlp-fos-hierarchy.owl#Recurrent_Neural_Network -->

    <owl:NamedIndividual rdf:about="http://nlpkg.sebis.cit.tum.de/nlp-fos-hierarchy.owl#Recurrent_Neural_Network">
        <rdf:type rdf:resource="http://nlpkg.sebis.cit.tum.de/nlp-fos-hierarchy.owl#Method"/>
        <rdf:type rdf:resource="http://nlpkg.sebis.cit.tum.de/nlp-taxonomy.owl#FieldOfStudy"/>
        <nlp-taxonomy:subFieldOf rdf:resource="http://nlpkg.sebis.cit.tum.de/nlp-taxonomy.owl#Language_Models"/>
        <relevantInformation>https://web.stanford.edu/~jurafsky/slp3/9.pdf</relevantInformation>
        <survey>https://arxiv.org/abs/2304.11461</survey>
        <nlp-taxonomy:level rdf:datatype="http://www.w3.org/2001/XMLSchema#integer">3</nlp-taxonomy:level>
        <dcterms:description xml:lang="en">A Recurrent Neural Network (RNN) is a type of artificial neural network designed to recognize patterns in sequences of data, such as text, genomes, handwriting, or spoken words. Unlike traditional neural networks, RNNs have loops, allowing information to persist, which makes them ideal for processing sequences. They are called recurrent because they perform the same task for every element of a sequence, with the output being dependent on the previous computations.</dcterms:description>
        <oboInOwl:hasSynonym xml:lang="en">RNN</oboInOwl:hasSynonym>
        <rdfs:label xml:lang="en">Recurrent Neural Network</rdfs:label>
    </owl:NamedIndividual>
    


    <!-- http://nlpkg.sebis.cit.tum.de/nlp-fos-hierarchy.owl#Referring_Expression_Comprehension -->

    <owl:NamedIndividual rdf:about="http://nlpkg.sebis.cit.tum.de/nlp-fos-hierarchy.owl#Referring_Expression_Comprehension">
        <rdf:type rdf:resource="http://nlpkg.sebis.cit.tum.de/nlp-fos-hierarchy.owl#Task"/>
        <rdf:type rdf:resource="http://nlpkg.sebis.cit.tum.de/nlp-taxonomy.owl#FieldOfStudy"/>
        <nlp-taxonomy:subFieldOf rdf:resource="http://nlpkg.sebis.cit.tum.de/nlp-taxonomy.owl#Visual_Data_In_NLP"/>
        <survey>https://arxiv.org/abs/2007.09554</survey>
        <nlp-taxonomy:level rdf:datatype="http://www.w3.org/2001/XMLSchema#integer">3</nlp-taxonomy:level>
        <dcterms:description xml:lang="en">Referring Expression Comprehension (REC) aims to localize a target object in an image described by a referring expression phrased in natural language.</dcterms:description>
        <oboInOwl:hasSynonym xml:lang="en">REC</oboInOwl:hasSynonym>
        <rdfs:label xml:lang="en">Referring Expression Comprehension</rdfs:label>
    </owl:NamedIndividual>
    


    <!-- http://nlpkg.sebis.cit.tum.de/nlp-fos-hierarchy.owl#Regularization -->

    <owl:NamedIndividual rdf:about="http://nlpkg.sebis.cit.tum.de/nlp-fos-hierarchy.owl#Regularization">
        <rdf:type rdf:resource="http://nlpkg.sebis.cit.tum.de/nlp-fos-hierarchy.owl#Task"/>
        <rdf:type rdf:resource="http://nlpkg.sebis.cit.tum.de/nlp-taxonomy.owl#FieldOfStudy"/>
        <nlp-taxonomy:subFieldOf rdf:resource="http://nlpkg.sebis.cit.tum.de/nlp-fos-hierarchy.owl#Language_Model_Mechanisms"/>
        <relevantInformation>https://towardsdatascience.com/regularization-in-deep-learning-l1-l2-and-dropout-377e75acc036</relevantInformation>
        <survey>https://www.deeplearningbook.org/contents/regularization.html</survey>
        <nlp-taxonomy:level rdf:datatype="http://www.w3.org/2001/XMLSchema#integer">4</nlp-taxonomy:level>
        <dcterms:description xml:lang="en">Regularization is a technique used to prevent overfitting in deep learning models. This helps to ensure that the model generalizes well to unseen data, improving its overall performance and accuracy.</dcterms:description>
        <rdfs:label xml:lang="en">Regularization</rdfs:label>
    </owl:NamedIndividual>
    


    <!-- http://nlpkg.sebis.cit.tum.de/nlp-fos-hierarchy.owl#Reinforcement_Learning -->

    <owl:NamedIndividual rdf:about="http://nlpkg.sebis.cit.tum.de/nlp-fos-hierarchy.owl#Reinforcement_Learning">
        <rdf:type rdf:resource="http://nlpkg.sebis.cit.tum.de/nlp-fos-hierarchy.owl#Task"/>
        <rdf:type rdf:resource="http://nlpkg.sebis.cit.tum.de/nlp-taxonomy.owl#FieldOfStudy"/>
        <nlp-taxonomy:subFieldOf rdf:resource="http://nlpkg.sebis.cit.tum.de/nlp-taxonomy.owl#Low-Resource_NLP"/>
        <code>https://github.com/huggingface/trl</code>
        <survey>https://arxiv.org/abs/1906.03926</survey>
        <survey>https://arxiv.org/abs/2104.05565</survey>
        <survey>https://arxiv.org/abs/2210.13623</survey>
        <survey>https://arxiv.org/abs/2310.06147</survey>
        <nlp-taxonomy:level rdf:datatype="http://www.w3.org/2001/XMLSchema#integer">3</nlp-taxonomy:level>
        <dcterms:description xml:lang="en">Reinforcement Learning (RL) is a type of machine learning where an agent learns to make decisions by interacting with an environment. It receives feedback in the form of rewards or punishments based on its actions and uses this feedback to improve its decision-making over time.</dcterms:description>
        <oboInOwl:hasSynonym xml:lang="en">RL</oboInOwl:hasSynonym>
        <rdfs:label xml:lang="en">Reinforcement Learning</rdfs:label>
    </owl:NamedIndividual>
    


    <!-- http://nlpkg.sebis.cit.tum.de/nlp-fos-hierarchy.owl#Relation_Directionality_Classification -->

    <owl:NamedIndividual rdf:about="http://nlpkg.sebis.cit.tum.de/nlp-fos-hierarchy.owl#Relation_Directionality_Classification">
        <rdf:type rdf:resource="http://nlpkg.sebis.cit.tum.de/nlp-fos-hierarchy.owl#Task"/>
        <rdf:type rdf:resource="http://nlpkg.sebis.cit.tum.de/nlp-taxonomy.owl#FieldOfStudy"/>
        <usedFor rdf:resource="http://nlpkg.sebis.cit.tum.de/nlp-fos-hierarchy.owl#Discourse_Parsing"/>
        <nlp-taxonomy:subFieldOf rdf:resource="http://nlpkg.sebis.cit.tum.de/nlp-taxonomy.owl#Relation_Extraction"/>
        <nlp-taxonomy:level rdf:datatype="http://www.w3.org/2001/XMLSchema#integer">3</nlp-taxonomy:level>
        <nlp-taxonomy:level rdf:datatype="http://www.w3.org/2001/XMLSchema#integer">4</nlp-taxonomy:level>
        <nlp-taxonomy:level rdf:datatype="http://www.w3.org/2001/XMLSchema#integer">8</nlp-taxonomy:level>
        <dcterms:description xml:lang="en">Relation Directionality Classification refers to the task of determining the direction of a relationship or interaction between entities mentioned in text. It involves classifying whether one entity is the subject performing an action on another entity (e.g., &quot;A is the parent of B&quot;) or vice versa (e.g., &quot;B is the child of A&quot;). This classification is essential for understanding the semantics and context of textual data.</dcterms:description>
        <rdfs:label xml:lang="en">Relation Directionality Classification</rdfs:label>
    </owl:NamedIndividual>
    


    <!-- http://nlpkg.sebis.cit.tum.de/nlp-fos-hierarchy.owl#Relation_Linking -->

    <owl:NamedIndividual rdf:about="http://nlpkg.sebis.cit.tum.de/nlp-fos-hierarchy.owl#Relation_Linking">
        <rdf:type rdf:resource="http://nlpkg.sebis.cit.tum.de/nlp-fos-hierarchy.owl#Task"/>
        <rdf:type rdf:resource="http://nlpkg.sebis.cit.tum.de/nlp-taxonomy.owl#FieldOfStudy"/>
        <nlp-taxonomy:subFieldOf rdf:resource="http://nlpkg.sebis.cit.tum.de/nlp-fos-hierarchy.owl#Knowledge_Graph_Construction_&amp;_Completion"/>
        <nlp-taxonomy:level rdf:datatype="http://www.w3.org/2001/XMLSchema#integer">7</nlp-taxonomy:level>
        <dcterms:description xml:lang="en">Relation Linking refers to the process of identifying the relations in a text and mapping them to the corresponding relations in a knowledge base.</dcterms:description>
        <rdfs:label xml:lang="en">Relation Linking</rdfs:label>
    </owl:NamedIndividual>
    


    <!-- http://nlpkg.sebis.cit.tum.de/nlp-fos-hierarchy.owl#Retrieval-based_Dialogue_Response_Generation -->

    <owl:NamedIndividual rdf:about="http://nlpkg.sebis.cit.tum.de/nlp-fos-hierarchy.owl#Retrieval-based_Dialogue_Response_Generation">
        <rdf:type rdf:resource="http://nlpkg.sebis.cit.tum.de/nlp-fos-hierarchy.owl#Task"/>
        <rdf:type rdf:resource="http://nlpkg.sebis.cit.tum.de/nlp-taxonomy.owl#FieldOfStudy"/>
        <uses rdf:resource="http://nlpkg.sebis.cit.tum.de/nlp-taxonomy.owl#Information_Retrieval"/>
        <nlp-taxonomy:subFieldOf rdf:resource="http://nlpkg.sebis.cit.tum.de/nlp-taxonomy.owl#Dialogue_Response_Generation"/>
        <nlp-taxonomy:level rdf:datatype="http://www.w3.org/2001/XMLSchema#integer">3</nlp-taxonomy:level>
        <nlp-taxonomy:level rdf:datatype="http://www.w3.org/2001/XMLSchema#integer">4</nlp-taxonomy:level>
        <dcterms:description xml:lang="en">Retrieval-based Dialogue Response Generation generates responses by selecting pre-existing responses from a predefined set of options or a database. It relies on retrieving the most appropriate response based on the input query or user message.</dcterms:description>
        <rdfs:label xml:lang="en">Retrieval-based Dialogue Response Generation</rdfs:label>
    </owl:NamedIndividual>
    


    <!-- http://nlpkg.sebis.cit.tum.de/nlp-fos-hierarchy.owl#Retrieval-based_Question_Answering -->

    <owl:NamedIndividual rdf:about="http://nlpkg.sebis.cit.tum.de/nlp-fos-hierarchy.owl#Retrieval-based_Question_Answering">
        <rdf:type rdf:resource="http://nlpkg.sebis.cit.tum.de/nlp-fos-hierarchy.owl#Task"/>
        <rdf:type rdf:resource="http://nlpkg.sebis.cit.tum.de/nlp-taxonomy.owl#FieldOfStudy"/>
        <uses rdf:resource="http://nlpkg.sebis.cit.tum.de/nlp-taxonomy.owl#Information_Retrieval"/>
        <nlp-taxonomy:subFieldOf rdf:resource="http://nlpkg.sebis.cit.tum.de/nlp-taxonomy.owl#Question_Answering"/>
        <nlp-taxonomy:superFieldOf rdf:resource="http://nlpkg.sebis.cit.tum.de/nlp-fos-hierarchy.owl#Retrieval_Augmented_Generation"/>
        <relevantInformation>https://web.stanford.edu/~jurafsky/slp3/14.pdf</relevantInformation>
        <nlp-taxonomy:level rdf:datatype="http://www.w3.org/2001/XMLSchema#integer">3</nlp-taxonomy:level>
        <dcterms:description xml:lang="en">Retrieval-based Question Answering is a technique where a system selects the most appropriate answer from a predefined set of responses or a larger corpus of text based on the input question. It typically involves matching the question with candidate answers and selecting the one that best matches the query using various similarity or ranking methods.</dcterms:description>
        <oboInOwl:hasSynonym xml:lang="en">Retrieval-based QA</oboInOwl:hasSynonym>
        <rdfs:label xml:lang="en">Retrieval-based Question Answering</rdfs:label>
    </owl:NamedIndividual>
    


    <!-- http://nlpkg.sebis.cit.tum.de/nlp-fos-hierarchy.owl#Retrieval_Augmented_Generation -->

    <owl:NamedIndividual rdf:about="http://nlpkg.sebis.cit.tum.de/nlp-fos-hierarchy.owl#Retrieval_Augmented_Generation">
        <rdf:type rdf:resource="http://nlpkg.sebis.cit.tum.de/nlp-fos-hierarchy.owl#Task"/>
        <rdf:type rdf:resource="http://nlpkg.sebis.cit.tum.de/nlp-taxonomy.owl#FieldOfStudy"/>
        <usedFor rdf:resource="http://nlpkg.sebis.cit.tum.de/nlp-fos-hierarchy.owl#Knowledge_Base_Question_Answering"/>
        <uses rdf:resource="http://nlpkg.sebis.cit.tum.de/nlp-taxonomy.owl#Document_Retrieval"/>
        <uses rdf:resource="http://nlpkg.sebis.cit.tum.de/nlp-taxonomy.owl#Passage_Retrieval"/>
        <uses rdf:resource="http://nlpkg.sebis.cit.tum.de/nlp-taxonomy.owl#Text_Generation"/>
        <nlp-taxonomy:subFieldOf rdf:resource="http://nlpkg.sebis.cit.tum.de/nlp-fos-hierarchy.owl#Generative_Question_Answering"/>
        <nlp-taxonomy:subFieldOf rdf:resource="http://nlpkg.sebis.cit.tum.de/nlp-fos-hierarchy.owl#Retrieval-based_Question_Answering"/>
        <origin>https://arxiv.org/abs/2005.11401</origin>
        <relevantInformation>https://ai.meta.com/blog/retrieval-augmented-generation-streamlining-the-creation-of-intelligent-natural-language-processing-models/</relevantInformation>
        <relevantInformation>https://python.langchain.com/docs/use_cases/question_answering/</relevantInformation>
        <relevantInformation>https://www.promptingguide.ai/techniques/rag</relevantInformation>
        <survey>https://arxiv.org/abs/2202.01110</survey>
        <survey>https://arxiv.org/abs/2303.10868</survey>
        <survey>https://arxiv.org/abs/2312.10997</survey>
        <survey>https://arxiv.org/abs/2401.08406</survey>
        <nlp-taxonomy:level rdf:datatype="http://www.w3.org/2001/XMLSchema#integer">4</nlp-taxonomy:level>
        <dcterms:description xml:lang="en">Retrieval Augmented Generation (RAG) is a concept that combines two key components: retrieval and generation. It involves retrieving relevant information from a large dataset or knowledge base and then using that information to generate natural language text or responses based on that retrieved information. RAG models typically consist of a retrieval module and a generation module, allowing them to access external knowledge to enhance the quality and relevance of generated text.</dcterms:description>
        <oboInOwl:hasSynonym xml:lang="en">RAG</oboInOwl:hasSynonym>
        <rdfs:label xml:lang="en">Retrieval Augmented Generation</rdfs:label>
    </owl:NamedIndividual>
    


    <!-- http://nlpkg.sebis.cit.tum.de/nlp-fos-hierarchy.owl#Rhetorical_Structure_Theory -->

    <owl:NamedIndividual rdf:about="http://nlpkg.sebis.cit.tum.de/nlp-fos-hierarchy.owl#Rhetorical_Structure_Theory">
        <rdf:type rdf:resource="http://nlpkg.sebis.cit.tum.de/nlp-fos-hierarchy.owl#OtherScientificField"/>
        <rdf:type rdf:resource="http://nlpkg.sebis.cit.tum.de/nlp-taxonomy.owl#FieldOfStudy"/>
        <nlp-taxonomy:subFieldOf rdf:resource="http://nlpkg.sebis.cit.tum.de/nlp-taxonomy.owl#Linguistic_Theories"/>
        <nlp-taxonomy:superFieldOf rdf:resource="http://nlpkg.sebis.cit.tum.de/nlp-fos-hierarchy.owl#Rhetorical_Structure_Theory_Discourse_Parsing"/>
        <survey>https://aclanthology.org/2022.lrec-1.635</survey>
        <nlp-taxonomy:level rdf:datatype="http://www.w3.org/2001/XMLSchema#integer">3</nlp-taxonomy:level>
        <dcterms:description xml:lang="en">Rhetorical Structure Theory (RST) is a framework used to analyze and represent the structure of texts by identifying the relationships between different parts of the text. It helps in understanding how different sentences or phrases within a text are interconnected to form a coherent and meaningful whole.</dcterms:description>
        <oboInOwl:hasSynonym xml:lang="en">RST</oboInOwl:hasSynonym>
        <rdfs:label xml:lang="en">Rhetorical Structure Theory</rdfs:label>
    </owl:NamedIndividual>
    


    <!-- http://nlpkg.sebis.cit.tum.de/nlp-fos-hierarchy.owl#Rhetorical_Structure_Theory_Discourse_Parsing -->

    <owl:NamedIndividual rdf:about="http://nlpkg.sebis.cit.tum.de/nlp-fos-hierarchy.owl#Rhetorical_Structure_Theory_Discourse_Parsing">
        <rdf:type rdf:resource="http://nlpkg.sebis.cit.tum.de/nlp-fos-hierarchy.owl#Task"/>
        <rdf:type rdf:resource="http://nlpkg.sebis.cit.tum.de/nlp-taxonomy.owl#FieldOfStudy"/>
        <nlp-taxonomy:subFieldOf rdf:resource="http://nlpkg.sebis.cit.tum.de/nlp-fos-hierarchy.owl#Discourse_Parsing"/>
        <nlp-taxonomy:subFieldOf rdf:resource="http://nlpkg.sebis.cit.tum.de/nlp-fos-hierarchy.owl#Rhetorical_Structure_Theory"/>
        <nlp-taxonomy:superFieldOf rdf:resource="http://nlpkg.sebis.cit.tum.de/nlp-fos-hierarchy.owl#Elementary_Discourse_Unit"/>
        <nlp-taxonomy:superFieldOf rdf:resource="http://nlpkg.sebis.cit.tum.de/nlp-fos-hierarchy.owl#Rhetorical_Structure_Theory_Discourse_Tree"/>
        <nlp-taxonomy:level rdf:datatype="http://www.w3.org/2001/XMLSchema#integer">4</nlp-taxonomy:level>
        <dcterms:description xml:lang="en">Rhetorical Structure Theory (RST) Discourse Parsing aims to uncover the hierarchical and rhetorical structure of a text, such as how sentences and paragraphs are connected, through a well-defined tree structure.</dcterms:description>
        <oboInOwl:hasSynonym xml:lang="en">RST Discourse Parsing</oboInOwl:hasSynonym>
        <oboInOwl:hasSynonym xml:lang="en">RST-DP</oboInOwl:hasSynonym>
        <rdfs:label xml:lang="en">Rhetorical Structure Theory Discourse Parsing</rdfs:label>
    </owl:NamedIndividual>
    


    <!-- http://nlpkg.sebis.cit.tum.de/nlp-fos-hierarchy.owl#Rhetorical_Structure_Theory_Discourse_Tree -->

    <owl:NamedIndividual rdf:about="http://nlpkg.sebis.cit.tum.de/nlp-fos-hierarchy.owl#Rhetorical_Structure_Theory_Discourse_Tree">
        <rdf:type rdf:resource="http://nlpkg.sebis.cit.tum.de/nlp-fos-hierarchy.owl#DataStructure"/>
        <rdf:type rdf:resource="http://nlpkg.sebis.cit.tum.de/nlp-taxonomy.owl#FieldOfStudy"/>
        <uses rdf:resource="http://nlpkg.sebis.cit.tum.de/nlp-fos-hierarchy.owl#Elementary_Discourse_Unit"/>
        <nlp-taxonomy:subFieldOf rdf:resource="http://nlpkg.sebis.cit.tum.de/nlp-fos-hierarchy.owl#Rhetorical_Structure_Theory_Discourse_Parsing"/>
        <nlp-taxonomy:subFieldOf rdf:resource="http://nlpkg.sebis.cit.tum.de/nlp-fos-hierarchy.owl#Tree"/>
        <nlp-taxonomy:level rdf:datatype="http://www.w3.org/2001/XMLSchema#integer">5</nlp-taxonomy:level>
        <dcterms:description xml:lang="en">Rhetorical Structure Theory (RST) Discourse Tree refers to a representation of the hierarchical structure of a text&apos;s discourse or the way information is organized within a document. RST discourse trees break down a text into segments and show how these segments are related in terms of rhetorical relationships like &quot;cause-effect,&quot; &quot;contrast,&quot; &quot;explanation,&quot; etc. These trees help analyze and understand the flow of information and coherence within a document.</dcterms:description>
        <oboInOwl:hasSynonym xml:lang="en">RST Discourse Tree</oboInOwl:hasSynonym>
        <rdfs:label xml:lang="en">Rhetorical Structure Theory Discourse Tree</rdfs:label>
    </owl:NamedIndividual>
    


    <!-- http://nlpkg.sebis.cit.tum.de/nlp-fos-hierarchy.owl#Rule-based_Dialogue_Response_Generation -->

    <owl:NamedIndividual rdf:about="http://nlpkg.sebis.cit.tum.de/nlp-fos-hierarchy.owl#Rule-based_Dialogue_Response_Generation">
        <rdf:type rdf:resource="http://nlpkg.sebis.cit.tum.de/nlp-fos-hierarchy.owl#Task"/>
        <rdf:type rdf:resource="http://nlpkg.sebis.cit.tum.de/nlp-taxonomy.owl#FieldOfStudy"/>
        <nlp-taxonomy:subFieldOf rdf:resource="http://nlpkg.sebis.cit.tum.de/nlp-taxonomy.owl#Dialogue_Response_Generation"/>
        <nlp-taxonomy:level rdf:datatype="http://www.w3.org/2001/XMLSchema#integer">3</nlp-taxonomy:level>
        <nlp-taxonomy:level rdf:datatype="http://www.w3.org/2001/XMLSchema#integer">4</nlp-taxonomy:level>
        <dcterms:description xml:lang="en">Rule-based dialogue response generation is a method of generating responses in a conversation by using predefined rules and patterns. Instead of relying on machine learning or natural language processing models, it follows explicit instructions or conditions to determine how to respond to user inputs. This approach is often used when precise and deterministic responses are required in dialogue systems and conversational agents.</dcterms:description>
        <oboInOwl:hasSynonym xml:lang="en">Rule-based Dialog Response Generation</oboInOwl:hasSynonym>
        <rdfs:label xml:lang="en">Rule-based Dialogue Response Generation</rdfs:label>
    </owl:NamedIndividual>
    


    <!-- http://nlpkg.sebis.cit.tum.de/nlp-fos-hierarchy.owl#Rule-based_Machine_Translation -->

    <owl:NamedIndividual rdf:about="http://nlpkg.sebis.cit.tum.de/nlp-fos-hierarchy.owl#Rule-based_Machine_Translation">
        <rdf:type rdf:resource="http://nlpkg.sebis.cit.tum.de/nlp-fos-hierarchy.owl#Task"/>
        <rdf:type rdf:resource="http://nlpkg.sebis.cit.tum.de/nlp-taxonomy.owl#FieldOfStudy"/>
        <nlp-taxonomy:subFieldOf rdf:resource="http://nlpkg.sebis.cit.tum.de/nlp-taxonomy.owl#Machine_Translation"/>
        <nlp-taxonomy:level rdf:datatype="http://www.w3.org/2001/XMLSchema#integer">3</nlp-taxonomy:level>
        <dcterms:description xml:lang="en">Rule-based Machine Translation (RBMT) is a type of machine translation method that relies on sets of linguistic rules. These rules are used to transfer the syntactic structure of the source language into the target language. The rules are typically created by linguists and the system often includes a bilingual dictionary for word translation. RBMT can provide high accuracy for language pairs with similar grammatical structures, but it may struggle with languages that have very different syntax or grammar rules.</dcterms:description>
        <oboInOwl:hasSynonym xml:lang="en">RBMT</oboInOwl:hasSynonym>
        <rdfs:label xml:lang="en">Rule-based Machine Translation</rdfs:label>
    </owl:NamedIndividual>
    


    <!-- http://nlpkg.sebis.cit.tum.de/nlp-fos-hierarchy.owl#Rumor_Detection -->

    <owl:NamedIndividual rdf:about="http://nlpkg.sebis.cit.tum.de/nlp-fos-hierarchy.owl#Rumor_Detection">
        <rdf:type rdf:resource="http://nlpkg.sebis.cit.tum.de/nlp-fos-hierarchy.owl#Task"/>
        <rdf:type rdf:resource="http://nlpkg.sebis.cit.tum.de/nlp-taxonomy.owl#FieldOfStudy"/>
        <nlp-taxonomy:subFieldOf rdf:resource="http://nlpkg.sebis.cit.tum.de/nlp-fos-hierarchy.owl#Claim_Detection"/>
        <nlp-taxonomy:subFieldOf rdf:resource="http://nlpkg.sebis.cit.tum.de/nlp-taxonomy.owl#Text_Classification"/>
        <survey>https://aclanthology.org/D19-5008</survey>
        <survey>https://arxiv.org/abs/1704.00656</survey>
        <nlp-taxonomy:level rdf:datatype="http://www.w3.org/2001/XMLSchema#integer">3</nlp-taxonomy:level>
        <nlp-taxonomy:level rdf:datatype="http://www.w3.org/2001/XMLSchema#integer">4</nlp-taxonomy:level>
        <dcterms:description xml:lang="en">Rumor Detection refers to the task of identifying rumors from texts i.e. statements whose veracity is not quickly or ever confirmed, in utterances on social media platforms.</dcterms:description>
        <oboInOwl:hasSynonym xml:lang="en">Rumor Identification</oboInOwl:hasSynonym>
        <oboInOwl:hasSynonym xml:lang="en">Rumour Detection</oboInOwl:hasSynonym>
        <oboInOwl:hasSynonym xml:lang="en">Rumour Identification</oboInOwl:hasSynonym>
        <rdfs:label xml:lang="en">Rumor Detection</rdfs:label>
    </owl:NamedIndividual>
    


    <!-- http://nlpkg.sebis.cit.tum.de/nlp-fos-hierarchy.owl#Sanitization -->

    <owl:NamedIndividual rdf:about="http://nlpkg.sebis.cit.tum.de/nlp-fos-hierarchy.owl#Sanitization">
        <rdf:type rdf:resource="http://nlpkg.sebis.cit.tum.de/nlp-fos-hierarchy.owl#Task"/>
        <rdf:type rdf:resource="http://nlpkg.sebis.cit.tum.de/nlp-taxonomy.owl#FieldOfStudy"/>
        <usedFor rdf:resource="http://nlpkg.sebis.cit.tum.de/nlp-fos-hierarchy.owl#Anonymization"/>
        <nlp-taxonomy:subFieldOf rdf:resource="http://nlpkg.sebis.cit.tum.de/nlp-fos-hierarchy.owl#Privacy,_Security_&amp;_Safety_in_NLP"/>
        <nlp-taxonomy:level rdf:datatype="http://www.w3.org/2001/XMLSchema#integer">4</nlp-taxonomy:level>
        <dcterms:description xml:lang="en">Sanitization is the task of removing sensitive or private information from a document so that it may be distributed to a broader audience. In a naive way, this simply involves blackening out sensitive parts in texts.</dcterms:description>
        <oboInOwl:hasSynonym xml:lang="en">Redaction</oboInOwl:hasSynonym>
        <oboInOwl:hasSynonym xml:lang="en">Sanitisation</oboInOwl:hasSynonym>
        <rdfs:label xml:lang="en">Sanitization</rdfs:label>
    </owl:NamedIndividual>
    


    <!-- http://nlpkg.sebis.cit.tum.de/nlp-fos-hierarchy.owl#Sarcasm_Detection -->

    <owl:NamedIndividual rdf:about="http://nlpkg.sebis.cit.tum.de/nlp-fos-hierarchy.owl#Sarcasm_Detection">
        <rdf:type rdf:resource="http://nlpkg.sebis.cit.tum.de/nlp-fos-hierarchy.owl#Task"/>
        <rdf:type rdf:resource="http://nlpkg.sebis.cit.tum.de/nlp-taxonomy.owl#FieldOfStudy"/>
        <nlp-taxonomy:subFieldOf rdf:resource="http://nlpkg.sebis.cit.tum.de/nlp-taxonomy.owl#Stylistic_Analysis"/>
        <nlp-taxonomy:subFieldOf rdf:resource="http://nlpkg.sebis.cit.tum.de/nlp-taxonomy.owl#Text_Classification"/>
        <survey>https://arxiv.org/abs/1602.03426</survey>
        <survey>https://arxiv.org/abs/2107.02276</survey>
        <survey>https://arxiv.org/abs/2202.02516</survey>
        <survey>https://arxiv.org/abs/2209.06170</survey>
        <nlp-taxonomy:level rdf:datatype="http://www.w3.org/2001/XMLSchema#integer">3</nlp-taxonomy:level>
        <dcterms:description xml:lang="en">Sarcasm Detection refers to the ability of AI systems to identify and understand sarcasm in text. It&apos;s a challenging aspect of sentiment analysis, as sarcasm often involves expressing negative sentiments using positive words in a context, making it difficult for machines to interpret. This requires advanced NLP techniques, including understanding of context, tone, and often cultural or situational nuances.</dcterms:description>
        <oboInOwl:hasSynonym xml:lang="en">Sarcasm Analysis</oboInOwl:hasSynonym>
        <oboInOwl:hasSynonym xml:lang="en">Sarcasm Classification</oboInOwl:hasSynonym>
        <oboInOwl:hasSynonym xml:lang="en">Sarcasm Identification</oboInOwl:hasSynonym>
        <rdfs:label xml:lang="en">Sarcasm Detection</rdfs:label>
    </owl:NamedIndividual>
    


    <!-- http://nlpkg.sebis.cit.tum.de/nlp-fos-hierarchy.owl#Scene_Text_Recognition -->

    <owl:NamedIndividual rdf:about="http://nlpkg.sebis.cit.tum.de/nlp-fos-hierarchy.owl#Scene_Text_Recognition">
        <rdf:type rdf:resource="http://nlpkg.sebis.cit.tum.de/nlp-fos-hierarchy.owl#Task"/>
        <rdf:type rdf:resource="http://nlpkg.sebis.cit.tum.de/nlp-taxonomy.owl#FieldOfStudy"/>
        <nlp-taxonomy:subFieldOf rdf:resource="http://nlpkg.sebis.cit.tum.de/nlp-taxonomy.owl#Visual_Data_In_NLP"/>
        <nlp-taxonomy:level rdf:datatype="http://www.w3.org/2001/XMLSchema#integer">3</nlp-taxonomy:level>
        <dcterms:description xml:lang="en">Scene Text Recognition is a task that involves automatically identifying and localizing text within natural images or videos. The goal of scene text detection is to develop algorithms that can robustly detect and and label text with bounding boxes in uncontrolled and complex environments, such as street signs, billboards, or license plates.</dcterms:description>
        <oboInOwl:hasSynonym xml:lang="en">Scene Text Classification</oboInOwl:hasSynonym>
        <oboInOwl:hasSynonym xml:lang="en">Scene Text Detection</oboInOwl:hasSynonym>
        <oboInOwl:hasSynonym xml:lang="en">Scene Text Identification</oboInOwl:hasSynonym>
        <rdfs:label xml:lang="en">Scene Text Recognition</rdfs:label>
    </owl:NamedIndividual>
    


    <!-- http://nlpkg.sebis.cit.tum.de/nlp-fos-hierarchy.owl#Segmented_Discourse_Representation_Theory_Discopurse_Parsing -->

    <owl:NamedIndividual rdf:about="http://nlpkg.sebis.cit.tum.de/nlp-fos-hierarchy.owl#Segmented_Discourse_Representation_Theory_Discopurse_Parsing">
        <rdf:type rdf:resource="http://nlpkg.sebis.cit.tum.de/nlp-fos-hierarchy.owl#Task"/>
        <rdf:type rdf:resource="http://nlpkg.sebis.cit.tum.de/nlp-taxonomy.owl#FieldOfStudy"/>
        <nlp-taxonomy:subFieldOf rdf:resource="http://nlpkg.sebis.cit.tum.de/nlp-fos-hierarchy.owl#Discourse_Parsing"/>
        <nlp-taxonomy:level rdf:datatype="http://www.w3.org/2001/XMLSchema#integer">4</nlp-taxonomy:level>
        <dcterms:description xml:lang="en">Segmented Discourse Representation Theory (SDRT) Discourse Parsing is an approach that focuses on structuring and understanding written or spoken language at a discourse level. It involves breaking down a text or conversation into segments or clauses, assigning semantic representations to these segments, and analyzing the relationships between them to capture the discourse&apos;s overall meaning and coherence.</dcterms:description>
        <oboInOwl:hasSynonym xml:lang="en">SDRT-style Discopurse Parsing</oboInOwl:hasSynonym>
        <rdfs:label xml:lang="en">Segmented Discourse Representation Theory Discopurse Parsing</rdfs:label>
    </owl:NamedIndividual>
    


    <!-- http://nlpkg.sebis.cit.tum.de/nlp-fos-hierarchy.owl#Self-supervised_Learning -->

    <owl:NamedIndividual rdf:about="http://nlpkg.sebis.cit.tum.de/nlp-fos-hierarchy.owl#Self-supervised_Learning">
        <rdf:type rdf:resource="http://nlpkg.sebis.cit.tum.de/nlp-fos-hierarchy.owl#Task"/>
        <rdf:type rdf:resource="http://nlpkg.sebis.cit.tum.de/nlp-taxonomy.owl#FieldOfStudy"/>
        <nlp-taxonomy:subFieldOf rdf:resource="http://nlpkg.sebis.cit.tum.de/nlp-taxonomy.owl#Low-Resource_NLP"/>
        <survey>https://arxiv.org/abs/2304.01008</survey>
        <nlp-taxonomy:level rdf:datatype="http://www.w3.org/2001/XMLSchema#integer">3</nlp-taxonomy:level>
        <dcterms:description xml:lang="en">Self-supervised Learning is a type of machine learning where the model learns to predict a part of the input data from other parts of the same input data. It does not require explicit labels provided by humans. Instead, it uses the structure of the data itself to generate labels. For example, in NLP, a model might be trained to predict the next word in a sentence, using the previous words as input, thereby learning the syntax, semantics, and other language rules.</dcterms:description>
        <oboInOwl:hasSynonym xml:lang="en">Self-supervised</oboInOwl:hasSynonym>
        <rdfs:label xml:lang="en">Self-supervised Learning</rdfs:label>
    </owl:NamedIndividual>
    


    <!-- http://nlpkg.sebis.cit.tum.de/nlp-fos-hierarchy.owl#Semantic_Matching -->

    <owl:NamedIndividual rdf:about="http://nlpkg.sebis.cit.tum.de/nlp-fos-hierarchy.owl#Semantic_Matching">
        <rdf:type rdf:resource="http://nlpkg.sebis.cit.tum.de/nlp-fos-hierarchy.owl#Task"/>
        <rdf:type rdf:resource="http://nlpkg.sebis.cit.tum.de/nlp-taxonomy.owl#FieldOfStudy"/>
        <nlp-taxonomy:subFieldOf rdf:resource="http://nlpkg.sebis.cit.tum.de/nlp-taxonomy.owl#Semantic_Search"/>
        <relevantInformation>https://medium.com/georgian-impact-blog/an-introduction-to-semantic-matching-techniques-in-nlp-and-computer-vision-c22bf3cee8e9</relevantInformation>
        <nlp-taxonomy:level rdf:datatype="http://www.w3.org/2001/XMLSchema#integer">3</nlp-taxonomy:level>
        <dcterms:description xml:lang="en">Semantic Matching refers to the process of identifying and linking words, phrases, or sentences that share similar meanings, even if they do not share the same surface form or structure. This involves understanding the context, synonyms, and intent behind the words, rather than just matching the exact words or phrases.</dcterms:description>
        <oboInOwl:hasSynonym xml:lang="en">Semantic Text Matching</oboInOwl:hasSynonym>
        <oboInOwl:hasSynonym xml:lang="en">Text Semantic Matching</oboInOwl:hasSynonym>
        <rdfs:label xml:lang="en">Semantic Matching</rdfs:label>
    </owl:NamedIndividual>
    


    <!-- http://nlpkg.sebis.cit.tum.de/nlp-fos-hierarchy.owl#Semantic_Treebank -->

    <owl:NamedIndividual rdf:about="http://nlpkg.sebis.cit.tum.de/nlp-fos-hierarchy.owl#Semantic_Treebank">
        <rdf:type rdf:resource="http://nlpkg.sebis.cit.tum.de/nlp-fos-hierarchy.owl#DataStructure"/>
        <rdf:type rdf:resource="http://nlpkg.sebis.cit.tum.de/nlp-taxonomy.owl#FieldOfStudy"/>
        <nlp-taxonomy:subFieldOf rdf:resource="http://nlpkg.sebis.cit.tum.de/nlp-fos-hierarchy.owl#Treebank"/>
        <nlp-taxonomy:level rdf:datatype="http://www.w3.org/2001/XMLSchema#integer">6</nlp-taxonomy:level>
        <dcterms:description xml:lang="en">A Semantic Treebank is a structured dataset or corpus that annotates sentences or text with detailed semantic information, often represented as labeled tree structures. These tree structures capture the relationships and meanings of words and phrases within the text.</dcterms:description>
        <oboInOwl:hasSynonym xml:lang="en">Semantic Tree-Bank</oboInOwl:hasSynonym>
        <rdfs:label xml:lang="en">Semantic Treebank</rdfs:label>
    </owl:NamedIndividual>
    


    <!-- http://nlpkg.sebis.cit.tum.de/nlp-fos-hierarchy.owl#Semi-supervised_Learning -->

    <owl:NamedIndividual rdf:about="http://nlpkg.sebis.cit.tum.de/nlp-fos-hierarchy.owl#Semi-supervised_Learning">
        <rdf:type rdf:resource="http://nlpkg.sebis.cit.tum.de/nlp-fos-hierarchy.owl#Task"/>
        <rdf:type rdf:resource="http://nlpkg.sebis.cit.tum.de/nlp-taxonomy.owl#FieldOfStudy"/>
        <nlp-taxonomy:subFieldOf rdf:resource="http://nlpkg.sebis.cit.tum.de/nlp-taxonomy.owl#Low-Resource_NLP"/>
        <survey>https://arxiv.org/abs/2103.07575</survey>
        <nlp-taxonomy:level rdf:datatype="http://www.w3.org/2001/XMLSchema#integer">3</nlp-taxonomy:level>
        <dcterms:description xml:lang="en">Semi-supervised learning is a machine learning approach where the model is trained using a combination of a small amount of labeled data and a large amount of unlabeled data. The idea is to use the unlabeled data to enhance the learning accuracy of the model derived from the labeled data. This method is particularly useful when it&apos;s expensive or time-consuming to label data but unlabeled data is abundant.</dcterms:description>
        <oboInOwl:hasSynonym xml:lang="en">Semi-supervised</oboInOwl:hasSynonym>
        <rdfs:label xml:lang="en">Semi-supervised Learning</rdfs:label>
    </owl:NamedIndividual>
    


    <!-- http://nlpkg.sebis.cit.tum.de/nlp-fos-hierarchy.owl#Sentence-Transformers -->

    <owl:NamedIndividual rdf:about="http://nlpkg.sebis.cit.tum.de/nlp-fos-hierarchy.owl#Sentence-Transformers">
        <rdf:type rdf:resource="http://nlpkg.sebis.cit.tum.de/nlp-fos-hierarchy.owl#OtherScientificField"/>
        <rdf:type rdf:resource="http://nlpkg.sebis.cit.tum.de/nlp-taxonomy.owl#FieldOfStudy"/>
        <usedFor rdf:resource="http://nlpkg.sebis.cit.tum.de/nlp-fos-hierarchy.owl#Aspect-specific_Sentence_Embeddings"/>
        <uses rdf:resource="http://nlpkg.sebis.cit.tum.de/nlp-fos-hierarchy.owl#Transformers_&amp;_Large_Language_Models"/>
        <nlp-taxonomy:subFieldOf rdf:resource="http://nlpkg.sebis.cit.tum.de/nlp-fos-hierarchy.owl#Contextualized_Embeddings"/>
        <nlp-taxonomy:subFieldOf rdf:resource="http://nlpkg.sebis.cit.tum.de/nlp-fos-hierarchy.owl#Dense_Embeddings"/>
        <nlp-taxonomy:subFieldOf rdf:resource="http://nlpkg.sebis.cit.tum.de/nlp-fos-hierarchy.owl#Sentence_Embeddings"/>
        <code>https://www.sbert.net/</code>
        <origin>https://aclanthology.org/D19-1410</origin>
        <nlp-taxonomy:level rdf:datatype="http://www.w3.org/2001/XMLSchema#integer">6</nlp-taxonomy:level>
        <dcterms:description xml:lang="en">Sentence Transformers is a framework that provides an easy method to compute dense vector representations for sentences and paragraphs. These representations (also known as embeddings) can then be compared for semantic similarity. This is achieved by fine-tuning transformer networks, like BERT, on specific NLP tasks, such as natural language inference.</dcterms:description>
        <oboInOwl:hasSynonym xml:lang="en">Sentence Transformers</oboInOwl:hasSynonym>
        <oboInOwl:hasSynonym xml:lang="en">SentenceTransformers</oboInOwl:hasSynonym>
        <rdfs:label xml:lang="en">Sentence-Transformers</rdfs:label>
    </owl:NamedIndividual>
    


    <!-- http://nlpkg.sebis.cit.tum.de/nlp-fos-hierarchy.owl#Sentence_Alignment -->

    <owl:NamedIndividual rdf:about="http://nlpkg.sebis.cit.tum.de/nlp-fos-hierarchy.owl#Sentence_Alignment">
        <rdf:type rdf:resource="http://nlpkg.sebis.cit.tum.de/nlp-fos-hierarchy.owl#Task"/>
        <rdf:type rdf:resource="http://nlpkg.sebis.cit.tum.de/nlp-taxonomy.owl#FieldOfStudy"/>
        <nlp-taxonomy:subFieldOf rdf:resource="http://nlpkg.sebis.cit.tum.de/nlp-fos-hierarchy.owl#Statistical_Machine_Translation"/>
        <nlp-taxonomy:level rdf:datatype="http://www.w3.org/2001/XMLSchema#integer">4</nlp-taxonomy:level>
        <dcterms:description xml:lang="en">Sentence Alignment refers to the process of identifying corresponding sentences in two different languages within a parallel corpus. This is a crucial step in training statistical machine translation models as it helps the model to learn how words and phrases in one language translate into another. The alignment is usually done based on sentence length and order, but more complex methods may also consider the actual content of the sentences.</dcterms:description>
        <rdfs:label xml:lang="en">Sentence Alignment</rdfs:label>
    </owl:NamedIndividual>
    


    <!-- http://nlpkg.sebis.cit.tum.de/nlp-fos-hierarchy.owl#Sentence_Embeddings -->

    <owl:NamedIndividual rdf:about="http://nlpkg.sebis.cit.tum.de/nlp-fos-hierarchy.owl#Sentence_Embeddings">
        <rdf:type rdf:resource="http://nlpkg.sebis.cit.tum.de/nlp-fos-hierarchy.owl#DataStructure"/>
        <rdf:type rdf:resource="http://nlpkg.sebis.cit.tum.de/nlp-taxonomy.owl#FieldOfStudy"/>
        <nlp-taxonomy:subFieldOf rdf:resource="http://nlpkg.sebis.cit.tum.de/nlp-fos-hierarchy.owl#Text_Embeddings"/>
        <nlp-taxonomy:superFieldOf rdf:resource="http://nlpkg.sebis.cit.tum.de/nlp-fos-hierarchy.owl#Aspect-specific_Sentence_Embeddings"/>
        <nlp-taxonomy:superFieldOf rdf:resource="http://nlpkg.sebis.cit.tum.de/nlp-fos-hierarchy.owl#Bag-of-Words"/>
        <nlp-taxonomy:superFieldOf rdf:resource="http://nlpkg.sebis.cit.tum.de/nlp-fos-hierarchy.owl#Sentence-Transformers"/>
        <survey>https://aclanthology.org/2023.findings-acl.439</survey>
        <survey>https://arxiv.org/abs/2305.12641</survey>
        <nlp-taxonomy:level rdf:datatype="http://www.w3.org/2001/XMLSchema#integer">5</nlp-taxonomy:level>
        <dcterms:description xml:lang="en">Sentence Embeddings refer to the numerical representation of sentences or short paragraphs in a multi-dimensional vector space. It is a form of feature extraction where sentences or short paragraphs are converted into vectors. These vectors capture the semantic meaning of the sentence, allowing similar sentences to be mapped close to each other in the vector space.</dcterms:description>
        <oboInOwl:hasSynonym xml:lang="en">Document Embeddings</oboInOwl:hasSynonym>
        <oboInOwl:hasSynonym xml:lang="en">Sentence Representations</oboInOwl:hasSynonym>
        <rdfs:label xml:lang="en">Sentence Embeddings</rdfs:label>
    </owl:NamedIndividual>
    


    <!-- http://nlpkg.sebis.cit.tum.de/nlp-fos-hierarchy.owl#Sequence_Labeling -->

    <owl:NamedIndividual rdf:about="http://nlpkg.sebis.cit.tum.de/nlp-fos-hierarchy.owl#Sequence_Labeling">
        <rdf:type rdf:resource="http://nlpkg.sebis.cit.tum.de/nlp-fos-hierarchy.owl#Task"/>
        <rdf:type rdf:resource="http://nlpkg.sebis.cit.tum.de/nlp-taxonomy.owl#FieldOfStudy"/>
        <usedFor rdf:resource="http://nlpkg.sebis.cit.tum.de/nlp-fos-hierarchy.owl#Part-of-Speech_Tagging"/>
        <usedFor rdf:resource="http://nlpkg.sebis.cit.tum.de/nlp-fos-hierarchy.owl#Slot_Filling"/>
        <usedFor rdf:resource="http://nlpkg.sebis.cit.tum.de/nlp-taxonomy.owl#Chunking"/>
        <usedFor rdf:resource="http://nlpkg.sebis.cit.tum.de/nlp-taxonomy.owl#Named_Entity_Recognition"/>
        <uses rdf:resource="http://nlpkg.sebis.cit.tum.de/nlp-fos-hierarchy.owl#Conditional_Random_Field"/>
        <nlp-taxonomy:subFieldOf rdf:resource="http://nlpkg.sebis.cit.tum.de/nlp-taxonomy.owl#Text_Classification"/>
        <relevantInformation>https://medium.com/mlearning-ai/sequence-labeling-the-basis-of-nlp-a52c8fffa567</relevantInformation>
        <relevantInformation>https://web.stanford.edu/~jurafsky/slp3/8.pdf</relevantInformation>
        <survey>https://aclanthology.org/C18-1327</survey>
        <survey>https://arxiv.org/abs/2011.06727</survey>
        <nlp-taxonomy:level rdf:datatype="http://www.w3.org/2001/XMLSchema#integer">3</nlp-taxonomy:level>
        <dcterms:description xml:lang="en">Sequence Labeling is a task where the model is trained to assign a label to each member in the sequence of input data. This is commonly used in NLP tasks such as part-of-speech tagging, named entity recognition, and text chunking where each word in a sentence needs to be labeled based on its role.</dcterms:description>
        <oboInOwl:hasSynonym xml:lang="en">Sequence Tagging</oboInOwl:hasSynonym>
        <rdfs:label xml:lang="en">Sequence Labeling</rdfs:label>
    </owl:NamedIndividual>
    


    <!-- http://nlpkg.sebis.cit.tum.de/nlp-fos-hierarchy.owl#Sign_Language_Recognition -->

    <owl:NamedIndividual rdf:about="http://nlpkg.sebis.cit.tum.de/nlp-fos-hierarchy.owl#Sign_Language_Recognition">
        <rdf:type rdf:resource="http://nlpkg.sebis.cit.tum.de/nlp-fos-hierarchy.owl#Task"/>
        <rdf:type rdf:resource="http://nlpkg.sebis.cit.tum.de/nlp-taxonomy.owl#FieldOfStudy"/>
        <nlp-taxonomy:subFieldOf rdf:resource="http://nlpkg.sebis.cit.tum.de/nlp-fos-hierarchy.owl#Image_Captioning"/>
        <nlp-taxonomy:subFieldOf rdf:resource="http://nlpkg.sebis.cit.tum.de/nlp-fos-hierarchy.owl#Video_Captioning"/>
        <survey>https://arxiv.org/abs/2305.13941</survey>
        <nlp-taxonomy:level rdf:datatype="http://www.w3.org/2001/XMLSchema#integer">4</nlp-taxonomy:level>
        <dcterms:description xml:lang="en">Sign Language Recognition is a computer vision and natural language processing task that involves automatically recognizing and translating sign language gestures into written or spoken language. The goal of sign language recognition is to develop algorithms that can understand and interpret sign language, enabling people who use sign language as their primary mode of communication to communicate more easily with non-signers.</dcterms:description>
        <rdfs:label xml:lang="en">Sign Language Recognition</rdfs:label>
    </owl:NamedIndividual>
    


    <!-- http://nlpkg.sebis.cit.tum.de/nlp-fos-hierarchy.owl#Slang_Detection -->

    <owl:NamedIndividual rdf:about="http://nlpkg.sebis.cit.tum.de/nlp-fos-hierarchy.owl#Slang_Detection">
        <rdf:type rdf:resource="http://nlpkg.sebis.cit.tum.de/nlp-fos-hierarchy.owl#Task"/>
        <rdf:type rdf:resource="http://nlpkg.sebis.cit.tum.de/nlp-taxonomy.owl#FieldOfStudy"/>
        <nlp-taxonomy:subFieldOf rdf:resource="http://nlpkg.sebis.cit.tum.de/nlp-taxonomy.owl#Stylistic_Analysis"/>
        <nlp-taxonomy:subFieldOf rdf:resource="http://nlpkg.sebis.cit.tum.de/nlp-taxonomy.owl#Text_Classification"/>
        <nlp-taxonomy:level rdf:datatype="http://www.w3.org/2001/XMLSchema#integer">3</nlp-taxonomy:level>
        <dcterms:description xml:lang="en">Slang Detection and Identification refers to the process of identifying and understanding slang words or phrases in a given text. Slang words are informal language, often specific to certain groups or cultures, and can be challenging for NLP algorithms to interpret due to their non-standard usage.</dcterms:description>
        <oboInOwl:hasSynonym xml:lang="en">Slang Classification</oboInOwl:hasSynonym>
        <oboInOwl:hasSynonym xml:lang="en">Slang Identification</oboInOwl:hasSynonym>
        <oboInOwl:hasSynonym xml:lang="en">Slang Recognition</oboInOwl:hasSynonym>
        <rdfs:label xml:lang="en">Slang Detection</rdfs:label>
    </owl:NamedIndividual>
    


    <!-- http://nlpkg.sebis.cit.tum.de/nlp-fos-hierarchy.owl#Slot_Filling -->

    <owl:NamedIndividual rdf:about="http://nlpkg.sebis.cit.tum.de/nlp-fos-hierarchy.owl#Slot_Filling">
        <rdf:type rdf:resource="http://nlpkg.sebis.cit.tum.de/nlp-fos-hierarchy.owl#Task"/>
        <rdf:type rdf:resource="http://nlpkg.sebis.cit.tum.de/nlp-taxonomy.owl#FieldOfStudy"/>
        <usedFor rdf:resource="http://nlpkg.sebis.cit.tum.de/nlp-fos-hierarchy.owl#Dialogue_State_Tracking"/>
        <usedFor rdf:resource="http://nlpkg.sebis.cit.tum.de/nlp-fos-hierarchy.owl#Spoken_Language_Understanding"/>
        <uses rdf:resource="http://nlpkg.sebis.cit.tum.de/nlp-fos-hierarchy.owl#Sequence_Labeling"/>
        <nlp-taxonomy:subFieldOf rdf:resource="http://nlpkg.sebis.cit.tum.de/nlp-taxonomy.owl#Semantic_Parsing"/>
        <nlp-taxonomy:superFieldOf rdf:resource="http://nlpkg.sebis.cit.tum.de/nlp-fos-hierarchy.owl#Explicit_Semantic_Role_Labeling"/>
        <nlp-taxonomy:superFieldOf rdf:resource="http://nlpkg.sebis.cit.tum.de/nlp-fos-hierarchy.owl#Implicit_Semantic_Role_Labeling"/>
        <relevantInformation>https://web.stanford.edu/~jurafsky/slp3/24.pdf</relevantInformation>
        <survey>https://aclanthology.org/2020.coling-main.42</survey>
        <survey>https://arxiv.org/abs/2101.08091</survey>
        <survey>https://arxiv.org/abs/2207.13211</survey>
        <nlp-taxonomy:level rdf:datatype="http://www.w3.org/2001/XMLSchema#integer">3</nlp-taxonomy:level>
        <dcterms:description xml:lang="en">Slot filling is a concept used in various applications, particularly in chatbots, virtual assistants, and information extraction systems. It involves identifying and extracting specific pieces of information, known as &quot;slots,&quot; from unstructured text or user input. These slots typically correspond to specific categories or entities, such as dates, names, locations, or any other predefined information. For instance, when a user queries for nearby restaurants, key slots for location and preferred food are required for a dialog system to retrieve the appropriate information. Thus, the main challenge in the slot-filling task is to extract the target entity.</dcterms:description>
        <oboInOwl:hasSynonym xml:lang="en">SRL</oboInOwl:hasSynonym>
        <oboInOwl:hasSynonym xml:lang="en">Semantic Role Labeling</oboInOwl:hasSynonym>
        <oboInOwl:hasSynonym xml:lang="en">Shallow Semantic Parsing</oboInOwl:hasSynonym>
        <rdfs:label xml:lang="en">Slot Filling</rdfs:label>
    </owl:NamedIndividual>
    


    <!-- http://nlpkg.sebis.cit.tum.de/nlp-fos-hierarchy.owl#Social_Bias -->

    <owl:NamedIndividual rdf:about="http://nlpkg.sebis.cit.tum.de/nlp-fos-hierarchy.owl#Social_Bias">
        <rdf:type rdf:resource="http://nlpkg.sebis.cit.tum.de/nlp-fos-hierarchy.owl#OtherScientificField"/>
        <rdf:type rdf:resource="http://nlpkg.sebis.cit.tum.de/nlp-taxonomy.owl#FieldOfStudy"/>
        <nlp-taxonomy:subFieldOf rdf:resource="http://nlpkg.sebis.cit.tum.de/nlp-fos-hierarchy.owl#Biases_&amp;_Fairness_in_NLP"/>
        <nlp-taxonomy:superFieldOf rdf:resource="http://nlpkg.sebis.cit.tum.de/nlp-fos-hierarchy.owl#Age_Bias"/>
        <nlp-taxonomy:superFieldOf rdf:resource="http://nlpkg.sebis.cit.tum.de/nlp-fos-hierarchy.owl#Gender_Bias"/>
        <nlp-taxonomy:superFieldOf rdf:resource="http://nlpkg.sebis.cit.tum.de/nlp-fos-hierarchy.owl#Political_Bias"/>
        <nlp-taxonomy:superFieldOf rdf:resource="http://nlpkg.sebis.cit.tum.de/nlp-fos-hierarchy.owl#Race_Bias"/>
        <survey>https://aclanthology.org/2020.acl-main.405</survey>
        <survey>https://aclanthology.org/2021.acl-long.148</survey>
        <survey>https://aclanthology.org/2021.acl-long.330/</survey>
        <survey>https://aclanthology.org/2022.aacl-main.49</survey>
        <survey>https://arxiv.org/abs/2306.08158</survey>
        <survey>https://arxiv.org/abs/2309.14381</survey>
        <nlp-taxonomy:level rdf:datatype="http://www.w3.org/2001/XMLSchema#integer">4</nlp-taxonomy:level>
        <dcterms:description xml:lang="en">Social Bias refers to discrimination for, or against, a person or group, or a set of ideas or beliefs, in a way that is prejudicial or unfair. Social bias often involves consciously or unconsciously stereotyping others and behaving in a way that disadvantages a person or group or advantages another. Social bias, both implicit and explicit, is at the core of racism, misogyny and discrimination based on sexual orientation or religion, and such biases may operate between individuals or at the level of the institution.</dcterms:description>
        <oboInOwl:hasSynonym xml:lang="en">Societal Bias</oboInOwl:hasSynonym>
        <oboInOwl:hasSynonym xml:lang="en">Sociodemographic Bias</oboInOwl:hasSynonym>
        <rdfs:label xml:lang="en">Social Bias</rdfs:label>
    </owl:NamedIndividual>
    


    <!-- http://nlpkg.sebis.cit.tum.de/nlp-fos-hierarchy.owl#Soft_Prompts -->

    <owl:NamedIndividual rdf:about="http://nlpkg.sebis.cit.tum.de/nlp-fos-hierarchy.owl#Soft_Prompts">
        <rdf:type rdf:resource="http://nlpkg.sebis.cit.tum.de/nlp-fos-hierarchy.owl#OtherScientificField"/>
        <rdf:type rdf:resource="http://nlpkg.sebis.cit.tum.de/nlp-taxonomy.owl#FieldOfStudy"/>
        <nlp-taxonomy:subFieldOf rdf:resource="http://nlpkg.sebis.cit.tum.de/nlp-fos-hierarchy.owl#Parameter-Efficient_Fine-Tuning"/>
        <nlp-taxonomy:subFieldOf rdf:resource="http://nlpkg.sebis.cit.tum.de/nlp-fos-hierarchy.owl#Prompt_Optimization"/>
        <nlp-taxonomy:level rdf:datatype="http://www.w3.org/2001/XMLSchema#integer">4</nlp-taxonomy:level>
        <nlp-taxonomy:level rdf:datatype="http://www.w3.org/2001/XMLSchema#integer">5</nlp-taxonomy:level>
        <dcterms:description xml:lang="en">Soft Prompts are learnable, continuous feature vectors that are added to the input prompt. Unlike hard prompts, they are learned during the training process and aren’t human-readable.</dcterms:description>
        <rdfs:label xml:lang="en">Soft Prompts</rdfs:label>
    </owl:NamedIndividual>
    


    <!-- http://nlpkg.sebis.cit.tum.de/nlp-fos-hierarchy.owl#Span_Detection -->

    <owl:NamedIndividual rdf:about="http://nlpkg.sebis.cit.tum.de/nlp-fos-hierarchy.owl#Span_Detection">
        <rdf:type rdf:resource="http://nlpkg.sebis.cit.tum.de/nlp-fos-hierarchy.owl#Task"/>
        <rdf:type rdf:resource="http://nlpkg.sebis.cit.tum.de/nlp-taxonomy.owl#FieldOfStudy"/>
        <usedFor rdf:resource="http://nlpkg.sebis.cit.tum.de/nlp-fos-hierarchy.owl#Keyword_&amp;_Keyphrase_Extraction"/>
        <usedFor rdf:resource="http://nlpkg.sebis.cit.tum.de/nlp-taxonomy.owl#Chunking"/>
        <usedFor rdf:resource="http://nlpkg.sebis.cit.tum.de/nlp-taxonomy.owl#Named_Entity_Recognition"/>
        <nlp-taxonomy:subFieldOf rdf:resource="http://nlpkg.sebis.cit.tum.de/nlp-taxonomy.owl#Text_Classification"/>
        <nlp-taxonomy:level rdf:datatype="http://www.w3.org/2001/XMLSchema#integer">3</nlp-taxonomy:level>
        <dcterms:description xml:lang="en">Span Detection refers to the task of identifying and categorizing specific portions or spans of text within a larger document or corpus. These spans can be words, phrases, or even whole sentences that are relevant to the task at hand.</dcterms:description>
        <oboInOwl:hasSynonym xml:lang="en">Span Classification</oboInOwl:hasSynonym>
        <oboInOwl:hasSynonym xml:lang="en">Span Extraction</oboInOwl:hasSynonym>
        <oboInOwl:hasSynonym xml:lang="en">Span Identification</oboInOwl:hasSynonym>
        <rdfs:label xml:lang="en">Span Detection</rdfs:label>
    </owl:NamedIndividual>
    


    <!-- http://nlpkg.sebis.cit.tum.de/nlp-fos-hierarchy.owl#Sparse_Document_Retrieval -->

    <owl:NamedIndividual rdf:about="http://nlpkg.sebis.cit.tum.de/nlp-fos-hierarchy.owl#Sparse_Document_Retrieval">
        <rdf:type rdf:resource="http://nlpkg.sebis.cit.tum.de/nlp-fos-hierarchy.owl#Task"/>
        <rdf:type rdf:resource="http://nlpkg.sebis.cit.tum.de/nlp-taxonomy.owl#FieldOfStudy"/>
        <uses rdf:resource="http://nlpkg.sebis.cit.tum.de/nlp-fos-hierarchy.owl#Sparse_Embeddings"/>
        <nlp-taxonomy:subFieldOf rdf:resource="http://nlpkg.sebis.cit.tum.de/nlp-taxonomy.owl#Document_Retrieval"/>
        <nlp-taxonomy:level rdf:datatype="http://www.w3.org/2001/XMLSchema#integer">3</nlp-taxonomy:level>
        <dcterms:description xml:lang="en">Sparse Document Retrieval refers to the process of finding the most relevant documents in a large dataset based on a specific query. This is typically done by creating a sparse representation of the documents, where each document is represented as a high-dimensional vector with most values being zero. The non-zero values in the vector represent the presence of specific words or phrases in the document. The relevance of a document to a query is then determined by comparing these vectors.</dcterms:description>
        <oboInOwl:hasSynonym xml:lang="en">Sparse Retrieval</oboInOwl:hasSynonym>
        <rdfs:label xml:lang="en">Sparse Document Retrieval</rdfs:label>
    </owl:NamedIndividual>
    


    <!-- http://nlpkg.sebis.cit.tum.de/nlp-fos-hierarchy.owl#Sparse_Embeddings -->

    <owl:NamedIndividual rdf:about="http://nlpkg.sebis.cit.tum.de/nlp-fos-hierarchy.owl#Sparse_Embeddings">
        <rdf:type rdf:resource="http://nlpkg.sebis.cit.tum.de/nlp-fos-hierarchy.owl#DataStructure"/>
        <rdf:type rdf:resource="http://nlpkg.sebis.cit.tum.de/nlp-taxonomy.owl#FieldOfStudy"/>
        <usedFor rdf:resource="http://nlpkg.sebis.cit.tum.de/nlp-fos-hierarchy.owl#Sparse_Document_Retrieval"/>
        <usedFor rdf:resource="http://nlpkg.sebis.cit.tum.de/nlp-fos-hierarchy.owl#Sparse_Passage_Retrieval"/>
        <nlp-taxonomy:subFieldOf rdf:resource="http://nlpkg.sebis.cit.tum.de/nlp-fos-hierarchy.owl#Text_Embeddings"/>
        <nlp-taxonomy:superFieldOf rdf:resource="http://nlpkg.sebis.cit.tum.de/nlp-fos-hierarchy.owl#Bag-of-Words"/>
        <nlp-taxonomy:level rdf:datatype="http://www.w3.org/2001/XMLSchema#integer">5</nlp-taxonomy:level>
        <dcterms:description xml:lang="en">Sparse Embeddings refer to the representation of words or phrases in a high-dimensional space where most of the elements are zero. This is in contrast to dense embeddings where all elements carry some value. Sparse embeddings can be beneficial in situations where the dataset is large and complex, as they can reduce computational load and memory requirements. However, they may not capture semantic relationships between words as effectively as dense embeddings.</dcterms:description>
        <oboInOwl:hasSynonym xml:lang="en">Localist Representations</oboInOwl:hasSynonym>
        <rdfs:label xml:lang="en">Sparse Embeddings</rdfs:label>
    </owl:NamedIndividual>
    


    <!-- http://nlpkg.sebis.cit.tum.de/nlp-fos-hierarchy.owl#Sparse_Passage_Retrieval -->

    <owl:NamedIndividual rdf:about="http://nlpkg.sebis.cit.tum.de/nlp-fos-hierarchy.owl#Sparse_Passage_Retrieval">
        <rdf:type rdf:resource="http://nlpkg.sebis.cit.tum.de/nlp-fos-hierarchy.owl#Task"/>
        <rdf:type rdf:resource="http://nlpkg.sebis.cit.tum.de/nlp-taxonomy.owl#FieldOfStudy"/>
        <uses rdf:resource="http://nlpkg.sebis.cit.tum.de/nlp-fos-hierarchy.owl#Sparse_Embeddings"/>
        <nlp-taxonomy:subFieldOf rdf:resource="http://nlpkg.sebis.cit.tum.de/nlp-taxonomy.owl#Passage_Retrieval"/>
        <nlp-taxonomy:level rdf:datatype="http://www.w3.org/2001/XMLSchema#integer">3</nlp-taxonomy:level>
        <dcterms:description xml:lang="en">Sparse Passage Retrieval in refers to the method of extracting relevant sections or passages from a large text corpus based on keyword matching. It uses traditional information retrieval techniques, such as Bag of Words or TF-IDF, to identify and retrieve passages that are most likely to contain the answer to a given query. This approach is called &quot;sparse&quot; because it does not consider the semantic relationships between words and often results in a high-dimensional, sparse vector representation of the text.</dcterms:description>
        <oboInOwl:hasSynonym xml:lang="en">Sparse Retrieval</oboInOwl:hasSynonym>
        <rdfs:label xml:lang="en">Sparse Passage Retrieval</rdfs:label>
    </owl:NamedIndividual>
    


    <!-- http://nlpkg.sebis.cit.tum.de/nlp-fos-hierarchy.owl#Speaker_Diarization -->

    <owl:NamedIndividual rdf:about="http://nlpkg.sebis.cit.tum.de/nlp-fos-hierarchy.owl#Speaker_Diarization">
        <rdf:type rdf:resource="http://nlpkg.sebis.cit.tum.de/nlp-fos-hierarchy.owl#Task"/>
        <rdf:type rdf:resource="http://nlpkg.sebis.cit.tum.de/nlp-taxonomy.owl#FieldOfStudy"/>
        <nlp-taxonomy:subFieldOf rdf:resource="http://nlpkg.sebis.cit.tum.de/nlp-taxonomy.owl#Speech_Recognition"/>
        <survey>https://arxiv.org/abs/2101.09624</survey>
        <nlp-taxonomy:level rdf:datatype="http://www.w3.org/2001/XMLSchema#integer">4</nlp-taxonomy:level>
        <dcterms:description xml:lang="en">Speaker diarization is a process that involves identifying and distinguishing different speakers in an audio recording or a continuous stream of speech. The primary goal of speaker diarization is to segment the audio into distinct speaker segments and associate each segment with a specific speaker identity.</dcterms:description>
        <rdfs:label xml:lang="en">Speaker Diarization</rdfs:label>
    </owl:NamedIndividual>
    


    <!-- http://nlpkg.sebis.cit.tum.de/nlp-fos-hierarchy.owl#Speaker_Recognition -->

    <owl:NamedIndividual rdf:about="http://nlpkg.sebis.cit.tum.de/nlp-fos-hierarchy.owl#Speaker_Recognition">
        <rdf:type rdf:resource="http://nlpkg.sebis.cit.tum.de/nlp-fos-hierarchy.owl#Task"/>
        <rdf:type rdf:resource="http://nlpkg.sebis.cit.tum.de/nlp-taxonomy.owl#FieldOfStudy"/>
        <nlp-taxonomy:subFieldOf rdf:resource="http://nlpkg.sebis.cit.tum.de/nlp-taxonomy.owl#Speech_&amp;_Audio_In_NLP"/>
        <nlp-taxonomy:level rdf:datatype="http://www.w3.org/2001/XMLSchema#integer">3</nlp-taxonomy:level>
        <dcterms:description xml:lang="en">Speaker Recognition refers to the technique of identifying a person based on their voice characteristics.</dcterms:description>
        <oboInOwl:hasSynonym xml:lang="en">Speaker Identification</oboInOwl:hasSynonym>
        <rdfs:label xml:lang="en">Speaker Recognition</rdfs:label>
    </owl:NamedIndividual>
    


    <!-- http://nlpkg.sebis.cit.tum.de/nlp-fos-hierarchy.owl#Speaker_Verification -->

    <owl:NamedIndividual rdf:about="http://nlpkg.sebis.cit.tum.de/nlp-fos-hierarchy.owl#Speaker_Verification">
        <rdf:type rdf:resource="http://nlpkg.sebis.cit.tum.de/nlp-fos-hierarchy.owl#Task"/>
        <rdf:type rdf:resource="http://nlpkg.sebis.cit.tum.de/nlp-taxonomy.owl#FieldOfStudy"/>
        <nlp-taxonomy:subFieldOf rdf:resource="http://nlpkg.sebis.cit.tum.de/nlp-taxonomy.owl#Speech_&amp;_Audio_In_NLP"/>
        <nlp-taxonomy:level rdf:datatype="http://www.w3.org/2001/XMLSchema#integer">3</nlp-taxonomy:level>
        <dcterms:description xml:lang="en">Speaker Verification is a process used to confirm the claimed identity of a speaker based on their voice characteristics. It involves comparing the speaker&apos;s voice with a previously stored voice model or voiceprint.</dcterms:description>
        <oboInOwl:hasSynonym xml:lang="en">Speaker Authentication</oboInOwl:hasSynonym>
        <rdfs:label xml:lang="en">Speaker Verification</rdfs:label>
    </owl:NamedIndividual>
    


    <!-- http://nlpkg.sebis.cit.tum.de/nlp-fos-hierarchy.owl#Speech_Segmentation -->

    <owl:NamedIndividual rdf:about="http://nlpkg.sebis.cit.tum.de/nlp-fos-hierarchy.owl#Speech_Segmentation">
        <rdf:type rdf:resource="http://nlpkg.sebis.cit.tum.de/nlp-fos-hierarchy.owl#Task"/>
        <rdf:type rdf:resource="http://nlpkg.sebis.cit.tum.de/nlp-taxonomy.owl#FieldOfStudy"/>
        <nlp-taxonomy:subFieldOf rdf:resource="http://nlpkg.sebis.cit.tum.de/nlp-taxonomy.owl#Speech_Recognition"/>
        <nlp-taxonomy:level rdf:datatype="http://www.w3.org/2001/XMLSchema#integer">4</nlp-taxonomy:level>
        <dcterms:description xml:lang="en">Speech segmentation refers to the process of dividing continuous spoken language or audio signals into smaller, meaningful units or segments such as words, syllables, or phonemes. These segments are typically characterized by pauses, changes in prosody (intonation and rhythm), or other acoustic features that signal the boundaries between different linguistic units. The primary goal of speech segmentation is to break down a continuous stream of speech into discrete, manageable units for further analysis or processing.</dcterms:description>
        <rdfs:label xml:lang="en">Speech Segmentation</rdfs:label>
    </owl:NamedIndividual>
    


    <!-- http://nlpkg.sebis.cit.tum.de/nlp-fos-hierarchy.owl#Speech_Synthesis -->

    <owl:NamedIndividual rdf:about="http://nlpkg.sebis.cit.tum.de/nlp-fos-hierarchy.owl#Speech_Synthesis">
        <rdf:type rdf:resource="http://nlpkg.sebis.cit.tum.de/nlp-fos-hierarchy.owl#Task"/>
        <rdf:type rdf:resource="http://nlpkg.sebis.cit.tum.de/nlp-taxonomy.owl#FieldOfStudy"/>
        <nlp-taxonomy:subFieldOf rdf:resource="http://nlpkg.sebis.cit.tum.de/nlp-taxonomy.owl#Speech_&amp;_Audio_In_NLP"/>
        <relevantInformation>https://web.stanford.edu/~jurafsky/slp3/16.pdf</relevantInformation>
        <survey>https://arxiv.org/abs/2104.09995</survey>
        <survey>https://arxiv.org/abs/2106.15561</survey>
        <nlp-taxonomy:level rdf:datatype="http://www.w3.org/2001/XMLSchema#integer">3</nlp-taxonomy:level>
        <dcterms:description xml:lang="en">Speech synthesis, also known as text-to-speech (TTS), is a technology that converts text or written content into spoken language. It is a process through which a computer or electronic device generates human-like speech by translating textual input into audible speech output.</dcterms:description>
        <oboInOwl:hasSynonym xml:lang="en">TTS</oboInOwl:hasSynonym>
        <oboInOwl:hasSynonym xml:lang="en">Text-to-Speech</oboInOwl:hasSynonym>
        <rdfs:label xml:lang="en">Speech Synthesis</rdfs:label>
    </owl:NamedIndividual>
    


    <!-- http://nlpkg.sebis.cit.tum.de/nlp-fos-hierarchy.owl#Spell_Checking -->

    <owl:NamedIndividual rdf:about="http://nlpkg.sebis.cit.tum.de/nlp-fos-hierarchy.owl#Spell_Checking">
        <rdf:type rdf:resource="http://nlpkg.sebis.cit.tum.de/nlp-fos-hierarchy.owl#Task"/>
        <rdf:type rdf:resource="http://nlpkg.sebis.cit.tum.de/nlp-taxonomy.owl#FieldOfStudy"/>
        <nlp-taxonomy:subFieldOf rdf:resource="http://nlpkg.sebis.cit.tum.de/nlp-taxonomy.owl#Text_Error_Correction"/>
        <relevantInformation>https://web.stanford.edu/~jurafsky/slp3/B.pdf</relevantInformation>
        <nlp-taxonomy:level rdf:datatype="http://www.w3.org/2001/XMLSchema#integer">3</nlp-taxonomy:level>
        <dcterms:description xml:lang="en">Spell Checking refers to the process of identifying and correcting spelling mistakes in text. It involves comparing each word in a text to a dictionary of correctly spelled words, and suggesting corrections for misspelled words.</dcterms:description>
        <oboInOwl:hasSynonym xml:lang="en">Spell Correction</oboInOwl:hasSynonym>
        <oboInOwl:hasSynonym xml:lang="en">Spelling Correction</oboInOwl:hasSynonym>
        <rdfs:label xml:lang="en">Spell Checking</rdfs:label>
    </owl:NamedIndividual>
    


    <!-- http://nlpkg.sebis.cit.tum.de/nlp-fos-hierarchy.owl#Spoken_Language_Understanding -->

    <owl:NamedIndividual rdf:about="http://nlpkg.sebis.cit.tum.de/nlp-fos-hierarchy.owl#Spoken_Language_Understanding">
        <rdf:type rdf:resource="http://nlpkg.sebis.cit.tum.de/nlp-fos-hierarchy.owl#Task"/>
        <rdf:type rdf:resource="http://nlpkg.sebis.cit.tum.de/nlp-taxonomy.owl#FieldOfStudy"/>
        <uses rdf:resource="http://nlpkg.sebis.cit.tum.de/nlp-fos-hierarchy.owl#Slot_Filling"/>
        <uses rdf:resource="http://nlpkg.sebis.cit.tum.de/nlp-taxonomy.owl#Intent_Recognition"/>
        <uses rdf:resource="http://nlpkg.sebis.cit.tum.de/nlp-taxonomy.owl#Speech_Recognition"/>
        <nlp-taxonomy:subFieldOf rdf:resource="http://nlpkg.sebis.cit.tum.de/nlp-taxonomy.owl#Speech_&amp;_Audio_In_NLP"/>
        <relevantInformation>https://aclanthology.org/sigs/sigslt/</relevantInformation>
        <survey>https://arxiv.org/abs/2103.03095</survey>
        <nlp-taxonomy:level rdf:datatype="http://www.w3.org/2001/XMLSchema#integer">3</nlp-taxonomy:level>
        <dcterms:description xml:lang="en">Spoken Language Understanding (SLU) focuses on the development of technologies and systems capable of processing and comprehending spoken language. The primary goal of SLU is to enable machines, such as voice assistants or automated customer service systems, to understand and extract meaning from spoken language input provided by humans.</dcterms:description>
        <oboInOwl:hasSynonym xml:lang="en">SLU</oboInOwl:hasSynonym>
        <rdfs:label xml:lang="en">Spoken Language Understanding</rdfs:label>
    </owl:NamedIndividual>
    


    <!-- http://nlpkg.sebis.cit.tum.de/nlp-fos-hierarchy.owl#Stance_Detection -->

    <owl:NamedIndividual rdf:about="http://nlpkg.sebis.cit.tum.de/nlp-fos-hierarchy.owl#Stance_Detection">
        <rdf:type rdf:resource="http://nlpkg.sebis.cit.tum.de/nlp-fos-hierarchy.owl#Task"/>
        <rdf:type rdf:resource="http://nlpkg.sebis.cit.tum.de/nlp-taxonomy.owl#FieldOfStudy"/>
        <usedFor rdf:resource="http://nlpkg.sebis.cit.tum.de/nlp-fos-hierarchy.owl#Evidence_Mining"/>
        <usedFor rdf:resource="http://nlpkg.sebis.cit.tum.de/nlp-fos-hierarchy.owl#Fake_News_Detection"/>
        <nlp-taxonomy:subFieldOf rdf:resource="http://nlpkg.sebis.cit.tum.de/nlp-taxonomy.owl#Opinion_Mining"/>
        <nlp-taxonomy:subFieldOf rdf:resource="http://nlpkg.sebis.cit.tum.de/nlp-taxonomy.owl#Text_Classification"/>
        <survey>https://aclanthology.org/2022.findings-naacl.94</survey>
        <survey>https://arxiv.org/abs/1907.00181</survey>
        <nlp-taxonomy:level rdf:datatype="http://www.w3.org/2001/XMLSchema#integer">3</nlp-taxonomy:level>
        <dcterms:description xml:lang="en">Stance Detection refers to the task of determining the attitude or stance of a speaker or writer with respect to some topic or the overall contextual polarity of a document. The stance could be in favor, against, or neutral towards the target topic.</dcterms:description>
        <oboInOwl:hasSynonym xml:lang="en">Stance Classification</oboInOwl:hasSynonym>
        <oboInOwl:hasSynonym xml:lang="en">Stance Identification</oboInOwl:hasSynonym>
        <rdfs:label xml:lang="en">Stance Detection</rdfs:label>
    </owl:NamedIndividual>
    


    <!-- http://nlpkg.sebis.cit.tum.de/nlp-fos-hierarchy.owl#Static_Embeddings -->

    <owl:NamedIndividual rdf:about="http://nlpkg.sebis.cit.tum.de/nlp-fos-hierarchy.owl#Static_Embeddings">
        <rdf:type rdf:resource="http://nlpkg.sebis.cit.tum.de/nlp-fos-hierarchy.owl#DataStructure"/>
        <rdf:type rdf:resource="http://nlpkg.sebis.cit.tum.de/nlp-taxonomy.owl#FieldOfStudy"/>
        <nlp-taxonomy:subFieldOf rdf:resource="http://nlpkg.sebis.cit.tum.de/nlp-fos-hierarchy.owl#Text_Embeddings"/>
        <nlp-taxonomy:superFieldOf rdf:resource="http://nlpkg.sebis.cit.tum.de/nlp-fos-hierarchy.owl#Bag-of-Words"/>
        <nlp-taxonomy:level rdf:datatype="http://www.w3.org/2001/XMLSchema#integer">5</nlp-taxonomy:level>
        <dcterms:description xml:lang="en">Static Embeddings refer to the method of representing words in a fixed, pre-trained vector space. Each word is assigned a specific vector that does not change regardless of the context in which the word is used. This method, while computationally efficient, does not account for the dynamic nature of language where the meaning of a word can change based on its surrounding context.</dcterms:description>
        <rdfs:label xml:lang="en">Static Embeddings</rdfs:label>
    </owl:NamedIndividual>
    


    <!-- http://nlpkg.sebis.cit.tum.de/nlp-fos-hierarchy.owl#Statistical_Machine_Translation -->

    <owl:NamedIndividual rdf:about="http://nlpkg.sebis.cit.tum.de/nlp-fos-hierarchy.owl#Statistical_Machine_Translation">
        <rdf:type rdf:resource="http://nlpkg.sebis.cit.tum.de/nlp-fos-hierarchy.owl#Task"/>
        <rdf:type rdf:resource="http://nlpkg.sebis.cit.tum.de/nlp-taxonomy.owl#FieldOfStudy"/>
        <nlp-taxonomy:subFieldOf rdf:resource="http://nlpkg.sebis.cit.tum.de/nlp-taxonomy.owl#Machine_Translation"/>
        <nlp-taxonomy:superFieldOf rdf:resource="http://nlpkg.sebis.cit.tum.de/nlp-fos-hierarchy.owl#Phrase-based_Machine_Translation"/>
        <nlp-taxonomy:superFieldOf rdf:resource="http://nlpkg.sebis.cit.tum.de/nlp-fos-hierarchy.owl#Sentence_Alignment"/>
        <nlp-taxonomy:superFieldOf rdf:resource="http://nlpkg.sebis.cit.tum.de/nlp-fos-hierarchy.owl#Syntax-based_Machine_Translation"/>
        <nlp-taxonomy:superFieldOf rdf:resource="http://nlpkg.sebis.cit.tum.de/nlp-fos-hierarchy.owl#Word-based_Machine_Translation"/>
        <nlp-taxonomy:superFieldOf rdf:resource="http://nlpkg.sebis.cit.tum.de/nlp-fos-hierarchy.owl#Word_Alignment"/>
        <relevantInformation>https://aclanthology.org/venues/wmt/</relevantInformation>
        <survey>https://aclanthology.org/J16-2001</survey>
        <nlp-taxonomy:level rdf:datatype="http://www.w3.org/2001/XMLSchema#integer">3</nlp-taxonomy:level>
        <dcterms:description xml:lang="en">Statistical Machine Translation (SMT) is a method of machine translation where the translation of text is generated on the basis of statistical models. These models are derived from the analysis of bilingual text corpora. The system learns to translate by being trained on large amounts of existing translations. It uses probability distributions to select the most likely translation among multiple possibilities.</dcterms:description>
        <oboInOwl:hasSynonym xml:lang="en">SMT</oboInOwl:hasSynonym>
        <rdfs:label xml:lang="en">Statistical Machine Translation</rdfs:label>
    </owl:NamedIndividual>
    


    <!-- http://nlpkg.sebis.cit.tum.de/nlp-fos-hierarchy.owl#Stemming -->

    <owl:NamedIndividual rdf:about="http://nlpkg.sebis.cit.tum.de/nlp-fos-hierarchy.owl#Stemming">
        <rdf:type rdf:resource="http://nlpkg.sebis.cit.tum.de/nlp-fos-hierarchy.owl#Task"/>
        <rdf:type rdf:resource="http://nlpkg.sebis.cit.tum.de/nlp-taxonomy.owl#FieldOfStudy"/>
        <usedFor rdf:resource="http://nlpkg.sebis.cit.tum.de/nlp-taxonomy.owl#Text_Normalization"/>
        <nlp-taxonomy:subFieldOf rdf:resource="http://nlpkg.sebis.cit.tum.de/nlp-taxonomy.owl#Morphology"/>
        <code>https://www.nltk.org/api/nltk.stem.html</code>
        <nlp-taxonomy:level rdf:datatype="http://www.w3.org/2001/XMLSchema#integer">3</nlp-taxonomy:level>
        <dcterms:description xml:lang="en">Stemming refers to the process of reducing inflected (or sometimes derived) words to their word stem or root form. The main purpose of stemming is to bring variation forms of a word back to its base form, such as &quot;running&quot; to &quot;run&quot;.</dcterms:description>
        <rdfs:label xml:lang="en">Stemming</rdfs:label>
    </owl:NamedIndividual>
    


    <!-- http://nlpkg.sebis.cit.tum.de/nlp-fos-hierarchy.owl#Story_Generation -->

    <owl:NamedIndividual rdf:about="http://nlpkg.sebis.cit.tum.de/nlp-fos-hierarchy.owl#Story_Generation">
        <rdf:type rdf:resource="http://nlpkg.sebis.cit.tum.de/nlp-fos-hierarchy.owl#Task"/>
        <rdf:type rdf:resource="http://nlpkg.sebis.cit.tum.de/nlp-taxonomy.owl#FieldOfStudy"/>
        <uses rdf:resource="http://nlpkg.sebis.cit.tum.de/nlp-fos-hierarchy.owl#Controllable_Text_Generation"/>
        <nlp-taxonomy:subFieldOf rdf:resource="http://nlpkg.sebis.cit.tum.de/nlp-taxonomy.owl#Text_Generation"/>
        <nlp-taxonomy:level rdf:datatype="http://www.w3.org/2001/XMLSchema#integer">2</nlp-taxonomy:level>
        <dcterms:description xml:lang="en">Story Generation is the task of automatically generating a coherent narrative, often from a set of premises or a brief summary.</dcterms:description>
        <rdfs:label xml:lang="en">Story Generation</rdfs:label>
    </owl:NamedIndividual>
    


    <!-- http://nlpkg.sebis.cit.tum.de/nlp-fos-hierarchy.owl#Structured_Data-specific_Language_Models -->

    <owl:NamedIndividual rdf:about="http://nlpkg.sebis.cit.tum.de/nlp-fos-hierarchy.owl#Structured_Data-specific_Language_Models">
        <rdf:type rdf:resource="http://nlpkg.sebis.cit.tum.de/nlp-fos-hierarchy.owl#OtherScientificField"/>
        <rdf:type rdf:resource="http://nlpkg.sebis.cit.tum.de/nlp-taxonomy.owl#FieldOfStudy"/>
        <nlp-taxonomy:subFieldOf rdf:resource="http://nlpkg.sebis.cit.tum.de/nlp-taxonomy.owl#Structured_Data_In_NLP"/>
        <survey>https://aclanthology.org/2023.tacl-1.14</survey>
        <survey>https://arxiv.org/abs/2201.09745</survey>
        <nlp-taxonomy:level rdf:datatype="http://www.w3.org/2001/XMLSchema#integer">3</nlp-taxonomy:level>
        <dcterms:description xml:lang="en">Structured Data-specific Language Models are trained to understand and generate text related to structured data formats, such as tables, graphs, databases, JSON, XML, or other organized data structures.</dcterms:description>
        <rdfs:label xml:lang="en">Structured Data-specific Language Models</rdfs:label>
    </owl:NamedIndividual>
    


    <!-- http://nlpkg.sebis.cit.tum.de/nlp-fos-hierarchy.owl#Subjectivity_Classification -->

    <owl:NamedIndividual rdf:about="http://nlpkg.sebis.cit.tum.de/nlp-fos-hierarchy.owl#Subjectivity_Classification">
        <rdf:type rdf:resource="http://nlpkg.sebis.cit.tum.de/nlp-fos-hierarchy.owl#Task"/>
        <rdf:type rdf:resource="http://nlpkg.sebis.cit.tum.de/nlp-taxonomy.owl#FieldOfStudy"/>
        <nlp-taxonomy:subFieldOf rdf:resource="http://nlpkg.sebis.cit.tum.de/nlp-taxonomy.owl#Sentiment_Analysis"/>
        <nlp-taxonomy:subFieldOf rdf:resource="http://nlpkg.sebis.cit.tum.de/nlp-taxonomy.owl#Text_Classification"/>
        <survey>https://doi.org/10.1017/9781108639286.005</survey>
        <survey>https://www.cs.uic.edu/~liub/FBS/NLP-handbook-sentiment-analysis.pdf</survey>
        <nlp-taxonomy:level rdf:datatype="http://www.w3.org/2001/XMLSchema#integer">2</nlp-taxonomy:level>
        <nlp-taxonomy:level rdf:datatype="http://www.w3.org/2001/XMLSchema#integer">3</nlp-taxonomy:level>
        <dcterms:description xml:lang="en">Subjectivity Classification refers to the process of determining whether a given text or sentence is subjective (expressing personal opinions, beliefs, emotions, judgments) or objective (providing factual information).</dcterms:description>
        <rdfs:label xml:lang="en">Subjectivity Classification</rdfs:label>
    </owl:NamedIndividual>
    


    <!-- http://nlpkg.sebis.cit.tum.de/nlp-fos-hierarchy.owl#Syntactic_Paths -->

    <owl:NamedIndividual rdf:about="http://nlpkg.sebis.cit.tum.de/nlp-fos-hierarchy.owl#Syntactic_Paths">
        <rdf:type rdf:resource="http://nlpkg.sebis.cit.tum.de/nlp-fos-hierarchy.owl#DataStructure"/>
        <rdf:type rdf:resource="http://nlpkg.sebis.cit.tum.de/nlp-taxonomy.owl#FieldOfStudy"/>
        <nlp-taxonomy:subFieldOf rdf:resource="http://nlpkg.sebis.cit.tum.de/nlp-fos-hierarchy.owl#Parse_Tree"/>
        <nlp-taxonomy:level rdf:datatype="http://www.w3.org/2001/XMLSchema#integer">6</nlp-taxonomy:level>
        <dcterms:description xml:lang="en">Syntactic Path refers to the grammatical relationships between words in a sentence. These paths are used to understand the structure of a sentence and the dependencies between words. They are often represented in a tree-like structure, known as a parse tree, where each node represents a word and the edges represent the syntactic relationships between words.</dcterms:description>
        <rdfs:label xml:lang="en">Syntactic Paths</rdfs:label>
    </owl:NamedIndividual>
    


    <!-- http://nlpkg.sebis.cit.tum.de/nlp-fos-hierarchy.owl#Syntactic_Treebank -->

    <owl:NamedIndividual rdf:about="http://nlpkg.sebis.cit.tum.de/nlp-fos-hierarchy.owl#Syntactic_Treebank">
        <rdf:type rdf:resource="http://nlpkg.sebis.cit.tum.de/nlp-fos-hierarchy.owl#DataStructure"/>
        <rdf:type rdf:resource="http://nlpkg.sebis.cit.tum.de/nlp-taxonomy.owl#FieldOfStudy"/>
        <uses rdf:resource="http://nlpkg.sebis.cit.tum.de/nlp-fos-hierarchy.owl#Parse_Tree"/>
        <nlp-taxonomy:subFieldOf rdf:resource="http://nlpkg.sebis.cit.tum.de/nlp-fos-hierarchy.owl#Treebank"/>
        <nlp-taxonomy:level rdf:datatype="http://www.w3.org/2001/XMLSchema#integer">6</nlp-taxonomy:level>
        <dcterms:description xml:lang="en">A &quot;Syntactic Treebank&quot; is a collection of sentences from a text corpus, where each sentence is parsed and represented as a syntactic tree. These trees break down the sentence&apos;s structure, showing how words and phrases relate to each other grammatically.</dcterms:description>
        <oboInOwl:hasSynonym xml:lang="en">Syntactic Tree-Bank</oboInOwl:hasSynonym>
        <rdfs:label xml:lang="en">Syntactic Treebank</rdfs:label>
    </owl:NamedIndividual>
    


    <!-- http://nlpkg.sebis.cit.tum.de/nlp-fos-hierarchy.owl#Syntax-based_Machine_Translation -->

    <owl:NamedIndividual rdf:about="http://nlpkg.sebis.cit.tum.de/nlp-fos-hierarchy.owl#Syntax-based_Machine_Translation">
        <rdf:type rdf:resource="http://nlpkg.sebis.cit.tum.de/nlp-fos-hierarchy.owl#Task"/>
        <rdf:type rdf:resource="http://nlpkg.sebis.cit.tum.de/nlp-taxonomy.owl#FieldOfStudy"/>
        <nlp-taxonomy:subFieldOf rdf:resource="http://nlpkg.sebis.cit.tum.de/nlp-fos-hierarchy.owl#Statistical_Machine_Translation"/>
        <nlp-taxonomy:superFieldOf rdf:resource="http://nlpkg.sebis.cit.tum.de/nlp-fos-hierarchy.owl#Hierarchical_Phrase-based_Machine_Translation"/>
        <nlp-taxonomy:level rdf:datatype="http://www.w3.org/2001/XMLSchema#integer">4</nlp-taxonomy:level>
        <dcterms:description xml:lang="en">Syntax-based Machine Translation is a type of machine translation approach that uses syntactic information from the source language to generate more accurate translations in the target language. It involves parsing the source language into a syntactic tree or structure, then transforming this into a similar structure in the target language, and finally generating the target language text from this structure. This approach can better handle differences in word order and grammatical structures between languages compared to phrase-based or word-based machine translation methods.</dcterms:description>
        <rdfs:label xml:lang="en">Syntax-based Machine Translation</rdfs:label>
    </owl:NamedIndividual>
    


    <!-- http://nlpkg.sebis.cit.tum.de/nlp-fos-hierarchy.owl#Table-to-Text -->

    <owl:NamedIndividual rdf:about="http://nlpkg.sebis.cit.tum.de/nlp-fos-hierarchy.owl#Table-to-Text">
        <rdf:type rdf:resource="http://nlpkg.sebis.cit.tum.de/nlp-fos-hierarchy.owl#Task"/>
        <rdf:type rdf:resource="http://nlpkg.sebis.cit.tum.de/nlp-taxonomy.owl#FieldOfStudy"/>
        <nlp-taxonomy:subFieldOf rdf:resource="http://nlpkg.sebis.cit.tum.de/nlp-taxonomy.owl#Data-to-Text_Generation"/>
        <nlp-taxonomy:level rdf:datatype="http://www.w3.org/2001/XMLSchema#integer">3</nlp-taxonomy:level>
        <nlp-taxonomy:level rdf:datatype="http://www.w3.org/2001/XMLSchema#integer">4</nlp-taxonomy:level>
        <dcterms:description xml:lang="en">Table-to-Text Generation is the task of generating natural language descriptions from tabular data.</dcterms:description>
        <oboInOwl:hasSynonym xml:lang="en">Table-to-Text Generation</oboInOwl:hasSynonym>
        <rdfs:label xml:lang="en">Table-to-Text</rdfs:label>
    </owl:NamedIndividual>
    


    <!-- http://nlpkg.sebis.cit.tum.de/nlp-fos-hierarchy.owl#Table_Question_Answering -->

    <owl:NamedIndividual rdf:about="http://nlpkg.sebis.cit.tum.de/nlp-fos-hierarchy.owl#Table_Question_Answering">
        <rdf:type rdf:resource="http://nlpkg.sebis.cit.tum.de/nlp-fos-hierarchy.owl#Task"/>
        <rdf:type rdf:resource="http://nlpkg.sebis.cit.tum.de/nlp-taxonomy.owl#FieldOfStudy"/>
        <nlp-taxonomy:subFieldOf rdf:resource="http://nlpkg.sebis.cit.tum.de/nlp-fos-hierarchy.owl#Knowledge_Base_Question_Answering"/>
        <survey>https://arxiv.org/abs/2207.05270</survey>
        <survey>https://arxiv.org/abs/2212.13465</survey>
        <nlp-taxonomy:level rdf:datatype="http://www.w3.org/2001/XMLSchema#integer">4</nlp-taxonomy:level>
        <nlp-taxonomy:level rdf:datatype="http://www.w3.org/2001/XMLSchema#integer">5</nlp-taxonomy:level>
        <dcterms:description xml:lang="en">Table Question Answering (Table QA) is a task that involves extracting answers from structured tabular data using natural language questions. It focuses on understanding and querying information stored in tables, such as databases or spreadsheets, to provide relevant responses to user queries.</dcterms:description>
        <oboInOwl:hasSynonym xml:lang="en">Table QA</oboInOwl:hasSynonym>
        <rdfs:label xml:lang="en">Table Question Answering</rdfs:label>
    </owl:NamedIndividual>
    


    <!-- http://nlpkg.sebis.cit.tum.de/nlp-fos-hierarchy.owl#Taxonomies -->

    <owl:NamedIndividual rdf:about="http://nlpkg.sebis.cit.tum.de/nlp-fos-hierarchy.owl#Taxonomies">
        <rdf:type rdf:resource="http://nlpkg.sebis.cit.tum.de/nlp-fos-hierarchy.owl#DataStructure"/>
        <rdf:type rdf:resource="http://nlpkg.sebis.cit.tum.de/nlp-taxonomy.owl#FieldOfStudy"/>
        <nlp-taxonomy:subFieldOf rdf:resource="http://nlpkg.sebis.cit.tum.de/nlp-fos-hierarchy.owl#Knowledge_Bases"/>
        <nlp-taxonomy:superFieldOf rdf:resource="http://nlpkg.sebis.cit.tum.de/nlp-fos-hierarchy.owl#Taxonomy_Learning"/>
        <nlp-taxonomy:level rdf:datatype="http://www.w3.org/2001/XMLSchema#integer">4</nlp-taxonomy:level>
        <dcterms:description xml:lang="en">Taxonomies are systems for classifying and organizing things or concepts, typically arranged in a hierarchical structure.</dcterms:description>
        <rdfs:label xml:lang="en">Taxonomies</rdfs:label>
    </owl:NamedIndividual>
    


    <!-- http://nlpkg.sebis.cit.tum.de/nlp-fos-hierarchy.owl#Taxonomy_Learning -->

    <owl:NamedIndividual rdf:about="http://nlpkg.sebis.cit.tum.de/nlp-fos-hierarchy.owl#Taxonomy_Learning">
        <rdf:type rdf:resource="http://nlpkg.sebis.cit.tum.de/nlp-fos-hierarchy.owl#Task"/>
        <rdf:type rdf:resource="http://nlpkg.sebis.cit.tum.de/nlp-taxonomy.owl#FieldOfStudy"/>
        <uses rdf:resource="http://nlpkg.sebis.cit.tum.de/nlp-taxonomy.owl#Coreference_Resolution"/>
        <uses rdf:resource="http://nlpkg.sebis.cit.tum.de/nlp-taxonomy.owl#Named_Entity_Recognition"/>
        <uses rdf:resource="http://nlpkg.sebis.cit.tum.de/nlp-taxonomy.owl#Relation_Extraction"/>
        <uses rdf:resource="http://nlpkg.sebis.cit.tum.de/nlp-taxonomy.owl#Term_Extraction"/>
        <nlp-taxonomy:subFieldOf rdf:resource="http://nlpkg.sebis.cit.tum.de/nlp-fos-hierarchy.owl#Taxonomies"/>
        <nlp-taxonomy:level rdf:datatype="http://www.w3.org/2001/XMLSchema#integer">5</nlp-taxonomy:level>
        <dcterms:description xml:lang="en">Taxonomy Learning refers to the process of automatically generating a hierarchical classification of concepts, entities or terms from a large amount of text data. It involves identifying relationships between different terms and organizing them into a tree-like structure, where each node represents a concept or category and each edge represents a relationship between two concepts.</dcterms:description>
        <rdfs:label xml:lang="en">Taxonomy Learning</rdfs:label>
    </owl:NamedIndividual>
    


    <!-- http://nlpkg.sebis.cit.tum.de/nlp-fos-hierarchy.owl#Text-to-Image -->

    <owl:NamedIndividual rdf:about="http://nlpkg.sebis.cit.tum.de/nlp-fos-hierarchy.owl#Text-to-Image">
        <rdf:type rdf:resource="http://nlpkg.sebis.cit.tum.de/nlp-fos-hierarchy.owl#Task"/>
        <rdf:type rdf:resource="http://nlpkg.sebis.cit.tum.de/nlp-taxonomy.owl#FieldOfStudy"/>
        <nlp-taxonomy:subFieldOf rdf:resource="http://nlpkg.sebis.cit.tum.de/nlp-taxonomy.owl#Visual_Data_In_NLP"/>
        <survey>https://arxiv.org/abs/1910.09399</survey>
        <survey>https://arxiv.org/abs/2204.13988</survey>
        <nlp-taxonomy:level rdf:datatype="http://www.w3.org/2001/XMLSchema#integer">3</nlp-taxonomy:level>
        <dcterms:description xml:lang="en">Text-to-Image refers to the process of generating visual content, such as images or illustrations, based on textual descriptions or input.</dcterms:description>
        <oboInOwl:hasSynonym xml:lang="en">Image Generation</oboInOwl:hasSynonym>
        <oboInOwl:hasSynonym xml:lang="en">T2I</oboInOwl:hasSynonym>
        <oboInOwl:hasSynonym xml:lang="en">Text to Image</oboInOwl:hasSynonym>
        <oboInOwl:hasSynonym xml:lang="en">Text to Image Generation</oboInOwl:hasSynonym>
        <oboInOwl:hasSynonym xml:lang="en">Text-to-Image Generation</oboInOwl:hasSynonym>
        <rdfs:label xml:lang="en">Text-to-Image</rdfs:label>
    </owl:NamedIndividual>
    


    <!-- http://nlpkg.sebis.cit.tum.de/nlp-fos-hierarchy.owl#Text-to-Image_Retrieval -->

    <owl:NamedIndividual rdf:about="http://nlpkg.sebis.cit.tum.de/nlp-fos-hierarchy.owl#Text-to-Image_Retrieval">
        <rdf:type rdf:resource="http://nlpkg.sebis.cit.tum.de/nlp-fos-hierarchy.owl#Task"/>
        <rdf:type rdf:resource="http://nlpkg.sebis.cit.tum.de/nlp-taxonomy.owl#FieldOfStudy"/>
        <nlp-taxonomy:subFieldOf rdf:resource="http://nlpkg.sebis.cit.tum.de/nlp-taxonomy.owl#Information_Retrieval"/>
        <nlp-taxonomy:subFieldOf rdf:resource="http://nlpkg.sebis.cit.tum.de/nlp-taxonomy.owl#Visual_Data_In_NLP"/>
        <survey>https://arxiv.org/abs/2203.14713</survey>
        <nlp-taxonomy:level rdf:datatype="http://www.w3.org/2001/XMLSchema#integer">2</nlp-taxonomy:level>
        <nlp-taxonomy:level rdf:datatype="http://www.w3.org/2001/XMLSchema#integer">3</nlp-taxonomy:level>
        <dcterms:description xml:lang="en">Text-to-Image Retrieval refers to the process of finding and retrieving relevant images based on a given text query. It involves using natural language processing techniques to understand textual descriptions and then searching for images that best match or represent the content described in the text.</dcterms:description>
        <oboInOwl:hasSynonym xml:lang="en">T2I Retrieval</oboInOwl:hasSynonym>
        <oboInOwl:hasSynonym xml:lang="en">TIR</oboInOwl:hasSynonym>
        <oboInOwl:hasSynonym xml:lang="en">Text to Image Retrieval</oboInOwl:hasSynonym>
        <oboInOwl:hasSynonym xml:lang="en">Text-Image Retrieval</oboInOwl:hasSynonym>
        <rdfs:label xml:lang="en">Text-to-Image Retrieval</rdfs:label>
    </owl:NamedIndividual>
    


    <!-- http://nlpkg.sebis.cit.tum.de/nlp-fos-hierarchy.owl#Text-to-SQL -->

    <owl:NamedIndividual rdf:about="http://nlpkg.sebis.cit.tum.de/nlp-fos-hierarchy.owl#Text-to-SQL">
        <rdf:type rdf:resource="http://nlpkg.sebis.cit.tum.de/nlp-fos-hierarchy.owl#Task"/>
        <rdf:type rdf:resource="http://nlpkg.sebis.cit.tum.de/nlp-taxonomy.owl#FieldOfStudy"/>
        <nlp-taxonomy:subFieldOf rdf:resource="http://nlpkg.sebis.cit.tum.de/nlp-taxonomy.owl#Code_Generation"/>
        <survey>https://aclanthology.org/2022.coling-1.190</survey>
        <survey>https://arxiv.org/abs/2005.07667</survey>
        <survey>https://arxiv.org/abs/2208.04415</survey>
        <survey>https://arxiv.org/abs/2208.13629</survey>
        <nlp-taxonomy:level rdf:datatype="http://www.w3.org/2001/XMLSchema#integer">3</nlp-taxonomy:level>
        <nlp-taxonomy:level rdf:datatype="http://www.w3.org/2001/XMLSchema#integer">4</nlp-taxonomy:level>
        <dcterms:description xml:lang="en">Text-to-SQL is a task where the goal is to automatically generate SQL queries from natural language text. The task involves converting the text input into a semantically correct SQL query that can be executed on a database.</dcterms:description>
        <oboInOwl:hasSynonym xml:lang="en">SQL Generation</oboInOwl:hasSynonym>
        <oboInOwl:hasSynonym xml:lang="en">SQL Query Generation</oboInOwl:hasSynonym>
        <rdfs:label xml:lang="en">Text-to-SQL</rdfs:label>
    </owl:NamedIndividual>
    


    <!-- http://nlpkg.sebis.cit.tum.de/nlp-fos-hierarchy.owl#Text-to-Structured_Data -->

    <owl:NamedIndividual rdf:about="http://nlpkg.sebis.cit.tum.de/nlp-fos-hierarchy.owl#Text-to-Structured_Data">
        <rdf:type rdf:resource="http://nlpkg.sebis.cit.tum.de/nlp-fos-hierarchy.owl#Task"/>
        <rdf:type rdf:resource="http://nlpkg.sebis.cit.tum.de/nlp-taxonomy.owl#FieldOfStudy"/>
        <nlp-taxonomy:subFieldOf rdf:resource="http://nlpkg.sebis.cit.tum.de/nlp-taxonomy.owl#Structured_Data_In_NLP"/>
        <nlp-taxonomy:level rdf:datatype="http://www.w3.org/2001/XMLSchema#integer">3</nlp-taxonomy:level>
        <dcterms:description xml:lang="en">Text-to-Structured Data refers to the process of converting unstructured or semi-structured textual information into a structured format that can be more easily analyzed, processed, and stored by computers. This conversion involves extracting meaningful data and organizing it into a structured representation, typically in the form of a database, spreadsheet, or some other structured data format.</dcterms:description>
        <oboInOwl:hasSynonym xml:lang="en">Text-to-Data</oboInOwl:hasSynonym>
        <oboInOwl:hasSynonym xml:lang="en">Text2Data</oboInOwl:hasSynonym>
        <rdfs:label xml:lang="en">Text-to-Structured Data</rdfs:label>
    </owl:NamedIndividual>
    


    <!-- http://nlpkg.sebis.cit.tum.de/nlp-fos-hierarchy.owl#Text-to-Video -->

    <owl:NamedIndividual rdf:about="http://nlpkg.sebis.cit.tum.de/nlp-fos-hierarchy.owl#Text-to-Video">
        <rdf:type rdf:resource="http://nlpkg.sebis.cit.tum.de/nlp-fos-hierarchy.owl#Task"/>
        <rdf:type rdf:resource="http://nlpkg.sebis.cit.tum.de/nlp-taxonomy.owl#FieldOfStudy"/>
        <nlp-taxonomy:subFieldOf rdf:resource="http://nlpkg.sebis.cit.tum.de/nlp-taxonomy.owl#Visual_Data_In_NLP"/>
        <nlp-taxonomy:level rdf:datatype="http://www.w3.org/2001/XMLSchema#integer">3</nlp-taxonomy:level>
        <dcterms:description xml:lang="en">Text-to-Video is a process that involves generating video content from textual input or descriptions.</dcterms:description>
        <oboInOwl:hasSynonym xml:lang="en">Text to Video</oboInOwl:hasSynonym>
        <oboInOwl:hasSynonym xml:lang="en">Text to Video generation</oboInOwl:hasSynonym>
        <oboInOwl:hasSynonym xml:lang="en">Text-to-Video Generation</oboInOwl:hasSynonym>
        <oboInOwl:hasSynonym xml:lang="en">Video Generation</oboInOwl:hasSynonym>
        <rdfs:label xml:lang="en">Text-to-Video</rdfs:label>
    </owl:NamedIndividual>
    


    <!-- http://nlpkg.sebis.cit.tum.de/nlp-fos-hierarchy.owl#Text_Embeddings -->

    <owl:NamedIndividual rdf:about="http://nlpkg.sebis.cit.tum.de/nlp-fos-hierarchy.owl#Text_Embeddings">
        <rdf:type rdf:resource="http://nlpkg.sebis.cit.tum.de/nlp-fos-hierarchy.owl#DataStructure"/>
        <rdf:type rdf:resource="http://nlpkg.sebis.cit.tum.de/nlp-taxonomy.owl#FieldOfStudy"/>
        <usedFor rdf:resource="http://nlpkg.sebis.cit.tum.de/nlp-fos-hierarchy.owl#Bilingual_Lexicon_Induction"/>
        <nlp-taxonomy:subFieldOf rdf:resource="http://nlpkg.sebis.cit.tum.de/nlp-fos-hierarchy.owl#Text_Representations"/>
        <nlp-taxonomy:superFieldOf rdf:resource="http://nlpkg.sebis.cit.tum.de/nlp-fos-hierarchy.owl#Contextualized_Embeddings"/>
        <nlp-taxonomy:superFieldOf rdf:resource="http://nlpkg.sebis.cit.tum.de/nlp-fos-hierarchy.owl#Dense_Embeddings"/>
        <nlp-taxonomy:superFieldOf rdf:resource="http://nlpkg.sebis.cit.tum.de/nlp-fos-hierarchy.owl#Sentence_Embeddings"/>
        <nlp-taxonomy:superFieldOf rdf:resource="http://nlpkg.sebis.cit.tum.de/nlp-fos-hierarchy.owl#Sparse_Embeddings"/>
        <nlp-taxonomy:superFieldOf rdf:resource="http://nlpkg.sebis.cit.tum.de/nlp-fos-hierarchy.owl#Static_Embeddings"/>
        <nlp-taxonomy:superFieldOf rdf:resource="http://nlpkg.sebis.cit.tum.de/nlp-fos-hierarchy.owl#Word_Embeddings"/>
        <relevantInformation>https://web.stanford.edu/~jurafsky/slp3/6.pdf</relevantInformation>
        <survey>https://aclanthology.org/2020.lrec-1.583</survey>
        <survey>https://aclanthology.org/Q19-1027</survey>
        <nlp-taxonomy:level rdf:datatype="http://www.w3.org/2001/XMLSchema#integer">4</nlp-taxonomy:level>
        <dcterms:description xml:lang="en">Text Embeddings refer to the representation of text in the form of vectors. The underlying idea is to convert text into a numerical form that can be easily processed by machines. These embeddings capture the semantic meaning or context of words or sentences, where similar words or sentences are closer in the vector space.</dcterms:description>
        <rdfs:label xml:lang="en">Text Embeddings</rdfs:label>
    </owl:NamedIndividual>
    


    <!-- http://nlpkg.sebis.cit.tum.de/nlp-fos-hierarchy.owl#Text_Regression -->

    <owl:NamedIndividual rdf:about="http://nlpkg.sebis.cit.tum.de/nlp-fos-hierarchy.owl#Text_Regression">
        <rdf:type rdf:resource="http://nlpkg.sebis.cit.tum.de/nlp-fos-hierarchy.owl#Task"/>
        <rdf:type rdf:resource="http://nlpkg.sebis.cit.tum.de/nlp-taxonomy.owl#FieldOfStudy"/>
        <nlp-taxonomy:subFieldOf rdf:resource="http://nlpkg.sebis.cit.tum.de/nlp-taxonomy.owl#Information_Retrieval"/>
        <nlp-taxonomy:subFieldOf rdf:resource="http://nlpkg.sebis.cit.tum.de/nlp-taxonomy.owl#Information_Extraction_&amp;_Text_Mining"/>
        <nlp-taxonomy:superFieldOf rdf:resource="http://nlpkg.sebis.cit.tum.de/nlp-fos-hierarchy.owl#Automatic_Essay_Scoring"/>
        <nlp-taxonomy:level rdf:datatype="http://www.w3.org/2001/XMLSchema#integer">2</nlp-taxonomy:level>
        <dcterms:description xml:lang="en">Text Regression refers to the application of regression analysis on text data. It involves predicting a continuous value (like a rating or a price) based on text data.</dcterms:description>
        <oboInOwl:hasSynonym xml:lang="en">Regression</oboInOwl:hasSynonym>
        <oboInOwl:hasSynonym xml:lang="en">Textual Regression</oboInOwl:hasSynonym>
        <rdfs:label xml:lang="en">Text Regression</rdfs:label>
    </owl:NamedIndividual>
    


    <!-- http://nlpkg.sebis.cit.tum.de/nlp-fos-hierarchy.owl#Text_Representations -->

    <owl:NamedIndividual rdf:about="http://nlpkg.sebis.cit.tum.de/nlp-fos-hierarchy.owl#Text_Representations">
        <rdf:type rdf:resource="http://nlpkg.sebis.cit.tum.de/nlp-fos-hierarchy.owl#DataStructure"/>
        <rdf:type rdf:resource="http://nlpkg.sebis.cit.tum.de/nlp-taxonomy.owl#FieldOfStudy"/>
        <usedFor rdf:resource="http://nlpkg.sebis.cit.tum.de/nlp-taxonomy.owl#Semantic_Search"/>
        <usedFor rdf:resource="http://nlpkg.sebis.cit.tum.de/nlp-taxonomy.owl#Text_Clustering"/>
        <nlp-taxonomy:subFieldOf rdf:resource="http://nlpkg.sebis.cit.tum.de/nlp-taxonomy.owl#Knowledge_Representation"/>
        <nlp-taxonomy:subFieldOf rdf:resource="http://nlpkg.sebis.cit.tum.de/nlp-taxonomy.owl#Representation_Learning"/>
        <nlp-taxonomy:superFieldOf rdf:resource="http://nlpkg.sebis.cit.tum.de/nlp-fos-hierarchy.owl#Abstract_Meaning_Representation"/>
        <nlp-taxonomy:superFieldOf rdf:resource="http://nlpkg.sebis.cit.tum.de/nlp-fos-hierarchy.owl#Text_Embeddings"/>
        <survey>https://aclanthology.org/2020.wnut-1.27</survey>
        <survey>https://arxiv.org/abs/1702.00764</survey>
        <survey>https://arxiv.org/abs/2211.14591</survey>
        <nlp-taxonomy:level rdf:datatype="http://www.w3.org/2001/XMLSchema#integer">3</nlp-taxonomy:level>
        <dcterms:description xml:lang="en">Text Representations aim to capture the semantic meaning, context, or sentiment of texts so they can be understood and processed by machines.</dcterms:description>
        <rdfs:label xml:lang="en">Text Representations</rdfs:label>
    </owl:NamedIndividual>
    


    <!-- http://nlpkg.sebis.cit.tum.de/nlp-fos-hierarchy.owl#Text_Scrubbing -->

    <owl:NamedIndividual rdf:about="http://nlpkg.sebis.cit.tum.de/nlp-fos-hierarchy.owl#Text_Scrubbing">
        <rdf:type rdf:resource="http://nlpkg.sebis.cit.tum.de/nlp-fos-hierarchy.owl#Task"/>
        <rdf:type rdf:resource="http://nlpkg.sebis.cit.tum.de/nlp-taxonomy.owl#FieldOfStudy"/>
        <nlp-taxonomy:subFieldOf rdf:resource="http://nlpkg.sebis.cit.tum.de/nlp-taxonomy.owl#Text_Normalization"/>
        <nlp-taxonomy:level rdf:datatype="http://www.w3.org/2001/XMLSchema#integer">3</nlp-taxonomy:level>
        <dcterms:description xml:lang="en">Text Scrubbing transforms or maps data into a format that can be easily analyzed. This may include removing punctuation, numbers, special characters, converting all text to lower or upper case, removing stop words, stemming, lemmatization, etc.</dcterms:description>
        <rdfs:label xml:lang="en">Text Scrubbing</rdfs:label>
    </owl:NamedIndividual>
    


    <!-- http://nlpkg.sebis.cit.tum.de/nlp-fos-hierarchy.owl#Text_Simplification -->

    <owl:NamedIndividual rdf:about="http://nlpkg.sebis.cit.tum.de/nlp-fos-hierarchy.owl#Text_Simplification">
        <rdf:type rdf:resource="http://nlpkg.sebis.cit.tum.de/nlp-fos-hierarchy.owl#Task"/>
        <rdf:type rdf:resource="http://nlpkg.sebis.cit.tum.de/nlp-taxonomy.owl#FieldOfStudy"/>
        <nlp-taxonomy:subFieldOf rdf:resource="http://nlpkg.sebis.cit.tum.de/nlp-taxonomy.owl#Paraphrasing"/>
        <nlp-taxonomy:superFieldOf rdf:resource="http://nlpkg.sebis.cit.tum.de/nlp-fos-hierarchy.owl#Lexical_Simplification"/>
        <survey>https://aclanthology.org/2020.cl-1.4</survey>
        <survey>https://aclanthology.org/2023.ranlp-1.36</survey>
        <nlp-taxonomy:level rdf:datatype="http://www.w3.org/2001/XMLSchema#integer">3</nlp-taxonomy:level>
        <dcterms:description xml:lang="en">Text Simplification (TS) is the process of transforming complex text into a simpler version that retains the original meaning. It involves reducing the linguistic complexity of the text, making it easier to read and understand. This can include simplifying vocabulary, grammar, or sentence structure. It&apos;s particularly useful for aiding language learning, improving readability for people with cognitive disabilities, or for processing text in machine learning algorithms.</dcterms:description>
        <oboInOwl:hasSynonym xml:lang="en">Sentence Simplification</oboInOwl:hasSynonym>
        <oboInOwl:hasSynonym xml:lang="en">TS</oboInOwl:hasSynonym>
        <rdfs:label xml:lang="en">Text Simplification</rdfs:label>
    </owl:NamedIndividual>
    


    <!-- http://nlpkg.sebis.cit.tum.de/nlp-fos-hierarchy.owl#Thesaurus -->

    <owl:NamedIndividual rdf:about="http://nlpkg.sebis.cit.tum.de/nlp-fos-hierarchy.owl#Thesaurus">
        <rdf:type rdf:resource="http://nlpkg.sebis.cit.tum.de/nlp-fos-hierarchy.owl#DataStructure"/>
        <rdf:type rdf:resource="http://nlpkg.sebis.cit.tum.de/nlp-taxonomy.owl#FieldOfStudy"/>
        <nlp-taxonomy:subFieldOf rdf:resource="http://nlpkg.sebis.cit.tum.de/nlp-fos-hierarchy.owl#Knowledge_Bases"/>
        <nlp-taxonomy:level rdf:datatype="http://www.w3.org/2001/XMLSchema#integer">4</nlp-taxonomy:level>
        <dcterms:description xml:lang="en">Thesaurus is a tool that lists words grouped together according to similarity of meaning. It is used for identifying synonyms, antonyms, and related terms to enhance the understanding and processing of language data.</dcterms:description>
        <rdfs:label xml:lang="en">Thesaurus</rdfs:label>
    </owl:NamedIndividual>
    


    <!-- http://nlpkg.sebis.cit.tum.de/nlp-fos-hierarchy.owl#Tokenization -->

    <owl:NamedIndividual rdf:about="http://nlpkg.sebis.cit.tum.de/nlp-fos-hierarchy.owl#Tokenization">
        <rdf:type rdf:resource="http://nlpkg.sebis.cit.tum.de/nlp-fos-hierarchy.owl#Task"/>
        <rdf:type rdf:resource="http://nlpkg.sebis.cit.tum.de/nlp-taxonomy.owl#FieldOfStudy"/>
        <usedFor rdf:resource="http://nlpkg.sebis.cit.tum.de/nlp-taxonomy.owl#Language_Models"/>
        <nlp-taxonomy:subFieldOf rdf:resource="http://nlpkg.sebis.cit.tum.de/nlp-taxonomy.owl#Text_Segmentation"/>
        <relevantInformation>https://huggingface.co/docs/transformers/tokenizer_summary</relevantInformation>
        <nlp-taxonomy:level rdf:datatype="http://www.w3.org/2001/XMLSchema#integer">3</nlp-taxonomy:level>
        <dcterms:description xml:lang="en">Tokenization is the process of breaking down a large paragraph of text into smaller parts, known as tokens. These tokens can be morphemes, word pieces, words, phrases, or sentences.</dcterms:description>
        <rdfs:label xml:lang="en">Tokenization</rdfs:label>
    </owl:NamedIndividual>
    


    <!-- http://nlpkg.sebis.cit.tum.de/nlp-fos-hierarchy.owl#Topic_Classification -->

    <owl:NamedIndividual rdf:about="http://nlpkg.sebis.cit.tum.de/nlp-fos-hierarchy.owl#Topic_Classification">
        <rdf:type rdf:resource="http://nlpkg.sebis.cit.tum.de/nlp-fos-hierarchy.owl#Task"/>
        <rdf:type rdf:resource="http://nlpkg.sebis.cit.tum.de/nlp-taxonomy.owl#FieldOfStudy"/>
        <nlp-taxonomy:subFieldOf rdf:resource="http://nlpkg.sebis.cit.tum.de/nlp-taxonomy.owl#Text_Classification"/>
        <nlp-taxonomy:level rdf:datatype="http://www.w3.org/2001/XMLSchema#integer">3</nlp-taxonomy:level>
        <dcterms:description xml:lang="en">Topic Classification is a machine learning technique used to categorize text or spoken language into predefined topics or categories. It involves training a model on a set of labeled texts, each associated with one or more topics. Once trained, the model can then be used to predict the topics of new, unseen texts.</dcterms:description>
        <rdfs:label xml:lang="en">Topic Classification</rdfs:label>
    </owl:NamedIndividual>
    


    <!-- http://nlpkg.sebis.cit.tum.de/nlp-fos-hierarchy.owl#Translation_Memory -->

    <owl:NamedIndividual rdf:about="http://nlpkg.sebis.cit.tum.de/nlp-fos-hierarchy.owl#Translation_Memory">
        <rdf:type rdf:resource="http://nlpkg.sebis.cit.tum.de/nlp-fos-hierarchy.owl#DataStructure"/>
        <rdf:type rdf:resource="http://nlpkg.sebis.cit.tum.de/nlp-taxonomy.owl#FieldOfStudy"/>
        <usedFor rdf:resource="http://nlpkg.sebis.cit.tum.de/nlp-taxonomy.owl#Machine_Translation"/>
        <uses rdf:resource="http://nlpkg.sebis.cit.tum.de/nlp-fos-hierarchy.owl#Bilingual_Lexicon_Induction"/>
        <nlp-taxonomy:subFieldOf rdf:resource="http://nlpkg.sebis.cit.tum.de/nlp-fos-hierarchy.owl#Dictionary"/>
        <nlp-taxonomy:level rdf:datatype="http://www.w3.org/2001/XMLSchema#integer">5</nlp-taxonomy:level>
        <dcterms:description xml:lang="en">Translation Memory (TM) is a database that stores sentences, paragraphs, or segments of text that have been previously translated, to aid in the translation of new texts. It allows for the reuse of translations, improving translation efficiency and consistency.</dcterms:description>
        <rdfs:label xml:lang="en">Translation Memory</rdfs:label>
    </owl:NamedIndividual>
    


    <!-- http://nlpkg.sebis.cit.tum.de/nlp-fos-hierarchy.owl#Tree -->

    <owl:NamedIndividual rdf:about="http://nlpkg.sebis.cit.tum.de/nlp-fos-hierarchy.owl#Tree">
        <rdf:type rdf:resource="http://nlpkg.sebis.cit.tum.de/nlp-fos-hierarchy.owl#DataStructure"/>
        <rdf:type rdf:resource="http://nlpkg.sebis.cit.tum.de/nlp-taxonomy.owl#FieldOfStudy"/>
        <nlp-taxonomy:subFieldOf rdf:resource="http://nlpkg.sebis.cit.tum.de/nlp-fos-hierarchy.owl#Knowledge_Bases"/>
        <nlp-taxonomy:superFieldOf rdf:resource="http://nlpkg.sebis.cit.tum.de/nlp-fos-hierarchy.owl#Constituency_Tree"/>
        <nlp-taxonomy:superFieldOf rdf:resource="http://nlpkg.sebis.cit.tum.de/nlp-fos-hierarchy.owl#Parse_Tree"/>
        <nlp-taxonomy:superFieldOf rdf:resource="http://nlpkg.sebis.cit.tum.de/nlp-fos-hierarchy.owl#Rhetorical_Structure_Theory_Discourse_Tree"/>
        <nlp-taxonomy:superFieldOf rdf:resource="http://nlpkg.sebis.cit.tum.de/nlp-fos-hierarchy.owl#Treebank"/>
        <nlp-taxonomy:level rdf:datatype="http://www.w3.org/2001/XMLSchema#integer">4</nlp-taxonomy:level>
        <dcterms:description xml:lang="en">Tree typically refers to a hierarchical data structure.</dcterms:description>
        <rdfs:label xml:lang="en">Tree</rdfs:label>
    </owl:NamedIndividual>
    


    <!-- http://nlpkg.sebis.cit.tum.de/nlp-fos-hierarchy.owl#Tree_Fragments -->

    <owl:NamedIndividual rdf:about="http://nlpkg.sebis.cit.tum.de/nlp-fos-hierarchy.owl#Tree_Fragments">
        <rdf:type rdf:resource="http://nlpkg.sebis.cit.tum.de/nlp-fos-hierarchy.owl#DataStructure"/>
        <rdf:type rdf:resource="http://nlpkg.sebis.cit.tum.de/nlp-taxonomy.owl#FieldOfStudy"/>
        <nlp-taxonomy:subFieldOf rdf:resource="http://nlpkg.sebis.cit.tum.de/nlp-fos-hierarchy.owl#Parse_Tree"/>
        <nlp-taxonomy:level rdf:datatype="http://www.w3.org/2001/XMLSchema#integer">6</nlp-taxonomy:level>
        <dcterms:description xml:lang="en">Tree Fragments refer to smaller parts or substructures of a parse tree. A parse tree represents the syntactic structure of a sentence according to a particular grammar.</dcterms:description>
        <rdfs:label xml:lang="en">Tree Fragments</rdfs:label>
    </owl:NamedIndividual>
    


    <!-- http://nlpkg.sebis.cit.tum.de/nlp-fos-hierarchy.owl#Treebank -->

    <owl:NamedIndividual rdf:about="http://nlpkg.sebis.cit.tum.de/nlp-fos-hierarchy.owl#Treebank">
        <rdf:type rdf:resource="http://nlpkg.sebis.cit.tum.de/nlp-fos-hierarchy.owl#DataStructure"/>
        <rdf:type rdf:resource="http://nlpkg.sebis.cit.tum.de/nlp-taxonomy.owl#FieldOfStudy"/>
        <nlp-taxonomy:subFieldOf rdf:resource="http://nlpkg.sebis.cit.tum.de/nlp-fos-hierarchy.owl#Tree"/>
        <nlp-taxonomy:superFieldOf rdf:resource="http://nlpkg.sebis.cit.tum.de/nlp-fos-hierarchy.owl#Semantic_Treebank"/>
        <nlp-taxonomy:superFieldOf rdf:resource="http://nlpkg.sebis.cit.tum.de/nlp-fos-hierarchy.owl#Syntactic_Treebank"/>
        <nlp-taxonomy:level rdf:datatype="http://www.w3.org/2001/XMLSchema#integer">5</nlp-taxonomy:level>
        <dcterms:description xml:lang="en">A Treebank is a corpus or collection of text samples that have been manually annotated usually with syntactic or grammatical structure in the form of parse trees. These parse trees represent the hierarchical structure of sentences, showing how words are related and organized in phrases and clauses. In addition to syntactic treebanks, semantic treebanks combine syntactical trees of sentences with the formal representation of their meaning in logical form.</dcterms:description>
        <oboInOwl:hasSynonym xml:lang="en">Tree-Bank</oboInOwl:hasSynonym>
        <rdfs:label xml:lang="en">Treebank</rdfs:label>
    </owl:NamedIndividual>
    


    <!-- http://nlpkg.sebis.cit.tum.de/nlp-fos-hierarchy.owl#Triple_Classification -->

    <owl:NamedIndividual rdf:about="http://nlpkg.sebis.cit.tum.de/nlp-fos-hierarchy.owl#Triple_Classification">
        <rdf:type rdf:resource="http://nlpkg.sebis.cit.tum.de/nlp-fos-hierarchy.owl#Task"/>
        <rdf:type rdf:resource="http://nlpkg.sebis.cit.tum.de/nlp-taxonomy.owl#FieldOfStudy"/>
        <nlp-taxonomy:subFieldOf rdf:resource="http://nlpkg.sebis.cit.tum.de/nlp-taxonomy.owl#Knowledge_Graph_Reasoning"/>
        <nlp-taxonomy:level rdf:datatype="http://www.w3.org/2001/XMLSchema#integer">3</nlp-taxonomy:level>
        <nlp-taxonomy:level rdf:datatype="http://www.w3.org/2001/XMLSchema#integer">7</nlp-taxonomy:level>
        <dcterms:description xml:lang="en">Triple Classification is a task of determining whether a given triple (subject, predicate, object) is correct or not based on the existing knowledge in the graph. It is a binary classification problem where the goal is to predict if a triple is true (exists in the graph) or false (does not exist in the graph).</dcterms:description>
        <rdfs:label xml:lang="en">Triple Classification</rdfs:label>
    </owl:NamedIndividual>
    


    <!-- http://nlpkg.sebis.cit.tum.de/nlp-fos-hierarchy.owl#Unsupervised_Learning -->

    <owl:NamedIndividual rdf:about="http://nlpkg.sebis.cit.tum.de/nlp-fos-hierarchy.owl#Unsupervised_Learning">
        <rdf:type rdf:resource="http://nlpkg.sebis.cit.tum.de/nlp-fos-hierarchy.owl#Task"/>
        <rdf:type rdf:resource="http://nlpkg.sebis.cit.tum.de/nlp-taxonomy.owl#FieldOfStudy"/>
        <nlp-taxonomy:subFieldOf rdf:resource="http://nlpkg.sebis.cit.tum.de/nlp-taxonomy.owl#Low-Resource_NLP"/>
        <nlp-taxonomy:superFieldOf rdf:resource="http://nlpkg.sebis.cit.tum.de/nlp-taxonomy.owl#Text_Clustering"/>
        <survey>https://aclanthology.org/2020.wnut-1.27</survey>
        <survey>https://aclanthology.org/W11-2205</survey>
        <survey>https://arxiv.org/abs/2211.16285</survey>
        <nlp-taxonomy:level rdf:datatype="http://www.w3.org/2001/XMLSchema#integer">3</nlp-taxonomy:level>
        <dcterms:description xml:lang="en">Unsupervised Learning refers to the machine learning task where a model learns and identifies patterns directly from unlabelled text data. This method does not require a predefined set of labels or training data.</dcterms:description>
        <oboInOwl:hasSynonym xml:lang="en">Unsupervised</oboInOwl:hasSynonym>
        <rdfs:label xml:lang="en">Unsupervised Learning</rdfs:label>
    </owl:NamedIndividual>
    


    <!-- http://nlpkg.sebis.cit.tum.de/nlp-fos-hierarchy.owl#Verdict_Prediction -->

    <owl:NamedIndividual rdf:about="http://nlpkg.sebis.cit.tum.de/nlp-fos-hierarchy.owl#Verdict_Prediction">
        <rdf:type rdf:resource="http://nlpkg.sebis.cit.tum.de/nlp-fos-hierarchy.owl#Task"/>
        <rdf:type rdf:resource="http://nlpkg.sebis.cit.tum.de/nlp-taxonomy.owl#FieldOfStudy"/>
        <nlp-taxonomy:subFieldOf rdf:resource="http://nlpkg.sebis.cit.tum.de/nlp-fos-hierarchy.owl#Claim_Verification"/>
        <nlp-taxonomy:subFieldOf rdf:resource="http://nlpkg.sebis.cit.tum.de/nlp-taxonomy.owl#Text_Classification"/>
        <nlp-taxonomy:level rdf:datatype="http://www.w3.org/2001/XMLSchema#integer">3</nlp-taxonomy:level>
        <nlp-taxonomy:level rdf:datatype="http://www.w3.org/2001/XMLSchema#integer">5</nlp-taxonomy:level>
        <dcterms:description xml:lang="en">Verdict Prediction attempts to determine the veracity of a claim. The simplest approach is binary classification, for example, labeling a claim as true or false.</dcterms:description>
        <rdfs:label xml:lang="en">Verdict Prediction</rdfs:label>
    </owl:NamedIndividual>
    


    <!-- http://nlpkg.sebis.cit.tum.de/nlp-fos-hierarchy.owl#Video-Text_Retrieval -->

    <owl:NamedIndividual rdf:about="http://nlpkg.sebis.cit.tum.de/nlp-fos-hierarchy.owl#Video-Text_Retrieval">
        <rdf:type rdf:resource="http://nlpkg.sebis.cit.tum.de/nlp-fos-hierarchy.owl#Task"/>
        <rdf:type rdf:resource="http://nlpkg.sebis.cit.tum.de/nlp-taxonomy.owl#FieldOfStudy"/>
        <nlp-taxonomy:subFieldOf rdf:resource="http://nlpkg.sebis.cit.tum.de/nlp-taxonomy.owl#Information_Retrieval"/>
        <nlp-taxonomy:subFieldOf rdf:resource="http://nlpkg.sebis.cit.tum.de/nlp-taxonomy.owl#Visual_Data_In_NLP"/>
        <survey>https://arxiv.org/abs/2302.12552</survey>
        <nlp-taxonomy:level rdf:datatype="http://www.w3.org/2001/XMLSchema#integer">2</nlp-taxonomy:level>
        <nlp-taxonomy:level rdf:datatype="http://www.w3.org/2001/XMLSchema#integer">3</nlp-taxonomy:level>
        <dcterms:description xml:lang="en">Video-Text Retrieval (VTR) aims to search for the most relevant video related to the semantics in a given sentence, and vice versa.</dcterms:description>
        <oboInOwl:hasSynonym xml:lang="en">VTR</oboInOwl:hasSynonym>
        <rdfs:label xml:lang="en">Video-Text Retrieval</rdfs:label>
    </owl:NamedIndividual>
    


    <!-- http://nlpkg.sebis.cit.tum.de/nlp-fos-hierarchy.owl#Video_Captioning -->

    <owl:NamedIndividual rdf:about="http://nlpkg.sebis.cit.tum.de/nlp-fos-hierarchy.owl#Video_Captioning">
        <rdf:type rdf:resource="http://nlpkg.sebis.cit.tum.de/nlp-fos-hierarchy.owl#Task"/>
        <rdf:type rdf:resource="http://nlpkg.sebis.cit.tum.de/nlp-taxonomy.owl#FieldOfStudy"/>
        <nlp-taxonomy:subFieldOf rdf:resource="http://nlpkg.sebis.cit.tum.de/nlp-taxonomy.owl#Captioning"/>
        <nlp-taxonomy:subFieldOf rdf:resource="http://nlpkg.sebis.cit.tum.de/nlp-taxonomy.owl#Visual_Data_In_NLP"/>
        <nlp-taxonomy:superFieldOf rdf:resource="http://nlpkg.sebis.cit.tum.de/nlp-fos-hierarchy.owl#Sign_Language_Recognition"/>
        <survey>https://arxiv.org/abs/2011.14752</survey>
        <survey>https://arxiv.org/abs/2103.14785</survey>
        <nlp-taxonomy:level rdf:datatype="http://www.w3.org/2001/XMLSchema#integer">3</nlp-taxonomy:level>
        <dcterms:description xml:lang="en">Video captioning is the process of adding textual descriptions or subtitles to a video, typically in real-time or as a post-production step. The primary purpose of video captioning is to make video content accessible to a wider audience, including those who are deaf or hard of hearing, as well as non-native speakers and individuals in noisy environments where audio may be difficult to hear.</dcterms:description>
        <oboInOwl:hasSynonym xml:lang="en">Video-to-Text</oboInOwl:hasSynonym>
        <rdfs:label xml:lang="en">Video Captioning</rdfs:label>
    </owl:NamedIndividual>
    


    <!-- http://nlpkg.sebis.cit.tum.de/nlp-fos-hierarchy.owl#Video_Question_Answering -->

    <owl:NamedIndividual rdf:about="http://nlpkg.sebis.cit.tum.de/nlp-fos-hierarchy.owl#Video_Question_Answering">
        <rdf:type rdf:resource="http://nlpkg.sebis.cit.tum.de/nlp-fos-hierarchy.owl#Task"/>
        <rdf:type rdf:resource="http://nlpkg.sebis.cit.tum.de/nlp-taxonomy.owl#FieldOfStudy"/>
        <nlp-taxonomy:subFieldOf rdf:resource="http://nlpkg.sebis.cit.tum.de/nlp-fos-hierarchy.owl#Visual_Question_Answering"/>
        <nlp-taxonomy:level rdf:datatype="http://www.w3.org/2001/XMLSchema#integer">4</nlp-taxonomy:level>
        <dcterms:description xml:lang="en">Video Question Answering (VideoQA) aims to answer natural language questions related to the content of a given video.</dcterms:description>
        <oboInOwl:hasSynonym xml:lang="en">VideoQA</oboInOwl:hasSynonym>
        <rdfs:label xml:lang="en">Video Question Answering</rdfs:label>
    </owl:NamedIndividual>
    


    <!-- http://nlpkg.sebis.cit.tum.de/nlp-fos-hierarchy.owl#Vision-specific_Language_Models -->

    <owl:NamedIndividual rdf:about="http://nlpkg.sebis.cit.tum.de/nlp-fos-hierarchy.owl#Vision-specific_Language_Models">
        <rdf:type rdf:resource="http://nlpkg.sebis.cit.tum.de/nlp-fos-hierarchy.owl#OtherScientificField"/>
        <rdf:type rdf:resource="http://nlpkg.sebis.cit.tum.de/nlp-taxonomy.owl#FieldOfStudy"/>
        <nlp-taxonomy:subFieldOf rdf:resource="http://nlpkg.sebis.cit.tum.de/nlp-fos-hierarchy.owl#Multimodal_Language_Models"/>
        <nlp-taxonomy:subFieldOf rdf:resource="http://nlpkg.sebis.cit.tum.de/nlp-taxonomy.owl#Visual_Data_In_NLP"/>
        <relevantInformation>https://aman.ai/primers/ai/VLM</relevantInformation>
        <survey>https://aclanthology.org/2022.findings-acl.320</survey>
        <survey>https://aclanthology.org/W19-0418</survey>
        <survey>https://arxiv.org/abs/2103.04037</survey>
        <survey>https://arxiv.org/abs/2109.09920</survey>
        <survey>https://arxiv.org/abs/2202.09061</survey>
        <survey>https://arxiv.org/abs/2202.10936</survey>
        <survey>https://arxiv.org/abs/2204.07356</survey>
        <survey>https://arxiv.org/abs/2305.06159</survey>
        <survey>https://arxiv.org/abs/2306.07198</survey>
        <survey>https://arxiv.org/abs/2307.03254</survey>
        <survey>https://arxiv.org/abs/2309.15857</survey>
        <nlp-taxonomy:level rdf:datatype="http://www.w3.org/2001/XMLSchema#integer">3</nlp-taxonomy:level>
        <nlp-taxonomy:level rdf:datatype="http://www.w3.org/2001/XMLSchema#integer">4</nlp-taxonomy:level>
        <dcterms:description xml:lang="en">Vision-specific Language Models refers to specialized language models that are designed and trained to understand and generate human language specifically in the context of visual data such as images and video.</dcterms:description>
        <oboInOwl:hasSynonym xml:lang="en">VLM</oboInOwl:hasSynonym>
        <oboInOwl:hasSynonym xml:lang="en">Vision-Language Models</oboInOwl:hasSynonym>
        <oboInOwl:hasSynonym xml:lang="en">Vision-Language Transformers</oboInOwl:hasSynonym>
        <rdfs:label xml:lang="en">Vision-specific Language Models</rdfs:label>
    </owl:NamedIndividual>
    


    <!-- http://nlpkg.sebis.cit.tum.de/nlp-fos-hierarchy.owl#Visual_Commonsense_Reasoning -->

    <owl:NamedIndividual rdf:about="http://nlpkg.sebis.cit.tum.de/nlp-fos-hierarchy.owl#Visual_Commonsense_Reasoning">
        <rdf:type rdf:resource="http://nlpkg.sebis.cit.tum.de/nlp-fos-hierarchy.owl#Task"/>
        <rdf:type rdf:resource="http://nlpkg.sebis.cit.tum.de/nlp-taxonomy.owl#FieldOfStudy"/>
        <nlp-taxonomy:subFieldOf rdf:resource="http://nlpkg.sebis.cit.tum.de/nlp-fos-hierarchy.owl#Visual_Reasoning"/>
        <nlp-taxonomy:subFieldOf rdf:resource="http://nlpkg.sebis.cit.tum.de/nlp-taxonomy.owl#Commonsense_Reasoning"/>
        <origin>https://arxiv.org/abs/1811.10830</origin>
        <relevantInformation>https://visualcommonsense.com</relevantInformation>
        <nlp-taxonomy:level rdf:datatype="http://www.w3.org/2001/XMLSchema#integer">3</nlp-taxonomy:level>
        <nlp-taxonomy:level rdf:datatype="http://www.w3.org/2001/XMLSchema#integer">4</nlp-taxonomy:level>
        <dcterms:description xml:lang="en">Visual Commonsense Reasoning is cognition-level visual understanding task. Given a challenging question about an image, machines need to present two sub-tasks: answer correctly and provide a rationale justifying its answer.</dcterms:description>
        <oboInOwl:hasSynonym xml:lang="en">VCR</oboInOwl:hasSynonym>
        <rdfs:label xml:lang="en">Visual Commonsense Reasoning</rdfs:label>
    </owl:NamedIndividual>
    


    <!-- http://nlpkg.sebis.cit.tum.de/nlp-fos-hierarchy.owl#Visual_Entailment -->

    <owl:NamedIndividual rdf:about="http://nlpkg.sebis.cit.tum.de/nlp-fos-hierarchy.owl#Visual_Entailment">
        <rdf:type rdf:resource="http://nlpkg.sebis.cit.tum.de/nlp-fos-hierarchy.owl#Task"/>
        <rdf:type rdf:resource="http://nlpkg.sebis.cit.tum.de/nlp-taxonomy.owl#FieldOfStudy"/>
        <nlp-taxonomy:subFieldOf rdf:resource="http://nlpkg.sebis.cit.tum.de/nlp-fos-hierarchy.owl#Visual_Reasoning"/>
        <origin>https://arxiv.org/abs/1811.10582</origin>
        <nlp-taxonomy:level rdf:datatype="http://www.w3.org/2001/XMLSchema#integer">3</nlp-taxonomy:level>
        <nlp-taxonomy:level rdf:datatype="http://www.w3.org/2001/XMLSchema#integer">4</nlp-taxonomy:level>
        <dcterms:description xml:lang="en">Visual Entailment (VE) is the task of determining whether a visual premise implies a textual hypothesis. The prediction can be either an entailment, neutral or a contradiction.</dcterms:description>
        <oboInOwl:hasSynonym xml:lang="en">VE</oboInOwl:hasSynonym>
        <rdfs:label xml:lang="en">Visual Entailment</rdfs:label>
    </owl:NamedIndividual>
    


    <!-- http://nlpkg.sebis.cit.tum.de/nlp-fos-hierarchy.owl#Visual_Question_Answering -->

    <owl:NamedIndividual rdf:about="http://nlpkg.sebis.cit.tum.de/nlp-fos-hierarchy.owl#Visual_Question_Answering">
        <rdf:type rdf:resource="http://nlpkg.sebis.cit.tum.de/nlp-fos-hierarchy.owl#Task"/>
        <rdf:type rdf:resource="http://nlpkg.sebis.cit.tum.de/nlp-taxonomy.owl#FieldOfStudy"/>
        <nlp-taxonomy:subFieldOf rdf:resource="http://nlpkg.sebis.cit.tum.de/nlp-taxonomy.owl#Question_Answering"/>
        <nlp-taxonomy:subFieldOf rdf:resource="http://nlpkg.sebis.cit.tum.de/nlp-taxonomy.owl#Visual_Data_In_NLP"/>
        <nlp-taxonomy:superFieldOf rdf:resource="http://nlpkg.sebis.cit.tum.de/nlp-fos-hierarchy.owl#Image_Question_Answering"/>
        <nlp-taxonomy:superFieldOf rdf:resource="http://nlpkg.sebis.cit.tum.de/nlp-fos-hierarchy.owl#Video_Question_Answering"/>
        <survey>https://arxiv.org/abs/1607.05910</survey>
        <survey>https://arxiv.org/abs/1610.01076</survey>
        <survey>https://arxiv.org/abs/1610.01465</survey>
        <survey>https://arxiv.org/abs/1705.03865</survey>
        <survey>https://arxiv.org/abs/1909.01860</survey>
        <survey>https://arxiv.org/abs/2203.01322</survey>
        <nlp-taxonomy:level rdf:datatype="http://www.w3.org/2001/XMLSchema#integer">3</nlp-taxonomy:level>
        <dcterms:description xml:lang="en">Visual Question Answering (VQA) is the task of answering open-ended questions based on visual input such as images or videos. The output consists of natural language responses to natural language questions.</dcterms:description>
        <oboInOwl:hasSynonym xml:lang="en">VQA</oboInOwl:hasSynonym>
        <rdfs:label xml:lang="en">Visual Question Answering</rdfs:label>
    </owl:NamedIndividual>
    


    <!-- http://nlpkg.sebis.cit.tum.de/nlp-fos-hierarchy.owl#Visual_Reasoning -->

    <owl:NamedIndividual rdf:about="http://nlpkg.sebis.cit.tum.de/nlp-fos-hierarchy.owl#Visual_Reasoning">
        <rdf:type rdf:resource="http://nlpkg.sebis.cit.tum.de/nlp-fos-hierarchy.owl#Task"/>
        <rdf:type rdf:resource="http://nlpkg.sebis.cit.tum.de/nlp-taxonomy.owl#FieldOfStudy"/>
        <nlp-taxonomy:subFieldOf rdf:resource="http://nlpkg.sebis.cit.tum.de/nlp-taxonomy.owl#Reasoning"/>
        <nlp-taxonomy:subFieldOf rdf:resource="http://nlpkg.sebis.cit.tum.de/nlp-taxonomy.owl#Visual_Data_In_NLP"/>
        <nlp-taxonomy:superFieldOf rdf:resource="http://nlpkg.sebis.cit.tum.de/nlp-fos-hierarchy.owl#Visual_Commonsense_Reasoning"/>
        <nlp-taxonomy:superFieldOf rdf:resource="http://nlpkg.sebis.cit.tum.de/nlp-fos-hierarchy.owl#Visual_Entailment"/>
        <survey>https://arxiv.org/abs/2207.07568</survey>
        <nlp-taxonomy:level rdf:datatype="http://www.w3.org/2001/XMLSchema#integer">2</nlp-taxonomy:level>
        <nlp-taxonomy:level rdf:datatype="http://www.w3.org/2001/XMLSchema#integer">3</nlp-taxonomy:level>
        <dcterms:description xml:lang="en">Visual reasoning is a task that requires multimodal perception and commonsense cognition of the world. It demands models to not only comprehend and interpret visual information but also to apply high-level cognition to derive logical conclusions.</dcterms:description>
        <rdfs:label xml:lang="en">Visual Reasoning</rdfs:label>
    </owl:NamedIndividual>
    


    <!-- http://nlpkg.sebis.cit.tum.de/nlp-fos-hierarchy.owl#Weak_Supervision -->

    <owl:NamedIndividual rdf:about="http://nlpkg.sebis.cit.tum.de/nlp-fos-hierarchy.owl#Weak_Supervision">
        <rdf:type rdf:resource="http://nlpkg.sebis.cit.tum.de/nlp-fos-hierarchy.owl#OtherScientificField"/>
        <rdf:type rdf:resource="http://nlpkg.sebis.cit.tum.de/nlp-taxonomy.owl#FieldOfStudy"/>
        <nlp-taxonomy:subFieldOf rdf:resource="http://nlpkg.sebis.cit.tum.de/nlp-taxonomy.owl#Low-Resource_NLP"/>
        <nlp-taxonomy:superFieldOf rdf:resource="http://nlpkg.sebis.cit.tum.de/nlp-fos-hierarchy.owl#Distant_Supervision"/>
        <nlp-taxonomy:level rdf:datatype="http://www.w3.org/2001/XMLSchema#integer">3</nlp-taxonomy:level>
        <dcterms:description xml:lang="en">Weak Supervision refers to the process of using less precise, often noisier sources of supervision to train machine learning models. This approach is typically used when there is a lack of sufficient labeled data for training. Weak supervision may involve heuristics or rules to generate labels.</dcterms:description>
        <oboInOwl:hasSynonym xml:lang="en">Weakly Supervised</oboInOwl:hasSynonym>
        <oboInOwl:hasSynonym xml:lang="en">Weakly Supervised Learning</oboInOwl:hasSynonym>
        <rdfs:label xml:lang="en">Weak Supervision</rdfs:label>
    </owl:NamedIndividual>
    


    <!-- http://nlpkg.sebis.cit.tum.de/nlp-fos-hierarchy.owl#Word-based_Machine_Translation -->

    <owl:NamedIndividual rdf:about="http://nlpkg.sebis.cit.tum.de/nlp-fos-hierarchy.owl#Word-based_Machine_Translation">
        <rdf:type rdf:resource="http://nlpkg.sebis.cit.tum.de/nlp-fos-hierarchy.owl#Task"/>
        <rdf:type rdf:resource="http://nlpkg.sebis.cit.tum.de/nlp-taxonomy.owl#FieldOfStudy"/>
        <nlp-taxonomy:subFieldOf rdf:resource="http://nlpkg.sebis.cit.tum.de/nlp-fos-hierarchy.owl#Statistical_Machine_Translation"/>
        <nlp-taxonomy:level rdf:datatype="http://www.w3.org/2001/XMLSchema#integer">4</nlp-taxonomy:level>
        <dcterms:description xml:lang="en">Word-based Machine Translation is a method where the translation from the source language to the target language is performed on a word-by-word basis. It involves direct substitution of words in one language for words in another. However, this approach often fails to capture the context and grammatical differences between languages, leading to inaccurate or nonsensical translations.</dcterms:description>
        <rdfs:label xml:lang="en">Word-based Machine Translation</rdfs:label>
    </owl:NamedIndividual>
    


    <!-- http://nlpkg.sebis.cit.tum.de/nlp-fos-hierarchy.owl#Word_Alignment -->

    <owl:NamedIndividual rdf:about="http://nlpkg.sebis.cit.tum.de/nlp-fos-hierarchy.owl#Word_Alignment">
        <rdf:type rdf:resource="http://nlpkg.sebis.cit.tum.de/nlp-fos-hierarchy.owl#Task"/>
        <rdf:type rdf:resource="http://nlpkg.sebis.cit.tum.de/nlp-taxonomy.owl#FieldOfStudy"/>
        <nlp-taxonomy:subFieldOf rdf:resource="http://nlpkg.sebis.cit.tum.de/nlp-fos-hierarchy.owl#Statistical_Machine_Translation"/>
        <survey>https://arxiv.org/abs/2212.00138</survey>
        <nlp-taxonomy:level rdf:datatype="http://www.w3.org/2001/XMLSchema#integer">4</nlp-taxonomy:level>
        <dcterms:description xml:lang="en">Word Alignment refers to the process of identifying which word or group of words in the source language corresponds to which word or group of words in the target language. This alignment is crucial for accurate translation as it helps in understanding the relationship between the words in different languages, thereby improving the quality of the translation.</dcterms:description>
        <oboInOwl:hasSynonym xml:lang="en">Bitext Word Alignment</oboInOwl:hasSynonym>
        <rdfs:label xml:lang="en">Word Alignment</rdfs:label>
    </owl:NamedIndividual>
    


    <!-- http://nlpkg.sebis.cit.tum.de/nlp-fos-hierarchy.owl#Word_Embeddings -->

    <owl:NamedIndividual rdf:about="http://nlpkg.sebis.cit.tum.de/nlp-fos-hierarchy.owl#Word_Embeddings">
        <rdf:type rdf:resource="http://nlpkg.sebis.cit.tum.de/nlp-fos-hierarchy.owl#DataStructure"/>
        <rdf:type rdf:resource="http://nlpkg.sebis.cit.tum.de/nlp-taxonomy.owl#FieldOfStudy"/>
        <uses rdf:resource="http://nlpkg.sebis.cit.tum.de/nlp-fos-hierarchy.owl#Distributional_Semantics"/>
        <nlp-taxonomy:subFieldOf rdf:resource="http://nlpkg.sebis.cit.tum.de/nlp-fos-hierarchy.owl#Text_Embeddings"/>
        <survey>https://aclanthology.org/2020.acl-main.405</survey>
        <survey>https://aclanthology.org/C18-1117</survey>
        <survey>https://aclanthology.org/P19-1329</survey>
        <survey>https://aclanthology.org/W19-3805</survey>
        <survey>https://arxiv.org/abs/1706.04902</survey>
        <survey>https://arxiv.org/abs/1801.09536</survey>
        <survey>https://arxiv.org/abs/1805.04032</survey>
        <survey>https://arxiv.org/abs/1807.02471</survey>
        <survey>https://arxiv.org/abs/1901.09069</survey>
        <survey>https://arxiv.org/abs/1902.00753</survey>
        <survey>https://arxiv.org/abs/2010.15036</survey>
        <survey>https://arxiv.org/abs/2110.01804</survey>
        <survey>https://arxiv.org/abs/2204.11660</survey>
        <nlp-taxonomy:level rdf:datatype="http://www.w3.org/2001/XMLSchema#integer">5</nlp-taxonomy:level>
        <dcterms:description xml:lang="en">Word Embeddings refer to words or phrases that are mapped to vectors of real numbers. These vectors capture the semantic and syntactic meaning, relationship with other words, and context of the words in a compact way.</dcterms:description>
        <oboInOwl:hasSynonym xml:lang="en">Distributed Word Representations</oboInOwl:hasSynonym>
        <oboInOwl:hasSynonym xml:lang="en">Word Representations</oboInOwl:hasSynonym>
        <rdfs:label xml:lang="en">Word Embeddings</rdfs:label>
    </owl:NamedIndividual>
    


    <!-- http://nlpkg.sebis.cit.tum.de/nlp-fos-hierarchy.owl#Word_Sense_Induction -->

    <owl:NamedIndividual rdf:about="http://nlpkg.sebis.cit.tum.de/nlp-fos-hierarchy.owl#Word_Sense_Induction">
        <rdf:type rdf:resource="http://nlpkg.sebis.cit.tum.de/nlp-fos-hierarchy.owl#Task"/>
        <rdf:type rdf:resource="http://nlpkg.sebis.cit.tum.de/nlp-taxonomy.owl#FieldOfStudy"/>
        <nlp-taxonomy:subFieldOf rdf:resource="http://nlpkg.sebis.cit.tum.de/nlp-taxonomy.owl#Word_Sense_Disambiguation"/>
        <relevantInformation>http://nlpprogress.com/english/word_sense_disambiguation.html</relevantInformation>
        <nlp-taxonomy:level rdf:datatype="http://www.w3.org/2001/XMLSchema#integer">3</nlp-taxonomy:level>
        <dcterms:description xml:lang="en">Word Sense Induction (WSI) is widely known as the “unsupervised version” of WSD. The problem states as: Given a target word (e.g., “cold”) and a collection of sentences (e.g., “I caught a cold”, “The weather is cold”) that use the word, cluster the sentences according to their different senses/meanings. We do not need to know the sense/meaning of each cluster, but sentences inside a cluster should have used the target words with the same sense.</dcterms:description>
        <oboInOwl:hasSynonym xml:lang="en">WSI</oboInOwl:hasSynonym>
        <rdfs:label xml:lang="en">Word Sense Induction</rdfs:label>
    </owl:NamedIndividual>
    


    <!-- http://nlpkg.sebis.cit.tum.de/nlp-fos-hierarchy.owl#Zero-shot_Entailment -->

    <owl:NamedIndividual rdf:about="http://nlpkg.sebis.cit.tum.de/nlp-fos-hierarchy.owl#Zero-shot_Entailment">
        <rdf:type rdf:resource="http://nlpkg.sebis.cit.tum.de/nlp-fos-hierarchy.owl#Method"/>
        <rdf:type rdf:resource="http://nlpkg.sebis.cit.tum.de/nlp-taxonomy.owl#FieldOfStudy"/>
        <usedFor rdf:resource="http://nlpkg.sebis.cit.tum.de/nlp-taxonomy.owl#Text_Classification"/>
        <nlp-taxonomy:subFieldOf rdf:resource="http://nlpkg.sebis.cit.tum.de/nlp-fos-hierarchy.owl#Zero-shot_Learning"/>
        <nlp-taxonomy:subFieldOf rdf:resource="http://nlpkg.sebis.cit.tum.de/nlp-taxonomy.owl#Textual_Inference"/>
        <code>https://github.com/yinwenpeng/BenchmarkingZeroShot</code>
        <origin>https://aclanthology.org/D19-1404</origin>
        <survey>https://arxiv.org/abs/2211.16285</survey>
        <nlp-taxonomy:level rdf:datatype="http://www.w3.org/2001/XMLSchema#integer">3</nlp-taxonomy:level>
        <nlp-taxonomy:level rdf:datatype="http://www.w3.org/2001/XMLSchema#integer">4</nlp-taxonomy:level>
        <dcterms:description xml:lang="en">Zero-shot Entailment is a method where a model, without being explicitly trained on any classification task, can classify unseen text into one or more categories. This is achieved by leveraging Natural Language Inference (NLI) models. The model is presented with a text and a hypothesis (usually a statement about the category), and it predicts whether the hypothesis can be inferred from the text. This allows the model to classify text into categories it has never seen during training, hence the term &quot;zero-shot&quot;.</dcterms:description>
        <oboInOwl:hasSynonym xml:lang="en">NLI-based Zero Shot Text Classification</oboInOwl:hasSynonym>
        <oboInOwl:hasSynonym xml:lang="en">Zero-shot NLI</oboInOwl:hasSynonym>
        <rdfs:label xml:lang="en">Zero-shot Entailment</rdfs:label>
    </owl:NamedIndividual>
    


    <!-- http://nlpkg.sebis.cit.tum.de/nlp-fos-hierarchy.owl#Zero-shot_Learning -->

    <owl:NamedIndividual rdf:about="http://nlpkg.sebis.cit.tum.de/nlp-fos-hierarchy.owl#Zero-shot_Learning">
        <rdf:type rdf:resource="http://nlpkg.sebis.cit.tum.de/nlp-fos-hierarchy.owl#Task"/>
        <rdf:type rdf:resource="http://nlpkg.sebis.cit.tum.de/nlp-taxonomy.owl#FieldOfStudy"/>
        <uses rdf:resource="http://nlpkg.sebis.cit.tum.de/nlp-fos-hierarchy.owl#Prompting,_Prompt_Learning_&amp;_Prompt_Engineering"/>
        <nlp-taxonomy:subFieldOf rdf:resource="http://nlpkg.sebis.cit.tum.de/nlp-taxonomy.owl#Language_Models"/>
        <nlp-taxonomy:subFieldOf rdf:resource="http://nlpkg.sebis.cit.tum.de/nlp-taxonomy.owl#Low-Resource_NLP"/>
        <nlp-taxonomy:subFieldOf rdf:resource="http://nlpkg.sebis.cit.tum.de/nlp-taxonomy.owl#Green_&amp;_Sustainable_NLP"/>
        <nlp-taxonomy:superFieldOf rdf:resource="http://nlpkg.sebis.cit.tum.de/nlp-fos-hierarchy.owl#Zero-shot_Entailment"/>
        <relevantInformation>https://joeddav.github.io/blog/2020/05/29/ZSL.html</relevantInformation>
        <survey>https://arxiv.org/abs/2211.16285</survey>
        <nlp-taxonomy:level rdf:datatype="http://www.w3.org/2001/XMLSchema#integer">3</nlp-taxonomy:level>
        <dcterms:description xml:lang="en">Zero-shot Learning refers to the ability of a model to understand and perform tasks it has not been explicitly trained on. It involves training a model on a set of tasks or languages, and then the model uses that knowledge to understand and perform new tasks or understand new languages. This concept is particularly useful in situations where labeled data is scarce or unavailable.</dcterms:description>
        <oboInOwl:hasSynonym xml:lang="en">ZSL</oboInOwl:hasSynonym>
        <oboInOwl:hasSynonym xml:lang="en">Zero shot</oboInOwl:hasSynonym>
        <oboInOwl:hasSynonym xml:lang="en">Zero-shot</oboInOwl:hasSynonym>
        <rdfs:label xml:lang="en">Zero-shot Learning</rdfs:label>
    </owl:NamedIndividual>
    


    <!-- http://nlpkg.sebis.cit.tum.de/nlp-fos-hierarchy.owl#Zero_Anaphora_Resolution -->

    <owl:NamedIndividual rdf:about="http://nlpkg.sebis.cit.tum.de/nlp-fos-hierarchy.owl#Zero_Anaphora_Resolution">
        <rdf:type rdf:resource="http://nlpkg.sebis.cit.tum.de/nlp-fos-hierarchy.owl#Task"/>
        <rdf:type rdf:resource="http://nlpkg.sebis.cit.tum.de/nlp-taxonomy.owl#FieldOfStudy"/>
        <nlp-taxonomy:subFieldOf rdf:resource="http://nlpkg.sebis.cit.tum.de/nlp-fos-hierarchy.owl#Anaphora_Resolution"/>
        <nlp-taxonomy:level rdf:datatype="http://www.w3.org/2001/XMLSchema#integer">4</nlp-taxonomy:level>
        <dcterms:description xml:lang="en">Zero Anaphora (ZA) Resolution refers to the process of identifying and resolving implicit or unstated subjects or objects in a sentence. It&apos;s a type of anaphora where the anaphoric expression is not overtly present in the discourse. This is common in many languages where the subject or object of a sentence can be dropped if it can be inferred from the context. The challenge in NLP is to correctly infer these missing elements to understand the complete meaning of the sentence.</dcterms:description>
        <oboInOwl:hasSynonym xml:lang="en">ZA Resolution</oboInOwl:hasSynonym>
        <rdfs:label xml:lang="en">Zero Anaphora Resolution</rdfs:label>
    </owl:NamedIndividual>
    


    <!-- http://nlpkg.sebis.cit.tum.de/nlp-fos-hierarchy.owl#n-gram -->

    <owl:NamedIndividual rdf:about="http://nlpkg.sebis.cit.tum.de/nlp-fos-hierarchy.owl#n-gram">
        <rdf:type rdf:resource="http://nlpkg.sebis.cit.tum.de/nlp-fos-hierarchy.owl#OtherScientificField"/>
        <rdf:type rdf:resource="http://nlpkg.sebis.cit.tum.de/nlp-taxonomy.owl#FieldOfStudy"/>
        <usedFor rdf:resource="http://nlpkg.sebis.cit.tum.de/nlp-fos-hierarchy.owl#n-gram_Language_Model"/>
        <nlp-taxonomy:subFieldOf rdf:resource="http://nlpkg.sebis.cit.tum.de/nlp-taxonomy.owl#Text_Segmentation"/>
        <nlp-taxonomy:level rdf:datatype="http://www.w3.org/2001/XMLSchema#integer">3</nlp-taxonomy:level>
        <dcterms:description xml:lang="en">An n-gram is a contiguous sequence of n items from a given sample of text or speech. N can be any integer number, and the items can be phonemes, syllables, letters, words or base pairs according to the application. For example, in a sentence, a 1-gram (or unigram) would be each individual word, a 2-gram (or bigram) would be each sequence of two words, a 3-gram (or trigram) would be each sequence of three words, and so on.</dcterms:description>
        <oboInOwl:hasSynonym xml:lang="en">n-Gram</oboInOwl:hasSynonym>
        <rdfs:label xml:lang="en">n-gram</rdfs:label>
    </owl:NamedIndividual>
    


    <!-- http://nlpkg.sebis.cit.tum.de/nlp-fos-hierarchy.owl#n-gram_Language_Model -->

    <owl:NamedIndividual rdf:about="http://nlpkg.sebis.cit.tum.de/nlp-fos-hierarchy.owl#n-gram_Language_Model">
        <rdf:type rdf:resource="http://nlpkg.sebis.cit.tum.de/nlp-fos-hierarchy.owl#Method"/>
        <rdf:type rdf:resource="http://nlpkg.sebis.cit.tum.de/nlp-taxonomy.owl#FieldOfStudy"/>
        <uses rdf:resource="http://nlpkg.sebis.cit.tum.de/nlp-fos-hierarchy.owl#n-gram"/>
        <nlp-taxonomy:subFieldOf rdf:resource="http://nlpkg.sebis.cit.tum.de/nlp-taxonomy.owl#Language_Models"/>
        <relevantInformation>https://web.stanford.edu/~jurafsky/slp3/3.pdf</relevantInformation>
        <nlp-taxonomy:level rdf:datatype="http://www.w3.org/2001/XMLSchema#integer">3</nlp-taxonomy:level>
        <dcterms:description xml:lang="en">n-gram Language Models are a probabilistic language models used to predict the next word in a sentence based on the previous &apos;n&apos; words. It uses the statistical properties of n-grams to predict the sequence of words in a sentence. The &apos;n&apos; in n-gram represents the number of words considered as context. For example, in a bigram model (n=2), the next word is predicted based on the previous word, while in a trigram model (n=3), the next word is predicted based on the previous two words.</dcterms:description>
        <oboInOwl:hasSynonym xml:lang="en">n-Gram Language Model</oboInOwl:hasSynonym>
        <rdfs:label xml:lang="en">n-gram Language Model</rdfs:label>
    </owl:NamedIndividual>
    


    <!-- http://nlpkg.sebis.cit.tum.de/nlp-fos-hierarchy.owl#Biases_&amp;_Fairness_in_NLP -->

    <owl:NamedIndividual rdf:about="http://nlpkg.sebis.cit.tum.de/nlp-fos-hierarchy.owl#Biases_&amp;_Fairness_in_NLP">
        <rdf:type rdf:resource="http://nlpkg.sebis.cit.tum.de/nlp-fos-hierarchy.owl#OtherScientificField"/>
        <rdf:type rdf:resource="http://nlpkg.sebis.cit.tum.de/nlp-taxonomy.owl#FieldOfStudy"/>
        <nlp-taxonomy:subFieldOf rdf:resource="http://nlpkg.sebis.cit.tum.de/nlp-taxonomy.owl#Ethical_NLP"/>
        <nlp-taxonomy:subFieldOf rdf:resource="http://nlpkg.sebis.cit.tum.de/nlp-taxonomy.owl#Robustness_In_NLP"/>
        <nlp-taxonomy:superFieldOf rdf:resource="http://nlpkg.sebis.cit.tum.de/nlp-fos-hierarchy.owl#Confounding_Bias"/>
        <nlp-taxonomy:superFieldOf rdf:resource="http://nlpkg.sebis.cit.tum.de/nlp-fos-hierarchy.owl#Debiasing"/>
        <nlp-taxonomy:superFieldOf rdf:resource="http://nlpkg.sebis.cit.tum.de/nlp-fos-hierarchy.owl#Exposure_Bias"/>
        <nlp-taxonomy:superFieldOf rdf:resource="http://nlpkg.sebis.cit.tum.de/nlp-fos-hierarchy.owl#Inductive_Bias"/>
        <nlp-taxonomy:superFieldOf rdf:resource="http://nlpkg.sebis.cit.tum.de/nlp-fos-hierarchy.owl#Media_Bias"/>
        <nlp-taxonomy:superFieldOf rdf:resource="http://nlpkg.sebis.cit.tum.de/nlp-fos-hierarchy.owl#Social_Bias"/>
        <survey>https://aclanthology.org/2020.acl-main.485</survey>
        <survey>https://aclanthology.org/2021.acl-short.39</survey>
        <survey>https://aclanthology.org/2022.coling-1.115</survey>
        <survey>https://aclanthology.org/2022.naacl-main.122</survey>
        <survey>https://aclanthology.org/2023.findings-acl.139</survey>
        <survey>https://aclanthology.org/W18-1401</survey>
        <survey>https://arxiv.org/abs/2204.09591</survey>
        <survey>https://arxiv.org/abs/2204.10365</survey>
        <survey>https://arxiv.org/abs/2211.08461</survey>
        <survey>https://arxiv.org/abs/2211.09511</survey>
        <survey>https://arxiv.org/abs/2307.15425</survey>
        <survey>https://arxiv.org/abs/2308.10149</survey>
        <survey>https://arxiv.org/abs/2309.00770</survey>
        <survey>https://doi.org/10.1145/3597307</survey>
        <nlp-taxonomy:level rdf:datatype="http://www.w3.org/2001/XMLSchema#integer">3</nlp-taxonomy:level>
        <dcterms:description xml:lang="en">Biases &amp; Fairness in NLP refer to the systematic and potentially harmful errors that arise as a result of a given choice of texts used to train a model.</dcterms:description>
        <oboInOwl:hasSynonym xml:lang="en">Bias</oboInOwl:hasSynonym>
        <oboInOwl:hasSynonym xml:lang="en">Fair</oboInOwl:hasSynonym>
        <oboInOwl:hasSynonym xml:lang="en">Fairness</oboInOwl:hasSynonym>
        <rdfs:label xml:lang="en">Biases &amp; Fairness in NLP</rdfs:label>
    </owl:NamedIndividual>
    


    <!-- http://nlpkg.sebis.cit.tum.de/nlp-fos-hierarchy.owl#Keyword_&amp;_Keyphrase_Extraction -->

    <owl:NamedIndividual rdf:about="http://nlpkg.sebis.cit.tum.de/nlp-fos-hierarchy.owl#Keyword_&amp;_Keyphrase_Extraction">
        <rdf:type rdf:resource="http://nlpkg.sebis.cit.tum.de/nlp-fos-hierarchy.owl#Task"/>
        <rdf:type rdf:resource="http://nlpkg.sebis.cit.tum.de/nlp-taxonomy.owl#FieldOfStudy"/>
        <uses rdf:resource="http://nlpkg.sebis.cit.tum.de/nlp-fos-hierarchy.owl#Span_Detection"/>
        <nlp-taxonomy:subFieldOf rdf:resource="http://nlpkg.sebis.cit.tum.de/nlp-taxonomy.owl#Term_Extraction"/>
        <survey>https://aclanthology.org/2023.findings-eacl.161</survey>
        <survey>https://arxiv.org/abs/1704.03242</survey>
        <survey>https://arxiv.org/abs/1905.05044</survey>
        <survey>https://arxiv.org/abs/1910.05059</survey>
        <survey>https://arxiv.org/abs/2110.01073</survey>
        <survey>https://arxiv.org/abs/2305.02579</survey>
        <nlp-taxonomy:level rdf:datatype="http://www.w3.org/2001/XMLSchema#integer">3</nlp-taxonomy:level>
        <dcterms:description xml:lang="en">Keyword &amp; Keyphrase Extraction is the task of identifying and extracting relevant words or phrases from a larger body of text. These keywords or keyphrases represent the core content or main topics in the text.</dcterms:description>
        <oboInOwl:hasSynonym xml:lang="en">KE</oboInOwl:hasSynonym>
        <oboInOwl:hasSynonym xml:lang="en">Keyphrase Extraction</oboInOwl:hasSynonym>
        <oboInOwl:hasSynonym xml:lang="en">Keyphrase Generation</oboInOwl:hasSynonym>
        <oboInOwl:hasSynonym xml:lang="en">Keyword Extraction</oboInOwl:hasSynonym>
        <oboInOwl:hasSynonym xml:lang="en">Keyword Generation</oboInOwl:hasSynonym>
        <rdfs:comment xml:lang="en">Keyphrase Prediction</rdfs:comment>
        <rdfs:comment xml:lang="en">Keyword Prediction</rdfs:comment>
        <rdfs:label xml:lang="en">Keyword &amp; Keyphrase Extraction</rdfs:label>
    </owl:NamedIndividual>
    


    <!-- http://nlpkg.sebis.cit.tum.de/nlp-fos-hierarchy.owl#Knowledge_Graph_Construction_&amp;_Completion -->

    <owl:NamedIndividual rdf:about="http://nlpkg.sebis.cit.tum.de/nlp-fos-hierarchy.owl#Knowledge_Graph_Construction_&amp;_Completion">
        <rdf:type rdf:resource="http://nlpkg.sebis.cit.tum.de/nlp-fos-hierarchy.owl#Task"/>
        <rdf:type rdf:resource="http://nlpkg.sebis.cit.tum.de/nlp-taxonomy.owl#FieldOfStudy"/>
        <uses rdf:resource="http://nlpkg.sebis.cit.tum.de/nlp-taxonomy.owl#Coreference_Resolution"/>
        <uses rdf:resource="http://nlpkg.sebis.cit.tum.de/nlp-taxonomy.owl#Knowledge_Graph_Reasoning"/>
        <uses rdf:resource="http://nlpkg.sebis.cit.tum.de/nlp-taxonomy.owl#Named_Entity_Recognition"/>
        <uses rdf:resource="http://nlpkg.sebis.cit.tum.de/nlp-taxonomy.owl#Relation_Extraction"/>
        <uses rdf:resource="http://nlpkg.sebis.cit.tum.de/nlp-taxonomy.owl#Term_Extraction"/>
        <nlp-taxonomy:subFieldOf rdf:resource="http://nlpkg.sebis.cit.tum.de/nlp-fos-hierarchy.owl#Knowledge_Graphs"/>
        <nlp-taxonomy:superFieldOf rdf:resource="http://nlpkg.sebis.cit.tum.de/nlp-fos-hierarchy.owl#Entity_Alignment"/>
        <nlp-taxonomy:superFieldOf rdf:resource="http://nlpkg.sebis.cit.tum.de/nlp-fos-hierarchy.owl#Entity_Linking"/>
        <nlp-taxonomy:superFieldOf rdf:resource="http://nlpkg.sebis.cit.tum.de/nlp-fos-hierarchy.owl#Entity_Resolution"/>
        <nlp-taxonomy:superFieldOf rdf:resource="http://nlpkg.sebis.cit.tum.de/nlp-fos-hierarchy.owl#Relation_Linking"/>
        <survey>https://aclanthology.org/2020.textgraphs-1.1</survey>
        <survey>https://aclanthology.org/2022.emnlp-main.1</survey>
        <survey>https://arxiv.org/abs/1703.08098</survey>
        <survey>https://arxiv.org/abs/2007.12374</survey>
        <survey>https://arxiv.org/abs/2202.05786</survey>
        <survey>https://arxiv.org/abs/2301.01172</survey>
        <survey>https://arxiv.org/abs/2302.01859</survey>
        <survey>https://arxiv.org/abs/2310.14771</survey>
        <nlp-taxonomy:level rdf:datatype="http://www.w3.org/2001/XMLSchema#integer">6</nlp-taxonomy:level>
        <dcterms:description xml:lang="en">Knowledge Graph Construction &amp; Completion refers to the process of creating and extending a structured graphical representation of information or knowledge. It involves extracting entities (like people, places, or things) and relationships (like actions or properties) from unstructured data, such as text, and organizing them into a graph format. Further, reasoning approaches can be applied to add missing edges or nodes. The knowledge graph can then be used to understand the context, semantics, and connections within the data.</dcterms:description>
        <oboInOwl:hasSynonym xml:lang="en">KG Completion</oboInOwl:hasSynonym>
        <oboInOwl:hasSynonym xml:lang="en">KG Construction</oboInOwl:hasSynonym>
        <oboInOwl:hasSynonym xml:lang="en">Knowledge Base Completion</oboInOwl:hasSynonym>
        <oboInOwl:hasSynonym xml:lang="en">Knowledge Base Construction</oboInOwl:hasSynonym>
        <oboInOwl:hasSynonym xml:lang="en">Knowledge Graph Completion</oboInOwl:hasSynonym>
        <oboInOwl:hasSynonym xml:lang="en">Knowledge Graph Construction</oboInOwl:hasSynonym>
        <rdfs:label xml:lang="en">Knowledge Graph Construction &amp; Completion</rdfs:label>
    </owl:NamedIndividual>
    


    <!-- http://nlpkg.sebis.cit.tum.de/nlp-fos-hierarchy.owl#Multi-Agent_Systems_&amp;_Multi-Model_Language_Models -->

    <owl:NamedIndividual rdf:about="http://nlpkg.sebis.cit.tum.de/nlp-fos-hierarchy.owl#Multi-Agent_Systems_&amp;_Multi-Model_Language_Models">
        <rdf:type rdf:resource="http://nlpkg.sebis.cit.tum.de/nlp-fos-hierarchy.owl#OtherScientificField"/>
        <rdf:type rdf:resource="http://nlpkg.sebis.cit.tum.de/nlp-taxonomy.owl#FieldOfStudy"/>
        <nlp-taxonomy:subFieldOf rdf:resource="http://nlpkg.sebis.cit.tum.de/nlp-taxonomy.owl#Language_Models"/>
        <nlp-taxonomy:superFieldOf rdf:resource="http://nlpkg.sebis.cit.tum.de/nlp-fos-hierarchy.owl#Ensemble_Models"/>
        <nlp-taxonomy:superFieldOf rdf:resource="http://nlpkg.sebis.cit.tum.de/nlp-fos-hierarchy.owl#Mixture_of_Experts"/>
        <nlp-taxonomy:level rdf:datatype="http://www.w3.org/2001/XMLSchema#integer">3</nlp-taxonomy:level>
        <dcterms:description xml:lang="en">Multi-Agent Systems &amp; Multi-Model Language Models refer to the combination of multiple agents or language models to solve problems that are difficult or impossible for an individual agent or a monolithic system to solve. Also, using multiple agents or models can improve the performance of natural language processing tasks.</dcterms:description>
        <oboInOwl:hasSynonym xml:lang="en">MAS</oboInOwl:hasSynonym>
        <oboInOwl:hasSynonym xml:lang="en">Multi-Agent Systems</oboInOwl:hasSynonym>
        <oboInOwl:hasSynonym xml:lang="en">Multi-Model Language Models</oboInOwl:hasSynonym>
        <oboInOwl:hasSynonym xml:lang="en">Self-Organized System</oboInOwl:hasSynonym>
        <rdfs:label xml:lang="en">Multi-Agent Systems &amp; Multi-Model Language Models</rdfs:label>
    </owl:NamedIndividual>
    


    <!-- http://nlpkg.sebis.cit.tum.de/nlp-fos-hierarchy.owl#Privacy,_Security_&amp;_Safety_in_NLP -->

    <owl:NamedIndividual rdf:about="http://nlpkg.sebis.cit.tum.de/nlp-fos-hierarchy.owl#Privacy,_Security_&amp;_Safety_in_NLP">
        <rdf:type rdf:resource="http://nlpkg.sebis.cit.tum.de/nlp-fos-hierarchy.owl#OtherScientificField"/>
        <rdf:type rdf:resource="http://nlpkg.sebis.cit.tum.de/nlp-taxonomy.owl#FieldOfStudy"/>
        <uses rdf:resource="http://nlpkg.sebis.cit.tum.de/nlp-taxonomy.owl#Robustness_In_NLP"/>
        <uses rdf:resource="http://nlpkg.sebis.cit.tum.de/nlp-taxonomy.owl#Stylistic_Analysis"/>
        <nlp-taxonomy:subFieldOf rdf:resource="http://nlpkg.sebis.cit.tum.de/nlp-taxonomy.owl#Ethical_NLP"/>
        <nlp-taxonomy:superFieldOf rdf:resource="http://nlpkg.sebis.cit.tum.de/nlp-fos-hierarchy.owl#Adversarial_Attacks"/>
        <nlp-taxonomy:superFieldOf rdf:resource="http://nlpkg.sebis.cit.tum.de/nlp-fos-hierarchy.owl#Backdoor_Attacks"/>
        <nlp-taxonomy:superFieldOf rdf:resource="http://nlpkg.sebis.cit.tum.de/nlp-fos-hierarchy.owl#De-Identification"/>
        <nlp-taxonomy:superFieldOf rdf:resource="http://nlpkg.sebis.cit.tum.de/nlp-fos-hierarchy.owl#Differential_Privacy"/>
        <nlp-taxonomy:superFieldOf rdf:resource="http://nlpkg.sebis.cit.tum.de/nlp-fos-hierarchy.owl#Federated_Learning"/>
        <nlp-taxonomy:superFieldOf rdf:resource="http://nlpkg.sebis.cit.tum.de/nlp-fos-hierarchy.owl#Inference_Attacks"/>
        <nlp-taxonomy:superFieldOf rdf:resource="http://nlpkg.sebis.cit.tum.de/nlp-fos-hierarchy.owl#Obfuscation"/>
        <nlp-taxonomy:superFieldOf rdf:resource="http://nlpkg.sebis.cit.tum.de/nlp-fos-hierarchy.owl#Prompt_Hacking"/>
        <nlp-taxonomy:superFieldOf rdf:resource="http://nlpkg.sebis.cit.tum.de/nlp-fos-hierarchy.owl#Sanitization"/>
        <relevantInformation>https://edwinwenink.github.io/ai-ethics-tool-landscape/values/privacy/</relevantInformation>
        <survey>https://aclanthology.org/2023.trustnlp-1.23</survey>
        <survey>https://arxiv.org/abs/2011.10180</survey>
        <survey>https://arxiv.org/abs/2205.10095</survey>
        <survey>https://arxiv.org/abs/2305.11391</survey>
        <survey>https://arxiv.org/abs/2310.01424</survey>
        <nlp-taxonomy:level rdf:datatype="http://www.w3.org/2001/XMLSchema#integer">3</nlp-taxonomy:level>
        <dcterms:description xml:lang="en">Privacy, Security &amp; Safety in NLP refers to the protection of sensitive and usually personal information that may be contained within the data being processed. This includes ensuring that identifiable information is not disclosed during data analysis and that the data is stored and processed in a secure manner.</dcterms:description>
        <oboInOwl:hasSynonym xml:lang="en">Privacy</oboInOwl:hasSynonym>
        <oboInOwl:hasSynonym xml:lang="en">Safety</oboInOwl:hasSynonym>
        <oboInOwl:hasSynonym xml:lang="en">Security</oboInOwl:hasSynonym>
        <rdfs:label xml:lang="en">Privacy, Security &amp; Safety in NLP</rdfs:label>
    </owl:NamedIndividual>
    


    <!-- http://nlpkg.sebis.cit.tum.de/nlp-fos-hierarchy.owl#Prompting,_Prompt_Learning_&amp;_Prompt_Engineering -->

    <owl:NamedIndividual rdf:about="http://nlpkg.sebis.cit.tum.de/nlp-fos-hierarchy.owl#Prompting,_Prompt_Learning_&amp;_Prompt_Engineering">
        <rdf:type rdf:resource="http://nlpkg.sebis.cit.tum.de/nlp-fos-hierarchy.owl#Task"/>
        <rdf:type rdf:resource="http://nlpkg.sebis.cit.tum.de/nlp-taxonomy.owl#FieldOfStudy"/>
        <usedFor rdf:resource="http://nlpkg.sebis.cit.tum.de/nlp-fos-hierarchy.owl#Zero-shot_Learning"/>
        <nlp-taxonomy:subFieldOf rdf:resource="http://nlpkg.sebis.cit.tum.de/nlp-taxonomy.owl#Language_Models"/>
        <nlp-taxonomy:subFieldOf rdf:resource="http://nlpkg.sebis.cit.tum.de/nlp-taxonomy.owl#Green_&amp;_Sustainable_NLP"/>
        <nlp-taxonomy:superFieldOf rdf:resource="http://nlpkg.sebis.cit.tum.de/nlp-fos-hierarchy.owl#In-Context_Learning"/>
        <nlp-taxonomy:superFieldOf rdf:resource="http://nlpkg.sebis.cit.tum.de/nlp-fos-hierarchy.owl#Instruction_Learning"/>
        <nlp-taxonomy:superFieldOf rdf:resource="http://nlpkg.sebis.cit.tum.de/nlp-fos-hierarchy.owl#Prompt_Hacking"/>
        <nlp-taxonomy:superFieldOf rdf:resource="http://nlpkg.sebis.cit.tum.de/nlp-fos-hierarchy.owl#Prompt_Optimization"/>
        <code>https://github.com/thunlp/OpenPrompt</code>
        <relevantInformation>http://pretrain.nlpedia.ai</relevantInformation>
        <relevantInformation>https://github.com/zjunlp/Prompt4ReasoningPapers</relevantInformation>
        <relevantInformation>https://learnprompting.org/docs/intro</relevantInformation>
        <relevantInformation>https://platform.openai.com/docs/guides/prompt-engineering</relevantInformation>
        <relevantInformation>https://www.promptingguide.ai</relevantInformation>
        <survey>https://aclanthology.org/2023.acl-long.294</survey>
        <survey>https://arxiv.org/abs/2107.13586</survey>
        <survey>https://arxiv.org/abs/2310.14735</survey>
        <survey>https://arxiv.org/abs/2402.07927</survey>
        <nlp-taxonomy:level rdf:datatype="http://www.w3.org/2001/XMLSchema#integer">3</nlp-taxonomy:level>
        <dcterms:description xml:lang="en">Prompting refers to the process of providing a model with a specific input or &quot;prompt&quot; to guide its output or response. It&apos;s like asking a question or giving a command that the model responds to.

Prompt Learning is a learning method where the model learns to generate appropriate responses to specific prompts. It&apos;s a way of training models to understand and respond to certain inputs in a desired manner.

Prompt Engineering is the process of designing and optimizing prompts to get the best possible output from a model. It involves crafting effective prompts that can guide the model to produce more accurate, relevant, and useful responses.</dcterms:description>
        <oboInOwl:hasSynonym xml:lang="en">Prompt</oboInOwl:hasSynonym>
        <rdfs:label xml:lang="en">Prompting, Prompt Learning &amp; Prompt Engineering</rdfs:label>
    </owl:NamedIndividual>
    


    <!-- http://nlpkg.sebis.cit.tum.de/nlp-fos-hierarchy.owl#Speech_&amp;_Audio-specific_Language_Models -->

    <owl:NamedIndividual rdf:about="http://nlpkg.sebis.cit.tum.de/nlp-fos-hierarchy.owl#Speech_&amp;_Audio-specific_Language_Models">
        <rdf:type rdf:resource="http://nlpkg.sebis.cit.tum.de/nlp-fos-hierarchy.owl#OtherScientificField"/>
        <rdf:type rdf:resource="http://nlpkg.sebis.cit.tum.de/nlp-taxonomy.owl#FieldOfStudy"/>
        <nlp-taxonomy:subFieldOf rdf:resource="http://nlpkg.sebis.cit.tum.de/nlp-fos-hierarchy.owl#Multimodal_Language_Models"/>
        <nlp-taxonomy:subFieldOf rdf:resource="http://nlpkg.sebis.cit.tum.de/nlp-taxonomy.owl#Speech_&amp;_Audio_In_NLP"/>
        <survey>https://arxiv.org/abs/2303.11607</survey>
        <nlp-taxonomy:level rdf:datatype="http://www.w3.org/2001/XMLSchema#integer">3</nlp-taxonomy:level>
        <nlp-taxonomy:level rdf:datatype="http://www.w3.org/2001/XMLSchema#integer">4</nlp-taxonomy:level>
        <dcterms:description xml:lang="en">Speech and Audo-specific Language Models refers to specialized language models that are designed and trained to understand and generate human language specifically in the context of speech and audio data. These models are tailored to handle spoken language and sound-related tasks.</dcterms:description>
        <oboInOwl:hasSynonym xml:lang="en">Audio-Language Models</oboInOwl:hasSynonym>
        <oboInOwl:hasSynonym xml:lang="en">Audio-Language Transformers</oboInOwl:hasSynonym>
        <oboInOwl:hasSynonym xml:lang="en">Speech-Language Models</oboInOwl:hasSynonym>
        <oboInOwl:hasSynonym xml:lang="en">Speech-Language transformers</oboInOwl:hasSynonym>
        <rdfs:label xml:lang="en">Speech &amp; Audio-specific Language Models</rdfs:label>
    </owl:NamedIndividual>
    


    <!-- http://nlpkg.sebis.cit.tum.de/nlp-fos-hierarchy.owl#Transformers_&amp;_Large_Language_Models -->

    <owl:NamedIndividual rdf:about="http://nlpkg.sebis.cit.tum.de/nlp-fos-hierarchy.owl#Transformers_&amp;_Large_Language_Models">
        <rdf:type rdf:resource="http://nlpkg.sebis.cit.tum.de/nlp-fos-hierarchy.owl#OtherScientificField"/>
        <rdf:type rdf:resource="http://nlpkg.sebis.cit.tum.de/nlp-taxonomy.owl#FieldOfStudy"/>
        <usedFor rdf:resource="http://nlpkg.sebis.cit.tum.de/nlp-fos-hierarchy.owl#Sentence-Transformers"/>
        <uses rdf:resource="http://nlpkg.sebis.cit.tum.de/nlp-fos-hierarchy.owl#Attention"/>
        <uses rdf:resource="http://nlpkg.sebis.cit.tum.de/nlp-fos-hierarchy.owl#Positional_Encoding"/>
        <nlp-taxonomy:subFieldOf rdf:resource="http://nlpkg.sebis.cit.tum.de/nlp-taxonomy.owl#Language_Models"/>
        <nlp-taxonomy:superFieldOf rdf:resource="http://nlpkg.sebis.cit.tum.de/nlp-fos-hierarchy.owl#Efficient_Transformers"/>
        <nlp-taxonomy:superFieldOf rdf:resource="http://nlpkg.sebis.cit.tum.de/nlp-fos-hierarchy.owl#Knowledge_Augmented_Language_Models"/>
        <origin>https://arxiv.org/abs/1706.03762</origin>
        <relevantInformation>http://jalammar.github.io/illustrated-transformer/</relevantInformation>
        <relevantInformation xml:lang="yulemoon/an-in-depth-look-at-the-transformer-based-models-22e5f5d17b6b">https://medium.com/</relevantInformation>
        <relevantInformation>https://towardsdatascience.com/transformers-explained-visually-part-2-how-it-works-step-by-step-b49fa4a64f34</relevantInformation>
        <relevantInformation>https://web.stanford.edu/~jurafsky/slp3/10.pdf</relevantInformation>
        <relevantInformation>https://www.youtube.com/watch?v=EixI6t5oif0</relevantInformation>
        <survey>https://aclanthology.org/2020.acl-main.463</survey>
        <survey>https://aclanthology.org/2021.emnlp-main.81/</survey>
        <survey>https://aclanthology.org/2022.acl-long.492</survey>
        <survey>https://aclanthology.org/2022.lrec-1.804</survey>
        <survey>https://aclanthology.org/2023.acl-long.95</survey>
        <survey>https://aclanthology.org/2023.findings-acl.67</survey>
        <survey>https://arxiv.org/abs/2003.08271</survey>
        <survey>https://arxiv.org/abs/2007.04239</survey>
        <survey>https://arxiv.org/abs/2104.10810</survey>
        <survey>https://arxiv.org/abs/2106.04554</survey>
        <survey>https://arxiv.org/abs/2106.07139</survey>
        <survey>https://arxiv.org/abs/2108.05542</survey>
        <survey>https://arxiv.org/abs/2111.01243</survey>
        <survey>https://arxiv.org/abs/2204.10365</survey>
        <survey>https://arxiv.org/abs/2206.07682</survey>
        <survey>https://arxiv.org/abs/2208.11857</survey>
        <survey>https://arxiv.org/abs/2302.09419</survey>
        <survey>https://arxiv.org/abs/2303.07616</survey>
        <survey>https://arxiv.org/abs/2303.11504</survey>
        <survey>https://arxiv.org/abs/2303.18223</survey>
        <survey>https://arxiv.org/abs/2304.00612</survey>
        <survey>https://arxiv.org/abs/2304.01852</survey>
        <survey>https://arxiv.org/abs/2304.02020</survey>
        <survey>https://arxiv.org/abs/2304.06488</survey>
        <survey>https://arxiv.org/abs/2304.08354</survey>
        <survey>https://arxiv.org/abs/2304.13712</survey>
        <survey>https://arxiv.org/abs/2305.11391</survey>
        <survey>https://arxiv.org/abs/2305.14965</survey>
        <survey>https://arxiv.org/abs/2305.18703</survey>
        <survey>https://arxiv.org/abs/2307.03109</survey>
        <survey>https://arxiv.org/abs/2307.06435</survey>
        <survey>https://arxiv.org/abs/2307.10169</survey>
        <survey>https://arxiv.org/abs/2307.10188</survey>
        <survey>https://arxiv.org/abs/2307.15425</survey>
        <survey>https://arxiv.org/abs/2308.03188</survey>
        <survey>https://arxiv.org/abs/2308.11432</survey>
        <survey>https://arxiv.org/abs/2308.14149</survey>
        <survey>https://arxiv.org/abs/2309.07864</survey>
        <survey>https://arxiv.org/abs/2310.05694</survey>
        <survey>https://arxiv.org/abs/2310.07225</survey>
        <survey>https://arxiv.org/abs/2310.07343</survey>
        <survey>https://arxiv.org/abs/2310.07521</survey>
        <survey>https://arxiv.org/abs/2310.10844</survey>
        <survey>https://arxiv.org/abs/2310.13650</survey>
        <survey>https://arxiv.org/abs/2310.14389</survey>
        <survey>https://arxiv.org/abs/2310.14540</survey>
        <survey>https://arxiv.org/abs/2310.14542</survey>
        <survey>https://arxiv.org/abs/2310.16218</survey>
        <survey>https://arxiv.org/abs/2310.16570</survey>
        <survey>https://arxiv.org/abs/2310.17551</survey>
        <survey>https://arxiv.org/abs/2310.19736</survey>
        <survey>https://arxiv.org/abs/2311.00681</survey>
        <survey>https://arxiv.org/abs/2311.00686</survey>
        <survey>https://arxiv.org/abs/2311.01964</survey>
        <survey>https://arxiv.org/abs/2311.02049</survey>
        <survey>https://arxiv.org/abs/2311.02216</survey>
        <survey>https://arxiv.org/abs/2311.05112</survey>
        <survey>https://arxiv.org/abs/2312.02783</survey>
        <survey>https://arxiv.org/abs/2312.07622</survey>
        <survey>https://arxiv.org/abs/2312.17617</survey>
        <survey>https://arxiv.org/abs/2401.07103</survey>
        <survey>https://arxiv.org/abs/2401.07872</survey>
        <survey>https://arxiv.org/abs/2402.07927</survey>
        <nlp-taxonomy:level rdf:datatype="http://www.w3.org/2001/XMLSchema#integer">3</nlp-taxonomy:level>
        <dcterms:description xml:lang="en">Transformers &amp; Large Language Models is concerned with models based on the transformer neural network architecture that introduced the attention mechanism and has become foundational in various machine learning applications. In addition, this concept includes Large Language Models, a specific application of transformers that are pre-trained on large amounts of textual data and excel at various natural language processing tasks.</dcterms:description>
        <oboInOwl:hasSynonym xml:lang="en">Foundation Models</oboInOwl:hasSynonym>
        <oboInOwl:hasSynonym xml:lang="en">LLM</oboInOwl:hasSynonym>
        <oboInOwl:hasSynonym xml:lang="en">LLMs</oboInOwl:hasSynonym>
        <oboInOwl:hasSynonym xml:lang="en">Large Language Model</oboInOwl:hasSynonym>
        <oboInOwl:hasSynonym xml:lang="en">Pre-trained Foundation Models</oboInOwl:hasSynonym>
        <oboInOwl:hasSynonym xml:lang="en">Pre-trained Language Models</oboInOwl:hasSynonym>
        <oboInOwl:hasSynonym xml:lang="en">Pre-trained Model</oboInOwl:hasSynonym>
        <oboInOwl:hasSynonym xml:lang="en">Pretrained Foundation Models</oboInOwl:hasSynonym>
        <oboInOwl:hasSynonym xml:lang="en">Pretrained Language Models</oboInOwl:hasSynonym>
        <oboInOwl:hasSynonym xml:lang="en">Pretrained Model</oboInOwl:hasSynonym>
        <oboInOwl:hasSynonym xml:lang="en">Transformer</oboInOwl:hasSynonym>
        <oboInOwl:hasSynonym xml:lang="en">Transformer Language Model</oboInOwl:hasSynonym>
        <oboInOwl:hasSynonym xml:lang="en">Transformer Language Models</oboInOwl:hasSynonym>
        <oboInOwl:hasSynonym xml:lang="en">Transformer Models</oboInOwl:hasSynonym>
        <rdfs:label xml:lang="en">Transformers &amp; Large Language Models</rdfs:label>
    </owl:NamedIndividual>
    


    <!-- http://nlpkg.sebis.cit.tum.de/nlp-taxonomy#Aspect-based_Sentiment_Analysis -->

    <owl:NamedIndividual rdf:about="http://nlpkg.sebis.cit.tum.de/nlp-taxonomy#Aspect-based_Sentiment_Analysis">
        <rdf:type rdf:resource="http://nlpkg.sebis.cit.tum.de/nlp-fos-hierarchy.owl#Task"/>
        <rdf:type rdf:resource="http://nlpkg.sebis.cit.tum.de/nlp-taxonomy.owl#FieldOfStudy"/>
        <nlp-taxonomy:subFieldOf rdf:resource="http://nlpkg.sebis.cit.tum.de/nlp-taxonomy.owl#Sentiment_Analysis"/>
        <nlp-taxonomy:superFieldOf rdf:resource="http://nlpkg.sebis.cit.tum.de/nlp-fos-hierarchy.owl#Aspect_Sentiment_Quad_Prediction"/>
        <nlp-taxonomy:superFieldOf rdf:resource="http://nlpkg.sebis.cit.tum.de/nlp-fos-hierarchy.owl#Aspect_Sentiment_Triplet_Extraction"/>
        <nlp-taxonomy:superFieldOf rdf:resource="http://nlpkg.sebis.cit.tum.de/nlp-fos-hierarchy.owl#Aspect_Term_Extraction"/>
        <survey>https://arxiv.org/abs/2006.04611</survey>
        <survey>https://arxiv.org/abs/2203.01054</survey>
        <survey>https://arxiv.org/abs/2203.14266</survey>
        <survey>https://arxiv.org/abs/2204.05232</survey>
        <nlp-taxonomy:level rdf:datatype="http://www.w3.org/2001/XMLSchema#integer">2</nlp-taxonomy:level>
        <dcterms:description xml:lang="en">Aspect-based Sentiment Analysis (ABSA) is a subfield of Sentiment Analysis that is concerned with automatically identifying and analyzing the sentiment of a natural language text with respect to various aspects or facets rather than considering the text as a whole.</dcterms:description>
        <oboInOwl:hasSynonym xml:lang="en">ABSA</oboInOwl:hasSynonym>
        <oboInOwl:hasSynonym xml:lang="en">Aspect-Level Sentiment Classification</oboInOwl:hasSynonym>
        <oboInOwl:hasSynonym xml:lang="en">Aspect-based Sentiment Classification</oboInOwl:hasSynonym>
        <rdfs:label xml:lang="en">Aspect-based Sentiment Analysis</rdfs:label>
    </owl:NamedIndividual>
    


    <!-- http://nlpkg.sebis.cit.tum.de/nlp-taxonomy.owl#Argument_Mining -->

    <owl:NamedIndividual rdf:about="http://nlpkg.sebis.cit.tum.de/nlp-taxonomy.owl#Argument_Mining">
        <rdf:type rdf:resource="http://nlpkg.sebis.cit.tum.de/nlp-fos-hierarchy.owl#Task"/>
        <rdf:type rdf:resource="http://nlpkg.sebis.cit.tum.de/nlp-taxonomy.owl#FieldOfStudy"/>
        <nlp-taxonomy:subFieldOf rdf:resource="http://nlpkg.sebis.cit.tum.de/nlp-taxonomy.owl#Reasoning"/>
        <nlp-taxonomy:superFieldOf rdf:resource="http://nlpkg.sebis.cit.tum.de/nlp-fos-hierarchy.owl#Argument_Extraction"/>
        <nlp-taxonomy:superFieldOf rdf:resource="http://nlpkg.sebis.cit.tum.de/nlp-fos-hierarchy.owl#Argument_Generation"/>
        <nlp-taxonomy:superFieldOf rdf:resource="http://nlpkg.sebis.cit.tum.de/nlp-fos-hierarchy.owl#Argument_Pair_Identification"/>
        <survey>https://aclanthology.org/2021.acl-long.107</survey>
        <survey>https://aclanthology.org/J19-4006</survey>
        <survey>https://arxiv.org/abs/2107.08523</survey>
        <nlp-taxonomy:level rdf:datatype="http://www.w3.org/2001/XMLSchema#integer">2</nlp-taxonomy:level>
        <dcterms:description xml:lang="en">Argument Mining is a subfield of Reasoning that concerned with automatically identifying and analyzing the structure of inference and reasoning expressed as arguments presented in a natural language text, such as a debate, an opinion article, or a legal case.</dcterms:description>
        <oboInOwl:hasSynonym xml:lang="en">Argumentation Mining</oboInOwl:hasSynonym>
        <rdfs:label xml:lang="en">Argument Mining</rdfs:label>
    </owl:NamedIndividual>
    


    <!-- http://nlpkg.sebis.cit.tum.de/nlp-taxonomy.owl#Captioning -->

    <owl:NamedIndividual rdf:about="http://nlpkg.sebis.cit.tum.de/nlp-taxonomy.owl#Captioning">
        <rdf:type rdf:resource="http://nlpkg.sebis.cit.tum.de/nlp-fos-hierarchy.owl#Task"/>
        <rdf:type rdf:resource="http://nlpkg.sebis.cit.tum.de/nlp-taxonomy.owl#FieldOfStudy"/>
        <nlp-taxonomy:subFieldOf rdf:resource="http://nlpkg.sebis.cit.tum.de/nlp-taxonomy.owl#Text_Generation"/>
        <nlp-taxonomy:superFieldOf rdf:resource="http://nlpkg.sebis.cit.tum.de/nlp-fos-hierarchy.owl#Image_Captioning"/>
        <nlp-taxonomy:superFieldOf rdf:resource="http://nlpkg.sebis.cit.tum.de/nlp-fos-hierarchy.owl#Video_Captioning"/>
        <nlp-taxonomy:level rdf:datatype="http://www.w3.org/2001/XMLSchema#integer">2</nlp-taxonomy:level>
        <dcterms:description xml:lang="en">Captioning is a subfield of Text Generation that deals with the automatic generation of textual descriptions or captions for visual data, such as images and videos. This involves understanding the content of the visual data and generating a coherent and informative description that accurately reflects the visual information.</dcterms:description>
        <rdfs:label xml:lang="en">Captioning</rdfs:label>
    </owl:NamedIndividual>
    


    <!-- http://nlpkg.sebis.cit.tum.de/nlp-taxonomy.owl#Chunking -->

    <owl:NamedIndividual rdf:about="http://nlpkg.sebis.cit.tum.de/nlp-taxonomy.owl#Chunking">
        <rdf:type rdf:resource="http://nlpkg.sebis.cit.tum.de/nlp-fos-hierarchy.owl#Task"/>
        <rdf:type rdf:resource="http://nlpkg.sebis.cit.tum.de/nlp-taxonomy.owl#FieldOfStudy"/>
        <usedFor rdf:resource="http://nlpkg.sebis.cit.tum.de/nlp-taxonomy.owl#Text_Segmentation"/>
        <uses rdf:resource="http://nlpkg.sebis.cit.tum.de/nlp-fos-hierarchy.owl#Sequence_Labeling"/>
        <uses rdf:resource="http://nlpkg.sebis.cit.tum.de/nlp-fos-hierarchy.owl#Span_Detection"/>
        <nlp-taxonomy:subFieldOf rdf:resource="http://nlpkg.sebis.cit.tum.de/nlp-taxonomy.owl#Syntactic_Text_Processing"/>
        <relevantInformation xml:lang="evertongomede/the-shallow-parsing-in-natural-language-processing-89cf3049f42c">https://medium.com/</relevantInformation>
        <relevantInformation>https://www.pinecone.io/learn/chunking-strategies/</relevantInformation>
        <nlp-taxonomy:level rdf:datatype="http://www.w3.org/2001/XMLSchema#integer">2</nlp-taxonomy:level>
        <dcterms:description xml:lang="en">Chunking is a subfield of Syntactic Text Processing that deals with the automatic identification and grouping of coherent sequences of words or other linguistic units that form grammatically meaningful units or phrases in a sentence.</dcterms:description>
        <oboInOwl:hasSynonym xml:lang="en">Light Parsing</oboInOwl:hasSynonym>
        <oboInOwl:hasSynonym xml:lang="en">Shallow Parsing</oboInOwl:hasSynonym>
        <oboInOwl:hasSynonym xml:lang="en">Text Chunking</oboInOwl:hasSynonym>
        <rdfs:label xml:lang="en">Chunking</rdfs:label>
    </owl:NamedIndividual>
    


    <!-- http://nlpkg.sebis.cit.tum.de/nlp-taxonomy.owl#Code-Switching -->

    <owl:NamedIndividual rdf:about="http://nlpkg.sebis.cit.tum.de/nlp-taxonomy.owl#Code-Switching">
        <rdf:type rdf:resource="http://nlpkg.sebis.cit.tum.de/nlp-fos-hierarchy.owl#Task"/>
        <rdf:type rdf:resource="http://nlpkg.sebis.cit.tum.de/nlp-taxonomy.owl#FieldOfStudy"/>
        <nlp-taxonomy:subFieldOf rdf:resource="http://nlpkg.sebis.cit.tum.de/nlp-taxonomy.owl#Multilinguality"/>
        <survey>https://aclanthology.org/2021.acl-long.131</survey>
        <survey>https://aclanthology.org/2023.findings-acl.185</survey>
        <survey>https://arxiv.org/abs/1904.00784</survey>
        <nlp-taxonomy:level rdf:datatype="http://www.w3.org/2001/XMLSchema#integer">2</nlp-taxonomy:level>
        <dcterms:description xml:lang="en">Code Switching is a subfield of Multilinguality that deals with switching between two or more languages or language varieties in a single conversation or text.</dcterms:description>
        <rdfs:label xml:lang="en">Code-Switching</rdfs:label>
    </owl:NamedIndividual>
    


    <!-- http://nlpkg.sebis.cit.tum.de/nlp-taxonomy.owl#Code_Generation -->

    <owl:NamedIndividual rdf:about="http://nlpkg.sebis.cit.tum.de/nlp-taxonomy.owl#Code_Generation">
        <rdf:type rdf:resource="http://nlpkg.sebis.cit.tum.de/nlp-fos-hierarchy.owl#Task"/>
        <rdf:type rdf:resource="http://nlpkg.sebis.cit.tum.de/nlp-taxonomy.owl#FieldOfStudy"/>
        <uses rdf:resource="http://nlpkg.sebis.cit.tum.de/nlp-taxonomy.owl#Semantic_Parsing"/>
        <nlp-taxonomy:subFieldOf rdf:resource="http://nlpkg.sebis.cit.tum.de/nlp-taxonomy.owl#Programming_Languages_In_NLP"/>
        <nlp-taxonomy:subFieldOf rdf:resource="http://nlpkg.sebis.cit.tum.de/nlp-taxonomy.owl#Text_Generation"/>
        <nlp-taxonomy:superFieldOf rdf:resource="http://nlpkg.sebis.cit.tum.de/nlp-fos-hierarchy.owl#Text-to-SQL"/>
        <survey>https://aclanthology.org/2023.acl-long.411</survey>
        <survey>https://arxiv.org/abs/2105.03317</survey>
        <survey>https://arxiv.org/abs/2306.06371</survey>
        <nlp-taxonomy:level rdf:datatype="http://www.w3.org/2001/XMLSchema#integer">2</nlp-taxonomy:level>
        <nlp-taxonomy:level rdf:datatype="http://www.w3.org/2001/XMLSchema#integer">3</nlp-taxonomy:level>
        <dcterms:description xml:lang="en">Code Generation is a subfield of Text Generation that deals with the automatic generation of executable code, such as a computer program, from multimodal inputs such as incomplete code, programs in another programming language, natural language descriptions, or execution examples.</dcterms:description>
        <oboInOwl:hasSynonym xml:lang="en">Code Synthesis</oboInOwl:hasSynonym>
        <oboInOwl:hasSynonym xml:lang="en">NL2Code</oboInOwl:hasSynonym>
        <oboInOwl:hasSynonym xml:lang="en">Program Synthesis</oboInOwl:hasSynonym>
        <oboInOwl:hasSynonym xml:lang="en">Text to Code</oboInOwl:hasSynonym>
        <oboInOwl:hasSynonym xml:lang="en">Text-to-Code</oboInOwl:hasSynonym>
        <oboInOwl:hasSynonym xml:lang="en">Text2Code</oboInOwl:hasSynonym>
        <rdfs:label xml:lang="en">Code Generation</rdfs:label>
    </owl:NamedIndividual>
    


    <!-- http://nlpkg.sebis.cit.tum.de/nlp-taxonomy.owl#Cognitive_Modeling -->

    <owl:NamedIndividual rdf:about="http://nlpkg.sebis.cit.tum.de/nlp-taxonomy.owl#Cognitive_Modeling">
        <rdf:type rdf:resource="http://nlpkg.sebis.cit.tum.de/nlp-fos-hierarchy.owl#Task"/>
        <rdf:type rdf:resource="http://nlpkg.sebis.cit.tum.de/nlp-taxonomy.owl#FieldOfStudy"/>
        <nlp-taxonomy:subFieldOf rdf:resource="http://nlpkg.sebis.cit.tum.de/nlp-taxonomy.owl#Linguistics_&amp;_Cognitive_NLP"/>
        <nlp-taxonomy:level rdf:datatype="http://www.w3.org/2001/XMLSchema#integer">2</nlp-taxonomy:level>
        <dcterms:description xml:lang="en">Cognitive Modeling is a subfield of Linguistics &amp; Cognitive Natural Language Processing that is concerned with modeling and simulating human cognitive processes in various forms, especially in a computational or mathematical form. This includes analyzing the cognitive processes and mechanisms underlying natural language use and developing models and simulations that can capture and predict human behavior and performance on language-related tasks.</dcterms:description>
        <rdfs:label xml:lang="en">Cognitive Modeling</rdfs:label>
    </owl:NamedIndividual>
    


    <!-- http://nlpkg.sebis.cit.tum.de/nlp-taxonomy.owl#Commonsense_Reasoning -->

    <owl:NamedIndividual rdf:about="http://nlpkg.sebis.cit.tum.de/nlp-taxonomy.owl#Commonsense_Reasoning">
        <rdf:type rdf:resource="http://nlpkg.sebis.cit.tum.de/nlp-fos-hierarchy.owl#Task"/>
        <rdf:type rdf:resource="http://nlpkg.sebis.cit.tum.de/nlp-taxonomy.owl#FieldOfStudy"/>
        <nlp-taxonomy:subFieldOf rdf:resource="http://nlpkg.sebis.cit.tum.de/nlp-taxonomy.owl#Reasoning"/>
        <nlp-taxonomy:superFieldOf rdf:resource="http://nlpkg.sebis.cit.tum.de/nlp-fos-hierarchy.owl#Commonsense_Question_Answering"/>
        <nlp-taxonomy:superFieldOf rdf:resource="http://nlpkg.sebis.cit.tum.de/nlp-fos-hierarchy.owl#Visual_Commonsense_Reasoning"/>
        <survey>https://arxiv.org/abs/2108.04674</survey>
        <survey>https://arxiv.org/abs/2201.12438</survey>
        <survey>https://arxiv.org/abs/2302.07926</survey>
        <nlp-taxonomy:level rdf:datatype="http://www.w3.org/2001/XMLSchema#integer">2</nlp-taxonomy:level>
        <dcterms:description xml:lang="en">Commonsense Reasoning is a subfield of Reasoning that is concerned with the development of algorithms and models for reasoning about everyday situations and concepts that are not explicitly stated in the text but require &quot;common sense&quot; or world knowledge and are commonly understood by humans. This world knowledge includes judgments about the nature of physical objects, taxonomic properties, or peoples&apos; intentions.</dcterms:description>
        <oboInOwl:hasSynonym xml:lang="en">Commonsense Knowledge Reasoning</oboInOwl:hasSynonym>
        <rdfs:label xml:lang="en">Commonsense Reasoning</rdfs:label>
    </owl:NamedIndividual>
    


    <!-- http://nlpkg.sebis.cit.tum.de/nlp-taxonomy.owl#Coreference_Resolution -->

    <owl:NamedIndividual rdf:about="http://nlpkg.sebis.cit.tum.de/nlp-taxonomy.owl#Coreference_Resolution">
        <rdf:type rdf:resource="http://nlpkg.sebis.cit.tum.de/nlp-fos-hierarchy.owl#Task"/>
        <rdf:type rdf:resource="http://nlpkg.sebis.cit.tum.de/nlp-taxonomy.owl#FieldOfStudy"/>
        <usedFor rdf:resource="http://nlpkg.sebis.cit.tum.de/nlp-fos-hierarchy.owl#Entity-Level_Sentiment_Analysis"/>
        <usedFor rdf:resource="http://nlpkg.sebis.cit.tum.de/nlp-fos-hierarchy.owl#Ontology_Learning"/>
        <usedFor rdf:resource="http://nlpkg.sebis.cit.tum.de/nlp-fos-hierarchy.owl#Taxonomy_Learning"/>
        <usedFor rdf:resource="http://nlpkg.sebis.cit.tum.de/nlp-fos-hierarchy.owl#Knowledge_Graph_Construction_&amp;_Completion"/>
        <nlp-taxonomy:subFieldOf rdf:resource="http://nlpkg.sebis.cit.tum.de/nlp-taxonomy.owl#Information_Extraction_&amp;_Text_Mining"/>
        <nlp-taxonomy:superFieldOf rdf:resource="http://nlpkg.sebis.cit.tum.de/nlp-fos-hierarchy.owl#Anaphora_Resolution"/>
        <nlp-taxonomy:superFieldOf rdf:resource="http://nlpkg.sebis.cit.tum.de/nlp-fos-hierarchy.owl#Event_Coreference_Resolution"/>
        <relevantInformation>https://aclanthology.org/venues/crac/</relevantInformation>
        <relevantInformation>https://web.stanford.edu/~jurafsky/slp3/26.pdf</relevantInformation>
        <survey>https://aclanthology.org/2021.crac-1.1</survey>
        <survey>https://arxiv.org/abs/1805.11824</survey>
        <survey>https://arxiv.org/abs/1910.09329</survey>
        <nlp-taxonomy:level rdf:datatype="http://www.w3.org/2001/XMLSchema#integer">2</nlp-taxonomy:level>
        <dcterms:description xml:lang="en">Coreference Resolution is a subfield of Information Extraction &amp; Text Mining that deals with identifying all expressions that refer to the same entity in a text. In other words, it is the task of determining which pronouns, nouns, or phrases in a text refer to the same person, place, thing, or concept.</dcterms:description>
        <rdfs:label xml:lang="en">Coreference Resolution</rdfs:label>
    </owl:NamedIndividual>
    


    <!-- http://nlpkg.sebis.cit.tum.de/nlp-taxonomy.owl#Cross-Lingual_Transfer -->

    <owl:NamedIndividual rdf:about="http://nlpkg.sebis.cit.tum.de/nlp-taxonomy.owl#Cross-Lingual_Transfer">
        <rdf:type rdf:resource="http://nlpkg.sebis.cit.tum.de/nlp-fos-hierarchy.owl#Task"/>
        <rdf:type rdf:resource="http://nlpkg.sebis.cit.tum.de/nlp-taxonomy.owl#FieldOfStudy"/>
        <uses rdf:resource="http://nlpkg.sebis.cit.tum.de/nlp-fos-hierarchy.owl#Meta-Learning"/>
        <uses rdf:resource="http://nlpkg.sebis.cit.tum.de/nlp-fos-hierarchy.owl#Multilingual_Language_Models"/>
        <nlp-taxonomy:subFieldOf rdf:resource="http://nlpkg.sebis.cit.tum.de/nlp-taxonomy.owl#Multilinguality"/>
        <survey>https://aclanthology.org/2022.tacl-1.75</survey>
        <survey>https://aclanthology.org/2023.acl-long.323</survey>
        <survey>https://aclanthology.org/2023.findings-acl.439</survey>
        <survey>https://aclanthology.org/D18-1269</survey>
        <survey>https://arxiv.org/abs/1706.04902</survey>
        <survey>https://arxiv.org/abs/1908.10461</survey>
        <nlp-taxonomy:level rdf:datatype="http://www.w3.org/2001/XMLSchema#integer">2</nlp-taxonomy:level>
        <dcterms:description xml:lang="en">Cross-Lingual Transfer is a subfield of Multilinguality that deals with developing techniques and models for transferring knowledge learned from one language to solve tasks in another, commonly more low-resource, language.</dcterms:description>
        <rdfs:label xml:lang="en">Cross-Lingual Transfer</rdfs:label>
    </owl:NamedIndividual>
    


    <!-- http://nlpkg.sebis.cit.tum.de/nlp-taxonomy.owl#Data-to-Text_Generation -->

    <owl:NamedIndividual rdf:about="http://nlpkg.sebis.cit.tum.de/nlp-taxonomy.owl#Data-to-Text_Generation">
        <rdf:type rdf:resource="http://nlpkg.sebis.cit.tum.de/nlp-fos-hierarchy.owl#Task"/>
        <rdf:type rdf:resource="http://nlpkg.sebis.cit.tum.de/nlp-taxonomy.owl#FieldOfStudy"/>
        <nlp-taxonomy:subFieldOf rdf:resource="http://nlpkg.sebis.cit.tum.de/nlp-taxonomy.owl#Structured_Data_In_NLP"/>
        <nlp-taxonomy:subFieldOf rdf:resource="http://nlpkg.sebis.cit.tum.de/nlp-taxonomy.owl#Text_Generation"/>
        <nlp-taxonomy:superFieldOf rdf:resource="http://nlpkg.sebis.cit.tum.de/nlp-fos-hierarchy.owl#Graph-to-Text"/>
        <nlp-taxonomy:superFieldOf rdf:resource="http://nlpkg.sebis.cit.tum.de/nlp-fos-hierarchy.owl#Table-to-Text"/>
        <survey>https://arxiv.org/abs/1610.08375</survey>
        <survey>https://arxiv.org/abs/2207.12571</survey>
        <nlp-taxonomy:level rdf:datatype="http://www.w3.org/2001/XMLSchema#integer">2</nlp-taxonomy:level>
        <nlp-taxonomy:level rdf:datatype="http://www.w3.org/2001/XMLSchema#integer">3</nlp-taxonomy:level>
        <dcterms:description xml:lang="en">Structured Data-to-Text is a task that involves converting structured data, often in the form of tables, databases, or other organized data formats, into human-readable and coherent natural language text. The goal of structured data-to-text systems is to automatically generate descriptive and informative narratives or textual summaries that convey the key information contained within the structured data.</dcterms:description>
        <oboInOwl:hasSynonym xml:lang="en">Data-to-Text</oboInOwl:hasSynonym>
        <oboInOwl:hasSynonym xml:lang="en">Data-to-Text Generation</oboInOwl:hasSynonym>
        <oboInOwl:hasSynonym xml:lang="en">Data2Text</oboInOwl:hasSynonym>
        <rdfs:label xml:lang="en">Structured Data-to-Text</rdfs:label>
    </owl:NamedIndividual>
    


    <!-- http://nlpkg.sebis.cit.tum.de/nlp-taxonomy.owl#Dialogue_Response_Generation -->

    <owl:NamedIndividual rdf:about="http://nlpkg.sebis.cit.tum.de/nlp-taxonomy.owl#Dialogue_Response_Generation">
        <rdf:type rdf:resource="http://nlpkg.sebis.cit.tum.de/nlp-fos-hierarchy.owl#Task"/>
        <rdf:type rdf:resource="http://nlpkg.sebis.cit.tum.de/nlp-taxonomy.owl#FieldOfStudy"/>
        <nlp-taxonomy:subFieldOf rdf:resource="http://nlpkg.sebis.cit.tum.de/nlp-taxonomy.owl#Text_Generation"/>
        <nlp-taxonomy:subFieldOf rdf:resource="http://nlpkg.sebis.cit.tum.de/nlp-taxonomy.owl#Dialogue_Systems_&amp;_Conversational_Agents"/>
        <nlp-taxonomy:superFieldOf rdf:resource="http://nlpkg.sebis.cit.tum.de/nlp-fos-hierarchy.owl#Generative_Dialogue_Response_Generation"/>
        <nlp-taxonomy:superFieldOf rdf:resource="http://nlpkg.sebis.cit.tum.de/nlp-fos-hierarchy.owl#Retrieval-based_Dialogue_Response_Generation"/>
        <nlp-taxonomy:superFieldOf rdf:resource="http://nlpkg.sebis.cit.tum.de/nlp-fos-hierarchy.owl#Rule-based_Dialogue_Response_Generation"/>
        <survey>https://arxiv.org/abs/1906.00500</survey>
        <nlp-taxonomy:level rdf:datatype="http://www.w3.org/2001/XMLSchema#integer">2</nlp-taxonomy:level>
        <nlp-taxonomy:level rdf:datatype="http://www.w3.org/2001/XMLSchema#integer">3</nlp-taxonomy:level>
        <dcterms:description xml:lang="en">Dialogue Response Generation is a subfield of Text Generation that deals with the automatic generation of natural language responses in a conversational setting, such as chatbots and virtual assistants. It requires understanding the natural language input and generating a coherent and appropriate response that follows the flow of the conversation, takes context into account, and adheres to social and cultural norms.</dcterms:description>
        <oboInOwl:hasSynonym xml:lang="en">Dialog Response Generation</oboInOwl:hasSynonym>
        <oboInOwl:hasSynonym xml:lang="en">Dialogue Generation</oboInOwl:hasSynonym>
        <oboInOwl:hasSynonym xml:lang="en">Response Generation</oboInOwl:hasSynonym>
        <rdfs:label xml:lang="en">Dialogue Response Generation</rdfs:label>
    </owl:NamedIndividual>
    


    <!-- http://nlpkg.sebis.cit.tum.de/nlp-taxonomy.owl#Document_Retrieval -->

    <owl:NamedIndividual rdf:about="http://nlpkg.sebis.cit.tum.de/nlp-taxonomy.owl#Document_Retrieval">
        <rdf:type rdf:resource="http://nlpkg.sebis.cit.tum.de/nlp-fos-hierarchy.owl#Task"/>
        <rdf:type rdf:resource="http://nlpkg.sebis.cit.tum.de/nlp-taxonomy.owl#FieldOfStudy"/>
        <usedFor rdf:resource="http://nlpkg.sebis.cit.tum.de/nlp-fos-hierarchy.owl#Retrieval_Augmented_Generation"/>
        <usedFor rdf:resource="http://nlpkg.sebis.cit.tum.de/nlp-taxonomy.owl#Semantic_Search"/>
        <uses rdf:resource="http://nlpkg.sebis.cit.tum.de/nlp-taxonomy.owl#Semantic_Similarity"/>
        <uses rdf:resource="http://nlpkg.sebis.cit.tum.de/nlp-taxonomy.owl#Text_Segmentation"/>
        <nlp-taxonomy:subFieldOf rdf:resource="http://nlpkg.sebis.cit.tum.de/nlp-taxonomy.owl#Information_Retrieval"/>
        <nlp-taxonomy:superFieldOf rdf:resource="http://nlpkg.sebis.cit.tum.de/nlp-fos-hierarchy.owl#Dense_Document_Retrieval"/>
        <nlp-taxonomy:superFieldOf rdf:resource="http://nlpkg.sebis.cit.tum.de/nlp-fos-hierarchy.owl#Query_Representation"/>
        <nlp-taxonomy:superFieldOf rdf:resource="http://nlpkg.sebis.cit.tum.de/nlp-fos-hierarchy.owl#Sparse_Document_Retrieval"/>
        <survey>https://arxiv.org/abs/2010.06467</survey>
        <nlp-taxonomy:level rdf:datatype="http://www.w3.org/2001/XMLSchema#integer">2</nlp-taxonomy:level>
        <dcterms:description xml:lang="en">Document Retrieval is a subfield of Information Retrieval that deals with finding and retrieving relevant documents from a large corpus of textual data in response to a user query. It involves developing algorithms and models that can analyze the query and the corpus and rank the documents based on their relevance and similarity to the query.</dcterms:description>
        <rdfs:label xml:lang="en">Document Retrieval</rdfs:label>
    </owl:NamedIndividual>
    


    <!-- http://nlpkg.sebis.cit.tum.de/nlp-taxonomy.owl#Emotion_Analysis -->

    <owl:NamedIndividual rdf:about="http://nlpkg.sebis.cit.tum.de/nlp-taxonomy.owl#Emotion_Analysis">
        <rdf:type rdf:resource="http://nlpkg.sebis.cit.tum.de/nlp-fos-hierarchy.owl#Task"/>
        <rdf:type rdf:resource="http://nlpkg.sebis.cit.tum.de/nlp-taxonomy.owl#FieldOfStudy"/>
        <nlp-taxonomy:subFieldOf rdf:resource="http://nlpkg.sebis.cit.tum.de/nlp-taxonomy.owl#Sentiment_Analysis"/>
        <nlp-taxonomy:subFieldOf rdf:resource="http://nlpkg.sebis.cit.tum.de/nlp-taxonomy.owl#Text_Classification"/>
        <nlp-taxonomy:superFieldOf rdf:resource="http://nlpkg.sebis.cit.tum.de/nlp-fos-hierarchy.owl#Emotion_Cause_Analysis"/>
        <survey>https://aclanthology.org/W14-6905</survey>
        <survey>https://arxiv.org/abs/1806.00674</survey>
        <survey>https://arxiv.org/abs/1808.03137</survey>
        <survey>https://arxiv.org/abs/1905.02947</survey>
        <survey>https://arxiv.org/abs/2205.03235</survey>
        <survey>https://arxiv.org/abs/2211.09172</survey>
        <nlp-taxonomy:level rdf:datatype="http://www.w3.org/2001/XMLSchema#integer">2</nlp-taxonomy:level>
        <nlp-taxonomy:level rdf:datatype="http://www.w3.org/2001/XMLSchema#integer">3</nlp-taxonomy:level>
        <dcterms:description xml:lang="en">Emotion Analysis is a subfield of Sentiment Analysis that deals with the automatic detection and analysis of emotions in natural language texts, such as joy, anger, fear, and sadness.</dcterms:description>
        <oboInOwl:hasSynonym xml:lang="en">Emotion Classification</oboInOwl:hasSynonym>
        <oboInOwl:hasSynonym xml:lang="en">Emotion Detection</oboInOwl:hasSynonym>
        <oboInOwl:hasSynonym xml:lang="en">Emotion Identification</oboInOwl:hasSynonym>
        <oboInOwl:hasSynonym xml:lang="en">Emotion Recognition</oboInOwl:hasSynonym>
        <rdfs:label xml:lang="en">Emotion Analysis</rdfs:label>
    </owl:NamedIndividual>
    


    <!-- http://nlpkg.sebis.cit.tum.de/nlp-taxonomy.owl#Ethical_NLP -->

    <owl:NamedIndividual rdf:about="http://nlpkg.sebis.cit.tum.de/nlp-taxonomy.owl#Ethical_NLP">
        <rdf:type rdf:resource="http://nlpkg.sebis.cit.tum.de/nlp-fos-hierarchy.owl#OtherScientificField"/>
        <rdf:type rdf:resource="http://nlpkg.sebis.cit.tum.de/nlp-taxonomy.owl#FieldOfStudy"/>
        <nlp-taxonomy:subFieldOf rdf:resource="http://nlpkg.sebis.cit.tum.de/nlp-taxonomy.owl#Responsible_&amp;_Trustworthy_NLP"/>
        <nlp-taxonomy:superFieldOf rdf:resource="http://nlpkg.sebis.cit.tum.de/nlp-fos-hierarchy.owl#Discrimination_Analysis"/>
        <nlp-taxonomy:superFieldOf rdf:resource="http://nlpkg.sebis.cit.tum.de/nlp-fos-hierarchy.owl#Language_Model_Alignment"/>
        <nlp-taxonomy:superFieldOf rdf:resource="http://nlpkg.sebis.cit.tum.de/nlp-fos-hierarchy.owl#Misinformation_Detection"/>
        <nlp-taxonomy:superFieldOf rdf:resource="http://nlpkg.sebis.cit.tum.de/nlp-fos-hierarchy.owl#Propaganda_Detection"/>
        <nlp-taxonomy:superFieldOf rdf:resource="http://nlpkg.sebis.cit.tum.de/nlp-fos-hierarchy.owl#Biases_&amp;_Fairness_in_NLP"/>
        <nlp-taxonomy:superFieldOf rdf:resource="http://nlpkg.sebis.cit.tum.de/nlp-fos-hierarchy.owl#Privacy,_Security_&amp;_Safety_in_NLP"/>
        <relevantInformation>https://edwinwenink.github.io/ai-ethics-tool-landscape/</relevantInformation>
        <survey>https://aclanthology.org/2023.eacl-main.241</survey>
        <survey>https://aclanthology.org/W17-1604</survey>
        <survey>https://aclanthology.org/W17-1610</survey>
        <survey>https://arxiv.org/abs/2305.05471</survey>
        <survey>https://arxiv.org/abs/2310.17551</survey>
        <nlp-taxonomy:level rdf:datatype="http://www.w3.org/2001/XMLSchema#integer">2</nlp-taxonomy:level>
        <dcterms:description xml:lang="en">Ethical NLP is a subfield of Responsible NLP that deals with the ethical and social implications of developing and using natural language processing technologies. It involves developing algorithms and models that can handle issues such as fairness, bias, privacy, and transparency, and designing systems that promote ethical and responsible use of the technology.</dcterms:description>
        <oboInOwl:hasSynonym xml:lang="en">NLP for Social Good</oboInOwl:hasSynonym>
        <rdfs:label xml:lang="en">Ethical NLP</rdfs:label>
    </owl:NamedIndividual>
    


    <!-- http://nlpkg.sebis.cit.tum.de/nlp-taxonomy.owl#Event_Extraction -->

    <owl:NamedIndividual rdf:about="http://nlpkg.sebis.cit.tum.de/nlp-taxonomy.owl#Event_Extraction">
        <rdf:type rdf:resource="http://nlpkg.sebis.cit.tum.de/nlp-fos-hierarchy.owl#Task"/>
        <rdf:type rdf:resource="http://nlpkg.sebis.cit.tum.de/nlp-taxonomy.owl#FieldOfStudy"/>
        <uses rdf:resource="http://nlpkg.sebis.cit.tum.de/nlp-taxonomy.owl#Named_Entity_Recognition"/>
        <uses rdf:resource="http://nlpkg.sebis.cit.tum.de/nlp-taxonomy.owl#Relation_Extraction"/>
        <nlp-taxonomy:subFieldOf rdf:resource="http://nlpkg.sebis.cit.tum.de/nlp-taxonomy.owl#Information_Extraction_&amp;_Text_Mining"/>
        <nlp-taxonomy:superFieldOf rdf:resource="http://nlpkg.sebis.cit.tum.de/nlp-fos-hierarchy.owl#Event_Argument_Extraction"/>
        <nlp-taxonomy:superFieldOf rdf:resource="http://nlpkg.sebis.cit.tum.de/nlp-fos-hierarchy.owl#Event_Coreference_Resolution"/>
        <nlp-taxonomy:superFieldOf rdf:resource="http://nlpkg.sebis.cit.tum.de/nlp-fos-hierarchy.owl#Event_Detection"/>
        <nlp-taxonomy:superFieldOf rdf:resource="http://nlpkg.sebis.cit.tum.de/nlp-fos-hierarchy.owl#Event_Sequencing"/>
        <relevantInformation>https://web.stanford.edu/~jurafsky/slp3/21.pdf</relevantInformation>
        <survey>https://arxiv.org/abs/2107.02126</survey>
        <survey>https://arxiv.org/abs/2111.03212</survey>
        <survey>https://arxiv.org/abs/2210.03419</survey>
        <nlp-taxonomy:level rdf:datatype="http://www.w3.org/2001/XMLSchema#integer">2</nlp-taxonomy:level>
        <dcterms:description xml:lang="en">Event Extraction is a subfield of Information Extraction &amp; Text Mining that deals with identifying, extracting, and classifying events, such as accidents, elections, and natural disasters, from natural language text.</dcterms:description>
        <rdfs:label xml:lang="en">Event Extraction</rdfs:label>
    </owl:NamedIndividual>
    


    <!-- http://nlpkg.sebis.cit.tum.de/nlp-taxonomy.owl#Indexing -->

    <owl:NamedIndividual rdf:about="http://nlpkg.sebis.cit.tum.de/nlp-taxonomy.owl#Indexing">
        <rdf:type rdf:resource="http://nlpkg.sebis.cit.tum.de/nlp-fos-hierarchy.owl#Task"/>
        <rdf:type rdf:resource="http://nlpkg.sebis.cit.tum.de/nlp-taxonomy.owl#FieldOfStudy"/>
        <nlp-taxonomy:subFieldOf rdf:resource="http://nlpkg.sebis.cit.tum.de/nlp-taxonomy.owl#Information_Retrieval"/>
        <nlp-taxonomy:level rdf:datatype="http://www.w3.org/2001/XMLSchema#integer">2</nlp-taxonomy:level>
        <dcterms:description xml:lang="en">Indexing is a subfield of Information Retrieval that deals with creating and maintaining indexes of textual data. The index provides a way to quickly locate and retrieve relevant documents or passages that contain a particular term or keyword.</dcterms:description>
        <rdfs:label xml:lang="en">Indexing</rdfs:label>
    </owl:NamedIndividual>
    


    <!-- http://nlpkg.sebis.cit.tum.de/nlp-taxonomy.owl#Information_Retrieval -->

    <owl:NamedIndividual rdf:about="http://nlpkg.sebis.cit.tum.de/nlp-taxonomy.owl#Information_Retrieval">
        <rdf:type rdf:resource="http://nlpkg.sebis.cit.tum.de/nlp-fos-hierarchy.owl#Task"/>
        <rdf:type rdf:resource="http://nlpkg.sebis.cit.tum.de/nlp-taxonomy.owl#FieldOfStudy"/>
        <usedFor rdf:resource="http://nlpkg.sebis.cit.tum.de/nlp-fos-hierarchy.owl#Retrieval-based_Dialogue_Response_Generation"/>
        <usedFor rdf:resource="http://nlpkg.sebis.cit.tum.de/nlp-fos-hierarchy.owl#Retrieval-based_Question_Answering"/>
        <nlp-taxonomy:subFieldOf rdf:resource="http://nlpkg.sebis.cit.tum.de/nlp-taxonomy.owl#Natural_Language_Processing"/>
        <nlp-taxonomy:superFieldOf rdf:resource="http://nlpkg.sebis.cit.tum.de/nlp-fos-hierarchy.owl#Image-to-Text_Retrieval"/>
        <nlp-taxonomy:superFieldOf rdf:resource="http://nlpkg.sebis.cit.tum.de/nlp-fos-hierarchy.owl#Text-to-Image_Retrieval"/>
        <nlp-taxonomy:superFieldOf rdf:resource="http://nlpkg.sebis.cit.tum.de/nlp-fos-hierarchy.owl#Text_Regression"/>
        <nlp-taxonomy:superFieldOf rdf:resource="http://nlpkg.sebis.cit.tum.de/nlp-fos-hierarchy.owl#Video-Text_Retrieval"/>
        <nlp-taxonomy:superFieldOf rdf:resource="http://nlpkg.sebis.cit.tum.de/nlp-taxonomy.owl#Document_Retrieval"/>
        <nlp-taxonomy:superFieldOf rdf:resource="http://nlpkg.sebis.cit.tum.de/nlp-taxonomy.owl#Indexing"/>
        <nlp-taxonomy:superFieldOf rdf:resource="http://nlpkg.sebis.cit.tum.de/nlp-taxonomy.owl#Passage_Retrieval"/>
        <nlp-taxonomy:superFieldOf rdf:resource="http://nlpkg.sebis.cit.tum.de/nlp-taxonomy.owl#Semantic_Search"/>
        <nlp-taxonomy:superFieldOf rdf:resource="http://nlpkg.sebis.cit.tum.de/nlp-taxonomy.owl#Text_Classification"/>
        <relevantInformation>https://web.stanford.edu/~jurafsky/slp3/14.pdf</relevantInformation>
        <survey>https://arxiv.org/abs/1607.06215</survey>
        <survey>https://arxiv.org/abs/1705.01509</survey>
        <survey>https://arxiv.org/abs/2111.13853</survey>
        <survey>https://arxiv.org/abs/2308.07107</survey>
        <nlp-taxonomy:level rdf:datatype="http://www.w3.org/2001/XMLSchema#integer">1</nlp-taxonomy:level>
        <dcterms:description xml:lang="en">Information Retrieval is a subfield of Natural Language Processing (NLP) that focuses on the automatic retrieval of relevant information from large collections of unstructured textual data. It involves developing techniques and algorithms to search, retrieve, and present information in response to user queries. Information Retrieval is concerned with understanding the meaning of the user&apos;s query and matching it with relevant information in the collection, taking into account factors such as word meaning, word similarity, and relevance.</dcterms:description>
        <oboInOwl:hasSynonym xml:lang="en">IR</oboInOwl:hasSynonym>
        <rdfs:label xml:lang="en">Information Retrieval</rdfs:label>
    </owl:NamedIndividual>
    


    <!-- http://nlpkg.sebis.cit.tum.de/nlp-taxonomy.owl#Intent_Recognition -->

    <owl:NamedIndividual rdf:about="http://nlpkg.sebis.cit.tum.de/nlp-taxonomy.owl#Intent_Recognition">
        <rdf:type rdf:resource="http://nlpkg.sebis.cit.tum.de/nlp-fos-hierarchy.owl#Task"/>
        <rdf:type rdf:resource="http://nlpkg.sebis.cit.tum.de/nlp-taxonomy.owl#FieldOfStudy"/>
        <usedFor rdf:resource="http://nlpkg.sebis.cit.tum.de/nlp-fos-hierarchy.owl#Dialogue_Understanding"/>
        <usedFor rdf:resource="http://nlpkg.sebis.cit.tum.de/nlp-fos-hierarchy.owl#Spoken_Language_Understanding"/>
        <nlp-taxonomy:subFieldOf rdf:resource="http://nlpkg.sebis.cit.tum.de/nlp-taxonomy.owl#Sentiment_Analysis"/>
        <nlp-taxonomy:subFieldOf rdf:resource="http://nlpkg.sebis.cit.tum.de/nlp-taxonomy.owl#Text_Classification"/>
        <survey>https://aclanthology.org/2020.coling-main.42</survey>
        <survey>https://arxiv.org/abs/2101.08091</survey>
        <survey>https://arxiv.org/abs/2207.13211</survey>
        <nlp-taxonomy:level rdf:datatype="http://www.w3.org/2001/XMLSchema#integer">2</nlp-taxonomy:level>
        <nlp-taxonomy:level rdf:datatype="http://www.w3.org/2001/XMLSchema#integer">3</nlp-taxonomy:level>
        <dcterms:description xml:lang="en">Intent Recognition is a subfield of Sentiment Analysis that deals with the automatic identification and classification of the intentions or goals associated with natural language texts or utterances.</dcterms:description>
        <oboInOwl:hasSynonym xml:lang="en">Intent Classification</oboInOwl:hasSynonym>
        <oboInOwl:hasSynonym xml:lang="en">Intent Detection</oboInOwl:hasSynonym>
        <oboInOwl:hasSynonym xml:lang="en">Intent Identification</oboInOwl:hasSynonym>
        <rdfs:label xml:lang="en">Intent Recognition</rdfs:label>
    </owl:NamedIndividual>
    


    <!-- http://nlpkg.sebis.cit.tum.de/nlp-taxonomy.owl#Knowledge_Graph_Reasoning -->

    <owl:NamedIndividual rdf:about="http://nlpkg.sebis.cit.tum.de/nlp-taxonomy.owl#Knowledge_Graph_Reasoning">
        <rdf:type rdf:resource="http://nlpkg.sebis.cit.tum.de/nlp-fos-hierarchy.owl#Task"/>
        <rdf:type rdf:resource="http://nlpkg.sebis.cit.tum.de/nlp-taxonomy.owl#FieldOfStudy"/>
        <usedFor rdf:resource="http://nlpkg.sebis.cit.tum.de/nlp-fos-hierarchy.owl#Knowledge_Graph_Construction_&amp;_Completion"/>
        <nlp-taxonomy:subFieldOf rdf:resource="http://nlpkg.sebis.cit.tum.de/nlp-fos-hierarchy.owl#Knowledge_Graphs"/>
        <nlp-taxonomy:subFieldOf rdf:resource="http://nlpkg.sebis.cit.tum.de/nlp-taxonomy.owl#Reasoning"/>
        <nlp-taxonomy:superFieldOf rdf:resource="http://nlpkg.sebis.cit.tum.de/nlp-fos-hierarchy.owl#Knowledge_Graph_Embeddings"/>
        <nlp-taxonomy:superFieldOf rdf:resource="http://nlpkg.sebis.cit.tum.de/nlp-fos-hierarchy.owl#Knowledge_Graph_Error_Detection"/>
        <nlp-taxonomy:superFieldOf rdf:resource="http://nlpkg.sebis.cit.tum.de/nlp-fos-hierarchy.owl#Link_Prediction"/>
        <nlp-taxonomy:superFieldOf rdf:resource="http://nlpkg.sebis.cit.tum.de/nlp-fos-hierarchy.owl#Triple_Classification"/>
        <nlp-taxonomy:superFieldOf rdf:resource="http://nlpkg.sebis.cit.tum.de/nlp-taxonomy.owl#Named_Entity_Recognition"/>
        <nlp-taxonomy:superFieldOf rdf:resource="http://nlpkg.sebis.cit.tum.de/nlp-taxonomy.owl#Relation_Extraction"/>
        <survey>https://arxiv.org/abs/2010.05446</survey>
        <survey>https://arxiv.org/abs/2202.12205</survey>
        <survey>https://arxiv.org/abs/2212.05767</survey>
        <nlp-taxonomy:level rdf:datatype="http://www.w3.org/2001/XMLSchema#integer">2</nlp-taxonomy:level>
        <nlp-taxonomy:level rdf:datatype="http://www.w3.org/2001/XMLSchema#integer">6</nlp-taxonomy:level>
        <dcterms:description xml:lang="en">Knowledge Graph Reasoning is a subfield of Reasoning that deals with inferring new knowledge from existing entities, relationships, and concepts in knowledge graphs.</dcterms:description>
        <oboInOwl:hasSynonym xml:lang="en">KG Reasoning</oboInOwl:hasSynonym>
        <rdfs:label xml:lang="en">Knowledge Graph Reasoning</rdfs:label>
    </owl:NamedIndividual>
    


    <!-- http://nlpkg.sebis.cit.tum.de/nlp-taxonomy.owl#Knowledge_Representation -->

    <owl:NamedIndividual rdf:about="http://nlpkg.sebis.cit.tum.de/nlp-taxonomy.owl#Knowledge_Representation">
        <rdf:type rdf:resource="http://nlpkg.sebis.cit.tum.de/nlp-fos-hierarchy.owl#DataStructure"/>
        <rdf:type rdf:resource="http://nlpkg.sebis.cit.tum.de/nlp-taxonomy.owl#FieldOfStudy"/>
        <nlp-taxonomy:subFieldOf rdf:resource="http://nlpkg.sebis.cit.tum.de/nlp-taxonomy.owl#Semantic_Text_Processing"/>
        <nlp-taxonomy:superFieldOf rdf:resource="http://nlpkg.sebis.cit.tum.de/nlp-fos-hierarchy.owl#Knowledge_Bases"/>
        <nlp-taxonomy:superFieldOf rdf:resource="http://nlpkg.sebis.cit.tum.de/nlp-fos-hierarchy.owl#Text_Representations"/>
        <nlp-taxonomy:level rdf:datatype="http://www.w3.org/2001/XMLSchema#integer">2</nlp-taxonomy:level>
        <dcterms:description xml:lang="en">Knowledge Representation is a subfield of Semantic Text Processing that deals with the representation, organization, and management of knowledge and information in a form that can be processed and used by computers in conjunction with natural language texts. It involves developing formal languages and frameworks, such as ontologies, semantic networks, and knowledge graphs, that can capture and represent the semantics, structure, and relations of concepts and entities in a domain-specific or general knowledge base.</dcterms:description>
        <rdfs:label xml:lang="en">Knowledge Representation</rdfs:label>
    </owl:NamedIndividual>
    


    <!-- http://nlpkg.sebis.cit.tum.de/nlp-taxonomy.owl#Language_Models -->

    <owl:NamedIndividual rdf:about="http://nlpkg.sebis.cit.tum.de/nlp-taxonomy.owl#Language_Models">
        <rdf:type rdf:resource="http://nlpkg.sebis.cit.tum.de/nlp-fos-hierarchy.owl#OtherScientificField"/>
        <rdf:type rdf:resource="http://nlpkg.sebis.cit.tum.de/nlp-taxonomy.owl#FieldOfStudy"/>
        <uses rdf:resource="http://nlpkg.sebis.cit.tum.de/nlp-fos-hierarchy.owl#Tokenization"/>
        <nlp-taxonomy:subFieldOf rdf:resource="http://nlpkg.sebis.cit.tum.de/nlp-taxonomy.owl#Semantic_Text_Processing"/>
        <nlp-taxonomy:superFieldOf rdf:resource="http://nlpkg.sebis.cit.tum.de/nlp-fos-hierarchy.owl#Autoencoder"/>
        <nlp-taxonomy:superFieldOf rdf:resource="http://nlpkg.sebis.cit.tum.de/nlp-fos-hierarchy.owl#Conditional_Random_Field"/>
        <nlp-taxonomy:superFieldOf rdf:resource="http://nlpkg.sebis.cit.tum.de/nlp-fos-hierarchy.owl#Curriculum_Learning"/>
        <nlp-taxonomy:superFieldOf rdf:resource="http://nlpkg.sebis.cit.tum.de/nlp-fos-hierarchy.owl#Domain_Adaptation"/>
        <nlp-taxonomy:superFieldOf rdf:resource="http://nlpkg.sebis.cit.tum.de/nlp-fos-hierarchy.owl#Few-shot_Learning"/>
        <nlp-taxonomy:superFieldOf rdf:resource="http://nlpkg.sebis.cit.tum.de/nlp-fos-hierarchy.owl#Language_Model_Alignment"/>
        <nlp-taxonomy:superFieldOf rdf:resource="http://nlpkg.sebis.cit.tum.de/nlp-fos-hierarchy.owl#Language_Model_Hallucination"/>
        <nlp-taxonomy:superFieldOf rdf:resource="http://nlpkg.sebis.cit.tum.de/nlp-fos-hierarchy.owl#Language_Model_Mechanisms"/>
        <nlp-taxonomy:superFieldOf rdf:resource="http://nlpkg.sebis.cit.tum.de/nlp-fos-hierarchy.owl#Language_Model_Quantization"/>
        <nlp-taxonomy:superFieldOf rdf:resource="http://nlpkg.sebis.cit.tum.de/nlp-fos-hierarchy.owl#Meta-Learning"/>
        <nlp-taxonomy:superFieldOf rdf:resource="http://nlpkg.sebis.cit.tum.de/nlp-fos-hierarchy.owl#Multi-task_Learning"/>
        <nlp-taxonomy:superFieldOf rdf:resource="http://nlpkg.sebis.cit.tum.de/nlp-fos-hierarchy.owl#Multilingual_Language_Models"/>
        <nlp-taxonomy:superFieldOf rdf:resource="http://nlpkg.sebis.cit.tum.de/nlp-fos-hierarchy.owl#Multimodal_Language_Models"/>
        <nlp-taxonomy:superFieldOf rdf:resource="http://nlpkg.sebis.cit.tum.de/nlp-fos-hierarchy.owl#Parameter-Efficient_Fine-Tuning"/>
        <nlp-taxonomy:superFieldOf rdf:resource="http://nlpkg.sebis.cit.tum.de/nlp-fos-hierarchy.owl#Probing"/>
        <nlp-taxonomy:superFieldOf rdf:resource="http://nlpkg.sebis.cit.tum.de/nlp-fos-hierarchy.owl#Recurrent_Neural_Network"/>
        <nlp-taxonomy:superFieldOf rdf:resource="http://nlpkg.sebis.cit.tum.de/nlp-fos-hierarchy.owl#Zero-shot_Learning"/>
        <nlp-taxonomy:superFieldOf rdf:resource="http://nlpkg.sebis.cit.tum.de/nlp-fos-hierarchy.owl#n-gram_Language_Model"/>
        <nlp-taxonomy:superFieldOf rdf:resource="http://nlpkg.sebis.cit.tum.de/nlp-fos-hierarchy.owl#Multi-Agent_Systems_&amp;_Multi-Model_Language_Models"/>
        <nlp-taxonomy:superFieldOf rdf:resource="http://nlpkg.sebis.cit.tum.de/nlp-fos-hierarchy.owl#Prompting,_Prompt_Learning_&amp;_Prompt_Engineering"/>
        <nlp-taxonomy:superFieldOf rdf:resource="http://nlpkg.sebis.cit.tum.de/nlp-fos-hierarchy.owl#Transformers_&amp;_Large_Language_Models"/>
        <relevantInformation>https://web.stanford.edu/~jurafsky/slp3/7.pdf</relevantInformation>
        <survey>https://aclanthology.org/2023.findings-eacl.180</survey>
        <survey>https://aclanthology.org/D19-1250</survey>
        <survey>https://arxiv.org/abs/1704.08531</survey>
        <survey>https://arxiv.org/abs/1708.02709</survey>
        <survey>https://arxiv.org/abs/1807.10854</survey>
        <survey>https://arxiv.org/abs/1906.03591</survey>
        <survey>https://arxiv.org/abs/2003.01200</survey>
        <survey>https://arxiv.org/abs/2006.01338</survey>
        <survey>https://arxiv.org/abs/2007.04239</survey>
        <survey>https://arxiv.org/abs/2204.06031</survey>
        <survey>https://arxiv.org/abs/2303.04226</survey>
        <nlp-taxonomy:level rdf:datatype="http://www.w3.org/2001/XMLSchema#integer">2</nlp-taxonomy:level>
        <dcterms:description xml:lang="en">Language Models &amp; Neural Networks is a subfield of Semantic Text Processing that deals with the probabilistic modeling and generation of natural language, based on a learned probability function of sequences of words. Language models generate probabilities by training on corpora of natural language texts and can be fine-tuned for a variety of different downstream tasks. Neural networks are methods in artificial intelligence (AI) that teach computers to process data in a way that is inspired by the human brain.</dcterms:description>
        <oboInOwl:hasSynonym xml:lang="en">Deep Learning</oboInOwl:hasSynonym>
        <oboInOwl:hasSynonym xml:lang="en">LM</oboInOwl:hasSynonym>
        <oboInOwl:hasSynonym xml:lang="en">LMs</oboInOwl:hasSynonym>
        <oboInOwl:hasSynonym xml:lang="en">Language Models</oboInOwl:hasSynonym>
        <oboInOwl:hasSynonym xml:lang="en">Neural Networks</oboInOwl:hasSynonym>
        <rdfs:label xml:lang="en">Language Models &amp; Neural Networks</rdfs:label>
    </owl:NamedIndividual>
    


    <!-- http://nlpkg.sebis.cit.tum.de/nlp-taxonomy.owl#Linguistic_Theories -->

    <owl:NamedIndividual rdf:about="http://nlpkg.sebis.cit.tum.de/nlp-taxonomy.owl#Linguistic_Theories">
        <rdf:type rdf:resource="http://nlpkg.sebis.cit.tum.de/nlp-fos-hierarchy.owl#OtherScientificField"/>
        <rdf:type rdf:resource="http://nlpkg.sebis.cit.tum.de/nlp-taxonomy.owl#FieldOfStudy"/>
        <nlp-taxonomy:subFieldOf rdf:resource="http://nlpkg.sebis.cit.tum.de/nlp-taxonomy.owl#Linguistics_&amp;_Cognitive_NLP"/>
        <nlp-taxonomy:superFieldOf rdf:resource="http://nlpkg.sebis.cit.tum.de/nlp-fos-hierarchy.owl#Construction_Grammar"/>
        <nlp-taxonomy:superFieldOf rdf:resource="http://nlpkg.sebis.cit.tum.de/nlp-fos-hierarchy.owl#Distributional_Semantics"/>
        <nlp-taxonomy:superFieldOf rdf:resource="http://nlpkg.sebis.cit.tum.de/nlp-fos-hierarchy.owl#Head-driven_Phrase_Structure_Grammar"/>
        <nlp-taxonomy:superFieldOf rdf:resource="http://nlpkg.sebis.cit.tum.de/nlp-fos-hierarchy.owl#Rhetorical_Structure_Theory"/>
        <nlp-taxonomy:level rdf:datatype="http://www.w3.org/2001/XMLSchema#integer">2</nlp-taxonomy:level>
        <dcterms:description xml:lang="en">Linguistic Theories is a subfield of Linguistics &amp; Cognitive Natural Language Processing that explores the nature of language and attempts to answer fundamental questions about what language is or what is the common basis of all languages. Additionally, the goal is also to provide a general theoretical framework that describes, explains, and predicts how language is used and processed.</dcterms:description>
        <rdfs:label xml:lang="en">Linguistic Theories</rdfs:label>
    </owl:NamedIndividual>
    


    <!-- http://nlpkg.sebis.cit.tum.de/nlp-taxonomy.owl#Low-Resource_NLP -->

    <owl:NamedIndividual rdf:about="http://nlpkg.sebis.cit.tum.de/nlp-taxonomy.owl#Low-Resource_NLP">
        <rdf:type rdf:resource="http://nlpkg.sebis.cit.tum.de/nlp-fos-hierarchy.owl#OtherScientificField"/>
        <rdf:type rdf:resource="http://nlpkg.sebis.cit.tum.de/nlp-taxonomy.owl#FieldOfStudy"/>
        <nlp-taxonomy:subFieldOf rdf:resource="http://nlpkg.sebis.cit.tum.de/nlp-taxonomy.owl#Responsible_&amp;_Trustworthy_NLP"/>
        <nlp-taxonomy:superFieldOf rdf:resource="http://nlpkg.sebis.cit.tum.de/nlp-fos-hierarchy.owl#Active_Learning"/>
        <nlp-taxonomy:superFieldOf rdf:resource="http://nlpkg.sebis.cit.tum.de/nlp-fos-hierarchy.owl#Data_Augmentation"/>
        <nlp-taxonomy:superFieldOf rdf:resource="http://nlpkg.sebis.cit.tum.de/nlp-fos-hierarchy.owl#Domain_Adaptation"/>
        <nlp-taxonomy:superFieldOf rdf:resource="http://nlpkg.sebis.cit.tum.de/nlp-fos-hierarchy.owl#Few-shot_Learning"/>
        <nlp-taxonomy:superFieldOf rdf:resource="http://nlpkg.sebis.cit.tum.de/nlp-fos-hierarchy.owl#Multi-task_Learning"/>
        <nlp-taxonomy:superFieldOf rdf:resource="http://nlpkg.sebis.cit.tum.de/nlp-fos-hierarchy.owl#Reinforcement_Learning"/>
        <nlp-taxonomy:superFieldOf rdf:resource="http://nlpkg.sebis.cit.tum.de/nlp-fos-hierarchy.owl#Self-supervised_Learning"/>
        <nlp-taxonomy:superFieldOf rdf:resource="http://nlpkg.sebis.cit.tum.de/nlp-fos-hierarchy.owl#Semi-supervised_Learning"/>
        <nlp-taxonomy:superFieldOf rdf:resource="http://nlpkg.sebis.cit.tum.de/nlp-fos-hierarchy.owl#Unsupervised_Learning"/>
        <nlp-taxonomy:superFieldOf rdf:resource="http://nlpkg.sebis.cit.tum.de/nlp-fos-hierarchy.owl#Weak_Supervision"/>
        <nlp-taxonomy:superFieldOf rdf:resource="http://nlpkg.sebis.cit.tum.de/nlp-fos-hierarchy.owl#Zero-shot_Learning"/>
        <relevantInformation>https://aclanthology.org/sigs/sigul/</relevantInformation>
        <survey>https://aclanthology.org/2020.lrec-1.230</survey>
        <survey>https://aclanthology.org/2021.naacl-main.201</survey>
        <survey>https://aclanthology.org/2022.cl-3.6</survey>
        <survey>https://arxiv.org/abs/1910.00373</survey>
        <survey>https://arxiv.org/abs/2006.07264</survey>
        <survey>https://arxiv.org/abs/2106.15115</survey>
        <survey>https://arxiv.org/abs/2107.04239</survey>
        <survey>https://arxiv.org/abs/2202.08063</survey>
        <nlp-taxonomy:level rdf:datatype="http://www.w3.org/2001/XMLSchema#integer">2</nlp-taxonomy:level>
        <dcterms:description xml:lang="en">Low-Resource NLP is a subfield of Responsible NLP which is concerned with the development of algorithms and models that work in resource-constrained environments, such as data scarcity and low-resource languages.</dcterms:description>
        <oboInOwl:hasSynonym xml:lang="en">Low-Resource</oboInOwl:hasSynonym>
        <rdfs:label xml:lang="en">Low-Resource NLP</rdfs:label>
    </owl:NamedIndividual>
    


    <!-- http://nlpkg.sebis.cit.tum.de/nlp-taxonomy.owl#Machine_Reading_Comprehension -->

    <owl:NamedIndividual rdf:about="http://nlpkg.sebis.cit.tum.de/nlp-taxonomy.owl#Machine_Reading_Comprehension">
        <rdf:type rdf:resource="http://nlpkg.sebis.cit.tum.de/nlp-fos-hierarchy.owl#Task"/>
        <rdf:type rdf:resource="http://nlpkg.sebis.cit.tum.de/nlp-taxonomy.owl#FieldOfStudy"/>
        <usedFor rdf:resource="http://nlpkg.sebis.cit.tum.de/nlp-taxonomy.owl#Question_Answering"/>
        <nlp-taxonomy:subFieldOf rdf:resource="http://nlpkg.sebis.cit.tum.de/nlp-taxonomy.owl#Reasoning"/>
        <nlp-taxonomy:superFieldOf rdf:resource="http://nlpkg.sebis.cit.tum.de/nlp-fos-hierarchy.owl#Conversational_Machine_Comprehension"/>
        <survey>https://aclanthology.org/2021.emnlp-main.693</survey>
        <survey>https://arxiv.org/abs/1906.03824</survey>
        <survey>https://arxiv.org/abs/1907.01118</survey>
        <survey>https://arxiv.org/abs/1907.01686</survey>
        <survey>https://arxiv.org/abs/2001.01582</survey>
        <survey>https://arxiv.org/abs/2005.06249</survey>
        <survey>https://arxiv.org/abs/2006.11880</survey>
        <survey>https://arxiv.org/abs/2010.00389</survey>
        <survey>https://arxiv.org/abs/2209.01824</survey>
        <survey>https://arxiv.org/abs/2212.04070</survey>
        <survey>https://arxiv.org/abs/2212.04072</survey>
        <nlp-taxonomy:level rdf:datatype="http://www.w3.org/2001/XMLSchema#integer">2</nlp-taxonomy:level>
        <dcterms:description xml:lang="en">Machine Reading Comprehension is a subfield of Reasoning that deals with the task of automatically reading and understanding a piece of text and answering questions about it, as a human would. It involves developing algorithms and models that can handle the complexity and ambiguity of natural language, and reason about the implicit and explicit information in the text to infer the correct answer.</dcterms:description>
        <oboInOwl:hasSynonym xml:lang="en">MRC</oboInOwl:hasSynonym>
        <oboInOwl:hasSynonym xml:lang="en">Machine Comprehension</oboInOwl:hasSynonym>
        <oboInOwl:hasSynonym xml:lang="en">Reading Comprehension</oboInOwl:hasSynonym>
        <rdfs:label xml:lang="en">Machine Reading Comprehension</rdfs:label>
    </owl:NamedIndividual>
    


    <!-- http://nlpkg.sebis.cit.tum.de/nlp-taxonomy.owl#Machine_Translation -->

    <owl:NamedIndividual rdf:about="http://nlpkg.sebis.cit.tum.de/nlp-taxonomy.owl#Machine_Translation">
        <rdf:type rdf:resource="http://nlpkg.sebis.cit.tum.de/nlp-fos-hierarchy.owl#Task"/>
        <rdf:type rdf:resource="http://nlpkg.sebis.cit.tum.de/nlp-taxonomy.owl#FieldOfStudy"/>
        <uses rdf:resource="http://nlpkg.sebis.cit.tum.de/nlp-fos-hierarchy.owl#Translation_Memory"/>
        <nlp-taxonomy:subFieldOf rdf:resource="http://nlpkg.sebis.cit.tum.de/nlp-taxonomy.owl#Multilinguality"/>
        <nlp-taxonomy:subFieldOf rdf:resource="http://nlpkg.sebis.cit.tum.de/nlp-taxonomy.owl#Text_Generation"/>
        <nlp-taxonomy:superFieldOf rdf:resource="http://nlpkg.sebis.cit.tum.de/nlp-fos-hierarchy.owl#Automatic_Post-Editing"/>
        <nlp-taxonomy:superFieldOf rdf:resource="http://nlpkg.sebis.cit.tum.de/nlp-fos-hierarchy.owl#Bilingual_Lexicon_Induction"/>
        <nlp-taxonomy:superFieldOf rdf:resource="http://nlpkg.sebis.cit.tum.de/nlp-fos-hierarchy.owl#Hybrid_Machine_Translation"/>
        <nlp-taxonomy:superFieldOf rdf:resource="http://nlpkg.sebis.cit.tum.de/nlp-fos-hierarchy.owl#Neural_Machine_Translation"/>
        <nlp-taxonomy:superFieldOf rdf:resource="http://nlpkg.sebis.cit.tum.de/nlp-fos-hierarchy.owl#Rule-based_Machine_Translation"/>
        <nlp-taxonomy:superFieldOf rdf:resource="http://nlpkg.sebis.cit.tum.de/nlp-fos-hierarchy.owl#Statistical_Machine_Translation"/>
        <relevantInformation>https://aclanthology.org/sigs/sigmt/</relevantInformation>
        <relevantInformation>https://web.stanford.edu/~jurafsky/slp3/13.pdf</relevantInformation>
        <survey>https://aclanthology.org/2021.motra-1.3</survey>
        <survey>https://aclanthology.org/2021.tacl-1.51</survey>
        <survey>https://aclanthology.org/2022.cl-3.6</survey>
        <survey>https://aclanthology.org/2023.acl-long.36</survey>
        <survey>https://aclanthology.org/D13-1111</survey>
        <survey>https://aclanthology.org/P19-1164</survey>
        <survey>https://arxiv.org/abs/1605.04515</survey>
        <survey>https://arxiv.org/abs/1610.03934</survey>
        <survey>https://arxiv.org/abs/1711.09476</survey>
        <survey>https://arxiv.org/abs/1901.01122</survey>
        <survey>https://arxiv.org/abs/1910.03118</survey>
        <survey>https://arxiv.org/abs/1911.12798</survey>
        <survey>https://arxiv.org/abs/2008.01391</survey>
        <survey>https://arxiv.org/abs/2306.07198</survey>
        <nlp-taxonomy:level rdf:datatype="http://www.w3.org/2001/XMLSchema#integer">2</nlp-taxonomy:level>
        <dcterms:description xml:lang="en">Machine Translation is a subfield of Multilinguality and Text Generation that deals with developing algorithms and models for automatically translating text or speech from one language to another. It involves analyzing the input text or speech, generating a representation of its meaning in the source language, and then producing a new text or speech in the target language that conveys the same meaning.</dcterms:description>
        <oboInOwl:hasSynonym xml:lang="en">MT</oboInOwl:hasSynonym>
        <rdfs:label xml:lang="en">Machine Translation</rdfs:label>
    </owl:NamedIndividual>
    


    <!-- http://nlpkg.sebis.cit.tum.de/nlp-taxonomy.owl#Morphology -->

    <owl:NamedIndividual rdf:about="http://nlpkg.sebis.cit.tum.de/nlp-taxonomy.owl#Morphology">
        <rdf:type rdf:resource="http://nlpkg.sebis.cit.tum.de/nlp-fos-hierarchy.owl#OtherScientificField"/>
        <rdf:type rdf:resource="http://nlpkg.sebis.cit.tum.de/nlp-taxonomy.owl#FieldOfStudy"/>
        <nlp-taxonomy:subFieldOf rdf:resource="http://nlpkg.sebis.cit.tum.de/nlp-taxonomy.owl#Syntactic_Text_Processing"/>
        <nlp-taxonomy:superFieldOf rdf:resource="http://nlpkg.sebis.cit.tum.de/nlp-fos-hierarchy.owl#Lemmatization"/>
        <nlp-taxonomy:superFieldOf rdf:resource="http://nlpkg.sebis.cit.tum.de/nlp-fos-hierarchy.owl#Morphological_Inflection"/>
        <nlp-taxonomy:superFieldOf rdf:resource="http://nlpkg.sebis.cit.tum.de/nlp-fos-hierarchy.owl#Morphological_Segmentation"/>
        <nlp-taxonomy:superFieldOf rdf:resource="http://nlpkg.sebis.cit.tum.de/nlp-fos-hierarchy.owl#Stemming"/>
        <relevantInformation>https://aclanthology.org/sigs/sigmorphon/</relevantInformation>
        <nlp-taxonomy:level rdf:datatype="http://www.w3.org/2001/XMLSchema#integer">2</nlp-taxonomy:level>
        <dcterms:description xml:lang="en">Morphology is a subfield of Syntactic Text Processing that deals with studying the structure and formation of word as well as their relationship to other words in the same language. It analyzes the structure of words and parts of words such as stems, root words, prefixes, and suffixes. Morphology also looks at parts of speech, intonation and stress, and the ways context can change a word&apos;s pronunciation and meaning.</dcterms:description>
        <oboInOwl:hasSynonym xml:lang="en">Morphological Analysis</oboInOwl:hasSynonym>
        <rdfs:label xml:lang="en">Morphology</rdfs:label>
    </owl:NamedIndividual>
    


    <!-- http://nlpkg.sebis.cit.tum.de/nlp-taxonomy.owl#Multilinguality -->

    <owl:NamedIndividual rdf:about="http://nlpkg.sebis.cit.tum.de/nlp-taxonomy.owl#Multilinguality">
        <rdf:type rdf:resource="http://nlpkg.sebis.cit.tum.de/nlp-fos-hierarchy.owl#OtherScientificField"/>
        <rdf:type rdf:resource="http://nlpkg.sebis.cit.tum.de/nlp-taxonomy.owl#FieldOfStudy"/>
        <nlp-taxonomy:subFieldOf rdf:resource="http://nlpkg.sebis.cit.tum.de/nlp-taxonomy.owl#Natural_Language_Processing"/>
        <nlp-taxonomy:superFieldOf rdf:resource="http://nlpkg.sebis.cit.tum.de/nlp-fos-hierarchy.owl#Multilingual_Language_Models"/>
        <nlp-taxonomy:superFieldOf rdf:resource="http://nlpkg.sebis.cit.tum.de/nlp-taxonomy.owl#Code-Switching"/>
        <nlp-taxonomy:superFieldOf rdf:resource="http://nlpkg.sebis.cit.tum.de/nlp-taxonomy.owl#Cross-Lingual_Transfer"/>
        <nlp-taxonomy:superFieldOf rdf:resource="http://nlpkg.sebis.cit.tum.de/nlp-taxonomy.owl#Machine_Translation"/>
        <nlp-taxonomy:superFieldOf rdf:resource="http://nlpkg.sebis.cit.tum.de/nlp-taxonomy.owl#Typology"/>
        <survey>https://aclanthology.org/2022.findings-emnlp.273</survey>
        <survey>https://arxiv.org/abs/1401.2937</survey>
        <survey>https://arxiv.org/abs/2210.16960</survey>
        <nlp-taxonomy:level rdf:datatype="http://www.w3.org/2001/XMLSchema#integer">1</nlp-taxonomy:level>
        <dcterms:description xml:lang="en">Multilinguality is a subfield of Natural Language Processing (NLP) that refers to the ability of machines to understand, process, and generate natural language text in multiple languages. Multilinguality is concerned with addressing the challenges that arise due to the linguistic and structural variations that exist across different languages. This includes variations in word order, syntax, grammar, or vocabulary.</dcterms:description>
        <rdfs:label xml:lang="en">Multilinguality</rdfs:label>
    </owl:NamedIndividual>
    


    <!-- http://nlpkg.sebis.cit.tum.de/nlp-taxonomy.owl#Multimodality -->

    <owl:NamedIndividual rdf:about="http://nlpkg.sebis.cit.tum.de/nlp-taxonomy.owl#Multimodality">
        <rdf:type rdf:resource="http://nlpkg.sebis.cit.tum.de/nlp-fos-hierarchy.owl#OtherScientificField"/>
        <rdf:type rdf:resource="http://nlpkg.sebis.cit.tum.de/nlp-taxonomy.owl#FieldOfStudy"/>
        <nlp-taxonomy:subFieldOf rdf:resource="http://nlpkg.sebis.cit.tum.de/nlp-taxonomy.owl#Natural_Language_Processing"/>
        <nlp-taxonomy:superFieldOf rdf:resource="http://nlpkg.sebis.cit.tum.de/nlp-fos-hierarchy.owl#Language_Grounding"/>
        <nlp-taxonomy:superFieldOf rdf:resource="http://nlpkg.sebis.cit.tum.de/nlp-fos-hierarchy.owl#Multimodal_Language_Models"/>
        <nlp-taxonomy:superFieldOf rdf:resource="http://nlpkg.sebis.cit.tum.de/nlp-taxonomy.owl#Programming_Languages_In_NLP"/>
        <nlp-taxonomy:superFieldOf rdf:resource="http://nlpkg.sebis.cit.tum.de/nlp-taxonomy.owl#Structured_Data_In_NLP"/>
        <nlp-taxonomy:superFieldOf rdf:resource="http://nlpkg.sebis.cit.tum.de/nlp-taxonomy.owl#Visual_Data_In_NLP"/>
        <nlp-taxonomy:superFieldOf rdf:resource="http://nlpkg.sebis.cit.tum.de/nlp-taxonomy.owl#Speech_&amp;_Audio_In_NLP"/>
        <survey>https://aclanthology.org/2022.coling-1.576</survey>
        <survey>https://arxiv.org/abs/1607.06215</survey>
        <survey>https://arxiv.org/abs/1705.09406</survey>
        <survey>https://arxiv.org/abs/1911.03977</survey>
        <survey>https://arxiv.org/abs/1911.12798</survey>
        <survey>https://arxiv.org/abs/2105.11087</survey>
        <survey>https://arxiv.org/abs/2109.05199</survey>
        <survey>https://arxiv.org/abs/2202.05786</survey>
        <survey>https://arxiv.org/abs/2210.16960</survey>
        <survey>https://arxiv.org/abs/2304.01008</survey>
        <nlp-taxonomy:level rdf:datatype="http://www.w3.org/2001/XMLSchema#integer">1</nlp-taxonomy:level>
        <dcterms:description xml:lang="en">Multimodality is a subfield of Natural Language Processing (NLP) that refers to the capability of a system or method to process input of different types or “modalities”, such as natural language text, speech, audio, images, video, and programming languages in NLP applications. It involves developing algorithms and models that can process and analyze information from multiple modalities, and integrate them to form a unified representation of the input.</dcterms:description>
        <oboInOwl:hasSynonym xml:lang="en">Cross-Modality</oboInOwl:hasSynonym>
        <oboInOwl:hasSynonym xml:lang="en">Multi-Modality</oboInOwl:hasSynonym>
        <rdfs:label xml:lang="en">Multimodality</rdfs:label>
    </owl:NamedIndividual>
    


    <!-- http://nlpkg.sebis.cit.tum.de/nlp-taxonomy.owl#Named_Entity_Recognition -->

    <owl:NamedIndividual rdf:about="http://nlpkg.sebis.cit.tum.de/nlp-taxonomy.owl#Named_Entity_Recognition">
        <rdf:type rdf:resource="http://nlpkg.sebis.cit.tum.de/nlp-fos-hierarchy.owl#Task"/>
        <rdf:type rdf:resource="http://nlpkg.sebis.cit.tum.de/nlp-taxonomy.owl#FieldOfStudy"/>
        <usedFor rdf:resource="http://nlpkg.sebis.cit.tum.de/nlp-fos-hierarchy.owl#Dialogue_Understanding"/>
        <usedFor rdf:resource="http://nlpkg.sebis.cit.tum.de/nlp-fos-hierarchy.owl#Entity-Level_Sentiment_Analysis"/>
        <usedFor rdf:resource="http://nlpkg.sebis.cit.tum.de/nlp-fos-hierarchy.owl#Ontology_Learning"/>
        <usedFor rdf:resource="http://nlpkg.sebis.cit.tum.de/nlp-fos-hierarchy.owl#Taxonomy_Learning"/>
        <usedFor rdf:resource="http://nlpkg.sebis.cit.tum.de/nlp-fos-hierarchy.owl#Knowledge_Graph_Construction_&amp;_Completion"/>
        <usedFor rdf:resource="http://nlpkg.sebis.cit.tum.de/nlp-taxonomy.owl#Event_Extraction"/>
        <uses rdf:resource="http://nlpkg.sebis.cit.tum.de/nlp-fos-hierarchy.owl#Gazetteers"/>
        <uses rdf:resource="http://nlpkg.sebis.cit.tum.de/nlp-fos-hierarchy.owl#Sequence_Labeling"/>
        <uses rdf:resource="http://nlpkg.sebis.cit.tum.de/nlp-fos-hierarchy.owl#Span_Detection"/>
        <nlp-taxonomy:subFieldOf rdf:resource="http://nlpkg.sebis.cit.tum.de/nlp-taxonomy.owl#Knowledge_Graph_Reasoning"/>
        <nlp-taxonomy:subFieldOf rdf:resource="http://nlpkg.sebis.cit.tum.de/nlp-taxonomy.owl#Text_Classification"/>
        <nlp-taxonomy:subFieldOf rdf:resource="http://nlpkg.sebis.cit.tum.de/nlp-taxonomy.owl#Information_Extraction_&amp;_Text_Mining"/>
        <code>https://github.com/tomaarsen/SpanMarkerNER</code>
        <code>https://spacy.io/usage/linguistic-features#named-entities</code>
        <survey>https://aclanthology.org/C18-1182</survey>
        <survey>https://aclanthology.org/J14-2008</survey>
        <survey>https://aclanthology.org/W16-2703</survey>
        <survey>https://arxiv.org/abs/1407.2918</survey>
        <survey>https://arxiv.org/abs/1812.09449</survey>
        <survey>https://arxiv.org/abs/2103.06118</survey>
        <survey>https://arxiv.org/abs/2310.19055</survey>
        <nlp-taxonomy:level rdf:datatype="http://www.w3.org/2001/XMLSchema#integer">2</nlp-taxonomy:level>
        <nlp-taxonomy:level rdf:datatype="http://www.w3.org/2001/XMLSchema#integer">3</nlp-taxonomy:level>
        <nlp-taxonomy:level rdf:datatype="http://www.w3.org/2001/XMLSchema#integer">7</nlp-taxonomy:level>
        <dcterms:description xml:lang="en">Named Entity Recognition (NER) is a subfield of Information Extraction &amp; Text Mining that deals with identifying, extracting, and classifying named entities, such as people, organizations, and locations, in unstructured natural language texts.</dcterms:description>
        <oboInOwl:hasSynonym xml:lang="en">Entity Chunking</oboInOwl:hasSynonym>
        <oboInOwl:hasSynonym xml:lang="en">Entity Classification</oboInOwl:hasSynonym>
        <oboInOwl:hasSynonym xml:lang="en">Entity Detection</oboInOwl:hasSynonym>
        <oboInOwl:hasSynonym xml:lang="en">Entity Extraction</oboInOwl:hasSynonym>
        <oboInOwl:hasSynonym xml:lang="en">Entity Identification</oboInOwl:hasSynonym>
        <oboInOwl:hasSynonym xml:lang="en">Entity Type Classification</oboInOwl:hasSynonym>
        <oboInOwl:hasSynonym xml:lang="en">Entity Type Detection</oboInOwl:hasSynonym>
        <oboInOwl:hasSynonym xml:lang="en">Entity Type Identification</oboInOwl:hasSynonym>
        <oboInOwl:hasSynonym xml:lang="en">Entity Typing</oboInOwl:hasSynonym>
        <oboInOwl:hasSynonym xml:lang="en">NER</oboInOwl:hasSynonym>
        <oboInOwl:hasSynonym xml:lang="en">Named Entity Identification</oboInOwl:hasSynonym>
        <rdfs:label xml:lang="en">Named Entity Recognition</rdfs:label>
    </owl:NamedIndividual>
    


    <!-- http://nlpkg.sebis.cit.tum.de/nlp-taxonomy.owl#Natural_Language_Interfaces -->

    <owl:NamedIndividual rdf:about="http://nlpkg.sebis.cit.tum.de/nlp-taxonomy.owl#Natural_Language_Interfaces">
        <rdf:type rdf:resource="http://nlpkg.sebis.cit.tum.de/nlp-fos-hierarchy.owl#OtherScientificField"/>
        <rdf:type rdf:resource="http://nlpkg.sebis.cit.tum.de/nlp-taxonomy.owl#FieldOfStudy"/>
        <uses rdf:resource="http://nlpkg.sebis.cit.tum.de/nlp-taxonomy.owl#Text_Generation"/>
        <nlp-taxonomy:subFieldOf rdf:resource="http://nlpkg.sebis.cit.tum.de/nlp-taxonomy.owl#Natural_Language_Processing"/>
        <nlp-taxonomy:superFieldOf rdf:resource="http://nlpkg.sebis.cit.tum.de/nlp-taxonomy.owl#Question_Answering"/>
        <nlp-taxonomy:superFieldOf rdf:resource="http://nlpkg.sebis.cit.tum.de/nlp-taxonomy.owl#Dialogue_Systems_&amp;_Conversational_Agents"/>
        <survey>https://aclanthology.org/2020.coling-main.34</survey>
        <survey>https://arxiv.org/abs/1906.08990</survey>
        <nlp-taxonomy:level rdf:datatype="http://www.w3.org/2001/XMLSchema#integer">1</nlp-taxonomy:level>
        <dcterms:description xml:lang="en">Natural Language Interfaces is a subfield of Natural Language Processing (NLP) that deals with the development of interfaces that enable humans to interact with computers using natural language. It involves developing algorithms and models that can understand and interpret human language and generate appropriate responses.</dcterms:description>
        <rdfs:label xml:lang="en">Natural Language Interfaces</rdfs:label>
    </owl:NamedIndividual>
    


    <!-- http://nlpkg.sebis.cit.tum.de/nlp-taxonomy.owl#Natural_Language_Processing -->

    <owl:NamedIndividual rdf:about="http://nlpkg.sebis.cit.tum.de/nlp-taxonomy.owl#Natural_Language_Processing">
        <rdf:type rdf:resource="http://nlpkg.sebis.cit.tum.de/nlp-fos-hierarchy.owl#OtherScientificField"/>
        <rdf:type rdf:resource="http://nlpkg.sebis.cit.tum.de/nlp-taxonomy.owl#FieldOfStudy"/>
        <nlp-taxonomy:superFieldOf rdf:resource="http://nlpkg.sebis.cit.tum.de/nlp-fos-hierarchy.owl#Evaluation"/>
        <nlp-taxonomy:superFieldOf rdf:resource="http://nlpkg.sebis.cit.tum.de/nlp-taxonomy.owl#Information_Retrieval"/>
        <nlp-taxonomy:superFieldOf rdf:resource="http://nlpkg.sebis.cit.tum.de/nlp-taxonomy.owl#Multilinguality"/>
        <nlp-taxonomy:superFieldOf rdf:resource="http://nlpkg.sebis.cit.tum.de/nlp-taxonomy.owl#Multimodality"/>
        <nlp-taxonomy:superFieldOf rdf:resource="http://nlpkg.sebis.cit.tum.de/nlp-taxonomy.owl#Natural_Language_Interfaces"/>
        <nlp-taxonomy:superFieldOf rdf:resource="http://nlpkg.sebis.cit.tum.de/nlp-taxonomy.owl#Reasoning"/>
        <nlp-taxonomy:superFieldOf rdf:resource="http://nlpkg.sebis.cit.tum.de/nlp-taxonomy.owl#Semantic_Text_Processing"/>
        <nlp-taxonomy:superFieldOf rdf:resource="http://nlpkg.sebis.cit.tum.de/nlp-taxonomy.owl#Sentiment_Analysis"/>
        <nlp-taxonomy:superFieldOf rdf:resource="http://nlpkg.sebis.cit.tum.de/nlp-taxonomy.owl#Syntactic_Text_Processing"/>
        <nlp-taxonomy:superFieldOf rdf:resource="http://nlpkg.sebis.cit.tum.de/nlp-taxonomy.owl#Text_Generation"/>
        <nlp-taxonomy:superFieldOf rdf:resource="http://nlpkg.sebis.cit.tum.de/nlp-taxonomy.owl#Information_Extraction_&amp;_Text_Mining"/>
        <nlp-taxonomy:superFieldOf rdf:resource="http://nlpkg.sebis.cit.tum.de/nlp-taxonomy.owl#Linguistics_&amp;_Cognitive_NLP"/>
        <nlp-taxonomy:superFieldOf rdf:resource="http://nlpkg.sebis.cit.tum.de/nlp-taxonomy.owl#Responsible_&amp;_Trustworthy_NLP"/>
        <relevantInformation>https://web.stanford.edu/~jurafsky/slp3/</relevantInformation>
        <survey>https://aclanthology.org/2023.ranlp-1.111</survey>
        <survey>https://aclanthology.org/L14-1511</survey>
        <survey>https://aclanthology.org/W12-3202</survey>
        <survey>https://arxiv.org/abs/2210.03050</survey>
        <survey>https://arxiv.org/abs/2305.12920</survey>
        <nlp-taxonomy:level rdf:datatype="http://www.w3.org/2001/XMLSchema#integer">0</nlp-taxonomy:level>
        <dcterms:description xml:lang="en">Natural Language Processing (NLP) is an interdisciplinary subfield of linguistics, computer science, and artificial intelligence concerned with the interactions between computers and human language, in particular how to program computers to process and analyze large amounts of natural language data. The goal is a computer capable of &apos;understanding&apos; the contents of documents, including the contextual nuances of the language within them. The technology can then accurately extract information and insights contained in the documents as well as categorize and organize the documents themselves.</dcterms:description>
        <oboInOwl:hasSynonym xml:lang="en">NLP</oboInOwl:hasSynonym>
        <oboInOwl:hasSynonym xml:lang="en">NLProc</oboInOwl:hasSynonym>
        <rdfs:label xml:lang="en">Natural Language Processing</rdfs:label>
    </owl:NamedIndividual>
    


    <!-- http://nlpkg.sebis.cit.tum.de/nlp-taxonomy.owl#Numerical_Reasoning -->

    <owl:NamedIndividual rdf:about="http://nlpkg.sebis.cit.tum.de/nlp-taxonomy.owl#Numerical_Reasoning">
        <rdf:type rdf:resource="http://nlpkg.sebis.cit.tum.de/nlp-fos-hierarchy.owl#Task"/>
        <rdf:type rdf:resource="http://nlpkg.sebis.cit.tum.de/nlp-taxonomy.owl#FieldOfStudy"/>
        <nlp-taxonomy:subFieldOf rdf:resource="http://nlpkg.sebis.cit.tum.de/nlp-taxonomy.owl#Reasoning"/>
        <nlp-taxonomy:superFieldOf rdf:resource="http://nlpkg.sebis.cit.tum.de/nlp-fos-hierarchy.owl#Math_Word_Problem_Solving"/>
        <relevantInformation>https://aclanthology.org/2021.mol-1</relevantInformation>
        <survey>https://aclanthology.org/2021.naacl-main.53</survey>
        <survey>https://aclanthology.org/2023.acl-long.817</survey>
        <survey>https://aclanthology.org/P18-1196</survey>
        <survey>https://aclanthology.org/P19-1329</survey>
        <survey>https://arxiv.org/abs/2205.15231</survey>
        <survey>https://arxiv.org/abs/2311.02216</survey>
        <survey>https://arxiv.org/abs/2312.07622</survey>
        <nlp-taxonomy:level rdf:datatype="http://www.w3.org/2001/XMLSchema#integer">2</nlp-taxonomy:level>
        <dcterms:description xml:lang="en">Numerical Reasoning is a subfield of Reasoning that is concerned with understanding and processing numerical data. It involves performing arithmetic operations such as addition, subtraction, sorting, and counting.</dcterms:description>
        <oboInOwl:hasSynonym xml:lang="en">Mathematical Reasoning</oboInOwl:hasSynonym>
        <oboInOwl:hasSynonym xml:lang="en">Numeracy</oboInOwl:hasSynonym>
        <rdfs:label xml:lang="en">Numerical Reasoning</rdfs:label>
    </owl:NamedIndividual>
    


    <!-- http://nlpkg.sebis.cit.tum.de/nlp-taxonomy.owl#Open_Information_Extraction -->

    <owl:NamedIndividual rdf:about="http://nlpkg.sebis.cit.tum.de/nlp-taxonomy.owl#Open_Information_Extraction">
        <rdf:type rdf:resource="http://nlpkg.sebis.cit.tum.de/nlp-fos-hierarchy.owl#Task"/>
        <rdf:type rdf:resource="http://nlpkg.sebis.cit.tum.de/nlp-taxonomy.owl#FieldOfStudy"/>
        <nlp-taxonomy:subFieldOf rdf:resource="http://nlpkg.sebis.cit.tum.de/nlp-taxonomy.owl#Information_Extraction_&amp;_Text_Mining"/>
        <survey>https://aclanthology.org/C18-1326/</survey>
        <survey>https://arxiv.org/abs/2205.11725</survey>
        <survey>https://arxiv.org/abs/2208.08690</survey>
        <nlp-taxonomy:level rdf:datatype="http://www.w3.org/2001/XMLSchema#integer">2</nlp-taxonomy:level>
        <dcterms:description xml:lang="en">Open Information Extraction is a subfield of Information Extraction &amp; Text Mining that deals with the extraction of structured factual information from natural language text, usually in the form of triples or n-ary propositions, without relying on predefined schemas or templates.</dcterms:description>
        <oboInOwl:hasSynonym xml:lang="en">OIE</oboInOwl:hasSynonym>
        <rdfs:label xml:lang="en">Open Information Extraction</rdfs:label>
    </owl:NamedIndividual>
    


    <!-- http://nlpkg.sebis.cit.tum.de/nlp-taxonomy.owl#Opinion_Mining -->

    <owl:NamedIndividual rdf:about="http://nlpkg.sebis.cit.tum.de/nlp-taxonomy.owl#Opinion_Mining">
        <rdf:type rdf:resource="http://nlpkg.sebis.cit.tum.de/nlp-fos-hierarchy.owl#Task"/>
        <rdf:type rdf:resource="http://nlpkg.sebis.cit.tum.de/nlp-taxonomy.owl#FieldOfStudy"/>
        <uses rdf:resource="http://nlpkg.sebis.cit.tum.de/nlp-taxonomy.owl#Polarity_Analysis"/>
        <nlp-taxonomy:subFieldOf rdf:resource="http://nlpkg.sebis.cit.tum.de/nlp-taxonomy.owl#Sentiment_Analysis"/>
        <nlp-taxonomy:superFieldOf rdf:resource="http://nlpkg.sebis.cit.tum.de/nlp-fos-hierarchy.owl#Stance_Detection"/>
        <survey>https://arxiv.org/abs/1307.3336</survey>
        <survey>https://arxiv.org/abs/1712.08941</survey>
        <survey>https://arxiv.org/abs/2005.01897</survey>
        <survey>https://arxiv.org/abs/2012.03091</survey>
        <survey>https://arxiv.org/abs/2305.09620</survey>
        <nlp-taxonomy:level rdf:datatype="http://www.w3.org/2001/XMLSchema#integer">2</nlp-taxonomy:level>
        <dcterms:description xml:lang="en">Opinion Mining is a subfield of Sentiment Analysis that deals with the automatic extraction and analysis of opinions, attitudes, and positions regarding a particular topic expressed in natural language texts.</dcterms:description>
        <oboInOwl:hasSynonym xml:lang="en">Opinion Classification</oboInOwl:hasSynonym>
        <oboInOwl:hasSynonym xml:lang="en">Opinion Detection</oboInOwl:hasSynonym>
        <oboInOwl:hasSynonym xml:lang="en">Opinion Identification</oboInOwl:hasSynonym>
        <oboInOwl:hasSynonym xml:lang="en">Opinion Prediction</oboInOwl:hasSynonym>
        <rdfs:label xml:lang="en">Opinion Mining</rdfs:label>
    </owl:NamedIndividual>
    


    <!-- http://nlpkg.sebis.cit.tum.de/nlp-taxonomy.owl#Paraphrasing -->

    <owl:NamedIndividual rdf:about="http://nlpkg.sebis.cit.tum.de/nlp-taxonomy.owl#Paraphrasing">
        <rdf:type rdf:resource="http://nlpkg.sebis.cit.tum.de/nlp-fos-hierarchy.owl#Task"/>
        <rdf:type rdf:resource="http://nlpkg.sebis.cit.tum.de/nlp-taxonomy.owl#FieldOfStudy"/>
        <uses rdf:resource="http://nlpkg.sebis.cit.tum.de/nlp-fos-hierarchy.owl#Controllable_Text_Generation"/>
        <nlp-taxonomy:subFieldOf rdf:resource="http://nlpkg.sebis.cit.tum.de/nlp-taxonomy.owl#Text_Generation"/>
        <nlp-taxonomy:superFieldOf rdf:resource="http://nlpkg.sebis.cit.tum.de/nlp-fos-hierarchy.owl#Text_Simplification"/>
        <survey>https://aclanthology.org/2021.emnlp-main.414</survey>
        <survey>https://arxiv.org/abs/0912.3747</survey>
        <nlp-taxonomy:level rdf:datatype="http://www.w3.org/2001/XMLSchema#integer">2</nlp-taxonomy:level>
        <dcterms:description xml:lang="en">Paraphrasing is a subfield of Text Generation that deals with the automatic generation of natural language text that expresses the same semantic meaning as a given input text, but using different words or syntactic structures. The goal of paraphrasing is to retain the original meaning while avoiding plagiarism, simplifying complex sentences, or adapting the language to a different audience.</dcterms:description>
        <oboInOwl:hasSynonym xml:lang="en">Paraphrase Generation</oboInOwl:hasSynonym>
        <rdfs:label xml:lang="en">Paraphrasing</rdfs:label>
    </owl:NamedIndividual>
    


    <!-- http://nlpkg.sebis.cit.tum.de/nlp-taxonomy.owl#Passage_Retrieval -->

    <owl:NamedIndividual rdf:about="http://nlpkg.sebis.cit.tum.de/nlp-taxonomy.owl#Passage_Retrieval">
        <rdf:type rdf:resource="http://nlpkg.sebis.cit.tum.de/nlp-fos-hierarchy.owl#Task"/>
        <rdf:type rdf:resource="http://nlpkg.sebis.cit.tum.de/nlp-taxonomy.owl#FieldOfStudy"/>
        <usedFor rdf:resource="http://nlpkg.sebis.cit.tum.de/nlp-fos-hierarchy.owl#Retrieval_Augmented_Generation"/>
        <usedFor rdf:resource="http://nlpkg.sebis.cit.tum.de/nlp-taxonomy.owl#Question_Answering"/>
        <usedFor rdf:resource="http://nlpkg.sebis.cit.tum.de/nlp-taxonomy.owl#Semantic_Search"/>
        <uses rdf:resource="http://nlpkg.sebis.cit.tum.de/nlp-taxonomy.owl#Semantic_Similarity"/>
        <uses rdf:resource="http://nlpkg.sebis.cit.tum.de/nlp-taxonomy.owl#Text_Segmentation"/>
        <nlp-taxonomy:subFieldOf rdf:resource="http://nlpkg.sebis.cit.tum.de/nlp-taxonomy.owl#Information_Retrieval"/>
        <nlp-taxonomy:superFieldOf rdf:resource="http://nlpkg.sebis.cit.tum.de/nlp-fos-hierarchy.owl#Dense_Passage_Retrieval"/>
        <nlp-taxonomy:superFieldOf rdf:resource="http://nlpkg.sebis.cit.tum.de/nlp-fos-hierarchy.owl#Query_Representation"/>
        <nlp-taxonomy:superFieldOf rdf:resource="http://nlpkg.sebis.cit.tum.de/nlp-fos-hierarchy.owl#Sparse_Passage_Retrieval"/>
        <survey>https://arxiv.org/abs/2010.06467</survey>
        <nlp-taxonomy:level rdf:datatype="http://www.w3.org/2001/XMLSchema#integer">2</nlp-taxonomy:level>
        <dcterms:description xml:lang="en">Passage Retrieval is a subfield of Information Retrieval that deals with retrieving relevant passages or snippets of text from a larger document or corpus in response to a user query. It involves developing algorithms and models that can identify and extract the most relevant and informative passages, and rank them based on their relevance and similarity to the query.</dcterms:description>
        <rdfs:label xml:lang="en">Passage Retrieval</rdfs:label>
    </owl:NamedIndividual>
    


    <!-- http://nlpkg.sebis.cit.tum.de/nlp-taxonomy.owl#Phonetics -->

    <owl:NamedIndividual rdf:about="http://nlpkg.sebis.cit.tum.de/nlp-taxonomy.owl#Phonetics">
        <rdf:type rdf:resource="http://nlpkg.sebis.cit.tum.de/nlp-fos-hierarchy.owl#OtherScientificField"/>
        <rdf:type rdf:resource="http://nlpkg.sebis.cit.tum.de/nlp-taxonomy.owl#FieldOfStudy"/>
        <nlp-taxonomy:subFieldOf rdf:resource="http://nlpkg.sebis.cit.tum.de/nlp-taxonomy.owl#Syntactic_Text_Processing"/>
        <relevantInformation>https://web.stanford.edu/~jurafsky/slp3/28.pdf</relevantInformation>
        <nlp-taxonomy:level rdf:datatype="http://www.w3.org/2001/XMLSchema#integer">2</nlp-taxonomy:level>
        <dcterms:description xml:lang="en">Phonetics is a subfield of Syntactic Text Processing that studies how humans produce and perceive sounds, or in the case of sign languages, the equivalent aspects of sign.</dcterms:description>
        <rdfs:label xml:lang="en">Phonetics</rdfs:label>
    </owl:NamedIndividual>
    


    <!-- http://nlpkg.sebis.cit.tum.de/nlp-taxonomy.owl#Phonology -->

    <owl:NamedIndividual rdf:about="http://nlpkg.sebis.cit.tum.de/nlp-taxonomy.owl#Phonology">
        <rdf:type rdf:resource="http://nlpkg.sebis.cit.tum.de/nlp-fos-hierarchy.owl#OtherScientificField"/>
        <rdf:type rdf:resource="http://nlpkg.sebis.cit.tum.de/nlp-taxonomy.owl#FieldOfStudy"/>
        <nlp-taxonomy:subFieldOf rdf:resource="http://nlpkg.sebis.cit.tum.de/nlp-taxonomy.owl#Syntactic_Text_Processing"/>
        <relevantInformation>https://aclanthology.org/sigs/sigmorphon/</relevantInformation>
        <nlp-taxonomy:level rdf:datatype="http://www.w3.org/2001/XMLSchema#integer">2</nlp-taxonomy:level>
        <dcterms:description xml:lang="en">Phonology is a subfield of Syntactic Text Processing that studies the sound of languages or dialects and the patterns and rules that govern the use and combination of sounds to form meaningful units. It involves the analysis of phonemes, prosody, and intonation of speech, and the development of models and theories that can explain and predict the behavior and variability of sounds in different contexts.</dcterms:description>
        <rdfs:label xml:lang="en">Phonology</rdfs:label>
    </owl:NamedIndividual>
    


    <!-- http://nlpkg.sebis.cit.tum.de/nlp-taxonomy.owl#Polarity_Analysis -->

    <owl:NamedIndividual rdf:about="http://nlpkg.sebis.cit.tum.de/nlp-taxonomy.owl#Polarity_Analysis">
        <rdf:type rdf:resource="http://nlpkg.sebis.cit.tum.de/nlp-fos-hierarchy.owl#Task"/>
        <rdf:type rdf:resource="http://nlpkg.sebis.cit.tum.de/nlp-taxonomy.owl#FieldOfStudy"/>
        <usedFor rdf:resource="http://nlpkg.sebis.cit.tum.de/nlp-taxonomy.owl#Opinion_Mining"/>
        <nlp-taxonomy:subFieldOf rdf:resource="http://nlpkg.sebis.cit.tum.de/nlp-taxonomy.owl#Sentiment_Analysis"/>
        <nlp-taxonomy:level rdf:datatype="http://www.w3.org/2001/XMLSchema#integer">2</nlp-taxonomy:level>
        <dcterms:description xml:lang="en">Polarity Analysis is a subfield of Sentiment Analysis that deals with automatically detecting and classifying the polarity or valence of a given natural language text, such as positive, negative, or neutral.</dcterms:description>
        <oboInOwl:hasSynonym xml:lang="en">Sentiment Polarity Analysis</oboInOwl:hasSynonym>
        <rdfs:label xml:lang="en">Polarity Analysis</rdfs:label>
    </owl:NamedIndividual>
    


    <!-- http://nlpkg.sebis.cit.tum.de/nlp-taxonomy.owl#Programming_Languages_In_NLP -->

    <owl:NamedIndividual rdf:about="http://nlpkg.sebis.cit.tum.de/nlp-taxonomy.owl#Programming_Languages_In_NLP">
        <rdf:type rdf:resource="http://nlpkg.sebis.cit.tum.de/nlp-fos-hierarchy.owl#OtherScientificField"/>
        <rdf:type rdf:resource="http://nlpkg.sebis.cit.tum.de/nlp-taxonomy.owl#FieldOfStudy"/>
        <usedFor rdf:resource="http://nlpkg.sebis.cit.tum.de/nlp-fos-hierarchy.owl#Language_Grounding"/>
        <nlp-taxonomy:subFieldOf rdf:resource="http://nlpkg.sebis.cit.tum.de/nlp-taxonomy.owl#Multimodality"/>
        <nlp-taxonomy:superFieldOf rdf:resource="http://nlpkg.sebis.cit.tum.de/nlp-fos-hierarchy.owl#Code-specific_Language_Models"/>
        <nlp-taxonomy:superFieldOf rdf:resource="http://nlpkg.sebis.cit.tum.de/nlp-fos-hierarchy.owl#Code_Search"/>
        <nlp-taxonomy:superFieldOf rdf:resource="http://nlpkg.sebis.cit.tum.de/nlp-fos-hierarchy.owl#Code_Summarization"/>
        <nlp-taxonomy:superFieldOf rdf:resource="http://nlpkg.sebis.cit.tum.de/nlp-taxonomy.owl#Code_Generation"/>
        <survey>https://arxiv.org/abs/2202.04847</survey>
        <survey>https://arxiv.org/abs/2212.05773</survey>
        <nlp-taxonomy:level rdf:datatype="http://www.w3.org/2001/XMLSchema#integer">2</nlp-taxonomy:level>
        <dcterms:description xml:lang="en">Programming Languages in NLP is a subfield of Multimodality that deals with the processing of programming languages and code in conjunction with natural language texts.</dcterms:description>
        <rdfs:label xml:lang="en">Programming Languages in NLP</rdfs:label>
    </owl:NamedIndividual>
    


    <!-- http://nlpkg.sebis.cit.tum.de/nlp-taxonomy.owl#Psycholinguistics -->

    <owl:NamedIndividual rdf:about="http://nlpkg.sebis.cit.tum.de/nlp-taxonomy.owl#Psycholinguistics">
        <rdf:type rdf:resource="http://nlpkg.sebis.cit.tum.de/nlp-fos-hierarchy.owl#OtherScientificField"/>
        <rdf:type rdf:resource="http://nlpkg.sebis.cit.tum.de/nlp-taxonomy.owl#FieldOfStudy"/>
        <nlp-taxonomy:subFieldOf rdf:resource="http://nlpkg.sebis.cit.tum.de/nlp-taxonomy.owl#Linguistics_&amp;_Cognitive_NLP"/>
        <nlp-taxonomy:level rdf:datatype="http://www.w3.org/2001/XMLSchema#integer">2</nlp-taxonomy:level>
        <dcterms:description xml:lang="en">Psycholinguistics is a subfield of Linguistics &amp; Cognitive NLP  that studies the psychological and neural processes which enable humans to understand and use language.</dcterms:description>
        <rdfs:label xml:lang="en">Psycholinguistics</rdfs:label>
    </owl:NamedIndividual>
    


    <!-- http://nlpkg.sebis.cit.tum.de/nlp-taxonomy.owl#Question_Answering -->

    <owl:NamedIndividual rdf:about="http://nlpkg.sebis.cit.tum.de/nlp-taxonomy.owl#Question_Answering">
        <rdf:type rdf:resource="http://nlpkg.sebis.cit.tum.de/nlp-fos-hierarchy.owl#Task"/>
        <rdf:type rdf:resource="http://nlpkg.sebis.cit.tum.de/nlp-taxonomy.owl#FieldOfStudy"/>
        <uses rdf:resource="http://nlpkg.sebis.cit.tum.de/nlp-taxonomy.owl#Machine_Reading_Comprehension"/>
        <uses rdf:resource="http://nlpkg.sebis.cit.tum.de/nlp-taxonomy.owl#Passage_Retrieval"/>
        <nlp-taxonomy:subFieldOf rdf:resource="http://nlpkg.sebis.cit.tum.de/nlp-taxonomy.owl#Natural_Language_Interfaces"/>
        <nlp-taxonomy:subFieldOf rdf:resource="http://nlpkg.sebis.cit.tum.de/nlp-taxonomy.owl#Text_Generation"/>
        <nlp-taxonomy:superFieldOf rdf:resource="http://nlpkg.sebis.cit.tum.de/nlp-fos-hierarchy.owl#Closed_Book_Question_Answering"/>
        <nlp-taxonomy:superFieldOf rdf:resource="http://nlpkg.sebis.cit.tum.de/nlp-fos-hierarchy.owl#Closed_Domain_Question_Answering"/>
        <nlp-taxonomy:superFieldOf rdf:resource="http://nlpkg.sebis.cit.tum.de/nlp-fos-hierarchy.owl#Commonsense_Question_Answering"/>
        <nlp-taxonomy:superFieldOf rdf:resource="http://nlpkg.sebis.cit.tum.de/nlp-fos-hierarchy.owl#Conversational_Question_Answering"/>
        <nlp-taxonomy:superFieldOf rdf:resource="http://nlpkg.sebis.cit.tum.de/nlp-fos-hierarchy.owl#Extractive_Question_Answering"/>
        <nlp-taxonomy:superFieldOf rdf:resource="http://nlpkg.sebis.cit.tum.de/nlp-fos-hierarchy.owl#Generative_Question_Answering"/>
        <nlp-taxonomy:superFieldOf rdf:resource="http://nlpkg.sebis.cit.tum.de/nlp-fos-hierarchy.owl#Knowledge_Base_Question_Answering"/>
        <nlp-taxonomy:superFieldOf rdf:resource="http://nlpkg.sebis.cit.tum.de/nlp-fos-hierarchy.owl#Open_Book_Question_Answering"/>
        <nlp-taxonomy:superFieldOf rdf:resource="http://nlpkg.sebis.cit.tum.de/nlp-fos-hierarchy.owl#Open_Domain_Question_Answering"/>
        <nlp-taxonomy:superFieldOf rdf:resource="http://nlpkg.sebis.cit.tum.de/nlp-fos-hierarchy.owl#Question_Classification"/>
        <nlp-taxonomy:superFieldOf rdf:resource="http://nlpkg.sebis.cit.tum.de/nlp-fos-hierarchy.owl#Retrieval-based_Question_Answering"/>
        <nlp-taxonomy:superFieldOf rdf:resource="http://nlpkg.sebis.cit.tum.de/nlp-fos-hierarchy.owl#Visual_Question_Answering"/>
        <survey>https://aclanthology.org/2022.findings-emnlp.441</survey>
        <survey>https://arxiv.org/abs/1904.05276</survey>
        <survey>https://arxiv.org/abs/1911.04879</survey>
        <survey>https://arxiv.org/abs/2002.06612</survey>
        <survey>https://arxiv.org/abs/2109.12264</survey>
        <survey>https://arxiv.org/abs/2112.03572</survey>
        <survey>https://arxiv.org/abs/2112.13634</survey>
        <survey>https://arxiv.org/abs/2204.09140</survey>
        <survey>https://arxiv.org/abs/2206.15030</survey>
        <survey>https://arxiv.org/abs/2209.01621</survey>
        <survey>https://arxiv.org/abs/2302.09051</survey>
        <survey>https://arxiv.org/abs/2310.07225</survey>
        <nlp-taxonomy:level rdf:datatype="http://www.w3.org/2001/XMLSchema#integer">2</nlp-taxonomy:level>
        <dcterms:description xml:lang="en">Question Answering is a subfield of Natural Language Interfaces that deals with the development of computer systems that can answer questions posed by humans in natural language. It involves the development of algorithms and models that can understand and interpret the meaning and intent of a question, retrieve relevant information from a knowledge base or document corpus, and generate a concise and accurate answer.</dcterms:description>
        <oboInOwl:hasSynonym xml:lang="en">Language Based QA</oboInOwl:hasSynonym>
        <oboInOwl:hasSynonym xml:lang="en">NLQA</oboInOwl:hasSynonym>
        <oboInOwl:hasSynonym xml:lang="en">QA</oboInOwl:hasSynonym>
        <rdfs:label xml:lang="en">Question Answering</rdfs:label>
    </owl:NamedIndividual>
    


    <!-- http://nlpkg.sebis.cit.tum.de/nlp-taxonomy.owl#Question_Generation -->

    <owl:NamedIndividual rdf:about="http://nlpkg.sebis.cit.tum.de/nlp-taxonomy.owl#Question_Generation">
        <rdf:type rdf:resource="http://nlpkg.sebis.cit.tum.de/nlp-fos-hierarchy.owl#Task"/>
        <rdf:type rdf:resource="http://nlpkg.sebis.cit.tum.de/nlp-taxonomy.owl#FieldOfStudy"/>
        <nlp-taxonomy:subFieldOf rdf:resource="http://nlpkg.sebis.cit.tum.de/nlp-taxonomy.owl#Text_Generation"/>
        <survey>https://arxiv.org/abs/1905.08949</survey>
        <nlp-taxonomy:level rdf:datatype="http://www.w3.org/2001/XMLSchema#integer">2</nlp-taxonomy:level>
        <dcterms:description xml:lang="en">Question Generation is a subfield of Text Generation that deals with the automatic generation of valid and fluent natural language questions based on given passages and target answers.</dcterms:description>
        <rdfs:label xml:lang="en">Question Generation</rdfs:label>
    </owl:NamedIndividual>
    


    <!-- http://nlpkg.sebis.cit.tum.de/nlp-taxonomy.owl#Reasoning -->

    <owl:NamedIndividual rdf:about="http://nlpkg.sebis.cit.tum.de/nlp-taxonomy.owl#Reasoning">
        <rdf:type rdf:resource="http://nlpkg.sebis.cit.tum.de/nlp-fos-hierarchy.owl#Task"/>
        <rdf:type rdf:resource="http://nlpkg.sebis.cit.tum.de/nlp-taxonomy.owl#FieldOfStudy"/>
        <nlp-taxonomy:subFieldOf rdf:resource="http://nlpkg.sebis.cit.tum.de/nlp-taxonomy.owl#Natural_Language_Processing"/>
        <nlp-taxonomy:superFieldOf rdf:resource="http://nlpkg.sebis.cit.tum.de/nlp-fos-hierarchy.owl#Analogical_Reasoning"/>
        <nlp-taxonomy:superFieldOf rdf:resource="http://nlpkg.sebis.cit.tum.de/nlp-fos-hierarchy.owl#Multi-Hop_Reasoning"/>
        <nlp-taxonomy:superFieldOf rdf:resource="http://nlpkg.sebis.cit.tum.de/nlp-fos-hierarchy.owl#One-Hop_Reasoning"/>
        <nlp-taxonomy:superFieldOf rdf:resource="http://nlpkg.sebis.cit.tum.de/nlp-fos-hierarchy.owl#Visual_Reasoning"/>
        <nlp-taxonomy:superFieldOf rdf:resource="http://nlpkg.sebis.cit.tum.de/nlp-taxonomy.owl#Argument_Mining"/>
        <nlp-taxonomy:superFieldOf rdf:resource="http://nlpkg.sebis.cit.tum.de/nlp-taxonomy.owl#Commonsense_Reasoning"/>
        <nlp-taxonomy:superFieldOf rdf:resource="http://nlpkg.sebis.cit.tum.de/nlp-taxonomy.owl#Knowledge_Graph_Reasoning"/>
        <nlp-taxonomy:superFieldOf rdf:resource="http://nlpkg.sebis.cit.tum.de/nlp-taxonomy.owl#Machine_Reading_Comprehension"/>
        <nlp-taxonomy:superFieldOf rdf:resource="http://nlpkg.sebis.cit.tum.de/nlp-taxonomy.owl#Numerical_Reasoning"/>
        <nlp-taxonomy:superFieldOf rdf:resource="http://nlpkg.sebis.cit.tum.de/nlp-taxonomy.owl#Textual_Inference"/>
        <nlp-taxonomy:superFieldOf rdf:resource="http://nlpkg.sebis.cit.tum.de/nlp-taxonomy.owl#Fact_&amp;_Claim_Verification"/>
        <relevantInformation>https://github.com/FreedomIntelligence/ReasoningNLP</relevantInformation>
        <relevantInformation>https://github.com/jeffhj/LM-reasoning</relevantInformation>
        <relevantInformation>https://github.com/zjunlp/Prompt4ReasoningPapers</relevantInformation>
        <survey>https://aclanthology.org/2023.acl-long.294</survey>
        <survey>https://aclanthology.org/2023.findings-acl.67</survey>
        <survey>https://arxiv.org/abs/2202.12205</survey>
        <survey>https://arxiv.org/abs/2207.07568</survey>
        <survey>https://arxiv.org/abs/2302.02093</survey>
        <survey>https://arxiv.org/abs/2303.12023</survey>
        <survey>https://arxiv.org/abs/2303.14725</survey>
        <survey>https://arxiv.org/abs/2310.00836</survey>
        <nlp-taxonomy:level rdf:datatype="http://www.w3.org/2001/XMLSchema#integer">1</nlp-taxonomy:level>
        <dcterms:description xml:lang="en">Reasoning is a subfield of Natural Language Processing (NLP) that enables machines to draw logical conclusions and derive new knowledge from natural language texts based on the information available to them, using techniques such as deduction and induction.</dcterms:description>
        <rdfs:label xml:lang="en">Reasoning</rdfs:label>
    </owl:NamedIndividual>
    


    <!-- http://nlpkg.sebis.cit.tum.de/nlp-taxonomy.owl#Relation_Extraction -->

    <owl:NamedIndividual rdf:about="http://nlpkg.sebis.cit.tum.de/nlp-taxonomy.owl#Relation_Extraction">
        <rdf:type rdf:resource="http://nlpkg.sebis.cit.tum.de/nlp-fos-hierarchy.owl#Task"/>
        <rdf:type rdf:resource="http://nlpkg.sebis.cit.tum.de/nlp-taxonomy.owl#FieldOfStudy"/>
        <usedFor rdf:resource="http://nlpkg.sebis.cit.tum.de/nlp-fos-hierarchy.owl#Discourse_Parsing"/>
        <usedFor rdf:resource="http://nlpkg.sebis.cit.tum.de/nlp-fos-hierarchy.owl#Ontology_Learning"/>
        <usedFor rdf:resource="http://nlpkg.sebis.cit.tum.de/nlp-fos-hierarchy.owl#Taxonomy_Learning"/>
        <usedFor rdf:resource="http://nlpkg.sebis.cit.tum.de/nlp-fos-hierarchy.owl#Knowledge_Graph_Construction_&amp;_Completion"/>
        <usedFor rdf:resource="http://nlpkg.sebis.cit.tum.de/nlp-taxonomy.owl#Event_Extraction"/>
        <uses rdf:resource="http://nlpkg.sebis.cit.tum.de/nlp-fos-hierarchy.owl#Distant_Supervision"/>
        <nlp-taxonomy:subFieldOf rdf:resource="http://nlpkg.sebis.cit.tum.de/nlp-taxonomy.owl#Knowledge_Graph_Reasoning"/>
        <nlp-taxonomy:subFieldOf rdf:resource="http://nlpkg.sebis.cit.tum.de/nlp-taxonomy.owl#Information_Extraction_&amp;_Text_Mining"/>
        <nlp-taxonomy:superFieldOf rdf:resource="http://nlpkg.sebis.cit.tum.de/nlp-fos-hierarchy.owl#Discourse_Relation_Recognition"/>
        <nlp-taxonomy:superFieldOf rdf:resource="http://nlpkg.sebis.cit.tum.de/nlp-fos-hierarchy.owl#Relation_Directionality_Classification"/>
        <relevantInformation>https://web.stanford.edu/~jurafsky/slp3/21.pdf</relevantInformation>
        <survey>https://aclanthology.org/2020.aacl-main.75</survey>
        <survey>https://aclanthology.org/2021.findings-acl.112</survey>
        <survey>https://aclanthology.org/2022.acl-srw.7</survey>
        <survey>https://arxiv.org/abs/1605.07895</survey>
        <survey>https://arxiv.org/abs/1705.03645</survey>
        <survey>https://arxiv.org/abs/1712.05191</survey>
        <survey>https://arxiv.org/abs/2004.03186</survey>
        <survey>https://arxiv.org/abs/2007.04247</survey>
        <survey>https://arxiv.org/abs/2012.04821</survey>
        <survey>https://arxiv.org/abs/2101.06426</survey>
        <survey>https://arxiv.org/abs/2103.06118</survey>
        <survey>https://arxiv.org/abs/2103.07575</survey>
        <survey>https://arxiv.org/abs/2103.16929</survey>
        <survey>https://arxiv.org/abs/2306.02051</survey>
        <survey>https://arxiv.org/abs/2309.16396</survey>
        <survey>https://arxiv.org/abs/2310.19055</survey>
        <nlp-taxonomy:level rdf:datatype="http://www.w3.org/2001/XMLSchema#integer">2</nlp-taxonomy:level>
        <nlp-taxonomy:level rdf:datatype="http://www.w3.org/2001/XMLSchema#integer">3</nlp-taxonomy:level>
        <nlp-taxonomy:level rdf:datatype="http://www.w3.org/2001/XMLSchema#integer">7</nlp-taxonomy:level>
        <dcterms:description xml:lang="en">Relation Extraction is a subfield of Information Extraction &amp; Text Mining that deals with identifying and extracting semantic relationships between entities mentioned in text. It involves identifying the relevant entities and the type of relationship that exists between them.</dcterms:description>
        <oboInOwl:hasSynonym xml:lang="en">RE</oboInOwl:hasSynonym>
        <oboInOwl:hasSynonym xml:lang="en">Relation Classification</oboInOwl:hasSynonym>
        <oboInOwl:hasSynonym xml:lang="en">Relation Detection</oboInOwl:hasSynonym>
        <oboInOwl:hasSynonym xml:lang="en">Relation Recognition</oboInOwl:hasSynonym>
        <rdfs:label xml:lang="en">Relation Extraction</rdfs:label>
    </owl:NamedIndividual>
    


    <!-- http://nlpkg.sebis.cit.tum.de/nlp-taxonomy.owl#Representation_Learning -->

    <owl:NamedIndividual rdf:about="http://nlpkg.sebis.cit.tum.de/nlp-taxonomy.owl#Representation_Learning">
        <rdf:type rdf:resource="http://nlpkg.sebis.cit.tum.de/nlp-fos-hierarchy.owl#Task"/>
        <rdf:type rdf:resource="http://nlpkg.sebis.cit.tum.de/nlp-taxonomy.owl#FieldOfStudy"/>
        <nlp-taxonomy:subFieldOf rdf:resource="http://nlpkg.sebis.cit.tum.de/nlp-taxonomy.owl#Semantic_Text_Processing"/>
        <nlp-taxonomy:superFieldOf rdf:resource="http://nlpkg.sebis.cit.tum.de/nlp-fos-hierarchy.owl#Knowledge_Graph_Embeddings"/>
        <nlp-taxonomy:superFieldOf rdf:resource="http://nlpkg.sebis.cit.tum.de/nlp-fos-hierarchy.owl#Text_Representations"/>
        <relevantInformation>https://aclanthology.org/sigs/sigrep/</relevantInformation>
        <nlp-taxonomy:level rdf:datatype="http://www.w3.org/2001/XMLSchema#integer">2</nlp-taxonomy:level>
        <dcterms:description xml:lang="en">Representation Learning is a subfield of Semantic Text Processing that deals with the automatic learning and extraction of useful and compact representations of textual data, such as words, sentences, and documents, that can capture their semantic, syntactic, and pragmatic properties. It involves the development of algorithms and models that can transform natural language text into low-dimensional, dense, and informative vectors or embeddings that can be used in downstream tasks. This also includes learning vector representations of different modalities that can be used in NLP tasks.</dcterms:description>
        <rdfs:label xml:lang="en">Representation Learning</rdfs:label>
    </owl:NamedIndividual>
    


    <!-- http://nlpkg.sebis.cit.tum.de/nlp-taxonomy.owl#Robustness_In_NLP -->

    <owl:NamedIndividual rdf:about="http://nlpkg.sebis.cit.tum.de/nlp-taxonomy.owl#Robustness_In_NLP">
        <rdf:type rdf:resource="http://nlpkg.sebis.cit.tum.de/nlp-fos-hierarchy.owl#OtherScientificField"/>
        <rdf:type rdf:resource="http://nlpkg.sebis.cit.tum.de/nlp-taxonomy.owl#FieldOfStudy"/>
        <usedFor rdf:resource="http://nlpkg.sebis.cit.tum.de/nlp-fos-hierarchy.owl#Privacy,_Security_&amp;_Safety_in_NLP"/>
        <uses rdf:resource="http://nlpkg.sebis.cit.tum.de/nlp-fos-hierarchy.owl#Language_Model_Alignment"/>
        <uses rdf:resource="http://nlpkg.sebis.cit.tum.de/nlp-fos-hierarchy.owl#Meta-Learning"/>
        <nlp-taxonomy:subFieldOf rdf:resource="http://nlpkg.sebis.cit.tum.de/nlp-taxonomy.owl#Responsible_&amp;_Trustworthy_NLP"/>
        <nlp-taxonomy:superFieldOf rdf:resource="http://nlpkg.sebis.cit.tum.de/nlp-fos-hierarchy.owl#Adversarial_Training"/>
        <nlp-taxonomy:superFieldOf rdf:resource="http://nlpkg.sebis.cit.tum.de/nlp-fos-hierarchy.owl#Language_Model_Hallucination"/>
        <nlp-taxonomy:superFieldOf rdf:resource="http://nlpkg.sebis.cit.tum.de/nlp-fos-hierarchy.owl#Biases_&amp;_Fairness_in_NLP"/>
        <survey>https://aclanthology.org/2021.emnlp-main.117</survey>
        <survey>https://aclanthology.org/2022.findings-emnlp.441</survey>
        <survey>https://aclanthology.org/2022.naacl-main.339</survey>
        <survey>https://arxiv.org/abs/1902.07285</survey>
        <nlp-taxonomy:level rdf:datatype="http://www.w3.org/2001/XMLSchema#integer">2</nlp-taxonomy:level>
        <dcterms:description xml:lang="en">Robustness NLP is a subfield of Responsible NLP that deals with developing algorithms and models that are insensitive to biases, resistant to data perturbations, and reliable for out-of-distribution predictions. Robust models can operate reliably and accurately even in the presence of biased, noisy or adversarial input, such as misspellings, grammatical errors, or intentional attacks.</dcterms:description>
        <rdfs:label xml:lang="en">Robustness in NLP</rdfs:label>
    </owl:NamedIndividual>
    


    <!-- http://nlpkg.sebis.cit.tum.de/nlp-taxonomy.owl#Semantic_Parsing -->

    <owl:NamedIndividual rdf:about="http://nlpkg.sebis.cit.tum.de/nlp-taxonomy.owl#Semantic_Parsing">
        <rdf:type rdf:resource="http://nlpkg.sebis.cit.tum.de/nlp-fos-hierarchy.owl#Task"/>
        <rdf:type rdf:resource="http://nlpkg.sebis.cit.tum.de/nlp-taxonomy.owl#FieldOfStudy"/>
        <usedFor rdf:resource="http://nlpkg.sebis.cit.tum.de/nlp-taxonomy.owl#Code_Generation"/>
        <nlp-taxonomy:subFieldOf rdf:resource="http://nlpkg.sebis.cit.tum.de/nlp-taxonomy.owl#Semantic_Text_Processing"/>
        <nlp-taxonomy:superFieldOf rdf:resource="http://nlpkg.sebis.cit.tum.de/nlp-fos-hierarchy.owl#Compositional_Semantic_Parsing"/>
        <nlp-taxonomy:superFieldOf rdf:resource="http://nlpkg.sebis.cit.tum.de/nlp-fos-hierarchy.owl#Discourse_Parsing"/>
        <nlp-taxonomy:superFieldOf rdf:resource="http://nlpkg.sebis.cit.tum.de/nlp-fos-hierarchy.owl#Slot_Filling"/>
        <relevantInformation>https://aclanthology.org/sigs/sigparse/</relevantInformation>
        <relevantInformation>https://medium.com/explorations-in-language-and-learning/trends-in-semantic-parsing-part-1-ba11888523cb#:~:text=As%20such%2C%20semantic%20parsing%20refers,for%20which%20inference%20is%20required.</relevantInformation>
        <survey>https://aclanthology.org/2020.coling-main.226</survey>
        <survey>https://arxiv.org/abs/1812.00978</survey>
        <survey>https://arxiv.org/abs/1908.10461</survey>
        <survey>https://arxiv.org/abs/2009.14116</survey>
        <survey>https://arxiv.org/abs/2105.03317</survey>
        <survey>https://arxiv.org/abs/2208.13629</survey>
        <nlp-taxonomy:level rdf:datatype="http://www.w3.org/2001/XMLSchema#integer">2</nlp-taxonomy:level>
        <dcterms:description xml:lang="en">Semantic Parsing is a subfield of Semantic Text Processing that deals with the problem of mapping the meaning of natural language expressions into formal representations, such as logical forms, knowledge graphs, or database queries. It involves developing algorithms and models that can parse and understand the syntax, semantics, and pragmatics of a sentence and generate a structured representation of its meaning.</dcterms:description>
        <rdfs:label xml:lang="en">Semantic Parsing</rdfs:label>
    </owl:NamedIndividual>
    


    <!-- http://nlpkg.sebis.cit.tum.de/nlp-taxonomy.owl#Semantic_Search -->

    <owl:NamedIndividual rdf:about="http://nlpkg.sebis.cit.tum.de/nlp-taxonomy.owl#Semantic_Search">
        <rdf:type rdf:resource="http://nlpkg.sebis.cit.tum.de/nlp-fos-hierarchy.owl#Task"/>
        <rdf:type rdf:resource="http://nlpkg.sebis.cit.tum.de/nlp-taxonomy.owl#FieldOfStudy"/>
        <uses rdf:resource="http://nlpkg.sebis.cit.tum.de/nlp-fos-hierarchy.owl#Text_Representations"/>
        <uses rdf:resource="http://nlpkg.sebis.cit.tum.de/nlp-taxonomy.owl#Document_Retrieval"/>
        <uses rdf:resource="http://nlpkg.sebis.cit.tum.de/nlp-taxonomy.owl#Passage_Retrieval"/>
        <uses rdf:resource="http://nlpkg.sebis.cit.tum.de/nlp-taxonomy.owl#Semantic_Similarity"/>
        <nlp-taxonomy:subFieldOf rdf:resource="http://nlpkg.sebis.cit.tum.de/nlp-taxonomy.owl#Information_Retrieval"/>
        <nlp-taxonomy:subFieldOf rdf:resource="http://nlpkg.sebis.cit.tum.de/nlp-taxonomy.owl#Semantic_Text_Processing"/>
        <nlp-taxonomy:superFieldOf rdf:resource="http://nlpkg.sebis.cit.tum.de/nlp-fos-hierarchy.owl#Code_Search"/>
        <nlp-taxonomy:superFieldOf rdf:resource="http://nlpkg.sebis.cit.tum.de/nlp-fos-hierarchy.owl#Document_Expansion"/>
        <nlp-taxonomy:superFieldOf rdf:resource="http://nlpkg.sebis.cit.tum.de/nlp-fos-hierarchy.owl#Query_Expansion"/>
        <nlp-taxonomy:superFieldOf rdf:resource="http://nlpkg.sebis.cit.tum.de/nlp-fos-hierarchy.owl#Semantic_Matching"/>
        <survey>https://arxiv.org/abs/2301.05046</survey>
        <nlp-taxonomy:level rdf:datatype="http://www.w3.org/2001/XMLSchema#integer">2</nlp-taxonomy:level>
        <dcterms:description xml:lang="en">Semantic Search &amp; Search Engines is a subfield of Semantic Text Processing and Information Retrieval that deals with the retrieval and ranking of information and documents based on their meaning and relevance to a user&apos;s query. It involves developing algorithms and models that can understand and analyze the semantic and pragmatic aspects of a query and a document, such as context, ambiguity, and intent, and generate a ranked list of relevant and diverse results.</dcterms:description>
        <oboInOwl:hasSynonym xml:lang="en">Semantic Search</oboInOwl:hasSynonym>
        <rdfs:label xml:lang="en">Semantic Search &amp; Search Engines</rdfs:label>
    </owl:NamedIndividual>
    


    <!-- http://nlpkg.sebis.cit.tum.de/nlp-taxonomy.owl#Semantic_Similarity -->

    <owl:NamedIndividual rdf:about="http://nlpkg.sebis.cit.tum.de/nlp-taxonomy.owl#Semantic_Similarity">
        <rdf:type rdf:resource="http://nlpkg.sebis.cit.tum.de/nlp-fos-hierarchy.owl#OtherScientificField"/>
        <rdf:type rdf:resource="http://nlpkg.sebis.cit.tum.de/nlp-taxonomy.owl#FieldOfStudy"/>
        <usedFor rdf:resource="http://nlpkg.sebis.cit.tum.de/nlp-taxonomy.owl#Document_Retrieval"/>
        <usedFor rdf:resource="http://nlpkg.sebis.cit.tum.de/nlp-taxonomy.owl#Passage_Retrieval"/>
        <usedFor rdf:resource="http://nlpkg.sebis.cit.tum.de/nlp-taxonomy.owl#Semantic_Search"/>
        <nlp-taxonomy:subFieldOf rdf:resource="http://nlpkg.sebis.cit.tum.de/nlp-taxonomy.owl#Semantic_Text_Processing"/>
        <survey>https://aclanthology.org/J06-1003</survey>
        <survey>https://aclanthology.org/Q18-1008</survey>
        <survey>https://arxiv.org/abs/0806.3787</survey>
        <survey>https://arxiv.org/abs/1203.1858</survey>
        <survey>https://arxiv.org/abs/1910.03940</survey>
        <survey>https://arxiv.org/abs/2004.13820</survey>
        <nlp-taxonomy:level rdf:datatype="http://www.w3.org/2001/XMLSchema#integer">2</nlp-taxonomy:level>
        <dcterms:description xml:lang="en">Semantic Similarity is a subfield of Semantic Text Processing that deals with the quantification and comparison of the semantic similarity or relatedness between two or more pieces of text, such as words, sentences, phrases, or documents. It includes metrics that estimate the distance or semantic relatedness of texts based on their meanings.</dcterms:description>
        <oboInOwl:hasSynonym xml:lang="en">Distributional Similarity</oboInOwl:hasSynonym>
        <oboInOwl:hasSynonym xml:lang="en">STS</oboInOwl:hasSynonym>
        <oboInOwl:hasSynonym xml:lang="en">Semantic Relatedness</oboInOwl:hasSynonym>
        <oboInOwl:hasSynonym xml:lang="en">Semantic Textual Similarity</oboInOwl:hasSynonym>
        <rdfs:label xml:lang="en">Semantic Similarity</rdfs:label>
    </owl:NamedIndividual>
    


    <!-- http://nlpkg.sebis.cit.tum.de/nlp-taxonomy.owl#Semantic_Text_Processing -->

    <owl:NamedIndividual rdf:about="http://nlpkg.sebis.cit.tum.de/nlp-taxonomy.owl#Semantic_Text_Processing">
        <rdf:type rdf:resource="http://nlpkg.sebis.cit.tum.de/nlp-fos-hierarchy.owl#Task"/>
        <rdf:type rdf:resource="http://nlpkg.sebis.cit.tum.de/nlp-taxonomy.owl#FieldOfStudy"/>
        <nlp-taxonomy:subFieldOf rdf:resource="http://nlpkg.sebis.cit.tum.de/nlp-taxonomy.owl#Natural_Language_Processing"/>
        <nlp-taxonomy:superFieldOf rdf:resource="http://nlpkg.sebis.cit.tum.de/nlp-taxonomy.owl#Knowledge_Representation"/>
        <nlp-taxonomy:superFieldOf rdf:resource="http://nlpkg.sebis.cit.tum.de/nlp-taxonomy.owl#Language_Models"/>
        <nlp-taxonomy:superFieldOf rdf:resource="http://nlpkg.sebis.cit.tum.de/nlp-taxonomy.owl#Representation_Learning"/>
        <nlp-taxonomy:superFieldOf rdf:resource="http://nlpkg.sebis.cit.tum.de/nlp-taxonomy.owl#Semantic_Parsing"/>
        <nlp-taxonomy:superFieldOf rdf:resource="http://nlpkg.sebis.cit.tum.de/nlp-taxonomy.owl#Semantic_Search"/>
        <nlp-taxonomy:superFieldOf rdf:resource="http://nlpkg.sebis.cit.tum.de/nlp-taxonomy.owl#Semantic_Similarity"/>
        <nlp-taxonomy:superFieldOf rdf:resource="http://nlpkg.sebis.cit.tum.de/nlp-taxonomy.owl#Text_Complexity"/>
        <nlp-taxonomy:superFieldOf rdf:resource="http://nlpkg.sebis.cit.tum.de/nlp-taxonomy.owl#Word_Sense_Disambiguation"/>
        <nlp-taxonomy:superFieldOf rdf:resource="http://nlpkg.sebis.cit.tum.de/nlp-taxonomy.owl#Discourse_&amp;_Pragmatics"/>
        <nlp-taxonomy:level rdf:datatype="http://www.w3.org/2001/XMLSchema#integer">1</nlp-taxonomy:level>
        <dcterms:description xml:lang="en">Semantic Text Processing is a subfield of Natural Language Processing (NLP) that attempts to derive meaning from natural language and helps machines interpret textual data semantically. It involves developing algorithms and models that can understand and represent the semantics of words and sentences, and the relationships between them.</dcterms:description>
        <rdfs:label xml:lang="en">Semantic Text Processing</rdfs:label>
    </owl:NamedIndividual>
    


    <!-- http://nlpkg.sebis.cit.tum.de/nlp-taxonomy.owl#Sentiment_Analysis -->

    <owl:NamedIndividual rdf:about="http://nlpkg.sebis.cit.tum.de/nlp-taxonomy.owl#Sentiment_Analysis">
        <rdf:type rdf:resource="http://nlpkg.sebis.cit.tum.de/nlp-fos-hierarchy.owl#Task"/>
        <rdf:type rdf:resource="http://nlpkg.sebis.cit.tum.de/nlp-taxonomy.owl#FieldOfStudy"/>
        <nlp-taxonomy:subFieldOf rdf:resource="http://nlpkg.sebis.cit.tum.de/nlp-taxonomy.owl#Natural_Language_Processing"/>
        <nlp-taxonomy:superFieldOf rdf:resource="http://nlpkg.sebis.cit.tum.de/nlp-fos-hierarchy.owl#Entity-Level_Sentiment_Analysis"/>
        <nlp-taxonomy:superFieldOf rdf:resource="http://nlpkg.sebis.cit.tum.de/nlp-fos-hierarchy.owl#Subjectivity_Classification"/>
        <nlp-taxonomy:superFieldOf rdf:resource="http://nlpkg.sebis.cit.tum.de/nlp-taxonomy#Aspect-based_Sentiment_Analysis"/>
        <nlp-taxonomy:superFieldOf rdf:resource="http://nlpkg.sebis.cit.tum.de/nlp-taxonomy.owl#Emotion_Analysis"/>
        <nlp-taxonomy:superFieldOf rdf:resource="http://nlpkg.sebis.cit.tum.de/nlp-taxonomy.owl#Intent_Recognition"/>
        <nlp-taxonomy:superFieldOf rdf:resource="http://nlpkg.sebis.cit.tum.de/nlp-taxonomy.owl#Opinion_Mining"/>
        <nlp-taxonomy:superFieldOf rdf:resource="http://nlpkg.sebis.cit.tum.de/nlp-taxonomy.owl#Polarity_Analysis"/>
        <nlp-taxonomy:superFieldOf rdf:resource="http://nlpkg.sebis.cit.tum.de/nlp-taxonomy.owl#Stylistic_Analysis"/>
        <survey>https://arxiv.org/abs/1405.2584</survey>
        <survey>https://arxiv.org/abs/1511.09142</survey>
        <survey>https://arxiv.org/abs/1601.00087</survey>
        <survey>https://arxiv.org/abs/1601.06971</survey>
        <survey>https://arxiv.org/abs/1612.01556</survey>
        <survey>https://arxiv.org/abs/1801.07883</survey>
        <survey>https://arxiv.org/abs/1807.02471</survey>
        <survey>https://arxiv.org/abs/1901.02780</survey>
        <survey>https://arxiv.org/abs/1902.00753</survey>
        <survey>https://arxiv.org/abs/2005.00357</survey>
        <survey>https://arxiv.org/abs/2207.02160</survey>
        <survey>https://arxiv.org/abs/2305.07611</survey>
        <survey>https://arxiv.org/abs/2305.14842</survey>
        <survey>https://arxiv.org/abs/2309.02045</survey>
        <survey>https://arxiv.org/abs/2310.12318</survey>
        <nlp-taxonomy:level rdf:datatype="http://www.w3.org/2001/XMLSchema#integer">1</nlp-taxonomy:level>
        <dcterms:description xml:lang="en">Sentiment Analysis is a subfield of Natural Language Processing (NLP) that deals with the identification, extraction and quantification of affective states and subjective information from textual data.</dcterms:description>
        <oboInOwl:hasSynonym xml:lang="en">Sentiment Classification</oboInOwl:hasSynonym>
        <oboInOwl:hasSynonym xml:lang="en">Sentiment Detection</oboInOwl:hasSynonym>
        <oboInOwl:hasSynonym xml:lang="en">Sentiment Identification</oboInOwl:hasSynonym>
        <oboInOwl:hasSynonym xml:lang="en">Subjectivity Analysis</oboInOwl:hasSynonym>
        <oboInOwl:hasSynonym xml:lang="en">Subjectivity Classification</oboInOwl:hasSynonym>
        <oboInOwl:hasSynonym xml:lang="en">Subjectivity Detection</oboInOwl:hasSynonym>
        <oboInOwl:hasSynonym xml:lang="en">Subjectivity Identification</oboInOwl:hasSynonym>
        <rdfs:label xml:lang="en">Sentiment Analysis</rdfs:label>
    </owl:NamedIndividual>
    


    <!-- http://nlpkg.sebis.cit.tum.de/nlp-taxonomy.owl#Speech_Recognition -->

    <owl:NamedIndividual rdf:about="http://nlpkg.sebis.cit.tum.de/nlp-taxonomy.owl#Speech_Recognition">
        <rdf:type rdf:resource="http://nlpkg.sebis.cit.tum.de/nlp-fos-hierarchy.owl#Task"/>
        <rdf:type rdf:resource="http://nlpkg.sebis.cit.tum.de/nlp-taxonomy.owl#FieldOfStudy"/>
        <usedFor rdf:resource="http://nlpkg.sebis.cit.tum.de/nlp-fos-hierarchy.owl#Spoken_Language_Understanding"/>
        <nlp-taxonomy:subFieldOf rdf:resource="http://nlpkg.sebis.cit.tum.de/nlp-taxonomy.owl#Text_Generation"/>
        <nlp-taxonomy:subFieldOf rdf:resource="http://nlpkg.sebis.cit.tum.de/nlp-taxonomy.owl#Speech_&amp;_Audio_In_NLP"/>
        <nlp-taxonomy:superFieldOf rdf:resource="http://nlpkg.sebis.cit.tum.de/nlp-fos-hierarchy.owl#Acoustic_Modeling"/>
        <nlp-taxonomy:superFieldOf rdf:resource="http://nlpkg.sebis.cit.tum.de/nlp-fos-hierarchy.owl#Acoustic_Signal_Processing"/>
        <nlp-taxonomy:superFieldOf rdf:resource="http://nlpkg.sebis.cit.tum.de/nlp-fos-hierarchy.owl#Speaker_Diarization"/>
        <nlp-taxonomy:superFieldOf rdf:resource="http://nlpkg.sebis.cit.tum.de/nlp-fos-hierarchy.owl#Speech_Segmentation"/>
        <relevantInformation>https://web.stanford.edu/~jurafsky/slp3/16.pdf</relevantInformation>
        <survey>https://aclanthology.org/2022.lrec-1.542</survey>
        <survey>https://arxiv.org/abs/1001.2267</survey>
        <survey>https://arxiv.org/abs/1610.03934</survey>
        <survey>https://arxiv.org/abs/2008.11897</survey>
        <survey>https://arxiv.org/abs/2012.07974</survey>
        <survey>https://arxiv.org/abs/2102.07259</survey>
        <survey>https://arxiv.org/abs/2104.10747</survey>
        <survey>https://arxiv.org/abs/2106.04897</survey>
        <survey>https://arxiv.org/abs/2108.10254</survey>
        <survey>https://arxiv.org/abs/2211.09511</survey>
        <survey>https://arxiv.org/abs/2303.03329</survey>
        <nlp-taxonomy:level rdf:datatype="http://www.w3.org/2001/XMLSchema#integer">3</nlp-taxonomy:level>
        <dcterms:description xml:lang="en">Automatic Speech Recognition (ASR), or Speech-to-Text (STT), is a technology that converts spoken language into written text. It is a field that focuses on the development of systems and algorithms capable of transcribing spoken language accurately. ASR systems are designed to understand and interpret human speech, allowing computers to process and analyze spoken words.</dcterms:description>
        <oboInOwl:hasSynonym xml:lang="en">ASR</oboInOwl:hasSynonym>
        <oboInOwl:hasSynonym xml:lang="en">Computer Speech Recognition</oboInOwl:hasSynonym>
        <oboInOwl:hasSynonym xml:lang="en">STT</oboInOwl:hasSynonym>
        <oboInOwl:hasSynonym xml:lang="en">Speech Recognition</oboInOwl:hasSynonym>
        <oboInOwl:hasSynonym xml:lang="en">Speech-to-Text</oboInOwl:hasSynonym>
        <rdfs:label xml:lang="en">Automatic Speech Recognition</rdfs:label>
    </owl:NamedIndividual>
    


    <!-- http://nlpkg.sebis.cit.tum.de/nlp-taxonomy.owl#Structured_Data_In_NLP -->

    <owl:NamedIndividual rdf:about="http://nlpkg.sebis.cit.tum.de/nlp-taxonomy.owl#Structured_Data_In_NLP">
        <rdf:type rdf:resource="http://nlpkg.sebis.cit.tum.de/nlp-fos-hierarchy.owl#OtherScientificField"/>
        <rdf:type rdf:resource="http://nlpkg.sebis.cit.tum.de/nlp-taxonomy.owl#FieldOfStudy"/>
        <usedFor rdf:resource="http://nlpkg.sebis.cit.tum.de/nlp-fos-hierarchy.owl#Language_Grounding"/>
        <nlp-taxonomy:subFieldOf rdf:resource="http://nlpkg.sebis.cit.tum.de/nlp-taxonomy.owl#Multimodality"/>
        <nlp-taxonomy:superFieldOf rdf:resource="http://nlpkg.sebis.cit.tum.de/nlp-fos-hierarchy.owl#Knowledge_Bases"/>
        <nlp-taxonomy:superFieldOf rdf:resource="http://nlpkg.sebis.cit.tum.de/nlp-fos-hierarchy.owl#Structured_Data-specific_Language_Models"/>
        <nlp-taxonomy:superFieldOf rdf:resource="http://nlpkg.sebis.cit.tum.de/nlp-fos-hierarchy.owl#Text-to-Structured_Data"/>
        <nlp-taxonomy:superFieldOf rdf:resource="http://nlpkg.sebis.cit.tum.de/nlp-taxonomy.owl#Data-to-Text_Generation"/>
        <nlp-taxonomy:level rdf:datatype="http://www.w3.org/2001/XMLSchema#integer">2</nlp-taxonomy:level>
        <dcterms:description xml:lang="en">Structured Data in NLP is a subfield of Multimodality that deals with the processing of structured data such as tables or graphs in conjunction with textual data. It involves the development of algorithms and models that can extract, represent, and use structured data in natural language form.</dcterms:description>
        <rdfs:label xml:lang="en">Structured Data in NLP</rdfs:label>
    </owl:NamedIndividual>
    


    <!-- http://nlpkg.sebis.cit.tum.de/nlp-taxonomy.owl#Stylistic_Analysis -->

    <owl:NamedIndividual rdf:about="http://nlpkg.sebis.cit.tum.de/nlp-taxonomy.owl#Stylistic_Analysis">
        <rdf:type rdf:resource="http://nlpkg.sebis.cit.tum.de/nlp-fos-hierarchy.owl#Task"/>
        <rdf:type rdf:resource="http://nlpkg.sebis.cit.tum.de/nlp-taxonomy.owl#FieldOfStudy"/>
        <usedFor rdf:resource="http://nlpkg.sebis.cit.tum.de/nlp-fos-hierarchy.owl#Privacy,_Security_&amp;_Safety_in_NLP"/>
        <nlp-taxonomy:subFieldOf rdf:resource="http://nlpkg.sebis.cit.tum.de/nlp-taxonomy.owl#Sentiment_Analysis"/>
        <nlp-taxonomy:superFieldOf rdf:resource="http://nlpkg.sebis.cit.tum.de/nlp-fos-hierarchy.owl#Figurative_Language"/>
        <nlp-taxonomy:superFieldOf rdf:resource="http://nlpkg.sebis.cit.tum.de/nlp-fos-hierarchy.owl#Irony_Detection"/>
        <nlp-taxonomy:superFieldOf rdf:resource="http://nlpkg.sebis.cit.tum.de/nlp-fos-hierarchy.owl#Metaphor_Detection"/>
        <nlp-taxonomy:superFieldOf rdf:resource="http://nlpkg.sebis.cit.tum.de/nlp-fos-hierarchy.owl#Multiword_Expression_Processing"/>
        <nlp-taxonomy:superFieldOf rdf:resource="http://nlpkg.sebis.cit.tum.de/nlp-fos-hierarchy.owl#Sarcasm_Detection"/>
        <nlp-taxonomy:superFieldOf rdf:resource="http://nlpkg.sebis.cit.tum.de/nlp-fos-hierarchy.owl#Slang_Detection"/>
        <nlp-taxonomy:level rdf:datatype="http://www.w3.org/2001/XMLSchema#integer">2</nlp-taxonomy:level>
        <dcterms:description xml:lang="en">Stylistic Analysis is a subfield of Sentiment Analysis that deals with automatically analyzing the stylistic features and patterns in a given text, such as tone, mood, and writing style to extract the meaning or message contained in texts.</dcterms:description>
        <rdfs:label xml:lang="en">Stylistic Analysis</rdfs:label>
    </owl:NamedIndividual>
    


    <!-- http://nlpkg.sebis.cit.tum.de/nlp-taxonomy.owl#Summarization -->

    <owl:NamedIndividual rdf:about="http://nlpkg.sebis.cit.tum.de/nlp-taxonomy.owl#Summarization">
        <rdf:type rdf:resource="http://nlpkg.sebis.cit.tum.de/nlp-fos-hierarchy.owl#Task"/>
        <rdf:type rdf:resource="http://nlpkg.sebis.cit.tum.de/nlp-taxonomy.owl#FieldOfStudy"/>
        <usedFor rdf:resource="http://nlpkg.sebis.cit.tum.de/nlp-fos-hierarchy.owl#Justification_Production"/>
        <nlp-taxonomy:subFieldOf rdf:resource="http://nlpkg.sebis.cit.tum.de/nlp-taxonomy.owl#Text_Generation"/>
        <nlp-taxonomy:subFieldOf rdf:resource="http://nlpkg.sebis.cit.tum.de/nlp-taxonomy.owl#Information_Extraction_&amp;_Text_Mining"/>
        <nlp-taxonomy:superFieldOf rdf:resource="http://nlpkg.sebis.cit.tum.de/nlp-fos-hierarchy.owl#Abstractive_Summarization"/>
        <nlp-taxonomy:superFieldOf rdf:resource="http://nlpkg.sebis.cit.tum.de/nlp-fos-hierarchy.owl#Code_Summarization"/>
        <nlp-taxonomy:superFieldOf rdf:resource="http://nlpkg.sebis.cit.tum.de/nlp-fos-hierarchy.owl#Extractive_Summarization"/>
        <survey>https://aclanthology.org/2020.emnlp-main.33</survey>
        <survey>https://aclanthology.org/2020.emnlp-main.751</survey>
        <survey>https://aclanthology.org/2021.eacl-main.160</survey>
        <survey>https://aclanthology.org/2021.tacl-1.24</survey>
        <survey>https://aclanthology.org/2022.tacl-1.75</survey>
        <survey>https://arxiv.org/abs/1704.03242</survey>
        <survey>https://arxiv.org/abs/1706.08162</survey>
        <survey>https://arxiv.org/abs/1707.02268</survey>
        <survey>https://arxiv.org/abs/1804.04589</survey>
        <survey>https://arxiv.org/abs/2005.04684</survey>
        <survey>https://arxiv.org/abs/2008.11897</survey>
        <survey>https://arxiv.org/abs/2011.04843</survey>
        <survey>https://arxiv.org/abs/2107.03175</survey>
        <survey>https://arxiv.org/abs/2109.05199</survey>
        <survey>https://arxiv.org/abs/2204.01849</survey>
        <survey>https://arxiv.org/abs/2204.09519</survey>
        <survey>https://arxiv.org/abs/2204.11190</survey>
        <survey>https://arxiv.org/abs/2211.11548</survey>
        <survey>https://arxiv.org/abs/2301.03403</survey>
        <survey>https://arxiv.org/abs/2309.09558</survey>
        <survey>https://arxiv.org/abs/2310.09411</survey>
        <nlp-taxonomy:level rdf:datatype="http://www.w3.org/2001/XMLSchema#integer">2</nlp-taxonomy:level>
        <dcterms:description xml:lang="en">Text Summarization is a subfield of Information Extraction &amp; Text Mining and Text Generation that deals with the automatic generation of a concise and coherent summary of a longer text. It involves developing algorithms and models that can identify the most important information in a text and generate a summary that captures the essence of the original text.</dcterms:description>
        <oboInOwl:hasSynonym xml:lang="en">Summarisation</oboInOwl:hasSynonym>
        <rdfs:label xml:lang="en">Summarization</rdfs:label>
    </owl:NamedIndividual>
    


    <!-- http://nlpkg.sebis.cit.tum.de/nlp-taxonomy.owl#Syntactic_Parsing -->

    <owl:NamedIndividual rdf:about="http://nlpkg.sebis.cit.tum.de/nlp-taxonomy.owl#Syntactic_Parsing">
        <rdf:type rdf:resource="http://nlpkg.sebis.cit.tum.de/nlp-fos-hierarchy.owl#Task"/>
        <rdf:type rdf:resource="http://nlpkg.sebis.cit.tum.de/nlp-taxonomy.owl#FieldOfStudy"/>
        <nlp-taxonomy:subFieldOf rdf:resource="http://nlpkg.sebis.cit.tum.de/nlp-taxonomy.owl#Syntactic_Text_Processing"/>
        <nlp-taxonomy:superFieldOf rdf:resource="http://nlpkg.sebis.cit.tum.de/nlp-fos-hierarchy.owl#Constituency_Parsing"/>
        <nlp-taxonomy:superFieldOf rdf:resource="http://nlpkg.sebis.cit.tum.de/nlp-fos-hierarchy.owl#Dependency_Parsing"/>
        <relevantInformation>https://aclanthology.org/sigs/sigparse/</relevantInformation>
        <nlp-taxonomy:level rdf:datatype="http://www.w3.org/2001/XMLSchema#integer">2</nlp-taxonomy:level>
        <dcterms:description xml:lang="en">Syntactic Parsing is a subfield of Syntactic Text Processing that deals with automatically analyzing the syntactic structure of a sentence or text, and representing it in a formal or graphical form, such as a parse tree or dependency graph. It involves developing algorithms and models that can identify and classify the syntactic constituents, such as noun phrases and verb phrases, and their relationships in a sentence, and generate a structured representation of the sentence.</dcterms:description>
        <rdfs:label xml:lang="en">Syntactic Parsing</rdfs:label>
    </owl:NamedIndividual>
    


    <!-- http://nlpkg.sebis.cit.tum.de/nlp-taxonomy.owl#Syntactic_Text_Processing -->

    <owl:NamedIndividual rdf:about="http://nlpkg.sebis.cit.tum.de/nlp-taxonomy.owl#Syntactic_Text_Processing">
        <rdf:type rdf:resource="http://nlpkg.sebis.cit.tum.de/nlp-fos-hierarchy.owl#Task"/>
        <rdf:type rdf:resource="http://nlpkg.sebis.cit.tum.de/nlp-taxonomy.owl#FieldOfStudy"/>
        <nlp-taxonomy:subFieldOf rdf:resource="http://nlpkg.sebis.cit.tum.de/nlp-taxonomy.owl#Natural_Language_Processing"/>
        <nlp-taxonomy:superFieldOf rdf:resource="http://nlpkg.sebis.cit.tum.de/nlp-taxonomy.owl#Chunking"/>
        <nlp-taxonomy:superFieldOf rdf:resource="http://nlpkg.sebis.cit.tum.de/nlp-taxonomy.owl#Morphology"/>
        <nlp-taxonomy:superFieldOf rdf:resource="http://nlpkg.sebis.cit.tum.de/nlp-taxonomy.owl#Phonetics"/>
        <nlp-taxonomy:superFieldOf rdf:resource="http://nlpkg.sebis.cit.tum.de/nlp-taxonomy.owl#Phonology"/>
        <nlp-taxonomy:superFieldOf rdf:resource="http://nlpkg.sebis.cit.tum.de/nlp-taxonomy.owl#Syntactic_Parsing"/>
        <nlp-taxonomy:superFieldOf rdf:resource="http://nlpkg.sebis.cit.tum.de/nlp-taxonomy.owl#Tagging"/>
        <nlp-taxonomy:superFieldOf rdf:resource="http://nlpkg.sebis.cit.tum.de/nlp-taxonomy.owl#Text_Error_Correction"/>
        <nlp-taxonomy:superFieldOf rdf:resource="http://nlpkg.sebis.cit.tum.de/nlp-taxonomy.owl#Text_Normalization"/>
        <nlp-taxonomy:superFieldOf rdf:resource="http://nlpkg.sebis.cit.tum.de/nlp-taxonomy.owl#Text_Segmentation"/>
        <nlp-taxonomy:superFieldOf rdf:resource="http://nlpkg.sebis.cit.tum.de/nlp-taxonomy.owl#Typology"/>
        <survey>https://arxiv.org/abs/2010.01063</survey>
        <nlp-taxonomy:level rdf:datatype="http://www.w3.org/2001/XMLSchema#integer">1</nlp-taxonomy:level>
        <dcterms:description xml:lang="en">Syntactic Text Processing is a subfield of Natural Language Processing (NLP) that deals with the analysis of the syntax and grammatical structure of natural language texts.</dcterms:description>
        <rdfs:label xml:lang="en">Syntactic Text Processing</rdfs:label>
    </owl:NamedIndividual>
    


    <!-- http://nlpkg.sebis.cit.tum.de/nlp-taxonomy.owl#Tagging -->

    <owl:NamedIndividual rdf:about="http://nlpkg.sebis.cit.tum.de/nlp-taxonomy.owl#Tagging">
        <rdf:type rdf:resource="http://nlpkg.sebis.cit.tum.de/nlp-fos-hierarchy.owl#Task"/>
        <rdf:type rdf:resource="http://nlpkg.sebis.cit.tum.de/nlp-taxonomy.owl#FieldOfStudy"/>
        <nlp-taxonomy:subFieldOf rdf:resource="http://nlpkg.sebis.cit.tum.de/nlp-taxonomy.owl#Syntactic_Text_Processing"/>
        <nlp-taxonomy:superFieldOf rdf:resource="http://nlpkg.sebis.cit.tum.de/nlp-fos-hierarchy.owl#Part-of-Speech_Tagging"/>
        <nlp-taxonomy:level rdf:datatype="http://www.w3.org/2001/XMLSchema#integer">2</nlp-taxonomy:level>
        <dcterms:description xml:lang="en">Tagging is a subfield of Syntactic Text Processing that deals with automatically assigning labels or tags to words or other units in a natural language texts, based on their grammatical or syntactic properties.</dcterms:description>
        <rdfs:label xml:lang="en">Tagging</rdfs:label>
    </owl:NamedIndividual>
    


    <!-- http://nlpkg.sebis.cit.tum.de/nlp-taxonomy.owl#Term_Extraction -->

    <owl:NamedIndividual rdf:about="http://nlpkg.sebis.cit.tum.de/nlp-taxonomy.owl#Term_Extraction">
        <rdf:type rdf:resource="http://nlpkg.sebis.cit.tum.de/nlp-fos-hierarchy.owl#Task"/>
        <rdf:type rdf:resource="http://nlpkg.sebis.cit.tum.de/nlp-taxonomy.owl#FieldOfStudy"/>
        <usedFor rdf:resource="http://nlpkg.sebis.cit.tum.de/nlp-fos-hierarchy.owl#Ontology_Learning"/>
        <usedFor rdf:resource="http://nlpkg.sebis.cit.tum.de/nlp-fos-hierarchy.owl#Taxonomy_Learning"/>
        <usedFor rdf:resource="http://nlpkg.sebis.cit.tum.de/nlp-fos-hierarchy.owl#Knowledge_Graph_Construction_&amp;_Completion"/>
        <nlp-taxonomy:subFieldOf rdf:resource="http://nlpkg.sebis.cit.tum.de/nlp-taxonomy.owl#Information_Extraction_&amp;_Text_Mining"/>
        <nlp-taxonomy:superFieldOf rdf:resource="http://nlpkg.sebis.cit.tum.de/nlp-fos-hierarchy.owl#Aspect_Term_Extraction"/>
        <nlp-taxonomy:superFieldOf rdf:resource="http://nlpkg.sebis.cit.tum.de/nlp-fos-hierarchy.owl#Keyword_&amp;_Keyphrase_Extraction"/>
        <survey>https://arxiv.org/abs/2301.06767</survey>
        <nlp-taxonomy:level rdf:datatype="http://www.w3.org/2001/XMLSchema#integer">2</nlp-taxonomy:level>
        <dcterms:description xml:lang="en">Term Extraction is a subfield of Information Extraction &amp; Text Mining that deals with identifying and extracting relevant terms such as keywords or keyphrases from natural language texts.</dcterms:description>
        <oboInOwl:hasSynonym xml:lang="en">Terminology Extraction</oboInOwl:hasSynonym>
        <rdfs:label xml:lang="en">Term Extraction</rdfs:label>
    </owl:NamedIndividual>
    


    <!-- http://nlpkg.sebis.cit.tum.de/nlp-taxonomy.owl#Text_Classification -->

    <owl:NamedIndividual rdf:about="http://nlpkg.sebis.cit.tum.de/nlp-taxonomy.owl#Text_Classification">
        <rdf:type rdf:resource="http://nlpkg.sebis.cit.tum.de/nlp-fos-hierarchy.owl#Task"/>
        <rdf:type rdf:resource="http://nlpkg.sebis.cit.tum.de/nlp-taxonomy.owl#FieldOfStudy"/>
        <uses rdf:resource="http://nlpkg.sebis.cit.tum.de/nlp-fos-hierarchy.owl#Zero-shot_Entailment"/>
        <nlp-taxonomy:subFieldOf rdf:resource="http://nlpkg.sebis.cit.tum.de/nlp-taxonomy.owl#Information_Retrieval"/>
        <nlp-taxonomy:subFieldOf rdf:resource="http://nlpkg.sebis.cit.tum.de/nlp-taxonomy.owl#Information_Extraction_&amp;_Text_Mining"/>
        <nlp-taxonomy:superFieldOf rdf:resource="http://nlpkg.sebis.cit.tum.de/nlp-fos-hierarchy.owl#Analogy_Detection"/>
        <nlp-taxonomy:superFieldOf rdf:resource="http://nlpkg.sebis.cit.tum.de/nlp-fos-hierarchy.owl#Argument_Pair_Identification"/>
        <nlp-taxonomy:superFieldOf rdf:resource="http://nlpkg.sebis.cit.tum.de/nlp-fos-hierarchy.owl#Authorship_Attribution"/>
        <nlp-taxonomy:superFieldOf rdf:resource="http://nlpkg.sebis.cit.tum.de/nlp-fos-hierarchy.owl#Automatic_Essay_Scoring"/>
        <nlp-taxonomy:superFieldOf rdf:resource="http://nlpkg.sebis.cit.tum.de/nlp-fos-hierarchy.owl#Binary_Classification"/>
        <nlp-taxonomy:superFieldOf rdf:resource="http://nlpkg.sebis.cit.tum.de/nlp-fos-hierarchy.owl#Claim_Detection"/>
        <nlp-taxonomy:superFieldOf rdf:resource="http://nlpkg.sebis.cit.tum.de/nlp-fos-hierarchy.owl#Decision_Tree"/>
        <nlp-taxonomy:superFieldOf rdf:resource="http://nlpkg.sebis.cit.tum.de/nlp-fos-hierarchy.owl#Euphemism_Detection"/>
        <nlp-taxonomy:superFieldOf rdf:resource="http://nlpkg.sebis.cit.tum.de/nlp-fos-hierarchy.owl#Event_Detection"/>
        <nlp-taxonomy:superFieldOf rdf:resource="http://nlpkg.sebis.cit.tum.de/nlp-fos-hierarchy.owl#Evidence_Mining"/>
        <nlp-taxonomy:superFieldOf rdf:resource="http://nlpkg.sebis.cit.tum.de/nlp-fos-hierarchy.owl#Hallucination_Detection"/>
        <nlp-taxonomy:superFieldOf rdf:resource="http://nlpkg.sebis.cit.tum.de/nlp-fos-hierarchy.owl#Hate_Speech_Detection"/>
        <nlp-taxonomy:superFieldOf rdf:resource="http://nlpkg.sebis.cit.tum.de/nlp-fos-hierarchy.owl#Idiom_Identification"/>
        <nlp-taxonomy:superFieldOf rdf:resource="http://nlpkg.sebis.cit.tum.de/nlp-fos-hierarchy.owl#Irony_Detection"/>
        <nlp-taxonomy:superFieldOf rdf:resource="http://nlpkg.sebis.cit.tum.de/nlp-fos-hierarchy.owl#Language_Identification"/>
        <nlp-taxonomy:superFieldOf rdf:resource="http://nlpkg.sebis.cit.tum.de/nlp-fos-hierarchy.owl#Machine_Generated_Text_Detection"/>
        <nlp-taxonomy:superFieldOf rdf:resource="http://nlpkg.sebis.cit.tum.de/nlp-fos-hierarchy.owl#Metaphor_Detection"/>
        <nlp-taxonomy:superFieldOf rdf:resource="http://nlpkg.sebis.cit.tum.de/nlp-fos-hierarchy.owl#Misinformation_Detection"/>
        <nlp-taxonomy:superFieldOf rdf:resource="http://nlpkg.sebis.cit.tum.de/nlp-fos-hierarchy.owl#Multi-class_Classification"/>
        <nlp-taxonomy:superFieldOf rdf:resource="http://nlpkg.sebis.cit.tum.de/nlp-fos-hierarchy.owl#Multi-label_Classification"/>
        <nlp-taxonomy:superFieldOf rdf:resource="http://nlpkg.sebis.cit.tum.de/nlp-fos-hierarchy.owl#Offensive_Language_Detection"/>
        <nlp-taxonomy:superFieldOf rdf:resource="http://nlpkg.sebis.cit.tum.de/nlp-fos-hierarchy.owl#Paraphrase_Detection"/>
        <nlp-taxonomy:superFieldOf rdf:resource="http://nlpkg.sebis.cit.tum.de/nlp-fos-hierarchy.owl#Propaganda_Detection"/>
        <nlp-taxonomy:superFieldOf rdf:resource="http://nlpkg.sebis.cit.tum.de/nlp-fos-hierarchy.owl#Question_Classification"/>
        <nlp-taxonomy:superFieldOf rdf:resource="http://nlpkg.sebis.cit.tum.de/nlp-fos-hierarchy.owl#Sarcasm_Detection"/>
        <nlp-taxonomy:superFieldOf rdf:resource="http://nlpkg.sebis.cit.tum.de/nlp-fos-hierarchy.owl#Sequence_Labeling"/>
        <nlp-taxonomy:superFieldOf rdf:resource="http://nlpkg.sebis.cit.tum.de/nlp-fos-hierarchy.owl#Slang_Detection"/>
        <nlp-taxonomy:superFieldOf rdf:resource="http://nlpkg.sebis.cit.tum.de/nlp-fos-hierarchy.owl#Span_Detection"/>
        <nlp-taxonomy:superFieldOf rdf:resource="http://nlpkg.sebis.cit.tum.de/nlp-fos-hierarchy.owl#Stance_Detection"/>
        <nlp-taxonomy:superFieldOf rdf:resource="http://nlpkg.sebis.cit.tum.de/nlp-fos-hierarchy.owl#Subjectivity_Classification"/>
        <nlp-taxonomy:superFieldOf rdf:resource="http://nlpkg.sebis.cit.tum.de/nlp-fos-hierarchy.owl#Topic_Classification"/>
        <nlp-taxonomy:superFieldOf rdf:resource="http://nlpkg.sebis.cit.tum.de/nlp-fos-hierarchy.owl#Verdict_Prediction"/>
        <nlp-taxonomy:superFieldOf rdf:resource="http://nlpkg.sebis.cit.tum.de/nlp-taxonomy.owl#Emotion_Analysis"/>
        <nlp-taxonomy:superFieldOf rdf:resource="http://nlpkg.sebis.cit.tum.de/nlp-taxonomy.owl#Intent_Recognition"/>
        <nlp-taxonomy:superFieldOf rdf:resource="http://nlpkg.sebis.cit.tum.de/nlp-taxonomy.owl#Named_Entity_Recognition"/>
        <survey>https://arxiv.org/abs/1904.08067</survey>
        <survey>https://arxiv.org/abs/2004.03705</survey>
        <survey>https://arxiv.org/abs/2008.00364</survey>
        <survey>https://arxiv.org/abs/2204.03954</survey>
        <survey>https://arxiv.org/abs/2211.16285</survey>
        <survey>https://arxiv.org/abs/2305.14104</survey>
        <nlp-taxonomy:level rdf:datatype="http://www.w3.org/2001/XMLSchema#integer">2</nlp-taxonomy:level>
        <dcterms:description xml:lang="en">Text Classification is a subfield of Information Retrieval and Information Extraction &amp; Text Mining that deals with automatically assigning a label or class to a natural language text. It involves the development of algorithms and models that can learn to recognize patterns in texts and classify them into predefined categories.</dcterms:description>
        <oboInOwl:hasSynonym xml:lang="en">Categorization</oboInOwl:hasSynonym>
        <oboInOwl:hasSynonym xml:lang="en">Classification</oboInOwl:hasSynonym>
        <oboInOwl:hasSynonym xml:lang="en">Text Categorization</oboInOwl:hasSynonym>
        <oboInOwl:hasSynonym xml:lang="en">Textual Categorization</oboInOwl:hasSynonym>
        <oboInOwl:hasSynonym xml:lang="en">Textual Classification</oboInOwl:hasSynonym>
        <rdfs:label xml:lang="en">Text Classification</rdfs:label>
    </owl:NamedIndividual>
    


    <!-- http://nlpkg.sebis.cit.tum.de/nlp-taxonomy.owl#Text_Clustering -->

    <owl:NamedIndividual rdf:about="http://nlpkg.sebis.cit.tum.de/nlp-taxonomy.owl#Text_Clustering">
        <rdf:type rdf:resource="http://nlpkg.sebis.cit.tum.de/nlp-fos-hierarchy.owl#Task"/>
        <rdf:type rdf:resource="http://nlpkg.sebis.cit.tum.de/nlp-taxonomy.owl#FieldOfStudy"/>
        <usedFor rdf:resource="http://nlpkg.sebis.cit.tum.de/nlp-taxonomy.owl#Topic_Modeling"/>
        <uses rdf:resource="http://nlpkg.sebis.cit.tum.de/nlp-fos-hierarchy.owl#Text_Representations"/>
        <nlp-taxonomy:subFieldOf rdf:resource="http://nlpkg.sebis.cit.tum.de/nlp-fos-hierarchy.owl#Unsupervised_Learning"/>
        <nlp-taxonomy:subFieldOf rdf:resource="http://nlpkg.sebis.cit.tum.de/nlp-taxonomy.owl#Information_Extraction_&amp;_Text_Mining"/>
        <nlp-taxonomy:superFieldOf rdf:resource="http://nlpkg.sebis.cit.tum.de/nlp-fos-hierarchy.owl#Hierarchical_Clustering"/>
        <survey>https://arxiv.org/abs/2208.01712</survey>
        <nlp-taxonomy:level rdf:datatype="http://www.w3.org/2001/XMLSchema#integer">2</nlp-taxonomy:level>
        <nlp-taxonomy:level rdf:datatype="http://www.w3.org/2001/XMLSchema#integer">4</nlp-taxonomy:level>
        <dcterms:description xml:lang="en">Text Clustering is a subfield of Information Extraction &amp; Text Mining that deals with grouping similar documents or sentences into clusters based on their content. The goal of text clustering is to discover patterns in large amounts of unstructured text data and identify groups of documents that share common themes, topics, or features.</dcterms:description>
        <rdfs:label xml:lang="en">Text Clustering</rdfs:label>
    </owl:NamedIndividual>
    


    <!-- http://nlpkg.sebis.cit.tum.de/nlp-taxonomy.owl#Text_Complexity -->

    <owl:NamedIndividual rdf:about="http://nlpkg.sebis.cit.tum.de/nlp-taxonomy.owl#Text_Complexity">
        <rdf:type rdf:resource="http://nlpkg.sebis.cit.tum.de/nlp-fos-hierarchy.owl#OtherScientificField"/>
        <rdf:type rdf:resource="http://nlpkg.sebis.cit.tum.de/nlp-taxonomy.owl#FieldOfStudy"/>
        <nlp-taxonomy:subFieldOf rdf:resource="http://nlpkg.sebis.cit.tum.de/nlp-taxonomy.owl#Semantic_Text_Processing"/>
        <nlp-taxonomy:level rdf:datatype="http://www.w3.org/2001/XMLSchema#integer">2</nlp-taxonomy:level>
        <dcterms:description xml:lang="en">Text Complexity is a subfield of Semantic Text Processing that deals with the analysis and assessment of the difficulty, readability, and suitability of texts for different audiences and purposes. It can be assessed based on a series of factors, such as the readability of the text, the levels of meaning or purpose in the text, the structure of the text, the conventionality and clarity of the language, and the knowledge demands of the text.</dcterms:description>
        <oboInOwl:hasSynonym xml:lang="en">Readability Assessment</oboInOwl:hasSynonym>
        <oboInOwl:hasSynonym xml:lang="en">Text Complexity Assessment</oboInOwl:hasSynonym>
        <rdfs:label xml:lang="en">Text Complexity</rdfs:label>
    </owl:NamedIndividual>
    


    <!-- http://nlpkg.sebis.cit.tum.de/nlp-taxonomy.owl#Text_Error_Correction -->

    <owl:NamedIndividual rdf:about="http://nlpkg.sebis.cit.tum.de/nlp-taxonomy.owl#Text_Error_Correction">
        <rdf:type rdf:resource="http://nlpkg.sebis.cit.tum.de/nlp-fos-hierarchy.owl#Task"/>
        <rdf:type rdf:resource="http://nlpkg.sebis.cit.tum.de/nlp-taxonomy.owl#FieldOfStudy"/>
        <nlp-taxonomy:subFieldOf rdf:resource="http://nlpkg.sebis.cit.tum.de/nlp-taxonomy.owl#Syntactic_Text_Processing"/>
        <nlp-taxonomy:superFieldOf rdf:resource="http://nlpkg.sebis.cit.tum.de/nlp-fos-hierarchy.owl#Grammar_Induction"/>
        <nlp-taxonomy:superFieldOf rdf:resource="http://nlpkg.sebis.cit.tum.de/nlp-fos-hierarchy.owl#Grammatical_Error_Correction"/>
        <nlp-taxonomy:superFieldOf rdf:resource="http://nlpkg.sebis.cit.tum.de/nlp-fos-hierarchy.owl#Spell_Checking"/>
        <nlp-taxonomy:level rdf:datatype="http://www.w3.org/2001/XMLSchema#integer">2</nlp-taxonomy:level>
        <dcterms:description xml:lang="en">Text Error Correction is a subfield of Syntactic Text Processing that deals with automatically detecting and correcting grammatical errors in a text, such as spelling mistakes, word choice errors, or syntax errors. It involves developing algorithms and models that can identify and diagnose the errors, generate corrected versions of the text, and evaluate the quality and accuracy of the corrections.</dcterms:description>
        <rdfs:label xml:lang="en">Text Error Correction</rdfs:label>
    </owl:NamedIndividual>
    


    <!-- http://nlpkg.sebis.cit.tum.de/nlp-taxonomy.owl#Text_Generation -->

    <owl:NamedIndividual rdf:about="http://nlpkg.sebis.cit.tum.de/nlp-taxonomy.owl#Text_Generation">
        <rdf:type rdf:resource="http://nlpkg.sebis.cit.tum.de/nlp-fos-hierarchy.owl#Task"/>
        <rdf:type rdf:resource="http://nlpkg.sebis.cit.tum.de/nlp-taxonomy.owl#FieldOfStudy"/>
        <usedFor rdf:resource="http://nlpkg.sebis.cit.tum.de/nlp-fos-hierarchy.owl#Retrieval_Augmented_Generation"/>
        <usedFor rdf:resource="http://nlpkg.sebis.cit.tum.de/nlp-taxonomy.owl#Natural_Language_Interfaces"/>
        <nlp-taxonomy:subFieldOf rdf:resource="http://nlpkg.sebis.cit.tum.de/nlp-taxonomy.owl#Natural_Language_Processing"/>
        <nlp-taxonomy:superFieldOf rdf:resource="http://nlpkg.sebis.cit.tum.de/nlp-fos-hierarchy.owl#Argument_Generation"/>
        <nlp-taxonomy:superFieldOf rdf:resource="http://nlpkg.sebis.cit.tum.de/nlp-fos-hierarchy.owl#Controllable_Text_Generation"/>
        <nlp-taxonomy:superFieldOf rdf:resource="http://nlpkg.sebis.cit.tum.de/nlp-fos-hierarchy.owl#Story_Generation"/>
        <nlp-taxonomy:superFieldOf rdf:resource="http://nlpkg.sebis.cit.tum.de/nlp-taxonomy.owl#Captioning"/>
        <nlp-taxonomy:superFieldOf rdf:resource="http://nlpkg.sebis.cit.tum.de/nlp-taxonomy.owl#Code_Generation"/>
        <nlp-taxonomy:superFieldOf rdf:resource="http://nlpkg.sebis.cit.tum.de/nlp-taxonomy.owl#Data-to-Text_Generation"/>
        <nlp-taxonomy:superFieldOf rdf:resource="http://nlpkg.sebis.cit.tum.de/nlp-taxonomy.owl#Dialogue_Response_Generation"/>
        <nlp-taxonomy:superFieldOf rdf:resource="http://nlpkg.sebis.cit.tum.de/nlp-taxonomy.owl#Machine_Translation"/>
        <nlp-taxonomy:superFieldOf rdf:resource="http://nlpkg.sebis.cit.tum.de/nlp-taxonomy.owl#Paraphrasing"/>
        <nlp-taxonomy:superFieldOf rdf:resource="http://nlpkg.sebis.cit.tum.de/nlp-taxonomy.owl#Question_Answering"/>
        <nlp-taxonomy:superFieldOf rdf:resource="http://nlpkg.sebis.cit.tum.de/nlp-taxonomy.owl#Question_Generation"/>
        <nlp-taxonomy:superFieldOf rdf:resource="http://nlpkg.sebis.cit.tum.de/nlp-taxonomy.owl#Speech_Recognition"/>
        <nlp-taxonomy:superFieldOf rdf:resource="http://nlpkg.sebis.cit.tum.de/nlp-taxonomy.owl#Summarization"/>
        <nlp-taxonomy:superFieldOf rdf:resource="http://nlpkg.sebis.cit.tum.de/nlp-taxonomy.owl#Text_Style_Transfer"/>
        <relevantInformation>https://aclanthology.org/sigs/siggen/</relevantInformation>
        <survey>https://aclanthology.org/2021.acl-long.565</survey>
        <survey>https://aclanthology.org/2021.gem-1.9/</survey>
        <survey>https://aclanthology.org/2021.nuse-1.8</survey>
        <survey>https://aclanthology.org/2022.insights-1.25</survey>
        <survey>https://arxiv.org/abs/1611.06216</survey>
        <survey>https://arxiv.org/abs/1703.09902</survey>
        <survey>https://arxiv.org/abs/1803.07133</survey>
        <survey>https://arxiv.org/abs/1911.06171</survey>
        <survey>https://arxiv.org/abs/2006.14799</survey>
        <survey>https://arxiv.org/abs/2007.15780</survey>
        <survey>https://arxiv.org/abs/2008.12009</survey>
        <survey>https://arxiv.org/abs/2010.04389</survey>
        <survey>https://arxiv.org/abs/2010.07279</survey>
        <survey>https://arxiv.org/abs/2101.05786</survey>
        <survey>https://arxiv.org/abs/2105.10311</survey>
        <survey>https://arxiv.org/abs/2112.11739</survey>
        <survey>https://arxiv.org/abs/2201.05273</survey>
        <survey>https://arxiv.org/abs/2201.05337</survey>
        <survey>https://arxiv.org/abs/2202.06935</survey>
        <survey>https://arxiv.org/abs/2203.03047</survey>
        <survey>https://arxiv.org/abs/2203.05227</survey>
        <survey>https://arxiv.org/abs/2212.03747</survey>
        <survey>https://arxiv.org/abs/2303.04226</survey>
        <survey>https://arxiv.org/abs/2305.00955</survey>
        <survey>https://arxiv.org/abs/2305.08493</survey>
        <survey>https://arxiv.org/abs/2312.10868</survey>
        <survey>https://arxiv.org/abs/2401.07103</survey>
        <nlp-taxonomy:level rdf:datatype="http://www.w3.org/2001/XMLSchema#integer">1</nlp-taxonomy:level>
        <dcterms:description xml:lang="en">Text Generation is a subfield of Natural Language Processing (NLP) which attempts to teach machines to automatically generate texts that are indistinguishable from texts written by humans.</dcterms:description>
        <oboInOwl:hasSynonym xml:lang="en">NLG</oboInOwl:hasSynonym>
        <oboInOwl:hasSynonym xml:lang="en">Natural Language Generation</oboInOwl:hasSynonym>
        <rdfs:label xml:lang="en">Text Generation</rdfs:label>
    </owl:NamedIndividual>
    


    <!-- http://nlpkg.sebis.cit.tum.de/nlp-taxonomy.owl#Text_Normalization -->

    <owl:NamedIndividual rdf:about="http://nlpkg.sebis.cit.tum.de/nlp-taxonomy.owl#Text_Normalization">
        <rdf:type rdf:resource="http://nlpkg.sebis.cit.tum.de/nlp-fos-hierarchy.owl#Task"/>
        <rdf:type rdf:resource="http://nlpkg.sebis.cit.tum.de/nlp-taxonomy.owl#FieldOfStudy"/>
        <uses rdf:resource="http://nlpkg.sebis.cit.tum.de/nlp-fos-hierarchy.owl#Lemmatization"/>
        <uses rdf:resource="http://nlpkg.sebis.cit.tum.de/nlp-fos-hierarchy.owl#Stemming"/>
        <nlp-taxonomy:subFieldOf rdf:resource="http://nlpkg.sebis.cit.tum.de/nlp-taxonomy.owl#Syntactic_Text_Processing"/>
        <nlp-taxonomy:superFieldOf rdf:resource="http://nlpkg.sebis.cit.tum.de/nlp-fos-hierarchy.owl#Text_Scrubbing"/>
        <relevantInformation>https://web.stanford.edu/~jurafsky/slp3/2.pdf</relevantInformation>
        <survey>https://aclanthology.org/2021.ranlp-1.7</survey>
        <nlp-taxonomy:level rdf:datatype="http://www.w3.org/2001/XMLSchema#integer">2</nlp-taxonomy:level>
        <dcterms:description xml:lang="en">Text Normalization is a subfield of Syntactic Text Processing that deals with the process of transforming text into a single canonical form that it might not have had before. It reduces variations in word forms to a common form when the variations mean the same thing by converting word tokens to their base form.</dcterms:description>
        <rdfs:label xml:lang="en">Text Normalization</rdfs:label>
    </owl:NamedIndividual>
    


    <!-- http://nlpkg.sebis.cit.tum.de/nlp-taxonomy.owl#Text_Segmentation -->

    <owl:NamedIndividual rdf:about="http://nlpkg.sebis.cit.tum.de/nlp-taxonomy.owl#Text_Segmentation">
        <rdf:type rdf:resource="http://nlpkg.sebis.cit.tum.de/nlp-fos-hierarchy.owl#Task"/>
        <rdf:type rdf:resource="http://nlpkg.sebis.cit.tum.de/nlp-taxonomy.owl#FieldOfStudy"/>
        <usedFor rdf:resource="http://nlpkg.sebis.cit.tum.de/nlp-taxonomy.owl#Document_Retrieval"/>
        <usedFor rdf:resource="http://nlpkg.sebis.cit.tum.de/nlp-taxonomy.owl#Passage_Retrieval"/>
        <uses rdf:resource="http://nlpkg.sebis.cit.tum.de/nlp-taxonomy.owl#Chunking"/>
        <nlp-taxonomy:subFieldOf rdf:resource="http://nlpkg.sebis.cit.tum.de/nlp-taxonomy.owl#Syntactic_Text_Processing"/>
        <nlp-taxonomy:superFieldOf rdf:resource="http://nlpkg.sebis.cit.tum.de/nlp-fos-hierarchy.owl#Morphological_Segmentation"/>
        <nlp-taxonomy:superFieldOf rdf:resource="http://nlpkg.sebis.cit.tum.de/nlp-fos-hierarchy.owl#Tokenization"/>
        <nlp-taxonomy:superFieldOf rdf:resource="http://nlpkg.sebis.cit.tum.de/nlp-fos-hierarchy.owl#n-gram"/>
        <nlp-taxonomy:level rdf:datatype="http://www.w3.org/2001/XMLSchema#integer">2</nlp-taxonomy:level>
        <dcterms:description xml:lang="en">Text Segmentation is a subfield of Syntactic Text Processing that deals with automatically dividing a text into smaller segments or units that can be analyzed or processed separately. It involves developing algorithms and models that can identify and classify the structural or semantic boundaries between different sections or paragraphs in a text, and group them into meaningful and coherent segments.</dcterms:description>
        <rdfs:label xml:lang="en">Text Segmentation</rdfs:label>
    </owl:NamedIndividual>
    


    <!-- http://nlpkg.sebis.cit.tum.de/nlp-taxonomy.owl#Text_Style_Transfer -->

    <owl:NamedIndividual rdf:about="http://nlpkg.sebis.cit.tum.de/nlp-taxonomy.owl#Text_Style_Transfer">
        <rdf:type rdf:resource="http://nlpkg.sebis.cit.tum.de/nlp-fos-hierarchy.owl#Task"/>
        <rdf:type rdf:resource="http://nlpkg.sebis.cit.tum.de/nlp-taxonomy.owl#FieldOfStudy"/>
        <nlp-taxonomy:subFieldOf rdf:resource="http://nlpkg.sebis.cit.tum.de/nlp-taxonomy.owl#Text_Generation"/>
        <survey>https://aclanthology.org/2021.gem-1.6</survey>
        <survey>https://aclanthology.org/2022.cl-1.6</survey>
        <survey>https://arxiv.org/abs/2005.02914</survey>
        <survey>https://arxiv.org/abs/2010.12742</survey>
        <survey>https://arxiv.org/abs/2106.04747</survey>
        <survey>https://arxiv.org/abs/2109.15144</survey>
        <survey>https://arxiv.org/abs/2110.15871</survey>
        <nlp-taxonomy:level rdf:datatype="http://www.w3.org/2001/XMLSchema#integer">2</nlp-taxonomy:level>
        <dcterms:description xml:lang="en">Text Style Transfer is a subfield of Text Generation that deals with adapting and/or changing the stylistic manner in which a text is written, while preserving the semantic meaning of the original text.</dcterms:description>
        <oboInOwl:hasSynonym xml:lang="en">Style Transfer</oboInOwl:hasSynonym>
        <oboInOwl:hasSynonym xml:lang="en">TST</oboInOwl:hasSynonym>
        <rdfs:label xml:lang="en">Text Style Transfer</rdfs:label>
    </owl:NamedIndividual>
    


    <!-- http://nlpkg.sebis.cit.tum.de/nlp-taxonomy.owl#Textual_Inference -->

    <owl:NamedIndividual rdf:about="http://nlpkg.sebis.cit.tum.de/nlp-taxonomy.owl#Textual_Inference">
        <rdf:type rdf:resource="http://nlpkg.sebis.cit.tum.de/nlp-fos-hierarchy.owl#Task"/>
        <rdf:type rdf:resource="http://nlpkg.sebis.cit.tum.de/nlp-taxonomy.owl#FieldOfStudy"/>
        <nlp-taxonomy:subFieldOf rdf:resource="http://nlpkg.sebis.cit.tum.de/nlp-taxonomy.owl#Reasoning"/>
        <nlp-taxonomy:superFieldOf rdf:resource="http://nlpkg.sebis.cit.tum.de/nlp-fos-hierarchy.owl#Zero-shot_Entailment"/>
        <survey>https://aclanthology.org/2020.acl-main.474</survey>
        <survey>https://aclanthology.org/2020.eval4nlp-1.10</survey>
        <survey>https://aclanthology.org/D19-1630</survey>
        <survey>https://arxiv.org/abs/0912.3747</survey>
        <survey>https://arxiv.org/abs/1904.01172</survey>
        <survey>https://arxiv.org/abs/2005.14709</survey>
        <survey>https://arxiv.org/abs/2010.03061</survey>
        <nlp-taxonomy:level rdf:datatype="http://www.w3.org/2001/XMLSchema#integer">2</nlp-taxonomy:level>
        <dcterms:description xml:lang="en">Textual Inference is a subfield of Reasoning that deals with the task of automatically determining whether a natural-language hypothesis can be inferred from a given premise, predicting their logical relationship, such as entailment, contradiction, or neutral.</dcterms:description>
        <oboInOwl:hasSynonym xml:lang="en">NLI</oboInOwl:hasSynonym>
        <oboInOwl:hasSynonym xml:lang="en">Natural Language Inference</oboInOwl:hasSynonym>
        <oboInOwl:hasSynonym xml:lang="en">RTE</oboInOwl:hasSynonym>
        <oboInOwl:hasSynonym xml:lang="en">Recognizing Textual Entailment</oboInOwl:hasSynonym>
        <oboInOwl:hasSynonym xml:lang="en">Textual Entailment</oboInOwl:hasSynonym>
        <rdfs:label xml:lang="en">Textual Inference</rdfs:label>
    </owl:NamedIndividual>
    


    <!-- http://nlpkg.sebis.cit.tum.de/nlp-taxonomy.owl#Topic_Modeling -->

    <owl:NamedIndividual rdf:about="http://nlpkg.sebis.cit.tum.de/nlp-taxonomy.owl#Topic_Modeling">
        <rdf:type rdf:resource="http://nlpkg.sebis.cit.tum.de/nlp-fos-hierarchy.owl#Task"/>
        <rdf:type rdf:resource="http://nlpkg.sebis.cit.tum.de/nlp-taxonomy.owl#FieldOfStudy"/>
        <uses rdf:resource="http://nlpkg.sebis.cit.tum.de/nlp-taxonomy.owl#Text_Clustering"/>
        <nlp-taxonomy:subFieldOf rdf:resource="http://nlpkg.sebis.cit.tum.de/nlp-taxonomy.owl#Information_Extraction_&amp;_Text_Mining"/>
        <survey>https://aclanthology.org/W13-0102</survey>
        <survey>https://arxiv.org/abs/1904.07695</survey>
        <survey>https://arxiv.org/abs/2103.00498</survey>
        <survey>https://arxiv.org/abs/2208.01712</survey>
        <nlp-taxonomy:level rdf:datatype="http://www.w3.org/2001/XMLSchema#integer">2</nlp-taxonomy:level>
        <dcterms:description xml:lang="en">Topic Modeling is a subfield of Information Extraction &amp; Text Mining that deals with automatically discovering latent topics or themes in a large corpus of natural language text. It involves developing algorithms and models that can identify and extract the main themes or topics in the text, and cluster the documents based on their topic distribution.</dcterms:description>
        <rdfs:label xml:lang="en">Topic Modeling</rdfs:label>
    </owl:NamedIndividual>
    


    <!-- http://nlpkg.sebis.cit.tum.de/nlp-taxonomy.owl#Typology -->

    <owl:NamedIndividual rdf:about="http://nlpkg.sebis.cit.tum.de/nlp-taxonomy.owl#Typology">
        <rdf:type rdf:resource="http://nlpkg.sebis.cit.tum.de/nlp-fos-hierarchy.owl#OtherScientificField"/>
        <rdf:type rdf:resource="http://nlpkg.sebis.cit.tum.de/nlp-taxonomy.owl#FieldOfStudy"/>
        <nlp-taxonomy:subFieldOf rdf:resource="http://nlpkg.sebis.cit.tum.de/nlp-taxonomy.owl#Multilinguality"/>
        <nlp-taxonomy:subFieldOf rdf:resource="http://nlpkg.sebis.cit.tum.de/nlp-taxonomy.owl#Syntactic_Text_Processing"/>
        <relevantInformation>https://aclanthology.org/sigs/sigtyp/</relevantInformation>
        <survey>https://aclanthology.org/C16-1123</survey>
        <survey>https://arxiv.org/abs/1807.00914</survey>
        <nlp-taxonomy:level rdf:datatype="http://www.w3.org/2001/XMLSchema#integer">2</nlp-taxonomy:level>
        <dcterms:description xml:lang="en">Typology is a subfield of Syntactic Text Processing and Multilinguality that deals with studying the diversity and commonalities of the grammatical structures and patterns in different languages to allow their comparison. Its aim is to describe and explain the structural diversity and the common properties of the world&apos;s languages.</dcterms:description>
        <rdfs:label xml:lang="en">Typology</rdfs:label>
    </owl:NamedIndividual>
    


    <!-- http://nlpkg.sebis.cit.tum.de/nlp-taxonomy.owl#Visual_Data_In_NLP -->

    <owl:NamedIndividual rdf:about="http://nlpkg.sebis.cit.tum.de/nlp-taxonomy.owl#Visual_Data_In_NLP">
        <rdf:type rdf:resource="http://nlpkg.sebis.cit.tum.de/nlp-fos-hierarchy.owl#OtherScientificField"/>
        <rdf:type rdf:resource="http://nlpkg.sebis.cit.tum.de/nlp-taxonomy.owl#FieldOfStudy"/>
        <usedFor rdf:resource="http://nlpkg.sebis.cit.tum.de/nlp-fos-hierarchy.owl#Language_Grounding"/>
        <nlp-taxonomy:subFieldOf rdf:resource="http://nlpkg.sebis.cit.tum.de/nlp-taxonomy.owl#Multimodality"/>
        <nlp-taxonomy:superFieldOf rdf:resource="http://nlpkg.sebis.cit.tum.de/nlp-fos-hierarchy.owl#Image-to-Text_Retrieval"/>
        <nlp-taxonomy:superFieldOf rdf:resource="http://nlpkg.sebis.cit.tum.de/nlp-fos-hierarchy.owl#Image_Captioning"/>
        <nlp-taxonomy:superFieldOf rdf:resource="http://nlpkg.sebis.cit.tum.de/nlp-fos-hierarchy.owl#Meme_Classification"/>
        <nlp-taxonomy:superFieldOf rdf:resource="http://nlpkg.sebis.cit.tum.de/nlp-fos-hierarchy.owl#Optical_Character_Recognition"/>
        <nlp-taxonomy:superFieldOf rdf:resource="http://nlpkg.sebis.cit.tum.de/nlp-fos-hierarchy.owl#Referring_Expression_Comprehension"/>
        <nlp-taxonomy:superFieldOf rdf:resource="http://nlpkg.sebis.cit.tum.de/nlp-fos-hierarchy.owl#Scene_Text_Recognition"/>
        <nlp-taxonomy:superFieldOf rdf:resource="http://nlpkg.sebis.cit.tum.de/nlp-fos-hierarchy.owl#Text-to-Image"/>
        <nlp-taxonomy:superFieldOf rdf:resource="http://nlpkg.sebis.cit.tum.de/nlp-fos-hierarchy.owl#Text-to-Image_Retrieval"/>
        <nlp-taxonomy:superFieldOf rdf:resource="http://nlpkg.sebis.cit.tum.de/nlp-fos-hierarchy.owl#Text-to-Video"/>
        <nlp-taxonomy:superFieldOf rdf:resource="http://nlpkg.sebis.cit.tum.de/nlp-fos-hierarchy.owl#Video-Text_Retrieval"/>
        <nlp-taxonomy:superFieldOf rdf:resource="http://nlpkg.sebis.cit.tum.de/nlp-fos-hierarchy.owl#Video_Captioning"/>
        <nlp-taxonomy:superFieldOf rdf:resource="http://nlpkg.sebis.cit.tum.de/nlp-fos-hierarchy.owl#Vision-specific_Language_Models"/>
        <nlp-taxonomy:superFieldOf rdf:resource="http://nlpkg.sebis.cit.tum.de/nlp-fos-hierarchy.owl#Visual_Question_Answering"/>
        <nlp-taxonomy:superFieldOf rdf:resource="http://nlpkg.sebis.cit.tum.de/nlp-fos-hierarchy.owl#Visual_Reasoning"/>
        <survey>https://aclanthology.org/2022.acl-long.524</survey>
        <survey>https://aclanthology.org/D15-1021</survey>
        <survey>https://arxiv.org/abs/1907.09358</survey>
        <survey>https://arxiv.org/abs/2010.09522</survey>
        <survey>https://arxiv.org/abs/2201.11794</survey>
        <survey>https://arxiv.org/abs/2207.07568</survey>
        <survey>https://arxiv.org/abs/2303.02411</survey>
        <survey>https://arxiv.org/abs/2305.14598</survey>
        <nlp-taxonomy:level rdf:datatype="http://www.w3.org/2001/XMLSchema#integer">2</nlp-taxonomy:level>
        <dcterms:description xml:lang="en">Visual Data in NLP is a subfield of Multimodality that deals with the processing of visual data such as images or videos in conjunction with textual data.</dcterms:description>
        <oboInOwl:hasSynonym xml:lang="en">VL</oboInOwl:hasSynonym>
        <oboInOwl:hasSynonym xml:lang="en">Visio-Linguistic Learning</oboInOwl:hasSynonym>
        <oboInOwl:hasSynonym xml:lang="en">Visio-Linguistics</oboInOwl:hasSynonym>
        <oboInOwl:hasSynonym xml:lang="en">Visiolinguistic Learning</oboInOwl:hasSynonym>
        <oboInOwl:hasSynonym xml:lang="en">Visiolinguistics</oboInOwl:hasSynonym>
        <oboInOwl:hasSynonym xml:lang="en">Vision in NLP</oboInOwl:hasSynonym>
        <oboInOwl:hasSynonym xml:lang="en">Vision-Language Learning</oboInOwl:hasSynonym>
        <oboInOwl:hasSynonym xml:lang="en">Visual-Linguistics</oboInOwl:hasSynonym>
        <rdfs:label xml:lang="en">Visual Data in NLP</rdfs:label>
    </owl:NamedIndividual>
    


    <!-- http://nlpkg.sebis.cit.tum.de/nlp-taxonomy.owl#Word_Sense_Disambiguation -->

    <owl:NamedIndividual rdf:about="http://nlpkg.sebis.cit.tum.de/nlp-taxonomy.owl#Word_Sense_Disambiguation">
        <rdf:type rdf:resource="http://nlpkg.sebis.cit.tum.de/nlp-fos-hierarchy.owl#Task"/>
        <rdf:type rdf:resource="http://nlpkg.sebis.cit.tum.de/nlp-taxonomy.owl#FieldOfStudy"/>
        <nlp-taxonomy:subFieldOf rdf:resource="http://nlpkg.sebis.cit.tum.de/nlp-taxonomy.owl#Semantic_Text_Processing"/>
        <nlp-taxonomy:superFieldOf rdf:resource="http://nlpkg.sebis.cit.tum.de/nlp-fos-hierarchy.owl#All-words_Word_Sense_Disambiguation"/>
        <nlp-taxonomy:superFieldOf rdf:resource="http://nlpkg.sebis.cit.tum.de/nlp-fos-hierarchy.owl#Lexical_Sample_Word_Sense_Disambiguation"/>
        <nlp-taxonomy:superFieldOf rdf:resource="http://nlpkg.sebis.cit.tum.de/nlp-fos-hierarchy.owl#Word_Sense_Induction"/>
        <relevantInformation>https://web.stanford.edu/~jurafsky/slp3/23.pdf</relevantInformation>
        <survey>https://aclanthology.org/2020.lrec-1.706</survey>
        <survey>https://arxiv.org/abs/1508.01346</survey>
        <nlp-taxonomy:level rdf:datatype="http://www.w3.org/2001/XMLSchema#integer">2</nlp-taxonomy:level>
        <dcterms:description xml:lang="en">Word Sense Disambiguation is a subfield of Semantic Text Processing that deals with the problem of identifying the correct meaning or sense of a word in a given context, which can be ambiguous or polysemous. It involves developing algorithms and models that can analyze the syntactic and semantic features of a sentence and disambiguate the senses of the words in it, based on their co-occurrence patterns, collocations, and relations with other words.</dcterms:description>
        <oboInOwl:hasSynonym xml:lang="en">WSD</oboInOwl:hasSynonym>
        <rdfs:label xml:lang="en">Word Sense Disambiguation</rdfs:label>
    </owl:NamedIndividual>
    


    <!-- http://nlpkg.sebis.cit.tum.de/nlp-taxonomy.owl#Dialogue_Systems_&amp;_Conversational_Agents -->

    <owl:NamedIndividual rdf:about="http://nlpkg.sebis.cit.tum.de/nlp-taxonomy.owl#Dialogue_Systems_&amp;_Conversational_Agents">
        <rdf:type rdf:resource="http://nlpkg.sebis.cit.tum.de/nlp-fos-hierarchy.owl#OtherScientificField"/>
        <rdf:type rdf:resource="http://nlpkg.sebis.cit.tum.de/nlp-taxonomy.owl#FieldOfStudy"/>
        <nlp-taxonomy:subFieldOf rdf:resource="http://nlpkg.sebis.cit.tum.de/nlp-taxonomy.owl#Natural_Language_Interfaces"/>
        <nlp-taxonomy:superFieldOf rdf:resource="http://nlpkg.sebis.cit.tum.de/nlp-fos-hierarchy.owl#Chatbots"/>
        <nlp-taxonomy:superFieldOf rdf:resource="http://nlpkg.sebis.cit.tum.de/nlp-fos-hierarchy.owl#Conversational_Question_Answering"/>
        <nlp-taxonomy:superFieldOf rdf:resource="http://nlpkg.sebis.cit.tum.de/nlp-fos-hierarchy.owl#Dialogue_Management"/>
        <nlp-taxonomy:superFieldOf rdf:resource="http://nlpkg.sebis.cit.tum.de/nlp-fos-hierarchy.owl#Dialogue_Understanding"/>
        <nlp-taxonomy:superFieldOf rdf:resource="http://nlpkg.sebis.cit.tum.de/nlp-taxonomy.owl#Dialogue_Response_Generation"/>
        <relevantInformation>https://aclanthology.org/sigs/sigdial/</relevantInformation>
        <relevantInformation>https://web.stanford.edu/~jurafsky/slp3/15.pdf</relevantInformation>
        <survey>https://aclanthology.org/2020.acl-main.183</survey>
        <survey>https://aclanthology.org/2020.coling-main.42</survey>
        <survey>https://aclanthology.org/2023.nlp4convai-1.12</survey>
        <survey>https://aclanthology.org/P18-5002</survey>
        <survey>https://arxiv.org/abs/1306.4134</survey>
        <survey>https://arxiv.org/abs/1512.05742</survey>
        <survey>https://arxiv.org/abs/1611.06216</survey>
        <survey>https://arxiv.org/abs/1709.04409</survey>
        <survey>https://arxiv.org/abs/1711.01731</survey>
        <survey>https://arxiv.org/abs/1803.08419</survey>
        <survey>https://arxiv.org/abs/1905.04071</survey>
        <survey>https://arxiv.org/abs/1905.05709</survey>
        <survey>https://arxiv.org/abs/1906.00500</survey>
        <survey>https://arxiv.org/abs/1907.12878</survey>
        <survey>https://arxiv.org/abs/2003.07490</survey>
        <survey>https://arxiv.org/abs/2004.13818</survey>
        <survey>https://arxiv.org/abs/2101.09459</survey>
        <survey>https://arxiv.org/abs/2104.10810</survey>
        <survey>https://arxiv.org/abs/2105.04387</survey>
        <survey>https://arxiv.org/abs/2106.10901</survey>
        <survey>https://arxiv.org/abs/2108.01369</survey>
        <survey>https://arxiv.org/abs/2111.01414</survey>
        <survey>https://arxiv.org/abs/2112.11176</survey>
        <survey>https://arxiv.org/abs/2202.03164</survey>
        <survey>https://arxiv.org/abs/2203.16891</survey>
        <survey>https://arxiv.org/abs/2205.00965</survey>
        <survey>https://arxiv.org/abs/2206.05017</survey>
        <survey>https://arxiv.org/abs/2207.13211</survey>
        <survey>https://arxiv.org/abs/2212.09252</survey>
        <survey>https://arxiv.org/abs/2302.07926</survey>
        <survey>https://arxiv.org/abs/2305.02750</survey>
        <survey>https://arxiv.org/abs/2305.16324</survey>
        <survey>https://arxiv.org/abs/2308.06095</survey>
        <nlp-taxonomy:level rdf:datatype="http://www.w3.org/2001/XMLSchema#integer">2</nlp-taxonomy:level>
        <dcterms:description xml:lang="en">Dialogue Systems &amp; Conversational Agents is a subfield of Natural Language Interfaces that deals with the development of computer systems that can interact with humans in natural language. It involves the development of algorithms and models that can understand and generate natural language responses based on contextual cues, user preferences, and conversational goals.</dcterms:description>
        <oboInOwl:hasSynonym xml:lang="en">Conversational AI</oboInOwl:hasSynonym>
        <oboInOwl:hasSynonym xml:lang="en">Dialog Systems &amp; Conversational Agents</oboInOwl:hasSynonym>
        <rdfs:label xml:lang="en">Dialogue Systems &amp; Conversational Agents</rdfs:label>
    </owl:NamedIndividual>
    


    <!-- http://nlpkg.sebis.cit.tum.de/nlp-taxonomy.owl#Discourse_&amp;_Pragmatics -->

    <owl:NamedIndividual rdf:about="http://nlpkg.sebis.cit.tum.de/nlp-taxonomy.owl#Discourse_&amp;_Pragmatics">
        <rdf:type rdf:resource="http://nlpkg.sebis.cit.tum.de/nlp-fos-hierarchy.owl#OtherScientificField"/>
        <rdf:type rdf:resource="http://nlpkg.sebis.cit.tum.de/nlp-taxonomy.owl#FieldOfStudy"/>
        <nlp-taxonomy:subFieldOf rdf:resource="http://nlpkg.sebis.cit.tum.de/nlp-taxonomy.owl#Semantic_Text_Processing"/>
        <nlp-taxonomy:superFieldOf rdf:resource="http://nlpkg.sebis.cit.tum.de/nlp-fos-hierarchy.owl#Discourse_Analysis"/>
        <nlp-taxonomy:superFieldOf rdf:resource="http://nlpkg.sebis.cit.tum.de/nlp-fos-hierarchy.owl#Discourse_Deixis_Resolution"/>
        <nlp-taxonomy:superFieldOf rdf:resource="http://nlpkg.sebis.cit.tum.de/nlp-fos-hierarchy.owl#Discourse_Parsing"/>
        <nlp-taxonomy:superFieldOf rdf:resource="http://nlpkg.sebis.cit.tum.de/nlp-fos-hierarchy.owl#Discourse_Segmentation"/>
        <nlp-taxonomy:superFieldOf rdf:resource="http://nlpkg.sebis.cit.tum.de/nlp-fos-hierarchy.owl#Pragmatic_Modeling"/>
        <relevantInformation>https://aclanthology.org/sigs/sigdial/</relevantInformation>
        <relevantInformation>https://web.stanford.edu/~jurafsky/slp3/27.pdf</relevantInformation>
        <nlp-taxonomy:level rdf:datatype="http://www.w3.org/2001/XMLSchema#integer">2</nlp-taxonomy:level>
        <dcterms:description xml:lang="en">Discourse &amp; Pragmatics is a subfield of Semantic Text Processing that deals with the analysis and understanding of language use in context, beyond the surface-level meaning of individual words or sentences. Discourse Analysis focuses on the organization and structure of text and conversation, and how they convey coherence, cohesion, and discourse relations, such as topic shifts, references, and implicatures. Pragmatics focuses on the study of language use in social and communicative situations, and how speakers and listeners use context, knowledge, and inference to convey meaning and achieve their communicative goals.</dcterms:description>
        <rdfs:label xml:lang="en">Discourse &amp; Pragmatics</rdfs:label>
    </owl:NamedIndividual>
    


    <!-- http://nlpkg.sebis.cit.tum.de/nlp-taxonomy.owl#Explainability_&amp;_Interpretability_In_NLP -->

    <owl:NamedIndividual rdf:about="http://nlpkg.sebis.cit.tum.de/nlp-taxonomy.owl#Explainability_&amp;_Interpretability_In_NLP">
        <rdf:type rdf:resource="http://nlpkg.sebis.cit.tum.de/nlp-fos-hierarchy.owl#OtherScientificField"/>
        <rdf:type rdf:resource="http://nlpkg.sebis.cit.tum.de/nlp-taxonomy.owl#FieldOfStudy"/>
        <usedFor rdf:resource="http://nlpkg.sebis.cit.tum.de/nlp-fos-hierarchy.owl#Justification_Production"/>
        <uses rdf:resource="http://nlpkg.sebis.cit.tum.de/nlp-fos-hierarchy.owl#Probing"/>
        <nlp-taxonomy:subFieldOf rdf:resource="http://nlpkg.sebis.cit.tum.de/nlp-taxonomy.owl#Responsible_&amp;_Trustworthy_NLP"/>
        <relevantInformation>https://aclanthology.org/venues/blackboxnlp/</relevantInformation>
        <relevantInformation>https://christophm.github.io/interpretable-ml-book/</relevantInformation>
        <relevantInformation>https://edwinwenink.github.io/ai-ethics-tool-landscape/values/explainability/</relevantInformation>
        <relevantInformation>https://github.com/JShollaj/awesome-llm-interpretability</relevantInformation>
        <relevantInformation>https://xainlp2020.github.io/xainlp/clickabletree</relevantInformation>
        <survey>https://aclanthology.org/2020.aacl-main.46</survey>
        <survey>https://aclanthology.org/2020.acl-main.491</survey>
        <survey>https://aclanthology.org/2020.coling-main.474</survey>
        <survey>https://aclanthology.org/2021.naacl-main.399</survey>
        <survey>https://aclanthology.org/2021.tacl-1.90</survey>
        <survey>https://aclanthology.org/2022.coling-1.406</survey>
        <survey>https://aclanthology.org/2022.tacl-1.74</survey>
        <survey>https://aclanthology.org/Q19-1004</survey>
        <survey>https://aclanthology.org/W19-8403</survey>
        <survey>https://arxiv.org/abs/2010.00389</survey>
        <survey>https://arxiv.org/abs/2010.10563</survey>
        <survey>https://arxiv.org/abs/2102.12060</survey>
        <survey>https://arxiv.org/abs/2108.04840</survey>
        <survey>https://arxiv.org/abs/2108.10274</survey>
        <survey>https://arxiv.org/abs/2110.10470</survey>
        <survey>https://arxiv.org/abs/2203.17081</survey>
        <survey>https://arxiv.org/abs/2207.13243</survey>
        <survey>https://arxiv.org/abs/2209.11326</survey>
        <survey>https://arxiv.org/abs/2212.07126</survey>
        <survey>https://arxiv.org/abs/2301.08912</survey>
        <survey>https://arxiv.org/abs/2302.09304</survey>
        <survey>https://arxiv.org/abs/2309.01029</survey>
        <survey>https://arxiv.org/abs/2310.11884</survey>
        <nlp-taxonomy:level rdf:datatype="http://www.w3.org/2001/XMLSchema#integer">2</nlp-taxonomy:level>
        <dcterms:description xml:lang="en">Explainability, Interpretability &amp; Transparency (XAI) in NLP is a subfield of Responsible NLP that deals with developing algorithms and models that can provide transparent and interpretable predictions, and explain the reasoning and decision-making processes behind them. It involves developing techniques that can generate human-readable explanations, highlight important features and patterns, and enable users to interact and refine the models.</dcterms:description>
        <oboInOwl:hasSynonym xml:lang="en">EXNLP</oboInOwl:hasSynonym>
        <oboInOwl:hasSynonym xml:lang="en">Explainability &amp; Interpretability in NLP</oboInOwl:hasSynonym>
        <oboInOwl:hasSynonym xml:lang="en">Explainable Natural Language Processing</oboInOwl:hasSynonym>
        <oboInOwl:hasSynonym xml:lang="en">XAI</oboInOwl:hasSynonym>
        <rdfs:label xml:lang="en">Explainability, Interpretability &amp; Transparency in NLP</rdfs:label>
    </owl:NamedIndividual>
    


    <!-- http://nlpkg.sebis.cit.tum.de/nlp-taxonomy.owl#Fact_&amp;_Claim_Verification -->

    <owl:NamedIndividual rdf:about="http://nlpkg.sebis.cit.tum.de/nlp-taxonomy.owl#Fact_&amp;_Claim_Verification">
        <rdf:type rdf:resource="http://nlpkg.sebis.cit.tum.de/nlp-fos-hierarchy.owl#Task"/>
        <rdf:type rdf:resource="http://nlpkg.sebis.cit.tum.de/nlp-taxonomy.owl#FieldOfStudy"/>
        <usedFor rdf:resource="http://nlpkg.sebis.cit.tum.de/nlp-fos-hierarchy.owl#Hallucination_Detection"/>
        <usedFor rdf:resource="http://nlpkg.sebis.cit.tum.de/nlp-fos-hierarchy.owl#Misinformation_Detection"/>
        <nlp-taxonomy:subFieldOf rdf:resource="http://nlpkg.sebis.cit.tum.de/nlp-taxonomy.owl#Reasoning"/>
        <nlp-taxonomy:superFieldOf rdf:resource="http://nlpkg.sebis.cit.tum.de/nlp-fos-hierarchy.owl#Claim_Detection"/>
        <nlp-taxonomy:superFieldOf rdf:resource="http://nlpkg.sebis.cit.tum.de/nlp-fos-hierarchy.owl#Factual_Verification"/>
        <survey>https://aclanthology.org/2020.coling-main.474</survey>
        <survey>https://aclanthology.org/2022.tacl-1.11</survey>
        <survey>https://aclanthology.org/2023.findings-acl.387</survey>
        <survey>https://arxiv.org/abs/2108.10274</survey>
        <survey>https://arxiv.org/abs/2109.11427</survey>
        <survey>https://arxiv.org/abs/2305.13507</survey>
        <survey>https://arxiv.org/abs/2310.13549</survey>
        <nlp-taxonomy:level rdf:datatype="http://www.w3.org/2001/XMLSchema#integer">2</nlp-taxonomy:level>
        <dcterms:description xml:lang="en">Automated Fact-Checking is a subfield of Reasoning that deals with the task of automatically verifying the veracity of facts or claims in natural language text, by comparing them against a knowledge base or external sources of information. It involves developing algorithms and models that can analyze the text and identify the relevant facts and evidence, and reason about the likelihood of the facts or claims being true or false.</dcterms:description>
        <oboInOwl:hasSynonym xml:lang="en">AFC</oboInOwl:hasSynonym>
        <oboInOwl:hasSynonym xml:lang="en">Automated Fact Checking</oboInOwl:hasSynonym>
        <oboInOwl:hasSynonym xml:lang="en">Fact Checking</oboInOwl:hasSynonym>
        <oboInOwl:hasSynonym xml:lang="en">Fact-Checking</oboInOwl:hasSynonym>
        <rdfs:label xml:lang="en">Automated Fact-Checking</rdfs:label>
    </owl:NamedIndividual>
    


    <!-- http://nlpkg.sebis.cit.tum.de/nlp-taxonomy.owl#Green_&amp;_Sustainable_NLP -->

    <owl:NamedIndividual rdf:about="http://nlpkg.sebis.cit.tum.de/nlp-taxonomy.owl#Green_&amp;_Sustainable_NLP">
        <rdf:type rdf:resource="http://nlpkg.sebis.cit.tum.de/nlp-fos-hierarchy.owl#OtherScientificField"/>
        <rdf:type rdf:resource="http://nlpkg.sebis.cit.tum.de/nlp-taxonomy.owl#FieldOfStudy"/>
        <nlp-taxonomy:subFieldOf rdf:resource="http://nlpkg.sebis.cit.tum.de/nlp-taxonomy.owl#Responsible_&amp;_Trustworthy_NLP"/>
        <nlp-taxonomy:superFieldOf rdf:resource="http://nlpkg.sebis.cit.tum.de/nlp-fos-hierarchy.owl#Active_Learning"/>
        <nlp-taxonomy:superFieldOf rdf:resource="http://nlpkg.sebis.cit.tum.de/nlp-fos-hierarchy.owl#Curriculum_Learning"/>
        <nlp-taxonomy:superFieldOf rdf:resource="http://nlpkg.sebis.cit.tum.de/nlp-fos-hierarchy.owl#Efficient_Transformers"/>
        <nlp-taxonomy:superFieldOf rdf:resource="http://nlpkg.sebis.cit.tum.de/nlp-fos-hierarchy.owl#Few-shot_Learning"/>
        <nlp-taxonomy:superFieldOf rdf:resource="http://nlpkg.sebis.cit.tum.de/nlp-fos-hierarchy.owl#Language_Model_Quantization"/>
        <nlp-taxonomy:superFieldOf rdf:resource="http://nlpkg.sebis.cit.tum.de/nlp-fos-hierarchy.owl#Multi-task_Learning"/>
        <nlp-taxonomy:superFieldOf rdf:resource="http://nlpkg.sebis.cit.tum.de/nlp-fos-hierarchy.owl#Parameter-Efficient_Fine-Tuning"/>
        <nlp-taxonomy:superFieldOf rdf:resource="http://nlpkg.sebis.cit.tum.de/nlp-fos-hierarchy.owl#Zero-shot_Learning"/>
        <nlp-taxonomy:superFieldOf rdf:resource="http://nlpkg.sebis.cit.tum.de/nlp-fos-hierarchy.owl#Prompting,_Prompt_Learning_&amp;_Prompt_Engineering"/>
        <survey>https://aclanthology.org/P19-1355</survey>
        <survey>https://arxiv.org/abs/2111.05193</survey>
        <survey>https://arxiv.org/abs/2202.07105</survey>
        <survey>https://arxiv.org/abs/2209.00099</survey>
        <survey>https://arxiv.org/abs/2302.01107</survey>
        <survey>https://arxiv.org/abs/2302.14017</survey>
        <survey>https://arxiv.org/abs/2304.03589</survey>
        <survey>https://arxiv.org/abs/2307.07982</survey>
        <survey>https://arxiv.org/abs/2308.07633</survey>
        <nlp-taxonomy:level rdf:datatype="http://www.w3.org/2001/XMLSchema#integer">2</nlp-taxonomy:level>
        <dcterms:description xml:lang="en">Green, Sustainable &amp; Efficient Methods in NLP is a subfield of Responsible &amp; Trustworthy NLP that is focused on efficient and sustainable approaches for text processing with minimal environmental impact. Efficient NLP methods can be considered under the aspects of both data efficiency and computational efficiency. They aim to lower the amount of data required, reduce computational complexity, improve speed, and increase accuracy in NLP tasks. Efficient NLP models can, therefore, recycle and reuse resources, optimize energy consumption, and reduce the carbon footprint.</dcterms:description>
        <dcterms:description xml:lang="en">Inference Optimization</dcterms:description>
        <oboInOwl:hasSynonym xml:lang="en">Green &amp; Sustainable NLP</oboInOwl:hasSynonym>
        <rdfs:label xml:lang="en">Green, Sustainable &amp; Efficient Methods in NLP</rdfs:label>
    </owl:NamedIndividual>
    


    <!-- http://nlpkg.sebis.cit.tum.de/nlp-taxonomy.owl#Information_Extraction_&amp;_Text_Mining -->

    <owl:NamedIndividual rdf:about="http://nlpkg.sebis.cit.tum.de/nlp-taxonomy.owl#Information_Extraction_&amp;_Text_Mining">
        <rdf:type rdf:resource="http://nlpkg.sebis.cit.tum.de/nlp-fos-hierarchy.owl#Task"/>
        <rdf:type rdf:resource="http://nlpkg.sebis.cit.tum.de/nlp-taxonomy.owl#FieldOfStudy"/>
        <nlp-taxonomy:subFieldOf rdf:resource="http://nlpkg.sebis.cit.tum.de/nlp-taxonomy.owl#Natural_Language_Processing"/>
        <nlp-taxonomy:superFieldOf rdf:resource="http://nlpkg.sebis.cit.tum.de/nlp-fos-hierarchy.owl#Text_Regression"/>
        <nlp-taxonomy:superFieldOf rdf:resource="http://nlpkg.sebis.cit.tum.de/nlp-taxonomy.owl#Coreference_Resolution"/>
        <nlp-taxonomy:superFieldOf rdf:resource="http://nlpkg.sebis.cit.tum.de/nlp-taxonomy.owl#Event_Extraction"/>
        <nlp-taxonomy:superFieldOf rdf:resource="http://nlpkg.sebis.cit.tum.de/nlp-taxonomy.owl#Named_Entity_Recognition"/>
        <nlp-taxonomy:superFieldOf rdf:resource="http://nlpkg.sebis.cit.tum.de/nlp-taxonomy.owl#Open_Information_Extraction"/>
        <nlp-taxonomy:superFieldOf rdf:resource="http://nlpkg.sebis.cit.tum.de/nlp-taxonomy.owl#Relation_Extraction"/>
        <nlp-taxonomy:superFieldOf rdf:resource="http://nlpkg.sebis.cit.tum.de/nlp-taxonomy.owl#Summarization"/>
        <nlp-taxonomy:superFieldOf rdf:resource="http://nlpkg.sebis.cit.tum.de/nlp-taxonomy.owl#Term_Extraction"/>
        <nlp-taxonomy:superFieldOf rdf:resource="http://nlpkg.sebis.cit.tum.de/nlp-taxonomy.owl#Text_Classification"/>
        <nlp-taxonomy:superFieldOf rdf:resource="http://nlpkg.sebis.cit.tum.de/nlp-taxonomy.owl#Text_Clustering"/>
        <nlp-taxonomy:superFieldOf rdf:resource="http://nlpkg.sebis.cit.tum.de/nlp-taxonomy.owl#Topic_Modeling"/>
        <survey>https://aclanthology.org/2020.coling-main.133</survey>
        <survey>https://aclanthology.org/2023.ranlp-1.12</survey>
        <survey>https://arxiv.org/abs/1401.2937</survey>
        <survey>https://arxiv.org/abs/1707.02919</survey>
        <survey>https://arxiv.org/abs/2202.08063</survey>
        <survey>https://arxiv.org/abs/2309.13249</survey>
        <survey>https://arxiv.org/abs/2312.17617</survey>
        <nlp-taxonomy:level rdf:datatype="http://www.w3.org/2001/XMLSchema#integer">1</nlp-taxonomy:level>
        <dcterms:description xml:lang="en">Information Extraction &amp; Text Mining is a subfield of Natural Language Processing (NLP) that focuses on automatically extracting structured information and knowledge from unstructured textual data.</dcterms:description>
        <oboInOwl:hasSynonym xml:lang="en">IE</oboInOwl:hasSynonym>
        <oboInOwl:hasSynonym xml:lang="en">Knowledge Extraction</oboInOwl:hasSynonym>
        <rdfs:label xml:lang="en">Information Extraction &amp; Text Mining</rdfs:label>
    </owl:NamedIndividual>
    


    <!-- http://nlpkg.sebis.cit.tum.de/nlp-taxonomy.owl#Linguistics_&amp;_Cognitive_NLP -->

    <owl:NamedIndividual rdf:about="http://nlpkg.sebis.cit.tum.de/nlp-taxonomy.owl#Linguistics_&amp;_Cognitive_NLP">
        <rdf:type rdf:resource="http://nlpkg.sebis.cit.tum.de/nlp-fos-hierarchy.owl#OtherScientificField"/>
        <rdf:type rdf:resource="http://nlpkg.sebis.cit.tum.de/nlp-taxonomy.owl#FieldOfStudy"/>
        <nlp-taxonomy:subFieldOf rdf:resource="http://nlpkg.sebis.cit.tum.de/nlp-taxonomy.owl#Natural_Language_Processing"/>
        <nlp-taxonomy:superFieldOf rdf:resource="http://nlpkg.sebis.cit.tum.de/nlp-taxonomy.owl#Cognitive_Modeling"/>
        <nlp-taxonomy:superFieldOf rdf:resource="http://nlpkg.sebis.cit.tum.de/nlp-taxonomy.owl#Linguistic_Theories"/>
        <nlp-taxonomy:superFieldOf rdf:resource="http://nlpkg.sebis.cit.tum.de/nlp-taxonomy.owl#Psycholinguistics"/>
        <nlp-taxonomy:level rdf:datatype="http://www.w3.org/2001/XMLSchema#integer">1</nlp-taxonomy:level>
        <dcterms:description xml:lang="en">Linguistics &amp; Cognitive Natural Language Processing is a subfield of Natural Language Processing (NLP) that focuses on the study of natural language from a linguistic and cognitive perspective. It studies natural language based on the assumptions that our linguistic abilities are firmly rooted in our cognitive abilities, that meaning is essentially conceptualization, and that grammar is shaped by usage.</dcterms:description>
        <rdfs:label xml:lang="en">Linguistics &amp; Cognitive NLP</rdfs:label>
    </owl:NamedIndividual>
    


    <!-- http://nlpkg.sebis.cit.tum.de/nlp-taxonomy.owl#Responsible_&amp;_Trustworthy_NLP -->

    <owl:NamedIndividual rdf:about="http://nlpkg.sebis.cit.tum.de/nlp-taxonomy.owl#Responsible_&amp;_Trustworthy_NLP">
        <rdf:type rdf:resource="http://nlpkg.sebis.cit.tum.de/nlp-fos-hierarchy.owl#OtherScientificField"/>
        <rdf:type rdf:resource="http://nlpkg.sebis.cit.tum.de/nlp-taxonomy.owl#FieldOfStudy"/>
        <nlp-taxonomy:subFieldOf rdf:resource="http://nlpkg.sebis.cit.tum.de/nlp-taxonomy.owl#Natural_Language_Processing"/>
        <nlp-taxonomy:superFieldOf rdf:resource="http://nlpkg.sebis.cit.tum.de/nlp-taxonomy.owl#Ethical_NLP"/>
        <nlp-taxonomy:superFieldOf rdf:resource="http://nlpkg.sebis.cit.tum.de/nlp-taxonomy.owl#Low-Resource_NLP"/>
        <nlp-taxonomy:superFieldOf rdf:resource="http://nlpkg.sebis.cit.tum.de/nlp-taxonomy.owl#Robustness_In_NLP"/>
        <nlp-taxonomy:superFieldOf rdf:resource="http://nlpkg.sebis.cit.tum.de/nlp-taxonomy.owl#Explainability_&amp;_Interpretability_In_NLP"/>
        <nlp-taxonomy:superFieldOf rdf:resource="http://nlpkg.sebis.cit.tum.de/nlp-taxonomy.owl#Green_&amp;_Sustainable_NLP"/>
        <survey>https://arxiv.org/abs/2305.03123</survey>
        <survey>https://arxiv.org/abs/2305.11391</survey>
        <survey>https://arxiv.org/abs/2307.16680</survey>
        <survey>https://arxiv.org/abs/2308.13534</survey>
        <nlp-taxonomy:level rdf:datatype="http://www.w3.org/2001/XMLSchema#integer">1</nlp-taxonomy:level>
        <dcterms:description xml:lang="en">Responsible &amp; Trustworthy NLP is a subfield of Natural Language Processing (NLP) that is concerned with implementing methods that focus on fairness, transparency, trustworthiness, explainability, accountability, and ethical aspects at its core. It involves considering the societal impact of NLP applications and ensuring that they do not perpetuate or amplify biases or discrimination. Additionally, responsible NLP also involves developing methods to ensure the privacy and security of user data, and to mitigate the risks of unintended consequences or misuse of NLP systems.</dcterms:description>
        <rdfs:label xml:lang="en">Responsible &amp; Trustworthy NLP</rdfs:label>
    </owl:NamedIndividual>
    


    <!-- http://nlpkg.sebis.cit.tum.de/nlp-taxonomy.owl#Speech_&amp;_Audio_In_NLP -->

    <owl:NamedIndividual rdf:about="http://nlpkg.sebis.cit.tum.de/nlp-taxonomy.owl#Speech_&amp;_Audio_In_NLP">
        <rdf:type rdf:resource="http://nlpkg.sebis.cit.tum.de/nlp-fos-hierarchy.owl#OtherScientificField"/>
        <rdf:type rdf:resource="http://nlpkg.sebis.cit.tum.de/nlp-taxonomy.owl#FieldOfStudy"/>
        <usedFor rdf:resource="http://nlpkg.sebis.cit.tum.de/nlp-fos-hierarchy.owl#Language_Grounding"/>
        <nlp-taxonomy:subFieldOf rdf:resource="http://nlpkg.sebis.cit.tum.de/nlp-taxonomy.owl#Multimodality"/>
        <nlp-taxonomy:superFieldOf rdf:resource="http://nlpkg.sebis.cit.tum.de/nlp-fos-hierarchy.owl#Music_in_NLP"/>
        <nlp-taxonomy:superFieldOf rdf:resource="http://nlpkg.sebis.cit.tum.de/nlp-fos-hierarchy.owl#Speaker_Recognition"/>
        <nlp-taxonomy:superFieldOf rdf:resource="http://nlpkg.sebis.cit.tum.de/nlp-fos-hierarchy.owl#Speaker_Verification"/>
        <nlp-taxonomy:superFieldOf rdf:resource="http://nlpkg.sebis.cit.tum.de/nlp-fos-hierarchy.owl#Speech_Synthesis"/>
        <nlp-taxonomy:superFieldOf rdf:resource="http://nlpkg.sebis.cit.tum.de/nlp-fos-hierarchy.owl#Spoken_Language_Understanding"/>
        <nlp-taxonomy:superFieldOf rdf:resource="http://nlpkg.sebis.cit.tum.de/nlp-fos-hierarchy.owl#Speech_&amp;_Audio-specific_Language_Models"/>
        <nlp-taxonomy:superFieldOf rdf:resource="http://nlpkg.sebis.cit.tum.de/nlp-taxonomy.owl#Speech_Recognition"/>
        <survey>https://arxiv.org/abs/2205.10643</survey>
        <nlp-taxonomy:level rdf:datatype="http://www.w3.org/2001/XMLSchema#integer">2</nlp-taxonomy:level>
        <dcterms:description xml:lang="en">Speech &amp; Audio in NLP is a subfield of Multimodality that deals with the processing of spoken language and audio data in conjunction with textual data. It involves developing algorithms and models that can recognize and transcribe speech and audio, understand and interpret their meaning, and generate natural language responses.</dcterms:description>
        <rdfs:label xml:lang="en">Speech &amp; Audio in NLP</rdfs:label>
    </owl:NamedIndividual>
</rdf:RDF>



<!-- Generated by the OWL API (version 4.5.9.2019-02-01T07:24:44Z) https://github.com/owlcs/owlapi -->

